<rdf:RDF
xmlns:rdf ="http://www.w3.org/1999/02/22-rdf-syntax-ns#"
xmlns:rdfs="http://www.w3.org/2000/01/rdf-schema#"
xmlns:owl="http://www.w3.org/2002/07/owl#"
xmlns:sumo="http://127.0.0.1:8000/ontology/SUMO.owl#"
xmlns     ="http://127.0.0.1:8000/ontology/Mid-level-ontology.owl#"
xml:base  ="http://127.0.0.1:8000/ontology/Mid-level-ontology.owl">

<owl:Ontology rdf:about="">
<owl:imports rdf:resource="http://127.0.0.1:8000/ontology/SUMO.owl" />
</owl:Ontology>

<owl:Class rdf:ID= "Icing">
<rdfs:subClassOf rdf:resource ="http://127.0.0.1:8000/ontology/SUMO.owl#WeatherProcess"/>
<rdfs:comment>Icing is the class of WeatherProcesses in which
the ambient temperature drops below the freezing point, and objects in the
affected area become coated with Ice.</rdfs:comment>
</owl:Class>

<owl:Class rdf:ID= "WarmFront">
<rdfs:subClassOf rdf:resource ="http://127.0.0.1:8000/ontology/Mid-level-ontology.owl#WeatherFront"/>
<rdfs:comment>WarmFront is the class of transitional
weather processes occurring between a warm air mass that is advancing
upon a cool air mass.</rdfs:comment>
</owl:Class>

<owl:Class rdf:ID= "WeatherSeason">
<rdfs:subClassOf rdf:resource ="http://127.0.0.1:8000/ontology/SUMO.owl#WeatherProcess"/>
<rdfs:comment>WeatherSeason is the class of seasonal
processes that are characterized by various weather patterns.
WeatherSeasons may recur on a regular annual basis, on a different
pattern, or irregularly.</rdfs:comment>
</owl:Class>

<owl:Class rdf:ID= "WeatherSystem">
<rdfs:subClassOf rdf:resource ="http://127.0.0.1:8000/ontology/SUMO.owl#WeatherProcess"/>
<rdfs:comment>WeatherSystem is the class of
large-scale atmospheric processes that influence weather in a region
for 2-5 days.</rdfs:comment>
</owl:Class>

<owl:Class rdf:ID= "Aborting">
<rdfs:subClassOf rdf:resource 
="http://127.0.0.1:8000/ontology/SUMO.owl#Removing"/>
<rdfs:comment>Removing a human fetus from a Pregnant woman
in such a way that the fetus cannot survive.</rdfs:comment>
</owl:Class>

<owl:Class rdf:ID= "AcademicDegree">
<rdfs:subClassOf rdf:resource 
="http://127.0.0.1:8000/ontology/SUMO.owl#Certificate"/>
<rdfs:comment>A Certificate that demonstrates that the holder
of the Certificate has successfully completed an 
EducationalProgram.</rdfs:comment>
</owl:Class>

<owl:Class rdf:ID= "Accelerating">
<rdfs:subClassOf rdf:resource 
="http://127.0.0.1:8000/ontology/SUMO.owl#Translocation"/>
<rdfs:subClassOf rdf:resource 
="http://127.0.0.1:8000/ontology/SUMO.owl#Increasing"/>
<rdfs:comment>Increasing the speed with which someone
or something is moving.</rdfs:comment>
</owl:Class>

<owl:Class rdf:ID= "Accountant">
<rdfs:subClassOf rdf:resource ="#Profession"/>
<rdfs:comment>The Profession of being an Accountant.</rdfs:comment>
</owl:Class>

<owl:Class rdf:ID= "Accrediting">
<rdfs:subClassOf rdf:resource 
="http://127.0.0.1:8000/ontology/SUMO.owl#Declaring"/>
<rdfs:comment>Any process of certifying an 
EducationalOrganization.</rdfs:comment>
</owl:Class>

<owl:Class rdf:ID= "Acre">
<rdfs:subClassOf rdf:resource 
="http://127.0.0.1:8000/ontology/SUMO.owl#AreaMeasure"/>
<rdf:type rdf:resource = 
"http://127.0.0.1:8000/ontology/SUMO.owl#UnitOfMeasure"/>
<rdfs:comment>A UnitOfMeasure equal to 4840 square yards.</rdfs:comment>
</owl:Class>

<owl:Class rdf:ID= "AcuteAngle">
<rdfs:subClassOf rdf:resource 
="http://127.0.0.1:8000/ontology/SUMO.owl#TwoDimensionalAngle"/>
<rdfs:comment>Any TwoDimensionalAngle that has an
angularMeasure that is less than 90 AngularDegrees.</rdfs:comment>
</owl:Class>

<owl:Class rdf:ID= "Address">
<rdfs:subClassOf rdf:resource 
="http://127.0.0.1:8000/ontology/SUMO.owl#RelationalAttribute"/>
<rdfs:comment>A RelationalAttribute that indicates an address
where an Agent can regularly be contacted.</rdfs:comment>
</owl:Class>

<owl:Class rdf:ID= "Advertising">
<rdfs:subClassOf rdf:resource 
="http://127.0.0.1:8000/ontology/SUMO.owl#Disseminating"/>
<rdfs:comment>A Disseminating whose purpose is to
promote the sale of an Object represented in a Text or Icon
(the advertisement).</rdfs:comment>
</owl:Class>

<owl:Class rdf:ID= "Aerating">
<rdfs:subClassOf rdf:resource 
="http://127.0.0.1:8000/ontology/SUMO.owl#Combining"/>
<rdfs:comment>Combining a substance with Air.</rdfs:comment>
</owl:Class>

<owl:Class rdf:ID= "Aerator">
<rdfs:subClassOf rdf:resource ="http://127.0.0.1:8000/ontology/SUMO.owl#Device"/>
<rdfs:comment>A Device whose purpose is to mix Substances with
Air.</rdfs:comment>
</owl:Class>

<owl:Class rdf:ID= "AerobicExerciseDevice">
<rdfs:subClassOf rdf:resource ="#RecreationOrExerciseDevice"/>
<rdfs:comment>An RecreationOrExerciseDevice whose purpose is
to develop the cardiovascular system.</rdfs:comment>
</owl:Class>

<owl:Class rdf:ID= "Afternoon">
<rdfs:subClassOf rdf:resource ="#DayTime"/>
<rdfs:comment>The class of TimeIntervals that begin at noon and
end at Sunset.</rdfs:comment>
</owl:Class>

<owl:Class rdf:ID= "Agency">
<rdfs:subClassOf rdf:resource 
="http://127.0.0.1:8000/ontology/SUMO.owl#CommercialAgent"/>
<rdfs:comment>A CommercialAgent whose customers are all other
CommercialAgents, e.g. staffing agencies, food-service providers, 
etc.</rdfs:comment>
</owl:Class>

<owl:Class rdf:about= "Agent">
</owl:Class>

<owl:Class rdf:ID= "Agriculture">
<rdfs:subClassOf rdf:resource 
="http://127.0.0.1:8000/ontology/SUMO.owl#Maintaining"/>
<rdfs:comment>Agriculture is a class of Processes
in which land, plants, or animals are cultivated in order to produce
food or other organic products.</rdfs:comment>
</owl:Class>

<owl:Class rdf:ID= "AirForce">
<rdfs:subClassOf rdf:resource ="#MilitaryService"/>
<rdfs:comment>AirForce is the subclass of MilitaryService
that comprises military air forces.</rdfs:comment>
</owl:Class>

<owl:Class rdf:ID= "AirStream">
<rdfs:subClassOf rdf:resource ="#FlowRegion"/>
<rdfs:subClassOf rdf:resource ="http://127.0.0.1:8000/ontology/SUMO.owl#Air"/>
<rdfs:comment>AirStream is the class of FlowRegions that
consist of air.</rdfs:comment>
</owl:Class>

<owl:Class rdf:ID= "AirTransportation">
<rdfs:subClassOf rdf:resource 
="http://127.0.0.1:8000/ontology/SUMO.owl#Transportation"/>
<rdfs:comment>Any instance of Transportation where the
instrument is an Aircraft and which is through an 
AtmosphericRegion.</rdfs:comment>
</owl:Class>

<owl:Class rdf:ID= "Aircraft">
<rdfs:subClassOf rdf:resource 
="http://127.0.0.1:8000/ontology/SUMO.owl#Vehicle"/>
<rdfs:comment>Any Vehicle which is capable of
AirTransportation.  Note that this class covers both fixed-wing aircraft
and helicopters.</rdfs:comment>
</owl:Class>

<owl:Class rdf:ID= "AircraftCarrier">
<rdfs:subClassOf rdf:resource ="#MilitaryShip"/>
<rdfs:comment>A MilitaryShip on which MilitaryAircraft can land
and take off.</rdfs:comment>
</owl:Class>

<owl:Class rdf:ID= "Airplane">
<rdfs:subClassOf rdf:resource ="#Aircraft"/>
<rdfs:comment>Airplane is the subclass of Aircraft that
are fixed-wing aircraft which carry their own power sources.  Airplane
includes jet airplanes and propeller planes, but not gliders.</rdfs:comment>
</owl:Class>

<owl:Class rdf:ID= "Airport">
<rdfs:subClassOf rdf:resource ="#TransitTerminal"/>
<rdfs:subClassOf rdf:resource 
="http://127.0.0.1:8000/ontology/SUMO.owl#LandTransitway"/>
<rdfs:comment>Airport is the subclass of TransitTerminals
for Airplanes (fixed-wing Aircraft).</rdfs:comment>
</owl:Class>

<owl:Class rdf:ID= "Airway">
<rdfs:subClassOf rdf:resource 
="http://127.0.0.1:8000/ontology/SUMO.owl#Transitway"/>
<rdfs:comment>The class of Transitways used to transport Air
to a location where it is absent or insufficient.</rdfs:comment>
</owl:Class>

<owl:Class rdf:ID= "Alcohol">
<rdfs:subClassOf rdf:resource ="#OrganicCompound"/>
<rdfs:comment>OrganicCompounds that are produced from hydrocarbons
by distillation.</rdfs:comment>
</owl:Class>

<owl:Class rdf:ID= "AlcoholicBeverage">
<rdfs:subClassOf rdf:resource 
="http://127.0.0.1:8000/ontology/SUMO.owl#Beverage"/>
<rdfs:subClassOf rdf:resource ="#Depressant"/>
<rdfs:comment>Any Beverage that contains Alcohol.</rdfs:comment>
</owl:Class>

<owl:Class rdf:ID= "Alkaloid">
<rdfs:subClassOf rdf:resource ="#ChemicalBase"/>
<rdfs:subClassOf rdf:resource 
="http://127.0.0.1:8000/ontology/SUMO.owl#PlantSubstance"/>
<rdfs:subClassOf rdf:resource 
="http://127.0.0.1:8000/ontology/SUMO.owl#BiologicallyActiveSubstance"/>
<rdfs:comment>A ChemicalBase found in Plants that has
physiological and psychological effects.</rdfs:comment>
</owl:Class>

<owl:Class rdf:ID= "AlphabeticCharacter">
<rdfs:subClassOf rdf:resource 
="http://127.0.0.1:8000/ontology/SUMO.owl#Character"/>
<rdfs:comment>Any Character that is comprised of a single
alphabetical character, e.g. A, B, C, D, ...</rdfs:comment>
</owl:Class>

<owl:Class rdf:ID= "Aluminum">
<rdfs:subClassOf rdf:resource 
="http://127.0.0.1:8000/ontology/SUMO.owl#ElementalSubstance"/>
<atomicNumber>13</atomicNumber>
<rdfs:comment>Silvery-white lustrous metallic element of group
3 of the periodic table.  Highly reactive but protected by a thin
transparent layer of the oxide which quickly forms in air.  There are many
alloys of aluminum, as well as a good number of industrial uses.  Makes up
8.1 percent of the Earth's crust, by weight.  Isolated in 1825 by H.C.
Oersted.</rdfs:comment>
</owl:Class>

<owl:Class rdf:ID= "Alveolus">
<rdfs:subClassOf rdf:resource 
="http://127.0.0.1:8000/ontology/SUMO.owl#BodyVessel"/>
<rdfs:subClassOf rdf:resource 
="http://127.0.0.1:8000/ontology/SUMO.owl#AnimalAnatomicalStructure"/>
<rdfs:comment>Tiny sacs in the Lung which absorb Oxygen
which is delivered to them by the BronchialDucts.</rdfs:comment>
</owl:Class>

<owl:Class rdf:ID= "Ambassador">
<rdfs:subClassOf rdf:resource ="#DiplomaticAgent"/>
<rdfs:comment>Ambassador is the class of DiplomaticAgents
that are the most highly-ranked foreign service representatives from the
government of one country to another.</rdfs:comment>
</owl:Class>

<owl:Class rdf:ID= "Ambulance">
<rdfs:subClassOf rdf:resource ="#EmergencyRoadVehicle"/>
<rdfs:comment>Ambulance is the subclass of
EmergencyRoadVehicles that represents ambulances.</rdfs:comment>
</owl:Class>

<owl:Class rdf:ID= "Ambush">
<rdfs:subClassOf rdf:resource 
="http://127.0.0.1:8000/ontology/SUMO.owl#Maneuver"/>
<rdfs:comment>Any Maneuver in a ViolentContest where one contestParticipant
attempts to conceal himself from another contestParticipant so that he can 
Attack the
other contestParticipant.</rdfs:comment>
</owl:Class>

<owl:Class rdf:ID= "AmericanCity">
<rdfs:subClassOf rdf:resource ="http://127.0.0.1:8000/ontology/SUMO.owl#City"/>
<rdfs:comment>The class of cities that are in the
UnitedStates.</rdfs:comment>
</owl:Class>

<owl:Class rdf:ID= "AmericanState">
<rdfs:subClassOf rdf:resource 
="http://127.0.0.1:8000/ontology/SUMO.owl#StateOrProvince"/>
<rdfs:comment>The class of states that make up the
UnitedStates.</rdfs:comment>
</owl:Class>

<owl:Class rdf:ID= "AminoAcid">
<rdfs:subClassOf rdf:resource ="#ChemicalAcid"/>
<rdfs:subClassOf rdf:resource ="#OrganicCompound"/>
<rdfs:comment>Organic acids that are the building blocks of
Proteins.</rdfs:comment>
</owl:Class>

<owl:Class rdf:ID= "Ampere">
<rdfs:subClassOf rdf:resource 
="http://127.0.0.1:8000/ontology/SUMO.owl#FunctionQuantity"/>
<rdf:type rdf:resource = 
"http://127.0.0.1:8000/ontology/SUMO.owl#SystemeInternationalUnit"/>
<rdfs:comment>SI electric current measure.  Symbol: A. It is
one of the base units in SI. It is defined as follows: the Ampere is
that constant current which, if maintained in two straight parallel
conductors of infinite length, of negligible circular cross-section, and
placed 1 Meter apart in a vacuum, would produce between these conductors
a force equal to 2*10^(-7) Newton per Meter of length.</rdfs:comment>
</owl:Class>

<owl:Class rdf:ID= "Amu">
<rdfs:subClassOf rdf:resource 
="http://127.0.0.1:8000/ontology/SUMO.owl#MassMeasure"/>
<rdf:type rdf:resource = 
"http://127.0.0.1:8000/ontology/SUMO.owl#UnitOfMeasure"/>
<rdfs:comment>Atomic mass unit.  Symbol: u. It is the mass of
the twelfth part of an atom of the Carbon 12 isotope.</rdfs:comment>
</owl:Class>

<owl:Class rdf:ID= "AnaerobicExerciseDevice">
<rdfs:subClassOf rdf:resource ="#RecreationOrExerciseDevice"/>
<sumo:disjoint rdf:resource = "#AerobicExerciseDevice" />
<rdfs:comment>An RecreationOrExerciseDevice whose purpose
is to develop Muscles without also developing the cardiovascular 
system.</rdfs:comment>
</owl:Class>

<owl:Class rdf:ID= "Anchor">
<rdfs:subClassOf rdf:resource 
="http://127.0.0.1:8000/ontology/SUMO.owl#AttachingDevice"/>
<rdfs:comment>An AttachingDevice which is large hook or set of hooks
that are used to secure a Ship on the open water.</rdfs:comment>
</owl:Class>

<owl:Class rdf:ID= "Angstrom">
<rdfs:subClassOf rdf:resource 
="http://127.0.0.1:8000/ontology/SUMO.owl#LengthMeasure"/>
<rdf:type rdf:resource = 
"http://127.0.0.1:8000/ontology/SUMO.owl#UnitOfMeasure"/>
<rdfs:comment>The Angstrom is a LengthMeasure.
1 Angstrom = 10^(-10) m</rdfs:comment>
</owl:Class>

<owl:Class rdf:ID= "AnimalController">
<rdfs:subClassOf rdf:resource ="http://127.0.0.1:8000/ontology/SUMO.owl#Device"/>
<rdfs:comment>Any Device which is used to control the
movements of an Animal or Human, e.g. leashes, reins, harnesses, muzzles,
bridles, shackles, handcuffs, etc.</rdfs:comment>
</owl:Class>

<owl:Class rdf:ID= "AnimalPoweredDevice">
<rdfs:subClassOf rdf:resource ="http://127.0.0.1:8000/ontology/SUMO.owl#Device"/>
<rdfs:comment>AnimalPoweredDevice is the subclass
of Devices that function with power supplied by animals.  Examples:
oxcarts, horse-drawn plows, mule-driven mills.</rdfs:comment>
</owl:Class>

<owl:Class rdf:ID= "AnimalResidence">
<rdfs:subClassOf rdf:resource 
="http://127.0.0.1:8000/ontology/SUMO.owl#Artifact"/>
<rdfs:comment>An Artifact which is intended to house
Animals and not Humans.  Note that an AnimalResidence may or may not
be a StationaryArtifact, e.g. a horse stall is stationary while a doghouse
generally is not.</rdfs:comment>
</owl:Class>

<owl:Class rdf:ID= "AnimalShell">
<rdfs:subClassOf rdf:resource 
="http://127.0.0.1:8000/ontology/SUMO.owl#AnimalAnatomicalStructure"/>
<rdfs:subClassOf rdf:resource 
="http://127.0.0.1:8000/ontology/SUMO.owl#BodyPart"/>
<rdfs:comment>A hard shell of calcium that serves as a
supporting structure for some Invertebrates.</rdfs:comment>
</owl:Class>

<owl:Class rdf:ID= "AnimalTeam">
<rdfs:subClassOf rdf:resource ="#GroupOfAnimals"/>
<rdfs:comment>A GroupOfAnimals which are Pulling something.</rdfs:comment>
</owl:Class>

<owl:Class rdf:ID= "Ankle">
<rdfs:subClassOf rdf:resource ="#BodyJoint"/>
<rdfs:comment>The joint in the Leg that connects the tibia and the
fibula to the talus.</rdfs:comment>
</owl:Class>

<owl:Class rdf:ID= "Announcement">
<rdfs:subClassOf rdf:resource 
="http://127.0.0.1:8000/ontology/SUMO.owl#FactualText"/>
<rdfs:comment>Any Text which contains information about
an event in the future.</rdfs:comment>
</owl:Class>

<owl:Class rdf:ID= "Answering">
<rdfs:subClassOf rdf:resource 
="http://127.0.0.1:8000/ontology/SUMO.owl#Stating"/>
<rdfs:comment>Responding to a Questioning, i.e. trying to answer
someone's question.</rdfs:comment>
</owl:Class>

<owl:Class rdf:ID= "AntInsect">
<rdfs:subClassOf rdf:resource ="http://127.0.0.1:8000/ontology/SUMO.owl#Insect"/>
<rdfs:comment>A colony Insect of three types:  males,
QueenInsect, and worker ants.</rdfs:comment>
</owl:Class>

<owl:Class rdf:ID= "AnteMeridiem">
<rdfs:subClassOf rdf:resource 
="http://127.0.0.1:8000/ontology/SUMO.owl#TimeInterval"/>
<rdfs:comment>The class of TimeIntervals that begin at midnight
and end at noon.</rdfs:comment>
</owl:Class>

<owl:Class rdf:ID= "Antelope">
<rdfs:subClassOf rdf:resource 
="http://127.0.0.1:8000/ontology/SUMO.owl#HoofedMammal"/>
<rdfs:comment>A HoofedMammal with long legs and backward-facing horns.
This class includes gazelles, addax, blackbucks, etc.</rdfs:comment>
</owl:Class>

<owl:Class rdf:ID= "Antenna">
<rdfs:subClassOf rdf:resource ="#CommunicationDevice"/>
<rdfs:comment>A CommunicationDevice which enables or improves
the reception of RadioEmissions by another CommunicationDevice (the
radio or television receiver).</rdfs:comment>
</owl:Class>

<owl:Class rdf:ID= "Antibiotic">
<rdfs:subClassOf rdf:resource 
="http://127.0.0.1:8000/ontology/SUMO.owl#BiologicallyActiveSubstance"/>
<rdfs:comment>A BiologicallyActiveSubstance than can kill
instances of Bacterium.</rdfs:comment>
</owl:Class>

<owl:Class rdf:ID= "Antibody">
<rdfs:subClassOf rdf:resource 
="http://127.0.0.1:8000/ontology/SUMO.owl#Protein"/>
<rdfs:comment>An immunoglobulin which is produced by the body
and which has the ability to neutralize Antigens.</rdfs:comment>
</owl:Class>

<owl:Class rdf:ID= "Antigen">
<rdfs:subClassOf rdf:resource 
="http://127.0.0.1:8000/ontology/SUMO.owl#BiologicallyActiveSubstance"/>
<rdfs:comment>Any BiologicallyActiveSubstance that has the
capacity to stimulate the production of Antibodies.</rdfs:comment>
</owl:Class>

<owl:Class rdf:ID= "AntigenA">
<rdfs:subClassOf rdf:resource ="#Antigen"/>
<rdfs:comment>An Antigen that is carried in the red blood
cells of those with BloodTypeA.</rdfs:comment>
</owl:Class>

<owl:Class rdf:ID= "AntigenB">
<rdfs:subClassOf rdf:resource ="#Antigen"/>
<rdfs:comment>An Antigen that is carried in the red blood
cells of those with BloodTypeB.</rdfs:comment>
</owl:Class>

<owl:Class rdf:ID= "ApartmentBuilding">
<rdfs:subClassOf rdf:resource 
="http://127.0.0.1:8000/ontology/SUMO.owl#ResidentialBuilding"/>
<sumo:disjoint rdf:resource = 
"http://127.0.0.1:8000/ontology/SUMO.owl#SingleFamilyResidence" />
<rdfs:comment>A ResidentialBuilding containing
ApartmentUnits.</rdfs:comment>
</owl:Class>

<owl:Class rdf:ID= "ApartmentUnit">
<rdfs:subClassOf rdf:resource 
="http://127.0.0.1:8000/ontology/SUMO.owl#SingleFamilyResidence"/>
<rdfs:comment>A SingleFamilyResidence that is not owned
by any member of the SocialUnit that lives there.</rdfs:comment>
</owl:Class>

<owl:Class rdf:ID= "Apple">
<rdfs:subClassOf rdf:resource 
="http://127.0.0.1:8000/ontology/SUMO.owl#FruitOrVegetable"/>
<rdfs:subClassOf rdf:resource ="http://127.0.0.1:8000/ontology/SUMO.owl#Food"/>
<rdfs:comment>A FruitOrVegetable that has a tart to sweet taste and
a spherical shape.</rdfs:comment>
</owl:Class>

<owl:Class rdf:ID= "Application">
<rdfs:subClassOf rdf:resource ="#FormText"/>
<rdfs:comment>A FormText whose purpose is to obtain admission
to an Organization or to receive assistance from an 
Organization.</rdfs:comment>
</owl:Class>

<owl:Class rdf:ID= "Appointing">
<rdfs:subClassOf rdf:resource 
="http://127.0.0.1:8000/ontology/SUMO.owl#Declaring"/>
<rdfs:comment>Any instance of Declaring by which the
patient is assigned to a Position within an Organization where
the patient previously had no position.  For example, the appointments
of people to non-elective offices in a government.</rdfs:comment>
</owl:Class>

<owl:Class rdf:ID= "Apron">
<rdfs:subClassOf rdf:resource 
="http://127.0.0.1:8000/ontology/SUMO.owl#Clothing"/>
<rdfs:comment>An item of Clothing that protects the front and
middle part of the body while one is Cooking or doing other 
work.</rdfs:comment>
</owl:Class>

<owl:Class rdf:ID= "Argon">
<rdfs:subClassOf rdf:resource 
="http://127.0.0.1:8000/ontology/SUMO.owl#ElementalSubstance"/>
<atomicNumber>18</atomicNumber>
<rdfs:comment>Monatomic noble gas.  Makes up 0.93 percent of the
air.  Colourless, odorless.  Is inert and has no true compounds.  Lord
Rayleigh and Sir william Ramsey identified argon in 1894.</rdfs:comment>
</owl:Class>

<owl:Class rdf:ID= "Arguing">
<rdfs:subClassOf rdf:resource 
="http://127.0.0.1:8000/ontology/SUMO.owl#Stating"/>
<rdfs:comment>Any Stating which has the form of an Argument.</rdfs:comment>
</owl:Class>

<owl:Class rdf:ID= "AridClimateZone">
<rdfs:subClassOf rdf:resource ="#ClimateZone"/>
<rdfs:comment>AridClimateZone is the
class of regions in which the climate is characterized by
a distinct dry season.  Annual rate of moisture evaporation
exceeds annual rate of precipitation. This is Class B in the
Koeppen climate system.</rdfs:comment>
</owl:Class>

<owl:Class rdf:ID= "Arm">
<rdfs:subClassOf rdf:resource ="#Limb"/>
<rdfs:comment>The upper Limbs of a Primate.</rdfs:comment>
</owl:Class>

<owl:Class rdf:ID= "Army">
<rdfs:subClassOf rdf:resource ="#MilitaryService"/>
<rdfs:comment>MilitaryServices that are land forces.</rdfs:comment>
</owl:Class>

<owl:Class rdf:ID= "Arriving">
<rdfs:subClassOf rdf:resource 
="http://127.0.0.1:8000/ontology/SUMO.owl#Translocation"/>
<rdfs:comment>The final part of any instance of 
Translocation.</rdfs:comment>
</owl:Class>

<owl:Class rdf:ID= "ArrowFigure">
<rdfs:subClassOf rdf:resource ="http://127.0.0.1:8000/ontology/SUMO.owl#Icon"/>
<rdfs:comment>An Icon which has the shape of an arrow and
which is used to indicate direction or a relationship betwee two 
things.</rdfs:comment>
</owl:Class>

<owl:Class rdf:ID= "ArrowProjectile">
<rdfs:subClassOf rdf:resource ="#Projectile"/>
<rdfs:comment>A long, thin Projectile with a pointed tip is
fired from a bow.</rdfs:comment>
</owl:Class>

<owl:Class rdf:ID= "ArtCritic">
<rdfs:subClassOf rdf:resource ="#Journalist"/>
<rdfs:comment>The Profession of reporting and critiquing current
ArtWorks.</rdfs:comment>
</owl:Class>

<owl:Class rdf:ID= "ArtPainting">
<rdfs:subClassOf rdf:resource 
="http://127.0.0.1:8000/ontology/SUMO.owl#ContentDevelopment"/>
<rdfs:subClassOf rdf:resource ="#Painting"/>
<rdfs:comment>Any ContentDevelopment that results in a
PaintedPicture.</rdfs:comment>
</owl:Class>

<owl:Class rdf:ID= "ArtSchool">
<rdfs:subClassOf rdf:resource ="#School"/>
<rdfs:comment>Any School whose aim is to teach students
how to create ArtWorks.</rdfs:comment>
</owl:Class>

<owl:Class rdf:ID= "ArtStudio">
<rdfs:subClassOf rdf:resource ="#Workshop"/>
<rdfs:comment>A Workshop devoted to the creation of ArtWorks.</rdfs:comment>
</owl:Class>

<owl:Class rdf:ID= "Artery">
<rdfs:subClassOf rdf:resource ="#BloodVessel"/>
<rdfs:comment>Any BloodVessel which transfers Blood from
the Heart to the extremities of the body.</rdfs:comment>
</owl:Class>

<owl:Class rdf:ID= "ArtificialSatellite">
<rdfs:subClassOf rdf:resource ="#Satellite"/>
<rdfs:subClassOf rdf:resource ="http://127.0.0.1:8000/ontology/SUMO.owl#Device"/>
<rdfs:comment>An ArtificialSatellite is a Device
that orbits the earth in space and performs various functions such as
aiding in communication, photographing the earth's surface, and 
others.</rdfs:comment>
</owl:Class>

<owl:Class rdf:ID= "ArtilleryGun">
<rdfs:subClassOf rdf:resource ="#Gun"/>
<rdfs:comment>A Gun that is too large to be carried and fired
by a single Human.  Typically, ArtilleryGuns are on wheels.</rdfs:comment>
</owl:Class>

<owl:Class rdf:ID= "Asphalt">
<rdfs:subClassOf rdf:resource ="#RefinedPetroleumProduct"/>
<sumo:disjoint rdf:resource = "#FossilFuel" />
<rdfs:comment>Asphalt is the subclass of
RefinedPetroleumProducts that are asphalts.</rdfs:comment>
</owl:Class>

<owl:Class rdf:ID= "Atmosphere">
<rdfs:subClassOf rdf:resource ="http://127.0.0.1:8000/ontology/SUMO.owl#Region"/>
<rdfs:comment>Atmosphere is a mixture of gases
surrounding any celestial object that has a gravitational field
strong enough to prevent the gases from escaping.</rdfs:comment>
</owl:Class>

<owl:Class rdf:ID= "AtmosphericPressureMeasure">
<rdfs:subClassOf rdf:resource 
="http://127.0.0.1:8000/ontology/SUMO.owl#ConstantQuantity"/>
<rdfs:comment>AtmosphericPressureMeasure is the class
of UnitsOfMeasure used to measure pressure (barometricPressure),
e.g., InchMercury.</rdfs:comment>
</owl:Class>

<owl:Class rdf:ID= "AtmosphericRegion">
<rdfs:subClassOf rdf:resource ="#SpaceRegion"/>
<rdfs:comment>AtmosphericRegion is the class of
all subregions of EarthsAtmosphere.</rdfs:comment>
</owl:Class>

<owl:Class rdf:ID= "AtomGram">
<rdfs:subClassOf rdf:resource 
="http://127.0.0.1:8000/ontology/SUMO.owl#MassMeasure"/>
<rdf:type rdf:resource = 
"http://127.0.0.1:8000/ontology/SUMO.owl#UnitOfMeasure"/>
<rdfs:comment>MassMeasure that is also known as the gram-atom.
Defined as the mass in grams of 1 Mole of pure substance.  For example,
1 AtomGram of Carbon 12 will be 12 Grams of pure Carbon 12.  2 AtomGrams
of the same substance will be 24 Grams of it.  This is an unusual unit in
that it is essentially 1 Mole of 'stuff' measured in grams, so that the
actual value (i.e. mass) depends on the type of substance.</rdfs:comment>
</owl:Class>

<owl:Class rdf:ID= "AtomicGroup">
<rdfs:subClassOf rdf:resource 
="http://127.0.0.1:8000/ontology/SUMO.owl#CompoundSubstance"/>
<rdfs:comment>Two or more Atoms that are bound together and
comprise part of a Molecule.</rdfs:comment>
</owl:Class>

<owl:Class rdf:ID= "Atrophy">
<rdfs:subClassOf rdf:resource 
="http://127.0.0.1:8000/ontology/SUMO.owl#PathologicProcess"/>
<rdfs:subClassOf rdf:resource 
="http://127.0.0.1:8000/ontology/SUMO.owl#Decreasing"/>
<rdfs:comment>Any decrease in the size of an Organ which is due to
disease or lack of use.</rdfs:comment>
</owl:Class>

<owl:Class rdf:ID= "Attorney">
<rdfs:subClassOf rdf:resource ="#Profession"/>
<rdfs:comment>The Profession of practicing law, whether as a
judge or as a legal advocate.</rdfs:comment>
</owl:Class>

<owl:Class rdf:ID= "AttorneyGeneral">
<rdfs:subClassOf rdf:resource ="#Attorney"/>
<rdfs:subClassOf rdf:resource ="#GovernmentOfficer"/>
<rdfs:comment>The head law officer of a GeopoliticalArea,
usually a Nation or StateOrProvince.</rdfs:comment>
</owl:Class>

<owl:Class rdf:ID= "AudioRecording">
<rdfs:subClassOf rdf:resource ="http://127.0.0.1:8000/ontology/SUMO.owl#Text"/>
<rdfs:comment>Any Text which is a recording of
RadiatingSound.</rdfs:comment>
</owl:Class>

<owl:Class rdf:ID= "Auditorium">
<rdfs:subClassOf rdf:resource 
="http://127.0.0.1:8000/ontology/SUMO.owl#Building"/>
<rdfs:comment>Any Building whose purpose is to hold concerts,
sports events, plays, etc. before an audience.  This class includes 
theaters,
sports stadiums, university auditoriums, etc.</rdfs:comment>
</owl:Class>

<owl:Class rdf:ID= "AuditoriumSeat">
<rdfs:subClassOf rdf:resource ="#Seat"/>
<rdfs:comment>A Seat within an Auditorium from which one
can observe the PerformanceStage.</rdfs:comment>
</owl:Class>

<owl:Class rdf:ID= "AuthorizationOfTransaction">
<rdfs:subClassOf rdf:resource ="#FinancialService"/>
<rdfs:subClassOf rdf:resource 
="http://127.0.0.1:8000/ontology/SUMO.owl#RegulatoryProcess"/>
<rdfs:comment>An activity which approves or
disapproves a transaction.</rdfs:comment>
</owl:Class>

<owl:Class rdf:ID= "AutomaticGun">
<rdfs:subClassOf rdf:resource ="#Gun"/>
<rdfs:comment>A Gun that fires a burst of Projectiles
with each pull of the trigger.  Also known as a machine gun.</rdfs:comment>
</owl:Class>

<owl:Class rdf:ID= "Automobile">
<rdfs:subClassOf rdf:resource ="#SelfPoweredRoadVehicle"/>
<rdfs:comment>Automobile is a subclass of
SelfPoweredRoadVehicles including passenger cars, family vans, light
trucks, and sport utility vehicles.  In general, this class covers
four-wheeled passenger road vehicles.</rdfs:comment>
</owl:Class>

<owl:Class rdf:ID= "Avocado">
<rdfs:subClassOf rdf:resource 
="http://127.0.0.1:8000/ontology/SUMO.owl#FruitOrVegetable"/>
<rdfs:subClassOf rdf:resource ="http://127.0.0.1:8000/ontology/SUMO.owl#Food"/>
<rdfs:comment>A FruitOrVegetable that is shaped like a pear and
has a dark green skin and a rich meat.</rdfs:comment>
</owl:Class>

<owl:Class rdf:ID= "Axle">
<rdfs:subClassOf rdf:resource ="http://127.0.0.1:8000/ontology/SUMO.owl#Device"/>
<rdfs:comment>Axle is a class of Devices each of which can
be paired with two VehicleWheels to rotate and move a 
RoadVehicle.</rdfs:comment>
</owl:Class>

<owl:Class rdf:ID= "BacterialDisease">
<rdfs:subClassOf rdf:resource ="#InfectiousDisease"/>
<rdfs:comment>A disease that is caused by instances of
Bacterium.</rdfs:comment>
</owl:Class>

<owl:Class rdf:ID= "Bag">
<rdfs:subClassOf rdf:resource ="#Container"/>
<rdfs:comment>Any Container which is made of Fabric.</rdfs:comment>
</owl:Class>

<owl:Class rdf:ID= "Baking">
<rdfs:subClassOf rdf:resource 
="http://127.0.0.1:8000/ontology/SUMO.owl#Cooking"/>
<rdfs:subClassOf rdf:resource 
="http://127.0.0.1:8000/ontology/SUMO.owl#Heating"/>
<rdfs:comment>Any instance of Cooking where the instrument
is an Oven.</rdfs:comment>
</owl:Class>

<owl:Class rdf:ID= "Ball">
<rdfs:subClassOf rdf:resource ="#GamePiece"/>
<rdfs:comment>Any GamePiece which has the shape of a sphere.</rdfs:comment>
</owl:Class>

<owl:Class rdf:ID= "BallisticMissile">
<rdfs:subClassOf rdf:resource ="#Missile"/>
<rdfs:comment>A Missile which is guided for the first stage
of its flight but then falls to its target for the second 
stage.</rdfs:comment>
</owl:Class>

<owl:Class rdf:ID= "Ballot">
<rdfs:subClassOf rdf:resource ="#FormText"/>
<rdfs:comment>A FormText which is used in Voting.  A list of
candidates is printed on the form, and the voter selects the candidate 
he/she
wants to vote for.</rdfs:comment>
</owl:Class>

<owl:Class rdf:ID= "Bandage">
<rdfs:subClassOf rdf:resource ="#FabricArtifact"/>
<rdfs:comment>A piece of Fabric that is used to cover an
open wound.</rdfs:comment>
</owl:Class>

<owl:Class rdf:ID= "Banker">
<rdfs:subClassOf rdf:resource ="#SkilledOccupation"/>
<rdfs:comment>Any SkilledOccupation which involves working in a
FinancialBank.</rdfs:comment>
</owl:Class>

<owl:Class rdf:ID= "Baptizing">
<rdfs:subClassOf rdf:resource 
="http://127.0.0.1:8000/ontology/SUMO.owl#ReligiousProcess"/>
<rdfs:subClassOf rdf:resource 
="http://127.0.0.1:8000/ontology/SUMO.owl#JoiningAnOrganization"/>
<rdfs:comment>A ReligiousProcess which marks the acceptance of
the person being baptized into the ReligiousOrganization.</rdfs:comment>
</owl:Class>

<owl:Class rdf:ID= "BargainSale">
<rdfs:subClassOf rdf:resource ="#OfferingForSale"/>
<rdfs:comment>Offering to sell something to someone at a
reduced price.</rdfs:comment>
</owl:Class>

<owl:Class rdf:ID= "Barking">
<rdfs:subClassOf rdf:resource 
="http://127.0.0.1:8000/ontology/SUMO.owl#RadiatingSound"/>
<rdfs:comment>Any instance of RadiatingSound which is produced
by a Canine.</rdfs:comment>
</owl:Class>

<owl:Class rdf:ID= "Baseball">
<rdfs:subClassOf rdf:resource ="#TeamSport"/>
<rdfs:comment>A TeamSport which involves two teams of 9 players
each that take turns at bat and attempt to score runs.  Note that each 
instance
of Baseball is a baseball game.</rdfs:comment>
</owl:Class>

<owl:Class rdf:ID= "BaseballBase">
<rdfs:subClassOf rdf:resource ="#GameArtifact"/>
<rdfs:comment>Any of four regions which must each be
successively touched after a BaseballHit in order to complete a
BaseballRun.</rdfs:comment>
</owl:Class>

<owl:Class rdf:ID= "BaseballBat">
<rdfs:subClassOf rdf:resource ="#GameArtifact"/>
<rdfs:comment>A bat which is used to hit the ball in
Baseball.</rdfs:comment>
</owl:Class>

<owl:Class rdf:ID= "BaseballDugout">
<rdfs:subClassOf rdf:resource 
="http://127.0.0.1:8000/ontology/SUMO.owl#Building"/>
<rdfs:comment>A Building which is used to house the members
of both Baseball teams while a game is being played.</rdfs:comment>
</owl:Class>

<owl:Class rdf:ID= "BaseballField">
<rdfs:subClassOf rdf:resource ="#SportsFacility"/>
<rdfs:comment>A SportsFacility which is dedicated to
Baseball.</rdfs:comment>
</owl:Class>

<owl:Class rdf:ID= "BaseballHit">
<rdfs:subClassOf rdf:resource ="#GameShot"/>
<rdfs:subClassOf rdf:resource ="#BaseballManeuver"/>
<rdfs:comment>Any base hit in Baseball.</rdfs:comment>
</owl:Class>

<owl:Class rdf:ID= "BaseballInning">
<rdfs:subClassOf rdf:resource ="#BaseballManeuver"/>
<rdfs:comment>A division of a Baseball game.  A normal game
consists of 9 innings, and each inning involves a turn a bat for both 
teams.</rdfs:comment>
</owl:Class>

<owl:Class rdf:ID= "BaseballManeuver">
<rdfs:subClassOf rdf:resource 
="http://127.0.0.1:8000/ontology/SUMO.owl#Maneuver"/>
<rdfs:comment>Any Maneuver in Baseball.</rdfs:comment>
</owl:Class>

<owl:Class rdf:ID= "BaseballRun">
<rdfs:subClassOf rdf:resource ="#BaseballHit"/>
<rdfs:subClassOf rdf:resource ="#Score"/>
<rdfs:comment>A Score in Baseball.  It consists of hitting
the ball with the bat and then touching all four bases of the diamond before
being tagged with the ball by a member of the opposite team.</rdfs:comment>
</owl:Class>

<owl:Class rdf:ID= "BaseballSingle">
<rdfs:subClassOf rdf:resource ="#BaseballHit"/>
<rdfs:comment>Any BaseballHit where the batter makes it
safely to first base by hitting the ball.</rdfs:comment>
</owl:Class>

<owl:Class rdf:ID= "BaseballSteal">
<rdfs:subClassOf rdf:resource ="#BaseballManeuver"/>
<sumo:disjoint rdf:resource = "#BaseballWalk" />
<sumo:disjoint rdf:resource = "#BaseballHit" />
<rdfs:comment>Any move from one base to another which is neither
a BaseballWalk nor a BaseballHit.</rdfs:comment>
</owl:Class>

<owl:Class rdf:ID= "BaseballTeam">
<rdfs:subClassOf rdf:resource ="#SportsTeam"/>
<rdfs:comment>The class of SportsTeams that play Baseball.</rdfs:comment>
</owl:Class>

<owl:Class rdf:ID= "BaseballWalk">
<rdfs:subClassOf rdf:resource ="#BaseballManeuver"/>
<sumo:disjoint rdf:resource = "#BaseballHit" />
<rdfs:comment>Taking first base after four balls have been
called by the umpire.</rdfs:comment>
</owl:Class>

<owl:Class rdf:ID= "Basement">
<rdfs:subClassOf rdf:resource ="#BuildingLevel"/>
<rdfs:comment>A BuildingLevel which satisfies two conditions, viz. it is
lower than all of the other BuildingLevels in the same Building and it is 
below
ground level.</rdfs:comment>
</owl:Class>

<owl:Class rdf:ID= "Basketball">
<rdfs:subClassOf rdf:resource ="#TeamSport"/>
<rdfs:comment>A TeamSport which involves two teams of 5 players
each.  The object of the game is to put the ball through a 
hoop.</rdfs:comment>
</owl:Class>

<owl:Class rdf:ID= "Bathing">
<rdfs:subClassOf rdf:resource ="#Washing"/>
<rdfs:comment>Washing the entire body of a Human or Animal.</rdfs:comment>
</owl:Class>

<owl:Class rdf:ID= "BathingDevice">
<rdfs:subClassOf rdf:resource ="#WashingDevice"/>
<rdfs:comment>A WashingDevice which is intended to be used by
Humans for washing their bodies.  Note that this class covers bathtubs, 
showers,
etc.</rdfs:comment>
</owl:Class>

<owl:Class rdf:ID= "Bathroom">
<rdfs:subClassOf rdf:resource ="http://127.0.0.1:8000/ontology/SUMO.owl#Room"/>
<rdfs:comment>A Room that contains a WashBasin and
possibly a Toilet.</rdfs:comment>
</owl:Class>

<owl:Class rdf:ID= "Baton">
<rdfs:subClassOf rdf:resource ="http://127.0.0.1:8000/ontology/SUMO.owl#Device"/>
<rdfs:comment>A thin stick which is used for 
OrchestralConducting.</rdfs:comment>
</owl:Class>

<owl:Class rdf:ID= "Battery">
<rdfs:subClassOf rdf:resource ="http://127.0.0.1:8000/ontology/SUMO.owl#Device"/>
<rdfs:comment>Battery is a subclass of Device.  Batteries are
devices that use chemical means to store or produce electrical 
power.</rdfs:comment>
</owl:Class>

<owl:Class rdf:ID= "BecomingDrunk">
<rdfs:subClassOf rdf:resource 
="http://127.0.0.1:8000/ontology/SUMO.owl#PsychologicalProcess"/>
<sumo:disjoint rdf:resource = "#SoberingUp" />
<rdfs:comment>The process of transitioning from a state of
being Sober to a state of being Drunk.</rdfs:comment>
</owl:Class>

<owl:Class rdf:ID= "Becquerel">
<rdfs:subClassOf rdf:resource 
="http://127.0.0.1:8000/ontology/SUMO.owl#TimeDependentQuantity"/>
<rdf:type rdf:resource = 
"http://127.0.0.1:8000/ontology/SUMO.owl#SystemeInternationalUnit"/>
<rdfs:comment>SI activity measure.  Symbol: Bq.  It measures
the amount of radioactivity contained in a given sample of matter. It is
that quantity of a radioactive element in which there is one atomic
disintegration per SecondDuration.  Becquerel = s^(-1).</rdfs:comment>
</owl:Class>

<owl:Class rdf:ID= "Bed">
<rdfs:subClassOf rdf:resource ="#Furniture"/>
<rdfs:comment>A piece of Furniture which is primarily for 
sleeping.</rdfs:comment>
</owl:Class>

<owl:Class rdf:ID= "Bedroom">
<rdfs:subClassOf rdf:resource ="http://127.0.0.1:8000/ontology/SUMO.owl#Room"/>
<rdfs:comment>A Room intended primarily for sleeping.</rdfs:comment>
</owl:Class>

<owl:Class rdf:ID= "Bee">
<rdfs:subClassOf rdf:resource ="http://127.0.0.1:8000/ontology/SUMO.owl#Insect"/>
<rdfs:comment>A hairy Insect, some species of which produce honey
and/or sting.</rdfs:comment>
</owl:Class>

<owl:Class rdf:ID= "Beef">
<rdfs:subClassOf rdf:resource ="http://127.0.0.1:8000/ontology/SUMO.owl#Meat"/>
<rdfs:comment>Meat that was originally part of a Cow.</rdfs:comment>
</owl:Class>

<owl:Class rdf:ID= "Beer">
<rdfs:subClassOf rdf:resource ="#AlcoholicBeverage"/>
<rdfs:comment>An AlcoholicBeverage that is prepared by fermenting
malt and hops.</rdfs:comment>
</owl:Class>

<owl:Class rdf:ID= "BeginningOperations">
<rdfs:subClassOf rdf:resource 
="http://127.0.0.1:8000/ontology/SUMO.owl#OrganizationalProcess"/>
<sumo:disjoint rdf:resource = "#CeasingOperations" />
<rdfs:comment>The process of an Organization
commencing operations.  In the case of a Corporation, this would be
the process of going into business.</rdfs:comment>
</owl:Class>

<owl:Class rdf:ID= "Bell">
<rdfs:subClassOf rdf:resource ="#PercussionInstrument"/>
<rdfs:comment>A PercussionInstrument which is made of Metal and
which produces a single tone when it is struck.</rdfs:comment>
</owl:Class>

<owl:Class rdf:ID= "Belt">
<rdfs:subClassOf rdf:resource 
="http://127.0.0.1:8000/ontology/SUMO.owl#Clothing"/>
<rdfs:comment>A piece of Clothing that is worn around the waist
of a pair of Trousers.</rdfs:comment>
</owl:Class>

<owl:Class rdf:ID= "Bequeathing">
<rdfs:subClassOf rdf:resource 
="http://127.0.0.1:8000/ontology/SUMO.owl#UnilateralGiving"/>
<rdfs:comment>Any UnilateralGiving where the agent
wills some part of his/her property to someone else upon his/her 
death.</rdfs:comment>
</owl:Class>

<owl:Class rdf:ID= "Bicycle">
<rdfs:subClassOf rdf:resource ="#Cycle-TransportationDevice"/>
<rdfs:comment>Bicycle is a class of two-wheeled,
UserPoweredVehicles.</rdfs:comment>
</owl:Class>

<owl:Class rdf:ID= "BiochemicalAgent">
<rdfs:subClassOf rdf:resource 
="http://127.0.0.1:8000/ontology/SUMO.owl#SelfConnectedObject"/>
<rdfs:comment>A BiologicalAgent or a ChemicalAgent.</rdfs:comment>
</owl:Class>

<owl:Class rdf:ID= "BiochemicalAttack">
<rdfs:subClassOf rdf:resource ="http://127.0.0.1:8000/ontology/SUMO.owl#Attack"/>
<rdfs:comment>Attacks in which a BiochemicalWeapon
is used against an Organism.</rdfs:comment>
</owl:Class>

<owl:Class rdf:ID= "BiochemicalWeapon">
<rdfs:subClassOf rdf:resource ="#WeaponOfMassDestruction"/>
<rdfs:comment>A WeaponOfMassDestruction that is
either a BiologicalWeapon or a ChemicalWeapon, i.e. not a
RadioactiveWeapon.</rdfs:comment>
</owl:Class>

<owl:Class rdf:ID= "Biography">
<rdfs:subClassOf rdf:resource ="#HistoricalAccount"/>
<rdfs:comment>A HistoricalAccount which is concerned
with the life of a single Human.</rdfs:comment>
</owl:Class>

<owl:Class rdf:ID= "BiologicalAgent">
<rdfs:subClassOf rdf:resource ="#BiochemicalAgent"/>
<rdfs:comment>A naturally occurring Substance, a
synthetic analogue of such a substance or an Organism that is capable
of inflicting severe harm on other Organisms.  All BiologicalWeapons
contain a BiologicalAgent.</rdfs:comment>
</owl:Class>

<owl:Class rdf:ID= "BiologicalConception">
<rdfs:subClassOf rdf:resource 
="http://127.0.0.1:8000/ontology/SUMO.owl#OrganOrTissueProcess"/>
<rdfs:comment>The production of a zygote from the fusion
of a male and female gamete.</rdfs:comment>
</owl:Class>

<owl:Class rdf:ID= "BiologicalSpecies">
<rdfs:subClassOf rdf:resource ="http://127.0.0.1:8000/ontology/SUMO.owl#Class"/>
<rdfs:comment>The Class of all biological species, i.e.
the class of all classes of Organism whose instances can 
interbreed.</rdfs:comment>
</owl:Class>

<owl:Class rdf:ID= "BiologicalWeapon">
<rdfs:subClassOf rdf:resource ="#BiochemicalWeapon"/>
<rdfs:comment>Weapons which contain a sample of
ToxicOrganism or a BiologicallyActiveSubstance that is produced by a
ToxicOrganism (or a synthetic analogue of the latter).</rdfs:comment>
</owl:Class>

<owl:Class rdf:ID= "Biopsy">
<rdfs:subClassOf rdf:resource 
="http://127.0.0.1:8000/ontology/SUMO.owl#DiagnosticProcess"/>
<rdfs:comment>Any DiagnosticProcess which involves the examination of
BodySubstances taken from a living Organism.</rdfs:comment>
</owl:Class>

<owl:Class rdf:ID= "BirdEgg">
<rdfs:subClassOf rdf:resource ="http://127.0.0.1:8000/ontology/SUMO.owl#Egg"/>
<rdfs:comment>Any Egg that is produced by a Bird.</rdfs:comment>
</owl:Class>

<owl:Class rdf:ID= "Biting">
<rdfs:subClassOf rdf:resource 
="http://127.0.0.1:8000/ontology/SUMO.owl#Grabbing"/>
<rdfs:comment>Any instance of Grabbing where the instrument is
the Mouth of the agent.</rdfs:comment>
</owl:Class>

<owl:Class rdf:ID= "Blanket">
<rdfs:subClassOf rdf:resource ="#FabricArtifact"/>
<rdfs:comment>An Artifact made of Fabric whose function is
to cover a sleeping person while he/she sleeps.</rdfs:comment>
</owl:Class>

<owl:Class rdf:ID= "Bleeding">
<rdfs:subClassOf rdf:resource 
="http://127.0.0.1:8000/ontology/SUMO.owl#AutonomicProcess"/>
<rdfs:comment>The release of Blood from an Animal in response
to an Injuring of some sort.</rdfs:comment>
</owl:Class>

<owl:Class rdf:ID= "Bloating">
<rdfs:subClassOf rdf:resource 
="http://127.0.0.1:8000/ontology/SUMO.owl#Increasing"/>
<rdfs:subClassOf rdf:resource 
="http://127.0.0.1:8000/ontology/SUMO.owl#PathologicProcess"/>
<rdfs:comment>Any Process where the stomach or instestines of a
Human or Animal become distended from excessive gas.</rdfs:comment>
</owl:Class>

<owl:Class rdf:ID= "Blockade">
<rdfs:subClassOf rdf:resource 
="http://127.0.0.1:8000/ontology/SUMO.owl#Maneuver"/>
<rdfs:comment>Any Maneuver in a Contest where one contestParticipant
attempts to deny access to something that is wanted by another 
contestParticipant.</rdfs:comment>
</owl:Class>

<owl:Class rdf:ID= "BloodCell">
<rdfs:subClassOf rdf:resource ="http://127.0.0.1:8000/ontology/SUMO.owl#Cell"/>
<rdfs:subClassOf rdf:resource 
="http://127.0.0.1:8000/ontology/SUMO.owl#AnimalAnatomicalStructure"/>
<rdfs:comment>A Cell that is normally present in Blood.</rdfs:comment>
</owl:Class>

<owl:Class rdf:ID= "BloodTypeA">
<rdfs:subClassOf rdf:resource ="http://127.0.0.1:8000/ontology/SUMO.owl#Blood"/>
<rdfs:comment>The subclass of Blood that contains AntigenA
and does not contain AntigenB.</rdfs:comment>
</owl:Class>

<owl:Class rdf:ID= "BloodTypeAB">
<rdfs:subClassOf rdf:resource ="http://127.0.0.1:8000/ontology/SUMO.owl#Blood"/>
<rdfs:comment>The subclass of Blood that contains both
AntigenA and AntigenB.</rdfs:comment>
</owl:Class>

<owl:Class rdf:ID= "BloodTypeB">
<rdfs:subClassOf rdf:resource ="http://127.0.0.1:8000/ontology/SUMO.owl#Blood"/>
<rdfs:comment>The subclass of Blood that contains AntigenB
and does not contain AntigenA.</rdfs:comment>
</owl:Class>

<owl:Class rdf:ID= "BloodTypeO">
<rdfs:subClassOf rdf:resource ="http://127.0.0.1:8000/ontology/SUMO.owl#Blood"/>
<rdfs:comment>The subclass of Blood that contains neither
AntigenA nor AntigenB.</rdfs:comment>
</owl:Class>

<owl:Class rdf:ID= "BloodVessel">
<rdfs:subClassOf rdf:resource 
="http://127.0.0.1:8000/ontology/SUMO.owl#BodyVessel"/>
<rdfs:subClassOf rdf:resource 
="http://127.0.0.1:8000/ontology/SUMO.owl#AnimalAnatomicalStructure"/>
<rdfs:comment>Any BodyVessel which is used to circulate
Blood from one part of the body to another.</rdfs:comment>
</owl:Class>

<owl:Class rdf:ID= "Blueprint">
<rdfs:subClassOf rdf:resource ="http://127.0.0.1:8000/ontology/SUMO.owl#Icon"/>
<rdfs:comment>An Icon which is a scale model of an Artifact,
whether the Artifact actually exists or not.</rdfs:comment>
</owl:Class>

<owl:Class rdf:ID= "Blushing">
<rdfs:subClassOf rdf:resource 
="http://127.0.0.1:8000/ontology/SUMO.owl#AutonomicProcess"/>
<rdfs:comment>The process of turning red in response to a
stimulus which has a deep emotional effect.</rdfs:comment>
</owl:Class>

<owl:Class rdf:ID= "BoardOrBlock">
<rdfs:subClassOf rdf:resource 
="http://127.0.0.1:8000/ontology/SUMO.owl#Artifact"/>
<rdfs:comment>A piece of material with flat, rectangular sides.
Note that boards and blocks are lumped into a single concept, because the
difference between these notions cannot be precisely defined.</rdfs:comment>
</owl:Class>

<owl:Class rdf:ID= "Boarding">
<rdfs:subClassOf rdf:resource 
="http://127.0.0.1:8000/ontology/SUMO.owl#Translocation"/>
<rdfs:comment>Getting on a Vehicle, e.g. getting into an
Automobile, boarding an Aircraft, etc.</rdfs:comment>
</owl:Class>

<owl:Class rdf:ID= "BoatDeck">
<rdfs:subClassOf rdf:resource 
="http://127.0.0.1:8000/ontology/SUMO.owl#Artifact"/>
<rdfs:comment>One of the levels of a Watercraft, e.g. the
upper deck and lower deck of small boats with a cabin.</rdfs:comment>
</owl:Class>

<owl:Class rdf:ID= "BodyJoint">
<rdfs:subClassOf rdf:resource 
="http://127.0.0.1:8000/ontology/SUMO.owl#AnimalAnatomicalStructure"/>
<rdfs:comment>BodyJunctions where different parts of the same
Skeleton come together.</rdfs:comment>
</owl:Class>

<owl:Class rdf:ID= "BodyOfWater">
<rdfs:subClassOf rdf:resource 
="http://127.0.0.1:8000/ontology/SUMO.owl#WaterArea"/>
<rdfs:subClassOf rdf:resource 
="http://127.0.0.1:8000/ontology/SUMO.owl#SelfConnectedObject"/>
<rdfs:comment>A BodyOfWater is a connected body of
water with established boundaries marked by either geographical features
or conventional borders.</rdfs:comment>
</owl:Class>

<owl:Class rdf:ID= "Bodybuilding">
<rdfs:subClassOf rdf:resource ="http://127.0.0.1:8000/ontology/SUMO.owl#Sport"/>
<rdfs:comment>A sport which involves the development of one's
Muscles and competition against other bodybuilders.</rdfs:comment>
</owl:Class>

<owl:Class rdf:ID= "Bomber">
<rdfs:subClassOf rdf:resource ="#MilitaryAircraft"/>
<rdfs:comment>Any MilitaryAircraft whose purpose is to deliver
ExplosiveDevices.</rdfs:comment>
</owl:Class>

<owl:Class rdf:ID= "Bond">
<rdfs:subClassOf rdf:resource 
="http://127.0.0.1:8000/ontology/SUMO.owl#FinancialInstrument"/>
<rdfs:comment>A debt instrument issued for a period of more than one year 
with
the purpose of raising capital by borrowing. The Federal government, states, 
cities,
corporations, and many other types of institutions sell bonds. A bond is 
generally a
promise to repay the principal along with interest on a specified 
maturityDate.</rdfs:comment>
</owl:Class>

<owl:Class rdf:ID= "BotanicalTree">
<rdfs:subClassOf rdf:resource 
="http://127.0.0.1:8000/ontology/SUMO.owl#FloweringPlant"/>
<rdfs:comment>BotanicalTree is an imprecise term
for a perennial woody plant that is larger than a bush or shrub,
generally understood to describe a large growth having one main trunk
with few or no branches projecting from its base, a well-developed crown
of foliage, and a height at maturity of at least 12 feet.</rdfs:comment>
</owl:Class>

<owl:Class rdf:ID= "Bottle">
<rdfs:subClassOf rdf:resource ="#FluidContainer"/>
<rdfs:comment>A Container whose top is narrower than its bottom,
which has no handle, and which is intended to store Liquids.</rdfs:comment>
</owl:Class>

<owl:Class rdf:ID= "Bowing">
<rdfs:subClassOf rdf:resource ="#Inclining"/>
<rdfs:subClassOf rdf:resource 
="http://127.0.0.1:8000/ontology/SUMO.owl#Gesture"/>
<rdfs:comment>Any downward motion of the body that indicates respect
for or submission to another Agent.</rdfs:comment>
</owl:Class>

<owl:Class rdf:ID= "Box">
<rdfs:subClassOf rdf:resource ="#Container"/>
<rdfs:comment>Any six-sided Container whose sides are
rectangular in shape.</rdfs:comment>
</owl:Class>

<owl:Class rdf:ID= "Boxcar">
<rdfs:subClassOf rdf:resource ="#FreightCar"/>
<rdfs:comment>Boxcar is the subclass of Railcars that are
general-purpose closed cars for hauling freight.</rdfs:comment>
</owl:Class>

<owl:Class rdf:ID= "Boxing">
<rdfs:subClassOf rdf:resource 
="http://127.0.0.1:8000/ontology/SUMO.owl#ViolentContest"/>
<rdfs:subClassOf rdf:resource ="http://127.0.0.1:8000/ontology/SUMO.owl#Sport"/>
<rdfs:comment>A sport which involves two participants who try to
knock each other out in a limited number of rounds.  Note that each instance
of Boxing is a boxing match.</rdfs:comment>
</owl:Class>

<owl:Class rdf:ID= "Boy">
<rdfs:subClassOf rdf:resource ="#HumanChild"/>
<rdfs:subClassOf rdf:resource ="http://127.0.0.1:8000/ontology/SUMO.owl#Man"/>
<rdfs:comment>A HumanChild who is Male.</rdfs:comment>
</owl:Class>

<owl:Class rdf:ID= "Brain">
<rdfs:subClassOf rdf:resource ="http://127.0.0.1:8000/ontology/SUMO.owl#Organ"/>
<rdfs:subClassOf rdf:resource 
="http://127.0.0.1:8000/ontology/SUMO.owl#AnimalAnatomicalStructure"/>
<rdfs:comment>The seat of the central nervous system.</rdfs:comment>
</owl:Class>

<owl:Class rdf:ID= "Brandy">
<rdfs:subClassOf rdf:resource ="#DistilledAlcoholicBeverage"/>
<rdfs:comment>A DistilledAlcoholicBeverage that is prepared by
distilling Wine.</rdfs:comment>
</owl:Class>

<owl:Class rdf:ID= "Brass">
<rdfs:subClassOf rdf:resource ="#MetallicAlloy"/>
<rdfs:comment>A MetallicAlloy made from Copper and Zinc.</rdfs:comment>
</owl:Class>

<owl:Class rdf:ID= "BreadOrBiscuit">
<rdfs:subClassOf rdf:resource ="#PreparedFood"/>
<rdfs:comment>Food that consists largely of grain flour
and water.  Note that this class covers crackers, cookies, as well as any
self-connected instance of bread, whether it is a loaf, a slice, a chunk
of bread, etc.</rdfs:comment>
</owl:Class>

<owl:Class rdf:ID= "BreakabilityAttribute">
<rdfs:subClassOf rdf:resource 
="http://127.0.0.1:8000/ontology/SUMO.owl#InternalAttribute"/>
<rdfs:comment>A subclass of Attributes for
characterizing the breakability of CorpuscularObjects.</rdfs:comment>
</owl:Class>

<owl:Class rdf:ID= "Breast">
<rdfs:subClassOf rdf:resource 
="http://127.0.0.1:8000/ontology/SUMO.owl#AnimalAnatomicalStructure"/>
<rdfs:subClassOf rdf:resource ="http://127.0.0.1:8000/ontology/SUMO.owl#Organ"/>
<rdfs:comment>The paired Organs which are part of the chests
of Primates.</rdfs:comment>
</owl:Class>

<owl:Class rdf:ID= "Brick">
<rdfs:subClassOf rdf:resource ="#BoardOrBlock"/>
<rdfs:comment>A block of fired Clay that is used in 
Constructing.</rdfs:comment>
</owl:Class>

<owl:Class rdf:ID= "Bridge">
<rdfs:subClassOf rdf:resource 
="http://127.0.0.1:8000/ontology/SUMO.owl#LandTransitway"/>
<rdfs:subClassOf rdf:resource 
="http://127.0.0.1:8000/ontology/SUMO.owl#StationaryArtifact"/>
<rdfs:comment>Bridge is the subclass of LandTransitways
that are artifacts used for crossing water or air-filled gaps that
could not be transited over a natural surface.</rdfs:comment>
</owl:Class>

<owl:Class rdf:ID= "BrigadierGeneral">
<rdfs:subClassOf rdf:resource ="#MilitaryGeneral"/>
<rdfs:comment>A MilitaryGeneral that ranks below
a MajorGeneral.</rdfs:comment>
</owl:Class>

<owl:Class rdf:ID= "BroadcastNetwork">
<rdfs:subClassOf rdf:resource ="#CommunicationSystem"/>
<rdfs:comment>BroadcastNetwork is the subclass of
CommunicationSystems consisting of BroadcastingStations that are linked
electronically and managed or owned by one organization.</rdfs:comment>
</owl:Class>

<owl:Class rdf:ID= "BroadcastProgram">
<rdfs:subClassOf rdf:resource ="http://127.0.0.1:8000/ontology/SUMO.owl#Series"/>
<rdfs:comment>A Series of episodes that are broadcast
on television or radio.</rdfs:comment>
</owl:Class>

<owl:Class rdf:ID= "Broadcasting">
<rdfs:subClassOf rdf:resource 
="http://127.0.0.1:8000/ontology/SUMO.owl#Disseminating"/>
<rdfs:subClassOf rdf:resource ="#RadioEmission"/>
<rdfs:comment>Disseminating information by using a
CommunicationDevice that radiates RadioEmissions.</rdfs:comment>
</owl:Class>

<owl:Class rdf:ID= "BroadcastingStation">
<rdfs:subClassOf rdf:resource 
="http://127.0.0.1:8000/ontology/SUMO.owl#StationaryArtifact"/>
<rdfs:subClassOf rdf:resource ="#CommunicationDevice"/>
<rdfs:comment>A BroadcastingStation is
a TelevisionStation or a RadioStation.</rdfs:comment>
</owl:Class>

<owl:Class rdf:ID= "BronchialDuct">
<rdfs:subClassOf rdf:resource 
="http://127.0.0.1:8000/ontology/SUMO.owl#BodyVessel"/>
<rdfs:subClassOf rdf:resource 
="http://127.0.0.1:8000/ontology/SUMO.owl#AnimalAnatomicalStructure"/>
<rdfs:comment>Any BodyVessel which is located in a
Lung and which carries oxygen from the trachea to the 
alveoli.</rdfs:comment>
</owl:Class>

<owl:Class rdf:ID= "Brood">
<rdfs:subClassOf rdf:resource ="#GroupOfAnimals"/>
<rdfs:comment>A GroupOfAnimals that are all born at the same time
and to the same parents.</rdfs:comment>
</owl:Class>

<owl:Class rdf:ID= "Broom">
<rdfs:subClassOf rdf:resource ="#BrushOrComb"/>
<rdfs:comment>A BrushOrComb whose purpose is to remove dirt and other
small particles from floors.</rdfs:comment>
</owl:Class>

<owl:Class rdf:ID= "BrushOrComb">
<rdfs:subClassOf rdf:resource ="http://127.0.0.1:8000/ontology/SUMO.owl#Device"/>
<rdfs:comment>A Device which consists of a handle and bristles and
whose purpose is to remove particles from something or to smooth something 
out.</rdfs:comment>
</owl:Class>

<owl:Class rdf:ID= "Bubble">
<rdfs:subClassOf rdf:resource 
="http://127.0.0.1:8000/ontology/SUMO.owl#CorpuscularObject"/>
<rdfs:comment>A globe which has a Liquid surface and which contains
a Gas.</rdfs:comment>
</owl:Class>

<owl:Class rdf:ID= "Buffalo">
<rdfs:subClassOf rdf:resource 
="http://127.0.0.1:8000/ontology/SUMO.owl#HoofedMammal"/>
<sumo:disjoint rdf:resource = "#DomesticAnimal" />
<rdfs:comment>A HoofedMammal with long hair whose habitat is the
plains of NorthAmerica.</rdfs:comment>
</owl:Class>

<owl:Class rdf:ID= "Bugle">
<rdfs:subClassOf rdf:resource ="#HornInstrument"/>
<rdfs:comment>A HornInstrument that has no valves.</rdfs:comment>
</owl:Class>

<owl:Class rdf:ID= "BuildingLevel">
<rdfs:subClassOf rdf:resource 
="http://127.0.0.1:8000/ontology/SUMO.owl#StationaryArtifact"/>
<rdfs:comment>The story or level of a building, e.g. the Basement,
the Attic, the ground level, the fourteenth floor, etc.</rdfs:comment>
</owl:Class>

<owl:Class rdf:ID= "Bull">
<rdfs:subClassOf rdf:resource ="#Cow"/>
<rdfs:comment>A Cow that is Male.</rdfs:comment>
</owl:Class>

<owl:Class rdf:ID= "Bullet">
<rdfs:subClassOf rdf:resource ="#Projectile"/>
<rdfs:comment>A Projectile that is designed to be fired by a 
Gun.</rdfs:comment>
</owl:Class>

<owl:Class rdf:ID= "BumbleBee">
<rdfs:subClassOf rdf:resource ="#Bee"/>
<rdfs:comment>A large Bee which lacks a stinger.</rdfs:comment>
</owl:Class>

<owl:Class rdf:ID= "Burrow">
<rdfs:subClassOf rdf:resource ="#Cave"/>
<rdfs:comment>A small Cave created by an Animal for the purpose
of inhabiting it.</rdfs:comment>
</owl:Class>

<owl:Class rdf:ID= "Burying">
<rdfs:subClassOf rdf:resource 
="http://127.0.0.1:8000/ontology/SUMO.owl#Putting"/>
<rdfs:comment>Putting something in the ground and then covering
it with Soil.</rdfs:comment>
</owl:Class>

<owl:Class rdf:ID= "Bus">
<rdfs:subClassOf rdf:resource ="#SelfPoweredRoadVehicle"/>
<rdfs:comment>Bus is the subclass of SelfPoweredRoadVehicles
that can transport large numbers of passengers (i.e., dozens) at one
time.</rdfs:comment>
</owl:Class>

<owl:Class rdf:ID= "BusinessCompetition">
<rdfs:subClassOf rdf:resource 
="http://127.0.0.1:8000/ontology/SUMO.owl#Contest"/>
<rdfs:comment>Any Contest where the contestParticipants
are CommercialAgents and the aim is to win as many customers as 
possible.</rdfs:comment>
</owl:Class>

<owl:Class rdf:ID= "Butter">
<rdfs:subClassOf rdf:resource ="#PreparedFood"/>
<rdfs:comment>An emulsion of fat which is produced by churning 
Milk.</rdfs:comment>
</owl:Class>

<owl:Class rdf:ID= "Button">
<rdfs:subClassOf rdf:resource 
="http://127.0.0.1:8000/ontology/SUMO.owl#AttachingDevice"/>
<rdfs:comment>An AttachingDevice that is used on Clothing.</rdfs:comment>
</owl:Class>

<owl:Class rdf:ID= "CPU">
<rdfs:subClassOf rdf:resource ="#ComputerHardware"/>
<rdfs:comment>CPU (Central Processing Unit) is the computing part
of the computer.</rdfs:comment>
</owl:Class>

<owl:Class rdf:ID= "Cafeteria">
<rdfs:subClassOf rdf:resource ="#Restaurant"/>
<rdfs:comment>Any Restaurant which does not offer table service.
Food is selected and purchased at a central counter.</rdfs:comment>
</owl:Class>

<owl:Class rdf:ID= "Calcium">
<rdfs:subClassOf rdf:resource 
="http://127.0.0.1:8000/ontology/SUMO.owl#ElementalSubstance"/>
<atomicNumber>20</atomicNumber>
<rdfs:comment>Soft grey metallic element belonging to group 2 of
the periodic table.  Used a reducing agent in the extraction of thorium,
zirconium and uranium.  Essential element for living 
organisms.</rdfs:comment>
</owl:Class>

<owl:Class rdf:ID= "Calf">
<rdfs:subClassOf rdf:resource ="#Cow"/>
<rdfs:comment>A young Cow, i.e. a Cow that is NonFullyFormed.</rdfs:comment>
</owl:Class>

<owl:Class rdf:ID= "Camera">
<rdfs:subClassOf rdf:resource ="http://127.0.0.1:8000/ontology/SUMO.owl#Device"/>
<rdfs:comment>A Device which is capable of Photographing.</rdfs:comment>
</owl:Class>

<owl:Class rdf:ID= "Campground">
<rdfs:subClassOf rdf:resource 
="http://127.0.0.1:8000/ontology/SUMO.owl#LandArea"/>
<rdfs:comment>A LandArea whose purpose is to have MobileResidences
(e.g. recreational vehicles, mobile homes, Tents, etc.) located 
there.</rdfs:comment>
</owl:Class>

<owl:Class rdf:ID= "Canal">
<rdfs:subClassOf rdf:resource ="#Waterway"/>
<rdfs:subClassOf rdf:resource 
="http://127.0.0.1:8000/ontology/SUMO.owl#StationaryArtifact"/>
<rdfs:comment>Canal is the subclass of Waterways that are
Artifacts constructed for the passage of Ships.</rdfs:comment>
</owl:Class>

<owl:Class rdf:ID= "Candela">
<rdfs:subClassOf rdf:resource 
="http://127.0.0.1:8000/ontology/SUMO.owl#FunctionQuantity"/>
<rdf:type rdf:resource = 
"http://127.0.0.1:8000/ontology/SUMO.owl#SystemeInternationalUnit"/>
<rdfs:comment>SI luminosity intensity measure.  Symbol: cd.
It is one of the base units in SI, and it is currently defined as
follows:  the Candela is the luminous intensity, in a given direction,
of a source that emits monochromatic radiation of frequency 540*10^12
Hertz and that has a radiant intensity in that direction of 1/683
Watt per Steradian.</rdfs:comment>
</owl:Class>

<owl:Class rdf:ID= "Candle">
<rdfs:subClassOf rdf:resource ="#IlluminationDevice"/>
<rdfs:comment>An IlluminationDevice that consists of Wax and a wick,
which is lit with a flame.</rdfs:comment>
</owl:Class>

<owl:Class rdf:ID= "Canyon">
<rdfs:subClassOf rdf:resource ="#LandForm"/>
<rdfs:comment>Canyon is the subclass of LandForms that are
narrow valleys with steep sides, usually created by water 
erosion.</rdfs:comment>
</owl:Class>

<owl:Class rdf:ID= "Capillary">
<rdfs:subClassOf rdf:resource ="#BloodVessel"/>
<rdfs:comment>A very small BloodVessel that connects arterioles
(very small Arteries) with venules (very small Veins).</rdfs:comment>
</owl:Class>

<owl:Class rdf:ID= "CaptainOfficer">
<rdfs:subClassOf rdf:resource ="#MilitaryOfficer"/>
<rdfs:comment>A commissioned MilitaryOfficer who ranks
above a Lieutenant but below a MajorOfficer.</rdfs:comment>
</owl:Class>

<owl:Class rdf:ID= "Carbon">
<rdfs:subClassOf rdf:resource 
="http://127.0.0.1:8000/ontology/SUMO.owl#ElementalSubstance"/>
<atomicNumber>6</atomicNumber>
<rdfs:comment>Carbon is a member of group 14 of the periodic
table.  It has three allotropic forms of it, diamonds, graphite and
fullerite.  Carbon-14 is commonly used in radioactive dating.  Carbon
occurs in all organic life and is the basis of organic chemistry.  Carbon
has the interesting chemical property of being able to bond with itself,
and a wide variety of other elements.</rdfs:comment>
</owl:Class>

<owl:Class rdf:ID= "CareOrganization">
<rdfs:subClassOf rdf:resource 
="http://127.0.0.1:8000/ontology/SUMO.owl#Organization"/>
<rdfs:comment>Any Organization whose purpose is to
provide medical care for for Humans who reside there, either permanently
or temporarily.</rdfs:comment>
</owl:Class>

<owl:Class rdf:ID= "CargoShip">
<rdfs:subClassOf rdf:resource ="#Ship"/>
<rdfs:comment>CargoShip is the subclass of Ships that
transport goods in exchange for payment.  CargoShip includes ships
that carry all kinds of cargo, including oil and bulk products as well
as packaged, palletized, or containerized goods.</rdfs:comment>
</owl:Class>

<owl:Class rdf:ID= "Carpenter">
<rdfs:subClassOf rdf:resource ="#OccupationalTrade"/>
<rdfs:comment>Any occupation that involves creating and repairing
Artifacts that are made chiefly of Wood.</rdfs:comment>
</owl:Class>

<owl:Class rdf:ID= "Catching">
<rdfs:subClassOf rdf:resource 
="http://127.0.0.1:8000/ontology/SUMO.owl#Touching"/>
<rdfs:subClassOf rdf:resource 
="http://127.0.0.1:8000/ontology/SUMO.owl#Maneuver"/>
<rdfs:comment>Any Maneuver in a Game which results in a
situation where the agent grasps the Ball.</rdfs:comment>
</owl:Class>

<owl:Class rdf:ID= "CausingHappiness">
<rdfs:subClassOf rdf:resource 
="http://127.0.0.1:8000/ontology/SUMO.owl#BiologicalProcess"/>
<rdfs:comment>Any Process whose result is that the
patient of the process is happy.</rdfs:comment>
</owl:Class>

<owl:Class rdf:ID= "CausingPain">
<rdfs:subClassOf rdf:resource ="#CausingUnhappiness"/>
<rdfs:comment>Any Process whose result is that the
patient of the process is in Pain.</rdfs:comment>
</owl:Class>

<owl:Class rdf:ID= "CausingUnhappiness">
<rdfs:subClassOf rdf:resource 
="http://127.0.0.1:8000/ontology/SUMO.owl#BiologicalProcess"/>
<rdfs:comment>Any Process whose result is that the
patient of the process is unhappy.</rdfs:comment>
</owl:Class>

<owl:Class rdf:ID= "CavalryUnit">
<rdfs:subClassOf rdf:resource ="#MilitaryUnit"/>
<rdfs:comment>MilitaryUnits composed primarily of Soldiers
who are mounted, i.e. who perform their combat missions from a Horse or
Vehicle.</rdfs:comment>
</owl:Class>

<owl:Class rdf:ID= "Cave">
<rdfs:subClassOf rdf:resource ="http://127.0.0.1:8000/ontology/SUMO.owl#Hole"/>
<rdfs:comment>A large Hole in the earth which can be entered either
from a WaterArea or from the surface of the earth.</rdfs:comment>
</owl:Class>

<owl:Class rdf:ID= "CeasingOperations">
<rdfs:subClassOf rdf:resource 
="http://127.0.0.1:8000/ontology/SUMO.owl#OrganizationalProcess"/>
<rdfs:comment>The process of an Organization
ceasing operations, i.e. its folding or going out of business in
some other fashion.</rdfs:comment>
</owl:Class>

<owl:Class rdf:ID= "Ceiling">
<rdfs:subClassOf rdf:resource 
="http://127.0.0.1:8000/ontology/SUMO.owl#StationaryArtifact"/>
<rdfs:comment>A StationaryArtifact that is the top surface
of a Room.</rdfs:comment>
</owl:Class>

<owl:Class rdf:ID= "CellNucleus">
<rdfs:subClassOf rdf:resource 
="http://127.0.0.1:8000/ontology/SUMO.owl#BodyPart"/>
<rdfs:comment>The part of the Cell that contains DNA and
RNA.</rdfs:comment>
</owl:Class>

<owl:Class rdf:ID= "Cellulose">
<rdfs:subClassOf rdf:resource 
="http://127.0.0.1:8000/ontology/SUMO.owl#PlantSubstance"/>
<rdfs:subClassOf rdf:resource 
="http://127.0.0.1:8000/ontology/SUMO.owl#Carbohydrate"/>
<rdfs:comment>The main component of Plant Tissue.</rdfs:comment>
</owl:Class>

<owl:Class rdf:ID= "Cement">
<rdfs:subClassOf rdf:resource 
="http://127.0.0.1:8000/ontology/SUMO.owl#Mixture"/>
<rdfs:comment>Cement is a subclass of Mixture
whose instances may contain various minerals or ores, prepared by
heating and pulverizing, and used in binding Concrete or in laying
brick or stone.</rdfs:comment>
</owl:Class>

<owl:Class rdf:ID= "Cemetery">
<rdfs:subClassOf rdf:resource 
="http://127.0.0.1:8000/ontology/SUMO.owl#LandArea"/>
<rdfs:comment>A LandArea which is used for burying the dead.</rdfs:comment>
</owl:Class>

<owl:Class rdf:ID= "CentrifugalMotion">
<rdfs:subClassOf rdf:resource ="#Rotating"/>
<sumo:disjoint rdf:resource = "#CentripetalMotion" />
<rdfs:comment>Any instance of Rotating where there is
Motion away from the center of the Rotating.</rdfs:comment>
</owl:Class>

<owl:Class rdf:ID= "CentripetalMotion">
<rdfs:subClassOf rdf:resource ="#Rotating"/>
<rdfs:comment>Any instance of Rotating where there is
Motion towards the center of the Rotating.</rdfs:comment>
</owl:Class>

<owl:Class rdf:ID= "Century">
<rdfs:subClassOf rdf:resource 
="http://127.0.0.1:8000/ontology/SUMO.owl#TimeDuration"/>
<rdf:type rdf:resource = 
"http://127.0.0.1:8000/ontology/SUMO.owl#UnitOfMeasure"/>
<rdfs:comment>The TimeDuration of 100 years.</rdfs:comment>
</owl:Class>

<owl:Class rdf:ID= "CerealGrain">
<rdfs:subClassOf rdf:resource ="http://127.0.0.1:8000/ontology/SUMO.owl#Seed"/>
<rdfs:subClassOf rdf:resource ="http://127.0.0.1:8000/ontology/SUMO.owl#Food"/>
<rdfs:comment>Any Seed which is produced by the cereal grasses,
e.g. rice, corn, wheat, etc.</rdfs:comment>
</owl:Class>

<owl:Class rdf:ID= "Chair">
<rdfs:subClassOf rdf:resource ="#Seat"/>
<rdfs:comment>A Seat that is designed to accommodate a single
Human.  Note that this class includes stools, as well as Seats with
arms and/or backs.</rdfs:comment>
</owl:Class>

<owl:Class rdf:ID= "ChangingClothing">
<rdfs:subClassOf rdf:resource 
="http://127.0.0.1:8000/ontology/SUMO.owl#Transfer"/>
<rdfs:comment>Any instance of a process of
RemovingClothing or PuttingOnClothing.</rdfs:comment>
</owl:Class>

<owl:Class rdf:ID= "Chapter">
<rdfs:subClassOf rdf:resource 
="http://127.0.0.1:8000/ontology/SUMO.owl#Article"/>
<rdfs:comment>A numbered and/or titled section of a Book, which is
typically indicated in a table of contents for the Book.</rdfs:comment>
</owl:Class>

<owl:Class rdf:ID= "ChargingAFee">
<rdfs:subClassOf rdf:resource 
="http://127.0.0.1:8000/ontology/SUMO.owl#FinancialTransaction"/>
<rdfs:comment>An activity of a fee being charged</rdfs:comment>
</owl:Class>

<owl:Class rdf:ID= "Check">
<rdfs:subClassOf rdf:resource 
="http://127.0.0.1:8000/ontology/SUMO.owl#FinancialInstrument"/>
<rdfs:comment>A FinancialInstrument drawn against deposited funds,
to pay a specified amount of money to a specific person upon 
demand.</rdfs:comment>
</owl:Class>

<owl:Class rdf:ID= "CheckingAccount">
<rdfs:subClassOf rdf:resource ="#DepositAccount"/>
<rdfs:comment>A bank account against which the depositor
can draw checks</rdfs:comment>
</owl:Class>

<owl:Class rdf:ID= "ChemicalAcid">
<rdfs:subClassOf rdf:resource 
="http://127.0.0.1:8000/ontology/SUMO.owl#CompoundSubstance"/>
<sumo:disjoint rdf:resource = "#ChemicalBase" />
<rdfs:comment>A bitter CompoundSubstance that is capable of
reacting with a ChemicalBase and forming a ChemicalSalt.</rdfs:comment>
</owl:Class>

<owl:Class rdf:ID= "ChemicalAgent">
<rdfs:subClassOf rdf:resource ="#BiochemicalAgent"/>
<rdfs:subClassOf rdf:resource 
="http://127.0.0.1:8000/ontology/SUMO.owl#CompoundSubstance"/>
<rdfs:subClassOf rdf:resource 
="http://127.0.0.1:8000/ontology/SUMO.owl#BiologicallyActiveSubstance"/>
<sumo:disjoint rdf:resource = 
"http://127.0.0.1:8000/ontology/SUMO.owl#OrganicObject" />
<rdfs:comment>Synthetic compounds that are not an analogue
of anything occurring naturally and that can result in serious burns,
paralysis, and death to Organisms.</rdfs:comment>
</owl:Class>

<owl:Class rdf:ID= "ChemicalBase">
<rdfs:subClassOf rdf:resource 
="http://127.0.0.1:8000/ontology/SUMO.owl#CompoundSubstance"/>
<rdfs:comment>A CompoundSubstance that is capable of
reacting with a ChemicalAcid and forming a ChemicalSalt.</rdfs:comment>
</owl:Class>

<owl:Class rdf:ID= "ChemicalReduction">
<rdfs:subClassOf rdf:resource 
="http://127.0.0.1:8000/ontology/SUMO.owl#ChemicalSynthesis"/>
<sumo:disjoint rdf:resource = "#Oxidation" />
<rdfs:comment>Any ChemicalProcess where Electrons
are added to the substance undergoing the ChemicalProcess.</rdfs:comment>
</owl:Class>

<owl:Class rdf:ID= "ChemicalSalt">
<rdfs:subClassOf rdf:resource 
="http://127.0.0.1:8000/ontology/SUMO.owl#CompoundSubstance"/>
<rdfs:comment>A bitter CompoundSubstance that is formed in a
chemical reaction of a ChemicalBase with a ChemicalAcid.</rdfs:comment>
</owl:Class>

<owl:Class rdf:ID= "ChemicalWeapon">
<rdfs:subClassOf rdf:resource ="#BiochemicalWeapon"/>
<rdfs:comment>Weapons that damage or destroy Organisms by means
of a ChemicalAgent.</rdfs:comment>
</owl:Class>

<owl:Class rdf:ID= "ChestOrCabinet">
<rdfs:subClassOf rdf:resource ="#Furniture"/>
<rdfs:subClassOf rdf:resource ="#Container"/>
<rdfs:comment>Any piece of Furniture which is also a
Container, e.g. a chest of drawers, a memory chest, an armoire, 
etc.</rdfs:comment>
</owl:Class>

<owl:Class rdf:ID= "Chewing">
<rdfs:subClassOf rdf:resource 
="http://127.0.0.1:8000/ontology/SUMO.owl#BodyMotion"/>
<rdfs:comment>Breaking up or mashing Food with one's teeth.</rdfs:comment>
</owl:Class>

<owl:Class rdf:ID= "Chicken">
<rdfs:subClassOf rdf:resource ="http://127.0.0.1:8000/ontology/SUMO.owl#Bird"/>
<rdfs:subClassOf rdf:resource ="#DomesticAnimal"/>
<rdfs:comment>A subclass of Bird that is raised for its meat
and for its eggs.</rdfs:comment>
</owl:Class>

<owl:Class rdf:ID= "ChickenMeat">
<rdfs:subClassOf rdf:resource ="http://127.0.0.1:8000/ontology/SUMO.owl#Meat"/>
<rdfs:comment>Meat that was originally part of a Chicken.</rdfs:comment>
</owl:Class>

<owl:Class rdf:ID= "Chimney">
<rdfs:subClassOf rdf:resource 
="http://127.0.0.1:8000/ontology/SUMO.owl#StationaryArtifact"/>
<rdfs:subClassOf rdf:resource ="http://127.0.0.1:8000/ontology/SUMO.owl#Device"/>
<rdfs:comment>A thin passageway through which Smoke from a controlled
fire is conducted outside of a Building or Room.</rdfs:comment>
</owl:Class>

<owl:Class rdf:ID= "Chin">
<rdfs:subClassOf rdf:resource 
="http://127.0.0.1:8000/ontology/SUMO.owl#AnimalAnatomicalStructure"/>
<rdfs:subClassOf rdf:resource 
="http://127.0.0.1:8000/ontology/SUMO.owl#BodyPart"/>
<rdfs:comment>A part of the Face which protrudes slightly and which
is lower than all other parts of the Face.</rdfs:comment>
</owl:Class>

<owl:Class rdf:ID= "Chlorine">
<rdfs:subClassOf rdf:resource 
="http://127.0.0.1:8000/ontology/SUMO.owl#ElementalSubstance"/>
<atomicNumber>17</atomicNumber>
<rdfs:comment>Halogen element.  Poisonous greenish-yellow gas.
Occurs widely in nature as sodium chloride in seawater.  Reacts directly
with many elements and compounds, strong oxidizing agent.  Discovered by
Karl Scheele in 1774.  Humphrey David confirmed it as an element in
1810.</rdfs:comment>
</owl:Class>

<owl:Class rdf:ID= "Cholesterol">
<rdfs:subClassOf rdf:resource ="#Steroid"/>
<rdfs:subClassOf rdf:resource 
="http://127.0.0.1:8000/ontology/SUMO.owl#AnimalSubstance"/>
<rdfs:comment>A Steroid that is produced by the Liver and that
is believed to be closely associated with various cardiological 
disorders.</rdfs:comment>
</owl:Class>

<owl:Class rdf:ID= "Choreographing">
<rdfs:subClassOf rdf:resource 
="http://127.0.0.1:8000/ontology/SUMO.owl#Planning"/>
<rdfs:comment>Planning that results in a sequence of dance
steps that are executed as part of a Performance.</rdfs:comment>
</owl:Class>

<owl:Class rdf:ID= "ChristianBible">
<rdfs:subClassOf rdf:resource ="http://127.0.0.1:8000/ontology/SUMO.owl#Book"/>
<sumo:subsumesContentClass rdf:resource = "#NewTestament" />
<sumo:subsumesContentClass rdf:resource = "#OldTestament" />
<rdfs:comment>Any instance of the collection of writings which
is regarded as scripture by those who embrace Christianity.</rdfs:comment>
</owl:Class>

<owl:Class rdf:ID= "ChristianGospel">
<rdfs:subClassOf rdf:resource ="http://127.0.0.1:8000/ontology/SUMO.owl#Text"/>
<rdfs:comment>Four books in the New Testament of the
ChristianBible that describe the life and teachings of Jesus Christ
and that are referred to, respectively, as Matthew, Mark, Luke, and 
John.</rdfs:comment>
</owl:Class>

<owl:Class rdf:ID= "ChristianService">
<rdfs:subClassOf rdf:resource ="#ReligiousService"/>
<rdfs:comment>Any ReligiousService that is conducted by
members of Christianity.</rdfs:comment>
</owl:Class>

<owl:Class rdf:ID= "Chromatography">
<rdfs:subClassOf rdf:resource 
="http://127.0.0.1:8000/ontology/SUMO.owl#Separating"/>
<rdfs:comment>Processes of Separating a LiquidMixture or
a GasMixture into some or all of the PureSubstances that comprise 
it.</rdfs:comment>
</owl:Class>

<owl:Class rdf:ID= "Chromium">
<rdfs:subClassOf rdf:resource 
="http://127.0.0.1:8000/ontology/SUMO.owl#ElementalSubstance"/>
<atomicNumber>24</atomicNumber>
<rdfs:comment>Hard silvery transition element.  Used in
decorative electroplating.  Discovered in 1797 by Vauquelin.</rdfs:comment>
</owl:Class>

<owl:Class rdf:ID= "CigarOrCigarette">
<rdfs:subClassOf rdf:resource ="#SmokingDevice"/>
<rdfs:comment>A tube of thin paper containing finely ground
tobacco that is smoked.</rdfs:comment>
</owl:Class>

<owl:Class rdf:ID= "Circle">
<rdfs:subClassOf rdf:resource ="#Oval"/>
<rdfs:comment>The class of Ovals such that all GeometricPoints
that make up the Circle are equidistant from a single GeometricPoint,
known as the center of the Circle.</rdfs:comment>
</owl:Class>

<owl:Class rdf:ID= "CircleSector">
<rdfs:subClassOf rdf:resource 
="http://127.0.0.1:8000/ontology/SUMO.owl#ClosedTwoDimensionalFigure"/>
<rdfs:comment>A slice of a Circle, i.e. any
ClosedTwoDimensionalFigure which consists of two Radii and the arc of
the Circle that they bound.</rdfs:comment>
</owl:Class>

<owl:Class rdf:ID= "CityBlock">
<rdfs:subClassOf rdf:resource 
="http://127.0.0.1:8000/ontology/SUMO.owl#LandArea"/>
<rdfs:comment>A square-shaped area surrounded by Roadways
which is part of a City and typically contains Buildings.</rdfs:comment>
</owl:Class>

<owl:Class rdf:ID= "CityDistrict">
<rdfs:subClassOf rdf:resource 
="http://127.0.0.1:8000/ontology/SUMO.owl#GeopoliticalArea"/>
<rdfs:comment>Any geopoliticalSubdivision of a City.</rdfs:comment>
</owl:Class>

<owl:Class rdf:ID= "CityGovernment">
<rdfs:subClassOf rdf:resource 
="http://127.0.0.1:8000/ontology/SUMO.owl#Government"/>
<rdfs:comment>CityGovernment is the class of
governments of Cities.</rdfs:comment>
</owl:Class>

<owl:Class rdf:ID= "CivilWar">
<rdfs:subClassOf rdf:resource ="http://127.0.0.1:8000/ontology/SUMO.owl#War"/>
<rdfs:comment>A War in which the fighting GeopoliticalAreas
are both part of the same Nation.</rdfs:comment>
</owl:Class>

<owl:Class rdf:ID= "Clamp">
<rdfs:subClassOf rdf:resource 
="http://127.0.0.1:8000/ontology/SUMO.owl#AttachingDevice"/>
<rdfs:comment>An AttachingDevice which is designed to attach
two things together by means of a movable part which can be tightened
or loosened.</rdfs:comment>
</owl:Class>

<owl:Class rdf:ID= "Clapping">
<rdfs:subClassOf rdf:resource ="#HandGesture"/>
<rdfs:subClassOf rdf:resource 
="http://127.0.0.1:8000/ontology/SUMO.owl#RadiatingSound"/>
<rdfs:comment>Bringing the Hands together repeatedly to make
a loud noise.</rdfs:comment>
</owl:Class>

<owl:Class rdf:ID= "Classroom">
<rdfs:subClassOf rdf:resource ="http://127.0.0.1:8000/ontology/SUMO.owl#Room"/>
<rdfs:comment>Any Room in a School where education
takes place.</rdfs:comment>
</owl:Class>

<owl:Class rdf:ID= "Clay">
<rdfs:subClassOf rdf:resource ="#Soil"/>
<rdfs:comment>Fine-grained soil consisting of mineral particles, not
necessarily clay minerals, that are less than 0.002 mm in their maximum 
dimension.</rdfs:comment>
</owl:Class>

<owl:Class rdf:ID= "Cleric">
<rdfs:subClassOf rdf:resource ="#ReligiousPosition"/>
<rdfs:comment>Any Position which involves being in charge of or ministering
to a ReligousOrganization.</rdfs:comment>
</owl:Class>

<owl:Class rdf:ID= "ClericalSecretary">
<rdfs:subClassOf rdf:resource ="#SkilledOccupation"/>
<rdfs:comment>The class of Positions where the position
holder is responsible for clerical duties, e.g. typing documents, answering
phones, keeping schedules, etc.</rdfs:comment>
</owl:Class>

<owl:Class rdf:ID= "ClimateZone">
<rdfs:subClassOf rdf:resource 
="http://127.0.0.1:8000/ontology/SUMO.owl#GeographicArea"/>
<rdfs:comment>ClimateZone is a subclass of GeographicArea in which regions
are classified according to their long-term weather conditions.
The subclasses of ClimateZone are based on the Koeppen Climate
Classification system.  In the Koeppen system, climate zones are
distinguished based on temperatures and rainfall.</rdfs:comment>
</owl:Class>

<owl:Class rdf:ID= "Cloak">
<rdfs:subClassOf rdf:resource 
="http://127.0.0.1:8000/ontology/SUMO.owl#Clothing"/>
<rdfs:comment>A piece of Clothing that covers the whole body
except the face (and possibly entire head), hands, and feet.</rdfs:comment>
</owl:Class>

<owl:Class rdf:ID= "Clock">
<rdfs:subClassOf rdf:resource 
="http://127.0.0.1:8000/ontology/SUMO.owl#MeasuringDevice"/>
<rdfs:comment>Any Device that measures and represents TimeDuration
or TimePosition.</rdfs:comment>
</owl:Class>

<owl:Class rdf:ID= "Closet">
<rdfs:subClassOf rdf:resource ="http://127.0.0.1:8000/ontology/SUMO.owl#Room"/>
<rdfs:comment>A relatively small Room used for storage.</rdfs:comment>
</owl:Class>

<owl:Class rdf:ID= "Closing">
<rdfs:subClassOf rdf:resource ="http://127.0.0.1:8000/ontology/SUMO.owl#Motion"/>
<rdfs:comment>The Class of Processes where an aperture is
closed in an Object.</rdfs:comment>
</owl:Class>

<owl:Class rdf:ID= "ClosingContract">
<rdfs:subClassOf rdf:resource 
="http://127.0.0.1:8000/ontology/SUMO.owl#Committing"/>
<rdfs:comment>Completing a Contract of some sort,
e.g. the purchase of a house, closing a business deal, etc.</rdfs:comment>
</owl:Class>

<owl:Class rdf:ID= "ClosingEyes">
<rdfs:subClassOf rdf:resource ="#EyeMotion"/>
<rdfs:comment>The EyeMotion of tensing the eye lids so that
the corneas are not exposed to light.</rdfs:comment>
</owl:Class>

<owl:Class rdf:ID= "ClothingSuit">
<rdfs:subClassOf rdf:resource 
="http://127.0.0.1:8000/ontology/SUMO.owl#Collection"/>
<rdfs:comment>A Collection of instances of Clothing that
are designed to be worn together.</rdfs:comment>
</owl:Class>

<owl:Class rdf:ID= "Coach">
<rdfs:subClassOf rdf:resource ="#SkilledOccupation"/>
<rdfs:comment>Any occupation that involves training an athlete or a
sports team.</rdfs:comment>
</owl:Class>

<owl:Class rdf:ID= "Coal">
<rdfs:subClassOf rdf:resource ="#FossilFuel"/>
<rdfs:subClassOf rdf:resource ="#OrganicCompound"/>
<rdfs:subClassOf rdf:resource 
="http://127.0.0.1:8000/ontology/SUMO.owl#Mineral"/>
<rdfs:comment>Coal is the class representing brownish-black or
black solid combustible organic substances formed by the decomposition
of vegetable matter, under the influence of moisture, pressure, and
temperature.</rdfs:comment>
</owl:Class>

<owl:Class rdf:ID= "CoastGuard">
<rdfs:subClassOf rdf:resource 
="http://127.0.0.1:8000/ontology/SUMO.owl#PoliceOrganization"/>
<rdfs:comment>CoastGuard is the subclass of GovernmentOrganizations
that enforce the maritime laws of a Nation and guard its Seacoast.  This may 
be
a military or quasi-military organization.</rdfs:comment>
</owl:Class>

<owl:Class rdf:ID= "Coat">
<rdfs:subClassOf rdf:resource ="#OutdoorClothing"/>
<rdfs:comment>Clothing that has sleeves and covers from the neck
down.  Coats are intended to be worn outdoors.</rdfs:comment>
</owl:Class>

<owl:Class rdf:ID= "Coconut">
<rdfs:subClassOf rdf:resource 
="http://127.0.0.1:8000/ontology/SUMO.owl#FruitOrVegetable"/>
<rdfs:subClassOf rdf:resource ="http://127.0.0.1:8000/ontology/SUMO.owl#Food"/>
<rdfs:comment>A FruitOrVegetable that is produced by a type of palm
and has an edible white meat.</rdfs:comment>
</owl:Class>

<owl:Class rdf:ID= "Coffee">
<rdfs:subClassOf rdf:resource 
="http://127.0.0.1:8000/ontology/SUMO.owl#Beverage"/>
<rdfs:subClassOf rdf:resource ="#PreparedFood"/>
<rdfs:comment>A Beverage which is prepared by infusing ground,
roasted coffee beans into hot water.</rdfs:comment>
</owl:Class>

<owl:Class rdf:ID= "Coffin">
<rdfs:subClassOf rdf:resource ="#Container"/>
<rdfs:comment>A Container for a HumanCorpse.</rdfs:comment>
</owl:Class>

<owl:Class rdf:ID= "ColdClimateZone">
<rdfs:subClassOf rdf:resource ="#ClimateZone"/>
<rdfs:comment>ColdClimateZone is the subclass
of ClimateZone that is characterized by a warmest month with average
temperature less than 10 degrees Celsius and a coldest month with
average temperature less than -3 degrees Celsius.  This is Koeppen climate
system Type D.</rdfs:comment>
</owl:Class>

<owl:Class rdf:ID= "ColdDampClimateZone">
<rdfs:subClassOf rdf:resource ="#ColdClimateZone"/>
<rdfs:comment>ColdDampClimateZone is the
subclass of ColdClimateZone that is characterized by having more
than 30 mm of precipitation in the driest month.  This is subtype
'Df' in the Koeppen climate system.</rdfs:comment>
</owl:Class>

<owl:Class rdf:ID= "Collage">
<rdfs:subClassOf rdf:resource 
="http://127.0.0.1:8000/ontology/SUMO.owl#ArtWork"/>
<sumo:disjoint rdf:resource = 
"http://127.0.0.1:8000/ontology/SUMO.owl#RepresentationalArtWork" />
<rdfs:comment>Any abstract ArtWork that is produced by arranging
bits of paper or photographs.</rdfs:comment>
</owl:Class>

<owl:Class rdf:ID= "Collar">
<rdfs:subClassOf rdf:resource 
="http://127.0.0.1:8000/ontology/SUMO.owl#Clothing"/>
<rdfs:comment>A piece of Clothing that fits around the Neck.
A Collar is always part of a Coat or a Shirt.</rdfs:comment>
</owl:Class>

<owl:Class rdf:ID= "College">
<rdfs:subClassOf rdf:resource ="#PostSecondarySchool"/>
<rdfs:comment>A School which admits students who have
graduated from high school and which confers a bachelor's degree,
normally requiring four years of study.  Note that a College does
not confer any graduate degrees.  For institutions that confer both
bachelor's and graduate degrees, the concept University should be
used.</rdfs:comment>
</owl:Class>

<owl:Class rdf:ID= "CollegeFreshman">
<rdfs:subClassOf rdf:resource ="#CollegeStudentPosition"/>
<rdfs:comment>The Positions of a student at a PostSecondarySchool
who has completed less than one year at the school.</rdfs:comment>
</owl:Class>

<owl:Class rdf:ID= "CollegeJunior">
<rdfs:subClassOf rdf:resource ="#CollegeStudentPosition"/>
<rdfs:comment>The Positions of a student at a PostSecondarySchool
who has completed at least two years and less than three years at the 
school.</rdfs:comment>
</owl:Class>

<owl:Class rdf:ID= "CollegeSenior">
<rdfs:subClassOf rdf:resource ="#CollegeStudentPosition"/>
<rdfs:comment>The Positions of a student at a PostSecondarySchool
who has completed at least three years and less than four years at the 
school.</rdfs:comment>
</owl:Class>

<owl:Class rdf:ID= "CollegeSophomore">
<rdfs:subClassOf rdf:resource ="#CollegeStudentPosition"/>
<rdfs:comment>The Positions of a student at a PostSecondarySchool
who has completed at least one year and less than two years at the 
school.</rdfs:comment>
</owl:Class>

<owl:Class rdf:ID= "CollegeStudentPosition">
<rdfs:subClassOf rdf:resource 
="http://127.0.0.1:8000/ontology/SUMO.owl#Position"/>
<rdfs:comment>Any Position at a PostSecondarySchool
which is occupied exclusively by students.</rdfs:comment>
</owl:Class>

<owl:Class rdf:ID= "Colonel">
<rdfs:subClassOf rdf:resource ="#MilitaryOfficer"/>
<rdfs:comment>A commissioned MilitaryOfficer who ranks above
a lieutenant colonel and below a brigadier general.</rdfs:comment>
</owl:Class>

<owl:Class rdf:ID= "Comedian">
<rdfs:subClassOf rdf:resource ="#EntertainmentProfession"/>
<rdfs:comment>Positions which involve performing stand-up comedy, which
is recorded and/or performed in front of live audiences.</rdfs:comment>
</owl:Class>

<owl:Class rdf:ID= "CommercialBuilding">
<rdfs:subClassOf rdf:resource 
="http://127.0.0.1:8000/ontology/SUMO.owl#Building"/>
<rdfs:subClassOf rdf:resource ="#PlaceOfCommerce"/>
<rdfs:comment>A Building which is intended for
organizational activities, e.g. retail or wholesale selling, manufacturing,
office work, etc.</rdfs:comment>
</owl:Class>

<owl:Class rdf:ID= "CommercialShipping">
<rdfs:subClassOf rdf:resource ="#Shipping"/>
<rdfs:subClassOf rdf:resource 
="http://127.0.0.1:8000/ontology/SUMO.owl#CommercialService"/>
<rdfs:comment>CommercialShipping is the subclass of
Transportation events in which a commercial agent provides transportation
of goods for remuneration.</rdfs:comment>
</owl:Class>

<owl:Class rdf:ID= "CommercialUnit">
<rdfs:subClassOf rdf:resource ="#PlaceOfCommerce"/>
<rdfs:comment>A Room or suite of Rooms intended for
clerical and/or professional work of a single Organization.</rdfs:comment>
</owl:Class>

<owl:Class rdf:ID= "Commission">
<rdfs:subClassOf rdf:resource 
="http://127.0.0.1:8000/ontology/SUMO.owl#Organization"/>
<rdfs:comment>A small, temporary Organization whose purpose
is to investigate some issue.</rdfs:comment>
</owl:Class>

<owl:Class rdf:ID= "CommonCarrier">
<rdfs:subClassOf rdf:resource ="#TransportationCompany"/>
<sumo:disjoint rdf:resource = "#ContractCarrier" />
<rdfs:comment>CommonCarrier is the subclass of
TransportationCompany whose instances must offer services to all
customers.  Contrast with ContractCarrier.</rdfs:comment>
</owl:Class>

<owl:Class rdf:about= "Communication">
<sumo:relatedInternalConcept rdf:resource = "#CommunicationDevice" />
</owl:Class>

<owl:Class rdf:ID= "CommunicationDevice">
<rdfs:subClassOf rdf:resource 
="http://127.0.0.1:8000/ontology/SUMO.owl#EngineeringComponent"/>
<rdfs:comment>A CommunicationDevice is a Device
which serves at the instrument in a Communication Process by allowing
the communicated message to be conveyed between the 
participants.</rdfs:comment>
</owl:Class>

<owl:Class rdf:ID= "CommunicationOrganization">
<rdfs:subClassOf rdf:resource 
="http://127.0.0.1:8000/ontology/SUMO.owl#Organization"/>
<rdfs:comment>CommunicationOrganization is
the subclass of Organizations that manage Communications over physical
infrastructure owned or leased by the organization.  Such organizations
may also produce and disseminate information, entertainment, or other
content.  Also see MediaOrganization.</rdfs:comment>
</owl:Class>

<owl:Class rdf:ID= "CommunicationSystem">
<rdfs:subClassOf rdf:resource 
="http://127.0.0.1:8000/ontology/SUMO.owl#Collection"/>
<rdfs:comment>CommunicationSystem is a complex
system with various components, enabling communication (in some
medium) between points in a specific area, whether local or 
worldwide.</rdfs:comment>
</owl:Class>

<owl:Class rdf:ID= "CommunistParty">
<rdfs:subClassOf rdf:resource ="#PoliticalParty"/>
<rdfs:comment>Any PoliticalParty that advocates for a
CommunistState.</rdfs:comment>
</owl:Class>

<owl:Class rdf:ID= "Compartment">
<rdfs:subClassOf rdf:resource ="#Container"/>
<rdfs:comment>A Container which is part of another Container,
e.g. a drawer, a zippered pouch in a piece of luggage, a compartment in a TV
dinner, etc.</rdfs:comment>
</owl:Class>

<owl:Class rdf:ID= "Compass">
<rdfs:subClassOf rdf:resource ="http://127.0.0.1:8000/ontology/SUMO.owl#Device"/>
<rdfs:comment>A Device that indicates the direction of North.</rdfs:comment>
</owl:Class>

<owl:Class rdf:ID= "ComposingMusic">
<rdfs:subClassOf rdf:resource 
="http://127.0.0.1:8000/ontology/SUMO.owl#ContentDevelopment"/>
<rdfs:comment>ContentDevelopment which results in a
MusicalComposition.</rdfs:comment>
</owl:Class>

<owl:Class rdf:ID= "Computer">
<rdfs:subClassOf rdf:resource ="#ElectricDevice"/>
<rdfs:comment>A programmable ElectricDevice that is capable of
processing data.  Note that this class comprises the physical parts of a
computer system, i.e. the machinery and equipment.</rdfs:comment>
</owl:Class>

<owl:Class rdf:ID= "ComputerHardware">
<rdfs:subClassOf rdf:resource 
="http://127.0.0.1:8000/ontology/SUMO.owl#EngineeringComponent"/>
<rdfs:comment>This class covers any component of
a Computer.</rdfs:comment>
</owl:Class>

<owl:Class rdf:ID= "ComputerMemory">
<rdfs:subClassOf rdf:resource ="#ComputerHardware"/>
<rdfs:comment>The computer's workspace (physically,
a collection of RAM chips). It is an important resource, since it
determines the size and number of programs that can be run at the
same time, as well as the amount of data that can be processed
instantly.</rdfs:comment>
</owl:Class>

<owl:Class rdf:ID= "ComputerProcess">
<rdfs:subClassOf rdf:resource 
="http://127.0.0.1:8000/ontology/SUMO.owl#InternalChange"/>
<rdfs:comment>The class of Processes which involve
manipulating data by a Computer.  This covers individual operations
of a Computer as well as complete realizations of 
ComputerPrograms.</rdfs:comment>
</owl:Class>

<owl:Class rdf:ID= "Concealing">
<rdfs:subClassOf rdf:resource 
="http://127.0.0.1:8000/ontology/SUMO.owl#Putting"/>
<rdfs:comment>Locating something in such a way that it cannot
be seen.</rdfs:comment>
</owl:Class>

<owl:Class rdf:ID= "Concentrating">
<rdfs:subClassOf rdf:resource 
="http://127.0.0.1:8000/ontology/SUMO.owl#Removing"/>
<rdfs:comment>Removing a Liquid from a Solution to
increase the concentration of the Solution.</rdfs:comment>
</owl:Class>

<owl:Class rdf:ID= "Concrete">
<rdfs:subClassOf rdf:resource 
="http://127.0.0.1:8000/ontology/SUMO.owl#Mixture"/>
<rdfs:comment>Concrete is a subclass of Mixture
used as building materials.  Concrete is made up of Mineral pieces
(sand or gravel) and a Cement material used to bind them 
together.</rdfs:comment>
</owl:Class>

<owl:Class rdf:ID= "CondominiumBuilding">
<rdfs:subClassOf rdf:resource 
="http://127.0.0.1:8000/ontology/SUMO.owl#ResidentialBuilding"/>
<sumo:disjoint rdf:resource = 
"http://127.0.0.1:8000/ontology/SUMO.owl#SingleFamilyResidence" />
<rdfs:comment>A ResidentialBuilding containing
CondominiumUnits.</rdfs:comment>
</owl:Class>

<owl:Class rdf:ID= "CondominiumUnit">
<rdfs:subClassOf rdf:resource 
="http://127.0.0.1:8000/ontology/SUMO.owl#SingleFamilyResidence"/>
<rdfs:comment>A SingleFamilyResidence that may be owned
by a member of the SocialUnit that lives there.</rdfs:comment>
</owl:Class>

<owl:Class rdf:ID= "Cone">
<rdfs:subClassOf rdf:resource 
="http://127.0.0.1:8000/ontology/SUMO.owl#ThreeDimensionalFigure"/>
<rdfs:comment>The class of ThreeDimensionalFigures which are
produced by rotating a RightTriangle around its RightAngle.</rdfs:comment>
</owl:Class>

<owl:Class rdf:ID= "ConfederateSoldier">
<rdfs:subClassOf rdf:resource ="#Soldier"/>
<rdfs:comment>Any Soldier that served on the confederate side
during the American Civil War.</rdfs:comment>
</owl:Class>

<owl:Class rdf:ID= "Congratulating">
<rdfs:subClassOf rdf:resource ="#ExpressingApproval"/>
<rdfs:comment>Any ExpressingApproval to a person for
something that the person did in the past and that is regarded as being
to the benefit of the person congratulated.</rdfs:comment>
</owl:Class>

<owl:Class rdf:ID= "ConjugatedSubstance">
<rdfs:subClassOf rdf:resource 
="http://127.0.0.1:8000/ontology/SUMO.owl#CompoundSubstance"/>
<rdfs:comment>A CompoundSubstance that results from
the ChemicalSynthesis of two or more CompoundSubstances.</rdfs:comment>
</owl:Class>

<owl:Class rdf:ID= "Consonant">
<rdfs:subClassOf rdf:resource ="#AlphabeticCharacter"/>
<rdfs:comment>An AlphabeticCharacter that denotes a speech sound
that results in audible friction when it is pronounced.</rdfs:comment>
</owl:Class>

<owl:Class rdf:ID= "ConstrictorSnake">
<rdfs:subClassOf rdf:resource ="#Snake"/>
<rdfs:comment>A Snake that lacks venom and kills its
prey by crushing it to death.</rdfs:comment>
</owl:Class>

<owl:Class rdf:ID= "Container">
<rdfs:subClassOf rdf:resource ="#Holder"/>
<rdfs:comment>Any Holder whose purpose is to contain
something else.  Note that Container is more specific in meaning
than Holder, because a Container must have a Hole that is at
least partially filled by the thing contained.</rdfs:comment>
</owl:Class>

<owl:Class rdf:ID= "ContinentalClimateZone">
<rdfs:subClassOf rdf:resource ="#TemperateClimateZone"/>
<rdfs:comment>ContinentalClimateZone is a subclass of TemperateClimateZone 
that is
characterized by cold winters and hot summers.</rdfs:comment>
</owl:Class>

<owl:Class rdf:ID= "ContraceptiveDevice">
<rdfs:subClassOf rdf:resource ="http://127.0.0.1:8000/ontology/SUMO.owl#Device"/>
<rdfs:comment>Devices which permit sexual intercourse but
which reduce the likelihood of conception.</rdfs:comment>
</owl:Class>

<owl:Class rdf:ID= "ContractCarrier">
<rdfs:subClassOf rdf:resource ="#TransportationCompany"/>
<rdfs:comment>ContractCarrier is the subclass of
TransportationCompany whose instances offer services to only one
customer, under contract.  Contrast with CommonCarrier.</rdfs:comment>
</owl:Class>

<owl:Class rdf:ID= "ControlledSubstance">
<rdfs:subClassOf rdf:resource 
="http://127.0.0.1:8000/ontology/SUMO.owl#BiologicallyActiveSubstance"/>
<rdfs:comment>ControlledSubstance is
the subclass of BiologicallyActiveSubstances whose distribution
and use is controlled by government regulation.</rdfs:comment>
</owl:Class>

<owl:Class rdf:ID= "CoolingDevice">
<rdfs:subClassOf rdf:resource ="http://127.0.0.1:8000/ontology/SUMO.owl#Device"/>
<rdfs:comment>A Device whose purpose is Cooling something,
e.g. air conditioners, refrigerators, freezers, etc.</rdfs:comment>
</owl:Class>

<owl:Class rdf:ID= "Copper">
<rdfs:subClassOf rdf:resource 
="http://127.0.0.1:8000/ontology/SUMO.owl#ElementalSubstance"/>
<atomicNumber>29</atomicNumber>
<rdfs:comment>Red-brown transition element.  Known by the Romans
as 'cuprum.' Extracted and used for thousands of years.  Malleable,
ductile and an excellent conductor of heat and electricity.  When in moist
conditions, a greenish layer forms on the outside.</rdfs:comment>
</owl:Class>

<owl:Class rdf:ID= "Copying">
<rdfs:subClassOf rdf:resource ="http://127.0.0.1:8000/ontology/SUMO.owl#Making"/>
<rdfs:comment>Making a copy of something.</rdfs:comment>
</owl:Class>

<owl:Class rdf:ID= "Corn">
<rdfs:subClassOf rdf:resource ="#CerealGrain"/>
<rdfs:comment>A CerealGrain which is found on long ears of a Plant
native to the Americas.</rdfs:comment>
</owl:Class>

<owl:Class rdf:ID= "Coroner">
<rdfs:subClassOf rdf:resource ="#GovernmentOfficer"/>
<rdfs:comment>A GovernmentOfficer who investigates deaths that are
suspected of being due to something other than natural 
causes.</rdfs:comment>
</owl:Class>

<owl:Class rdf:ID= "Corporal">
<rdfs:subClassOf rdf:resource ="#MilitaryOfficer"/>
<rdfs:comment>A noncomissioned MilitaryOfficer.</rdfs:comment>
</owl:Class>

<owl:Class rdf:ID= "Corresponding">
<rdfs:subClassOf rdf:resource 
="http://127.0.0.1:8000/ontology/SUMO.owl#LinguisticCommunication"/>
<rdfs:comment>Instances of LinguisticCommunication which
are achieved by means of Texts that are mailed between the persons
communicating with one another.</rdfs:comment>
</owl:Class>

<owl:Class rdf:ID= "Cotton">
<rdfs:subClassOf rdf:resource 
="http://127.0.0.1:8000/ontology/SUMO.owl#PlantAnatomicalStructure"/>
<rdfs:comment>Fibers from the cotton plant that are used in
Making CottonFabric.</rdfs:comment>
</owl:Class>

<owl:Class rdf:ID= "CottonFabric">
<rdfs:subClassOf rdf:resource ="http://127.0.0.1:8000/ontology/SUMO.owl#Fabric"/>
<rdfs:comment>Any Fabric that is made entirely out of Cotton.</rdfs:comment>
</owl:Class>

<owl:Class rdf:ID= "Coulomb">
<rdfs:subClassOf rdf:resource 
="http://127.0.0.1:8000/ontology/SUMO.owl#TimeDependentQuantity"/>
<rdf:type rdf:resource = 
"http://127.0.0.1:8000/ontology/SUMO.owl#SystemeInternationalUnit"/>
<rdfs:comment>SI electric charge measure.  Symbol: C. It is
the quantity of electric charge transported through a cross section of
a conductor in an electric circuit during each SecondDuration by a
current of 1 Ampere.  Coulomb = s*A.</rdfs:comment>
</owl:Class>

<owl:Class rdf:ID= "County">
<rdfs:subClassOf rdf:resource 
="http://127.0.0.1:8000/ontology/SUMO.owl#GeopoliticalArea"/>
<rdfs:subClassOf rdf:resource 
="http://127.0.0.1:8000/ontology/SUMO.owl#LandArea"/>
<rdfs:comment>A GeopoliticalArea that is a subdivision of a
StateOrProvince.  Aside from City, this is the smallest geopolitical
subdivision, and it is known by various names in various counties, e.g.
parrish, commune, etc.</rdfs:comment>
</owl:Class>

<owl:Class rdf:ID= "CourtRoom">
<rdfs:subClassOf rdf:resource ="http://127.0.0.1:8000/ontology/SUMO.owl#Room"/>
<rdfs:comment>Any Room whose purpose is to realize
JudicialProcesses.</rdfs:comment>
</owl:Class>

<owl:Class rdf:ID= "Cow">
<rdfs:subClassOf rdf:resource 
="http://127.0.0.1:8000/ontology/SUMO.owl#HoofedMammal"/>
<rdfs:subClassOf rdf:resource ="#DomesticAnimal"/>
<rdfs:comment>A domesticated HoofedMammal that is raised for milk
and beef, and is also used for work.</rdfs:comment>
</owl:Class>

<owl:Class rdf:ID= "Crane">
<rdfs:subClassOf rdf:resource ="#MaterialHandlingEquipment"/>
<rdfs:comment>Crane is a subclass of mechanical Devices
that consist of a HoistingDevice on a moveable boom, designed to
assist in moving heavy loads.</rdfs:comment>
</owl:Class>

<owl:Class rdf:ID= "CreditAccount">
<rdfs:subClassOf rdf:resource ="#LiabilityAccount"/>
<rdfs:comment>Credit extended by a business to a customer.</rdfs:comment>
</owl:Class>

<owl:Class rdf:ID= "CreditCardAccount">
<rdfs:subClassOf rdf:resource ="#CreditAccount"/>
<rdfs:comment>A type of CreditAccount which uses a CreditCard for
FinancialTransactions.</rdfs:comment>
</owl:Class>

<owl:Class rdf:ID= "CreditUnion">
<rdfs:subClassOf rdf:resource ="#FinancialCompany"/>
<rdfs:comment>Credit unions are non-profit, member-owned,
financial cooperatives. They are operated entirely by and for their
members. When money is deposited in a credit union, the depositor
becomes a member of the union because the deposit is considered partial
ownership in the credit union. Many large organizations have established
credit unions for their employees.</rdfs:comment>
</owl:Class>

<owl:Class rdf:ID= "Creek">
<rdfs:subClassOf rdf:resource ="#BodyOfWater"/>
<rdfs:subClassOf rdf:resource 
="http://127.0.0.1:8000/ontology/SUMO.owl#StreamWaterArea"/>
<rdfs:subClassOf rdf:resource 
="http://127.0.0.1:8000/ontology/SUMO.owl#FreshWaterArea"/>
<sumo:disjoint rdf:resource = "#River" />
<rdfs:comment>Creek is the class of small streams of fresh
water flowing through land, usually into a River.</rdfs:comment>
</owl:Class>

<owl:Class rdf:ID= "CreoleLanguage">
<rdfs:subClassOf rdf:resource 
="http://127.0.0.1:8000/ontology/SUMO.owl#SpokenHumanLanguage"/>
<rdfs:comment>A CreoleLanguage is a PidginLanguage that
has developed and become the mother tongue for a community of people. This
process is called 'creolization' and results in an expanded vocabulary and
grammar structure that allow for communication as rich and complex as that 
of
non-creole languages. While pidgins are regarded as reduced languages, 
creoles
are considered expanded languages. That is, while pidgins develop to enable
communication in relatively isolated domains, creoles allow for a full range
of expressive possibilities on a par with more 'recognized' 
languages.</rdfs:comment>
</owl:Class>

<owl:Class rdf:ID= "CriminalAction">
<rdfs:subClassOf rdf:resource 
="http://127.0.0.1:8000/ontology/SUMO.owl#IntentionalProcess"/>
<rdfs:comment>Any IntentionalProcess that violates a Law.</rdfs:comment>
</owl:Class>

<owl:Class rdf:ID= "CriminalGang">
<rdfs:subClassOf rdf:resource 
="http://127.0.0.1:8000/ontology/SUMO.owl#GroupOfPeople"/>
<rdfs:comment>A GroupOfPeople which exists (partially or
wholly) for the purpose of CriminalAction.</rdfs:comment>
</owl:Class>

<owl:Class rdf:ID= "CubicFoot">
<rdf:type rdf:resource = 
"http://127.0.0.1:8000/ontology/SUMO.owl#UnitOfMeasure"/>
<rdfs:subClassOf rdf:resource 
="http://127.0.0.1:8000/ontology/SUMO.owl#VolumeMeasure"/>
<rdfs:comment>CubicFoot is a unit for measuring volume,
equal to a volume of one foot length in each dimension of length, width,
and height.</rdfs:comment>
</owl:Class>

<owl:Class rdf:ID= "CultivatedLandArea">
<rdfs:subClassOf rdf:resource 
="http://127.0.0.1:8000/ontology/SUMO.owl#LandArea"/>
<rdfs:comment>A LandArea which is dedicated to
Agriculture, e.g. Lawns, gardens, and fields for growing 
crops.</rdfs:comment>
</owl:Class>

<owl:Class rdf:about= "Cup">
<rdfs:subClassOf rdf:resource ="#FluidContainer"/>
<rdfs:comment>An open FluidContainer that is intended to serve a
Beverage to a single person.  Note that this class includes both cups
with handles and drinking glasses.</rdfs:comment>
</owl:Class>

<owl:Class rdf:ID= "Curb">
<rdfs:subClassOf rdf:resource 
="http://127.0.0.1:8000/ontology/SUMO.owl#StationaryArtifact"/>
<rdfs:comment>A raised concrete or asphalt structure that connects a
Sidewalk with a Roadway.</rdfs:comment>
</owl:Class>

<owl:Class rdf:ID= "Curtain">
<rdfs:subClassOf rdf:resource ="#WindowCovering"/>
<rdfs:subClassOf rdf:resource ="#FabricArtifact"/>
<rdfs:comment>A piece of Fabric whose purpose is Covering a
Window so as to keep out the light or prevent people from seeing 
inside.</rdfs:comment>
</owl:Class>

<owl:Class rdf:ID= "CuttingDevice">
<rdfs:subClassOf rdf:resource ="http://127.0.0.1:8000/ontology/SUMO.owl#Device"/>
<rdfs:comment>Any Device whose purpose is Cutting something
else.  This class covers knives of all times, axes, saws, razors, chisels 
etc.</rdfs:comment>
</owl:Class>

<owl:Class rdf:ID= "Cycle-TransportationDevice">
<rdfs:subClassOf rdf:resource ="#LandVehicle"/>
<rdfs:subClassOf rdf:resource ="#UserPoweredDevice"/>
<rdfs:comment>Cycle-TransportationDevice
is a class of wheeled, pedal-driven UserPoweredVehicles that are
designed to be ridden on roads or trails.</rdfs:comment>
</owl:Class>

<owl:Class rdf:ID= "Cylinder">
<rdfs:subClassOf rdf:resource 
="http://127.0.0.1:8000/ontology/SUMO.owl#ThreeDimensionalFigure"/>
<rdfs:comment>The class of ThreeDimensionalFigures such that
all GeometricPoints that make up the Cylinder are equidistant from a
OneDimensionalFigure, known as the axis of the Cylinder.</rdfs:comment>
</owl:Class>

<owl:Class rdf:ID= "Dam">
<rdfs:subClassOf rdf:resource 
="http://127.0.0.1:8000/ontology/SUMO.owl#StationaryArtifact"/>
<rdfs:comment>Dam is the subclass of StationaryArtifacts that
are walls built across a stream or river to hold back water.</rdfs:comment>
</owl:Class>

<owl:Class rdf:ID= "Dancing">
<rdfs:subClassOf rdf:resource 
="http://127.0.0.1:8000/ontology/SUMO.owl#BodyMotion"/>
<rdfs:comment>Any BodyMotion of Humans which is
deliberately coordinated with music.</rdfs:comment>
</owl:Class>

<owl:Class rdf:ID= "DateFruit">
<rdfs:subClassOf rdf:resource 
="http://127.0.0.1:8000/ontology/SUMO.owl#FruitOrVegetable"/>
<rdfs:subClassOf rdf:resource ="http://127.0.0.1:8000/ontology/SUMO.owl#Food"/>
<rdfs:comment>A FruitOrVegetable that is produced by the date
palm.</rdfs:comment>
</owl:Class>

<owl:Class rdf:ID= "DaySchool">
<rdfs:subClassOf rdf:resource ="#School"/>
<rdfs:comment>A School that does not board its students, i.e.
students attend classes during the day and then return to a private 
residence
for the night.</rdfs:comment>
</owl:Class>

<owl:Class rdf:ID= "DayTime">
<rdfs:subClassOf rdf:resource 
="http://127.0.0.1:8000/ontology/SUMO.owl#TimeInterval"/>
<rdfs:comment>The class of TimeIntervals that begin at Sunrise
and end at Sunset.</rdfs:comment>
</owl:Class>

<owl:Class rdf:ID= "Deacon">
<rdfs:subClassOf rdf:resource ="#ReligiousPosition"/>
<rdfs:subClassOf rdf:resource ="#PartTimePosition"/>
<rdfs:comment>Any Position within a ReligiousOrganization that is held
by a layman, which is part-time, and which involves assisting a 
Cleric.</rdfs:comment>
</owl:Class>

<owl:Class rdf:ID= "DeafSignLanguage">
<rdfs:subClassOf rdf:resource 
="http://127.0.0.1:8000/ontology/SUMO.owl#ManualHumanLanguage"/>
<rdfs:comment>A DeafSignLanguage is a
ManualHumanLanguage primarily intended for communication between a
deaf individual and a hearing individual or between deaf 
individuals.</rdfs:comment>
</owl:Class>

<owl:Class rdf:ID= "Debating">
<rdfs:subClassOf rdf:resource 
="http://127.0.0.1:8000/ontology/SUMO.owl#Contest"/>
<rdfs:subClassOf rdf:resource 
="http://127.0.0.1:8000/ontology/SUMO.owl#LinguisticCommunication"/>
<rdfs:comment>A Contest where each participant holds a different
view regarding some issue, and each participant attempts to prove, by
rhetoric or evidence, that his/her own views about a particular matter are
correct and/or that the views of the other participants are 
incorrect.</rdfs:comment>
</owl:Class>

<owl:Class rdf:ID= "Deboarding">
<rdfs:subClassOf rdf:resource 
="http://127.0.0.1:8000/ontology/SUMO.owl#Translocation"/>
<rdfs:comment>Getting off a Vehicle, e.g. getting out of an
Automobile, deplaning, getting off a Watercraft, etc.</rdfs:comment>
</owl:Class>

<owl:Class rdf:ID= "Decade">
<rdfs:subClassOf rdf:resource 
="http://127.0.0.1:8000/ontology/SUMO.owl#TimeDuration"/>
<rdf:type rdf:resource = 
"http://127.0.0.1:8000/ontology/SUMO.owl#UnitOfMeasure"/>
<rdfs:comment>The TimeDuration of 10 years.</rdfs:comment>
</owl:Class>

<owl:Class rdf:ID= "Decelerating">
<rdfs:subClassOf rdf:resource 
="http://127.0.0.1:8000/ontology/SUMO.owl#Translocation"/>
<rdfs:subClassOf rdf:resource 
="http://127.0.0.1:8000/ontology/SUMO.owl#Decreasing"/>
<rdfs:comment>Decreasing the speed with which someone
or something is moving.</rdfs:comment>
</owl:Class>

<owl:Class rdf:ID= "DefinedContributionPlan">
<rdfs:subClassOf rdf:resource ="#PensionPlan"/>
<rdfs:comment>A company retirement plan, such as
a 401(k) or 403(b), in which the employee elects to defer some amount of
his/her salary into the plan and bears the investment risk.</rdfs:comment>
</owl:Class>

<owl:Class rdf:ID= "Dentist">
<rdfs:subClassOf rdf:resource ="#Profession"/>
<rdfs:comment>The Profession of being a dentist, i.e. diagnosing
and treating problems related to the teeth.</rdfs:comment>
</owl:Class>

<owl:Class rdf:ID= "DependencyOrSpecialSovereigntyArea">
<rdfs:subClassOf rdf:resource 
="http://127.0.0.1:8000/ontology/SUMO.owl#GeopoliticalArea"/>
<rdfs:comment>DependencyOrSpecialSovereigntyArea
is a subclass of GeopoliticalArea, representing the classification 
'Dependency or
Special Sovereignty Area' used by the CIA World Fact Book.</rdfs:comment>
</owl:Class>

<owl:Class rdf:ID= "Deposit">
<rdfs:subClassOf rdf:resource 
="http://127.0.0.1:8000/ontology/SUMO.owl#FinancialTransaction"/>
<sumo:disjoint rdf:resource = "#Withdrawal" />
<rdfs:comment>An Activity of money being transferred into a customer's
account at a financial institution.</rdfs:comment>
</owl:Class>

<owl:Class rdf:ID= "DepositAccount">
<rdfs:subClassOf rdf:resource ="#FinancialAccount"/>
<rdfs:comment>An account where money is deposited for checking,
savings or brokerage use.</rdfs:comment>
</owl:Class>

<owl:Class rdf:ID= "DepositingACheck">
<rdfs:subClassOf rdf:resource ="#UsingAnAccount"/>
<rdfs:comment>An activity of depositing a check into a
FinancialCompany.</rdfs:comment>
</owl:Class>

<owl:Class rdf:ID= "Depressant">
<rdfs:subClassOf rdf:resource 
="http://127.0.0.1:8000/ontology/SUMO.owl#BiologicallyActiveSubstance"/>
<rdfs:comment>Any BiologicallyActiveSubstance which has
the effect of depressing the central nervous system, i.e. decreasing
function or activity in the Brain or SpinalCord.</rdfs:comment>
</owl:Class>

<owl:Class rdf:ID= "Deputy">
<rdfs:subClassOf rdf:resource ="#PoliceOfficer"/>
<rdfs:comment>A Position which authorizes the holder of the position
to act as the sheriff when the sheriff is not available.</rdfs:comment>
</owl:Class>

<owl:Class rdf:ID= "DesertClimateZone">
<rdfs:subClassOf rdf:resource ="#AridClimateZone"/>
<rdfs:comment>DesertClimateZone
is the class of AridClimateZones characterized by
sparse, desert vegetation.  Koeppen system 'BW'.</rdfs:comment>
</owl:Class>

<owl:Class rdf:ID= "Desk">
<rdfs:subClassOf rdf:resource ="#Table"/>
<rdfs:comment>A Table for a single person which is intended to be
used for paperwork.</rdfs:comment>
</owl:Class>

<owl:Class rdf:ID= "Detergent">
<rdfs:subClassOf rdf:resource 
="http://127.0.0.1:8000/ontology/SUMO.owl#Mixture"/>
<rdfs:comment>Any Mixture whose purpose is to remove Soil
and/or other undesirable substances from the surfaces of 
objects.</rdfs:comment>
</owl:Class>

<owl:Class rdf:ID= "DeviceAttribute">
<rdfs:subClassOf rdf:resource 
="http://127.0.0.1:8000/ontology/SUMO.owl#ObjectiveNorm"/>
<rdfs:comment>This class contains Attributes that
are specific to the functioning of Devices.</rdfs:comment>
</owl:Class>

<owl:Class rdf:ID= "DeviceStateAttribute">
<rdfs:subClassOf rdf:resource ="#DeviceAttribute"/>
<rdfs:comment>DeviceStateAttribute is the class
of attributes that represent different states that a Device may be in.
Examples: DeviceOff, DeviceOn, DeviceOpen, and DeviceClosed.</rdfs:comment>
</owl:Class>

<owl:Class rdf:ID= "Dialysis">
<rdfs:subClassOf rdf:resource 
="http://127.0.0.1:8000/ontology/SUMO.owl#Separating"/>
<rdfs:comment>Any process of Separating a Solution into two or more
constituent PureSubstances by means of their unequal diffusion through 
membranes
that are partially permeable.</rdfs:comment>
</owl:Class>

<owl:Class rdf:ID= "Diamond">
<rdfs:subClassOf rdf:resource 
="http://127.0.0.1:8000/ontology/SUMO.owl#Mineral"/>
<rdfs:subClassOf rdf:resource ="#Carbon"/>
<rdfs:comment>Crystalline Carbon that is valued as a gem and
used in industrial applications.</rdfs:comment>
</owl:Class>

<owl:Class rdf:ID= "Dictionary">
<rdfs:subClassOf rdf:resource ="#ReferenceText"/>
<rdfs:comment>A ReferenceText which specifies the meanings
of the Words of a Language or of a technical jargon.</rdfs:comment>
</owl:Class>

<owl:Class rdf:ID= "DieselEngine">
<rdfs:subClassOf rdf:resource ="#InternalCombustionEngine"/>
<rdfs:comment>DieselEngine is the subclass of
InternalCombustionEngines that use DieselFuel as their 
resource.</rdfs:comment>
</owl:Class>

<owl:Class rdf:ID= "DieselFuel">
<rdfs:subClassOf rdf:resource ="#RefinedPetroleumProduct"/>
<rdfs:subClassOf rdf:resource ="#FossilFuel"/>
<rdfs:comment>DieselFuel is the subclass of
RefinedPetroleumProducts that are fuels for diesel engines.</rdfs:comment>
</owl:Class>

<owl:Class rdf:ID= "Diet">
<rdfs:subClassOf rdf:resource ="http://127.0.0.1:8000/ontology/SUMO.owl#Plan"/>
<rdfs:comment>A Plan regarding what one is allowed to eat.</rdfs:comment>
</owl:Class>

<owl:Class rdf:ID= "Digging">
<rdfs:subClassOf rdf:resource 
="http://127.0.0.1:8000/ontology/SUMO.owl#IntentionalProcess"/>
<rdfs:subClassOf rdf:resource 
="http://127.0.0.1:8000/ontology/SUMO.owl#SurfaceChange"/>
<rdfs:comment>Any Process of removing or turning over the 
Soil.</rdfs:comment>
</owl:Class>

<owl:Class rdf:ID= "DigitAppendage">
<rdfs:subClassOf rdf:resource 
="http://127.0.0.1:8000/ontology/SUMO.owl#AnimalAnatomicalStructure"/>
<rdfs:subClassOf rdf:resource 
="http://127.0.0.1:8000/ontology/SUMO.owl#BodyPart"/>
<rdfs:comment>Any of the extremities of Limbs that are
found in the higer Vertebrates and the Amphibians.</rdfs:comment>
</owl:Class>

<owl:Class rdf:ID= "DigitCharacter">
<rdfs:subClassOf rdf:resource 
="http://127.0.0.1:8000/ontology/SUMO.owl#Character"/>
<sumo:disjoint rdf:resource = "#AlphabeticCharacter" />
<rdfs:comment>Any Character that is comprised of a single digit,
i.e. one of the numerals 0, 1, 2, 3, 4, 5, 6, 7, 8, 9.</rdfs:comment>
</owl:Class>

<owl:Class rdf:ID= "Diluting">
<rdfs:subClassOf rdf:resource 
="http://127.0.0.1:8000/ontology/SUMO.owl#Putting"/>
<rdfs:comment>Adding a Liquid to a Solution to decrease
the concentration of the Solution.</rdfs:comment>
</owl:Class>

<owl:Class rdf:ID= "DiningRoom">
<rdfs:subClassOf rdf:resource ="http://127.0.0.1:8000/ontology/SUMO.owl#Room"/>
<rdfs:comment>A Room intended primarily for Eating.</rdfs:comment>
</owl:Class>

<owl:Class rdf:ID= "DiplomaticAgent">
<rdfs:subClassOf rdf:resource ="#ForeignServicePosition"/>
<rdfs:comment>DiplomaticAgent is the class of Positions
where one is charged to represent one national government to another nation
or international organization.  This includes any Ambassador or head of
a diplomatic mission.  Individuals with this attribute may also hold a
career diplomatic position (see ForeignServicePosition).</rdfs:comment>
</owl:Class>

<owl:Class rdf:ID= "DirectedGraph">
<rdfs:subClassOf rdf:resource ="#Graph"/>
<rdfs:comment>The Class of directed graphs.  A
directed graph is a Graph in which all GraphArcs
have direction, i.e. every GraphArc has an initial node (see
InitialNodeFn) and a terminal node (see TerminalNodeFn).</rdfs:comment>
</owl:Class>

<owl:Class rdf:ID= "Dish">
<rdfs:subClassOf rdf:resource ="#Holder"/>
<rdfs:comment>A Holder for Food while the Food is being 
eaten.</rdfs:comment>
</owl:Class>

<owl:Class rdf:ID= "Dismounting">
<rdfs:subClassOf rdf:resource 
="http://127.0.0.1:8000/ontology/SUMO.owl#BodyMotion"/>
<rdfs:comment>Any BodyMotion which results in not being On
something else.</rdfs:comment>
</owl:Class>

<owl:Class rdf:ID= "DisplacementHullWatercraft">
<rdfs:subClassOf rdf:resource ="#Watercraft"/>
<sumo:disjoint rdf:resource = "#PlaningHullWatercraft" />
<rdfs:comment>DisplacementHullWatercraft is
a subclass of Watercraft with hulls designed to move water aside as they
move through the water.  Contrast with PlaningHullWatercraft.</rdfs:comment>
</owl:Class>

<owl:Class rdf:ID= "DisplayArtifact">
<rdfs:subClassOf rdf:resource 
="http://127.0.0.1:8000/ontology/SUMO.owl#Artifact"/>
<rdfs:comment>Something for posting content so
that it can be disseminated to the public.</rdfs:comment>
</owl:Class>

<owl:Class rdf:ID= "DistilledAlcoholicBeverage">
<rdfs:subClassOf rdf:resource ="#AlcoholicBeverage"/>
<rdfs:comment>An AlcoholicBeverage that has
had some part of its Water content removed by distillation.  This class
covers drinks of unmixed, hard liquor.</rdfs:comment>
</owl:Class>

<owl:Class rdf:ID= "Divorcing">
<rdfs:subClassOf rdf:resource 
="http://127.0.0.1:8000/ontology/SUMO.owl#Declaring"/>
<rdfs:comment>A legal act whereby a marriage is dissolved.</rdfs:comment>
</owl:Class>

<owl:Class rdf:ID= "Documentary">
<rdfs:subClassOf rdf:resource ="#MotionPicture"/>
<rdfs:subClassOf rdf:resource 
="http://127.0.0.1:8000/ontology/SUMO.owl#FactualText"/>
<rdfs:comment>A MotionPicture which purports to represent the
facts about a person, event, etc.</rdfs:comment>
</owl:Class>

<owl:Class rdf:ID= "Dodging">
<rdfs:subClassOf rdf:resource 
="http://127.0.0.1:8000/ontology/SUMO.owl#BodyMotion"/>
<rdfs:subClassOf rdf:resource 
="http://127.0.0.1:8000/ontology/SUMO.owl#IntentionalProcess"/>
<rdfs:comment>Purposely moving one's body in such a way as
to avoid being hit by something.</rdfs:comment>
</owl:Class>

<owl:Class rdf:ID= "DomesticAnimal">
<rdfs:subClassOf rdf:resource ="http://127.0.0.1:8000/ontology/SUMO.owl#Animal"/>
<sumo:disjoint rdf:resource = "http://127.0.0.1:8000/ontology/SUMO.owl#Human" />
<rdfs:comment>Any Animal that is kept by a Human, as
a pet, as livestock, for exhibition, etc.</rdfs:comment>
</owl:Class>

<owl:Class rdf:ID= "DomesticCat">
<rdfs:subClassOf rdf:resource ="#DomesticAnimal"/>
<rdfs:subClassOf rdf:resource ="http://127.0.0.1:8000/ontology/SUMO.owl#Feline"/>
<rdfs:comment>A variety of Feline which has been domesticated
by selective breeding.</rdfs:comment>
</owl:Class>

<owl:Class rdf:ID= "DomesticDog">
<rdfs:subClassOf rdf:resource ="#DomesticAnimal"/>
<rdfs:subClassOf rdf:resource ="http://127.0.0.1:8000/ontology/SUMO.owl#Canine"/>
<rdfs:comment>Canines which have evolved from the common
wolf by selective breeding.</rdfs:comment>
</owl:Class>

<owl:Class rdf:ID= "Donkey">
<rdfs:subClassOf rdf:resource 
="http://127.0.0.1:8000/ontology/SUMO.owl#HoofedMammal"/>
<rdfs:subClassOf rdf:resource ="#DomesticAnimal"/>
<rdfs:comment>A domesticated HoofedMammal that is used for
work.</rdfs:comment>
</owl:Class>

<owl:Class rdf:ID= "Door">
<rdfs:subClassOf rdf:resource 
="http://127.0.0.1:8000/ontology/SUMO.owl#Artifact"/>
<rdfs:comment>An Artifact that restricts and permits access to a
StationaryArtifact (e.g. Building or Room) depending on whether the
Door is open or locked.  Note that the class Door also covers gates,
because it is not possible to define objective criteria that reliably
distinguish doors from gates.</rdfs:comment>
</owl:Class>

<owl:Class rdf:ID= "Doorway">
<rdfs:subClassOf rdf:resource 
="http://127.0.0.1:8000/ontology/SUMO.owl#StationaryArtifact"/>
<rdfs:comment>A StationaryArtifact consisting of a frame that
holds a Door.</rdfs:comment>
</owl:Class>

<owl:Class rdf:ID= "Dormitory">
<rdfs:subClassOf rdf:resource 
="http://127.0.0.1:8000/ontology/SUMO.owl#ResidentialBuilding"/>
<rdfs:subClassOf rdf:resource 
="http://127.0.0.1:8000/ontology/SUMO.owl#TemporaryResidence"/>
<sumo:disjoint rdf:resource = 
"http://127.0.0.1:8000/ontology/SUMO.owl#SingleFamilyResidence" />
<rdfs:comment>A TemporaryResidence which is owned by a School
and which is used to house students while they take classes at the 
School.</rdfs:comment>
</owl:Class>

<owl:Class rdf:ID= "Dough">
<rdfs:subClassOf rdf:resource ="#PreparedFood"/>
<rdfs:subClassOf rdf:resource 
="http://127.0.0.1:8000/ontology/SUMO.owl#Mixture"/>
<rdfs:comment>A Mixture of Flour, Water, etc. which is used in
making BreadOrBiscuits.</rdfs:comment>
</owl:Class>

<owl:Class rdf:ID= "Downtown">
<rdfs:subClassOf rdf:resource ="#CityDistrict"/>
<rdfs:comment>The commercial center of a City.  The part of the
City that contains more shops and offices than any other 
part.</rdfs:comment>
</owl:Class>

<owl:Class rdf:ID= "DramaticActing">
<rdfs:subClassOf rdf:resource 
="http://127.0.0.1:8000/ontology/SUMO.owl#Pretending"/>
<rdfs:comment>Playing a character in a Performance,
MotionPicture, etc.</rdfs:comment>
</owl:Class>

<owl:Class rdf:ID= "DramaticCast">
<rdfs:subClassOf rdf:resource 
="http://127.0.0.1:8000/ontology/SUMO.owl#GroupOfPeople"/>
<rdfs:comment>The GroupOfPeople who engage in DramaticActing
as part of the realization of a single FictionalText.</rdfs:comment>
</owl:Class>

<owl:Class rdf:ID= "DramaticDirecting">
<rdfs:subClassOf rdf:resource 
="http://127.0.0.1:8000/ontology/SUMO.owl#Guiding"/>
<rdfs:comment>The process of directing a DramaticActing
in a MotionPicture or the Performance of a DramaticPlay.</rdfs:comment>
</owl:Class>

<owl:Class rdf:ID= "DramaticPerformance">
<rdfs:subClassOf rdf:resource ="#Performance"/>
<rdfs:comment>A Performance that consists exclusively of
DramaticActing, e.g. a live performance of Death_of_a_Salesman in front
of an audience.</rdfs:comment>
</owl:Class>

<owl:Class rdf:ID= "DramaticPlay">
<rdfs:subClassOf rdf:resource 
="http://127.0.0.1:8000/ontology/SUMO.owl#FictionalText"/>
<rdfs:comment>A FictionalText that is intended to be realized
as DramaticActing.</rdfs:comment>
</owl:Class>

<owl:Class rdf:ID= "Drawing">
<rdfs:subClassOf rdf:resource 
="http://127.0.0.1:8000/ontology/SUMO.owl#ContentDevelopment"/>
<rdfs:subClassOf rdf:resource 
="http://127.0.0.1:8000/ontology/SUMO.owl#SurfaceChange"/>
<rdfs:comment>Any ContentDevelopment that results in a 
Sketch.</rdfs:comment>
</owl:Class>

<owl:Class rdf:ID= "DrawingACheck">
<rdfs:subClassOf rdf:resource ="#UsingAnAccount"/>
<rdfs:comment>An activity of paying by a check.</rdfs:comment>
</owl:Class>

<owl:Class rdf:ID= "Dreaming">
<rdfs:subClassOf rdf:resource ="#Imagining"/>
<sumo:disjoint rdf:resource = 
"http://127.0.0.1:8000/ontology/SUMO.owl#IntentionalProcess" />
<rdfs:comment>A Process of producing metal images which occurs
while one is Asleep.</rdfs:comment>
</owl:Class>

<owl:Class rdf:ID= "Dress">
<rdfs:subClassOf rdf:resource 
="http://127.0.0.1:8000/ontology/SUMO.owl#Clothing"/>
<rdfs:comment>An item of Clothing which covers the lower body
(and possibly torso) of a Woman.</rdfs:comment>
</owl:Class>

<owl:Class rdf:ID= "DressingRoom">
<rdfs:subClassOf rdf:resource ="http://127.0.0.1:8000/ontology/SUMO.owl#Room"/>
<rdfs:comment>Any Room which is intended for
ChangingClothing.</rdfs:comment>
</owl:Class>

<owl:Class rdf:ID= "Drilling">
<rdfs:subClassOf rdf:resource 
="http://127.0.0.1:8000/ontology/SUMO.owl#IntentionalProcess"/>
<rdfs:subClassOf rdf:resource 
="http://127.0.0.1:8000/ontology/SUMO.owl#SurfaceChange"/>
<rdfs:comment>Any Process of producing a hole in a
SelfConnectedObject which involves rotating a long, thin bit.</rdfs:comment>
</owl:Class>

<owl:Class rdf:ID= "Dripping">
<rdfs:subClassOf rdf:resource 
="http://127.0.0.1:8000/ontology/SUMO.owl#LiquidMotion"/>
<rdfs:comment>Any LiquidMotion where the Liquid is moved
drop by drop.</rdfs:comment>
</owl:Class>

<owl:Class rdf:ID= "DriveComponent">
<rdfs:subClassOf rdf:resource 
="http://127.0.0.1:8000/ontology/SUMO.owl#EngineeringComponent"/>
<rdfs:comment>An EngineeringComponent whose purpose is to
transfer force from one part of a Device to another part.</rdfs:comment>
</owl:Class>

<owl:Class rdf:ID= "DriversLicense">
<rdfs:subClassOf rdf:resource ="#License"/>
<rdfs:comment>A License which identifies the holder and
indicates that he has the right to drive a certain class of 
RoadVehicle.</rdfs:comment>
</owl:Class>

<owl:Class rdf:ID= "Driveway">
<rdfs:subClassOf rdf:resource 
="http://127.0.0.1:8000/ontology/SUMO.owl#Roadway"/>
<rdfs:comment>A small, private Roadway that is used for parking
Automobiles or for connecting a Garage to a public Roadway.</rdfs:comment>
</owl:Class>

<owl:Class rdf:ID= "Drought">
<rdfs:subClassOf rdf:resource 
="http://127.0.0.1:8000/ontology/SUMO.owl#WeatherProcess"/>
<rdfs:comment>Drought is the subclass of WeatherProcess
that represents long periods without precipitation, which is damaging
to crops, livestock, and human life.</rdfs:comment>
</owl:Class>

<owl:Class rdf:ID= "DrugStore">
<rdfs:subClassOf rdf:resource ="#RetailStore"/>
<rdfs:comment>A RetailStore that sells Medicine, and
perhaps other items as well.</rdfs:comment>
</owl:Class>

<owl:Class rdf:ID= "Drum">
<rdfs:subClassOf rdf:resource ="#PercussionInstrument"/>
<rdfs:comment>An atonal PercussionInstrument which consists of a
hollow cylinder and a fabric stretched across at least one end of the
cylinder.</rdfs:comment>
</owl:Class>

<owl:Class rdf:ID= "DryWinterColdClimateZone">
<rdfs:subClassOf rdf:resource ="#ColdClimateZone"/>
<rdfs:comment>DryWinterColdClimateZone
is a subclass of ColdClimateZone that is characterized by having
at least ten times as much precipitation in the wettest summer month
as in the driest winter month.  This is Koeppen climate system subtype
'Dw'.</rdfs:comment>
</owl:Class>

<owl:Class rdf:ID= "Duck">
<rdfs:subClassOf rdf:resource ="http://127.0.0.1:8000/ontology/SUMO.owl#Bird"/>
<rdfs:comment>A subclass of Bird with webbed feet and a large bill.
Some ducks live in the wild, and some are raised for meat and/or 
eggs.</rdfs:comment>
</owl:Class>

<owl:Class rdf:ID= "DutyTax">
<rdfs:subClassOf rdf:resource ="#Tax"/>
<rdfs:comment>A Tax that is levied on imports and/or exports.</rdfs:comment>
</owl:Class>

<owl:Class rdf:ID= "Ear">
<rdfs:subClassOf rdf:resource ="http://127.0.0.1:8000/ontology/SUMO.owl#Organ"/>
<rdfs:subClassOf rdf:resource 
="http://127.0.0.1:8000/ontology/SUMO.owl#AnimalAnatomicalStructure"/>
<rdfs:comment>The Organ of hearing.</rdfs:comment>
</owl:Class>

<owl:Class rdf:ID= "EarthTremor">
<rdfs:subClassOf rdf:resource ="#Tremor"/>
<rdfs:subClassOf rdf:resource 
="http://127.0.0.1:8000/ontology/SUMO.owl#GeologicalProcess"/>
<rdfs:comment>An EarthTremor is an individual seismic
event in which the earth shakes due to release of seismic 
pressures.</rdfs:comment>
</owl:Class>

<owl:Class rdf:ID= "Earthquake">
<rdfs:subClassOf rdf:resource 
="http://127.0.0.1:8000/ontology/SUMO.owl#GeologicalProcess"/>
<rdfs:comment>Earthquake is the class of events in
which the earth shakes while its layers readjust due to tensional
stresses in the surface of the earth.  A single earthquake may consist
of one or more EarthTremors.</rdfs:comment>
</owl:Class>

<owl:Class rdf:ID= "Echoing">
<rdfs:subClassOf rdf:resource 
="http://127.0.0.1:8000/ontology/SUMO.owl#RadiatingSound"/>
<rdfs:comment>Instances of RadiatingSound where the instrument
is a surface which bounces sound waves back to their origin, where they can
be heard again.</rdfs:comment>
</owl:Class>

<owl:Class rdf:ID= "EconomicAttribute">
<rdfs:subClassOf rdf:resource ="#PoliticoEconomicAttribute"/>
<rdfs:comment>EconomicAttribute is the class
of terms including all Attributes used to characterize the
economic systems or development levels of Nations or dependent
GeopoliticalAreas.</rdfs:comment>
</owl:Class>

<owl:Class rdf:ID= "EconomicRelation">
<rdfs:subClassOf rdf:resource 
="http://127.0.0.1:8000/ontology/SUMO.owl#BinaryRelation"/>
<rdfs:comment>A class of Relations which are used
to specify various economic measures, e.g. the GDP, the consumer price
index, and the trade deficit.</rdfs:comment>
</owl:Class>

<owl:Class rdf:ID= "EconomicSystemAttribute">
<rdfs:subClassOf rdf:resource ="#EconomicAttribute"/>
<rdfs:comment>EconomicSystemAttribute
is the class of Attributes that describe the type of economic
system that a country or area has.  For example, CapitalistEconomy
or SocialistEconomy.</rdfs:comment>
</owl:Class>

<owl:Class rdf:ID= "EducationalCourse">
<rdfs:subClassOf rdf:resource ="#EducationalProgram"/>
<rdfs:comment>A schedule of class meetings offered by an
EducationalOrganization.</rdfs:comment>
</owl:Class>

<owl:Class rdf:ID= "EducationalProgram">
<rdfs:subClassOf rdf:resource ="http://127.0.0.1:8000/ontology/SUMO.owl#Plan"/>
<rdfs:comment>A series of EducationalCourses that must
be completed to receive an AcademicDegree or other Certificate.  Note that
an EducationalProgram, unlike an EducationalCourse, may be realized at more
than one EducationalOrganization.</rdfs:comment>
</owl:Class>

<owl:Class rdf:ID= "Elbow">
<rdfs:subClassOf rdf:resource ="#BodyJoint"/>
<rdfs:comment>The joint in the Arm connecting the forearm and the
upper arm.</rdfs:comment>
</owl:Class>

<owl:Class rdf:ID= "ElectoralCollegeElection">
<rdfs:subClassOf rdf:resource ="#GeneralElection"/>
<rdfs:comment>ElectoralCollegeElection is
the class of Elections in which the outcome is decided by the votes of
electors who have been chosen by popular vote, rather than directly by
results of the popular vote.  ElectoralCollegeElection is an indirect
method of election, in contrast to PopularElection.</rdfs:comment>
</owl:Class>

<owl:Class rdf:ID= "ElectricDevice">
<rdfs:subClassOf rdf:resource ="http://127.0.0.1:8000/ontology/SUMO.owl#Device"/>
<rdfs:comment>Any Device that is powered by electricity.</rdfs:comment>
</owl:Class>

<owl:Class rdf:ID= "ElectricMotor">
<rdfs:subClassOf rdf:resource ="#Engine"/>
<rdfs:subClassOf rdf:resource ="#ElectricDevice"/>
<rdfs:comment>ElectricMotor is the subclass of Engines
that produce mechanical power from electricity.</rdfs:comment>
</owl:Class>

<owl:Class rdf:ID= "ElectricalSignalling">
<rdfs:subClassOf rdf:resource ="#Signalling"/>
<rdfs:comment>ElectricalSignalling is the
subclass of Signalling processes that involve control of an electrical
current.  Cf. ElectronicSignalling.</rdfs:comment>
</owl:Class>

<owl:Class rdf:ID= "ElectrifiedRailwayCar">
<rdfs:subClassOf rdf:resource ="#RollingStock"/>
<rdfs:subClassOf rdf:resource ="#SelfPoweredVehicle"/>
<rdfs:subClassOf rdf:resource ="#ElectricDevice"/>
<rdfs:comment>ElectrifiedRailwayCar is the
subclass of railway cars that are powered by electricity, which is
provided to the car through an overhead link or electrified third 
rail.</rdfs:comment>
</owl:Class>

<owl:Class rdf:ID= "ElectronVolt">
<rdfs:subClassOf rdf:resource 
="http://127.0.0.1:8000/ontology/SUMO.owl#FunctionQuantity"/>
<rdf:type rdf:resource = 
"http://127.0.0.1:8000/ontology/SUMO.owl#UnitOfMeasure"/>
<rdfs:comment>The ElectronVolt is an energy measure.
Symbol: eV.  It is the kinetic energy acquired by an electron in passing
through a potential difference of 1 Volt in a vacuum.</rdfs:comment>
</owl:Class>

<owl:Class rdf:ID= "ElectronicSignalling">
<rdfs:subClassOf rdf:resource ="#Signalling"/>
<rdfs:comment>ElectronicSignalling is the
subclass of Signalling processes that involve a signal generated by
a computer.</rdfs:comment>
</owl:Class>

<owl:Class rdf:ID= "Elephant">
<rdfs:subClassOf rdf:resource ="#Herbivore"/>
<rdfs:comment>A very large, almost hairless Herbivore with a long
trunk.</rdfs:comment>
</owl:Class>

<owl:Class rdf:ID= "Elevator">
<rdfs:subClassOf rdf:resource 
="http://127.0.0.1:8000/ontology/SUMO.owl#TransportationDevice"/>
<rdfs:comment>A TransportationDevice consisting of a car that moves
up and down in a vertical shaft so that people can move from one floor to 
another
in a building.</rdfs:comment>
</owl:Class>

<owl:Class rdf:ID= "Embracing">
<rdfs:subClassOf rdf:resource 
="http://127.0.0.1:8000/ontology/SUMO.owl#Touching"/>
<rdfs:comment>The class of Touching processes where one Human
hugs another one.</rdfs:comment>
</owl:Class>

<owl:Class rdf:ID= "EmergencyRoadVehicle">
<rdfs:subClassOf rdf:resource ="#EmergencyVehicle"/>
<rdfs:subClassOf rdf:resource ="#SelfPoweredRoadVehicle"/>
<rdfs:comment>EmergencyRoadVehicle is the
subclass of EmergencyVehicle that includes RoadVehicles designed
for special use in emergencies, e.g., Ambulances, 
FireEngines.</rdfs:comment>
</owl:Class>

<owl:Class rdf:ID= "EmergencyVehicle">
<rdfs:subClassOf rdf:resource ="#SelfPoweredVehicle"/>
<rdfs:comment>EmergencyVehicle is the subclass of
Vehicles that are used for special-purpose emergency 
response.</rdfs:comment>
</owl:Class>

<owl:Class rdf:ID= "EmploymentFiring">
<rdfs:subClassOf rdf:resource 
="http://127.0.0.1:8000/ontology/SUMO.owl#TerminatingEmployment"/>
<rdfs:comment>Involuntarily ending one's employment.
Note that this covers termination due to inadequate performance, as
well as layoffs.</rdfs:comment>
</owl:Class>

<owl:Class rdf:ID= "Engine">
<rdfs:subClassOf rdf:resource ="#Transducer"/>
<rdfs:comment>Engine is a subclass of Transducer.  Engines
are devices for converting some form of energy resource into mechanical
power.</rdfs:comment>
</owl:Class>

<owl:Class rdf:ID= "EntertainmentCompany">
<rdfs:subClassOf rdf:resource 
="http://127.0.0.1:8000/ontology/SUMO.owl#CommercialAgent"/>
<rdfs:comment>Any business whose services include
Performances.  This class covers nightclubs, commercial live theaters,
and comedy clubs.</rdfs:comment>
</owl:Class>

<owl:Class rdf:ID= "EntertainmentProfession">
<rdfs:subClassOf rdf:resource ="#SkilledOccupation"/>
<rdfs:comment>Positions which involve creating
content or performances that are intended to entertain.  This class covers
the TheaterProfession, FilmMakingProfession, being a comedian, 
etc.</rdfs:comment>
</owl:Class>

<owl:Class rdf:ID= "Entombing">
<rdfs:subClassOf rdf:resource 
="http://127.0.0.1:8000/ontology/SUMO.owl#Putting"/>
<rdfs:comment>More commonly known as burying, this is the class
of processes of putting a HumanCorpse into a Tomb.  Note that this class
is not a subclass of Burying, since some Tombs are not covered with Soil,
e.g. those in a mausoleum.</rdfs:comment>
</owl:Class>

<owl:Class rdf:ID= "Envelope">
<rdfs:subClassOf rdf:resource ="#Container"/>
<rdfs:comment>A sealable Container for one or more pieces of
paper which is designed to protect the papers while they are transferred to
someone.</rdfs:comment>
</owl:Class>

<owl:Class rdf:ID= "Enzyme">
<rdfs:subClassOf rdf:resource 
="http://127.0.0.1:8000/ontology/SUMO.owl#Protein"/>
<rdfs:comment>A complex Protein that is produced by living
cells and which catalyzes specific biochemical reactions. There are six
main types of enzymes:  oxidoreductases, transferases, hydrolases,
lyases, isomerases, and ligases.</rdfs:comment>
</owl:Class>

<owl:Class rdf:ID= "Erosion">
<rdfs:subClassOf rdf:resource 
="http://127.0.0.1:8000/ontology/SUMO.owl#GeologicalProcess"/>
<rdfs:subClassOf rdf:resource 
="http://127.0.0.1:8000/ontology/SUMO.owl#Removing"/>
<rdfs:comment>Erosion is the subclass of Removing processes
in which rock and soil material are removed from LandForms in one area
and deposited elsewhere by wind, running water, ice, heat, and other
GeologicalProcesses.</rdfs:comment>
</owl:Class>

<owl:Class rdf:ID= "Escaping">
<rdfs:subClassOf rdf:resource 
="http://127.0.0.1:8000/ontology/SUMO.owl#Translocation"/>
<rdfs:comment>Any instance of Translocation where the agent brings
it about that he/she is no longer confined without having the right to do
so.</rdfs:comment>
</owl:Class>

<owl:Class rdf:ID= "Espionage">
<rdfs:subClassOf rdf:resource 
="http://127.0.0.1:8000/ontology/SUMO.owl#PoliticalProcess"/>
<rdfs:subClassOf rdf:resource 
="http://127.0.0.1:8000/ontology/SUMO.owl#Investigating"/>
<rdfs:comment>Any Investigating by one Government of another
Government where the second Government does not know that it is being
spied upon.</rdfs:comment>
</owl:Class>

<owl:Class rdf:ID= "EuropeanCity">
<rdfs:subClassOf rdf:resource ="http://127.0.0.1:8000/ontology/SUMO.owl#City"/>
<rdfs:comment>The class of cities that are in Europe.</rdfs:comment>
</owl:Class>

<owl:Class rdf:ID= "EuropeanNation">
<rdfs:subClassOf rdf:resource ="http://127.0.0.1:8000/ontology/SUMO.owl#Nation"/>
<rdfs:comment>The class of nations that are in Europe.</rdfs:comment>
</owl:Class>

<owl:Class rdf:ID= "Execution">
<rdfs:subClassOf rdf:resource 
="http://127.0.0.1:8000/ontology/SUMO.owl#Killing"/>
<rdfs:comment>Killing of a Human by a Government for
the commission of a CriminalAction.</rdfs:comment>
</owl:Class>

<owl:Class rdf:ID= "ExecutiveResidence">
<rdfs:subClassOf rdf:resource 
="http://127.0.0.1:8000/ontology/SUMO.owl#PermanentResidence"/>
<rdfs:comment>A Residence of a chiefOfState, e.g.
the White House, a state governor's mansion, Buckingham Palace, 
etc.</rdfs:comment>
</owl:Class>

<owl:Class rdf:ID= "Exhaling">
<rdfs:subClassOf rdf:resource 
="http://127.0.0.1:8000/ontology/SUMO.owl#Breathing"/>
<rdfs:comment>Any instance of Breathing where the breath is
expelled from the Lungs.</rdfs:comment>
</owl:Class>

<owl:Class rdf:ID= "Explosion">
<rdfs:subClassOf rdf:resource 
="http://127.0.0.1:8000/ontology/SUMO.owl#Radiating"/>
<rdfs:comment>Any sudden and massive release of energy that is
the product of a chemical reaction.</rdfs:comment>
</owl:Class>

<owl:Class rdf:ID= "ExplosiveDevice">
<rdfs:subClassOf rdf:resource ="http://127.0.0.1:8000/ontology/SUMO.owl#Device"/>
<rdfs:comment>A Device whose purpose is to explode.  Note
that ExplosiveDevice is not a subclass of Weapon, since explosives can be
used in demolition work and in fireworks displays, for 
example.</rdfs:comment>
</owl:Class>

<owl:Class rdf:ID= "ExplosiveMine">
<rdfs:subClassOf rdf:resource ="#ExplosiveDevice"/>
<rdfs:subClassOf rdf:resource ="http://127.0.0.1:8000/ontology/SUMO.owl#Weapon"/>
<rdfs:comment>An ExplosiveDevice which is designed to
explode when there is movement over it, e.g. by a person on foot, by a
RoadVehicle, etc.</rdfs:comment>
</owl:Class>

<owl:Class rdf:ID= "ExplosiveSubstance">
<rdfs:subClassOf rdf:resource 
="http://127.0.0.1:8000/ontology/SUMO.owl#Substance"/>
<rdfs:comment>Any Substance which is capable of exploding.</rdfs:comment>
</owl:Class>

<owl:Class rdf:ID= "Exporting">
<rdfs:subClassOf rdf:resource 
="http://127.0.0.1:8000/ontology/SUMO.owl#FinancialTransaction"/>
<rdfs:comment>Exporting is the class of actions in
which there is a ChangeOfPossession of goods shipped from a
provider in one Nation to a destination in another Nation.
Typically, there are Selling and Buying events associated
with an Exporting.  Either the seller or the exporting country
may be considered the origin of Exporting.</rdfs:comment>
</owl:Class>

<owl:Class rdf:ID= "ExpressingApproval">
<rdfs:subClassOf rdf:resource 
="http://127.0.0.1:8000/ontology/SUMO.owl#Expressing"/>
<rdfs:comment>Expressing favor about a physical thing
or a state of affairs.</rdfs:comment>
</owl:Class>

<owl:Class rdf:ID= "ExpressingDisapproval">
<rdfs:subClassOf rdf:resource 
="http://127.0.0.1:8000/ontology/SUMO.owl#Expressing"/>
<rdfs:comment>Expressing disfavor about a physical
thing or a state of affairs.</rdfs:comment>
</owl:Class>

<owl:Class rdf:ID= "ExpressingFarewell">
<rdfs:subClassOf rdf:resource 
="http://127.0.0.1:8000/ontology/SUMO.owl#Expressing"/>
<rdfs:comment>Any instance of Expressing an acknowledgment
of a person's departure.  Note that this class is not a subclass of
LinguisticCommunication, because it covers gestures of departure, e.g. 
Waving
and Nodding in certain circumstances.</rdfs:comment>
</owl:Class>

<owl:Class rdf:ID= "Expressway">
<rdfs:subClassOf rdf:resource ="#SurfacedRoadway"/>
<rdfs:comment>Expressway is the subclass of
SurfacedRoadways that are multiple-lane, limited-access highways
designed for rapid travel by MotorVehicles.</rdfs:comment>
</owl:Class>

<owl:Class rdf:ID= "Eye">
<rdfs:subClassOf rdf:resource ="http://127.0.0.1:8000/ontology/SUMO.owl#Organ"/>
<rdfs:subClassOf rdf:resource 
="http://127.0.0.1:8000/ontology/SUMO.owl#AnimalAnatomicalStructure"/>
<rdfs:comment>The Organ of sight.</rdfs:comment>
</owl:Class>

<owl:Class rdf:ID= "EyeGlass">
<rdfs:subClassOf rdf:resource ="#OpticalDevice"/>
<rdfs:comment>A lens or pair of lenses with or without frames whose
purpose is to to correct a defect in vision.  This class covers ordinary eye
glasses, reading glasses, contact lenses, monocles, etc.</rdfs:comment>
</owl:Class>

<owl:Class rdf:ID= "EyeMotion">
<rdfs:subClassOf rdf:resource 
="http://127.0.0.1:8000/ontology/SUMO.owl#BodyMotion"/>
<rdfs:comment>Any Motion where a patient is the agent's
own Eyelid or Eyelids.</rdfs:comment>
</owl:Class>

<owl:Class rdf:ID= "Eyelid">
<rdfs:subClassOf rdf:resource ="#Skin"/>
<rdfs:comment>Folds of Skin that can be manipulated to
cover or uncover Eyes.</rdfs:comment>
</owl:Class>

<owl:Class rdf:ID= "FabricArtifact">
<rdfs:subClassOf rdf:resource 
="http://127.0.0.1:8000/ontology/SUMO.owl#Artifact"/>
<rdfs:comment>Any Artifact that is made out of Fabric.</rdfs:comment>
</owl:Class>

<owl:Class rdf:ID= "Face">
<rdfs:subClassOf rdf:resource 
="http://127.0.0.1:8000/ontology/SUMO.owl#AnimalAnatomicalStructure"/>
<rdfs:subClassOf rdf:resource 
="http://127.0.0.1:8000/ontology/SUMO.owl#BodyPart"/>
<rdfs:comment>The part of the Head from forehead to chin and
from ear to ear.</rdfs:comment>
</owl:Class>

<owl:Class rdf:ID= "FacialExpression">
<rdfs:subClassOf rdf:resource 
="http://127.0.0.1:8000/ontology/SUMO.owl#Gesture"/>
<rdfs:comment>Any Gesture whose instrument is the Face.</rdfs:comment>
</owl:Class>

<owl:Class rdf:ID= "FacialHair">
<rdfs:subClassOf rdf:resource ="#Hair"/>
<rdfs:comment>Hair that grows on the Face.  This
class covers bears, mustaches, sideburns, midnight shadow, 
etc.</rdfs:comment>
</owl:Class>

<owl:Class rdf:ID= "Fact">
<rdfs:subClassOf rdf:resource ="#Statement"/>
<rdfs:comment>The class of Statements that are True.</rdfs:comment>
</owl:Class>

<owl:Class rdf:ID= "Factory">
<rdfs:subClassOf rdf:resource 
="http://127.0.0.1:8000/ontology/SUMO.owl#Building"/>
<rdfs:comment>A building intended to house a process that
produces goods of some value.</rdfs:comment>
</owl:Class>

<owl:Class rdf:ID= "FallSeason">
<rdfs:subClassOf rdf:resource ="#SeasonOfYear"/>
<rdfs:comment>The SeasonOfYear that begins at the autumnal
equinox and ends at the winter solstice.</rdfs:comment>
</owl:Class>

<owl:Class rdf:ID= "Falling">
<rdfs:subClassOf rdf:resource 
="http://127.0.0.1:8000/ontology/SUMO.owl#Translocation"/>
<rdfs:subClassOf rdf:resource ="#MotionDownward"/>
<sumo:disjoint rdf:resource = 
"http://127.0.0.1:8000/ontology/SUMO.owl#IntentionalProcess" />
<rdfs:comment>The class of Translocations where
something moves from a higher location to a lower location
under the force of gravity and without intending to do so.</rdfs:comment>
</owl:Class>

<owl:Class rdf:ID= "FallingAsleep">
<rdfs:subClassOf rdf:resource 
="http://127.0.0.1:8000/ontology/SUMO.owl#PsychologicalProcess"/>
<sumo:disjoint rdf:resource = "#WakingUp" />
<rdfs:comment>The process of transitioning from a state of
being Awake to a state of being Asleep.</rdfs:comment>
</owl:Class>

<owl:Class rdf:ID= "Fallout">
<rdfs:subClassOf rdf:resource ="#Powder"/>
<rdfs:comment>Radioactive powder that is typically dispersed by
the explosion of a nuclear weapon.</rdfs:comment>
</owl:Class>

<owl:Class rdf:ID= "FamilyBusiness">
<rdfs:subClassOf rdf:resource ="#Partnership"/>
<rdfs:comment>A Partnership that is owned by a single
family.</rdfs:comment>
</owl:Class>

<owl:Class rdf:ID= "FanDevice">
<rdfs:subClassOf rdf:resource ="#CoolingDevice"/>
<rdfs:comment>A CoolingDevice which consists simply of one or more
blades that circulate the air.  Note that this class covers both electrical 
fans
and fans that are manually operated.</rdfs:comment>
</owl:Class>

<owl:Class rdf:ID= "Farad">
<rdfs:subClassOf rdf:resource 
="http://127.0.0.1:8000/ontology/SUMO.owl#FunctionQuantity"/>
<rdf:type rdf:resource = 
"http://127.0.0.1:8000/ontology/SUMO.owl#SystemeInternationalUnit"/>
<rdfs:comment>SI capacitance measure.  Symbol: F.  It is the
capacitance of a capacitator between the plates of which there appears
a difference of potential of 1 Volt when it is charged by a quantity
of electricity equal to 1 Coulomb.  Farad = C/V =
m^(-2)*kg(-1)*s^4*A^2.</rdfs:comment>
</owl:Class>

<owl:Class rdf:ID= "Farm">
<rdfs:subClassOf rdf:resource 
="http://127.0.0.1:8000/ontology/SUMO.owl#StationaryArtifact"/>
<rdfs:comment>A StationaryArtifact consisting of a cultivated
LandArea and Buildings for maintaining the land and/or the Animals
on the land.</rdfs:comment>
</owl:Class>

<owl:Class rdf:ID= "FarmBuilding">
<rdfs:subClassOf rdf:resource 
="http://127.0.0.1:8000/ontology/SUMO.owl#Building"/>
<sumo:disjoint rdf:resource = 
"http://127.0.0.1:8000/ontology/SUMO.owl#ResidentialBuilding" />
<rdfs:comment>A Building on a Farm that is used for keeping
DomesticAnimals, Fodder or harvested crops.</rdfs:comment>
</owl:Class>

<owl:Class rdf:ID= "FarmHand">
<rdfs:subClassOf rdf:resource ="#OccupationalTrade"/>
<rdfs:comment>OccupationalTrades which involve Agriculture.</rdfs:comment>
</owl:Class>

<owl:Class rdf:ID= "Feather">
<rdfs:subClassOf rdf:resource 
="http://127.0.0.1:8000/ontology/SUMO.owl#AnimalAnatomicalStructure"/>
<rdfs:subClassOf rdf:resource 
="http://127.0.0.1:8000/ontology/SUMO.owl#BodyPart"/>
<rdfs:comment>Each instance of this class is one of the structures
that make up the external covering of Birds.</rdfs:comment>
</owl:Class>

<owl:Class rdf:ID= "Feeding">
<rdfs:subClassOf rdf:resource ="http://127.0.0.1:8000/ontology/SUMO.owl#Giving"/>
<rdfs:comment>Giving Food to a Human or Animal.</rdfs:comment>
</owl:Class>

<owl:Class rdf:ID= "FemaleCow">
<rdfs:subClassOf rdf:resource ="#Cow"/>
<rdfs:comment>A Cow that is Female.</rdfs:comment>
</owl:Class>

<owl:Class rdf:ID= "Fence">
<rdfs:subClassOf rdf:resource 
="http://127.0.0.1:8000/ontology/SUMO.owl#StationaryArtifact"/>
<rdfs:comment>A StationaryArtifact that serves to demarcate or
to prevent access to or from the area that the Fence 
surrounds.</rdfs:comment>
</owl:Class>

<owl:Class rdf:ID= "Fertilizer">
<rdfs:subClassOf rdf:resource 
="http://127.0.0.1:8000/ontology/SUMO.owl#Mixture"/>
<rdfs:comment>Any Mixture which is used to provide nutrients to
living Plants.  Fertilizers can be made up of plant or animal material, e.g.
compost, or they can be entirely synthetic, e.g. ammonium 
nitrate.</rdfs:comment>
</owl:Class>

<owl:Class rdf:ID= "Field">
<rdfs:subClassOf rdf:resource 
="http://127.0.0.1:8000/ontology/SUMO.owl#LandArea"/>
<rdfs:comment>A LandArea that has been cleared of BotanicalTrees.
Note that a Field is not necessarily used for the cultivation of crops and
that a Field may be small.</rdfs:comment>
</owl:Class>

<owl:Class rdf:ID= "Fighter">
<rdfs:subClassOf rdf:resource ="#MilitaryAircraft"/>
<rdfs:comment>Any high-speed MilitaryAircraft whose purpose is
to destroy enemy MilitaryAircraft.</rdfs:comment>
</owl:Class>

<owl:Class rdf:ID= "FileDevice">
<rdfs:subClassOf rdf:resource ="http://127.0.0.1:8000/ontology/SUMO.owl#Device"/>
<rdfs:comment>A Device whose purpose is to make something
smoother by removing small particles from an Object.  For example, a nail
file is used to even out the tips of one's finger nails.</rdfs:comment>
</owl:Class>

<owl:Class rdf:ID= "FillingAnOrder">
<rdfs:subClassOf rdf:resource 
="http://127.0.0.1:8000/ontology/SUMO.owl#FinancialTransaction"/>
<rdfs:comment>Execute an order or buy or sell a Security.</rdfs:comment>
</owl:Class>

<owl:Class rdf:ID= "FilmDirector">
<rdfs:subClassOf rdf:resource ="#FilmMakingProfession"/>
<rdfs:comment>Positions which involve directing 
MotionPictures.</rdfs:comment>
</owl:Class>

<owl:Class rdf:ID= "FilmMaking">
<rdfs:subClassOf rdf:resource 
="http://127.0.0.1:8000/ontology/SUMO.owl#ContentDevelopment"/>
<rdfs:comment>ContentDevelopment where the result is a
MotionPicture.</rdfs:comment>
</owl:Class>

<owl:Class rdf:ID= "FilmMakingProfession">
<rdfs:subClassOf rdf:resource ="#EntertainmentProfession"/>
<rdfs:comment>Positions which involve FilmMaking,
i.e. acting in films, directing films, producing films, etc.</rdfs:comment>
</owl:Class>

<owl:Class rdf:ID= "FilmProducer">
<rdfs:subClassOf rdf:resource ="#FilmMakingProfession"/>
<rdfs:comment>Positions which involve producing MotionPictures,
i.e arranging the financing for the MotionPicture and supervising its 
production.</rdfs:comment>
</owl:Class>

<owl:Class rdf:ID= "Filter">
<rdfs:subClassOf rdf:resource ="http://127.0.0.1:8000/ontology/SUMO.owl#Device"/>
<rdfs:comment>A Device whose purpose is to remove part of a
Solution that is passed through the Filter.</rdfs:comment>
</owl:Class>

<owl:Class rdf:ID= "FinancialAccount">
<sumo:subAttribute rdf:resource = 
"http://127.0.0.1:8000/ontology/SUMO.owl#Contract" />
<rdfs:comment>A formal banking, brokerage, or business
relationship established to provide for regular services, dealings, and
other financial transactions.</rdfs:comment>
</owl:Class>

<owl:Class rdf:ID= "FinancialBank">
<rdfs:subClassOf rdf:resource ="#FinancialCompany"/>
<rdfs:comment>An organization, chartered by a state
or federal government, which does most or all of the following: receives
Deposits, honors FinancialInstruments drawn on them, and pays
interest on them; discounts Notes, makes Loans, and invests in
SecuredLoans; collects Checks, Drafts and Notes, certifies
depositor's checks; and issues drafts and Cashier's checks.</rdfs:comment>
</owl:Class>

<owl:Class rdf:ID= "FinancialBill">
<rdfs:subClassOf rdf:resource ="#FinancialText"/>
<rdfs:comment>A brief statement that the stated amount
of money is owed by the person to whom the bill is delivered.</rdfs:comment>
</owl:Class>

<owl:Class rdf:ID= "FinancialCompany">
<rdfs:subClassOf rdf:resource 
="http://127.0.0.1:8000/ontology/SUMO.owl#CommercialAgent"/>
<rdfs:comment>The class FinancialCompany
includes, as subclasses, FinancialBank, CreditUnion and 
SavingsAndLoan.</rdfs:comment>
</owl:Class>

<owl:Class rdf:ID= "FinancialService">
<rdfs:subClassOf rdf:resource 
="http://127.0.0.1:8000/ontology/SUMO.owl#CommercialService"/>
<rdfs:comment>Services performed by
FinancialOrganizations.</rdfs:comment>
</owl:Class>

<owl:Class rdf:ID= "FinancialText">
<rdfs:subClassOf rdf:resource ="#Report"/>
<rdfs:comment>A Report about monetary figures.  This
class covers FinancialBills, balance sheets, account statements, 
etc.</rdfs:comment>
</owl:Class>

<owl:Class rdf:ID= "Financing">
<rdfs:subClassOf rdf:resource 
="http://127.0.0.1:8000/ontology/SUMO.owl#Funding"/>
<rdfs:subClassOf rdf:resource ="#FinancialService"/>
<rdfs:comment>Any Funding which is provided by a FinancialCompany
with the aim of making a profit on the money invested.</rdfs:comment>
</owl:Class>

<owl:Class rdf:ID= "Finger">
<rdfs:subClassOf rdf:resource ="#DigitAppendage"/>
<rdfs:comment>The five extremities of Hands.</rdfs:comment>
</owl:Class>

<owl:Class rdf:ID= "Fingerprint">
<rdfs:subClassOf rdf:resource 
="http://127.0.0.1:8000/ontology/SUMO.owl#ShapeAttribute"/>
<rdfs:comment>That pattern of arches, loops, and whorls that mark
the imprint of a Finger.</rdfs:comment>
</owl:Class>

<owl:Class rdf:ID= "FireEngine">
<rdfs:subClassOf rdf:resource ="#EmergencyRoadVehicle"/>
<rdfs:comment>FireEngine is the subclass of
EmergencyRoadVehicles that represents fire engines.</rdfs:comment>
</owl:Class>

<owl:Class rdf:ID= "Firearm">
<rdfs:subClassOf rdf:resource ="#Gun"/>
<rdfs:comment>A Gun that is small enough to be carried and fired by
a single Human.</rdfs:comment>
</owl:Class>

<owl:Class rdf:ID= "Fireplace">
<rdfs:subClassOf rdf:resource 
="http://127.0.0.1:8000/ontology/SUMO.owl#StationaryArtifact"/>
<rdfs:subClassOf rdf:resource ="http://127.0.0.1:8000/ontology/SUMO.owl#Device"/>
<rdfs:comment>A Device in a Building which is used for burning wood,
coal, etc for heat.</rdfs:comment>
</owl:Class>

<owl:Class rdf:ID= "FishMeat">
<rdfs:subClassOf rdf:resource ="http://127.0.0.1:8000/ontology/SUMO.owl#Meat"/>
<rdfs:comment>Meat that was originally part of a Fish.</rdfs:comment>
</owl:Class>

<owl:Class rdf:ID= "Fishing">
<rdfs:subClassOf rdf:resource ="#Hunting"/>
<rdfs:comment>Fishing is the class of Processes in which
Fish are hunted.</rdfs:comment>
</owl:Class>

<owl:Class rdf:ID= "FixedHoliday">
<rdfs:subClassOf rdf:resource ="#Holiday"/>
<rdfs:comment>FixedHoliday is the class of Holidays
whose observance is fixed to recurrences of the calendar day that the
holiday commemorates.</rdfs:comment>
</owl:Class>

<owl:Class rdf:ID= "Flag">
<rdfs:subClassOf rdf:resource ="http://127.0.0.1:8000/ontology/SUMO.owl#Icon"/>
<rdfs:comment>An Icon made of Fabric that refers to a particular
GeopoliticalArea.</rdfs:comment>
</owl:Class>

<owl:Class rdf:ID= "Flooding">
<rdfs:subClassOf rdf:resource 
="http://127.0.0.1:8000/ontology/SUMO.owl#LiquidMotion"/>
<rdfs:comment>Flooding is the subclass of LiquidMotion
processes in which the water level of a Waterway rises or water spreads
over a flood plain along a Waterway.</rdfs:comment>
</owl:Class>

<owl:Class rdf:ID= "Floor">
<rdfs:subClassOf rdf:resource 
="http://127.0.0.1:8000/ontology/SUMO.owl#StationaryArtifact"/>
<rdfs:comment>A StationaryArtifact that is the bottom surface
of a Room.</rdfs:comment>
</owl:Class>

<owl:Class rdf:ID= "Flour">
<rdfs:subClassOf rdf:resource ="#PreparedFood"/>
<rdfs:subClassOf rdf:resource ="#Powder"/>
<rdfs:comment>A Powder that is prepared from CerealGrain, e.g.
wheat flour, rice flour, etc.  Flour is most often used in the making
of BreadOrBiscuits.</rdfs:comment>
</owl:Class>

<owl:Class rdf:ID= "FlowRegion">
<rdfs:subClassOf rdf:resource 
="http://127.0.0.1:8000/ontology/SUMO.owl#SelfConnectedObject"/>
<rdfs:comment>FlowRegion is a class of things whose
boundaries are relatively stable but whose constitutive material is
continuously moving through the region itself and being replaced by
other, similar material.  Each FlowRegion is constituted by a stream
of matter moving as a whole.  A FlowRegion may be liquid or gaseous.
A wind may be considered as a Process or as a FlowRegion, similarly
an ocean current or a WaterWave.  Note that certain
properties belong to the FlowRegion itself (e.g., mass, length, volume,
temperature, and speed or velocity of the region moving as a whole),
while other properties of interest belong to the Motion of its
constitutive stuff (e.g., velocity, direction).  The motion of
a FlowRegion as a whole (e.g. the jet stream moves within the atmosphere)
is distinguished from the motion of the pieces of stuff constituting the
FlowRegion.</rdfs:comment>
</owl:Class>

<owl:Class rdf:ID= "Flower">
<rdfs:subClassOf rdf:resource 
="http://127.0.0.1:8000/ontology/SUMO.owl#PlantAnatomicalStructure"/>
<rdfs:subClassOf rdf:resource ="http://127.0.0.1:8000/ontology/SUMO.owl#Organ"/>
<rdfs:comment>The reproductive organ of FloweringPlants.</rdfs:comment>
</owl:Class>

<owl:Class rdf:ID= "FluidContainer">
<rdfs:subClassOf rdf:resource ="#Container"/>
<rdfs:comment>A Container which is used to store Fluids,
i.e. Liquids and Gases.</rdfs:comment>
</owl:Class>

<owl:Class rdf:ID= "FlyInsect">
<rdfs:subClassOf rdf:resource ="http://127.0.0.1:8000/ontology/SUMO.owl#Insect"/>
<rdfs:comment>Insects with Wings and two Limbs.</rdfs:comment>
</owl:Class>

<owl:Class rdf:ID= "Flying">
<rdfs:subClassOf rdf:resource 
="http://127.0.0.1:8000/ontology/SUMO.owl#Translocation"/>
<rdfs:comment>Any instance of Translocation which is through an
AtmosphericRegion and which is powered by the Wings of an 
Animal.</rdfs:comment>
</owl:Class>

<owl:Class rdf:ID= "Focusing">
<rdfs:subClassOf rdf:resource 
="http://127.0.0.1:8000/ontology/SUMO.owl#QuantityChange"/>
<rdfs:comment>Altering the relative distance of a Lens
so that a visual image is sharper.</rdfs:comment>
</owl:Class>

<owl:Class rdf:ID= "Fodder">
<rdfs:subClassOf rdf:resource ="http://127.0.0.1:8000/ontology/SUMO.owl#Food"/>
<rdfs:comment>Fodder is the subclass of Food that is intended
for instances of DomesticAnimal.</rdfs:comment>
</owl:Class>

<owl:Class rdf:ID= "Fog">
<rdfs:subClassOf rdf:resource 
="http://127.0.0.1:8000/ontology/SUMO.owl#WaterCloud"/>
<rdfs:comment>Any WaterCloud that is in contact with the 
ground.</rdfs:comment>
</owl:Class>

<owl:Class rdf:ID= "Folding">
<rdfs:subClassOf rdf:resource 
="http://127.0.0.1:8000/ontology/SUMO.owl#ShapeChange"/>
<rdfs:comment>Bending something in such a way that one part of
it covers another part.</rdfs:comment>
</owl:Class>

<owl:Class rdf:ID= "Foot">
<rdfs:subClassOf rdf:resource 
="http://127.0.0.1:8000/ontology/SUMO.owl#AnimalAnatomicalStructure"/>
<rdfs:subClassOf rdf:resource 
="http://127.0.0.1:8000/ontology/SUMO.owl#BodyPart"/>
<rdfs:comment>The lower part of a Limb, the part which makes contact
with the ground in locomotion of the Animal.</rdfs:comment>
</owl:Class>

<owl:Class rdf:ID= "Football">
<rdfs:subClassOf rdf:resource ="#TeamSport"/>
<rdfs:comment>A TeamSport where each team tries to place the ball
in the other's goal.  Note that each instance of Football is a football 
game.</rdfs:comment>
</owl:Class>

<owl:Class rdf:ID= "FootballManeuver">
<rdfs:subClassOf rdf:resource 
="http://127.0.0.1:8000/ontology/SUMO.owl#Maneuver"/>
<rdfs:comment>Any Maneuver in Football.</rdfs:comment>
</owl:Class>

<owl:Class rdf:ID= "FootballPass">
<rdfs:subClassOf rdf:resource ="#FootballManeuver"/>
<rdfs:comment>Any FootballManeuver where the member of one
team throws the ball to another member of the same team.</rdfs:comment>
</owl:Class>

<owl:Class rdf:ID= "FootballTeam">
<rdfs:subClassOf rdf:resource ="#SportsTeam"/>
<rdfs:comment>The class of SportsTeams that play Football.</rdfs:comment>
</owl:Class>

<owl:Class rdf:ID= "FootballTouchdown">
<rdfs:subClassOf rdf:resource ="#FootballManeuver"/>
<rdfs:subClassOf rdf:resource ="#Score"/>
<rdfs:comment>Any FootballManeuver which is also a
Score, i.e. any play in a Football game which results in one team
being in possession of the ball on the inside of the opponent's goal 
line.</rdfs:comment>
</owl:Class>

<owl:Class rdf:ID= "ForeignServicePosition">
<rdfs:subClassOf rdf:resource 
="http://127.0.0.1:8000/ontology/SUMO.owl#Position"/>
<rdfs:comment>ForeignServicePosition is the
subclass of Positions that belong to foreign service personnel working
for a national government or international organization.</rdfs:comment>
</owl:Class>

<owl:Class rdf:ID= "Forest">
<rdfs:subClassOf rdf:resource 
="http://127.0.0.1:8000/ontology/SUMO.owl#LandArea"/>
<sumo:disjoint rdf:resource = "#Field" />
<rdfs:comment>Forest is the class of large LandAreas that
are covered by trees and associated undergrowth, either growing wild or
managed for the purpose of timber production.</rdfs:comment>
</owl:Class>

<owl:Class rdf:ID= "FormOfGovernment">
<rdfs:subClassOf rdf:resource ="#PoliticoEconomicAttribute"/>
<rdfs:comment>FormOfGovernment is a class of
Attributes used to describe the characteristics of a government,
especially a NationalGovernment.  The concept FormOfGovernment is
interpreted broadly enough to include Anarchy and 
Factionalism.</rdfs:comment>
</owl:Class>

<owl:Class rdf:ID= "FormText">
<rdfs:subClassOf rdf:resource ="http://127.0.0.1:8000/ontology/SUMO.owl#Text"/>
<rdfs:comment>A page or set of pages containing spaces where
information is to be entered by an Agent.</rdfs:comment>
</owl:Class>

<owl:Class rdf:ID= "FormalMeeting">
<rdfs:subClassOf rdf:resource 
="http://127.0.0.1:8000/ontology/SUMO.owl#Meeting"/>
<sumo:disjoint rdf:resource = "#SocialParty" />
<rdfs:comment>Any Meeting which is the result of Planning
and whose purpose is not socializing.  This covers organizatinal meetings, 
as
well as events like funerals.</rdfs:comment>
</owl:Class>

<owl:Class rdf:ID= "FossilFuel">
<rdfs:subClassOf rdf:resource ="#Fuel"/>
<rdfs:subClassOf rdf:resource ="#PetroleumProduct"/>
<rdfs:comment>FossilFuel is the subclass of Fuel whose
instances are derived from fossilized organic deposits, such as Coal
and LiquefiedPetroleumGas.</rdfs:comment>
</owl:Class>

<owl:Class rdf:ID= "Founding">
<rdfs:subClassOf rdf:resource 
="http://127.0.0.1:8000/ontology/SUMO.owl#Declaring"/>
<rdfs:subClassOf rdf:resource 
="http://127.0.0.1:8000/ontology/SUMO.owl#OrganizationalProcess"/>
<rdfs:comment>Setting up an Organization.</rdfs:comment>
</owl:Class>

<owl:Class rdf:ID= "Fox">
<rdfs:subClassOf rdf:resource ="http://127.0.0.1:8000/ontology/SUMO.owl#Canine"/>
<rdfs:comment>Canines with a bushy tail and pointed ears and nose.
Foxes tend to be much smaller than most DomesticDogs.</rdfs:comment>
</owl:Class>

<owl:Class rdf:ID= "FreeAtom">
<rdfs:subClassOf rdf:resource ="http://127.0.0.1:8000/ontology/SUMO.owl#Atom"/>
<rdfs:comment>Any Atom which is not part of a Molecule.</rdfs:comment>
</owl:Class>

<owl:Class rdf:ID= "FreightCar">
<rdfs:subClassOf rdf:resource ="#Railcar"/>
<rdfs:comment>FreightCar is the subclass of Railcars that
are used for hauling freight: bulk materials, manufactured goods, and other
commodities.</rdfs:comment>
</owl:Class>

<owl:Class rdf:ID= "Frightening">
<rdfs:subClassOf rdf:resource 
="http://127.0.0.1:8000/ontology/SUMO.owl#PsychologicalProcess"/>
<rdfs:comment>Any PsychologicalProcess where the patient
comes to feel Anxiety.</rdfs:comment>
</owl:Class>

<owl:Class rdf:ID= "Frowning">
<rdfs:subClassOf rdf:resource ="#FacialExpression"/>
<rdfs:comment>Furrowing the forehead in such a way as to convey
unhappiness.</rdfs:comment>
</owl:Class>

<owl:Class rdf:ID= "Fuel">
<rdfs:subClassOf rdf:resource 
="http://127.0.0.1:8000/ontology/SUMO.owl#Substance"/>
<rdfs:comment>Fuel is the class of Substances that can be
used as resources in Combustion processes in order to produce heat.
Mechanical energy can be produced by burning fuel in an 
Engine.</rdfs:comment>
</owl:Class>

<owl:Class rdf:ID= "FullTimePosition">
<rdfs:subClassOf rdf:resource 
="http://127.0.0.1:8000/ontology/SUMO.owl#Position"/>
<rdfs:comment>Any Position where the employee is either
salaried or paid for at least 40 hour of work per week.</rdfs:comment>
</owl:Class>

<owl:Class rdf:ID= "Funeral">
<rdfs:subClassOf rdf:resource ="#FormalMeeting"/>
<rdfs:comment>A FormalMeeting whose purpose is to commemorate
the death of someone.</rdfs:comment>
</owl:Class>

<owl:Class rdf:ID= "Furniture">
<rdfs:subClassOf rdf:resource 
="http://127.0.0.1:8000/ontology/SUMO.owl#Artifact"/>
<sumo:disjoint rdf:resource = "http://127.0.0.1:8000/ontology/SUMO.owl#Device" />
<rdfs:comment>Any free-standing Artifacts which are not
Devices and which are used in day-to-day living.</rdfs:comment>
</owl:Class>

<owl:Class rdf:ID= "GainingConsciousness">
<rdfs:subClassOf rdf:resource 
="http://127.0.0.1:8000/ontology/SUMO.owl#PsychologicalProcess"/>
<rdfs:comment>The process of transitioning from a state
of being Unconscious to a state of being Awake.</rdfs:comment>
</owl:Class>

<owl:Class rdf:ID= "GameArtifact">
<rdfs:subClassOf rdf:resource 
="http://127.0.0.1:8000/ontology/SUMO.owl#Artifact"/>
<rdfs:comment>An Artifact that is designed to be used
in a Game.</rdfs:comment>
</owl:Class>

<owl:Class rdf:ID= "GameAttribute">
<rdfs:subClassOf rdf:resource 
="http://127.0.0.1:8000/ontology/SUMO.owl#ContestAttribute"/>
<rdfs:comment>Any ContestAttribute that is specific
to a Game.</rdfs:comment>
</owl:Class>

<owl:Class rdf:ID= "GameBoard">
<rdfs:subClassOf rdf:resource ="#GameArtifact"/>
<rdfs:comment>A GameArtifact which is intended to be used as the
game area for playing a particular game.</rdfs:comment>
</owl:Class>

<owl:Class rdf:ID= "GameCall">
<rdfs:subClassOf rdf:resource 
="http://127.0.0.1:8000/ontology/SUMO.owl#Deciding"/>
<rdfs:subClassOf rdf:resource 
="http://127.0.0.1:8000/ontology/SUMO.owl#Declaring"/>
<rdfs:comment>A decision issued by an official referee in a
Game.  Note that GameCall is a subclass of Declaring, because these
decisions have binding, normative force.</rdfs:comment>
</owl:Class>

<owl:Class rdf:ID= "GameDie">
<rdfs:subClassOf rdf:resource ="#GamePiece"/>
<rdfs:comment>A small cube with 1 to 6 dots on each face that is
used to generate numbers at random in a Game.</rdfs:comment>
</owl:Class>

<owl:Class rdf:ID= "GameGoal">
<rdfs:subClassOf rdf:resource ="#GameArtifact"/>
<rdfs:comment>The location where a GameShot must end up if it
is to constitute a Score.</rdfs:comment>
</owl:Class>

<owl:Class rdf:ID= "GamePiece">
<rdfs:subClassOf rdf:resource ="#GameArtifact"/>
<rdfs:comment>A GameArtifact that is moved in a game area.</rdfs:comment>
</owl:Class>

<owl:Class rdf:ID= "GameReferee">
<rdfs:subClassOf rdf:resource ="#SkilledOccupation"/>
<rdfs:comment>A position which involves adjudicating contested
Maneuvers in a Game, i.e. deciding whether or not the Maneuvers are
permitted by the rules of the Game.</rdfs:comment>
</owl:Class>

<owl:Class rdf:ID= "GameShot">
<rdfs:subClassOf rdf:resource 
="http://127.0.0.1:8000/ontology/SUMO.owl#Impelling"/>
<rdfs:subClassOf rdf:resource 
="http://127.0.0.1:8000/ontology/SUMO.owl#Maneuver"/>
<rdfs:comment>Impelling a GamePiece for the purpose of
scoring a point or preventing the opposing player or team from scoring
a point.  Note that this class does not cover shots which are disallowed
by the rules of the game.</rdfs:comment>
</owl:Class>

<owl:Class rdf:ID= "Garage">
<rdfs:subClassOf rdf:resource 
="http://127.0.0.1:8000/ontology/SUMO.owl#StationaryArtifact"/>
<rdfs:comment>A Building or part of a Building which is intended
to house one or more Automobiles.</rdfs:comment>
</owl:Class>

<owl:Class rdf:ID= "Gasoline">
<rdfs:subClassOf rdf:resource ="#RefinedPetroleumProduct"/>
<rdfs:subClassOf rdf:resource ="#FossilFuel"/>
<rdfs:comment>Gasoline is the subclass of
RefinedPetroleumProducts that are fuels for internal combustion 
engines.</rdfs:comment>
</owl:Class>

<owl:Class rdf:ID= "GasolineEngine">
<rdfs:subClassOf rdf:resource ="#InternalCombustionEngine"/>
<rdfs:comment>GasolineEngine is the subclass of
InternalCombustionEngines that use Gasoline as their 
resource.</rdfs:comment>
</owl:Class>

<owl:Class rdf:ID= "Gastropod">
<rdfs:subClassOf rdf:resource 
="http://127.0.0.1:8000/ontology/SUMO.owl#Mollusk"/>
<rdfs:comment>A Mollusk with a distinct head that has no
shell (e.g. slugs) or a univalve shell (e.g. snails).</rdfs:comment>
</owl:Class>

<owl:Class rdf:ID= "GeneralElection">
<rdfs:subClassOf rdf:resource 
="http://127.0.0.1:8000/ontology/SUMO.owl#Election"/>
<rdfs:comment>GeneralElection is the subclass of
Elections that are held at regular intervals and in which all or most
constituencies of a GeopoliticalArea participate.</rdfs:comment>
</owl:Class>

<owl:Class rdf:ID= "Germanium">
<rdfs:subClassOf rdf:resource 
="http://127.0.0.1:8000/ontology/SUMO.owl#ElementalSubstance"/>
<atomicNumber>32</atomicNumber>
<rdfs:comment>Lustrous hard metalloid element, belongs to
group 14 of the periodic table.  Forms a large number of organometallic
compounds.  Predicted by Mendeleev in 1871, it was actually found in 1886
by Winkler.</rdfs:comment>
</owl:Class>

<owl:Class rdf:ID= "Girl">
<rdfs:subClassOf rdf:resource ="#HumanChild"/>
<rdfs:subClassOf rdf:resource ="http://127.0.0.1:8000/ontology/SUMO.owl#Woman"/>
<rdfs:comment>A HumanChild who is Female.</rdfs:comment>
</owl:Class>

<owl:Class rdf:ID= "Gland">
<rdfs:subClassOf rdf:resource ="http://127.0.0.1:8000/ontology/SUMO.owl#Organ"/>
<rdfs:subClassOf rdf:resource 
="http://127.0.0.1:8000/ontology/SUMO.owl#AnimalAnatomicalStructure"/>
<rdfs:comment>An Organ that removes Substances from the Blood,
alters them in some way, and then releases them.</rdfs:comment>
</owl:Class>

<owl:Class rdf:ID= "Glass">
<rdfs:subClassOf rdf:resource 
="http://127.0.0.1:8000/ontology/SUMO.owl#Mixture"/>
<rdfs:comment>A transparent or translucent Mixture of 
silicates.</rdfs:comment>
</owl:Class>

<owl:Class rdf:ID= "Glove">
<rdfs:subClassOf rdf:resource 
="http://127.0.0.1:8000/ontology/SUMO.owl#Clothing"/>
<rdfs:comment>Clothing that is intended to be worn on the Hand.
Note that this class covers both gloves which have individual compartments
for each of the Fingers and mittens.</rdfs:comment>
</owl:Class>

<owl:Class rdf:ID= "Glue">
<rdfs:subClassOf rdf:resource 
="http://127.0.0.1:8000/ontology/SUMO.owl#Solution"/>
<rdfs:comment>Any Solution whose purpose is to be used as the instrument
of Attaching one thing to another or one part of something to another 
part.</rdfs:comment>
</owl:Class>

<owl:Class rdf:ID= "Goat">
<rdfs:subClassOf rdf:resource 
="http://127.0.0.1:8000/ontology/SUMO.owl#HoofedMammal"/>
<rdfs:subClassOf rdf:resource ="#DomesticAnimal"/>
<rdfs:comment>A domesticated HoofedMammal that is raised primarily
for milk.</rdfs:comment>
</owl:Class>

<owl:Class rdf:ID= "Gold">
<rdfs:subClassOf rdf:resource 
="http://127.0.0.1:8000/ontology/SUMO.owl#ElementalSubstance"/>
<atomicNumber>79</atomicNumber>
<rdfs:comment>Gold is gold colored.  It is the most malleable and
ductile metal known.  There is only one stable isotope of gold, and five
radioisotopes of gold, Au-195 being the most stable with a half-life of
186 days.  Gold is used as a monetary standard, in jewelry, dentistry,
electronics.  Au-198 is used in treating cancer and some other medical
conditions.  Gold has been known to exist as far back as 2600 BC.  Gold
comes from the Anglo-Saxon word gold.  Its symbol, Au, comes from the
Latin word aurum, which means gold.  Gold is not particularly toxic,
however it is known to cause damage to the liver and kidneys in 
some.</rdfs:comment>
</owl:Class>

<owl:Class rdf:ID= "Golf">
<rdfs:subClassOf rdf:resource ="http://127.0.0.1:8000/ontology/SUMO.owl#Sport"/>
<rdfs:comment>A sport which has a course of 9 or 18 holes and where
the object is to hit a ball with a club into each hole in turn with the 
fewest
number of strokes.</rdfs:comment>
</owl:Class>

<owl:Class rdf:ID= "GolfHole">
<rdfs:subClassOf rdf:resource ="#GolfManeuver"/>
<rdfs:comment>A division of a Golf game.  A normal game
consists of 9 to 18 holes, and each hole involves a turn for each of
the players in the Golf game.</rdfs:comment>
</owl:Class>

<owl:Class rdf:ID= "GolfManeuver">
<rdfs:subClassOf rdf:resource 
="http://127.0.0.1:8000/ontology/SUMO.owl#Maneuver"/>
<rdfs:comment>Any Maneuver in Golf.</rdfs:comment>
</owl:Class>

<owl:Class rdf:ID= "Goose">
<rdfs:subClassOf rdf:resource ="http://127.0.0.1:8000/ontology/SUMO.owl#Bird"/>
<rdfs:comment>A subclass of Bird with webbed feet and a long neck
and a large body.  These Birds are often raised for their 
meat.</rdfs:comment>
</owl:Class>

<owl:Class rdf:ID= "GovernmentOfficer">
<rdfs:subClassOf rdf:resource ="#Profession"/>
<rdfs:comment>Any Profession where the position occupied
is within a GovernmentOrganization.</rdfs:comment>
</owl:Class>

<owl:Class rdf:ID= "GovernmentSecretary">
<rdfs:subClassOf rdf:resource ="#SkilledOccupation"/>
<rdfs:comment>The class of Positions where the position holder
is head of an adminstrative department of Government.</rdfs:comment>
</owl:Class>

<owl:Class rdf:ID= "GraduateSchool">
<rdfs:subClassOf rdf:resource ="#PostSecondarySchool"/>
<rdfs:comment>A School which is devoted to a specific
subject area, which admits students that have a bachelor's degree, which
grants masters and/or doctorate degrees, and which is part of a 
University.</rdfs:comment>
</owl:Class>

<owl:Class rdf:ID= "Graph">
<rdfs:subClassOf rdf:resource 
="http://127.0.0.1:8000/ontology/SUMO.owl#Abstract"/>
<rdfs:comment>The Class of graphs, where a graph is understood
to be a set of GraphNodes connected by GraphArcs.  Note that this
Class includes only connected graphs, i.e. graphs in which there is a
GraphPath between any two GraphNodes.  Note too that every Graph
is assumed to contain at least two GraphArcs and three 
GraphNodes.</rdfs:comment>
</owl:Class>

<owl:Class rdf:ID= "GraphArc">
<rdfs:subClassOf rdf:resource ="#GraphElement"/>
<rdfs:comment>Graphs are comprised of GraphNodes
and GraphArcs.  Every GraphArc links two GraphNodes.</rdfs:comment>
</owl:Class>

<owl:Class rdf:ID= "GraphCircuit">
<rdfs:subClassOf rdf:resource ="#GraphPath"/>
<rdfs:comment>A GraphPath that begins (see
BeginNodeFn) and ends (see EndNodeFn) at the same
GraphNode.</rdfs:comment>
</owl:Class>

<owl:Class rdf:ID= "GraphDiagram">
<rdfs:subClassOf rdf:resource ="http://127.0.0.1:8000/ontology/SUMO.owl#Icon"/>
<rdfs:comment>An Icon which depicts one or more quantities.</rdfs:comment>
</owl:Class>

<owl:Class rdf:ID= "GraphElement">
<rdfs:subClassOf rdf:resource 
="http://127.0.0.1:8000/ontology/SUMO.owl#Abstract"/>
<rdfs:comment>Noncompositional parts of Graphs.
These parts are restricted to GraphNodes and GraphArcs.</rdfs:comment>
</owl:Class>

<owl:Class rdf:ID= "GraphLoop">
<rdfs:subClassOf rdf:resource ="#GraphArc"/>
<rdfs:comment>A GraphArc in which a GraphNode is
linked to itself.</rdfs:comment>
</owl:Class>

<owl:Class rdf:ID= "GraphNode">
<rdfs:subClassOf rdf:resource ="#GraphElement"/>
<rdfs:comment>Graphs are comprised of GraphNodes
and GraphArcs.  Every GraphNode is linked by a GraphArc.</rdfs:comment>
</owl:Class>

<owl:Class rdf:ID= "GraphPath">
<rdfs:subClassOf rdf:resource ="#DirectedGraph"/>
<rdfs:comment>Informally, a single, directed route between
two GraphNodes in a Graph.  Formally, a DirectedGraph that is a
subGraph of the original Graph and such that no two GraphArcs in
the DirectedGraph have the same intial node (see InitialNodeFn) or
the same terminal node (see TerminalNodeFn).</rdfs:comment>
</owl:Class>

<owl:Class rdf:ID= "Grass">
<rdfs:subClassOf rdf:resource 
="http://127.0.0.1:8000/ontology/SUMO.owl#FloweringPlant"/>
<rdfs:comment>FloweringPlants with green, narrow leaves that are
used for lawns and Fields.</rdfs:comment>
</owl:Class>

<owl:Class rdf:ID= "Grasshopper">
<rdfs:subClassOf rdf:resource ="http://127.0.0.1:8000/ontology/SUMO.owl#Insect"/>
<rdfs:comment>Insects with enormous legs that are used for
jumping.</rdfs:comment>
</owl:Class>

<owl:Class rdf:ID= "Gray">
<rdf:type rdf:resource = "#SecondaryColor"/>
<rdfs:comment>A SecondaryColor that results from mixing Black and
White.</rdfs:comment>
<rdfs:subClassOf rdf:resource 
="http://127.0.0.1:8000/ontology/SUMO.owl#FunctionQuantity"/>
<rdf:type rdf:resource = 
"http://127.0.0.1:8000/ontology/SUMO.owl#SystemeInternationalUnit"/>
<rdfs:comment>SI absorbed dose measure.  Symbol: Gy.  It measures
the dose of radiation absorbed in living tissue. It is equal approximately
to the absorbed dose delivered when the energy per unit mass imparted to
matter by ionizing radiation is 1 Joule per kilogram.  Gray = J/kg
= m^2*s^(-2).</rdfs:comment>
</owl:Class>

<owl:Class rdf:ID= "Greeting">
<rdfs:subClassOf rdf:resource 
="http://127.0.0.1:8000/ontology/SUMO.owl#Expressing"/>
<rdfs:comment>Any instance of Expressing an acknowledgment of a
person's arrival.  Note that this class is not a subclass of 
LinguisticCommunication,
because it covers gestures of greeting, e.g. Waving and Nodding in certain
circumstances.</rdfs:comment>
</owl:Class>

<owl:Class rdf:ID= "GroceryStore">
<rdfs:subClassOf rdf:resource ="#RetailStore"/>
<rdfs:comment>A RetailStore that sells Food, and perhaps
other items as well.</rdfs:comment>
</owl:Class>

<owl:Class rdf:ID= "GroupOfAnimals">
<rdfs:subClassOf rdf:resource ="http://127.0.0.1:8000/ontology/SUMO.owl#Group"/>
<rdfs:comment>Any Group which contains exclusively
non-human members.</rdfs:comment>
</owl:Class>

<owl:Class rdf:ID= "Guitar">
<rdfs:subClassOf rdf:resource ="#StringInstrument"/>
<rdfs:comment>A StringInstrument that has six to twelve strings and
is played by strumming with one hand while grasping frets with the other 
hand.</rdfs:comment>
</owl:Class>

<owl:Class rdf:ID= "Gulf">
<rdfs:subClassOf rdf:resource ="#BodyOfWater"/>
<rdfs:subClassOf rdf:resource 
="http://127.0.0.1:8000/ontology/SUMO.owl#SaltWaterArea"/>
<rdfs:comment>Gulf is the class of extensions of a Sea or
Ocean that reach into a land mass or are partially enclosed by a
LandArea.</rdfs:comment>
</owl:Class>

<owl:Class rdf:ID= "Gun">
<rdfs:subClassOf rdf:resource ="#ProjectileLauncher"/>
<rdfs:comment>A ProjectileLauncher that shoots Bullets.</rdfs:comment>
</owl:Class>

<owl:Class rdf:ID= "GunBarrel">
<rdfs:subClassOf rdf:resource 
="http://127.0.0.1:8000/ontology/SUMO.owl#EngineeringComponent"/>
<rdfs:comment>The part of a Gun through which a Projectile travels
when it is fired.</rdfs:comment>
</owl:Class>

<owl:Class rdf:ID= "GunPowder">
<rdfs:subClassOf rdf:resource 
="http://127.0.0.1:8000/ontology/SUMO.owl#Mixture"/>
<rdfs:comment>A Mixture of potassium nitrate, sulfur, and
charcoal that is used in ExplosiveDevices and to propell Projectiles
in ProjectileWeapons.</rdfs:comment>
</owl:Class>

<owl:Class rdf:ID= "GunStock">
<rdfs:subClassOf rdf:resource 
="http://127.0.0.1:8000/ontology/SUMO.owl#EngineeringComponent"/>
<rdfs:comment>The part of a Gun that is placed against the
shoulder to absorb some of the recoil action when it is 
fired.</rdfs:comment>
</owl:Class>

<owl:Class rdf:ID= "GunTrigger">
<rdfs:subClassOf rdf:resource 
="http://127.0.0.1:8000/ontology/SUMO.owl#EngineeringComponent"/>
<rdfs:comment>The part of the Gun which is pulled in Shooting
the Gun.</rdfs:comment>
</owl:Class>

<owl:Class rdf:ID= "Gymnastics">
<rdfs:subClassOf rdf:resource ="http://127.0.0.1:8000/ontology/SUMO.owl#Sport"/>
<rdfs:comment>A sport which involves exercises of agility on a
range of gymnastic equipment.</rdfs:comment>
</owl:Class>

<owl:Class rdf:ID= "Hailing">
<rdfs:subClassOf rdf:resource 
="http://127.0.0.1:8000/ontology/SUMO.owl#Precipitation"/>
<rdfs:comment>Hailing is a precipitation process
in which water falls in a Solid state with round, hard 
pellets.</rdfs:comment>
</owl:Class>

<owl:Class rdf:ID= "Hair">
<rdfs:subClassOf rdf:resource 
="http://127.0.0.1:8000/ontology/SUMO.owl#AnimalAnatomicalStructure"/>
<rdfs:comment>A filament that covers part of the body of many
Mammals.</rdfs:comment>
</owl:Class>

<owl:Class rdf:ID= "HairRemoval">
<rdfs:subClassOf rdf:resource 
="http://127.0.0.1:8000/ontology/SUMO.owl#Removing"/>
<rdfs:comment>Removing (some or all) the Hair from the
body of an Animal.  Note that this covers shaving hair, cutting hair,
pulling hair out by the roots, etc.</rdfs:comment>
</owl:Class>

<owl:Class rdf:ID= "Hammer">
<rdfs:subClassOf rdf:resource ="http://127.0.0.1:8000/ontology/SUMO.owl#Device"/>
<rdfs:comment>A Device that is used to pound Nails into a
surface, where they become firmly attached.</rdfs:comment>
</owl:Class>

<owl:Class rdf:ID= "Hand">
<rdfs:subClassOf rdf:resource 
="http://127.0.0.1:8000/ontology/SUMO.owl#AnimalAnatomicalStructure"/>
<rdfs:subClassOf rdf:resource 
="http://127.0.0.1:8000/ontology/SUMO.owl#BodyPart"/>
<rdfs:comment>The grasping, fingered part of an upper limb of a
Primate.</rdfs:comment>
</owl:Class>

<owl:Class rdf:ID= "HandGesture">
<rdfs:subClassOf rdf:resource 
="http://127.0.0.1:8000/ontology/SUMO.owl#Gesture"/>
<rdfs:comment>Any Gesture which involves the Hands.</rdfs:comment>
</owl:Class>

<owl:Class rdf:ID= "Handle">
<rdfs:subClassOf rdf:resource 
="http://127.0.0.1:8000/ontology/SUMO.owl#EngineeringComponent"/>
<rdfs:comment>The part or parts of an Artifact that are designed to be
held with the Hands when the Artifact is used or carried.</rdfs:comment>
</owl:Class>

<owl:Class rdf:ID= "Hanging">
<rdfs:subClassOf rdf:resource ="#Suffocating"/>
<rdfs:comment>Suffocating someone by suspending him/her from
a rope wound around the neck until asphyxiation occurs.</rdfs:comment>
</owl:Class>

<owl:Class rdf:ID= "HardDiskDrive">
<rdfs:subClassOf rdf:resource ="#ComputerHardware"/>
<rdfs:comment>The primary computer storage medium, which
is made of one or more aluminum or glass platters, coated with a
ferromagnetic material. Most hard disks are fixed disks, which are
permanently sealed in the drive.</rdfs:comment>
</owl:Class>

<owl:Class rdf:ID= "Harvesting">
<rdfs:subClassOf rdf:resource 
="http://127.0.0.1:8000/ontology/SUMO.owl#Removing"/>
<rdfs:comment>Gathering the plant results of Agriculture.</rdfs:comment>
</owl:Class>

<owl:Class rdf:ID= "Hat">
<rdfs:subClassOf rdf:resource ="#OutdoorClothing"/>
<rdfs:comment>A type of Clothing that is worn on the Head.  Note
that this class covers caps, bonnets, berets, etc.</rdfs:comment>
</owl:Class>

<owl:Class rdf:ID= "Hay">
<rdfs:subClassOf rdf:resource ="#Fodder"/>
<rdfs:comment>Grass that has been cut and cured for use as 
Fodder.</rdfs:comment>
</owl:Class>

<owl:Class rdf:ID= "Head">
<rdfs:subClassOf rdf:resource 
="http://127.0.0.1:8000/ontology/SUMO.owl#AnimalAnatomicalStructure"/>
<rdfs:subClassOf rdf:resource 
="http://127.0.0.1:8000/ontology/SUMO.owl#BodyPart"/>
<rdfs:comment>The part of the body containing the sense organs and
the brain.</rdfs:comment>
</owl:Class>

<owl:Class rdf:ID= "Headlight">
<rdfs:subClassOf rdf:resource ="#VehicleLight"/>
<rdfs:comment>Any VehicleLight which is attached to the front
of a Vehicle.</rdfs:comment>
</owl:Class>

<owl:Class rdf:ID= "Heart">
<rdfs:subClassOf rdf:resource ="http://127.0.0.1:8000/ontology/SUMO.owl#Organ"/>
<rdfs:subClassOf rdf:resource 
="http://127.0.0.1:8000/ontology/SUMO.owl#AnimalAnatomicalStructure"/>
<rdfs:comment>The Organ that pumps Blood throughout the body.</rdfs:comment>
</owl:Class>

<owl:Class rdf:ID= "HeatingDevice">
<rdfs:subClassOf rdf:resource ="http://127.0.0.1:8000/ontology/SUMO.owl#Device"/>
<rdfs:comment>A Device whose purpose is Heating something,
e.g. electric heaters, heat lamps, ovens, stoves, etc.</rdfs:comment>
</owl:Class>

<owl:Class rdf:ID= "Helicopter">
<rdfs:subClassOf rdf:resource ="#Aircraft"/>
<rdfs:comment>Any Aircraft with rapidly rotating wings.</rdfs:comment>
</owl:Class>

<owl:Class rdf:ID= "Helium">
<rdfs:subClassOf rdf:resource 
="http://127.0.0.1:8000/ontology/SUMO.owl#ElementalSubstance"/>
<atomicNumber>2</atomicNumber>
<rdfs:comment>Colourless, odourless gaseous nonmetallic element.
Belongs to group 18 of the periodic table.  Lowest boiling point of all
elements and can only be solidified under pressure.  Chemically inert, no
known compounds.  Discovered in the solar spectrum in 1868 by 
Lockyer.</rdfs:comment>
</owl:Class>

<owl:Class rdf:ID= "Hemisphere">
<rdfs:subClassOf rdf:resource 
="http://127.0.0.1:8000/ontology/SUMO.owl#GeographicArea"/>
<rdfs:comment>Any half of the PlanetEarth, e.g. the northern
hemisphere, the southern hemisphere, the eastern hemisphere or the western
hemisphere.</rdfs:comment>
</owl:Class>

<owl:Class rdf:ID= "Hen">
<rdfs:subClassOf rdf:resource ="#Chicken"/>
<rdfs:comment>A Female Chicken.</rdfs:comment>
</owl:Class>

<owl:Class rdf:ID= "Henry">
<rdfs:subClassOf rdf:resource 
="http://127.0.0.1:8000/ontology/SUMO.owl#FunctionQuantity"/>
<rdf:type rdf:resource = 
"http://127.0.0.1:8000/ontology/SUMO.owl#SystemeInternationalUnit"/>
<rdfs:comment>SI inductance measure.  Symbol: H.  One Henry
is equivalent to one Volt divided by one Ampere per SecondDuration.
If a current changing at the rate of one Ampere per SecondDuration
induces an electromotive force of one Volt, the circuit has an
inductance of one Henry.  Henry = Wb/A = 
m^2*kg*s^(-2)*A^(-2).</rdfs:comment>
</owl:Class>

<owl:Class rdf:ID= "Herbivore">
<rdfs:subClassOf rdf:resource ="http://127.0.0.1:8000/ontology/SUMO.owl#Mammal"/>
<sumo:disjoint rdf:resource = "http://127.0.0.1:8000/ontology/SUMO.owl#Carnivore"
/>
<rdfs:comment>A plant-eating Mammal.</rdfs:comment>
</owl:Class>

<owl:Class rdf:ID= "HighTide">
<rdfs:subClassOf rdf:resource ="#TidalProcess"/>
<rdfs:comment>HighTide is the class of TidalProcesses that
occur twice a day in marine waters, in which the water level rises above
the mean sea level.</rdfs:comment>
</owl:Class>

<owl:Class rdf:ID= "Hijacking">
<rdfs:subClassOf rdf:resource ="#Robbing"/>
<rdfs:comment>Robbing a Vehicle and then driving it away.</rdfs:comment>
</owl:Class>

<owl:Class rdf:ID= "Hinge">
<rdfs:subClassOf rdf:resource 
="http://127.0.0.1:8000/ontology/SUMO.owl#EngineeringComponent"/>
<rdfs:comment>An EngineeringComponent that connects one thing to
another in such a way that they can move relative to one 
another.</rdfs:comment>
</owl:Class>

<owl:Class rdf:ID= "HistoricalAccount">
<rdfs:subClassOf rdf:resource 
="http://127.0.0.1:8000/ontology/SUMO.owl#FactualText"/>
<rdfs:subClassOf rdf:resource ="#NarrativeText"/>
<rdfs:comment>A FactualAccount that describes
events that are believed by the author of the account to have
occurred in the past.</rdfs:comment>
</owl:Class>

<owl:Class rdf:ID= "HoistingDevice">
<rdfs:subClassOf rdf:resource ="#MaterialHandlingEquipment"/>
<rdfs:comment>HoistingDevice is a subclass of
mechanical Devices that provide a mechanical advantage in lifting
and lowering, e.g., by use of a block and tackle.</rdfs:comment>
</owl:Class>

<owl:Class rdf:ID= "Holder">
<rdfs:subClassOf rdf:resource ="http://127.0.0.1:8000/ontology/SUMO.owl#Device"/>
<rdfs:comment>A large class of Devices whose purpose is to hold
something else, i.e. be the instrument of a Keeping.</rdfs:comment>
</owl:Class>

<owl:Class rdf:ID= "Holiday">
<rdfs:subClassOf rdf:resource 
="http://127.0.0.1:8000/ontology/SUMO.owl#TimeInterval"/>
<rdfs:comment>Holiday is the class of time periods that are
observed as holidays in a country, culture, or religion.  Holidays may
recur annually on the same date, or they may be moveable, for example,
Thanksgiving Day falls on the last Thursday of each November.</rdfs:comment>
</owl:Class>

<owl:Class rdf:ID= "HolidayCard">
<rdfs:subClassOf rdf:resource 
="http://127.0.0.1:8000/ontology/SUMO.owl#ContentBearingObject"/>
<rdfs:comment>A stiff piece of Paper, usually folded over, which
is sent to others in celebration of a Holiday.</rdfs:comment>
</owl:Class>

<owl:Class rdf:ID= "Holster">
<rdfs:subClassOf rdf:resource ="#Container"/>
<rdfs:comment>A Container for a Pistol.  It is generally made of
Leather and worn on either the shoulder or the waist.</rdfs:comment>
</owl:Class>

<owl:Class rdf:ID= "HomeBase">
<rdfs:subClassOf rdf:resource ="#BaseballBase"/>
<rdfs:comment>The final BaseballBase which must be touched
by the batter in order to achieve a BaseballRun.</rdfs:comment>
</owl:Class>

<owl:Class rdf:ID= "HomeRun">
<rdfs:subClassOf rdf:resource ="#BaseballRun"/>
<rdfs:comment>A BaseballRun where the batter touches home base
during his turn at bat.</rdfs:comment>
</owl:Class>

<owl:Class rdf:ID= "Honey">
<rdfs:subClassOf rdf:resource 
="http://127.0.0.1:8000/ontology/SUMO.owl#AnimalSubstance"/>
<rdfs:subClassOf rdf:resource ="http://127.0.0.1:8000/ontology/SUMO.owl#Food"/>
<rdfs:comment>An edible, sweet Substance produced by some species of
Bees.</rdfs:comment>
</owl:Class>

<owl:Class rdf:ID= "Hoof">
<rdfs:subClassOf rdf:resource 
="http://127.0.0.1:8000/ontology/SUMO.owl#AnimalAnatomicalStructure"/>
<rdfs:subClassOf rdf:resource 
="http://127.0.0.1:8000/ontology/SUMO.owl#BodyPart"/>
<rdfs:comment>The hard end of the Foot of a HoofedMammal.</rdfs:comment>
</owl:Class>

<owl:Class rdf:ID= "Hormone">
<rdfs:subClassOf rdf:resource 
="http://127.0.0.1:8000/ontology/SUMO.owl#BodySubstance"/>
<rdfs:subClassOf rdf:resource 
="http://127.0.0.1:8000/ontology/SUMO.owl#BiologicallyActiveSubstance"/>
<rdfs:comment>In Animals, a chemical secreted by an
endocrine gland whose products are released into the circulating fluid.
Plant hormones or synthetic hormones which are used only to alter or
control various physiologic processes, e.g., reproductive control agents,
are assigned to the Class BiologicallyActiveSubstance. Hormones act as
chemical messengers and regulate various physiologic processes such as
growth, reproduction, metabolism, etc.  They usually fall into two broad
categories, viz. steroid hormones and peptide hormones.</rdfs:comment>
</owl:Class>

<owl:Class rdf:ID= "Horn">
<rdfs:subClassOf rdf:resource ="http://127.0.0.1:8000/ontology/SUMO.owl#Bone"/>
<rdfs:comment>An outgrowth of Bone that is found on some
HoofedMammals.</rdfs:comment>
</owl:Class>

<owl:Class rdf:ID= "HornInstrument">
<rdfs:subClassOf rdf:resource 
="http://127.0.0.1:8000/ontology/SUMO.owl#MusicalInstrument"/>
<rdfs:comment>A MusicalInstrument which is played by
blowing it and which does not use a reed.</rdfs:comment>
</owl:Class>

<owl:Class rdf:ID= "Horse">
<rdfs:subClassOf rdf:resource ="#DomesticAnimal"/>
<rdfs:subClassOf rdf:resource 
="http://127.0.0.1:8000/ontology/SUMO.owl#HoofedMammal"/>
<rdfs:comment>A domesticated HoofedMammal that is used for
transportation and work.</rdfs:comment>
</owl:Class>

<owl:Class rdf:ID= "HorseRiding">
<rdfs:subClassOf rdf:resource 
="http://127.0.0.1:8000/ontology/SUMO.owl#Carrying"/>
<rdfs:comment>Any instance of Carrying where the Animal is
a Horse.</rdfs:comment>
</owl:Class>

<owl:Class rdf:ID= "Horsepower">
<rdfs:subClassOf rdf:resource 
="http://127.0.0.1:8000/ontology/SUMO.owl#FunctionQuantity"/>
<rdf:type rdf:resource = 
"http://127.0.0.1:8000/ontology/SUMO.owl#UnitOfMeasure"/>
<rdfs:comment>A power measure that is equal to 746 Watts.</rdfs:comment>
</owl:Class>

<owl:Class rdf:ID= "Hospital">
<rdfs:subClassOf rdf:resource ="#CareOrganization"/>
<rdfs:subClassOf rdf:resource 
="http://127.0.0.1:8000/ontology/SUMO.owl#TemporaryResidence"/>
<rdfs:comment>A CareOrganization where patients reside for a
short period of time while they undergo treatment for a disease or 
disorder.</rdfs:comment>
</owl:Class>

<owl:Class rdf:ID= "House">
<rdfs:subClassOf rdf:resource 
="http://127.0.0.1:8000/ontology/SUMO.owl#ResidentialBuilding"/>
<rdfs:subClassOf rdf:resource 
="http://127.0.0.1:8000/ontology/SUMO.owl#SingleFamilyResidence"/>
<rdfs:comment>A ResidentialBuilding which is intended to be
inhabited by members of the same SocialUnit.  Houses are distinguished
from temporary housing like hotels and multi-family dwellings like 
condominium
and apartment buildings.</rdfs:comment>
</owl:Class>

<owl:Class rdf:ID= "HumanAdult">
<rdfs:subClassOf rdf:resource ="http://127.0.0.1:8000/ontology/SUMO.owl#Human"/>
<rdfs:comment>The class of Humans that are 18 years of
age or older.</rdfs:comment>
</owl:Class>

<owl:Class rdf:ID= "HumanChild">
<rdfs:subClassOf rdf:resource ="#HumanYouth"/>
<rdfs:comment>A HumanYouth between birth and puberty, i.e a
Human who is NonFullyFormed.</rdfs:comment>
</owl:Class>

<owl:Class rdf:ID= "HumanCorpse">
<rdfs:subClassOf rdf:resource ="http://127.0.0.1:8000/ontology/SUMO.owl#Human"/>
<rdfs:comment>A Human which is Dead.</rdfs:comment>
</owl:Class>

<owl:Class rdf:ID= "HumanInfant">
<rdfs:subClassOf rdf:resource ="#HumanChild"/>
<rdfs:comment>A Human between birth and the first year of 
age.</rdfs:comment>
</owl:Class>

<owl:Class rdf:ID= "HumanSlave">
<rdfs:subClassOf rdf:resource ="http://127.0.0.1:8000/ontology/SUMO.owl#Human"/>
<rdfs:comment>A Human who is owned by someone else.</rdfs:comment>
</owl:Class>

<owl:Class rdf:ID= "HumanYouth">
<rdfs:subClassOf rdf:resource ="http://127.0.0.1:8000/ontology/SUMO.owl#Human"/>
<rdfs:comment>The class of Humans that are younger than
18 years of age.</rdfs:comment>
</owl:Class>

<owl:Class rdf:ID= "Humus">
<rdfs:subClassOf rdf:resource 
="http://127.0.0.1:8000/ontology/SUMO.owl#Mixture"/>
<rdfs:comment>Humus is decaying organic matter found in Soil and derived
from dead animal and plant material.</rdfs:comment>
</owl:Class>

<owl:Class rdf:ID= "Hunting">
<rdfs:subClassOf rdf:resource 
="http://127.0.0.1:8000/ontology/SUMO.owl#Pursuing"/>
<rdfs:comment>Hunting is the class of Processes in which
an animal or animals are pursued and sometimes captured and/or 
killed.</rdfs:comment>
</owl:Class>

<owl:Class rdf:ID= "Hydrocarbon">
<rdfs:subClassOf rdf:resource ="#OrganicCompound"/>
<rdfs:comment>Any OrganicCompound that contains only Carbon
and Hydrogen.</rdfs:comment>
</owl:Class>

<owl:Class rdf:ID= "Hydrogen">
<rdfs:subClassOf rdf:resource 
="http://127.0.0.1:8000/ontology/SUMO.owl#ElementalSubstance"/>
<atomicNumber>1</atomicNumber>
<rdfs:comment>Colourless, odourless gaseous chemical element.
Lightest and most abundant element in the universe.  Present in water and
in all organic compounds.  Chemically reacts with most elements.
Discovered by Henry Cavendish in 1776.</rdfs:comment>
</owl:Class>

<owl:Class rdf:ID= "Hypothalamus">
<rdfs:subClassOf rdf:resource 
="http://127.0.0.1:8000/ontology/SUMO.owl#BodyPart"/>
<rdfs:subClassOf rdf:resource 
="http://127.0.0.1:8000/ontology/SUMO.owl#AnimalAnatomicalStructure"/>
<rdfs:comment>The part of the Brain lying below the
thalamus that serves to regulate AutonomicProcesses.</rdfs:comment>
</owl:Class>

<owl:Class rdf:ID= "Ice">
<rdfs:subClassOf rdf:resource ="http://127.0.0.1:8000/ontology/SUMO.owl#Water"/>
<rdfs:comment>Water that has the PhysicalState of Solid.</rdfs:comment>
</owl:Class>

<owl:Class rdf:ID= "IlluminationDevice">
<rdfs:subClassOf rdf:resource ="http://127.0.0.1:8000/ontology/SUMO.owl#Device"/>
<rdfs:comment>Any Device whose purpose is to be a source of
visible light.</rdfs:comment>
</owl:Class>

<owl:Class rdf:ID= "Imagining">
<rdfs:subClassOf rdf:resource 
="http://127.0.0.1:8000/ontology/SUMO.owl#PsychologicalProcess"/>
<rdfs:comment>Forming a mental picture of something which
is not present.</rdfs:comment>
</owl:Class>

<owl:Class rdf:ID= "Immigrating">
<rdfs:subClassOf rdf:resource 
="http://127.0.0.1:8000/ontology/SUMO.owl#Translocation"/>
<rdfs:comment>Any Translocation by a Human from one Nation
to another Nation where the person is not a citizen for the purpose of 
taking
up residence.</rdfs:comment>
</owl:Class>

<owl:Class rdf:ID= "Imprisoning">
<rdfs:subClassOf rdf:resource 
="http://127.0.0.1:8000/ontology/SUMO.owl#Confining"/>
<rdfs:comment>The class of Confining processes where the detainee
is put in Prison.</rdfs:comment>
</owl:Class>

<owl:Class rdf:ID= "InchMercury">
<rdfs:subClassOf rdf:resource ="#AtmosphericPressureMeasure"/>
<rdf:type rdf:resource = 
"http://127.0.0.1:8000/ontology/SUMO.owl#UnitOfMeasure"/>
<rdfs:comment>InchMercury is a UnitOfMeasure
for barometricPressure.  It is used to express the number of
inches of mercury supported in a mercurial barometer by the
surrounding air pressure.</rdfs:comment>
</owl:Class>

<owl:Class rdf:ID= "Inclining">
<rdfs:subClassOf rdf:resource 
="http://127.0.0.1:8000/ontology/SUMO.owl#BodyMotion"/>
<rdfs:subClassOf rdf:resource ="#MotionDownward"/>
<rdfs:comment>Moving one's body downward from a vertical position.
Note that this class covers cases of leaning forward, as well as those of
reclining backwards.</rdfs:comment>
</owl:Class>

<owl:Class rdf:ID= "IncomeTax">
<rdfs:subClassOf rdf:resource ="#Tax"/>
<rdfs:comment>A Tax on annual income.</rdfs:comment>
</owl:Class>

<owl:Class rdf:ID= "IndependentState">
<rdfs:subClassOf rdf:resource 
="http://127.0.0.1:8000/ontology/SUMO.owl#GeopoliticalArea"/>
<rdfs:subClassOf rdf:resource ="http://127.0.0.1:8000/ontology/SUMO.owl#Nation"/>
<sumo:disjoint rdf:resource = "#DependencyOrSpecialSovereigntyArea" />
<rdfs:comment>IndependentState is a subclass of
GeopoliticalArea, representing the classification 'Independent State'
used by the CIA World Fact Book.</rdfs:comment>
</owl:Class>

<owl:Class rdf:ID= "Indicating">
<rdfs:subClassOf rdf:resource 
="http://127.0.0.1:8000/ontology/SUMO.owl#Communication"/>
<rdfs:subClassOf rdf:resource 
="http://127.0.0.1:8000/ontology/SUMO.owl#BodyMotion"/>
<rdfs:comment>Pointing out a person, place or thing with
a BodyPart or with an Artifact.</rdfs:comment>
</owl:Class>

<owl:Class rdf:ID= "IndividualRetirementAccount">
<rdfs:subClassOf rdf:resource ="#PensionPlan"/>
<rdfs:comment>A tax-deferred retirement
account for an individual that permits individuals to set aside a certain
amount per year, with earnings tax-deferred until withdrawals at retirement
age(or earlier, with a penalty).  Only those who do not participate in a
pension plan at work or who do participate and meet certain income 
guidelines
can make deductible contributions to an IRA.  All others can make 
contributions
to an IRA on a non-deductible basis.  Such contributions qualify as a 
deduction
against income earned in that year and interest accumulates tax-deferred 
until
the funds are withdrawn.</rdfs:comment>
</owl:Class>

<owl:Class rdf:ID= "IndustrialPlant">
<rdfs:subClassOf rdf:resource 
="http://127.0.0.1:8000/ontology/SUMO.owl#StationaryArtifact"/>
<rdfs:comment>A Building or part of a Building or group
of Buildings whose purpose is to Manufacture something.</rdfs:comment>
</owl:Class>

<owl:Class rdf:ID= "Industry">
<rdfs:subClassOf rdf:resource 
="http://127.0.0.1:8000/ontology/SUMO.owl#Collection"/>
<rdfs:comment>The class of Collections of Corporations
which are in the same line of business.</rdfs:comment>
</owl:Class>

<owl:Class rdf:ID= "InfantryUnit">
<rdfs:subClassOf rdf:resource ="#MilitaryUnit"/>
<rdfs:comment>MilitaryUnits composed primarily of Soldiers
who fight on foot, i.e. without the use of ArtilleryGuns.</rdfs:comment>
</owl:Class>

<owl:Class rdf:ID= "InfectiousDisease">
<rdfs:subClassOf rdf:resource 
="http://127.0.0.1:8000/ontology/SUMO.owl#DiseaseOrSyndrome"/>
<rdfs:comment>Any DiseaseOrSyndrome that is caused by a
Microorganism.</rdfs:comment>
</owl:Class>

<owl:Class rdf:ID= "Inhaling">
<rdfs:subClassOf rdf:resource 
="http://127.0.0.1:8000/ontology/SUMO.owl#Breathing"/>
<rdfs:comment>Any instance of Breathing where the breath is
taken into the Lungs.</rdfs:comment>
</owl:Class>

<owl:Class rdf:ID= "Inheriting">
<rdfs:subClassOf rdf:resource 
="http://127.0.0.1:8000/ontology/SUMO.owl#UnilateralGetting"/>
<rdfs:comment>Any UnilateralGetting where the agent
receives some part of the property of a person upon the death of the
person.</rdfs:comment>
</owl:Class>

<owl:Class rdf:ID= "Inlet">
<rdfs:subClassOf rdf:resource ="#BodyOfWater"/>
<rdfs:comment>Inlet is the class of bays or other recesses
into the shore of a lake, sea, or river; includes narrow inlets, which
are passages leading from open water through some barrier to a bay or
lagoon.</rdfs:comment>
</owl:Class>

<owl:Class rdf:ID= "Installing">
<rdfs:subClassOf rdf:resource 
="http://127.0.0.1:8000/ontology/SUMO.owl#Putting"/>
<rdfs:comment>Putting a Device in a location and configuring
the Device so that it can be used as intended after the 
installation.</rdfs:comment>
</owl:Class>

<owl:Class rdf:ID= "InstrumentalMusic">
<rdfs:subClassOf rdf:resource ="http://127.0.0.1:8000/ontology/SUMO.owl#Music"/>
<rdfs:comment>Music which is produced exclusively
by MusicalInstruments.</rdfs:comment>
</owl:Class>

<owl:Class rdf:ID= "Insulin">
<rdfs:subClassOf rdf:resource ="#Hormone"/>
<rdfs:comment>A Hormone secreted by the Pancreas that is used
to regulate the metabolism of Carbohydrates.</rdfs:comment>
</owl:Class>

<owl:Class rdf:ID= "InsuranceCompany">
<rdfs:subClassOf rdf:resource 
="http://127.0.0.1:8000/ontology/SUMO.owl#CommercialAgent"/>
<rdfs:comment>A CommercialAgent that insures Agents
for the payment of a premium or premiums.</rdfs:comment>
</owl:Class>

<owl:Class rdf:ID= "InsurancePolicy">
<rdfs:subClassOf rdf:resource 
="http://127.0.0.1:8000/ontology/SUMO.owl#Certificate"/>
<rdfs:comment>A Certificate that states the terms of an
insurance contract.</rdfs:comment>
</owl:Class>

<owl:Class rdf:ID= "InterestBearingAccount">
<rdfs:subClassOf rdf:resource ="#FinancialAccount"/>
<rdfs:comment>FinancialAccounts that have a fixed
or adjustable interest rate.</rdfs:comment>
</owl:Class>

<owl:Class rdf:ID= "InternalCombustionEngine">
<rdfs:subClassOf rdf:resource ="#Engine"/>
<rdfs:comment>InternalCombustionEngine is
the subclass of Engines in which a heat reaction that occurs inside
the engine is transformed into mechanical energy.</rdfs:comment>
</owl:Class>

<owl:Class rdf:ID= "InternationalOrganization">
<rdfs:subClassOf rdf:resource 
="http://127.0.0.1:8000/ontology/SUMO.owl#Organization"/>
<rdfs:comment>InternationalOrganization is
the class of Organizations whose activities have international scope and
which typically have members who are, or are from, different 
Nations.</rdfs:comment>
</owl:Class>

<owl:Class rdf:ID= "Interviewing">
<rdfs:subClassOf rdf:resource ="#FormalMeeting"/>
<rdfs:comment>A FormalMeeting whose purpose is to acquire
information from the interviewee that can be used in a media 
report.</rdfs:comment>
</owl:Class>

<owl:Class rdf:ID= "Intestine">
<rdfs:subClassOf rdf:resource 
="http://127.0.0.1:8000/ontology/SUMO.owl#BodyVessel"/>
<rdfs:subClassOf rdf:resource 
="http://127.0.0.1:8000/ontology/SUMO.owl#AnimalAnatomicalStructure"/>
<rdfs:comment>A BodyVessel which connects the Stomach to
the anus and which is used in digesting Food.</rdfs:comment>
</owl:Class>

<owl:Class rdf:ID= "Investing">
<rdfs:subClassOf rdf:resource 
="http://127.0.0.1:8000/ontology/SUMO.owl#FinancialTransaction"/>
<rdfs:comment>An activity of commiting money or capital in order to
gain a financial return.</rdfs:comment>
</owl:Class>

<owl:Class rdf:ID= "Iodine">
<rdfs:subClassOf rdf:resource 
="http://127.0.0.1:8000/ontology/SUMO.owl#ElementalSubstance"/>
<atomicNumber>53</atomicNumber>
<rdfs:comment>Dark violet nonmetallic element, belongs to group
17 of the periodic table.  Insoluble in water.  Required as a trace
element for living organisms.  One stable isotope, I-127 exists, in
addition to fourteen radioactive isotopes.  Chemically the least reactive
of the halogens, and the most electropositive metallic halogen.
Discovered in 1812 by Courtois.</rdfs:comment>
</owl:Class>

<owl:Class rdf:ID= "Ion">
<rdfs:subClassOf rdf:resource 
="http://127.0.0.1:8000/ontology/SUMO.owl#PureSubstance"/>
<rdfs:comment>An electronically charged Atom or Molecule.  In
other words, a PureSubstance that has lost one of its 
Electrons.</rdfs:comment>
</owl:Class>

<owl:Class rdf:ID= "Iron">
<rdfs:subClassOf rdf:resource 
="http://127.0.0.1:8000/ontology/SUMO.owl#ElementalSubstance"/>
<atomicNumber>26</atomicNumber>
<rdfs:comment>Silvery malleable and ductile metallic transition
element.  Has nine isotopes and is the fourth most abundant element in the
earth's crust.  Required by living organisms as a trace element (used in
hemoglobin in humans.) Quite reactive, oxidizes in moist air, displaces
hydrogen from dilute acids and combines with nonmetallic 
elements.</rdfs:comment>
</owl:Class>

<owl:Class rdf:ID= "Ivory">
<rdfs:subClassOf rdf:resource ="http://127.0.0.1:8000/ontology/SUMO.owl#Bone"/>
<rdfs:comment>A very hard substance that makes up the tusks of
elephants and walruses.</rdfs:comment>
</owl:Class>

<owl:Class rdf:ID= "Janitor">
<rdfs:subClassOf rdf:resource ="#UnskilledOccupation"/>
<rdfs:comment>Any Position which involves cleaning a Building
or some of the Rooms within a Building.</rdfs:comment>
</owl:Class>

<owl:Class rdf:ID= "Joule">
<rdfs:subClassOf rdf:resource 
="http://127.0.0.1:8000/ontology/SUMO.owl#FunctionQuantity"/>
<rdf:type rdf:resource = 
"http://127.0.0.1:8000/ontology/SUMO.owl#SystemeInternationalUnit"/>
<rdfs:comment>SI energy measure.  Symbol: J.  It is the work
done when the point of application of 1 Newton is displaced a distance
of 1 Meter in the direction of the force.  Joule = N*m =
m^2*kg*s^(-2).</rdfs:comment>
</owl:Class>

<owl:Class rdf:ID= "Journalist">
<rdfs:subClassOf rdf:resource ="#Profession"/>
<rdfs:comment>The Profession of being a news reporter, i.e.
investigating and reporting, in a publication or broadcast program, current
events.</rdfs:comment>
</owl:Class>

<owl:Class rdf:ID= "Judge">
<rdfs:subClassOf rdf:resource ="#Attorney"/>
<rdfs:subClassOf rdf:resource ="#GovernmentOfficer"/>
<rdfs:comment>An Attorney who has the power of deciding legal 
cases.</rdfs:comment>
</owl:Class>

<owl:Class rdf:ID= "Jumping">
<rdfs:subClassOf rdf:resource 
="http://127.0.0.1:8000/ontology/SUMO.owl#BodyMotion"/>
<rdfs:subClassOf rdf:resource ="#MotionUpward"/>
<rdfs:comment>Any MotionUpward which is done by one's body
and which results in a situation where one's feet are 
unsupported.</rdfs:comment>
</owl:Class>

<owl:Class rdf:ID= "JuniorCollege">
<rdfs:subClassOf rdf:resource ="#PostSecondarySchool"/>
<rdfs:comment>The class of PostSecondarySchools that
offer an associate's degree and do not offer a bachelor's 
degree.</rdfs:comment>
</owl:Class>

<owl:Class rdf:ID= "Jury">
<rdfs:subClassOf rdf:resource 
="http://127.0.0.1:8000/ontology/SUMO.owl#GroupOfPeople"/>
<rdfs:comment>A GroupOfPeople who are given the duty of rendering a
verdict with respect to a LegalAction.</rdfs:comment>
</owl:Class>

<owl:Class rdf:ID= "Key">
<rdfs:subClassOf rdf:resource ="#SecurityDevice"/>
<rdfs:comment>A Device which opens and closes a Lock.</rdfs:comment>
</owl:Class>

<owl:Class rdf:ID= "Kicking">
<rdfs:subClassOf rdf:resource 
="http://127.0.0.1:8000/ontology/SUMO.owl#Impelling"/>
<rdfs:comment>Any instance of Impelling where the instrument
is a Foot of the agent.</rdfs:comment>
</owl:Class>

<owl:Class rdf:ID= "Kidnapping">
<rdfs:subClassOf rdf:resource ="#Robbing"/>
<rdfs:comment>Robbing a Human, i.e. taking him/her away
with the threat of force.</rdfs:comment>
</owl:Class>

<owl:Class rdf:ID= "Kidney">
<rdfs:subClassOf rdf:resource ="http://127.0.0.1:8000/ontology/SUMO.owl#Organ"/>
<rdfs:subClassOf rdf:resource 
="http://127.0.0.1:8000/ontology/SUMO.owl#AnimalAnatomicalStructure"/>
<rdfs:comment>An Organ that separates urine from other
BodySubstances and passes it to the bladder.</rdfs:comment>
</owl:Class>

<owl:Class rdf:ID= "KilowattHour">
<rdf:type rdf:resource = 
"http://127.0.0.1:8000/ontology/SUMO.owl#UnitOfMeasure"/>
<rdfs:subClassOf rdf:resource 
="http://127.0.0.1:8000/ontology/SUMO.owl#FunctionQuantity"/>
<rdfs:comment>KilowattHour is a UnitOfMeasure for
energy that represents 1000 Watts (1 kW) of power expended over one
hour (1 h) of time.  This is the unit commonly used in commercial
power contexts.  It is equivalent to 3,600,000 Joules.</rdfs:comment>
</owl:Class>

<owl:Class rdf:ID= "Kissing">
<rdfs:subClassOf rdf:resource 
="http://127.0.0.1:8000/ontology/SUMO.owl#Touching"/>
<rdfs:comment>The class of Touching processes where the lips
are brought into contact with something else.</rdfs:comment>
</owl:Class>

<owl:Class rdf:ID= "Kitchen">
<rdfs:subClassOf rdf:resource ="http://127.0.0.1:8000/ontology/SUMO.owl#Room"/>
<rdfs:comment>A Room intended for Cooking.</rdfs:comment>
</owl:Class>

<owl:Class rdf:ID= "Knee">
<rdfs:subClassOf rdf:resource ="#BodyJoint"/>
<rdfs:comment>The joint in the Leg connecting the tibia and fibula
with the femur.</rdfs:comment>
</owl:Class>

<owl:Class rdf:ID= "Knuckle">
<rdfs:subClassOf rdf:resource ="#BodyJoint"/>
<rdfs:comment>Any joint in a Finger.</rdfs:comment>
</owl:Class>

<owl:Class rdf:ID= "Label">
<rdfs:subClassOf rdf:resource ="http://127.0.0.1:8000/ontology/SUMO.owl#Text"/>
<rdfs:comment>A very brief Text that is attached to an Object
and that indicates very specific information about the Object, e.g. its
name, its monetaryValue, etc.</rdfs:comment>
</owl:Class>

<owl:Class rdf:ID= "LaborStriking">
<rdfs:subClassOf rdf:resource 
="http://127.0.0.1:8000/ontology/SUMO.owl#OrganizationalProcess"/>
<rdfs:comment>A Process in which some or all of the
employees of a UnionOrganization refuse to work until their pay is
increased or their working conditions are improved in some 
respect.</rdfs:comment>
</owl:Class>

<owl:Class rdf:ID= "Laboratory">
<rdfs:subClassOf rdf:resource 
="http://127.0.0.1:8000/ontology/SUMO.owl#StationaryArtifact"/>
<rdfs:comment>A Building, Room or suite of Rooms where
scientific research, i.e. Experimenting, is conducted.</rdfs:comment>
</owl:Class>

<owl:Class rdf:ID= "Ladder">
<rdfs:subClassOf rdf:resource 
="http://127.0.0.1:8000/ontology/SUMO.owl#Artifact"/>
<rdfs:comment>An Artifact which consists of two parallel supports
connected by a series of rungs which can be used to ascend or 
descend.</rdfs:comment>
</owl:Class>

<owl:Class rdf:ID= "Lamb">
<rdfs:subClassOf rdf:resource ="#Sheep"/>
<rdfs:comment>A young Sheep, i.e. a Sheep that is 
NonFullyFormed.</rdfs:comment>
</owl:Class>

<owl:Class rdf:ID= "LandForm">
<rdfs:subClassOf rdf:resource 
="http://127.0.0.1:8000/ontology/SUMO.owl#LandArea"/>
<rdfs:comment>A LandForm is the class of geographically and/or
geologically distinct areas that occur on Earth's surface, including 
mountains,
hills, plains, valleys, deltas, and features of submerged land areas such as
the ocean floor.</rdfs:comment>
</owl:Class>

<owl:Class rdf:about= "LandTransitway">
<rdfs:subClassOf rdf:resource 
="http://127.0.0.1:8000/ontology/SUMO.owl#Transitway"/>
<rdfs:subClassOf rdf:resource 
="http://127.0.0.1:8000/ontology/SUMO.owl#LandArea"/>
<rdfs:comment>LandTransitway is the subclass of
Transitway that represents areas intended for motion over the 
ground.</rdfs:comment>
</owl:Class>

<owl:Class rdf:ID= "LandTransportation">
<rdfs:subClassOf rdf:resource 
="http://127.0.0.1:8000/ontology/SUMO.owl#Transportation"/>
<rdfs:comment>Any instance of Transportation where the
instrument is a LandVehicle.</rdfs:comment>
</owl:Class>

<owl:Class rdf:ID= "LandVehicle">
<rdfs:subClassOf rdf:resource 
="http://127.0.0.1:8000/ontology/SUMO.owl#Vehicle"/>
<rdfs:comment>LandVehicle is the class of Vehicles that
travel on land.  The two main types of LandVehicle are RoadVehicle and
RollingStock.</rdfs:comment>
</owl:Class>

<owl:Class rdf:ID= "Landing">
<rdfs:subClassOf rdf:resource 
="http://127.0.0.1:8000/ontology/SUMO.owl#Translocation"/>
<rdfs:comment>Any instance of Translocation which ends up on
something other than an AtmosphericRegion and which has an instance of
Flying as a subProcess.</rdfs:comment>
</owl:Class>

<owl:Class rdf:ID= "LandlockedWater">
<rdfs:subClassOf rdf:resource ="#BodyOfWater"/>
<rdfs:comment>LandlockedWater includes water
areas that are surrounded by land, including salt lakes, fresh
water lakes, ponds, reservoirs, and (more or less) wetlands.</rdfs:comment>
</owl:Class>

<owl:Class rdf:ID= "Laughing">
<rdfs:subClassOf rdf:resource 
="http://127.0.0.1:8000/ontology/SUMO.owl#Vocalizing"/>
<rdfs:subClassOf rdf:resource ="#FacialExpression"/>
<rdfs:comment>Expressing happiness by Vocalizing in a
certain way.</rdfs:comment>
</owl:Class>

<owl:Class rdf:ID= "LawEnforcement">
<rdfs:subClassOf rdf:resource 
="http://127.0.0.1:8000/ontology/SUMO.owl#PoliticalProcess"/>
<rdfs:subClassOf rdf:resource 
="http://127.0.0.1:8000/ontology/SUMO.owl#RegulatoryProcess"/>
<rdfs:comment>Any RegulatoryProcess where the agent is either
a PoliceOrganization or a member of a PoliceOrganization.  This covers
everything from issuing a traffic ticket to arresting someone on suspicion 
of having
committed a Murder.</rdfs:comment>
</owl:Class>

<owl:Class rdf:ID= "Lawn">
<rdfs:subClassOf rdf:resource ="#CultivatedLandArea"/>
<rdfs:comment>A CultivatedLandArea containing mowed Grass.</rdfs:comment>
</owl:Class>

<owl:Class rdf:ID= "LayingEggs">
<rdfs:subClassOf rdf:resource 
="http://127.0.0.1:8000/ontology/SUMO.owl#OrganismProcess"/>
<rdfs:comment>Any OrganismProcess where an Egg is expelled
from the body of a Animal, e.g. a Bird or Reptile laying 
eggs.</rdfs:comment>
</owl:Class>

<owl:Class rdf:ID= "Lead">
<rdfs:subClassOf rdf:resource 
="http://127.0.0.1:8000/ontology/SUMO.owl#ElementalSubstance"/>
<atomicNumber>82</atomicNumber>
<rdfs:comment>Heavy dull grey ductile metallic element, belongs to
group 14.  Used in building construction, lead-place accumulators, bullets
and shot, and is part of solder, pewter, bearing metals, type metals and
fusible alloys.</rdfs:comment>
</owl:Class>

<owl:Class rdf:ID= "Leather">
<rdfs:subClassOf rdf:resource ="http://127.0.0.1:8000/ontology/SUMO.owl#Fabric"/>
<rdfs:comment>A Fabric that is the result of tanning an Animal
Skin.</rdfs:comment>
</owl:Class>

<owl:Class rdf:ID= "Leaving">
<rdfs:subClassOf rdf:resource 
="http://127.0.0.1:8000/ontology/SUMO.owl#Translocation"/>
<rdfs:comment>The initial part of any instance of 
Translocation.</rdfs:comment>
</owl:Class>

<owl:Class rdf:ID= "Lecture">
<rdfs:subClassOf rdf:resource 
="http://127.0.0.1:8000/ontology/SUMO.owl#Demonstrating"/>
<rdfs:subClassOf rdf:resource 
="http://127.0.0.1:8000/ontology/SUMO.owl#Speaking"/>
<rdfs:comment>Any instance of Speaking which is done before an
assembled audience.</rdfs:comment>
</owl:Class>

<owl:Class rdf:ID= "Leg">
<rdfs:subClassOf rdf:resource ="#Limb"/>
<rdfs:comment>The lower Limbs of Primates.</rdfs:comment>
</owl:Class>

<owl:Class rdf:ID= "LegalAppeal">
<rdfs:subClassOf rdf:resource 
="http://127.0.0.1:8000/ontology/SUMO.owl#Requesting"/>
<rdfs:subClassOf rdf:resource 
="http://127.0.0.1:8000/ontology/SUMO.owl#JudicialProcess"/>
<rdfs:comment>Asking that a higher court reconsider a LegalDecision
of a lower court.</rdfs:comment>
</owl:Class>

<owl:Class rdf:ID= "LegalAquittal">
<rdfs:subClassOf rdf:resource 
="http://127.0.0.1:8000/ontology/SUMO.owl#LegalDecision"/>
<rdfs:comment>Any LegalDecision where the defendant is found
not to be guilty of the crime for which the corresponding trial was 
held.</rdfs:comment>
</owl:Class>

<owl:Class rdf:ID= "LegalAward">
<rdfs:subClassOf rdf:resource 
="http://127.0.0.1:8000/ontology/SUMO.owl#LegalDecision"/>
<rdfs:comment>Any LegalDecision which gives to the plaintiff of
the corresponding LegalAction some amount of monetary 
compensation.</rdfs:comment>
</owl:Class>

<owl:Class rdf:ID= "LegalCharge">
<rdfs:subClassOf rdf:resource 
="http://127.0.0.1:8000/ontology/SUMO.owl#LegalAction"/>
<rdfs:comment>Any LegalAction of which a Government is
the agent.</rdfs:comment>
</owl:Class>

<owl:Class rdf:ID= "LegalConviction">
<rdfs:subClassOf rdf:resource 
="http://127.0.0.1:8000/ontology/SUMO.owl#LegalDecision"/>
<rdfs:comment>Any LegalDecision where the defendant is found
guilty of the crime for which the corresponding trial was 
held.</rdfs:comment>
</owl:Class>

<owl:Class rdf:ID= "LegalDismissal">
<rdfs:subClassOf rdf:resource 
="http://127.0.0.1:8000/ontology/SUMO.owl#LegalDecision"/>
<rdfs:comment>Any LegalDecision where the LegalAction of
the plaintiff is dismissed by the court, e.g. for lack of 
merit.</rdfs:comment>
</owl:Class>

<owl:Class rdf:ID= "LegalOpinion">
<rdfs:subClassOf rdf:resource 
="http://127.0.0.1:8000/ontology/SUMO.owl#Argument"/>
<rdfs:comment>An Argument that explains the reasoning behind a
LegalDecision.</rdfs:comment>
</owl:Class>

<owl:Class rdf:ID= "LegalSummons">
<rdfs:subClassOf rdf:resource 
="http://127.0.0.1:8000/ontology/SUMO.owl#Ordering"/>
<rdfs:subClassOf rdf:resource 
="http://127.0.0.1:8000/ontology/SUMO.owl#JudicialProcess"/>
<rdfs:comment>An official order that a person appear at a
CourtRoom at a specified time.</rdfs:comment>
</owl:Class>

<owl:Class rdf:ID= "LegalSystemAttribute">
<rdfs:subClassOf rdf:resource 
="http://127.0.0.1:8000/ontology/SUMO.owl#RelationalAttribute"/>
<rdfs:comment>LegalSystemAttribute is the class
of Attributes that are used to characterize legal systems, as, e.g.,
according to their sources, areas of concern, or principles of
organization.</rdfs:comment>
</owl:Class>

<owl:Class rdf:ID= "LegislativeOrganization">
<rdfs:subClassOf rdf:resource 
="http://127.0.0.1:8000/ontology/SUMO.owl#Organization"/>
<rdfs:comment>LegislativeOrganization is the
class of Organizations that have as their main purpose the passing of
laws or regulations.</rdfs:comment>
</owl:Class>

<owl:Class rdf:ID= "LemonFruit">
<rdfs:subClassOf rdf:resource 
="http://127.0.0.1:8000/ontology/SUMO.owl#FruitOrVegetable"/>
<rdfs:subClassOf rdf:resource ="http://127.0.0.1:8000/ontology/SUMO.owl#Food"/>
<rdfs:comment>A citrus FruitOrVegetable that has a yellow skin
and a tart, acidic flavor.</rdfs:comment>
</owl:Class>

<owl:Class rdf:ID= "Lengthening">
<rdfs:subClassOf rdf:resource 
="http://127.0.0.1:8000/ontology/SUMO.owl#Increasing"/>
<rdfs:comment>Increasing the length of something.</rdfs:comment>
</owl:Class>

<owl:Class rdf:ID= "Lens">
<rdfs:subClassOf rdf:resource ="#OpticalDevice"/>
<rdfs:comment>An OpticalDevice which consists of a polished,
transparent piece of glass or plastic.  Lenses are often part of
other OpticalDevices.</rdfs:comment>
</owl:Class>

<owl:Class rdf:ID= "Lesion">
<rdfs:subClassOf rdf:resource 
="http://127.0.0.1:8000/ontology/SUMO.owl#AbnormalAnatomicalStructure"/>
<rdfs:comment>Any AbnormalAnatomicalStructure which is the result of
an Injuring and which is found on the surface of an Organ.</rdfs:comment>
</owl:Class>

<owl:Class rdf:ID= "LiabilityAccount">
<rdfs:subClassOf rdf:resource ="#FinancialAccount"/>
<rdfs:comment>An account for which a person is liable.</rdfs:comment>
</owl:Class>

<owl:Class rdf:ID= "Library">
<rdfs:subClassOf rdf:resource 
="http://127.0.0.1:8000/ontology/SUMO.owl#EducationalOrganization"/>
<rdfs:comment>An EducationalOrganization which is a repository
of Texts which have been classified for efficient retrieval.</rdfs:comment>
</owl:Class>

<owl:Class rdf:ID= "License">
<rdfs:subClassOf rdf:resource 
="http://127.0.0.1:8000/ontology/SUMO.owl#Certificate"/>
<rdfs:comment>License is the subclass of Certificates that
are granted by a GovernmentOrganization and that authorize the performance
of a kind of action, e.g., driving, exporting, travelling to another
country, etc.</rdfs:comment>
</owl:Class>

<owl:Class rdf:ID= "Licking">
<rdfs:subClassOf rdf:resource 
="http://127.0.0.1:8000/ontology/SUMO.owl#Touching"/>
<rdfs:comment>The class of Touching processes where the Tongue
is brought into contact with something else.</rdfs:comment>
</owl:Class>

<owl:Class rdf:ID= "Lieutenant">
<rdfs:subClassOf rdf:resource ="#MilitaryOfficer"/>
<rdfs:comment>A commissioned MilitaryOfficer.</rdfs:comment>
</owl:Class>

<owl:Class rdf:ID= "Lightning">
<rdfs:subClassOf rdf:resource 
="http://127.0.0.1:8000/ontology/SUMO.owl#WeatherProcess"/>
<rdfs:subClassOf rdf:resource 
="http://127.0.0.1:8000/ontology/SUMO.owl#Radiating"/>
<rdfs:comment>A WeatherProcess which involves a significant
release of electricity from a Cloud.</rdfs:comment>
</owl:Class>

<owl:Class rdf:ID= "LilacFlower">
<rdfs:subClassOf rdf:resource 
="http://127.0.0.1:8000/ontology/SUMO.owl#FloweringPlant"/>
<rdfs:comment>A FloweringPlant that has large clusters of
aromatic flowers.</rdfs:comment>
</owl:Class>

<owl:Class rdf:ID= "Limb">
<rdfs:subClassOf rdf:resource 
="http://127.0.0.1:8000/ontology/SUMO.owl#AnimalAnatomicalStructure"/>
<rdfs:subClassOf rdf:resource 
="http://127.0.0.1:8000/ontology/SUMO.owl#BodyPart"/>
<rdfs:comment>Animal Appendages with joints that are used for movement
and grasping.</rdfs:comment>
</owl:Class>

<owl:Class rdf:ID= "LinguisticAttribute">
<rdfs:subClassOf rdf:resource 
="http://127.0.0.1:8000/ontology/SUMO.owl#InternalAttribute"/>
<rdfs:comment>Any Attribute that is
expressed by a Language or class of Languages.</rdfs:comment>
</owl:Class>

<owl:Class rdf:ID= "Lip">
<rdfs:subClassOf rdf:resource 
="http://127.0.0.1:8000/ontology/SUMO.owl#AnimalAnatomicalStructure"/>
<rdfs:subClassOf rdf:resource 
="http://127.0.0.1:8000/ontology/SUMO.owl#BodyPart"/>
<rdfs:comment>Folds of Tissue surrounding the mouths of some
Vertebrates.</rdfs:comment>
</owl:Class>

<owl:Class rdf:ID= "LiquefiedPetroleumGas">
<rdfs:subClassOf rdf:resource ="#FossilFuel"/>
<rdfs:subClassOf rdf:resource ="#RefinedPetroleumProduct"/>
<rdfs:comment>LiquefiedPetroleumGas is a
compressed hydrocarbon gas.</rdfs:comment>
</owl:Class>

<owl:Class rdf:ID= "LiquidBodySubstance">
<rdfs:subClassOf rdf:resource 
="http://127.0.0.1:8000/ontology/SUMO.owl#BodySubstance"/>
<rdfs:comment>Any BodySubstance which is Liquid
under normal circumstances.</rdfs:comment>
</owl:Class>

<owl:Class rdf:ID= "LiquorShot">
<rdfs:subClassOf rdf:resource ="#DistilledAlcoholicBeverage"/>
<rdfs:comment>A small serving of a 
DistilledAlcoholicBeverage.</rdfs:comment>
</owl:Class>

<owl:Class rdf:ID= "Liver">
<rdfs:subClassOf rdf:resource ="http://127.0.0.1:8000/ontology/SUMO.owl#Organ"/>
<rdfs:subClassOf rdf:resource 
="http://127.0.0.1:8000/ontology/SUMO.owl#AnimalAnatomicalStructure"/>
<rdfs:comment>An Organ that secretes bile and serves metabolic
functions.</rdfs:comment>
</owl:Class>

<owl:Class rdf:ID= "LoadingWeapon">
<rdfs:subClassOf rdf:resource 
="http://127.0.0.1:8000/ontology/SUMO.owl#Inserting"/>
<rdfs:comment>Inserting ammunition into a ProjectileWeapon
in such a way that the ammunition can be fired by the weapon.</rdfs:comment>
</owl:Class>

<owl:Class rdf:ID= "Loan">
<rdfs:subClassOf rdf:resource ="#LiabilityAccount"/>
<rdfs:comment>An arrangement in which a lender gives money or property to a 
borrower,
and the borrower agrees to return the property or repay the money, usually 
along with interest,
at some future point(s) in time.</rdfs:comment>
</owl:Class>

<owl:Class rdf:ID= "Lock">
<rdfs:subClassOf rdf:resource ="#SecurityDevice"/>
<rdfs:comment>A Device, which, through a Key or a combination prevents
access to a Container or StationaryArtifact.</rdfs:comment>
</owl:Class>

<owl:Class rdf:ID= "Locomotive">
<rdfs:subClassOf rdf:resource ="#RollingStock"/>
<rdfs:subClassOf rdf:resource ="#SelfPoweredVehicle"/>
<rdfs:comment>Locomotive is the subclass of RollingStock
that represents train locomotives, including those with DieselEngines
and with SteamEngines.</rdfs:comment>
</owl:Class>

<owl:Class rdf:ID= "LosingConsciousness">
<rdfs:subClassOf rdf:resource 
="http://127.0.0.1:8000/ontology/SUMO.owl#PsychologicalProcess"/>
<sumo:disjoint rdf:resource = "#GainingConsciousness" />
<rdfs:comment>The process of transitioning from a state
of being Awake to a state of being Unconscious.</rdfs:comment>
</owl:Class>

<owl:Class rdf:ID= "LowTide">
<rdfs:subClassOf rdf:resource ="#TidalProcess"/>
<rdfs:comment>LowTide is the class of TidalProcesses that
occur twice a day in marine waters, in which the water level falls below
the mean sea level.</rdfs:comment>
</owl:Class>

<owl:Class rdf:ID= "LowlandArea">
<rdfs:subClassOf rdf:resource ="#LandForm"/>
<rdfs:comment>A LowlandArea is a land area lower than the surrounding 
region, and usually level land.</rdfs:comment>
</owl:Class>

<owl:Class rdf:ID= "Lumen">
<rdfs:subClassOf rdf:resource 
="http://127.0.0.1:8000/ontology/SUMO.owl#FunctionQuantity"/>
<rdf:type rdf:resource = 
"http://127.0.0.1:8000/ontology/SUMO.owl#SystemeInternationalUnit"/>
<rdfs:comment>SI luminous flux measure.  Symbol: lm.  It is the
amount streaming outward through one solid angle of 1 Steradian from a
uniform point source having an intensity of one Candela.  Lumen =
cd*sr = cd * 1.</rdfs:comment>
</owl:Class>

<owl:Class rdf:ID= "Lung">
<rdfs:subClassOf rdf:resource ="http://127.0.0.1:8000/ontology/SUMO.owl#Organ"/>
<rdfs:subClassOf rdf:resource 
="http://127.0.0.1:8000/ontology/SUMO.owl#AnimalAnatomicalStructure"/>
<rdfs:comment>A respiratory organ of Vertebrates.  Its function is
to furnish the blood with oxygen and to remove carbon 
dioxide.</rdfs:comment>
</owl:Class>

<owl:Class rdf:ID= "Lux">
<rdfs:subClassOf rdf:resource 
="http://127.0.0.1:8000/ontology/SUMO.owl#FunctionQuantity"/>
<rdf:type rdf:resource = 
"http://127.0.0.1:8000/ontology/SUMO.owl#SystemeInternationalUnit"/>
<rdfs:comment>SI illuminance measure.  Symbol: lx.  It is the
amount of illumination provided when one Lumen is evenly distributed
over an area of 1 square Meter. This is also equivalent to the
illumination that would exist on a surface all points of which are one
Meter from a point source of one Candela.  Lux = lm/m^2 =
m^(-2)*cd.</rdfs:comment>
</owl:Class>

<owl:Class rdf:ID= "LyingDown">
<rdfs:subClassOf rdf:resource 
="http://127.0.0.1:8000/ontology/SUMO.owl#BodyMotion"/>
<rdfs:comment>The BodyMotion of moving from a Sitting
to a Prostrate position.</rdfs:comment>
</owl:Class>

<owl:Class rdf:ID= "Lyrics">
<rdfs:subClassOf rdf:resource ="http://127.0.0.1:8000/ontology/SUMO.owl#Text"/>
<rdfs:comment>Any Text which contains just the words of
a MusicalComposition.</rdfs:comment>
</owl:Class>

<owl:Class rdf:ID= "Magazine">
<rdfs:subClassOf rdf:resource 
="http://127.0.0.1:8000/ontology/SUMO.owl#Periodical"/>
<rdfs:comment>A Periodical that is softbound and printed on
glossy paper.</rdfs:comment>
</owl:Class>

<owl:Class rdf:ID= "Magnetism">
<rdfs:subClassOf rdf:resource 
="http://127.0.0.1:8000/ontology/SUMO.owl#Radiating"/>
<rdfs:comment>Any instance of Radiating which
involves the attraction of Iron.</rdfs:comment>
</owl:Class>

<owl:Class rdf:ID= "Maid">
<rdfs:subClassOf rdf:resource ="#ServicePosition"/>
<rdfs:comment>Any ServicePosition where various needs of a person
or family are served over a long period of time.  Note that these Positions
are, by definition, filled only by Women.</rdfs:comment>
</owl:Class>

<owl:Class rdf:ID= "Mailbox">
<rdfs:subClassOf rdf:resource ="#Container"/>
<rdfs:comment>A Container whose purpose is to receive items
that are mailed to the address associated with the Mailbox.</rdfs:comment>
</owl:Class>

<owl:Class rdf:ID= "Mailing">
<rdfs:subClassOf rdf:resource 
="http://127.0.0.1:8000/ontology/SUMO.owl#Transfer"/>
<rdfs:comment>Any instance of Transfer where a postal system is
used to move the patient, either a Message or a package.</rdfs:comment>
</owl:Class>

<owl:Class rdf:ID= "MajorGeneral">
<rdfs:subClassOf rdf:resource ="#MilitaryGeneral"/>
<rdfs:comment>A MilitaryGeneral that ranks above a
BrigadierGeneral.</rdfs:comment>
</owl:Class>

<owl:Class rdf:ID= "Manifold">
<rdfs:subClassOf rdf:resource 
="http://127.0.0.1:8000/ontology/SUMO.owl#EngineeringComponent"/>
<rdfs:comment>A pipe which has several outlets for other pipes that
flow into or out of it.</rdfs:comment>
</owl:Class>

<owl:Class rdf:ID= "ManualLabor">
<rdfs:subClassOf rdf:resource 
="http://127.0.0.1:8000/ontology/SUMO.owl#Position"/>
<rdfs:comment>Any Position which involves manual
work.</rdfs:comment>
</owl:Class>

<owl:Class rdf:ID= "Map">
<rdfs:subClassOf rdf:resource ="http://127.0.0.1:8000/ontology/SUMO.owl#Icon"/>
<rdfs:comment>An Icon which represents one or more GeographicAreas
(or even the entire Earth).</rdfs:comment>
</owl:Class>

<owl:Class rdf:ID= "Marble">
<rdfs:subClassOf rdf:resource ="#Rock"/>
<rdfs:comment>A metamorphic Rock that is used in Constructing
and in creating Sculptures.</rdfs:comment>
</owl:Class>

<owl:Class rdf:ID= "MarineCorps">
<rdfs:subClassOf rdf:resource 
="http://127.0.0.1:8000/ontology/SUMO.owl#MilitaryOrganization"/>
<sumo:relatedInternalConcept rdf:resource = "#Navy" />
<rdfs:comment>MarineCorps is the subclass of
MilitaryOrganization consisting of infantry forces that are ship-based
or otherwise affiliated with naval forces, and assigned to tasks such as
protecting ships or taking beachhead positions.</rdfs:comment>
</owl:Class>

<owl:Class rdf:ID= "Marshal">
<rdfs:subClassOf rdf:resource ="#PoliceOfficer"/>
<rdfs:comment>A PoliceOfficer whose responsibility is to enforce
the decisions of a law court.</rdfs:comment>
</owl:Class>

<owl:Class rdf:ID= "Massaging">
<rdfs:subClassOf rdf:resource 
="http://127.0.0.1:8000/ontology/SUMO.owl#TherapeuticProcess"/>
<rdfs:subClassOf rdf:resource 
="http://127.0.0.1:8000/ontology/SUMO.owl#Touching"/>
<rdfs:comment>A subclass of TherapeuticProcess which involves
kneading Muscles in such a way that tension is relieved, blood circulation
is increased, etc.</rdfs:comment>
</owl:Class>

<owl:Class rdf:ID= "Mast">
<rdfs:subClassOf rdf:resource 
="http://127.0.0.1:8000/ontology/SUMO.owl#Artifact"/>
<rdfs:comment>A large pole in the center of a Watercraft which is
used to support a sail.</rdfs:comment>
</owl:Class>

<owl:Class rdf:ID= "MatchDevice">
<rdfs:subClassOf rdf:resource ="http://127.0.0.1:8000/ontology/SUMO.owl#Device"/>
<rdfs:comment>A small stick of carboard or wood that is treated
with chemicals that can be easily ignited with friction.  MatchDevices are
used for starting fires.</rdfs:comment>
</owl:Class>

<owl:Class rdf:ID= "MaterialHandlingEquipment">
<rdfs:subClassOf rdf:resource ="http://127.0.0.1:8000/ontology/SUMO.owl#Device"/>
<rdfs:comment>MaterialHandlingEquipment
is a class of Devices that are equipment used for handling goods and
supplies more efficiently or safely.  Examples are cranes, hoists,
forklifts, conveyors, racks, etc.</rdfs:comment>
</owl:Class>

<owl:Class rdf:ID= "Mating">
<rdfs:subClassOf rdf:resource 
="http://127.0.0.1:8000/ontology/SUMO.owl#OrganismProcess"/>
<rdfs:comment>Any process of sexual intercourse between two Humans
or Animals.</rdfs:comment>
</owl:Class>

<owl:Class rdf:ID= "MediaOrganization">
<rdfs:subClassOf rdf:resource 
="http://127.0.0.1:8000/ontology/SUMO.owl#Organization"/>
<rdfs:comment>MediaOrganization is the subclass
of Organization for groups whose primary purpose is the production or
dissemination of media content.  For organizations that physically enable
Communication, see CommunicationOrganization.</rdfs:comment>
</owl:Class>

<owl:Class rdf:ID= "MedicalClinic">
<rdfs:subClassOf rdf:resource ="#CareOrganization"/>
<sumo:disjoint rdf:resource = "http://127.0.0.1:8000/ontology/SUMO.owl#Residence"
/>
<rdfs:comment>A CareOrganization which provides medical care
on an out-patient basis only, i.e. there are no rooms where patients may 
take
up residence for a period of time while they receive care.</rdfs:comment>
</owl:Class>

<owl:Class rdf:ID= "MedicalDoctor">
<rdfs:subClassOf rdf:resource ="#Profession"/>
<rdfs:comment>The Profession of being a medical doctor,
i.e. having attended medical school and being licensed to practice 
medicine.</rdfs:comment>
</owl:Class>

<owl:Class rdf:ID= "MedicalSchool">
<rdfs:subClassOf rdf:resource ="#GraduateSchool"/>
<rdfs:comment>A GraduateSchool that is devoted to
MedicalScience and that grants the degree of doctor of 
medicine.</rdfs:comment>
</owl:Class>

<owl:Class rdf:ID= "Medicine">
<rdfs:subClassOf rdf:resource 
="http://127.0.0.1:8000/ontology/SUMO.owl#BiologicallyActiveSubstance"/>
<rdfs:comment>Any BiologicallyActiveSubstance which has a
therapeutic effect under certain conditions.</rdfs:comment>
</owl:Class>

<owl:Class rdf:ID= "MediterraneanClimateZone">
<rdfs:subClassOf rdf:resource ="#TemperateClimateZone"/>
<rdfs:comment>MediterraneanClimateZone
is a subclass of TemperateClimateZone that is characterized by
mild, cool, wet winters and warm dry summers.  Mediterranean shores
are the archetype, but the Mediterranean climate is also found 
elsewhere.</rdfs:comment>
</owl:Class>

<owl:Class rdf:ID= "Memorizing">
<rdfs:subClassOf rdf:resource 
="http://127.0.0.1:8000/ontology/SUMO.owl#Learning"/>
<rdfs:comment>The process of committing a Text to memory.</rdfs:comment>
</owl:Class>

<owl:Class rdf:ID= "Menstruation">
<rdfs:subClassOf rdf:resource 
="http://127.0.0.1:8000/ontology/SUMO.owl#OrganOrTissueProcess"/>
<rdfs:comment>A periodic discharge of Blood and other
BiologicalSubstances by Females that is part of a readjustment of
the uterus.</rdfs:comment>
</owl:Class>

<owl:Class rdf:ID= "Mercury">
<rdfs:subClassOf rdf:resource 
="http://127.0.0.1:8000/ontology/SUMO.owl#ElementalSubstance"/>
<atomicNumber>80</atomicNumber>
<rdfs:comment>Heavy silvery liquid metallic element, belongs to
the zinc group.  Used in thermometers, barometers and other scientific
apparatus.  Less reactive than zinc and cadmium, does not displace
hydrogen from acids.  Forms a number of complexes and organomercury
compounds.</rdfs:comment>
</owl:Class>

<owl:Class rdf:ID= "Message">
<rdfs:subClassOf rdf:resource 
="http://127.0.0.1:8000/ontology/SUMO.owl#FactualText"/>
<rdfs:comment>A FactualText which is intended to be delivered to
and read by a Human, GroupOfPeople or Organization.</rdfs:comment>
</owl:Class>

<owl:Class rdf:ID= "Messaging">
<rdfs:subClassOf rdf:resource 
="http://127.0.0.1:8000/ontology/SUMO.owl#Transfer"/>
<rdfs:comment>Any instance of Transfer where a Message is the
patient.</rdfs:comment>
</owl:Class>

<owl:Class rdf:ID= "MetallicAlloy">
<rdfs:subClassOf rdf:resource 
="http://127.0.0.1:8000/ontology/SUMO.owl#Mixture"/>
<rdfs:comment>A Mixture of two or more Metals, and
possibly nonmetallic elements as well.  For example, steel is an alloy
containing iron and manganese.</rdfs:comment>
</owl:Class>

<owl:Class rdf:ID= "Meteorite">
<rdfs:subClassOf rdf:resource ="#Meteoroid"/>
<rdfs:comment>Any Meteoroid that leaves traces on the surface
of Earth.</rdfs:comment>
</owl:Class>

<owl:Class rdf:ID= "Meteoroid">
<rdfs:subClassOf rdf:resource 
="http://127.0.0.1:8000/ontology/SUMO.owl#AstronomicalBody"/>
<rdfs:comment>Any AstronomicalBody that breaks through the
atmosphere of Earth.</rdfs:comment>
</owl:Class>

<owl:Class rdf:ID= "MetricTon">
<rdf:type rdf:resource = 
"http://127.0.0.1:8000/ontology/SUMO.owl#UnitOfMeasure"/>
<rdfs:subClassOf rdf:resource 
="http://127.0.0.1:8000/ontology/SUMO.owl#MassMeasure"/>
<rdfs:comment>MetricTon is a UnitOfMeasure that represents
a weight of 2,205 PoundMass.</rdfs:comment>
</owl:Class>

<owl:Class rdf:ID= "Microphone">
<rdfs:subClassOf rdf:resource ="#ElectricDevice"/>
<rdfs:subClassOf rdf:resource ="#CommunicationDevice"/>
<rdfs:comment>A CommunicationDevice that converts sound
into electrical energy.</rdfs:comment>
</owl:Class>

<owl:Class rdf:ID= "Microscope">
<rdfs:subClassOf rdf:resource ="#OpticalDevice"/>
<rdfs:comment>An OpticalDevice with a stand and a focus, which is
used for magnifying the images of things that are placed in the 
stand.</rdfs:comment>
</owl:Class>

<owl:Class rdf:ID= "MiddleLatitudeDesertClimateZone">
<rdfs:subClassOf rdf:resource ="#DesertClimateZone"/>
<rdfs:comment>MiddleLatitudeDesertClimateZone is the subclass of
DesertClimateZone characterized by a cool dry climate
typical of middle latitude deserts.  This is subtype 'BWk'
in the Keoppen climate system.</rdfs:comment>
</owl:Class>

<owl:Class rdf:ID= "MidlatitudeContinentalClimateZone">
<rdfs:subClassOf rdf:resource ="#ClimateZone"/>
<rdfs:comment>MidlatitudeContinentalClimateZone is a subclass of
TemperateClimateZone that is characterized by cool winters
and hot summers.</rdfs:comment>
</owl:Class>

<owl:Class rdf:ID= "MilitaryAircraft">
<rdfs:subClassOf rdf:resource ="#Aircraft"/>
<rdfs:subClassOf rdf:resource ="#MilitaryVehicle"/>
<rdfs:comment>Any Aircraft which is made for a
MilitaryOrganization.  This includes fighters, Bombers, attack
helicopters, etc.</rdfs:comment>
</owl:Class>

<owl:Class rdf:ID= "MilitaryArtifact">
<rdfs:subClassOf rdf:resource 
="http://127.0.0.1:8000/ontology/SUMO.owl#Artifact"/>
<rdfs:comment>Any Artifact which is made for a
MilitaryOrganization.</rdfs:comment>
</owl:Class>

<owl:Class rdf:ID= "MilitaryBrigade">
<rdfs:subClassOf rdf:resource ="#MilitaryUnit"/>
<rdfs:comment>Any MilitaryUnit with the rank of
brigade.</rdfs:comment>
</owl:Class>

<owl:Class rdf:ID= "MilitaryCompany">
<rdfs:subClassOf rdf:resource ="#MilitaryUnit"/>
<rdfs:comment>Any MilitaryUnit with the rank of
company.</rdfs:comment>
</owl:Class>

<owl:Class rdf:ID= "MilitaryCorps">
<rdfs:subClassOf rdf:resource ="#MilitaryUnit"/>
<rdfs:comment>Any MilitaryUnit with the rank of
corps.</rdfs:comment>
</owl:Class>

<owl:Class rdf:ID= "MilitaryDivision">
<rdfs:subClassOf rdf:resource ="#MilitaryUnit"/>
<rdfs:comment>Any MilitaryUnit with the rank of
division.</rdfs:comment>
</owl:Class>

<owl:Class rdf:ID= "MilitaryFront">
<rdfs:subClassOf rdf:resource 
="http://127.0.0.1:8000/ontology/SUMO.owl#GeographicArea"/>
<rdfs:comment>A GeographicArea along which opposing military
forces confront one another in a Battle.</rdfs:comment>
</owl:Class>

<owl:Class rdf:ID= "MilitaryGeneral">
<rdfs:subClassOf rdf:resource ="#MilitaryOfficer"/>
<rdfs:comment>MilitaryGeneral is a generic Position
that indicates holding (or having held) the rank of General in some
military force.  An indicator that someone uses the title, without
committing to his or her exact rank or military affiliation.</rdfs:comment>
</owl:Class>

<owl:Class rdf:ID= "MilitaryInfiltration">
<rdfs:subClassOf rdf:resource 
="http://127.0.0.1:8000/ontology/SUMO.owl#MilitaryProcess"/>
<rdfs:subClassOf rdf:resource 
="http://127.0.0.1:8000/ontology/SUMO.owl#Translocation"/>
<rdfs:comment>Any Process by a MilitaryOrganization
which involves moving through enemy positions without detection by the 
enemy.</rdfs:comment>
</owl:Class>

<owl:Class rdf:ID= "MilitaryInstallation">
<rdfs:subClassOf rdf:resource 
="http://127.0.0.1:8000/ontology/SUMO.owl#StationaryArtifact"/>
<rdfs:subClassOf rdf:resource ="#MilitaryArtifact"/>
<rdfs:comment>A StationaryArtifact consisting of grounds
and Buildings that is intended to be used by a 
MilitaryOrganization.</rdfs:comment>
</owl:Class>

<owl:Class rdf:ID= "MilitaryManeuver">
<rdfs:subClassOf rdf:resource 
="http://127.0.0.1:8000/ontology/SUMO.owl#Maneuver"/>
<rdfs:comment>Any Maneuver which takes place in a Battle
and which is intended to secure a tactical advantage for one of the agents 
of
the Battle.</rdfs:comment>
</owl:Class>

<owl:Class rdf:ID= "MilitaryOfficer">
<rdfs:subClassOf rdf:resource ="#Soldier"/>
<rdfs:comment>The class of Soldiers who have authority or 
command.</rdfs:comment>
</owl:Class>

<owl:Class rdf:ID= "MilitaryPlatoon">
<rdfs:subClassOf rdf:resource ="#MilitaryUnit"/>
<rdfs:comment>Any MilitaryUnit with the rank of
platoon.</rdfs:comment>
</owl:Class>

<owl:Class rdf:ID= "MilitaryPrivate">
<rdfs:subClassOf rdf:resource ="#Soldier"/>
<rdfs:comment>An enlisted Soldier of the lowest rank.</rdfs:comment>
</owl:Class>

<owl:Class rdf:ID= "MilitaryRegiment">
<rdfs:subClassOf rdf:resource ="#MilitaryUnit"/>
<rdfs:comment>Any MilitaryUnit with the rank of
regiment.</rdfs:comment>
</owl:Class>

<owl:Class rdf:ID= "MilitaryReserveForce">
<rdfs:subClassOf rdf:resource 
="http://127.0.0.1:8000/ontology/SUMO.owl#MilitaryOrganization"/>
<rdfs:comment>MilitaryReserveForce is the subclass
of MilitaryOrganizations that consist of forces trained in military
procedures and activities, which are subject to being called to active duty
if needed.</rdfs:comment>
</owl:Class>

<owl:Class rdf:ID= "MilitaryService">
<rdfs:subClassOf rdf:resource 
="http://127.0.0.1:8000/ontology/SUMO.owl#MilitaryOrganization"/>
<rdfs:comment>A branch of the armed forces of a Nation.
For example, there are five military services in the United States, the 
army,
the navy, the air force, the marines, and the coast guard.</rdfs:comment>
</owl:Class>

<owl:Class rdf:ID= "MilitaryShip">
<rdfs:subClassOf rdf:resource ="#Ship"/>
<rdfs:subClassOf rdf:resource ="#MilitaryVehicle"/>
<rdfs:comment>Any Ship which is made for a MilitaryOrganization.
This includes aircraft carriers, destroyers, etc.</rdfs:comment>
</owl:Class>

<owl:Class rdf:ID= "MilitarySquad">
<rdfs:subClassOf rdf:resource ="#MilitaryUnit"/>
<rdfs:comment>Any MilitaryUnit with the rank of squad.</rdfs:comment>
</owl:Class>

<owl:Class rdf:ID= "MilitarySurplus">
<rdfs:subClassOf rdf:resource ="#MilitaryArtifact"/>
<rdfs:comment>Any MilitaryArtifact which is sold to a
non-military customer.</rdfs:comment>
</owl:Class>

<owl:Class rdf:ID= "MilitaryTank">
<rdfs:subClassOf rdf:resource ="#MilitaryVehicle"/>
<rdfs:subClassOf rdf:resource ="#RoadVehicle"/>
<rdfs:subClassOf rdf:resource ="#ArtilleryGun"/>
<rdfs:comment>A MilitaryVehicle that moves along the ground
on treaded wheels and that contains a large cannon.</rdfs:comment>
</owl:Class>

<owl:Class rdf:ID= "MilitaryUnit">
<rdfs:subClassOf rdf:resource 
="http://127.0.0.1:8000/ontology/SUMO.owl#MilitaryOrganization"/>
<rdfs:comment>Any MilitaryOrganization that can be dispatched
to an area of operations.</rdfs:comment>
</owl:Class>

<owl:Class rdf:ID= "MilitaryVehicle">
<rdfs:subClassOf rdf:resource 
="http://127.0.0.1:8000/ontology/SUMO.owl#Vehicle"/>
<rdfs:comment>Any Vehicle which is intended to be
used by a MilitaryOrganization.</rdfs:comment>
</owl:Class>

<owl:Class rdf:ID= "MilitaryWatercraft">
<rdfs:subClassOf rdf:resource ="#Watercraft"/>
<rdfs:comment>MilitaryWatercraft is the class of
all Watercraft owned or leased for use by some 
MilitaryOrganization.</rdfs:comment>
</owl:Class>

<owl:Class rdf:ID= "Milk">
<rdfs:subClassOf rdf:resource ="#LiquidBodySubstance"/>
<rdfs:subClassOf rdf:resource 
="http://127.0.0.1:8000/ontology/SUMO.owl#Beverage"/>
<rdfs:comment>A nutritious BodySubstance produced by Mammals.</rdfs:comment>
</owl:Class>

<owl:Class rdf:ID= "Millennium">
<rdfs:subClassOf rdf:resource 
="http://127.0.0.1:8000/ontology/SUMO.owl#TimeDuration"/>
<rdfs:subClassOf rdf:resource 
="http://127.0.0.1:8000/ontology/SUMO.owl#UnitOfMeasure"/>
<rdfs:comment>The TimeDuration of 1000 years.</rdfs:comment>
</owl:Class>

<owl:Class rdf:ID= "MineOrWell">
<rdfs:subClassOf rdf:resource 
="http://127.0.0.1:8000/ontology/SUMO.owl#StationaryArtifact"/>
<rdfs:comment>An construction in the earth from which
Minerals or Water is removed, either in pure form or as part of
some other Substance.</rdfs:comment>
</owl:Class>

<owl:Class rdf:ID= "Mirror">
<rdfs:subClassOf rdf:resource 
="http://127.0.0.1:8000/ontology/SUMO.owl#Artifact"/>
<rdfs:comment>An Artifact with a surface that is capable of
displaying an image by reflecting light.</rdfs:comment>
</owl:Class>

<owl:Class rdf:ID= "Missile">
<rdfs:subClassOf rdf:resource ="#Projectile"/>
<rdfs:subClassOf rdf:resource ="#SelfPoweredDevice"/>
<rdfs:comment>A Projectile that is self-propelled and contains
an ExplosiveDevice.</rdfs:comment>
</owl:Class>

<owl:Class rdf:ID= "MissionOrganization">
<rdfs:subClassOf rdf:resource 
="http://127.0.0.1:8000/ontology/SUMO.owl#ReligiousOrganization"/>
<rdfs:comment>The class of ReligiousOrganizations
that send members to foreign countries with the aim of converting citizens
of those countries to the beliefs of the 
ReligiousOrganization.</rdfs:comment>
</owl:Class>

<owl:Class rdf:ID= "MixedLanguage">
<rdfs:subClassOf rdf:resource 
="http://127.0.0.1:8000/ontology/SUMO.owl#SpokenHumanLanguage"/>
<rdfs:comment>A MixedLanguage is a SpokenHumanLanguage
that combines grammar and lexical items from two or more languages to create
a new language that is essentially a linguistic mixture.</rdfs:comment>
</owl:Class>

<owl:Class rdf:ID= "MmMercury">
<rdfs:subClassOf rdf:resource ="#AtmosphericPressureMeasure"/>
<rdf:type rdf:resource = 
"http://127.0.0.1:8000/ontology/SUMO.owl#UnitOfMeasure"/>
<rdfs:comment>MmMercury is a UnitOfMeasure
for barometricPressure.  It is used to express the number
of millimeters of mercury supported in a mercurial barometer
by the surrounding air pressure.</rdfs:comment>
</owl:Class>

<owl:Class rdf:ID= "MobileResidence">
<rdfs:subClassOf rdf:resource 
="http://127.0.0.1:8000/ontology/SUMO.owl#Artifact"/>
<sumo:disjoint rdf:resource = "http://127.0.0.1:8000/ontology/SUMO.owl#Residence"
/>
<rdfs:comment>Anything which serves to house people but
which changes its location from time to time, e.g. a motorhome, a mobile
home, a Tend, etc.  Note that MobileResidence is disjoint from Residence,
because the latter is a subclass of StationaryArtifact.</rdfs:comment>
</owl:Class>

<owl:Class rdf:ID= "ModellingPosition">
<rdfs:subClassOf rdf:resource 
="http://127.0.0.1:8000/ontology/SUMO.owl#Position"/>
<rdfs:comment>Any Position which involves posing for an
artist or photographer.</rdfs:comment>
</owl:Class>

<owl:Class rdf:ID= "Mole">
<rdfs:subClassOf rdf:resource 
="http://127.0.0.1:8000/ontology/SUMO.owl#MassMeasure"/>
<rdf:type rdf:resource = 
"http://127.0.0.1:8000/ontology/SUMO.owl#SystemeInternationalUnit"/>
<rdfs:comment>SI amount of substance unit. symbol: mol. It is one
of the base units in SI. It is defined as follows:  the Mole is the
amount of substance of a system which contains as many elementary entities
as there are atoms in 0.012 Kilograms of carbon 12.  Note that, when this
UnitOfMeasure is used, the elementary entities must be specified - they
may be atoms, molecules, ions, electrons, etc. or groups of such
particles.</rdfs:comment>
</owl:Class>

<owl:Class rdf:ID= "MonophonicMusic">
<rdfs:subClassOf rdf:resource ="http://127.0.0.1:8000/ontology/SUMO.owl#Music"/>
<rdfs:comment>Music which has a single part, i.e. Music
which cannot be divided into two or more contemporaneous subProcesses which
are also instances of Music.</rdfs:comment>
</owl:Class>

<owl:Class rdf:ID= "MonsoonClimateZone">
<rdfs:subClassOf rdf:resource ="#TropicalClimateZone"/>
<rdfs:comment>MonsoonClimateZone is the class
of TropicalClimateZones in which there is a short dry season between
rains heavy enough to keep the ground wet all through the year.  This
is Koeppen climate system subtype 'Aw'.</rdfs:comment>
</owl:Class>

<owl:Class rdf:ID= "Monument">
<rdfs:subClassOf rdf:resource 
="http://127.0.0.1:8000/ontology/SUMO.owl#StationaryArtifact"/>
<rdfs:comment>A StationaryArtifact whose purpose is to commemorate
a person, animal or event.</rdfs:comment>
</owl:Class>

<owl:Class rdf:ID= "Moon">
<rdfs:subClassOf rdf:resource ="#NaturalSatellite"/>
<rdfs:comment>Moon is the class of NaturalSatellites that
orbit planets or large asteroids.</rdfs:comment>
</owl:Class>

<owl:Class rdf:ID= "Morning">
<rdfs:subClassOf rdf:resource ="#DayTime"/>
<rdfs:comment>The class of TimeIntervals that begin at Sunrise
and end at noon.</rdfs:comment>
</owl:Class>

<owl:Class rdf:ID= "MortarGun">
<rdfs:subClassOf rdf:resource ="#ArtilleryGun"/>
<rdfs:comment>A short-range Gun that is positioned on the ground
at a high angle and fires explosive shells.</rdfs:comment>
</owl:Class>

<owl:Class rdf:ID= "Mortgage">
<rdfs:subClassOf rdf:resource ="#Loan"/>
<rdfs:comment>A loan to finance the purchase of real estate, usually with 
specified payment
periods and interest rates.</rdfs:comment>
</owl:Class>

<owl:Class rdf:ID= "Moth">
<rdfs:subClassOf rdf:resource ="http://127.0.0.1:8000/ontology/SUMO.owl#Insect"/>
<rdfs:comment>Nocturnal Insect with a large body and 
antennae.</rdfs:comment>
</owl:Class>

<owl:Class rdf:ID= "MotionDownward">
<rdfs:subClassOf rdf:resource ="http://127.0.0.1:8000/ontology/SUMO.owl#Motion"/>
<rdfs:comment>Motion where an Object is moving toward the
ground.</rdfs:comment>
</owl:Class>

<owl:Class rdf:ID= "MotionPicture">
<rdfs:subClassOf rdf:resource 
="http://127.0.0.1:8000/ontology/SUMO.owl#ContentBearingObject"/>
<rdfs:comment>A ContentBearingObject which depicts motion
(and which may have an audio or text component as well).  This Class covers
films, videos, etc.</rdfs:comment>
</owl:Class>

<owl:Class rdf:ID= "MotionPictureScene">
<rdfs:subClassOf rdf:resource ="#MotionPicture"/>
<rdfs:comment>A discrete part of a MotionPicture which is set in
the same time period and the same location.</rdfs:comment>
</owl:Class>

<owl:Class rdf:ID= "MotionPictureShot">
<rdfs:subClassOf rdf:resource ="#MotionPicture"/>
<rdfs:comment>A unit of action in a MotionPicture, a
MotionPictureShot is a sequence of images which are captured by a single
camera without interruption.</rdfs:comment>
</owl:Class>

<owl:Class rdf:ID= "MotionUpward">
<rdfs:subClassOf rdf:resource ="http://127.0.0.1:8000/ontology/SUMO.owl#Motion"/>
<sumo:disjoint rdf:resource = "#MotionDownward" />
<rdfs:comment>Motion where an Object is moving away
from the ground.</rdfs:comment>
</owl:Class>

<owl:Class rdf:ID= "MotorOil">
<rdfs:subClassOf rdf:resource ="#PetroleumLubricant"/>
<rdfs:comment>MotorOil is the subclass of PetroleumLubricants
that are used to lubricate motors.</rdfs:comment>
</owl:Class>

<owl:Class rdf:ID= "Motorcycle">
<rdfs:subClassOf rdf:resource ="#SelfPoweredRoadVehicle"/>
<rdfs:comment>Motorcycle is the subclass of RoadVehicles
that have two wheels one behind the other in the frame, upon which the rider
sits on a seat above the engine.</rdfs:comment>
</owl:Class>

<owl:Class rdf:ID= "MotorizedRailwayCar">
<rdfs:subClassOf rdf:resource ="#RollingStock"/>
<rdfs:subClassOf rdf:resource ="#SelfPoweredVehicle"/>
<rdfs:comment>MotorizedRailwayCar is the subclass
of railway cars that carry their own power source.</rdfs:comment>
</owl:Class>

<owl:Class rdf:ID= "Mounting">
<rdfs:subClassOf rdf:resource 
="http://127.0.0.1:8000/ontology/SUMO.owl#BodyMotion"/>
<rdfs:comment>Any BodyMotion which results in being On
something else.</rdfs:comment>
</owl:Class>

<owl:Class rdf:ID= "Mouse">
<rdfs:subClassOf rdf:resource ="http://127.0.0.1:8000/ontology/SUMO.owl#Rodent"/>
<rdfs:comment>A Rodent that has a hairless tail like a Rat
but that is smaller than a Rat.</rdfs:comment>
</owl:Class>

<owl:Class rdf:ID= "Mouth">
<rdfs:subClassOf rdf:resource 
="http://127.0.0.1:8000/ontology/SUMO.owl#AnimalAnatomicalStructure"/>
<rdfs:subClassOf rdf:resource 
="http://127.0.0.1:8000/ontology/SUMO.owl#BodyPart"/>
<rdfs:comment>Part of the Face, used for Ingesting Food
and Vocalizing.</rdfs:comment>
</owl:Class>

<owl:Class rdf:ID= "MoveableHoliday">
<rdfs:subClassOf rdf:resource ="#Holiday"/>
<rdfs:comment>MoveableHoliday is the class of
Holidays whose observance is not fixed to recurrences of any particular
calendar day.  For example, Memorial Day is observed on the last Monday
of May.</rdfs:comment>
</owl:Class>

<owl:Class rdf:ID= "MovingResidence">
<rdfs:subClassOf rdf:resource 
="http://127.0.0.1:8000/ontology/SUMO.owl#Transfer"/>
<rdfs:comment>Any instance of the process of changing one's
residence, i.e. moving one's belongings to a new home.</rdfs:comment>
</owl:Class>

<owl:Class rdf:ID= "Mule">
<rdfs:subClassOf rdf:resource 
="http://127.0.0.1:8000/ontology/SUMO.owl#HoofedMammal"/>
<rdfs:subClassOf rdf:resource ="#DomesticAnimal"/>
<rdfs:comment>The product of a Male Donkey and a Female
Horse.  Mules are always sterile.</rdfs:comment>
</owl:Class>

<owl:Class rdf:ID= "MultiGraph">
<rdfs:subClassOf rdf:resource ="#Graph"/>
<rdfs:comment>The Class of multigraphs.  A multigraph
is a Graph containing at least one pair of GraphNodes that are
connected by more than one GraphArc.</rdfs:comment>
</owl:Class>

<owl:Class rdf:ID= "Murder">
<rdfs:subClassOf rdf:resource 
="http://127.0.0.1:8000/ontology/SUMO.owl#Killing"/>
<rdfs:subClassOf rdf:resource ="#CriminalAction"/>
<rdfs:comment>Impermissible Killing of a Human.</rdfs:comment>
</owl:Class>

<owl:Class rdf:ID= "Museum">
<rdfs:subClassOf rdf:resource 
="http://127.0.0.1:8000/ontology/SUMO.owl#EducationalOrganization"/>
<rdfs:comment>An EducationalOrganization where Artifacts of historic,
scientific or aesthetic value are collected and exhibited.</rdfs:comment>
</owl:Class>

<owl:Class rdf:ID= "MusicalComposition">
<rdfs:subClassOf rdf:resource ="http://127.0.0.1:8000/ontology/SUMO.owl#Text"/>
<rdfs:comment>A Text that expresses the notes,
words, etc. of a song or other sort of Music.</rdfs:comment>
</owl:Class>

<owl:Class rdf:ID= "MusicalPerformance">
<rdfs:subClassOf rdf:resource ="#Performance"/>
<rdfs:comment>A Performance that consists exclusively of
Music, e.g. an orchestra playing a symphony to an assembled 
audience.</rdfs:comment>
</owl:Class>

<owl:Class rdf:ID= "MysteryStory">
<rdfs:subClassOf rdf:resource 
="http://127.0.0.1:8000/ontology/SUMO.owl#FictionalText"/>
<rdfs:comment>A FictionalText whose central plot element is a
crime of some sort, usually a murder.</rdfs:comment>
</owl:Class>

<owl:Class rdf:ID= "Nail">
<rdfs:subClassOf rdf:resource 
="http://127.0.0.1:8000/ontology/SUMO.owl#AttachingDevice"/>
<rdfs:comment>An AttachingDevice which is a thin piece of metal, with
or without a head, that is fastened with a hammer.</rdfs:comment>
</owl:Class>

<owl:Class rdf:ID= "NailDigit">
<rdfs:subClassOf rdf:resource 
="http://127.0.0.1:8000/ontology/SUMO.owl#AnimalAnatomicalStructure"/>
<rdfs:comment>Any of the horny structures which are found
on the DigitAppendages of Primates and other Animals.</rdfs:comment>
</owl:Class>

<owl:Class rdf:ID= "Narcotic">
<rdfs:subClassOf rdf:resource ="#ControlledSubstance"/>
<rdfs:comment>Narcotic is a subclass of addictive
BiologicallyActiveSubstances that have damping effects on the
nervous system and may be fatal in large doses.</rdfs:comment>
</owl:Class>

<owl:Class rdf:ID= "NarrativeText">
<rdfs:subClassOf rdf:resource ="http://127.0.0.1:8000/ontology/SUMO.owl#Text"/>
<rdfs:comment>Any Text that tells a story, whether true
or false.</rdfs:comment>
</owl:Class>

<owl:Class rdf:ID= "NationalFlag">
<rdfs:subClassOf rdf:resource ="#Flag"/>
<rdfs:comment>A Flag that is the official flag of a Nation,
e.g. the stars and stripes is the NationalFlag of the 
UnitedStates.</rdfs:comment>
</owl:Class>

<owl:Class rdf:ID= "NationalGovernment">
<rdfs:subClassOf rdf:resource 
="http://127.0.0.1:8000/ontology/SUMO.owl#Government"/>
<rdfs:comment>NationalGovernment is the class of
governments of Nations.</rdfs:comment>
</owl:Class>

<owl:Class rdf:ID= "NaturalSatellite">
<rdfs:subClassOf rdf:resource ="#Satellite"/>
<rdfs:subClassOf rdf:resource 
="http://127.0.0.1:8000/ontology/SUMO.owl#AstronomicalBody"/>
<sumo:disjoint rdf:resource = "http://127.0.0.1:8000/ontology/SUMO.owl#Artifact"
/>
<rdfs:comment>NaturalSatellite is the class of
large, naturally occurring astronomical bodies orbiting some other
AstronomicalBody.</rdfs:comment>
</owl:Class>

<owl:Class rdf:ID= "Navy">
<rdfs:subClassOf rdf:resource ="#MilitaryService"/>
<rdfs:comment>MilitaryServices that are sea forces.</rdfs:comment>
</owl:Class>

<owl:Class rdf:ID= "Neck">
<rdfs:subClassOf rdf:resource 
="http://127.0.0.1:8000/ontology/SUMO.owl#AnimalAnatomicalStructure"/>
<rdfs:subClassOf rdf:resource 
="http://127.0.0.1:8000/ontology/SUMO.owl#BodyPart"/>
<rdfs:comment>The part of the body that connects the Head to the
rest of the body.</rdfs:comment>
</owl:Class>

<owl:Class rdf:ID= "Nectar">
<rdfs:subClassOf rdf:resource 
="http://127.0.0.1:8000/ontology/SUMO.owl#PlantSubstance"/>
<rdfs:comment>A sweet, sticky liquid that is produced by Plants
and that attracts Insects.</rdfs:comment>
</owl:Class>

<owl:Class rdf:ID= "Negotiating">
<rdfs:subClassOf rdf:resource 
="http://127.0.0.1:8000/ontology/SUMO.owl#Contest"/>
<rdfs:subClassOf rdf:resource 
="http://127.0.0.1:8000/ontology/SUMO.owl#LinguisticCommunication"/>
<rdfs:comment>A Contest where each participant attempts to
maximize his self-interest in a Promise that marks the end of the 
Contest.</rdfs:comment>
</owl:Class>

<owl:Class rdf:ID= "NerveCell">
<rdfs:subClassOf rdf:resource ="http://127.0.0.1:8000/ontology/SUMO.owl#Cell"/>
<rdfs:subClassOf rdf:resource 
="http://127.0.0.1:8000/ontology/SUMO.owl#AnimalAnatomicalStructure"/>
<rdfs:comment>The Cells that make up a NervousSystem.</rdfs:comment>
</owl:Class>

<owl:Class rdf:ID= "NervousSystem">
<rdfs:subClassOf rdf:resource ="http://127.0.0.1:8000/ontology/SUMO.owl#Organ"/>
<rdfs:subClassOf rdf:resource 
="http://127.0.0.1:8000/ontology/SUMO.owl#AnimalAnatomicalStructure"/>
<rdfs:comment>A system in Vertebrates that is made up of
the Brain, the spinal cord, nerves, etc.</rdfs:comment>
</owl:Class>

<owl:Class rdf:ID= "Nest">
<rdfs:subClassOf rdf:resource 
="http://127.0.0.1:8000/ontology/SUMO.owl#CorpuscularObject"/>
<rdfs:comment>Any structure which is created by nonhuman Animals for
the purpose of giving birth to their offspring.</rdfs:comment>
</owl:Class>

<owl:Class rdf:ID= "Neurosis">
<rdfs:comment>Any PsychologicalDysfunction which is not due
to an organic impairment of the NervousSystem.</rdfs:comment>
</owl:Class>

<owl:Class rdf:ID= "NewTestament">
<rdfs:subClassOf rdf:resource ="http://127.0.0.1:8000/ontology/SUMO.owl#Book"/>
<sumo:subsumesContentClass rdf:resource = "#ChristianGospel" />
<rdfs:comment>The second and final part of the ChristianBible,
describing the life and teachings of Jesus Christ and the activities of his
apostles.</rdfs:comment>
</owl:Class>

<owl:Class rdf:ID= "NewsProgram">
<rdfs:subClassOf rdf:resource ="#BroadcastProgram"/>
<rdfs:comment>A BroadcastProgram that is devoted to
reporting the latest events in a city, region, nation or the world at
large.</rdfs:comment>
</owl:Class>

<owl:Class rdf:ID= "Newspaper">
<rdfs:subClassOf rdf:resource 
="http://127.0.0.1:8000/ontology/SUMO.owl#Periodical"/>
<rdfs:comment>A Periodical that is published on a daily or
weekly basis, that contains Reports, and whose issues are printed on
newsprint paper.</rdfs:comment>
</owl:Class>

<owl:Class rdf:ID= "Newton">
<rdfs:subClassOf rdf:resource 
="http://127.0.0.1:8000/ontology/SUMO.owl#FunctionQuantity"/>
<rdf:type rdf:resource = 
"http://127.0.0.1:8000/ontology/SUMO.owl#SystemeInternationalUnit"/>
<rdfs:comment>SI force measure.  Symbol: N. It is that force
which gives to a mass of 1 kilogram an acceleration of 1 Meter per
SecondDuration.  Newton = m*kg*s^(-2).</rdfs:comment>
</owl:Class>

<owl:Class rdf:ID= "Nickel">
<rdfs:subClassOf rdf:resource 
="http://127.0.0.1:8000/ontology/SUMO.owl#ElementalSubstance"/>
<atomicNumber>28</atomicNumber>
<rdfs:comment>Malleable ductile silvery metallic transition
element.  Discovered by A.F. Cronstedt in 1751.</rdfs:comment>
</owl:Class>

<owl:Class rdf:ID= "NightTime">
<rdfs:subClassOf rdf:resource 
="http://127.0.0.1:8000/ontology/SUMO.owl#TimeInterval"/>
<rdfs:comment>The class of TimeIntervals that begin at Sunset
and end at Sunrise.</rdfs:comment>
</owl:Class>

<owl:Class rdf:ID= "Nitrogen">
<rdfs:subClassOf rdf:resource 
="http://127.0.0.1:8000/ontology/SUMO.owl#ElementalSubstance"/>
<atomicNumber>7</atomicNumber>
<rdfs:comment>Colourless, gaseous element which belongs to
group 15 of the periodic table.  Constitutes ~78 percent of the atmosphere
and is an essential part of the ecosystem.  Nitrogen for industrial
purposes is acquired by the fractional distillation of liquid air.
Chemically inactive, reactive generally only at high temperatures or in
electrical discharges.  It was discovered in 1772 by D.  
Rutherford.</rdfs:comment>
</owl:Class>

<owl:Class rdf:ID= "Nodding">
<rdfs:subClassOf rdf:resource 
="http://127.0.0.1:8000/ontology/SUMO.owl#Gesture"/>
<rdfs:comment>Moving the Head up and down or side to side
to indicate approval or disapproval.</rdfs:comment>
</owl:Class>

<owl:Class rdf:ID= "NonprofitOrganization">
<rdfs:subClassOf rdf:resource 
="http://127.0.0.1:8000/ontology/SUMO.owl#Organization"/>
<sumo:disjoint rdf:resource = 
"http://127.0.0.1:8000/ontology/SUMO.owl#CommercialAgent" />
<rdfs:comment>Any Organization whose purpose is something
other than making a profit.</rdfs:comment>
</owl:Class>

<owl:Class rdf:ID= "NonspecificDisease">
<rdfs:subClassOf rdf:resource ="#InfectiousDisease"/>
<rdfs:comment>The class of InfectiousDiseases that
are not caused by a single type of Microorganism.</rdfs:comment>
</owl:Class>

<owl:Class rdf:ID= "Nose">
<rdfs:subClassOf rdf:resource ="http://127.0.0.1:8000/ontology/SUMO.owl#Organ"/>
<rdfs:subClassOf rdf:resource 
="http://127.0.0.1:8000/ontology/SUMO.owl#AnimalAnatomicalStructure"/>
<rdfs:comment>The Organ of Smelling.</rdfs:comment>
</owl:Class>

<owl:Class rdf:ID= "Nostril">
<rdfs:subClassOf rdf:resource 
="http://127.0.0.1:8000/ontology/SUMO.owl#BodyVessel"/>
<rdfs:subClassOf rdf:resource 
="http://127.0.0.1:8000/ontology/SUMO.owl#AnimalAnatomicalStructure"/>
<rdfs:comment>Either of two BodyVessels that run through the Nose
and connect it to the Throat.</rdfs:comment>
</owl:Class>

<owl:Class rdf:ID= "Novel">
<rdfs:subClassOf rdf:resource 
="http://127.0.0.1:8000/ontology/SUMO.owl#FictionalText"/>
<rdfs:subClassOf rdf:resource ="http://127.0.0.1:8000/ontology/SUMO.owl#Book"/>
<rdfs:comment>A FictionalText that is larger than a ShortStory
and that is bound independently (i.e. it is a Book).</rdfs:comment>
</owl:Class>

<owl:Class rdf:ID= "NuclearWeapon">
<rdfs:subClassOf rdf:resource ="#ExplosiveDevice"/>
<rdfs:subClassOf rdf:resource ="http://127.0.0.1:8000/ontology/SUMO.owl#Weapon"/>
<rdfs:comment>An ExplosiveDevice which achieves its effect
by means of a critical mass of a radioactive substance.</rdfs:comment>
<rdfs:subClassOf rdf:resource ="#RadioactiveWeapon"/>
<rdfs:comment>RadioactiveWeapons whose destructive power is
achieved through nuclear energy.</rdfs:comment>
</owl:Class>

<owl:Class rdf:ID= "OakWood">
<rdfs:subClassOf rdf:resource ="#WoodArtifact"/>
<rdfs:comment>Any WoodArtifact that is made from the Wood of an
oak tree.</rdfs:comment>
</owl:Class>

<owl:Class rdf:ID= "Oar">
<rdfs:subClassOf rdf:resource 
="http://127.0.0.1:8000/ontology/SUMO.owl#TransportationDevice"/>
<rdfs:comment>A Device consisting of a flat, broad surface attached to a
handle that is used as an instrument in Rowing.</rdfs:comment>
</owl:Class>

<owl:Class rdf:ID= "ObliqueAngle">
<rdfs:subClassOf rdf:resource 
="http://127.0.0.1:8000/ontology/SUMO.owl#TwoDimensionalAngle"/>
<rdfs:comment>Any TwoDimensionalAngle that has an
angularMeasure that is greater than 90 AngularDegrees.</rdfs:comment>
</owl:Class>

<owl:Class rdf:ID= "OccupationalTrade">
<rdfs:subClassOf rdf:resource ="#SkilledOccupation"/>
<rdfs:subClassOf rdf:resource ="#ManualLabor"/>
<rdfs:comment>Any Position that involves skilled
manual work.</rdfs:comment>
</owl:Class>

<owl:Class rdf:ID= "Ocean">
<rdfs:subClassOf rdf:resource 
="http://127.0.0.1:8000/ontology/SUMO.owl#SaltWaterArea"/>
<rdfs:subClassOf rdf:resource ="#BodyOfWater"/>
<rdfs:comment>Ocean is the class containing the oceans
that are the major subdivisions of the WorldOcean.  According to
the International Hydrographic Association, there are five oceans:
the AtlanticOcean, PacificOcean, IndianOcean, SouthernOcean,
and ArcticOcean.  Note: The largest oceans, the Atlantic and Pacific,
are subdivided into Northern and Southern regions, but those regions
are not separate Oceans.</rdfs:comment>
</owl:Class>

<owl:Class rdf:ID= "OfferingForPurchase">
<rdfs:subClassOf rdf:resource 
="http://127.0.0.1:8000/ontology/SUMO.owl#Offering"/>
<rdfs:comment>Offering to buy something from someone.</rdfs:comment>
</owl:Class>

<owl:Class rdf:ID= "OfferingForSale">
<rdfs:subClassOf rdf:resource 
="http://127.0.0.1:8000/ontology/SUMO.owl#Offering"/>
<rdfs:comment>Offering to sell something to someone.</rdfs:comment>
</owl:Class>

<owl:Class rdf:ID= "Ohm">
<rdfs:subClassOf rdf:resource 
="http://127.0.0.1:8000/ontology/SUMO.owl#FunctionQuantity"/>
<rdf:type rdf:resource = 
"http://127.0.0.1:8000/ontology/SUMO.owl#SystemeInternationalUnit"/>
<rdfs:comment>SI electric resistance measure. It is the electric
resistance between two points of a conductor when a constant difference
of potential of 1 Volt, applied between these two points,
produces in this conductor a current of 1 Ampere, this conductor not
being the force of any electromotive force.  Ohm = V/A =
m^2*kg*s^(-3)*A^(-2).</rdfs:comment>
</owl:Class>

<owl:Class rdf:ID= "Oil">
<rdfs:subClassOf rdf:resource 
="http://127.0.0.1:8000/ontology/SUMO.owl#Solution"/>
<rdfs:comment>A greasy, viscous Solution that cannot be mixed
with Water.  Note that this general class covers petroleum oil,
vegetable oil, animal fat, etc.</rdfs:comment>
</owl:Class>

<owl:Class rdf:ID= "OilPaint">
<rdfs:subClassOf rdf:resource ="#Paint"/>
<sumo:disjoint rdf:resource = "#WatercolorPaint" />
<rdfs:comment>Any Paint which is an oil-based Solution.</rdfs:comment>
</owl:Class>

<owl:Class rdf:ID= "OilPicture">
<rdfs:subClassOf rdf:resource ="#PaintedPicture"/>
<sumo:disjoint rdf:resource = "#WatercolorPicture" />
<rdfs:comment>Any OilPicture which is created
with oil-based paints.</rdfs:comment>
</owl:Class>

<owl:Class rdf:ID= "OldTestament">
<rdfs:subClassOf rdf:resource ="http://127.0.0.1:8000/ontology/SUMO.owl#Book"/>
<rdfs:comment>The first part of the ChristianBible, describing
the history of the Hebrew people.</rdfs:comment>
</owl:Class>

<owl:Class rdf:ID= "OlympicGames">
<rdfs:subClassOf rdf:resource ="http://127.0.0.1:8000/ontology/SUMO.owl#Sport"/>
<rdfs:comment>A sports event where athletes from various countries
compete against one another.  The Olympics are now held every two years, 
either in
the winter or the summer.</rdfs:comment>
</owl:Class>

<owl:Class rdf:ID= "Opening">
<rdfs:subClassOf rdf:resource ="http://127.0.0.1:8000/ontology/SUMO.owl#Motion"/>
<sumo:relatedInternalConcept rdf:resource = "#Closing" />
<rdfs:comment>The Class of Processes where an aperture is
created in an Object.  Note that the aperture may be created intentionally,
as when one opens a door, or unintentionally, as when the ground ruptures
in a seismic event.</rdfs:comment>
</owl:Class>

<owl:Class rdf:ID= "OpeningEyes">
<rdfs:subClassOf rdf:resource ="#EyeMotion"/>
<sumo:disjoint rdf:resource = "#ClosingEyes" />
<rdfs:comment>The EyeMotion of relaxing the eye lids so that
the corneas are exposed to light.</rdfs:comment>
</owl:Class>

<owl:Class rdf:ID= "Opera">
<rdfs:subClassOf rdf:resource ="#DramaticPlay"/>
<rdfs:comment>A DramaticPlay that is set to Music.</rdfs:comment>
</owl:Class>

<owl:Class rdf:ID= "Opium">
<rdfs:subClassOf rdf:resource ="#Depressant"/>
<rdfs:subClassOf rdf:resource 
="http://127.0.0.1:8000/ontology/SUMO.owl#PlantSubstance"/>
<rdfs:comment>A substance harvested from the seed capsules of the
opium poppy that contains various powerful alkaloids.</rdfs:comment>
</owl:Class>

<owl:Class rdf:ID= "OpticalDevice">
<rdfs:subClassOf rdf:resource ="http://127.0.0.1:8000/ontology/SUMO.owl#Device"/>
<rdfs:comment>A Device which enables someone to see something
more clearly or with greater magnification.</rdfs:comment>
</owl:Class>

<owl:Class rdf:ID= "OrangeFruit">
<rdfs:subClassOf rdf:resource 
="http://127.0.0.1:8000/ontology/SUMO.owl#FruitOrVegetable"/>
<rdfs:subClassOf rdf:resource ="http://127.0.0.1:8000/ontology/SUMO.owl#Food"/>
<rdfs:comment>A citrus FruitOrVegetable that has an orange
skin and a sweet, acidic flavor.</rdfs:comment>
</owl:Class>

<owl:Class rdf:ID= "Orchestra">
<rdfs:subClassOf rdf:resource 
="http://127.0.0.1:8000/ontology/SUMO.owl#GroupOfPeople"/>
<rdfs:comment>A GroupOfPeople that create InstrumentalMusic
together.  Note that this class covers marching bands, rock and jazz bands,
as well as groups of people that play classical music 
together.</rdfs:comment>
</owl:Class>

<owl:Class rdf:ID= "OrchestralConducting">
<rdfs:subClassOf rdf:resource 
="http://127.0.0.1:8000/ontology/SUMO.owl#Guiding"/>
<rdfs:comment>The Process of directing an orchestra.</rdfs:comment>
</owl:Class>

<owl:Class rdf:ID= "Order">
<rdfs:subClassOf rdf:resource 
="http://127.0.0.1:8000/ontology/SUMO.owl#Sentence"/>
<rdfs:comment>A Sentence that expresses an order for something or
that something be done.</rdfs:comment>
</owl:Class>

<owl:Class rdf:ID= "OrganicCompound">
<rdfs:subClassOf rdf:resource 
="http://127.0.0.1:8000/ontology/SUMO.owl#CompoundSubstance"/>
<rdfs:comment>Any CompoundSubstance that has a Carbon
base.</rdfs:comment>
</owl:Class>

<owl:Class rdf:ID= "Organification">
<rdfs:subClassOf rdf:resource 
="http://127.0.0.1:8000/ontology/SUMO.owl#OrganOrTissueProcess"/>
<rdfs:comment>Any BiologicalProcess that results in
the formation of an Organ.</rdfs:comment>
</owl:Class>

<owl:Class rdf:ID= "OrganizationOfNations">
<rdfs:subClassOf rdf:resource ="#InternationalOrganization"/>
<rdfs:comment>InternationalOrganization is the
class of Organizations whose members are Nations.</rdfs:comment>
</owl:Class>

<owl:Class rdf:ID= "OrganizationalBoard">
<rdfs:subClassOf rdf:resource 
="http://127.0.0.1:8000/ontology/SUMO.owl#Organization"/>
<rdfs:comment>Part of an Organization that
is responsible for managing the Organization.</rdfs:comment>
</owl:Class>

<owl:Class rdf:ID= "OrganizationalMerging">
<rdfs:subClassOf rdf:resource 
="http://127.0.0.1:8000/ontology/SUMO.owl#OrganizationalProcess"/>
<rdfs:comment>The process of two or more
Organizations merging into a single Organization.</rdfs:comment>
</owl:Class>

<owl:Class rdf:ID= "Orthography">
<rdfs:subClassOf rdf:resource 
="http://127.0.0.1:8000/ontology/SUMO.owl#Procedure"/>
<rdfs:comment>A method for representing the sounds of a Language
with written Characters.</rdfs:comment>
</owl:Class>

<owl:Class rdf:ID= "Ossification">
<rdfs:subClassOf rdf:resource 
="http://127.0.0.1:8000/ontology/SUMO.owl#OrganOrTissueProcess"/>
<rdfs:comment>Any BiologicalProcess that results in the
formation of Bones.</rdfs:comment>
</owl:Class>

<owl:Class rdf:ID= "OutdoorClothing">
<rdfs:subClassOf rdf:resource 
="http://127.0.0.1:8000/ontology/SUMO.owl#Clothing"/>
<rdfs:comment>Clothing that is intended to be worn
outdoors.</rdfs:comment>
</owl:Class>

<owl:Class rdf:ID= "OuterSpaceRegion">
<rdfs:subClassOf rdf:resource ="#SpaceRegion"/>
<rdfs:comment>The class of all Regions which are
neither GeographicAreas nor AtmosphericRegions.</rdfs:comment>
</owl:Class>

<owl:Class rdf:ID= "Outside">
<rdfs:subClassOf rdf:resource ="http://127.0.0.1:8000/ontology/SUMO.owl#Region"/>
<rdfs:comment>Any Region which is not enclosed by a Building
or part of a Building.</rdfs:comment>
</owl:Class>

<owl:Class rdf:ID= "Oval">
<rdfs:subClassOf rdf:resource 
="http://127.0.0.1:8000/ontology/SUMO.owl#ClosedTwoDimensionalFigure"/>
<rdfs:comment>The class of ClosedTwoDimensionalFigures that are
produced by the intersection of a Cone with a 
ClosedTwoDimensionalFigure.</rdfs:comment>
</owl:Class>

<owl:Class rdf:ID= "Oven">
<rdfs:subClassOf rdf:resource ="#HeatingDevice"/>
<rdfs:subClassOf rdf:resource ="#Container"/>
<rdfs:comment>A HeatingDevice with a door for inserting and removing
Food that is to be baked.</rdfs:comment>
</owl:Class>

<owl:Class rdf:ID= "OverseasArea">
<rdfs:subClassOf rdf:resource ="#DependencyOrSpecialSovereigntyArea"/>
<rdfs:comment>OverseasArea is the class of
GeopoliticalAreas that are related to a Nation as overseas
territories, possessions, protectorates, or departments.</rdfs:comment>
</owl:Class>

<owl:Class rdf:ID= "Owl">
<rdfs:subClassOf rdf:resource ="http://127.0.0.1:8000/ontology/SUMO.owl#Bird"/>
<rdfs:comment>A nocturnal bird of prey with a large head and
forward-facing eyes.</rdfs:comment>
</owl:Class>

<owl:Class rdf:ID= "Oxidation">
<rdfs:subClassOf rdf:resource 
="http://127.0.0.1:8000/ontology/SUMO.owl#ChemicalDecomposition"/>
<rdfs:comment>Any ChemicalProcess where Electrons
are removed from the substance undergoing the 
ChemicalProcess.</rdfs:comment>
</owl:Class>

<owl:Class rdf:ID= "Oxygen">
<rdfs:subClassOf rdf:resource 
="http://127.0.0.1:8000/ontology/SUMO.owl#ElementalSubstance"/>
<atomicNumber>8</atomicNumber>
<rdfs:comment>A colourless, odourless gaseous element belonging to
group 16 of the periodic table. It is the most abundant element present in
the earth's crust. It also makes up 20.8 percent of the Earth's atmosphere.
For industrial purposes, it is separated from liquid air by fractional
distillation. It is used in high temperature welding, and in breathing. It
commonly comes in the form of Oxygen, but is found as Ozone in the upper
atmosphere. It was discovered by Priestley in 1774.</rdfs:comment>
</owl:Class>

<owl:Class rdf:ID= "Page">
<rdfs:subClassOf rdf:resource 
="http://127.0.0.1:8000/ontology/SUMO.owl#Artifact"/>
<rdfs:comment>A single piece of Paper.</rdfs:comment>
</owl:Class>

<owl:Class rdf:ID= "Paint">
<rdfs:subClassOf rdf:resource 
="http://127.0.0.1:8000/ontology/SUMO.owl#Solution"/>
<rdfs:comment>Any Solution which is capable of Coloring 
something.</rdfs:comment>
</owl:Class>

<owl:Class rdf:ID= "PaintedPicture">
<rdfs:subClassOf rdf:resource 
="http://127.0.0.1:8000/ontology/SUMO.owl#ArtWork"/>
<rdfs:comment>Any ArtWork which is produced by Painting.</rdfs:comment>
</owl:Class>

<owl:Class rdf:ID= "Painting">
<rdfs:subClassOf rdf:resource 
="http://127.0.0.1:8000/ontology/SUMO.owl#Covering"/>
<rdfs:subClassOf rdf:resource 
="http://127.0.0.1:8000/ontology/SUMO.owl#Coloring"/>
<rdfs:comment>The application of Paint to a surface.  Note that
this class covers both ArtPainting (the creation of PaintedPictures), as
well as painting one's kitchen, for example.</rdfs:comment>
</owl:Class>

<owl:Class rdf:ID= "Pancreas">
<rdfs:subClassOf rdf:resource ="#Gland"/>
<rdfs:comment>A large Gland that secretes Insulin and other
substances.</rdfs:comment>
</owl:Class>

<owl:Class rdf:ID= "Paper">
<rdfs:subClassOf rdf:resource 
="http://127.0.0.1:8000/ontology/SUMO.owl#Artifact"/>
<rdfs:comment>An Artifact made of cellulose pulp that is intended
to contain a Text.</rdfs:comment>
</owl:Class>

<owl:Class rdf:ID= "Paragraph">
<rdfs:subClassOf rdf:resource ="http://127.0.0.1:8000/ontology/SUMO.owl#Text"/>
<rdfs:comment>A Text which consists of one or more sentences,
begins with an indented line, and expresses a single topic.</rdfs:comment>
</owl:Class>

<owl:Class rdf:ID= "Park">
<rdfs:subClassOf rdf:resource 
="http://127.0.0.1:8000/ontology/SUMO.owl#LandArea"/>
<rdfs:comment>A LandArea which is intended to be used for
recreation and/or exercise.  Note that a Park can be either publicly
or privately owned.</rdfs:comment>
</owl:Class>

<owl:Class rdf:ID= "ParkingLot">
<rdfs:subClassOf rdf:resource 
="http://127.0.0.1:8000/ontology/SUMO.owl#StationaryArtifact"/>
<rdfs:comment>A LandArea which has been levelled, paved, and
marked off for parking Automobiles.</rdfs:comment>
</owl:Class>

<owl:Class rdf:ID= "Parliament">
<rdfs:subClassOf rdf:resource ="#LegislativeOrganization"/>
<rdfs:comment>Parliament is the subclass of
LegislativeOrganizations similar to that of the United 
Kingdom.</rdfs:comment>
</owl:Class>

<owl:Class rdf:ID= "PartTimePosition">
<rdfs:subClassOf rdf:resource 
="http://127.0.0.1:8000/ontology/SUMO.owl#Position"/>
<rdfs:comment>Any Position where the employee is not
salaried and is paid for less than 40 hours of work per week.</rdfs:comment>
</owl:Class>

<owl:Class rdf:ID= "Partnership">
<rdfs:subClassOf rdf:resource 
="http://127.0.0.1:8000/ontology/SUMO.owl#CommercialAgent"/>
<rdfs:comment>A CommercialAgent that is owned by more
than one person.</rdfs:comment>
</owl:Class>

<owl:Class rdf:ID= "PartyPlatform">
<rdfs:subClassOf rdf:resource 
="http://127.0.0.1:8000/ontology/SUMO.owl#FactualText"/>
<rdfs:comment>A Text which is authored by a PoliticalParty
and which contains the core goals and principles of the PoliticalParty for a
particular year or election cycle.</rdfs:comment>
</owl:Class>

<owl:Class rdf:ID= "Pascal">
<rdfs:subClassOf rdf:resource 
="http://127.0.0.1:8000/ontology/SUMO.owl#FunctionQuantity"/>
<rdf:type rdf:resource = 
"http://127.0.0.1:8000/ontology/SUMO.owl#SystemeInternationalUnit"/>
<rdfs:comment>SI pressure measure.  Symbol:Pa. It is the
pressure of one Newton per square Meter.  Pascal = N/m^2
= m^(-1)*kg*s^(-2).</rdfs:comment>
</owl:Class>

<owl:Class rdf:ID= "PassCertificate">
<rdfs:subClassOf rdf:resource 
="http://127.0.0.1:8000/ontology/SUMO.owl#Certificate"/>
<rdfs:comment>A Certificate that allows the holder to
be at or away from a specified location, e.g. a pass for a leave of
absence, a hall pass, a pass to enter a cleared facility, 
etc.</rdfs:comment>
</owl:Class>

<owl:Class rdf:ID= "PassingABill">
<rdfs:subClassOf rdf:resource 
="http://127.0.0.1:8000/ontology/SUMO.owl#PoliticalProcess"/>
<rdfs:subClassOf rdf:resource 
="http://127.0.0.1:8000/ontology/SUMO.owl#Declaring"/>
<rdfs:comment>The Process of converting a LegislativeBill
into Law by a duly authorized legislative body of Government.</rdfs:comment>
</owl:Class>

<owl:Class rdf:ID= "Passport">
<rdfs:subClassOf rdf:resource ="#License"/>
<rdfs:comment>A License which identifies the holder and permits
travel between different countries.</rdfs:comment>
</owl:Class>

<owl:Class rdf:ID= "PayCheck">
<rdfs:subClassOf rdf:resource ="#Check"/>
<rdfs:comment>A check issued to an employee in payment of salary or 
wages.</rdfs:comment>
</owl:Class>

<owl:Class rdf:ID= "Payment">
<rdfs:subClassOf rdf:resource 
="http://127.0.0.1:8000/ontology/SUMO.owl#FinancialTransaction"/>
<rdfs:comment>The partial or complete discharge of an obligation by
its settlement in the form of the transfer of funds, assets, or services 
equal
to the monetary value of part or all of the debtor's 
obligation.</rdfs:comment>
</owl:Class>

<owl:Class rdf:ID= "Pea">
<rdfs:subClassOf rdf:resource ="http://127.0.0.1:8000/ontology/SUMO.owl#Seed"/>
<rdfs:subClassOf rdf:resource ="http://127.0.0.1:8000/ontology/SUMO.owl#Food"/>
<rdfs:comment>The edible Seed of a pea plant.</rdfs:comment>
</owl:Class>

<owl:Class rdf:ID= "PearFruit">
<rdfs:subClassOf rdf:resource 
="http://127.0.0.1:8000/ontology/SUMO.owl#FruitOrVegetable"/>
<rdfs:subClassOf rdf:resource ="http://127.0.0.1:8000/ontology/SUMO.owl#Food"/>
<rdfs:comment>A FruitOrVegetable that has a thick skin and the
shape of a tear drop.</rdfs:comment>
</owl:Class>

<owl:Class rdf:ID= "Peeling">
<rdfs:subClassOf rdf:resource 
="http://127.0.0.1:8000/ontology/SUMO.owl#Removing"/>
<rdfs:comment>Removing the Skin (or part of the Skin) from
an Organism.  Note that this class covers a large range of cases, including
peeling an orange, pelting an Animal, etc.</rdfs:comment>
</owl:Class>

<owl:Class rdf:ID= "Pencil">
<rdfs:subClassOf rdf:resource ="#WritingDevice"/>
<rdfs:comment>A WritingDevice that consists of an encased piece of
graphite.</rdfs:comment>
</owl:Class>

<owl:Class rdf:ID= "Peninsula">
<rdfs:subClassOf rdf:resource ="#LandForm"/>
<rdfs:comment>Peninsula is a subclass of LandForm consisting
of pieces of land that extend into a BodyOfWater and are surrounded on
three sides by water.  Typically Peninsulas are connected to the mainland
by an Isthmus or neck of land that is narrower than the main portion of
the peninsula (in contrast to Capes).</rdfs:comment>
</owl:Class>

<owl:Class rdf:ID= "PensionPlan">
<rdfs:subClassOf rdf:resource ="#FinancialAccount"/>
<rdfs:comment>A qualified retirement plan set up by a
corporation, labor union, government, or other organization for its
employees.  Examples include profit-sharing plans, stock bonus and
employee stock ownership plans, thrift plans, target benefit plans,
money purchase plans, and defined benefit plans.</rdfs:comment>
</owl:Class>

<owl:Class rdf:ID= "PercussionInstrument">
<rdfs:subClassOf rdf:resource 
="http://127.0.0.1:8000/ontology/SUMO.owl#MusicalInstrument"/>
<rdfs:comment>A MusicalInstrument which does not
have strings and which is played by striking it.</rdfs:comment>
</owl:Class>

<owl:Class rdf:ID= "Performance">
<rdfs:subClassOf rdf:resource 
="http://127.0.0.1:8000/ontology/SUMO.owl#Demonstrating"/>
<rdfs:comment>A Demonstrating which which is intended to entertain
the audience, e.g. DramaticActing and/or Music.</rdfs:comment>
</owl:Class>

<owl:Class rdf:ID= "PerformanceAct">
<rdfs:subClassOf rdf:resource ="#Performance"/>
<rdfs:comment>A discrete subProcess of a Performance,
e.g. an act of a play, a movement of a performance of a symphony, 
etc.</rdfs:comment>
</owl:Class>

<owl:Class rdf:ID= "PerformanceProgram">
<rdfs:subClassOf rdf:resource 
="http://127.0.0.1:8000/ontology/SUMO.owl#FactualText"/>
<rdfs:comment>A Text that describes the events
and/or participants in a Performance.</rdfs:comment>
</owl:Class>

<owl:Class rdf:ID= "PerformanceStage">
<rdfs:subClassOf rdf:resource 
="http://127.0.0.1:8000/ontology/SUMO.owl#StationaryArtifact"/>
<rdfs:comment>A large platform for theatrical plays,
lectures, dances, music recitals, etc, which can be observed by an 
audience.</rdfs:comment>
</owl:Class>

<owl:Class rdf:ID= "PerformanceStageWing">
<rdfs:subClassOf rdf:resource 
="http://127.0.0.1:8000/ontology/SUMO.owl#StationaryArtifact"/>
<rdfs:comment>A part of the PerformanceStage that is not
visible to members of the audience.</rdfs:comment>
</owl:Class>

<owl:Class rdf:ID= "PeriodicalPublisher">
<rdfs:subClassOf rdf:resource ="#Publisher"/>
<rdfs:comment>Any Publisher that publishes
Periodicals, e.g. newspaper and magazine publishing houses.</rdfs:comment>
</owl:Class>

<owl:Class rdf:ID= "Petroleum">
<rdfs:subClassOf rdf:resource ="#PetroleumProduct"/>
<rdfs:comment>Also known as crude oil.  It can be converted into
RefinedPetroleumProducts.</rdfs:comment>
</owl:Class>

<owl:Class rdf:ID= "PetroleumLubricant">
<rdfs:subClassOf rdf:resource ="#RefinedPetroleumProduct"/>
<rdfs:comment>PetroleumLubricant is the subclass of
RefinedPetroleumProducts that are lubricants.</rdfs:comment>
</owl:Class>

<owl:Class rdf:ID= "PetroleumProduct">
<rdfs:subClassOf rdf:resource ="#OrganicCompound"/>
<rdfs:comment>PetroleumProduct is a broad class that
includes both crude oil (Petroleum) and 
RefinedPetroleumProducts.</rdfs:comment>
</owl:Class>

<owl:Class rdf:ID= "Pharmacist">
<rdfs:subClassOf rdf:resource ="#Profession"/>
<rdfs:comment>The Profession of being a pharmacist, i.e.
preparing and dispensing BiologicallyActiveSubstances.</rdfs:comment>
</owl:Class>

<owl:Class rdf:ID= "Photograph">
<rdfs:subClassOf rdf:resource ="http://127.0.0.1:8000/ontology/SUMO.owl#Icon"/>
<rdfs:comment>An Icon that is the result of a process of
Photographing.</rdfs:comment>
</owl:Class>

<owl:Class rdf:ID= "PhotographicFilm">
<rdfs:subClassOf rdf:resource 
="http://127.0.0.1:8000/ontology/SUMO.owl#Artifact"/>
<rdfs:comment>Celluloid covered with an emulsion which can
be converted into photographic negatives by a Camera.</rdfs:comment>
</owl:Class>

<owl:Class rdf:ID= "Photographing">
<rdfs:subClassOf rdf:resource 
="http://127.0.0.1:8000/ontology/SUMO.owl#ContentDevelopment"/>
<rdfs:comment>ContentDevelopment where the instrument
is a camera and the result is a Photograph.</rdfs:comment>
</owl:Class>

<owl:Class rdf:ID= "Piano">
<rdfs:subClassOf rdf:resource ="#StringInstrument"/>
<rdfs:comment>A StringInstrument which is played with keys that
activate hammers that strike strings.</rdfs:comment>
</owl:Class>

<owl:Class rdf:ID= "PictureFrame">
<rdfs:subClassOf rdf:resource 
="http://127.0.0.1:8000/ontology/SUMO.owl#Artifact"/>
<rdfs:comment>A frame which surrounds a PaintedPicture or
Photograph and has the function of protecting and accenting the 
picture.</rdfs:comment>
</owl:Class>

<owl:Class rdf:ID= "PidginLanguage">
<rdfs:subClassOf rdf:resource 
="http://127.0.0.1:8000/ontology/SUMO.owl#SpokenHumanLanguage"/>
<rdfs:comment>A PidginLanguage is not the native language
of anyone but is used as an auxiliary or supplemental language between two
mutually unintelligible speech communities. Pidgins are reduced languages,
characterized by having a limited vocabulary and a simple grammar which 
serve
to satisfy basic communication needs. Historically these languages have
primarily arisen in trade centers and plantations (with slaves from 
different
language backgrounds), areas where large groups of people lacking a common
language need to communicate. By definition, a pidgin has no native 
speakers;
it is always a person's second (or more) language.</rdfs:comment>
</owl:Class>

<owl:Class rdf:ID= "Pig">
<rdfs:subClassOf rdf:resource 
="http://127.0.0.1:8000/ontology/SUMO.owl#HoofedMammal"/>
<rdfs:subClassOf rdf:resource ="#DomesticAnimal"/>
<rdfs:comment>A domesticated HoofedMammal that is raised for 
pork.</rdfs:comment>
</owl:Class>

<owl:Class rdf:ID= "Pigeon">
<rdfs:subClassOf rdf:resource ="http://127.0.0.1:8000/ontology/SUMO.owl#Bird"/>
<rdfs:comment>A subclass of Bird with a stout body and short 
legs.</rdfs:comment>
</owl:Class>

<owl:Class rdf:ID= "Pillow">
<rdfs:subClassOf rdf:resource 
="http://127.0.0.1:8000/ontology/SUMO.owl#Artifact"/>
<rdfs:comment>A soft, stuffed Artifact to support the Head or
the body as a whole while one is sleeping or relaxing.</rdfs:comment>
</owl:Class>

<owl:Class rdf:ID= "Pipeline">
<rdfs:subClassOf rdf:resource 
="http://127.0.0.1:8000/ontology/SUMO.owl#Transitway"/>
<rdfs:comment>Pipeline is the class of pipelines used
to transport various kinds of fluids.</rdfs:comment>
</owl:Class>

<owl:Class rdf:ID= "Pistol">
<rdfs:subClassOf rdf:resource ="#Firearm"/>
<rdfs:comment>A Firearm that is intended to be aimed and fired with a
single hand.</rdfs:comment>
</owl:Class>

<owl:Class rdf:ID= "PitchersMound">
<rdfs:subClassOf rdf:resource ="#GameArtifact"/>
<rdfs:comment>The place where the pitcher in Baseball
stands when he is throwing balls to the batter.</rdfs:comment>
</owl:Class>

<owl:Class rdf:ID= "Pitching">
<rdfs:subClassOf rdf:resource ="#Throwing"/>
<rdfs:comment>Throwing a Ball.</rdfs:comment>
</owl:Class>

<owl:Class rdf:ID= "PituitaryGland">
<rdfs:subClassOf rdf:resource ="#Gland"/>
<rdfs:comment>The main Gland of the endocrine system.</rdfs:comment>
</owl:Class>

<owl:Class rdf:ID= "PlaceOfCommerce">
<rdfs:subClassOf rdf:resource 
="http://127.0.0.1:8000/ontology/SUMO.owl#StationaryArtifact"/>
<rdfs:comment>A Building or part of a Building which is
intended for organizational activities, e.g. retail or wholesale selling,
manufacturing, office work, etc.</rdfs:comment>
</owl:Class>

<owl:Class rdf:ID= "Planet">
<rdfs:subClassOf rdf:resource ="#NaturalSatellite"/>
<rdfs:comment>Planet is the class of large NaturalSatellites
that revolve around a star.</rdfs:comment>
</owl:Class>

<owl:Class rdf:ID= "PlaningHullWatercraft">
<rdfs:subClassOf rdf:resource ="#Watercraft"/>
<rdfs:comment>PlaningHullWatercraft is a subclass
of Watercraft with hulls designed for a position partially on or above
the water surface when they are in motion, in order to reduce drag.  See
also DisplacementHullWatercraft.</rdfs:comment>
</owl:Class>

<owl:Class rdf:ID= "PlantBranch">
<rdfs:subClassOf rdf:resource 
="http://127.0.0.1:8000/ontology/SUMO.owl#PlantAnatomicalStructure"/>
<rdfs:subClassOf rdf:resource 
="http://127.0.0.1:8000/ontology/SUMO.owl#BodyPart"/>
<rdfs:comment>The stem of a Plant or any shoot arising from
the stem of a Plant.</rdfs:comment>
</owl:Class>

<owl:Class rdf:ID= "PlantLeaf">
<rdfs:subClassOf rdf:resource 
="http://127.0.0.1:8000/ontology/SUMO.owl#PlantAnatomicalStructure"/>
<rdfs:subClassOf rdf:resource ="http://127.0.0.1:8000/ontology/SUMO.owl#Organ"/>
<rdfs:comment>An Organ of Plants whose main purpose is
photosynthesis.</rdfs:comment>
</owl:Class>

<owl:Class rdf:ID= "PlantRoot">
<rdfs:subClassOf rdf:resource 
="http://127.0.0.1:8000/ontology/SUMO.owl#PlantAnatomicalStructure"/>
<rdfs:subClassOf rdf:resource ="http://127.0.0.1:8000/ontology/SUMO.owl#Organ"/>
<rdfs:comment>An Organ of Plants whose main purpose is
twofold, viz. to absorb nutrients from the ground and to anchor the Plant
in place.</rdfs:comment>
</owl:Class>

<owl:Class rdf:ID= "Planting">
<rdfs:subClassOf rdf:resource 
="http://127.0.0.1:8000/ontology/SUMO.owl#Putting"/>
<rdfs:comment>Planting is the class of processes in
which Plants are planted or transplanted, whether as seeds, seedlings,
or mature plants.</rdfs:comment>
</owl:Class>

<owl:Class rdf:ID= "Platinum">
<rdfs:subClassOf rdf:resource 
="http://127.0.0.1:8000/ontology/SUMO.owl#ElementalSubstance"/>
<atomicNumber>78</atomicNumber>
<rdfs:comment>Attractive greyish-white metal.  When pure, it is
malleable and ductile.  Does not oxidize in air, insoluble in hydrochloric
and nitric acid.  Corroded by halogens, cyandies, sulphur and alkalis.
{Hydrogen} and {oxygen} react explosively in the presence of platinum.
There are six stable isotopes and three radioisotopes, the most stable
being Pt-193 with a half-life of 60 years.  Platinum is used in jewelry,
laboratory equipment, electrical contacts, dentistry, and anti-pollution
devices in cars.  PtCl2(NH3)2 is used to treat some forms of cancer.
Platinum-{cobalt} alloys have magnetic properties.  It is also used in the
definition of the Standard Hydrogen Electrode.  Discovered by Antonio de
Ulloa in South America in 1735.  The name comes from the Spanish word
platina which means silver.  Platinum metal is generally not a health
concern due to its unreactivity, however platinum compounds should be
considered highly toxic.</rdfs:comment>
</owl:Class>

<owl:Class rdf:ID= "PlayingCard">
<rdfs:subClassOf rdf:resource ="#GameArtifact"/>
<rdfs:subClassOf rdf:resource 
="http://127.0.0.1:8000/ontology/SUMO.owl#ContentBearingObject"/>
<rdfs:comment>A small piece of stiff paper with markings
which is intended to be used for playing card games.</rdfs:comment>
</owl:Class>

<owl:Class rdf:ID= "Pleading">
<rdfs:subClassOf rdf:resource 
="http://127.0.0.1:8000/ontology/SUMO.owl#Stating"/>
<rdfs:comment>Stating in a court of law a claim about whether or
not one is guilty of the crime of which one has been accused.</rdfs:comment>
</owl:Class>

<owl:Class rdf:ID= "Plug">
<rdfs:subClassOf rdf:resource 
="http://127.0.0.1:8000/ontology/SUMO.owl#Artifact"/>
<rdfs:comment>An Artifact which is designed to fit snugly within
a Hole.</rdfs:comment>
</owl:Class>

<owl:Class rdf:ID= "Plumber">
<rdfs:subClassOf rdf:resource ="#OccupationalTrade"/>
<rdfs:comment>Any occupation that involves installing, repairing, and
replacing pipes and pipe fixtures.</rdfs:comment>
</owl:Class>

<owl:Class rdf:ID= "Pocket">
<rdfs:subClassOf rdf:resource ="#FabricArtifact"/>
<rdfs:comment>A pouch of Fabric in an instance of Clothing where
something can be kept.</rdfs:comment>
</owl:Class>

<owl:Class rdf:ID= "Poisoning">
<rdfs:subClassOf rdf:resource 
="http://127.0.0.1:8000/ontology/SUMO.owl#Injuring"/>
<rdfs:comment>A Poisoning is caused by an external
substance.  Since Poisoning is not possible without some biologic
function which affects the Organism being injured, it is a subclass
of BiologicalProcess.</rdfs:comment>
</owl:Class>

<owl:Class rdf:ID= "PolarClimateZone">
<rdfs:subClassOf rdf:resource ="#ClimateZone"/>
<rdfs:comment>PolarClimateZone is a subclass of
ClimateZone characterized by having an average temperature less than
10 degrees Celsius in the warmest month.  This is Koeppen climate system
Type E.  No agriculture is supported in polar climates.</rdfs:comment>
</owl:Class>

<owl:Class rdf:ID= "PolarTypeFClimateZone">
<rdfs:subClassOf rdf:resource ="#PolarClimateZone"/>
<rdfs:comment>PolarTypeFClimateZone is a
subclass of PolarClimateZone characterized by having no month in
which the temperature rises to 10 degrees Celsius or above.</rdfs:comment>
</owl:Class>

<owl:Class rdf:ID= "PoliceCaptain">
<rdfs:subClassOf rdf:resource ="#PoliceOfficer"/>
<rdfs:comment>A PoliceOfficer who is in charge of a precinct.</rdfs:comment>
</owl:Class>

<owl:Class rdf:ID= "PoliceDetective">
<rdfs:subClassOf rdf:resource ="#PoliceOfficer"/>
<rdfs:comment>The Profession of being a police
detective, i.e. being a PoliceOfficer whose duties include the
investigation of crimes.</rdfs:comment>
</owl:Class>

<owl:Class rdf:ID= "PoliceOfficer">
<rdfs:subClassOf rdf:resource ="#GovernmentOfficer"/>
<rdfs:comment>The Profession of being a police officer, i.e.
working for a law enforcement agency that is part of a 
Government.</rdfs:comment>
</owl:Class>

<owl:Class rdf:ID= "PoliceSergeant">
<rdfs:subClassOf rdf:resource ="#PoliceOfficer"/>
<rdfs:comment>A PoliceOfficer with the rank of sergeant.</rdfs:comment>
</owl:Class>

<owl:Class rdf:ID= "PoliticalCrime">
<rdfs:subClassOf rdf:resource ="#CriminalAction"/>
<rdfs:subClassOf rdf:resource 
="http://127.0.0.1:8000/ontology/SUMO.owl#PoliticalProcess"/>
<rdfs:comment>A CriminalAction that is committed by or
against Governments.</rdfs:comment>
</owl:Class>

<owl:Class rdf:ID= "PoliticalParty">
<rdfs:subClassOf rdf:resource 
="http://127.0.0.1:8000/ontology/SUMO.owl#PoliticalOrganization"/>
<rdfs:comment>PoliticalParty is the class of
PoliticalOrganizations that may sponsor candidates for 
Elections.</rdfs:comment>
</owl:Class>

<owl:Class rdf:ID= "PoliticalRevolution">
<rdfs:subClassOf rdf:resource 
="http://127.0.0.1:8000/ontology/SUMO.owl#PoliticalProcess"/>
<rdfs:subClassOf rdf:resource 
="http://127.0.0.1:8000/ontology/SUMO.owl#ViolentContest"/>
<rdfs:comment>The violent overthrow of one Government
and its replacement by another.  This covers grass-roots revolutions, as 
well
as coups d'etat.</rdfs:comment>
</owl:Class>

<owl:Class rdf:ID= "PoliticoEconomicAttribute">
<rdfs:subClassOf rdf:resource 
="http://127.0.0.1:8000/ontology/SUMO.owl#RelationalAttribute"/>
<rdfs:comment>Any Attribute of a Government
which specifies some aspect of the political or economic system of the
Government.</rdfs:comment>
</owl:Class>

<owl:Class rdf:ID= "Polling">
<rdfs:subClassOf rdf:resource 
="http://127.0.0.1:8000/ontology/SUMO.owl#Investigating"/>
<rdfs:comment>Investigating what people believe (and in what proportions)
by asking a set of structured questions to a random sample of 
people.</rdfs:comment>
</owl:Class>

<owl:Class rdf:ID= "Polygon">
<rdfs:subClassOf rdf:resource 
="http://127.0.0.1:8000/ontology/SUMO.owl#ClosedTwoDimensionalFigure"/>
<rdfs:comment>A ClosedTwoDimensionalFigure that is composed
exclusively of straight lines, i.e. OneDimensionalFigures.</rdfs:comment>
</owl:Class>

<owl:Class rdf:ID= "PolyphonicMusic">
<rdfs:subClassOf rdf:resource ="http://127.0.0.1:8000/ontology/SUMO.owl#Music"/>
<rdfs:comment>Music which has two or more parts, i.e. Music
which can be divided into two or more contemporaneous subProcesses which are
also instances of Music.</rdfs:comment>
</owl:Class>

<owl:Class rdf:ID= "PopularElection">
<rdfs:subClassOf rdf:resource ="#GeneralElection"/>
<rdfs:comment>PopularElection is the class of
Elections in which office-holders and issues are determined directly by
the outcome of the votes cast by the enfranchised.  For example, U.S.
Senators and Representatives are elected by PopularElection.  By
contrast, U.S. Presidents are elected by indirect elections, in which the
Electoral College determines the actual outcome.  See 
electionWinner.</rdfs:comment>
</owl:Class>

<owl:Class rdf:ID= "Porch">
<rdfs:subClassOf rdf:resource 
="http://127.0.0.1:8000/ontology/SUMO.owl#StationaryArtifact"/>
<rdfs:comment>A StationaryArtifact which is connected to a
Building and which provides some shelter in entering or leaving the
Building or in sitting outside.</rdfs:comment>
</owl:Class>

<owl:Class rdf:ID= "Pork">
<rdfs:subClassOf rdf:resource ="http://127.0.0.1:8000/ontology/SUMO.owl#Meat"/>
<rdfs:comment>Meat that was originally part of a Pig.</rdfs:comment>
</owl:Class>

<owl:Class rdf:ID= "PortFacility">
<rdfs:subClassOf rdf:resource 
="http://127.0.0.1:8000/ontology/SUMO.owl#GeopoliticalArea"/>
<rdfs:comment>PortFacility is the class of port
complexes, including piers and docking space, moorings, cargo-handling
and other support facilities for marine traffic.  Ships are loaded and
unloaded at a PortFacility.</rdfs:comment>
</owl:Class>

<owl:Class rdf:ID= "Portrait">
<rdfs:subClassOf rdf:resource ="#PaintedPicture"/>
<rdfs:comment>A PaintedPicture that represents someone's 
Face.</rdfs:comment>
</owl:Class>

<owl:Class rdf:ID= "PostMeridiem">
<rdfs:subClassOf rdf:resource 
="http://127.0.0.1:8000/ontology/SUMO.owl#TimeInterval"/>
<rdfs:comment>The class of TimeIntervals that begin at noon and
end at midnight.</rdfs:comment>
</owl:Class>

<owl:Class rdf:ID= "PostSecondarySchool">
<rdfs:subClassOf rdf:resource ="#School"/>
<rdfs:comment>The class of Schools that offer
an associate's degree, a bachelor's degree or a graduate 
degree.</rdfs:comment>
</owl:Class>

<owl:Class rdf:ID= "PotOrPan">
<rdfs:subClassOf rdf:resource ="#Container"/>
<rdfs:comment>A Container which has a handle and is used for
Cooking.</rdfs:comment>
</owl:Class>

<owl:Class rdf:ID= "Potassium">
<rdfs:subClassOf rdf:resource 
="http://127.0.0.1:8000/ontology/SUMO.owl#ElementalSubstance"/>
<atomicNumber>19</atomicNumber>
<rdfs:comment>Soft silvery metallic element belonging to group
1 of the periodic table (alkali metals).  Occurs naturally in seawater and
a many minerals.  Highly reactive, chemically, it resembles sodium in its
behavior and compounds.  Discovered by Sir Humphry Davy in 
1807.</rdfs:comment>
</owl:Class>

<owl:Class rdf:ID= "Potter">
<rdfs:subClassOf rdf:resource ="#OccupationalTrade"/>
<rdfs:comment>Any occupation that involves the creation of 
Pottery.</rdfs:comment>
</owl:Class>

<owl:Class rdf:ID= "Pottery">
<rdfs:subClassOf rdf:resource 
="http://127.0.0.1:8000/ontology/SUMO.owl#Artifact"/>
<rdfs:comment>Household Artifacts that are made out of baked 
Clay.</rdfs:comment>
</owl:Class>

<owl:Class rdf:ID= "PoundForce">
<rdfs:subClassOf rdf:resource 
="http://127.0.0.1:8000/ontology/SUMO.owl#FunctionQuantity"/>
<rdf:type rdf:resource = 
"http://127.0.0.1:8000/ontology/SUMO.owl#UnitOfMeasure"/>
<rdfs:comment>English pound of force. The conversion
factor depends on the local value of the acceleration of free fall. A
mean value is used in the conversion axiom associated with this
constant.</rdfs:comment>
</owl:Class>

<owl:Class rdf:ID= "Pouring">
<rdfs:subClassOf rdf:resource 
="http://127.0.0.1:8000/ontology/SUMO.owl#LiquidMotion"/>
<rdfs:subClassOf rdf:resource 
="http://127.0.0.1:8000/ontology/SUMO.owl#Transfer"/>
<rdfs:comment>Any instance of Transfer from one Container to
another, where the thing transferred is a Liquid.</rdfs:comment>
</owl:Class>

<owl:Class rdf:ID= "Powder">
<rdfs:subClassOf rdf:resource 
="http://127.0.0.1:8000/ontology/SUMO.owl#Substance"/>
<rdfs:comment>Any Solid Substance which consists of loose,
identical, and very small particles.</rdfs:comment>
</owl:Class>

<owl:Class rdf:ID= "Praying">
<rdfs:subClassOf rdf:resource 
="http://127.0.0.1:8000/ontology/SUMO.owl#ReligiousProcess"/>
<rdfs:subClassOf rdf:resource 
="http://127.0.0.1:8000/ontology/SUMO.owl#Requesting"/>
<rdfs:comment>A formal or informal process of private worship which
may or may not be carried out in a ReligiousBuilding.</rdfs:comment>
</owl:Class>

<owl:Class rdf:ID= "PreparedFood">
<rdfs:subClassOf rdf:resource ="http://127.0.0.1:8000/ontology/SUMO.owl#Food"/>
<rdfs:comment>Food that is the result of Cooking.</rdfs:comment>
</owl:Class>

<owl:Class rdf:ID= "PressureMeasuringDevice">
<rdfs:subClassOf rdf:resource 
="http://127.0.0.1:8000/ontology/SUMO.owl#MeasuringDevice"/>
<rdfs:comment>Any Device that measures and
represents AtmosphericPressureMeasure.</rdfs:comment>
</owl:Class>

<owl:Class rdf:ID= "Prison">
<rdfs:subClassOf rdf:resource 
="http://127.0.0.1:8000/ontology/SUMO.owl#StationaryArtifact"/>
<rdfs:comment>An installation which is owned and maintained by
a Government for the purpose of Confining people.  This class covers
jails, federal prisons, concentration camps, gulags, etc.</rdfs:comment>
</owl:Class>

<owl:Class rdf:ID= "PrivateDetective">
<rdfs:subClassOf rdf:resource ="#Profession"/>
<sumo:disjoint rdf:resource = "#PoliceDetective" />
<rdfs:comment>The Profession of being a private detective,
i.e. a detective who can be hired for a fee to investigate 
something.</rdfs:comment>
</owl:Class>

<owl:Class rdf:ID= "PrivateSchool">
<rdfs:subClassOf rdf:resource ="#School"/>
<sumo:disjoint rdf:resource = 
"http://127.0.0.1:8000/ontology/SUMO.owl#GovernmentOrganization" />
<rdfs:comment>A School which is not publicly owned.</rdfs:comment>
</owl:Class>

<owl:Class rdf:ID= "ProcessingACheck">
<rdfs:subClassOf rdf:resource ="#AuthorizationOfTransaction"/>
<rdfs:comment>An activity of paying the amount specified on the
check from funds on deposit.</rdfs:comment>
</owl:Class>

<owl:Class rdf:ID= "Proclaiming">
<rdfs:subClassOf rdf:resource ="#Lecture"/>
<rdfs:subClassOf rdf:resource 
="http://127.0.0.1:8000/ontology/SUMO.owl#Declaring"/>
<rdfs:comment>Any instance of Speaking before an assembled
audience that effects an institutional change, e.g. a change in the laws of
the government.</rdfs:comment>
</owl:Class>

<owl:Class rdf:ID= "Profession">
<rdfs:subClassOf rdf:resource ="#SkilledOccupation"/>
<sumo:disjoint rdf:resource = "#OccupationalTrade" />
<rdfs:comment>Any occupation that requires at least a bachelor's
degree.</rdfs:comment>
</owl:Class>

<owl:Class rdf:ID= "Professor">
<rdfs:subClassOf rdf:resource ="#Teacher"/>
<rdfs:comment>The Profession of being a teacher at a
PostSecondarySchool.</rdfs:comment>
</owl:Class>

<owl:Class rdf:ID= "ProfitSharingPlan">
<rdfs:subClassOf rdf:resource ="#PensionPlan"/>
<rdfs:comment>An arrangement in which an employer
shares its profits with its employees.  The compensation can be stocks,
bonds or cash, and can be immediate or deferred until 
retirement.</rdfs:comment>
</owl:Class>

<owl:Class rdf:ID= "Projectile">
<rdfs:subClassOf rdf:resource ="http://127.0.0.1:8000/ontology/SUMO.owl#Weapon"/>
<rdfs:comment>A missile, bullet, etc. that is fired from
a Weapon.</rdfs:comment>
</owl:Class>

<owl:Class rdf:ID= "ProjectileLauncher">
<rdfs:subClassOf rdf:resource ="http://127.0.0.1:8000/ontology/SUMO.owl#Weapon"/>
<rdfs:comment>A Weapon that shoots a Projectile.</rdfs:comment>
</owl:Class>

<owl:Class rdf:ID= "ProjectileShell">
<rdfs:subClassOf rdf:resource ="#Container"/>
<rdfs:comment>The case or cartridge of a Projectile.</rdfs:comment>
</owl:Class>

<owl:Class rdf:ID= "ProjectionScreen">
<rdfs:subClassOf rdf:resource ="#CommunicationDevice"/>
<rdfs:comment>A CommunicationDevice upon which images
are projected so that they can be viewed.</rdfs:comment>
</owl:Class>

<owl:Class rdf:ID= "Proprietorship">
<rdfs:subClassOf rdf:resource 
="http://127.0.0.1:8000/ontology/SUMO.owl#CommercialAgent"/>
<rdfs:comment>A CommercialAgent that is owned by a
single person.</rdfs:comment>
</owl:Class>

<owl:Class rdf:ID= "Protozoa">
<rdfs:subClassOf rdf:resource 
="http://127.0.0.1:8000/ontology/SUMO.owl#Microorganism"/>
<rdfs:comment>Unicellular Organisms that are capable of movement
and that are found in almost every part of the world.  This class includes
amoebas, sporozoans, and paramecia.</rdfs:comment>
</owl:Class>

<owl:Class rdf:ID= "PseudoGraph">
<rdfs:subClassOf rdf:resource ="#Graph"/>
<rdfs:comment>The Class of pseudographs.  A pseudograph
is a Graph containing at least one GraphLoop.</rdfs:comment>
</owl:Class>

<owl:Class rdf:ID= "Psychosis">
<rdfs:comment>Any PsychologicalDysfunction which is the
result of an organic impairment of the NervousSystem.</rdfs:comment>
</owl:Class>

<owl:Class rdf:ID= "PublicDefender">
<rdfs:subClassOf rdf:resource ="#Attorney"/>
<rdfs:subClassOf rdf:resource ="#GovernmentOfficer"/>
<rdfs:comment>An Attorney who defends criminal cases for a
GovernmentOrganization.</rdfs:comment>
</owl:Class>

<owl:Class rdf:ID= "PublicLibrary">
<rdfs:subClassOf rdf:resource ="#Library"/>
<rdfs:subClassOf rdf:resource 
="http://127.0.0.1:8000/ontology/SUMO.owl#GovernmentOrganization"/>
<rdfs:comment>A Library which is financed by taxes and which
is open to everyone.</rdfs:comment>
</owl:Class>

<owl:Class rdf:ID= "PublicPark">
<rdfs:subClassOf rdf:resource ="#Park"/>
<rdfs:comment>A Park that is publicly owned, i.e. owned
by a Government.</rdfs:comment>
</owl:Class>

<owl:Class rdf:ID= "PublicProsecutor">
<rdfs:subClassOf rdf:resource ="#Attorney"/>
<rdfs:subClassOf rdf:resource ="#GovernmentOfficer"/>
<rdfs:comment>An Attorney who prosecutes criminal cases for
a GovernmentOrganization.</rdfs:comment>
</owl:Class>

<owl:Class rdf:ID= "PublicSchool">
<rdfs:subClassOf rdf:resource ="#School"/>
<rdfs:subClassOf rdf:resource 
="http://127.0.0.1:8000/ontology/SUMO.owl#GovernmentOrganization"/>
<rdfs:comment>A School which is financed primarily by taxes.</rdfs:comment>
</owl:Class>

<owl:Class rdf:ID= "Publisher">
<rdfs:subClassOf rdf:resource 
="http://127.0.0.1:8000/ontology/SUMO.owl#CommercialAgent"/>
<rdfs:comment>Any business whose services include the
Publication of Texts.</rdfs:comment>
</owl:Class>

<owl:Class rdf:ID= "Pulling">
<rdfs:subClassOf rdf:resource ="#LandTransportation"/>
<rdfs:comment>Any instance of LandTransportation, where a
TransportationDevice is dragged by something else, whether the something
else is an Animal or a self-powered TransportationDevice.</rdfs:comment>
</owl:Class>

<owl:Class rdf:ID= "PulmonaryArtery">
<rdfs:subClassOf rdf:resource ="#Artery"/>
<rdfs:comment>An Artery that carries Blood from
the Heart to the Lungs.</rdfs:comment>
</owl:Class>

<owl:Class rdf:ID= "PulmonaryVein">
<rdfs:subClassOf rdf:resource ="#Vein"/>
<rdfs:comment>A Vein that carries Blood from the
Lungs to the Heart.</rdfs:comment>
</owl:Class>

<owl:Class rdf:ID= "Pump">
<rdfs:subClassOf rdf:resource 
="http://127.0.0.1:8000/ontology/SUMO.owl#TransportationDevice"/>
<rdfs:comment>A Device that moves Fluids by means of pressure or 
suction.</rdfs:comment>
</owl:Class>

<owl:Class rdf:ID= "Punching">
<rdfs:subClassOf rdf:resource 
="http://127.0.0.1:8000/ontology/SUMO.owl#Impelling"/>
<rdfs:comment>Any instance of Impelling where the instrument
is a Fist of the agent.</rdfs:comment>
</owl:Class>

<owl:Class rdf:ID= "Punishing">
<rdfs:subClassOf rdf:resource 
="http://127.0.0.1:8000/ontology/SUMO.owl#RegulatoryProcess"/>
<rdfs:comment>A RegulatoryProcess where the agent does
something to the destination that the agent knows is undesirable
for the destination.</rdfs:comment>
</owl:Class>

<owl:Class rdf:ID= "PuttingOnClothing">
<rdfs:subClassOf rdf:resource 
="http://127.0.0.1:8000/ontology/SUMO.owl#Covering"/>
<rdfs:comment>Putting Clothing on a Human or
Animal in such a way that the Human or Animal wears the 
Clothing.</rdfs:comment>
</owl:Class>

<owl:Class rdf:ID= "Quadrilateral">
<rdfs:subClassOf rdf:resource ="#Polygon"/>
<rdfs:comment>Any four-sided Polygon.</rdfs:comment>
</owl:Class>

<owl:Class rdf:ID= "QueenInsect">
<rdfs:subClassOf rdf:resource ="http://127.0.0.1:8000/ontology/SUMO.owl#Insect"/>
<sumo:disjoint rdf:resource = "#WorkerInsect" />
<rdfs:comment>A Female Insect which is the sole member of
her colony with the capability to reproduce.</rdfs:comment>
</owl:Class>

<owl:Class rdf:ID= "Question">
<rdfs:subClassOf rdf:resource 
="http://127.0.0.1:8000/ontology/SUMO.owl#Sentence"/>
<rdfs:comment>An interrogative Sentence, a Sentence that
poses a question.</rdfs:comment>
</owl:Class>

<owl:Class rdf:ID= "Rabbit">
<rdfs:subClassOf rdf:resource ="http://127.0.0.1:8000/ontology/SUMO.owl#Rodent"/>
<rdfs:comment>A burrowing Rodent with a short tail and long 
ears.</rdfs:comment>
</owl:Class>

<owl:Class rdf:ID= "RacialEthnicGroup">
<rdfs:subClassOf rdf:resource 
="http://127.0.0.1:8000/ontology/SUMO.owl#EthnicGroup"/>
<rdfs:comment>A RacialEthnicGroup is an
EthnicGroup based on common racial background.</rdfs:comment>
</owl:Class>

<owl:Class rdf:ID= "Racing">
<rdfs:subClassOf rdf:resource ="http://127.0.0.1:8000/ontology/SUMO.owl#Sport"/>
<rdfs:comment>A sport which involves a contest of speed between the
participants.  Note that this covers a variety of things, including auto
racing, running competitions, etc.</rdfs:comment>
</owl:Class>

<owl:Class rdf:ID= "RadarOrSonar">
<rdfs:subClassOf rdf:resource ="#ElectricDevice"/>
<rdfs:comment>An ElectricDevice that emits and receives
microwave radiation for the purpose of locating and tracking distant 
objects.</rdfs:comment>
</owl:Class>

<owl:Class rdf:ID= "RadiatingInfrared">
<rdfs:subClassOf rdf:resource 
="http://127.0.0.1:8000/ontology/SUMO.owl#Radiating"/>
<sumo:disjoint rdf:resource = 
"http://127.0.0.1:8000/ontology/SUMO.owl#RadiatingLight" />
<sumo:disjoint rdf:resource = "#RadioEmission" />
<rdfs:comment>Any instance of Radiating where the
wavelengths are longer than those of visible light and shorter than those
of radio emissions.</rdfs:comment>
</owl:Class>

<owl:Class rdf:ID= "RadiatingSoundUltrasonic">
<rdfs:subClassOf rdf:resource 
="http://127.0.0.1:8000/ontology/SUMO.owl#RadiatingSound"/>
<rdfs:comment>All sound waves that have frequencies
above those that normal Human ears can detect.</rdfs:comment>
</owl:Class>

<owl:Class rdf:ID= "RadiatingUltraviolet">
<rdfs:subClassOf rdf:resource 
="http://127.0.0.1:8000/ontology/SUMO.owl#Radiating"/>
<sumo:disjoint rdf:resource = 
"http://127.0.0.1:8000/ontology/SUMO.owl#RadiatingLight" />
<sumo:disjoint rdf:resource = "#XRayRadiation" />
<rdfs:comment>Any instance of Radiating where the
wavelengths are shorter than those of visible light and longer than those
of X-Rays.</rdfs:comment>
</owl:Class>

<owl:Class rdf:ID= "RadiatingVisibleLight">
<rdfs:subClassOf rdf:resource 
="http://127.0.0.1:8000/ontology/SUMO.owl#RadiatingLight"/>
<sumo:disjoint rdf:resource = "#RadiatingUltraviolet" />
<rdfs:comment>Any instance of RadiatingLight that can
be detected by normal human visual perception.</rdfs:comment>
</owl:Class>

<owl:Class rdf:ID= "RadioBroadcasting">
<rdfs:subClassOf rdf:resource ="#Broadcasting"/>
<rdfs:comment>Any instance of Broadcasting which is
intended to be received by a Radio.</rdfs:comment>
</owl:Class>

<owl:Class rdf:ID= "RadioEmission">
<rdfs:subClassOf rdf:resource 
="http://127.0.0.1:8000/ontology/SUMO.owl#Radiating"/>
<rdfs:comment>Any instance of Radiating
where the waves have a wavelength between 5 milimeters and 30,000 
meters.</rdfs:comment>
</owl:Class>

<owl:Class rdf:ID= "RadioReceiver">
<rdfs:subClassOf rdf:resource ="#ReceiverDevice"/>
<rdfs:comment>A RadioReceiver is a Device for receiving
radio broadcast signals from a RadioStation.</rdfs:comment>
</owl:Class>

<owl:Class rdf:ID= "RadioStation">
<rdfs:subClassOf rdf:resource ="#BroadcastingStation"/>
<rdfs:comment>A RadioStation is a BroadcastingStation
that broadcasts programs that are intended to be received by 
Radios.</rdfs:comment>
</owl:Class>

<owl:Class rdf:ID= "RadioactiveWeapon">
<rdfs:subClassOf rdf:resource ="#WeaponOfMassDestruction"/>
<sumo:disjoint rdf:resource = "#BiochemicalWeapon" />
<rdfs:comment>A WeaponOfMassDestruction which
achieves its effect through radioactivity, either by an explosion resulting
from nuclear fission or by a conventional explosive device that scatters
radioactive debris.</rdfs:comment>
</owl:Class>

<owl:Class rdf:ID= "RadiologicalWeapon">
<rdfs:comment>Weapons which are designed to spread
radioactive particles over a large area by means of a conventional
explosive device rather than a nuclear reaction.  These weapons are often
referred to as 'dirty bombs'.</rdfs:comment>
<rdfs:subClassOf rdf:resource ="#RadioactiveWeapon"/>
</owl:Class>

<owl:Class rdf:ID= "Radish">
<rdfs:subClassOf rdf:resource ="#PlantRoot"/>
<rdfs:subClassOf rdf:resource ="http://127.0.0.1:8000/ontology/SUMO.owl#Food"/>
<rdfs:comment>A PlantRoot that is often used in salads.</rdfs:comment>
</owl:Class>

<owl:Class rdf:ID= "RailTransportationSystem">
<rdfs:subClassOf rdf:resource ="#TransportationSystem"/>
<rdfs:comment>RailTransportationSystem
is the subclass of TransportationSystems whose routes are 
Railways.</rdfs:comment>
</owl:Class>

<owl:Class rdf:ID= "Railcar">
<rdfs:subClassOf rdf:resource ="#RollingStock"/>
<sumo:disjoint rdf:resource = "#SelfPoweredVehicle" />
<rdfs:comment>Railcar is the subclass of RollingStock that
includes all non-locomotive, non-self-powered 
RailwayVehicles.</rdfs:comment>
</owl:Class>

<owl:Class rdf:ID= "RailroadCompany">
<rdfs:subClassOf rdf:resource ="#TransportationCompany"/>
<rdfs:comment>Any TransportationCompany whose services
include Transportation by Train.</rdfs:comment>
</owl:Class>

<owl:Class rdf:ID= "RailroadTrack">
<rdfs:subClassOf rdf:resource 
="http://127.0.0.1:8000/ontology/SUMO.owl#StationaryArtifact"/>
<rdfs:comment>RailroadTrack is the class of
StationaryArtifacts consisting of rails laid on supports to form
a track for railway vehicles.</rdfs:comment>
</owl:Class>

<owl:Class rdf:ID= "Railway">
<rdfs:subClassOf rdf:resource 
="http://127.0.0.1:8000/ontology/SUMO.owl#LandTransitway"/>
<rdfs:subClassOf rdf:resource 
="http://127.0.0.1:8000/ontology/SUMO.owl#StationaryArtifact"/>
<rdfs:comment>Railway is the subclass of
LandTransitways that have rails along which Trains may travel.
A railway consists of the rail bed, sleepers, tracks, electric
rails, switches, sensors, lights, crossing grades, and any other
integral machinery or parts of a section of railway.</rdfs:comment>
</owl:Class>

<owl:Class rdf:ID= "RailwayTerminal">
<rdfs:subClassOf rdf:resource ="#TransitTerminal"/>
<rdfs:comment>RailwayTerminal is the subclass of
TransitTerminals designed for Trains.  A RailwayTerminal includes
all the RailroadTrack and any outbuildings or other related structure
in the terminal, as well as the TrainStation (if there is 
one).</rdfs:comment>
</owl:Class>

<owl:Class rdf:ID= "RailwayVehicle">
<rdfs:subClassOf rdf:resource ="#LandVehicle"/>
<rdfs:comment>RailwayVehicle is the subclass of
Vehicles that are designed to run on Railways, including both Trains
and individual cars (RollingStock).</rdfs:comment>
</owl:Class>

<owl:Class rdf:ID= "Raining">
<rdfs:subClassOf rdf:resource 
="http://127.0.0.1:8000/ontology/SUMO.owl#Precipitation"/>
<rdfs:comment>Raining is a precipitation process
in which water falls in a Liquid state.</rdfs:comment>
</owl:Class>

<owl:Class rdf:ID= "Ramp">
<rdfs:subClassOf rdf:resource ="http://127.0.0.1:8000/ontology/SUMO.owl#Object"/>
<rdfs:comment>Ramp is the class of Objects that are
inclined planes used for moving objects from one level to another,
especially used for wheeled vehicles and people who cannot climb 
stairs.</rdfs:comment>
</owl:Class>

<owl:Class rdf:ID= "Raping">
<rdfs:subClassOf rdf:resource ="#Mating"/>
<rdfs:subClassOf rdf:resource ="#CriminalAction"/>
<rdfs:comment>Any instance of Mating where one participant does not
consent.</rdfs:comment>
</owl:Class>

<owl:Class rdf:ID= "Rat">
<rdfs:subClassOf rdf:resource ="http://127.0.0.1:8000/ontology/SUMO.owl#Rodent"/>
<rdfs:comment>A Rodent that has a hairless tail like a Mouse
but that is larger than a Mouse.</rdfs:comment>
</owl:Class>

<owl:Class rdf:ID= "Rattlesnake">
<rdfs:subClassOf rdf:resource ="#Snake"/>
<rdfs:comment>A subclass of Snake which derives its name
from the fact that it can manipulate its tail in such a way as to produce
a sound like that of a rattle.</rdfs:comment>
</owl:Class>

<owl:Class rdf:ID= "RawFood">
<rdfs:subClassOf rdf:resource ="http://127.0.0.1:8000/ontology/SUMO.owl#Food"/>
<rdfs:comment>Food that is not the result of Cooking.</rdfs:comment>
</owl:Class>

<owl:Class rdf:ID= "RealEstate">
<rdfs:subClassOf rdf:resource 
="http://127.0.0.1:8000/ontology/SUMO.owl#CorpuscularObject"/>
<rdfs:comment>Land, including all the natural resources and permanent 
buildings on it.</rdfs:comment>
</owl:Class>

<owl:Class rdf:ID= "RearWindow">
<rdfs:subClassOf rdf:resource ="#VehicleWindow"/>
<rdfs:comment>Any VehicleWindow which is located at the back
of an Automobile.</rdfs:comment>
</owl:Class>

<owl:Class rdf:ID= "ReceiverDevice">
<rdfs:subClassOf rdf:resource ="#CommunicationDevice"/>
<rdfs:subClassOf rdf:resource ="#ElectricDevice"/>
<rdfs:comment>An ElectricDevice that is capable of
receiving and decoding RadioEmissions, e.g. Radios and 
Televisions.</rdfs:comment>
</owl:Class>

<owl:Class rdf:ID= "Reciting">
<rdfs:subClassOf rdf:resource 
="http://127.0.0.1:8000/ontology/SUMO.owl#Speaking"/>
<rdfs:comment>Any instance of Speaking where what is
uttered is contained within a Text.</rdfs:comment>
</owl:Class>

<owl:Class rdf:ID= "RecordAlbum">
<rdfs:subClassOf rdf:resource ="#AudioRecording"/>
<rdfs:comment>A AudioRecording that has the form of a
plastic or glass disk with continuous grooves that are transformed into
sound by a record player.</rdfs:comment>
</owl:Class>

<owl:Class rdf:ID= "RecoveringFromIllness">
<rdfs:subClassOf rdf:resource 
="http://127.0.0.1:8000/ontology/SUMO.owl#OrganismProcess"/>
<rdfs:comment>Any Process where the experiencer recovers
from a DiseaseOrSyndrome.</rdfs:comment>
</owl:Class>

<owl:Class rdf:ID= "RecreationOrExerciseDevice">
<rdfs:subClassOf rdf:resource ="http://127.0.0.1:8000/ontology/SUMO.owl#Device"/>
<rdfs:comment>A Device whose purpose is RecreationOrExercise.</rdfs:comment>
</owl:Class>

<owl:Class rdf:ID= "Rectangle">
<rdfs:subClassOf rdf:resource ="#Quadrilateral"/>
<rdfs:comment>Any Quadrilateral whose angles are all
RightAngles.</rdfs:comment>
</owl:Class>

<owl:Class rdf:ID= "RedBloodCell">
<rdfs:subClassOf rdf:resource ="#BloodCell"/>
<rdfs:comment>BloodCells that contain hemoglobin, lack a
CellNucleus, and carry Oxygen to the tissues of the body.</rdfs:comment>
</owl:Class>

<owl:Class rdf:ID= "RedcoatSoldier">
<rdfs:subClassOf rdf:resource ="#Soldier"/>
<rdfs:comment>Any Soldier that served on the British side during
the American revolutionary war.</rdfs:comment>
</owl:Class>

<owl:Class rdf:ID= "ReferenceText">
<rdfs:subClassOf rdf:resource 
="http://127.0.0.1:8000/ontology/SUMO.owl#FactualText"/>
<rdfs:comment>A Text which is not intended to be read
from beginning to end, but which is meant to be consulted to answer specific
factual questions, e.g. about the meaning of a word, the location of a
country, etc.</rdfs:comment>
</owl:Class>

<owl:Class rdf:ID= "RefinedPetroleumProduct">
<rdfs:subClassOf rdf:resource ="#PetroleumProduct"/>
<rdfs:comment>RefinedPetroleumProduct is the
subclass of PetroleumProducts that are refined from Petroleum (crude 
oil).</rdfs:comment>
</owl:Class>

<owl:Class rdf:ID= "Reflecting">
<rdfs:subClassOf rdf:resource 
="http://127.0.0.1:8000/ontology/SUMO.owl#Radiating"/>
<rdfs:comment>Any instance of Radiating where the radiated
waves rebound from a surface, e.g. an echo of sound or a reflection of
light.</rdfs:comment>
</owl:Class>

<owl:Class rdf:ID= "ReflectingLight">
<rdfs:subClassOf rdf:resource ="#Reflecting"/>
<rdfs:subClassOf rdf:resource 
="http://127.0.0.1:8000/ontology/SUMO.owl#RadiatingLight"/>
<rdfs:comment>Those instances of RadiatingLight where the
instrument is not a light source, but is simply a surface which bends light
waves that come in contact with it.</rdfs:comment>
</owl:Class>

<owl:Class rdf:ID= "ReflexiveProcess">
<rdfs:subClassOf rdf:resource 
="http://127.0.0.1:8000/ontology/SUMO.owl#AutonomicProcess"/>
<rdfs:comment>Any Muscle reaction which is a response
to a specific stimulus and which does not reach the level of 
consciousness.</rdfs:comment>
</owl:Class>

<owl:Class rdf:ID= "Refrigerator">
<rdfs:subClassOf rdf:resource ="#CoolingDevice"/>
<rdfs:subClassOf rdf:resource ="#ElectricDevice"/>
<rdfs:subClassOf rdf:resource ="#Container"/>
<rdfs:comment>The intersection of Containers and ElectricDevices
in which the temperature is reduced from that of the outside air by a 
Cooling
process.</rdfs:comment>
</owl:Class>

<owl:Class rdf:ID= "Registering">
<rdfs:subClassOf rdf:resource 
="http://127.0.0.1:8000/ontology/SUMO.owl#Stating"/>
<rdfs:subClassOf rdf:resource 
="http://127.0.0.1:8000/ontology/SUMO.owl#PoliticalProcess"/>
<rdfs:comment>Submitting official paperwork to an organization,
typically a GovernmentOrganization or an EducationalOrganization.  This
class covers things like filing for divorce, making a legal claim against 
someone,
enrolling in an educational program, etc.</rdfs:comment>
</owl:Class>

<owl:Class rdf:ID= "Regretting">
<rdfs:subClassOf rdf:resource ="#ExpressingDisapproval"/>
<rdfs:comment>ExpressingDisapproval about a state of affairs
that has already occurred.</rdfs:comment>
</owl:Class>

<owl:Class rdf:ID= "Releasing">
<rdfs:subClassOf rdf:resource 
="http://127.0.0.1:8000/ontology/SUMO.owl#Translocation"/>
<sumo:disjoint rdf:resource = "#Escaping" />
<rdfs:comment>Any instance of Translocation where the experiencer
is released from confinement by right.</rdfs:comment>
</owl:Class>

<owl:Class rdf:ID= "RelievingPain">
<rdfs:subClassOf rdf:resource 
="http://127.0.0.1:8000/ontology/SUMO.owl#TherapeuticProcess"/>
<rdfs:subClassOf rdf:resource ="#CausingHappiness"/>
<rdfs:comment>Any TherapeuticProcess that removes Pain from
the patient of the process.</rdfs:comment>
</owl:Class>

<owl:Class rdf:ID= "ReligiousBuilding">
<rdfs:subClassOf rdf:resource 
="http://127.0.0.1:8000/ontology/SUMO.owl#Building"/>
<rdfs:comment>A Building which is intended to be
used for religious worship.  This class covers churches, temples,
religious shrines, etc.</rdfs:comment>
</owl:Class>

<owl:Class rdf:ID= "ReligiousPosition">
<rdfs:subClassOf rdf:resource 
="http://127.0.0.1:8000/ontology/SUMO.owl#Position"/>
<rdfs:comment>Any Position within a ReligousOrganization.</rdfs:comment>
</owl:Class>

<owl:Class rdf:ID= "ReligiousService">
<rdfs:subClassOf rdf:resource 
="http://127.0.0.1:8000/ontology/SUMO.owl#ReligiousProcess"/>
<rdfs:subClassOf rdf:resource 
="http://127.0.0.1:8000/ontology/SUMO.owl#Demonstrating"/>
<rdfs:comment>A formal process of public worship which is
typically carried out in a church, temple or other sanctified building and
which typically accords with a prescribed set of rules.</rdfs:comment>
</owl:Class>

<owl:Class rdf:ID= "Reminding">
<rdfs:subClassOf rdf:resource 
="http://127.0.0.1:8000/ontology/SUMO.owl#Requesting"/>
<rdfs:comment>Any Requesting that is intended to cause a
Remembering of something.</rdfs:comment>
</owl:Class>

<owl:Class rdf:ID= "RemovingClothing">
<rdfs:subClassOf rdf:resource 
="http://127.0.0.1:8000/ontology/SUMO.owl#Uncovering"/>
<rdfs:comment>Removing Clothing from a Human or
Animal in such a way that the Human or Animal no longer wears the
Clothing.</rdfs:comment>
</owl:Class>

<owl:Class rdf:ID= "Renting">
<rdfs:subClassOf rdf:resource 
="http://127.0.0.1:8000/ontology/SUMO.owl#FinancialTransaction"/>
<rdfs:subClassOf rdf:resource 
="http://127.0.0.1:8000/ontology/SUMO.owl#Borrowing"/>
<rdfs:comment>Giving money to the owner of an Object in
exchange for the right to use the Object for a fixed time 
period.</rdfs:comment>
</owl:Class>

<owl:Class rdf:ID= "Report">
<rdfs:subClassOf rdf:resource 
="http://127.0.0.1:8000/ontology/SUMO.owl#FactualText"/>
<rdfs:subClassOf rdf:resource 
="http://127.0.0.1:8000/ontology/SUMO.owl#Article"/>
<rdfs:comment>A relatively brief FactualText, often it
describes the findings of a study or experiment, or a series of
observations.</rdfs:comment>
</owl:Class>

<owl:Class rdf:ID= "Request">
<rdfs:subClassOf rdf:resource 
="http://127.0.0.1:8000/ontology/SUMO.owl#Sentence"/>
<rdfs:comment>A Sentence that expresses a request for something or
that something be done.</rdfs:comment>
</owl:Class>

<owl:Class rdf:ID= "Researcher">
<rdfs:subClassOf rdf:resource ="#Profession"/>
<rdfs:comment>The Profession of being a scientific
researcher.</rdfs:comment>
</owl:Class>

<owl:Class rdf:ID= "Resigning">
<rdfs:subClassOf rdf:resource 
="http://127.0.0.1:8000/ontology/SUMO.owl#TerminatingEmployment"/>
<rdfs:comment>Voluntarily ending one's employment.</rdfs:comment>
</owl:Class>

<owl:Class rdf:ID= "Resistor">
<rdfs:subClassOf rdf:resource 
="http://127.0.0.1:8000/ontology/SUMO.owl#EngineeringComponent"/>
<rdfs:comment>A Device which resists passage of an electric current
through it.  It is used for various purposes in an electrical 
circuit.</rdfs:comment>
</owl:Class>

<owl:Class rdf:ID= "Resolution">
<rdfs:subClassOf rdf:resource 
="http://127.0.0.1:8000/ontology/SUMO.owl#Deciding"/>
<rdfs:comment>Any instance of Deciding which is conducted at a
FormalMeeting and where the agent is an Organization.</rdfs:comment>
</owl:Class>

<owl:Class rdf:ID= "Restaurant">
<rdfs:subClassOf rdf:resource 
="http://127.0.0.1:8000/ontology/SUMO.owl#CommercialAgent"/>
<rdfs:comment>Any CommercialAgent whose services include selling
Food to customers which is intended to be eaten on the 
premises.</rdfs:comment>
</owl:Class>

<owl:Class rdf:ID= "RetailStore">
<rdfs:subClassOf rdf:resource 
="http://127.0.0.1:8000/ontology/SUMO.owl#MercantileOrganization"/>
<sumo:disjoint rdf:resource = "#WholesaleStore" />
<rdfs:comment>The complement of WholesaleStore, i.e.
MercantileOrganizations that sell their goods to the general 
public.</rdfs:comment>
</owl:Class>

<owl:Class rdf:ID= "Retina">
<rdfs:subClassOf rdf:resource ="http://127.0.0.1:8000/ontology/SUMO.owl#Organ"/>
<rdfs:subClassOf rdf:resource 
="http://127.0.0.1:8000/ontology/SUMO.owl#AnimalAnatomicalStructure"/>
<rdfs:comment>A membrane that covers the Eye and converts
the image formed by the lens of the Eye into neurochemical impulses
which can be processed by the Brain.</rdfs:comment>
</owl:Class>

<owl:Class rdf:ID= "Retiring">
<rdfs:subClassOf rdf:resource ="#Resigning"/>
<rdfs:comment>Voluntarily leaving employment at the end of one's
career in order to take time off in the later years of one's 
life.</rdfs:comment>
</owl:Class>

<owl:Class rdf:ID= "Returning">
<rdfs:subClassOf rdf:resource 
="http://127.0.0.1:8000/ontology/SUMO.owl#Translocation"/>
<rdfs:comment>Any instance of Translocation where the agent
goes to a location where he/she had been before the Translocation took 
place.</rdfs:comment>
</owl:Class>

<owl:Class rdf:ID= "Reversing">
<rdfs:subClassOf rdf:resource ="http://127.0.0.1:8000/ontology/SUMO.owl#Motion"/>
<rdfs:comment>Moving something in such a way that its top
becomes its bottom and vice versa.</rdfs:comment>
</owl:Class>

<owl:Class rdf:ID= "RevolverGun">
<rdfs:subClassOf rdf:resource ="#Pistol"/>
<rdfs:comment>A Pistol whose magazine is a revolving cylinder with
six chambers for Bullets.</rdfs:comment>
</owl:Class>

<owl:Class rdf:ID= "Rice">
<rdfs:subClassOf rdf:resource ="#CerealGrain"/>
<rdfs:comment>A CerealGrain which has short and long grain varieties
and which is usually prepared for eating by steaming.</rdfs:comment>
</owl:Class>

<owl:Class rdf:ID= "Rifle">
<rdfs:subClassOf rdf:resource ="#Firearm"/>
<rdfs:comment>A Firearm with a long barrel that is intended to be fired
from the shoulder.</rdfs:comment>
</owl:Class>

<owl:Class rdf:ID= "RightAngle">
<rdfs:subClassOf rdf:resource 
="http://127.0.0.1:8000/ontology/SUMO.owl#TwoDimensionalAngle"/>
<rdfs:comment>Any TwoDimensionalAngle that has the
angularMeasure of 90 AngularDegrees.</rdfs:comment>
</owl:Class>

<owl:Class rdf:ID= "RightTriangle">
<rdfs:subClassOf rdf:resource ="#Triangle"/>
<rdfs:comment>Any Triangle that contains a RightAngle.</rdfs:comment>
</owl:Class>

<owl:Class rdf:ID= "Ringing">
<rdfs:subClassOf rdf:resource 
="http://127.0.0.1:8000/ontology/SUMO.owl#RadiatingSound"/>
<rdfs:comment>Any instance of RadiatingSound which is produced by
a Bell.</rdfs:comment>
</owl:Class>

<owl:Class rdf:ID= "River">
<rdfs:subClassOf rdf:resource ="#BodyOfWater"/>
<rdfs:subClassOf rdf:resource 
="http://127.0.0.1:8000/ontology/SUMO.owl#StreamWaterArea"/>
<rdfs:subClassOf rdf:resource 
="http://127.0.0.1:8000/ontology/SUMO.owl#FreshWaterArea"/>
<rdfs:comment>River is the class of large streams of fresh
water flowing through land into a lake, ocean, or other body of 
water.</rdfs:comment>
</owl:Class>

<owl:Class rdf:ID= "RoadJunction">
<rdfs:subClassOf rdf:resource ="#TransitwayJunction"/>
<rdfs:subClassOf rdf:resource 
="http://127.0.0.1:8000/ontology/SUMO.owl#Roadway"/>
<rdfs:comment>RoadJunction is the subclass of
TransitwayJunctions where two or more Roadways come together.</rdfs:comment>
</owl:Class>

<owl:Class rdf:ID= "RoadTransportationSystem">
<rdfs:subClassOf rdf:resource ="#TransportationSystem"/>
<rdfs:comment>RoadTransportationSystem
is the subclass of TransportationSystems whose routes are 
Roadways.</rdfs:comment>
</owl:Class>

<owl:Class rdf:ID= "RoadVehicle">
<rdfs:subClassOf rdf:resource ="#LandVehicle"/>
<rdfs:comment>The class of LandVehicles that are not
RollingStock.</rdfs:comment>
</owl:Class>

<owl:Class rdf:ID= "Robbing">
<rdfs:subClassOf rdf:resource ="#Stealing"/>
<rdfs:comment>Any instance of Stealing which involves the threat
of the use of force.</rdfs:comment>
</owl:Class>

<owl:Class rdf:ID= "Rock">
<rdfs:subClassOf rdf:resource 
="http://127.0.0.1:8000/ontology/SUMO.owl#Substance"/>
<rdfs:comment>Rock is any naturally formed aggregate of
one or more minerals, consolidated or not, with some degree of
mineralogic and chemical constancy; in popular use the term is
usually restricted to those aggregates that are hard, compact,
and coherent.</rdfs:comment>
</owl:Class>

<owl:Class rdf:ID= "Rocket">
<rdfs:subClassOf rdf:resource ="#Spacecraft"/>
<rdfs:comment>A Spacecraft which has the shape of a cylinder
with a cone on top and which is powered by a jet engine.</rdfs:comment>
</owl:Class>

<owl:Class rdf:ID= "RollingStock">
<rdfs:subClassOf rdf:resource ="#RailwayVehicle"/>
<rdfs:comment>RollingStock is the subclass of
RailwayVehicles that are individual railway cars.  RollingStock includes
locomotives, motorized transit cars, trolleys, and all kinds of 
railcars.</rdfs:comment>
</owl:Class>

<owl:Class rdf:ID= "Roof">
<rdfs:subClassOf rdf:resource 
="http://127.0.0.1:8000/ontology/SUMO.owl#StationaryArtifact"/>
<rdfs:comment>The top of a Building.</rdfs:comment>
</owl:Class>

<owl:Class rdf:ID= "Rooster">
<rdfs:subClassOf rdf:resource ="#Chicken"/>
<rdfs:comment>A Male Chicken.</rdfs:comment>
</owl:Class>

<owl:Class rdf:ID= "Rotating">
<rdfs:subClassOf rdf:resource ="http://127.0.0.1:8000/ontology/SUMO.owl#Motion"/>
<rdfs:comment>Motion that begins and ends at the same point,
because the trajectory of the Motion is circular.</rdfs:comment>
</owl:Class>

<owl:Class rdf:ID= "Rotor">
<rdfs:subClassOf rdf:resource 
="http://127.0.0.1:8000/ontology/SUMO.owl#EngineeringComponent"/>
<rdfs:comment>The Rotating component of a motor, generator or similar
Device.</rdfs:comment>
</owl:Class>

<owl:Class rdf:ID= "Rowing">
<rdfs:subClassOf rdf:resource ="#WaterTransportation"/>
<rdfs:comment>Any instance of WaterTransportation where the
instrument is an Oar that is manually powered.</rdfs:comment>
</owl:Class>

<owl:Class rdf:ID= "Rubber">
<rdfs:subClassOf rdf:resource 
="http://127.0.0.1:8000/ontology/SUMO.owl#PlantSubstance"/>
<rdfs:comment>A latex that is produced by certain species of
BotanticalTrees.</rdfs:comment>
</owl:Class>

<owl:Class rdf:ID= "Rug">
<rdfs:subClassOf rdf:resource ="#FabricArtifact"/>
<rdfs:comment>A piece of Fabric whose purpose is to cover a 
Floor.</rdfs:comment>
</owl:Class>

<owl:Class rdf:ID= "Runway">
<rdfs:subClassOf rdf:resource 
="http://127.0.0.1:8000/ontology/SUMO.owl#LandTransitway"/>
<rdfs:comment>Runway is the class of Transitways that are
used for the takeoff and landing of Airplanes.  Runways are
Transitways for an intermodal transit, which begins with a land transit
and ends with air transit, or vice versa.</rdfs:comment>
</owl:Class>

<owl:Class rdf:ID= "Saddle">
<rdfs:subClassOf rdf:resource ="#Holder"/>
<rdfs:comment>A Device which allows a Human to ride on a
Horse.</rdfs:comment>
</owl:Class>

<owl:Class rdf:ID= "SafeContainer">
<rdfs:subClassOf rdf:resource ="#Container"/>
<rdfs:subClassOf rdf:resource ="#SecurityDevice"/>
<rdfs:comment>A Container with a Lock which is intended
to secure items from theft.  Note that this covers safes, lockers, and 
locked
storage compartments.</rdfs:comment>
</owl:Class>

<owl:Class rdf:ID= "Sailor">
<rdfs:subClassOf rdf:resource ="#SkilledOccupation"/>
<rdfs:comment>The class of Positions which involve working on a
ship, whether a merchant ship or a navy ship.</rdfs:comment>
</owl:Class>

<owl:Class rdf:ID= "SalesPosition">
<rdfs:subClassOf rdf:resource ="#SkilledOccupation"/>
<rdfs:comment>Any Position which involves Selling
or trying to sell items.</rdfs:comment>
</owl:Class>

<owl:Class rdf:ID= "SalineSolution">
<rdfs:subClassOf rdf:resource 
="http://127.0.0.1:8000/ontology/SUMO.owl#Solution"/>
<rdfs:comment>A Solution consisting of SodiumChloride
and Water.</rdfs:comment>
</owl:Class>

<owl:Class rdf:ID= "SaltLake">
<rdfs:subClassOf rdf:resource 
="http://127.0.0.1:8000/ontology/SUMO.owl#SaltWaterArea"/>
<rdfs:subClassOf rdf:resource ="#LandlockedWater"/>
<rdfs:comment>SaltLake is the class of landlocked
bodies of salt water, including those referred to as 'Seas', e.g.,
the CaspianSea.  But note that the MediterraneanSea is a Sea.</rdfs:comment>
</owl:Class>

<owl:Class rdf:ID= "Sand">
<rdfs:subClassOf rdf:resource ="#Soil"/>
<rdfs:comment>Sand is loose fragments of minerals or rocks.
Smaller than gravel and larger than silt and clay, sand particles
range from 8/10,000 to 8/100 inch (0.02 to 2 millimeters) in diameter.
Sand is formed by the Erosion of rocks through the action of water,
ice, or air.</rdfs:comment>
</owl:Class>

<owl:Class rdf:ID= "Sandwich">
<rdfs:subClassOf rdf:resource ="#PreparedFood"/>
<rdfs:comment>Any Food which consists of two or more pieces
of bread and some sort of filling between the two pieces of 
bread.</rdfs:comment>
</owl:Class>

<owl:Class rdf:ID= "Satellite">
<rdfs:comment>Satellite is the collection of bodies that
revolve around some  astronomical body, e.g., planets around a 
star.</rdfs:comment>
</owl:Class>

<owl:Class rdf:ID= "Saving">
<rdfs:subClassOf rdf:resource 
="http://127.0.0.1:8000/ontology/SUMO.owl#Decreasing"/>
<rdfs:comment>Any instance of Decreasing where the PhysicalQuantity
involved is a CurrencyMeasure.</rdfs:comment>
</owl:Class>

<owl:Class rdf:ID= "SavingsAccount">
<rdfs:subClassOf rdf:resource ="#InterestBearingAccount"/>
<rdfs:subClassOf rdf:resource ="#DepositAccount"/>
<rdfs:comment>An account in a bank on which interest is
usually paid and from which withdrawals can be made usually only by
presentation of a passbook or by written authorization on a prescribed 
form.</rdfs:comment>
</owl:Class>

<owl:Class rdf:ID= "SavingsAndLoan">
<rdfs:subClassOf rdf:resource ="#FinancialCompany"/>
<rdfs:comment>A federally or state chartered
FinancialCompany that takes Deposits from individuals, funds
Mortgages, and pays Dividends.</rdfs:comment>
</owl:Class>

<owl:Class rdf:ID= "Scar">
<rdfs:subClassOf rdf:resource 
="http://127.0.0.1:8000/ontology/SUMO.owl#AbnormalAnatomicalStructure"/>
<rdfs:comment>Any AbnormalAnatomicalStructure which results from the
healing of a Lesion.</rdfs:comment>
</owl:Class>

<owl:Class rdf:ID= "Scholarship">
<rdfs:subClassOf rdf:resource 
="http://127.0.0.1:8000/ontology/SUMO.owl#Funding"/>
<rdfs:comment>Any Funding which is made on the basis of merit
and whose purpose is to allow the destination to realize an
EducationalProgram.</rdfs:comment>
</owl:Class>

<owl:Class rdf:ID= "School">
<rdfs:subClassOf rdf:resource 
="http://127.0.0.1:8000/ontology/SUMO.owl#EducationalOrganization"/>
<rdfs:comment>An EducationalOrganization with a curriculum,
teachers, and students.  Most Schools are housed in a Building
dedicated to the EducationalOrganization.</rdfs:comment>
</owl:Class>

<owl:Class rdf:ID= "Science">
<rdfs:subClassOf rdf:resource 
="http://127.0.0.1:8000/ontology/SUMO.owl#FieldOfStudy"/>
<rdfs:comment>Any FieldOfStudy which tests theories on the basis of
careful observations and/or experiments and which has a cumulative body of 
results.</rdfs:comment>
</owl:Class>

<owl:Class rdf:ID= "Score">
<rdfs:subClassOf rdf:resource ="#GameShot"/>
<rdfs:comment>A successful attempt to score a point in a 
Game.</rdfs:comment>
</owl:Class>

<owl:Class rdf:ID= "Screw">
<rdfs:subClassOf rdf:resource 
="http://127.0.0.1:8000/ontology/SUMO.owl#AttachingDevice"/>
<rdfs:comment>An AttachingDevice which contains a spiral of grooves to
hold it in place and which is fastened with a screwdriver.</rdfs:comment>
</owl:Class>

<owl:Class rdf:ID= "Sculpture">
<rdfs:subClassOf rdf:resource 
="http://127.0.0.1:8000/ontology/SUMO.owl#ArtWork"/>
<rdfs:comment>Any ArtWork which is not constructed on the
two-dimensional surface of a canvas, piece of paper, etc.</rdfs:comment>
</owl:Class>

<owl:Class rdf:ID= "Sea">
<rdfs:subClassOf rdf:resource 
="http://127.0.0.1:8000/ontology/SUMO.owl#SaltWaterArea"/>
<rdfs:subClassOf rdf:resource ="#BodyOfWater"/>
<rdfs:comment>Sea is the class of smaller subdivisions of
the WorldOcean, typically partially surrounded by land.</rdfs:comment>
</owl:Class>

<owl:Class rdf:ID= "SeasonOfYear">
<rdfs:subClassOf rdf:resource 
="http://127.0.0.1:8000/ontology/SUMO.owl#TimeInterval"/>
<rdfs:comment>SeasonOfYear is the class of four
seasons correlated with the calendar Year and associated with
changes in the length of daylight and with overall temperature
changes. Depending upon the GeographicArea, a SeasonOfYear
may also be associated with weather patterns (e.g., rainy, dry,
windy). The characteristics of seasons (cold vs. hot temperatures,
long vs. short days) are reversed from the NorthernHemisphere
to the SouthernHemisphere.</rdfs:comment>
</owl:Class>

<owl:Class rdf:ID= "Seat">
<rdfs:subClassOf rdf:resource ="#Furniture"/>
<rdfs:comment>Any instance of Furniture which is designed to
accommodate Humans who are Sitting.</rdfs:comment>
</owl:Class>

<owl:Class rdf:ID= "Seating">
<rdfs:subClassOf rdf:resource 
="http://127.0.0.1:8000/ontology/SUMO.owl#Guiding"/>
<rdfs:comment>Guiding someone to a Seat, e.g. as when an usher
shows someone to a Seat in an Auditorium.</rdfs:comment>
</owl:Class>

<owl:Class rdf:ID= "SecondaryColor">
<rdfs:comment>A color that is the product of mixing together
two or more PrimaryColors.</rdfs:comment>
</owl:Class>

<owl:Class rdf:ID= "SecondarySchool">
<rdfs:subClassOf rdf:resource ="#School"/>
<rdfs:comment>A School which admits students who have
graduated from a middle school and which normally covers the ninth through
twelfth grades.  A SecondarySchool confers a high school 
diploma.</rdfs:comment>
</owl:Class>

<owl:Class rdf:ID= "Security">
<rdfs:subClassOf rdf:resource 
="http://127.0.0.1:8000/ontology/SUMO.owl#FinancialInstrument"/>
<rdfs:comment>An investment instrument, other than an insurance
policy or a fixed annuity issued by a corporation, government, or other
organization which offers evidence of debt or equity.</rdfs:comment>
</owl:Class>

<owl:Class rdf:ID= "SecurityAlarm">
<rdfs:subClassOf rdf:resource ="#SecurityDevice"/>
<rdfs:subClassOf rdf:resource ="#ElectricDevice"/>
<rdfs:comment>A SecurityDevice that detects intrusions to
a StationaryArtifact and issues a warning of some sort.</rdfs:comment>
</owl:Class>

<owl:Class rdf:ID= "SecurityDevice">
<rdfs:subClassOf rdf:resource ="http://127.0.0.1:8000/ontology/SUMO.owl#Device"/>
<rdfs:comment>A Device whose purpose is to protect people or
property from kidnappers and/or thieves.</rdfs:comment>
</owl:Class>

<owl:Class rdf:ID= "SecurityUnit">
<rdfs:subClassOf rdf:resource 
="http://127.0.0.1:8000/ontology/SUMO.owl#Organization"/>
<rdfs:comment>The Organization that is charged with
ensuring the security of members of the overall Organization and the
property of the Organization.</rdfs:comment>
</owl:Class>

<owl:Class rdf:ID= "SeizingProperty">
<rdfs:subClassOf rdf:resource 
="http://127.0.0.1:8000/ontology/SUMO.owl#UnilateralGetting"/>
<rdfs:comment>Any instance of UnilateralGetting which is done by
a Government and which is not permitted by the origin of the 
UnilateralGetting.</rdfs:comment>
</owl:Class>

<owl:Class rdf:ID= "SelfPoweredDevice">
<rdfs:subClassOf rdf:resource ="http://127.0.0.1:8000/ontology/SUMO.owl#Device"/>
<rdfs:comment>SelfPoweredDevice is the subclass of Devices whose action is
powered by some kind of on-board component or power source (not the 
user).</rdfs:comment>
</owl:Class>

<owl:Class rdf:ID= "SelfPoweredRoadVehicle">
<rdfs:subClassOf rdf:resource ="#RoadVehicle"/>
<rdfs:subClassOf rdf:resource ="#SelfPoweredVehicle"/>
<rdfs:comment>SelfPoweredRoadVehicle is the
class of RoadVehicles that are also SelfPoweredVehicles.
SelfPoweredRoadVehicle covers motorcycles, semi-trailers, RVs, etc.,
as well as Automobiles.  This class includes vehicles powered by
electricity, gasoline, diesel, and other fuels.</rdfs:comment>
</owl:Class>

<owl:Class rdf:ID= "SelfPoweredVehicle">
<rdfs:subClassOf rdf:resource 
="http://127.0.0.1:8000/ontology/SUMO.owl#Vehicle"/>
<rdfs:subClassOf rdf:resource ="#SelfPoweredDevice"/>
<rdfs:comment>SelfPoweredVehicle is the subclass
of Vehicles whose motion is powered by some kind of on-board power
source.</rdfs:comment>
</owl:Class>

<owl:Class rdf:ID= "Sentencing">
<rdfs:subClassOf rdf:resource 
="http://127.0.0.1:8000/ontology/SUMO.owl#LegalDecision"/>
<rdfs:comment>Any LegalDecision where the defendant is assigned
a punishment for a CriminalAction which was the subject of an earlier
LegalConviction.</rdfs:comment>
</owl:Class>

<owl:Class rdf:ID= "Sergeant">
<rdfs:subClassOf rdf:resource ="#MilitaryOfficer"/>
<rdfs:comment>A noncomissioned MilitaryOfficer.</rdfs:comment>
</owl:Class>

<owl:Class rdf:ID= "Sermon">
<rdfs:subClassOf rdf:resource ="#Lecture"/>
<rdfs:comment>A Lecture that is part of a ReligiousService.</rdfs:comment>
</owl:Class>

<owl:Class rdf:ID= "Serum">
<rdfs:subClassOf rdf:resource ="#LiquidBodySubstance"/>
<sumo:disjoint rdf:resource = "http://127.0.0.1:8000/ontology/SUMO.owl#Blood" />
<rdfs:comment>Any LiquidBodySubstance other than Blood.</rdfs:comment>
</owl:Class>

<owl:Class rdf:ID= "ServicePosition">
<rdfs:subClassOf rdf:resource ="#SkilledOccupation"/>
<rdfs:comment>Any Position which involves working
as a waiter or servant, either for an Organization (e.g. a restaurant)
or for a person or family.</rdfs:comment>
</owl:Class>

<owl:Class rdf:ID= "Sewage">
<rdfs:subClassOf rdf:resource 
="http://127.0.0.1:8000/ontology/SUMO.owl#Mixture"/>
<rdfs:comment>Waste products produced by Humans.</rdfs:comment>
</owl:Class>

<owl:Class rdf:ID= "SewageSystem">
<rdfs:subClassOf rdf:resource ="#Pipeline"/>
<rdfs:comment>A Pipline which is used to transport human
waste to an area where it can be treated and/or disposed of.</rdfs:comment>
</owl:Class>

<owl:Class rdf:ID= "Sewing">
<rdfs:subClassOf rdf:resource 
="http://127.0.0.1:8000/ontology/SUMO.owl#Attaching"/>
<rdfs:comment>Attaching two pieces of Fabric or one part of a
piece of Fabric to another part by means of needle and 
thread.</rdfs:comment>
</owl:Class>

<owl:Class rdf:ID= "Share">
<rdfs:subClassOf rdf:resource 
="http://127.0.0.1:8000/ontology/SUMO.owl#CurrencyMeasure"/>
<rdf:type rdf:resource = 
"http://127.0.0.1:8000/ontology/SUMO.owl#UnitOfMeasure"/>
<rdfs:comment>A UnitOfMeasure representing one unit of ownership
in a corporation, MutualFund, or limited partnership.</rdfs:comment>
</owl:Class>

<owl:Class rdf:ID= "Sharing">
<rdfs:subClassOf rdf:resource 
="http://127.0.0.1:8000/ontology/SUMO.owl#ChangeOfPossession"/>
<rdfs:comment>The subclass of ChangeOfPossession where a
properPart of the patient is given by the agent to the 
destination.</rdfs:comment>
</owl:Class>

<owl:Class rdf:ID= "Sheep">
<rdfs:subClassOf rdf:resource 
="http://127.0.0.1:8000/ontology/SUMO.owl#HoofedMammal"/>
<rdfs:subClassOf rdf:resource ="#DomesticAnimal"/>
<rdfs:comment>A domesticated HoofedMammal that is bred for its
wool and for its meat (known as mutton).</rdfs:comment>
</owl:Class>

<owl:Class rdf:ID= "Shelf">
<rdfs:subClassOf rdf:resource 
="http://127.0.0.1:8000/ontology/SUMO.owl#Artifact"/>
<rdfs:comment>An piece of Furniture or part of a piece of Furniture
that is used for keeping or displaying things.</rdfs:comment>
</owl:Class>

<owl:Class rdf:ID= "Sheriff">
<rdfs:subClassOf rdf:resource ="#PoliceOfficer"/>
<rdfs:comment>A PoliceOfficer whose jurisdiction is a County.</rdfs:comment>
</owl:Class>

<owl:Class rdf:ID= "Shield">
<rdfs:subClassOf rdf:resource 
="http://127.0.0.1:8000/ontology/SUMO.owl#Artifact"/>
<rdfs:comment>An Artifact that is held by the hand or whole arm and
is used to prevent injuries from Weapons.</rdfs:comment>
</owl:Class>

<owl:Class rdf:ID= "Ship">
<rdfs:subClassOf rdf:resource ="#DisplacementHullWatercraft"/>
<rdfs:comment>Ship is the class of large Watercraft used
for travel on oceans, seas, or large lakes.</rdfs:comment>
</owl:Class>

<owl:Class rdf:ID= "ShipCaptain">
<rdfs:subClassOf rdf:resource ="#SkilledOccupation"/>
<rdfs:comment>The class of Positions which involve the command
of a ship.</rdfs:comment>
</owl:Class>

<owl:Class rdf:ID= "ShipMate">
<rdfs:subClassOf rdf:resource ="#SkilledOccupation"/>
<rdfs:comment>The class of Positions that involve some responsibility
on a ship and are lower in rank than ShipCaptain.</rdfs:comment>
</owl:Class>

<owl:Class rdf:ID= "ShipOfficer">
<rdfs:subClassOf rdf:resource ="#Sailor"/>
<rdfs:comment>The class of Sailors which have a position of
responsibility on a Ship.</rdfs:comment>
</owl:Class>

<owl:Class rdf:ID= "Shipping">
<rdfs:subClassOf rdf:resource 
="http://127.0.0.1:8000/ontology/SUMO.owl#Transportation"/>
<rdfs:comment>Shipping is the subclass of Transportation
events in which goods are transported from one place to another by an
agent who is entrusted with the goods temporarily just in order to move
them.  Shipping may be done within an organization or it may be done
by an outside commercial agent.  See CommercialShipping.</rdfs:comment>
</owl:Class>

<owl:Class rdf:ID= "Shirt">
<rdfs:subClassOf rdf:resource 
="http://127.0.0.1:8000/ontology/SUMO.owl#Clothing"/>
<rdfs:comment>An item of Clothing which covers the upper body of a
Human.</rdfs:comment>
</owl:Class>

<owl:Class rdf:ID= "Shoe">
<rdfs:subClassOf rdf:resource 
="http://127.0.0.1:8000/ontology/SUMO.owl#Clothing"/>
<rdfs:comment>Clothing that is intended to be worn on the Foot.
It consists of an upper, a sole, and a heel.</rdfs:comment>
</owl:Class>

<owl:Class rdf:ID= "ShoppingMall">
<rdfs:subClassOf rdf:resource 
="http://127.0.0.1:8000/ontology/SUMO.owl#MercantileOrganization"/>
<rdfs:comment>A MercantileOrganization which is a collection
of various shops gathered together in a single, modern 
development.</rdfs:comment>
</owl:Class>

<owl:Class rdf:ID= "ShortStory">
<rdfs:subClassOf rdf:resource 
="http://127.0.0.1:8000/ontology/SUMO.owl#FictionalText"/>
<rdfs:subClassOf rdf:resource 
="http://127.0.0.1:8000/ontology/SUMO.owl#Article"/>
<rdfs:comment>A brief work of fiction, often bound with other
short stories in a Book or Periodical.</rdfs:comment>
</owl:Class>

<owl:Class rdf:ID= "Shortening">
<rdfs:subClassOf rdf:resource 
="http://127.0.0.1:8000/ontology/SUMO.owl#Decreasing"/>
<rdfs:comment>Decreasing the length of something.</rdfs:comment>
</owl:Class>

<owl:Class rdf:ID= "ShotBall">
<rdfs:subClassOf rdf:resource ="#Ball"/>
<rdfs:comment>A solid metal Ball that is used in the sport of
shotput.</rdfs:comment>
</owl:Class>

<owl:Class rdf:ID= "Shoulder">
<rdfs:subClassOf rdf:resource 
="http://127.0.0.1:8000/ontology/SUMO.owl#AnimalAnatomicalStructure"/>
<rdfs:subClassOf rdf:resource 
="http://127.0.0.1:8000/ontology/SUMO.owl#BodyPart"/>
<rdfs:comment>The part of a Primate between the Arm and
the neck.</rdfs:comment>
</owl:Class>

<owl:Class rdf:ID= "Shrub">
<rdfs:subClassOf rdf:resource 
="http://127.0.0.1:8000/ontology/SUMO.owl#FloweringPlant"/>
<rdfs:comment>Shrub is the class of low, perennial,
typically multi-stemmed woody plants, called shrubs or 
bushes.</rdfs:comment>
</owl:Class>

<owl:Class rdf:ID= "Shrugging">
<rdfs:subClassOf rdf:resource 
="http://127.0.0.1:8000/ontology/SUMO.owl#Gesture"/>
<rdfs:comment>Moving the Shoulders in such a way that the motion
is intended to express something to someone else.</rdfs:comment>
</owl:Class>

<owl:Class rdf:ID= "Sidewalk">
<rdfs:subClassOf rdf:resource 
="http://127.0.0.1:8000/ontology/SUMO.owl#StationaryArtifact"/>
<rdfs:comment>A prepared path for pedestrians alongside a 
Roadway.</rdfs:comment>
</owl:Class>

<owl:Class rdf:ID= "Siemens">
<rdfs:subClassOf rdf:resource 
="http://127.0.0.1:8000/ontology/SUMO.owl#FunctionQuantity"/>
<rdf:type rdf:resource = 
"http://127.0.0.1:8000/ontology/SUMO.owl#SystemeInternationalUnit"/>
<rdfs:comment>SI electric conductance measure.  Symbol:  S.
In the case of direct current, the conductance in Siemens is the
reciprocal of the resistance in Ohms; in the case of alternating current,
it is the reciprocal of the impedance in ohms.  siemens = A/V =
m^(-2)*kg(-1)*s^(3)*A^2.</rdfs:comment>
</owl:Class>

<owl:Class rdf:ID= "Sievert">
<rdfs:subClassOf rdf:resource 
="http://127.0.0.1:8000/ontology/SUMO.owl#FunctionQuantity"/>
<rdf:type rdf:resource = 
"http://127.0.0.1:8000/ontology/SUMO.owl#SystemeInternationalUnit"/>
<rdfs:comment>SI dose equivalent measure.  Symbol: Sv.  It is
a unit of biologic dose of ionizing radiation.  The Sievert makes it
possible to normalize doses of different types of radiation. It takes
into account the relative biologic effectiveness of ionizing radiation,
since each form of such radiation--e.g., X rays, gamma rays, neutrons--
has a slightly different effect on living tissue for a given absorbed
dose. The dose equivalent of a given type of radiation (in Sievert) is
the dose of the radiation in Gray multiplied by a quality factor that
is based on the relative biologic effectiveness of the radiation.
Accordingly, one Sievert is generally defined as the amount of radiation
roughly equivalent in biologic effectiveness to one Gray of gamma
radiation.  Sievert = J/kg = m^2*s^(-2)</rdfs:comment>
</owl:Class>

<owl:Class rdf:ID= "Signalling">
<rdfs:subClassOf rdf:resource 
="http://127.0.0.1:8000/ontology/SUMO.owl#Guiding"/>
<rdfs:comment>Signalling is the subclass of Guiding
processes in which an agent, animate or inanimate, sends a signal to
another Object.  In many cases, this signal will be an electrical or
electronic one.  Some signals may directly control the behavior of
the object signalled, while others may merely cause information to be
presented.  Instances of electrical Signalling are typically more
complex than simply than operation of a DeviceSwitch, though in some
cases, Signalling involves remote activation of such a switch by another
device.</rdfs:comment>
</owl:Class>

<owl:Class rdf:ID= "SigningADocument">
<rdfs:subClassOf rdf:resource 
="http://127.0.0.1:8000/ontology/SUMO.owl#Committing"/>
<rdfs:comment>SigningADocument is the class of
actions in which an agent affixes a signature, stamp, or other evidence
of authorization or attestation to a document.  The document and signature
may be electronic.  Signings count as SocialInteractions even if done in
private, because their significance derives from a social 
context.</rdfs:comment>
</owl:Class>

<owl:Class rdf:ID= "Silk">
<rdfs:subClassOf rdf:resource ="http://127.0.0.1:8000/ontology/SUMO.owl#Fabric"/>
<rdfs:comment>Fabric that is woven from the strands produced by
certain Larval Insects.</rdfs:comment>
</owl:Class>

<owl:Class rdf:ID= "Silver">
<rdfs:subClassOf rdf:resource 
="http://127.0.0.1:8000/ontology/SUMO.owl#ElementalSubstance"/>
<atomicNumber>47</atomicNumber>
<rdfs:comment>White lustrous soft metallic transition element.
Found in both its elemental form and in minerals.  Used in jewellery,
tableware and so on.  Less reactive than silver, chemically.</rdfs:comment>
</owl:Class>

<owl:Class rdf:ID= "Sinking">
<rdfs:subClassOf rdf:resource ="#Falling"/>
<rdfs:comment>The class of Falling processes that occur
in a BodyOfWater.</rdfs:comment>
</owl:Class>

<owl:Class rdf:ID= "SittingDown">
<rdfs:subClassOf rdf:resource 
="http://127.0.0.1:8000/ontology/SUMO.owl#BodyMotion"/>
<rdfs:comment>The BodyMotion of moving from a Standing
to a Sitting position.</rdfs:comment>
</owl:Class>

<owl:Class rdf:ID= "Skeleton">
<rdfs:subClassOf rdf:resource 
="http://127.0.0.1:8000/ontology/SUMO.owl#AnimalAnatomicalStructure"/>
<rdfs:subClassOf rdf:resource 
="http://127.0.0.1:8000/ontology/SUMO.owl#BodyPart"/>
<rdfs:comment>The system of Bones that make up the supporting structure
of Vertebrates.</rdfs:comment>
</owl:Class>

<owl:Class rdf:ID= "Sketch">
<rdfs:subClassOf rdf:resource 
="http://127.0.0.1:8000/ontology/SUMO.owl#ArtWork"/>
<rdfs:comment>Any ArtWork which is produced by a pencil or
piece of charcoal.</rdfs:comment>
</owl:Class>

<owl:Class rdf:ID= "SkilledOccupation">
<rdfs:subClassOf rdf:resource 
="http://127.0.0.1:8000/ontology/SUMO.owl#Position"/>
<rdfs:comment>Any Position which requires
learning a set of skills.</rdfs:comment>
</owl:Class>

<owl:Class rdf:ID= "Skin">
<rdfs:subClassOf rdf:resource 
="http://127.0.0.1:8000/ontology/SUMO.owl#BodyCovering"/>
<rdfs:comment>A BodyCovering that comprises part of the surface
of Organisms.</rdfs:comment>
</owl:Class>

<owl:Class rdf:ID= "Skull">
<rdfs:subClassOf rdf:resource ="http://127.0.0.1:8000/ontology/SUMO.owl#Bone"/>
<rdfs:comment>The Bone that is found in the Heads of 
Vertebrates.</rdfs:comment>
</owl:Class>

<owl:Class rdf:ID= "Skylight">
<rdfs:subClassOf rdf:resource ="#Window"/>
<rdfs:comment>A Window that is part of the Ceiling of
a Room.</rdfs:comment>
</owl:Class>

<owl:Class rdf:ID= "Sleeve">
<rdfs:subClassOf rdf:resource 
="http://127.0.0.1:8000/ontology/SUMO.owl#Clothing"/>
<rdfs:comment>A piece of Clothing that covers the Arm.  A
Sleeve is always part of a Coat or a Shirt.</rdfs:comment>
</owl:Class>

<owl:Class rdf:ID= "SlopedArea">
<rdfs:subClassOf rdf:resource ="#LandForm"/>
<rdfs:comment>A SlopedArea is a land surface which lies at an
angle to the horizontal so that some points on it are higher than others; a
slope.</rdfs:comment>
</owl:Class>

<owl:Class rdf:ID= "Slug">
<rdfs:subClassOf rdf:resource 
="http://127.0.0.1:8000/ontology/SUMO.owl#MassMeasure"/>
<rdf:type rdf:resource = 
"http://127.0.0.1:8000/ontology/SUMO.owl#UnitOfMeasure"/>
<rdfs:comment>English mass unit of slugs.</rdfs:comment>
</owl:Class>

<owl:Class rdf:ID= "Smiling">
<rdfs:subClassOf rdf:resource ="#FacialExpression"/>
<rdfs:comment>Spreading the lips in such a way as to convey
happiness.</rdfs:comment>
</owl:Class>

<owl:Class rdf:ID= "Smoking">
<rdfs:subClassOf rdf:resource 
="http://127.0.0.1:8000/ontology/SUMO.owl#RecreationOrExercise"/>
<rdfs:comment>Inhaling and exhaling Smoke produced by a
SmokingDevice.</rdfs:comment>
</owl:Class>

<owl:Class rdf:ID= "SmokingDevice">
<rdfs:subClassOf rdf:resource ="http://127.0.0.1:8000/ontology/SUMO.owl#Device"/>
<rdfs:comment>Any Device whose purpose is Smoking.</rdfs:comment>
</owl:Class>

<owl:Class rdf:ID= "SmokingPipe">
<rdfs:subClassOf rdf:resource ="#SmokingDevice"/>
<rdfs:comment>A SmokingDevice consisting of a tube and a small
bowl.</rdfs:comment>
</owl:Class>

<owl:Class rdf:ID= "Smuggling">
<rdfs:subClassOf rdf:resource 
="http://127.0.0.1:8000/ontology/SUMO.owl#Transportation"/>
<rdfs:subClassOf rdf:resource ="#CriminalAction"/>
<rdfs:comment>Any instance Transportation which is also a
CriminalAction.</rdfs:comment>
</owl:Class>

<owl:Class rdf:ID= "Snake">
<rdfs:subClassOf rdf:resource 
="http://127.0.0.1:8000/ontology/SUMO.owl#Reptile"/>
<rdfs:comment>A long and narrow Reptile which lacks Limbs.</rdfs:comment>
</owl:Class>

<owl:Class rdf:ID= "Snowing">
<rdfs:subClassOf rdf:resource 
="http://127.0.0.1:8000/ontology/SUMO.owl#Precipitation"/>
<rdfs:comment>Snowing is a precipitation process
in which water falls in a Solid state.</rdfs:comment>
</owl:Class>

<owl:Class rdf:ID= "SoberingUp">
<rdfs:subClassOf rdf:resource 
="http://127.0.0.1:8000/ontology/SUMO.owl#PsychologicalProcess"/>
<rdfs:comment>The process of transitioning from a state of
being Drunk to a state of being Sober.</rdfs:comment>
</owl:Class>

<owl:Class rdf:ID= "SocialParty">
<rdfs:subClassOf rdf:resource 
="http://127.0.0.1:8000/ontology/SUMO.owl#Meeting"/>
<rdfs:subClassOf rdf:resource 
="http://127.0.0.1:8000/ontology/SUMO.owl#RecreationOrExercise"/>
<rdfs:comment>Any Meeting where the intent is primarily
to socialize and be entertained.</rdfs:comment>
</owl:Class>

<owl:Class rdf:ID= "SocialScience">
<rdfs:subClassOf rdf:resource ="#Science"/>
<rdfs:comment>Any Science which studies human behavior, either in
the aggregate, as do, for example, Economics and Linguistics, or with 
respect to
the individual, as does Psychology.</rdfs:comment>
</owl:Class>

<owl:Class rdf:ID= "Sock">
<rdfs:subClassOf rdf:resource 
="http://127.0.0.1:8000/ontology/SUMO.owl#Clothing"/>
<rdfs:comment>A piece of Clothing that is made of a soft Fabric
like Cotton and that is intended to be worn on the Foot.</rdfs:comment>
</owl:Class>

<owl:Class rdf:ID= "Sodium">
<rdfs:subClassOf rdf:resource 
="http://127.0.0.1:8000/ontology/SUMO.owl#ElementalSubstance"/>
<atomicNumber>11</atomicNumber>
<rdfs:comment>Soft silvery reactive element belonging to group 1
of the periodic table (alkali metals).  It is highly reactive, oxidizing
in air and reacting violently with water, forcing it to be kept under oil.
It was first isolated by Humphrey Davy in 1807.</rdfs:comment>
</owl:Class>

<owl:Class rdf:ID= "SodiumChloride">
<rdfs:subClassOf rdf:resource 
="http://127.0.0.1:8000/ontology/SUMO.owl#CompoundSubstance"/>
<rdfs:comment>The CompoundSubstance formed from Sodium
and Chlorine.</rdfs:comment>
</owl:Class>

<owl:Class rdf:ID= "Sofa">
<rdfs:subClassOf rdf:resource ="#Seat"/>
<rdfs:comment>A padded Seat that is designed to accommodate more
than one Human.</rdfs:comment>
</owl:Class>

<owl:Class rdf:ID= "Soil">
<rdfs:subClassOf rdf:resource 
="http://127.0.0.1:8000/ontology/SUMO.owl#Mixture"/>
<rdfs:comment>Soil is a substance composed of fine rock material
disintegrated by geological processes, mixed with humus, the organic remains
of decomposed vegetation.</rdfs:comment>
</owl:Class>

<owl:Class rdf:ID= "SolarSystem">
<rdfs:subClassOf rdf:resource 
="http://127.0.0.1:8000/ontology/SUMO.owl#Collection"/>
<rdfs:comment>SolarSystem is the class of systems that
consist of a star or stars and any encircling astronomical 
bodies.</rdfs:comment>
</owl:Class>

<owl:Class rdf:ID= "Soldering">
<rdfs:subClassOf rdf:resource 
="http://127.0.0.1:8000/ontology/SUMO.owl#Attaching"/>
<rdfs:comment>Attaching two things by means of a 
MetallicAlloy.</rdfs:comment>
</owl:Class>

<owl:Class rdf:ID= "Soldier">
<rdfs:subClassOf rdf:resource ="#SkilledOccupation"/>
<rdfs:comment>The class of Positions which involve serving in
the armed forces of a Nation.</rdfs:comment>
</owl:Class>

<owl:Class rdf:ID= "Somersaulting">
<rdfs:subClassOf rdf:resource 
="http://127.0.0.1:8000/ontology/SUMO.owl#BodyMotion"/>
<rdfs:comment>Any BodyMotion which begins and ends in
a Sitting position and where the feet roll over the head and return to
their original position.</rdfs:comment>
</owl:Class>

<owl:Class rdf:ID= "Song">
<rdfs:subClassOf rdf:resource ="#MusicalComposition"/>
<rdfs:comment>Any MusicalComposition which contains Lyrics.</rdfs:comment>
</owl:Class>

<owl:Class rdf:ID= "SoupStock">
<rdfs:subClassOf rdf:resource ="#PreparedFood"/>
<rdfs:comment>Food which is prepared by reducing Meat
and/or FruitOrVegetables to a translucent broth which can be used as
a base for soups or sauces.</rdfs:comment>
</owl:Class>

<owl:Class rdf:ID= "SpaceRegion">
<rdfs:subClassOf rdf:resource ="http://127.0.0.1:8000/ontology/SUMO.owl#Region"/>
<sumo:disjoint rdf:resource = 
"http://127.0.0.1:8000/ontology/SUMO.owl#GeographicArea" />
<rdfs:comment>The class of all Regions which are not
GeographicAreas.</rdfs:comment>
</owl:Class>

<owl:Class rdf:ID= "SpaceTransportation">
<rdfs:subClassOf rdf:resource 
="http://127.0.0.1:8000/ontology/SUMO.owl#Transportation"/>
<rdfs:comment>Any instance of Transportation where the
instrument is a Spacecraft and which is through a 
SpaceRegion.</rdfs:comment>
</owl:Class>

<owl:Class rdf:ID= "Spacecraft">
<rdfs:subClassOf rdf:resource 
="http://127.0.0.1:8000/ontology/SUMO.owl#Vehicle"/>
<rdfs:comment>Any Vehicle which is capable of
SpaceTransportation.</rdfs:comment>
</owl:Class>

<owl:Class rdf:ID= "Spear">
<rdfs:subClassOf rdf:resource ="http://127.0.0.1:8000/ontology/SUMO.owl#Weapon"/>
<rdfs:comment>A Weapon with a long handle and a short
blade.</rdfs:comment>
</owl:Class>

<owl:Class rdf:ID= "Sphere">
<rdfs:subClassOf rdf:resource 
="http://127.0.0.1:8000/ontology/SUMO.owl#ThreeDimensionalFigure"/>
<rdfs:comment>The class of ThreeDimensionalFigures such that
all GeometricPoints that make up the Sphere are equidistant from a
single GeometricPoint, known as the center of the Sphere.</rdfs:comment>
</owl:Class>

<owl:Class rdf:ID= "SpinalColumn">
<rdfs:subClassOf rdf:resource ="http://127.0.0.1:8000/ontology/SUMO.owl#Bone"/>
<rdfs:comment>A flexible column made out of bones called
vertebrae. The main function of the SpinalColumn is to protect the
spinal cord.</rdfs:comment>
</owl:Class>

<owl:Class rdf:ID= "SpinalCord">
<rdfs:subClassOf rdf:resource ="http://127.0.0.1:8000/ontology/SUMO.owl#Organ"/>
<rdfs:comment>A cord of nerves that carries impulses to
and from the Brain.  It is contained within the SpinalColumn.</rdfs:comment>
</owl:Class>

<owl:Class rdf:ID= "Spitting">
<rdfs:subClassOf rdf:resource 
="http://127.0.0.1:8000/ontology/SUMO.owl#Impelling"/>
<rdfs:comment>Any instance of Impelling where the origin is
the Mouth of the agent.</rdfs:comment>
</owl:Class>

<owl:Class rdf:ID= "Spleen">
<rdfs:subClassOf rdf:resource ="http://127.0.0.1:8000/ontology/SUMO.owl#Organ"/>
<rdfs:subClassOf rdf:resource 
="http://127.0.0.1:8000/ontology/SUMO.owl#AnimalAnatomicalStructure"/>
<rdfs:comment>An Organ on the left side of the body that produces
Cells that play a crucial role in immune response.</rdfs:comment>
</owl:Class>

<owl:Class rdf:ID= "SportServe">
<rdfs:subClassOf rdf:resource ="#GameShot"/>
<rdfs:comment>A GameShot which is part of a Sport and
which serves to start the Sport, e.g. the beginning shot in Tennis,
Badminton or Squash.</rdfs:comment>
</owl:Class>

<owl:Class rdf:ID= "SportsAttribute">
<rdfs:subClassOf rdf:resource ="#GameAttribute"/>
<rdfs:comment>Any GameAttribute that is specific to
a Sport.</rdfs:comment>
</owl:Class>

<owl:Class rdf:ID= "SportsFacility">
<rdfs:subClassOf rdf:resource 
="http://127.0.0.1:8000/ontology/SUMO.owl#StationaryArtifact"/>
<rdfs:comment>A specially designated and maintained facility
where Sports are played.  Note that this covers sports fields, stadiums,
and gymnasiums.</rdfs:comment>
</owl:Class>

<owl:Class rdf:ID= "SportsLeague">
<rdfs:subClassOf rdf:resource 
="http://127.0.0.1:8000/ontology/SUMO.owl#Organization"/>
<rdfs:comment>An Organization whose members are SportsTeams
and whose purpose is to set up games between its members.</rdfs:comment>
</owl:Class>

<owl:Class rdf:ID= "SportsPlay">
<rdfs:subClassOf rdf:resource ="http://127.0.0.1:8000/ontology/SUMO.owl#Plan"/>
<rdfs:comment>A Plan for a Maneuver within a TeamSport.</rdfs:comment>
</owl:Class>

<owl:Class rdf:ID= "SportsPosition">
<rdfs:subClassOf rdf:resource ="#SkilledOccupation"/>
<rdfs:comment>A Position which is filled by someone on a
SportsTeam and which represents the role played by the person on the 
team.</rdfs:comment>
</owl:Class>

<owl:Class rdf:ID= "SportsTeam">
<rdfs:subClassOf rdf:resource 
="http://127.0.0.1:8000/ontology/SUMO.owl#Organization"/>
<rdfs:comment>An Organization which habitually plays a Sport
together, either as an occupation or as a leisure activity.</rdfs:comment>
</owl:Class>

<owl:Class rdf:ID= "Spraying">
<rdfs:subClassOf rdf:resource 
="http://127.0.0.1:8000/ontology/SUMO.owl#LiquidMotion"/>
<rdfs:subClassOf rdf:resource 
="http://127.0.0.1:8000/ontology/SUMO.owl#Transfer"/>
<rdfs:comment>Any instance of Transfer of a Liquid which is
accomplished by converting the Liquid into a mist.</rdfs:comment>
</owl:Class>

<owl:Class rdf:ID= "SpringSeason">
<rdfs:subClassOf rdf:resource ="#SeasonOfYear"/>
<rdfs:comment>The SeasonOfYear that begins at the spring
equinox and ends at the summer solstice.</rdfs:comment>
</owl:Class>

<owl:Class rdf:ID= "Square">
<rdfs:subClassOf rdf:resource ="#Rectangle"/>
<rdfs:comment>Any Rectangle whose sides are all equal.</rdfs:comment>
</owl:Class>

<owl:Class rdf:ID= "SquareMeter">
<rdf:type rdf:resource = 
"http://127.0.0.1:8000/ontology/SUMO.owl#UnitOfMeasure"/>
<rdfs:subClassOf rdf:resource 
="http://127.0.0.1:8000/ontology/SUMO.owl#AreaMeasure"/>
<rdfs:comment>SquareMeter represents a UnitOfMeasure
equal to one square Meter.</rdfs:comment>
</owl:Class>

<owl:Class rdf:ID= "SquareMile">
<rdf:type rdf:resource = 
"http://127.0.0.1:8000/ontology/SUMO.owl#UnitOfMeasure"/>
<rdfs:subClassOf rdf:resource 
="http://127.0.0.1:8000/ontology/SUMO.owl#AreaMeasure"/>
<rdfs:comment>SquareMile represents a UnitOfMeasure
equal to one square Mile.</rdfs:comment>
</owl:Class>

<owl:Class rdf:ID= "SquareYard">
<rdf:type rdf:resource = 
"http://127.0.0.1:8000/ontology/SUMO.owl#UnitOfMeasure"/>
<rdfs:subClassOf rdf:resource 
="http://127.0.0.1:8000/ontology/SUMO.owl#AreaMeasure"/>
<rdfs:comment>SquareYard represents a UnitOfMeasure
equal to one square YardLength.</rdfs:comment>
</owl:Class>

<owl:Class rdf:ID= "Squirrel">
<rdfs:subClassOf rdf:resource ="http://127.0.0.1:8000/ontology/SUMO.owl#Rodent"/>
<rdfs:comment>A tree-dwelling Rodent with a bushy tail.</rdfs:comment>
</owl:Class>

<owl:Class rdf:ID= "StageCoach">
<rdfs:subClassOf rdf:resource ="#Wagon"/>
<rdfs:comment>A Wagon that is pulled by Horses and whose purpose
was to transport Humans and their luggage from one City to the next, 
especially
in areas which did not have an established transportation system, e.g. the 
old west.</rdfs:comment>
</owl:Class>

<owl:Class rdf:ID= "Stairway">
<rdfs:subClassOf rdf:resource 
="http://127.0.0.1:8000/ontology/SUMO.owl#StationaryArtifact"/>
<rdfs:comment>A StationaryArtifact which allows one to climb, step
by step, from one level to another.</rdfs:comment>
</owl:Class>

<owl:Class rdf:ID= "StandardBearer">
<rdfs:subClassOf rdf:resource ="#Soldier"/>
<rdfs:comment>Any Soldier who is tasked with carrying the colors of
his/her unit in Battles and parades.</rdfs:comment>
</owl:Class>

<owl:Class rdf:ID= "StandingUp">
<rdfs:subClassOf rdf:resource 
="http://127.0.0.1:8000/ontology/SUMO.owl#BodyMotion"/>
<rdfs:comment>The BodyMotion of moving from a Sitting
to a Standing position.</rdfs:comment>
</owl:Class>

<owl:Class rdf:ID= "Star">
<rdfs:subClassOf rdf:resource 
="http://127.0.0.1:8000/ontology/SUMO.owl#AstronomicalBody"/>
<rdfs:comment>Star is the class of hot gaseous astronomical 
bodies.</rdfs:comment>
</owl:Class>

<owl:Class rdf:ID= "Starch">
<rdfs:subClassOf rdf:resource 
="http://127.0.0.1:8000/ontology/SUMO.owl#Carbohydrate"/>
<rdfs:comment>A complex Carbohydrate that is the main form in
which Carbohydrates are stored.</rdfs:comment>
</owl:Class>

<owl:Class rdf:ID= "Starving">
<rdfs:subClassOf rdf:resource 
="http://127.0.0.1:8000/ontology/SUMO.owl#Killing"/>
<rdfs:comment>Killing someone by depriving them of Food.</rdfs:comment>
</owl:Class>

<owl:Class rdf:ID= "StateGovernment">
<rdfs:subClassOf rdf:resource 
="http://127.0.0.1:8000/ontology/SUMO.owl#Government"/>
<rdfs:comment>The class of Governments whose
jurisdictions are StateOrProvinces.</rdfs:comment>
</owl:Class>

<owl:Class rdf:ID= "Statement">
<rdfs:subClassOf rdf:resource 
="http://127.0.0.1:8000/ontology/SUMO.owl#Sentence"/>
<rdfs:comment>A Sentence that is stated to be true.</rdfs:comment>
</owl:Class>

<owl:Class rdf:ID= "Stealing">
<rdfs:subClassOf rdf:resource 
="http://127.0.0.1:8000/ontology/SUMO.owl#UnilateralGetting"/>
<rdfs:subClassOf rdf:resource ="#CriminalAction"/>
<rdfs:comment>Any UnilateralGetting which is not permitted by the
origin of the UnilateralGetting.  These cases of UnilateralGetting are
distinguished from ones where the destination is the subject of charity or
other forms of benefaction.</rdfs:comment>
</owl:Class>

<owl:Class rdf:ID= "SteamEngine">
<rdfs:subClassOf rdf:resource ="#Engine"/>
<rdfs:comment>SteamEngine is the subclass of Engines
that produce mechanical power from heat and steam pressure.</rdfs:comment>
</owl:Class>

<owl:Class rdf:ID= "Steel">
<rdfs:subClassOf rdf:resource ="#MetallicAlloy"/>
<rdfs:comment>A MetallicAlloy made from Iron and other 
elements.</rdfs:comment>
</owl:Class>

<owl:Class rdf:ID= "Steeple">
<rdfs:subClassOf rdf:resource 
="http://127.0.0.1:8000/ontology/SUMO.owl#StationaryArtifact"/>
<rdfs:comment>A component of a ReligiousBuilding that is tall
and narrow and symbolizes the connection between humanity and a 
deity.</rdfs:comment>
</owl:Class>

<owl:Class rdf:ID= "SteeringWheel">
<rdfs:subClassOf rdf:resource ="#VehicleController"/>
<rdfs:comment>A VehicleController which enables one to steer
a Vehicle.</rdfs:comment>
</owl:Class>

<owl:Class rdf:ID= "SteppeClimateZone">
<rdfs:subClassOf rdf:resource ="#AridClimateZone"/>
<rdfs:comment>SteppeClimateZone
is the class of AridClimateZones where the dominant
vegetation type is grasses, with no trees.  Koeppen
system 'BS'.</rdfs:comment>
</owl:Class>

<owl:Class rdf:ID= "Stepping">
<rdfs:subClassOf rdf:resource 
="http://127.0.0.1:8000/ontology/SUMO.owl#BodyMotion"/>
<rdfs:comment>The BodyMotion of extending one foot forward
and then bringing the other foot to the same lateral position as the
first leg.</rdfs:comment>
</owl:Class>

<owl:Class rdf:ID= "Steroid">
<rdfs:subClassOf rdf:resource ="#OrganicCompound"/>
<rdfs:subClassOf rdf:resource 
="http://127.0.0.1:8000/ontology/SUMO.owl#BiologicallyActiveSubstance"/>
<rdfs:comment>A class of OrganicCompounds having the same basic
chemical structure and having significant physiological 
effects.</rdfs:comment>
</owl:Class>

<owl:Class rdf:ID= "Stimulant">
<rdfs:subClassOf rdf:resource 
="http://127.0.0.1:8000/ontology/SUMO.owl#BiologicallyActiveSubstance"/>
<sumo:disjoint rdf:resource = "#Depressant" />
<rdfs:comment>Any BiologicallyActiveSubstance which has
the effect of stimulating the central nervous system, i.e. increasing
function or activity in the Brain or SpinalCord.</rdfs:comment>
</owl:Class>

<owl:Class rdf:ID= "Stirring">
<rdfs:subClassOf rdf:resource 
="http://127.0.0.1:8000/ontology/SUMO.owl#LiquidMotion"/>
<rdfs:subClassOf rdf:resource 
="http://127.0.0.1:8000/ontology/SUMO.owl#Combining"/>
<rdfs:comment>Any instance of LiquidMotion which is also an
instance of Combining two or more Liquids.</rdfs:comment>
</owl:Class>

<owl:Class rdf:ID= "Stock">
<rdfs:subClassOf rdf:resource 
="http://127.0.0.1:8000/ontology/SUMO.owl#FinancialInstrument"/>
<rdfs:comment>An instrument that signifies an ownership position,
or equity, in a Corporation, and represents a claim on its proportionate
share in the corporation's assets and profits.</rdfs:comment>
</owl:Class>

<owl:Class rdf:ID= "StockMarket">
<rdfs:subClassOf rdf:resource 
="http://127.0.0.1:8000/ontology/SUMO.owl#Organization"/>
<rdfs:comment>General term for organizations where stocks are traded,
either in formal exchanges or over-the-counter.</rdfs:comment>
</owl:Class>

<owl:Class rdf:ID= "Stomach">
<rdfs:subClassOf rdf:resource ="http://127.0.0.1:8000/ontology/SUMO.owl#Organ"/>
<rdfs:subClassOf rdf:resource 
="http://127.0.0.1:8000/ontology/SUMO.owl#AnimalAnatomicalStructure"/>
<rdfs:comment>A muscular sac that is the principal organ of
digestion.</rdfs:comment>
</owl:Class>

<owl:Class rdf:ID= "Store">
<rdfs:subClassOf rdf:resource 
="http://127.0.0.1:8000/ontology/SUMO.owl#Building"/>
<rdfs:comment>A Building that has the purpose of housing
FinancialTransactions.</rdfs:comment>
</owl:Class>

<owl:Class rdf:ID= "StormFront">
<rdfs:subClassOf rdf:resource ="#AtmosphericRegion"/>
<rdfs:comment>The Region where two or more unstable air
masses meet.</rdfs:comment>
</owl:Class>

<owl:Class rdf:ID= "Stove">
<rdfs:subClassOf rdf:resource ="#HeatingDevice"/>
<rdfs:comment>A HeatingDevice which consists one or more burners for
heating pots and pans of Food.</rdfs:comment>
</owl:Class>

<owl:Class rdf:ID= "Strait">
<rdfs:subClassOf rdf:resource ="#BodyOfWater"/>
<rdfs:comment>Strait is the subclass of BodyOfWater that
consists of narrow water areas connecting two larger bodies of water.
Straits are naturally occurring bodies of water.</rdfs:comment>
</owl:Class>

<owl:Class rdf:ID= "Strangling">
<rdfs:subClassOf rdf:resource 
="http://127.0.0.1:8000/ontology/SUMO.owl#Grabbing"/>
<rdfs:comment>Any instance of Grabbing where the patient is
someone else's throat and the intention is to make it impossible for the 
other
person to breathe.</rdfs:comment>
</owl:Class>

<owl:Class rdf:ID= "Streetcar">
<rdfs:subClassOf rdf:resource ="#ElectrifiedRailwayCar"/>
<rdfs:comment>Streetcar is the subclass of
ElectrifiedRailwayCars that run on tracks laid into, along, or
beside city Streets.</rdfs:comment>
</owl:Class>

<owl:Class rdf:ID= "Stretching">
<rdfs:subClassOf rdf:resource ="#Lengthening"/>
<rdfs:comment>Lengthening an object by pulling two sides
of it in opposite directions.</rdfs:comment>
</owl:Class>

<owl:Class rdf:ID= "String">
<rdfs:subClassOf rdf:resource 
="http://127.0.0.1:8000/ontology/SUMO.owl#Artifact"/>
<rdfs:comment>A long, thin strand of Fabric that is used for Tying
things together, etc.  Note that this class covers a cord of any width, 
including
rope, twine, and thread, for example.</rdfs:comment>
</owl:Class>

<owl:Class rdf:ID= "StringInstrument">
<rdfs:subClassOf rdf:resource 
="http://127.0.0.1:8000/ontology/SUMO.owl#MusicalInstrument"/>
<rdfs:comment>A MusicalInstrument which is played by
striking strings, either directly as with a guitar or indirectly via keys
as with Pianos.</rdfs:comment>
</owl:Class>

<owl:Class rdf:ID= "Submarine">
<rdfs:subClassOf rdf:resource ="#Watercraft"/>
<rdfs:comment>A Watercraft which is capable of travelling
under the water level by filling tanks water.</rdfs:comment>
</owl:Class>

<owl:Class rdf:ID= "SubtropicalDesertClimateZone">
<rdfs:subClassOf rdf:resource ="#DesertClimateZone"/>
<rdfs:comment>SubtropicalDesertClimateZone is a subclass of 
DesertClimateZone
that is characterized by an average temperature greater than 18
degrees Celsius, as well as very low rainfall.  This is Koeppen
system 'BWh'.</rdfs:comment>
</owl:Class>

<owl:Class rdf:ID= "SubwaySystem">
<rdfs:subClassOf rdf:resource ="#RailTransportationSystem"/>
<rdfs:comment>Any RailTransportationSystem that runs
exclusively through Tunnels.</rdfs:comment>
</owl:Class>

<owl:Class rdf:ID= "Suffocating">
<rdfs:subClassOf rdf:resource 
="http://127.0.0.1:8000/ontology/SUMO.owl#Killing"/>
<rdfs:comment>Killing someone by asphyxiation, i.e. by
depriving them of oxygen.</rdfs:comment>
</owl:Class>

<owl:Class rdf:ID= "Sugar">
<rdfs:subClassOf rdf:resource 
="http://127.0.0.1:8000/ontology/SUMO.owl#Carbohydrate"/>
<rdfs:comment>A simple Carbohydrate that has a sweet taste and
consists mostly or entirely of sucrose.</rdfs:comment>
</owl:Class>

<owl:Class rdf:ID= "Suicide">
<rdfs:subClassOf rdf:resource 
="http://127.0.0.1:8000/ontology/SUMO.owl#Killing"/>
<rdfs:comment>Any instance of Killing where the agent and
the patient are identical.</rdfs:comment>
</owl:Class>

<owl:Class rdf:ID= "SummerSeason">
<rdfs:subClassOf rdf:resource ="#SeasonOfYear"/>
<rdfs:comment>The SeasonOfYear that begins at the summer
solstice and ends at the autumnal equinox.</rdfs:comment>
</owl:Class>

<owl:Class rdf:ID= "Sunlight">
<rdfs:subClassOf rdf:resource 
="http://127.0.0.1:8000/ontology/SUMO.owl#RadiatingLight"/>
<rdfs:comment>Any instance of RadiatingLight where the
Sun (Sol) is the origin.</rdfs:comment>
</owl:Class>

<owl:Class rdf:ID= "Sunrise">
<rdfs:subClassOf rdf:resource 
="http://127.0.0.1:8000/ontology/SUMO.owl#TimeInterval"/>
<rdfs:comment>The TimeInterval of each Day when the sun is rising
and is partially overlapped by the horizon line.</rdfs:comment>
</owl:Class>

<owl:Class rdf:ID= "Sunset">
<rdfs:subClassOf rdf:resource 
="http://127.0.0.1:8000/ontology/SUMO.owl#TimeInterval"/>
<rdfs:comment>The TimeInterval of each Day when the sun is setting
and is partially overlapped by the horizon line.</rdfs:comment>
</owl:Class>

<owl:Class rdf:ID= "Supposition">
<rdfs:subClassOf rdf:resource 
="http://127.0.0.1:8000/ontology/SUMO.owl#Sentence"/>
<rdfs:comment>A Sentence that is assumed to be true, possibly
just for the sake of argument.</rdfs:comment>
</owl:Class>

<owl:Class rdf:ID= "SurfacedRoadway">
<rdfs:subClassOf rdf:resource 
="http://127.0.0.1:8000/ontology/SUMO.owl#Roadway"/>
<sumo:disjoint rdf:resource = "#UnsurfacedRoadway" />
<rdfs:comment>SurfacedRoadway is the subclass of
Roadways that have been improved by covering them with a substance
to increase the hardness and smoothness of the surface.  Covering
materials include pavement, concrete, asphalt, macadam, and 
gravel.</rdfs:comment>
</owl:Class>

<owl:Class rdf:ID= "Surgeon">
<rdfs:subClassOf rdf:resource ="#MedicalDoctor"/>
<rdfs:comment>The Profession of being a surgeon, i.e. being a
medical doctor who specializes in performing surgical 
operations.</rdfs:comment>
</owl:Class>

<owl:Class rdf:ID= "Swamp">
<rdfs:subClassOf rdf:resource 
="http://127.0.0.1:8000/ontology/SUMO.owl#StaticWaterArea"/>
<rdfs:comment>Swamp is a subclass of StaticWaterAreas that are
stagnant and relatively shallow.  They are situated in low, wet land with
grasses and possibly trees as vegetation.</rdfs:comment>
</owl:Class>

<owl:Class rdf:ID= "Sweat">
<rdfs:subClassOf rdf:resource 
="http://127.0.0.1:8000/ontology/SUMO.owl#AnimalSubstance"/>
<rdfs:comment>An AnimalSubstance that contains SodiumChloride
and is produced by the sweat glands.</rdfs:comment>
</owl:Class>

<owl:Class rdf:ID= "Sweeping">
<rdfs:subClassOf rdf:resource 
="http://127.0.0.1:8000/ontology/SUMO.owl#Removing"/>
<rdfs:comment>Removing small particles from the floor by means of
a Broom.</rdfs:comment>
</owl:Class>

<owl:Class rdf:ID= "Swimming">
<rdfs:subClassOf rdf:resource 
="http://127.0.0.1:8000/ontology/SUMO.owl#BodyMotion"/>
<rdfs:comment>Any deliberate and controlled BodyMotion
through water that is accomplished by an Organism.</rdfs:comment>
</owl:Class>

<owl:Class rdf:ID= "SwimmingPool">
<rdfs:subClassOf rdf:resource ="#FluidContainer"/>
<rdfs:subClassOf rdf:resource 
="http://127.0.0.1:8000/ontology/SUMO.owl#StationaryArtifact"/>
<rdfs:comment>A FluidContainer that is filled with Water
and that is used for Swimming.</rdfs:comment>
</owl:Class>

<owl:Class rdf:ID= "SwitchDevice">
<rdfs:subClassOf rdf:resource 
="http://127.0.0.1:8000/ontology/SUMO.owl#EngineeringComponent"/>
<rdfs:comment>An EngineeringComponent which is capable of turning
an ElectricDevice on and off.</rdfs:comment>
</owl:Class>

<owl:Class rdf:ID= "Sword">
<rdfs:subClassOf rdf:resource ="http://127.0.0.1:8000/ontology/SUMO.owl#Weapon"/>
<rdfs:comment>A Weapon with a long blade and covered
handle.</rdfs:comment>
</owl:Class>

<owl:Class rdf:ID= "Syllable">
<rdfs:subClassOf rdf:resource 
="http://127.0.0.1:8000/ontology/SUMO.owl#SymbolicString"/>
<rdfs:comment>A sequence of Characters from the same Word
that denote a single sound.</rdfs:comment>
</owl:Class>

<owl:Class rdf:ID= "Table">
<rdfs:subClassOf rdf:resource ="#Furniture"/>
<rdfs:comment>A piece of Furniture that is elevated from the floor
and has a flat top.  It is used for eating, paperwork, manual work, 
meetings,
etc.</rdfs:comment>
</owl:Class>

<owl:Class rdf:ID= "Tableware">
<rdfs:subClassOf rdf:resource ="http://127.0.0.1:8000/ontology/SUMO.owl#Device"/>
<rdfs:comment>Devices that are used in Ingesting (Eating
and/or Drinking) a meal.  This coves dishware, flatware, and 
glassware.</rdfs:comment>
</owl:Class>

<owl:Class rdf:ID= "Tail">
<rdfs:subClassOf rdf:resource 
="http://127.0.0.1:8000/ontology/SUMO.owl#AnimalAnatomicalStructure"/>
<rdfs:comment>A BodyPart which extends from the rear of the
main body of some Vertebrates.</rdfs:comment>
</owl:Class>

<owl:Class rdf:ID= "Taillight">
<rdfs:subClassOf rdf:resource ="#VehicleLight"/>
<rdfs:comment>Any VehicleLight which is attached to the back
of a Vehicle.</rdfs:comment>
</owl:Class>

<owl:Class rdf:ID= "TakingIll">
<rdfs:subClassOf rdf:resource 
="http://127.0.0.1:8000/ontology/SUMO.owl#PathologicProcess"/>
<rdfs:comment>Any Process where the experiencer contracts a
DiseaseOrSyndrome.</rdfs:comment>
</owl:Class>

<owl:Class rdf:ID= "TakingOff">
<rdfs:subClassOf rdf:resource 
="http://127.0.0.1:8000/ontology/SUMO.owl#Translocation"/>
<rdfs:comment>Any instance of Translocation which starts
on something other than an AtmosphericRegion and which has an instance
of Flying as a subProcess.</rdfs:comment>
</owl:Class>

<owl:Class rdf:ID= "Tape">
<rdfs:subClassOf rdf:resource 
="http://127.0.0.1:8000/ontology/SUMO.owl#AttachingDevice"/>
<rdfs:comment>A thin strip of Fabric or Paper that is used to attach
two things.</rdfs:comment>
</owl:Class>

<owl:Class rdf:ID= "Tavern">
<rdfs:subClassOf rdf:resource ="#Restaurant"/>
<rdfs:comment>A Restaurant whose primary service is selling
AlcoholicBeverages to customers.</rdfs:comment>
</owl:Class>

<owl:Class rdf:ID= "Tax">
<rdfs:subClassOf rdf:resource ="#ChargingAFee"/>
<rdfs:comment>A fee charged by a government on a product, income
or activity.</rdfs:comment>
</owl:Class>

<owl:Class rdf:ID= "TaxReturn">
<rdfs:subClassOf rdf:resource ="#FormText"/>
<rdfs:comment>A FormText that is used for calculating the amount
of income tax owed in a given year.</rdfs:comment>
</owl:Class>

<owl:Class rdf:ID= "Taxicab">
<rdfs:subClassOf rdf:resource ="#Automobile"/>
<rdfs:comment>An Automobile which is used to transport people
on short trips in exchange for a fare.</rdfs:comment>
</owl:Class>

<owl:Class rdf:ID= "Tea">
<rdfs:subClassOf rdf:resource 
="http://127.0.0.1:8000/ontology/SUMO.owl#Beverage"/>
<rdfs:subClassOf rdf:resource ="#PreparedFood"/>
<rdfs:comment>A Beverage which is prepared by infusing tea leaves
into hot water.</rdfs:comment>
</owl:Class>

<owl:Class rdf:ID= "Teacher">
<rdfs:subClassOf rdf:resource ="#Profession"/>
<rdfs:comment>The Profession of being a teacher.</rdfs:comment>
</owl:Class>

<owl:Class rdf:ID= "TeamSport">
<rdfs:subClassOf rdf:resource ="http://127.0.0.1:8000/ontology/SUMO.owl#Sport"/>
<rdfs:comment>Any Sport which is played by SportsTeams, e.g.
Baseball and Football.</rdfs:comment>
</owl:Class>

<owl:Class rdf:ID= "TearSubstance">
<rdfs:subClassOf rdf:resource ="#LiquidBodySubstance"/>
<rdfs:subClassOf rdf:resource ="#SalineSolution"/>
<rdfs:comment>The class of SalineSolutions produced by
the lacrimal glands of the Eyes.</rdfs:comment>
</owl:Class>

<owl:Class rdf:ID= "Teenager">
<rdfs:subClassOf rdf:resource ="#HumanYouth"/>
<rdfs:comment>A HumanYouth between puberty and the age of 19.</rdfs:comment>
</owl:Class>

<owl:Class rdf:ID= "Telegraph">
<rdfs:subClassOf rdf:resource ="#ElectricDevice"/>
<rdfs:subClassOf rdf:resource ="#CommunicationDevice"/>
<rdfs:comment>A Device that permits LinguisticCommunication
between remote points by means of a code of aural dots and dashes that can
be converted into letters of an alphabet.</rdfs:comment>
</owl:Class>

<owl:Class rdf:ID= "Telephone">
<rdfs:subClassOf rdf:resource ="#ElectricDevice"/>
<rdfs:subClassOf rdf:resource ="#CommunicationDevice"/>
<rdfs:comment>A Device that permits LinguisticCommunication
between remote points by converting sound into electrical signals that are
then transmitted.  When the signals are received, they are converted back
into sound.</rdfs:comment>
</owl:Class>

<owl:Class rdf:ID= "TelephoneLine">
<rdfs:subClassOf rdf:resource ="#WireLine"/>
<rdfs:comment>A WireLine that carries telephone signals and
allows users of Telephones or Telegraphs to communicate with one 
another.</rdfs:comment>
</owl:Class>

<owl:Class rdf:ID= "Telephoning">
<rdfs:subClassOf rdf:resource 
="http://127.0.0.1:8000/ontology/SUMO.owl#Speaking"/>
<rdfs:comment>Any instance of Speaking where the
instrument of Communication is a Telephone.</rdfs:comment>
</owl:Class>

<owl:Class rdf:ID= "TelevisionBroadcasting">
<rdfs:subClassOf rdf:resource ="#Broadcasting"/>
<rdfs:comment>Any instance of Broadcasting which
is intended to be received by a TelevisionReceiver.</rdfs:comment>
</owl:Class>

<owl:Class rdf:ID= "TelevisionReceiver">
<rdfs:subClassOf rdf:resource ="#ReceiverDevice"/>
<rdfs:comment>A TelevisionReceiver is a Device for
receiving television broadcast signals from a 
TelevisionStation.</rdfs:comment>
</owl:Class>

<owl:Class rdf:ID= "TelevisionStation">
<rdfs:subClassOf rdf:resource ="#BroadcastingStation"/>
<rdfs:comment>A TelevisionStation is a
BroadcastingStation that broadcasts programs that are intended to be
received by a TelevisionReceiver.</rdfs:comment>
</owl:Class>

<owl:Class rdf:ID= "TellingALie">
<rdfs:subClassOf rdf:resource 
="http://127.0.0.1:8000/ontology/SUMO.owl#Stating"/>
<rdfs:comment>Any Stating which is both False and believed
to be False by the agent of the Stating.</rdfs:comment>
</owl:Class>

<owl:Class rdf:ID= "TemperateClimateZone">
<rdfs:subClassOf rdf:resource ="#ClimateZone"/>
<rdfs:comment>TemperateClimateZone is the
subclass of ClimateZone whose warmest month has an average
temperature greater than 10 degrees Celsius and whose coolest month
has an average temperature between 18 degrees and -3 degrees Celsius.
This is Class C in the Koeppen climate system.</rdfs:comment>
</owl:Class>

<owl:Class rdf:ID= "TemperateSummerDryClimateZone">
<rdfs:subClassOf rdf:resource ="#TemperateClimateZone"/>
<rdfs:comment>TemperateSummerDryClimateZone is the subclass of 
TemperateClimateZone
that is characterized by dry summers, and in which the wettest winter month
has at least three times the moisture of the driest summer month.  The
driest month has less than an average of 30 mm of precipitation.  Koeppen
climate system type 'Cs'.</rdfs:comment>
</owl:Class>

<owl:Class rdf:ID= "TemperateWinterDryClimateZone">
<rdfs:subClassOf rdf:resource ="#TemperateClimateZone"/>
<rdfs:comment>TemperateWinterDryClimateZone is a subclass of 
TemperateClimateZone
characterized by having at least 10 times as much precipitation in the
wettest summer month as in the driest winter month. Koeppen climate
system type 'Cw'.</rdfs:comment>
</owl:Class>

<owl:Class rdf:ID= "Tendon">
<rdfs:subClassOf rdf:resource ="http://127.0.0.1:8000/ontology/SUMO.owl#Tissue"/>
<rdfs:subClassOf rdf:resource 
="http://127.0.0.1:8000/ontology/SUMO.owl#AnimalSubstance"/>
<rdfs:comment>Tissue that connects Muscle to Bone.</rdfs:comment>
</owl:Class>

<owl:Class rdf:ID= "Tent">
<rdfs:subClassOf rdf:resource ="#MobileResidence"/>
<rdfs:comment>A MobileResidence that is made of Fabric and poles and
can be easily assembled and disassembled.</rdfs:comment>
</owl:Class>

<owl:Class rdf:ID= "TerminalBuilding">
<rdfs:subClassOf rdf:resource 
="http://127.0.0.1:8000/ontology/SUMO.owl#Building"/>
<rdfs:comment>A TerminalBuilding is a Building
located at a TransitTerminal and used in connection with its
functions.</rdfs:comment>
</owl:Class>

<owl:Class rdf:ID= "Tesla">
<rdfs:subClassOf rdf:resource 
="http://127.0.0.1:8000/ontology/SUMO.owl#FunctionQuantity"/>
<rdf:type rdf:resource = 
"http://127.0.0.1:8000/ontology/SUMO.owl#SystemeInternationalUnit"/>
<rdfs:comment>SI magnetic flux density measure.  Symbol:  T.
One Tesla equals one Weber per square Meter.  Tesla = Wb/m^2 =
kg*s^(-2)*A^(-1).</rdfs:comment>
</owl:Class>

<owl:Class rdf:ID= "TestForm">
<rdfs:subClassOf rdf:resource ="#FormText"/>
<rdfs:subClassOf rdf:resource 
="http://127.0.0.1:8000/ontology/SUMO.owl#MeasuringDevice"/>
<rdfs:comment>A FormText which is intended to measure some aspect
of the cognitive capabilities, e.g. intelligence or knowledge of a domain,
of the person taking the test.</rdfs:comment>
</owl:Class>

<owl:Class rdf:ID= "Testament">
<rdfs:subClassOf rdf:resource 
="http://127.0.0.1:8000/ontology/SUMO.owl#Certificate"/>
<rdfs:comment>A Certificate that describes how a person's
property is to be distributed after the death of the person.</rdfs:comment>
</owl:Class>

<owl:Class rdf:ID= "Testifying">
<rdfs:subClassOf rdf:resource 
="http://127.0.0.1:8000/ontology/SUMO.owl#Stating"/>
<rdfs:comment>Giving testimony as part of a JudicialProcess.</rdfs:comment>
</owl:Class>

<owl:Class rdf:ID= "Thanking">
<rdfs:subClassOf rdf:resource ="#ExpressingApproval"/>
<rdfs:comment>Any ExpressingApproval to a person for something
that the person did in the past and that is regarded as being to the 
thanker's
benefit.</rdfs:comment>
</owl:Class>

<owl:Class rdf:ID= "TheaterProfession">
<rdfs:subClassOf rdf:resource ="#EntertainmentProfession"/>
<rdfs:comment>Often know as the stage, Positions which
involve performing live plays.</rdfs:comment>
</owl:Class>

<owl:Class rdf:ID= "Thermometer">
<rdfs:subClassOf rdf:resource 
="http://127.0.0.1:8000/ontology/SUMO.owl#MeasuringDevice"/>
<rdfs:comment>Any Device that measures and represents
TemperatureMeasure.</rdfs:comment>
</owl:Class>

<owl:Class rdf:ID= "Threatening">
<rdfs:subClassOf rdf:resource 
="http://127.0.0.1:8000/ontology/SUMO.owl#Committing"/>
<rdfs:comment>Any Committing where the thing promised
is something that is deemed undesirable by the destination of the
Committing.</rdfs:comment>
</owl:Class>

<owl:Class rdf:ID= "Throat">
<rdfs:subClassOf rdf:resource 
="http://127.0.0.1:8000/ontology/SUMO.owl#AnimalAnatomicalStructure"/>
<rdfs:subClassOf rdf:resource 
="http://127.0.0.1:8000/ontology/SUMO.owl#BodyVessel"/>
<rdfs:comment>A BodyVessel which connects the Mouth to the
lungs and stomach.</rdfs:comment>
</owl:Class>

<owl:Class rdf:ID= "Throwing">
<rdfs:subClassOf rdf:resource 
="http://127.0.0.1:8000/ontology/SUMO.owl#Impelling"/>
<rdfs:subClassOf rdf:resource 
="http://127.0.0.1:8000/ontology/SUMO.owl#BodyMotion"/>
<rdfs:comment>Any instance of Impelling where the instrument is
an Arm.</rdfs:comment>
</owl:Class>

<owl:Class rdf:ID= "Thumb">
<rdfs:subClassOf rdf:resource ="#Finger"/>
<rdfs:comment>The thick, short Finger of each Hand.</rdfs:comment>
</owl:Class>

<owl:Class rdf:ID= "Thunder">
<rdfs:subClassOf rdf:resource 
="http://127.0.0.1:8000/ontology/SUMO.owl#WeatherProcess"/>
<rdfs:subClassOf rdf:resource 
="http://127.0.0.1:8000/ontology/SUMO.owl#RadiatingSound"/>
<rdfs:comment>Any instance of RadiatingSound which is caused by
an instance of Lightning.</rdfs:comment>
</owl:Class>

<owl:Class rdf:ID= "ThyroidGland">
<rdfs:subClassOf rdf:resource ="#Gland"/>
<rdfs:comment>A Gland in the neck that produces
ThyroidHormone, which regulates body weight, metabolic rate, 
etc.</rdfs:comment>
</owl:Class>

<owl:Class rdf:ID= "ThyroidHormone">
<rdfs:subClassOf rdf:resource ="#Hormone"/>
<rdfs:comment>A Hormone secreted by the ThyroidGland.</rdfs:comment>
</owl:Class>

<owl:Class rdf:ID= "Ticket">
<rdfs:subClassOf rdf:resource 
="http://127.0.0.1:8000/ontology/SUMO.owl#Certificate"/>
<rdfs:comment>A Certificate that allows the holder to perform
a specified act once, e.g. ride a bus, attend a concert, obtain a prize,
etc.</rdfs:comment>
</owl:Class>

<owl:Class rdf:ID= "TidalProcess">
<rdfs:subClassOf rdf:resource 
="http://127.0.0.1:8000/ontology/SUMO.owl#InternalChange"/>
<rdfs:comment>TidalProcess is the class of daily
recurring events in which the water level in a BodyOfWater rises
and falls with the changing position between Earth and the 
Moon.</rdfs:comment>
</owl:Class>

<owl:Class rdf:ID= "TieClothing">
<rdfs:subClassOf rdf:resource 
="http://127.0.0.1:8000/ontology/SUMO.owl#Clothing"/>
<rdfs:comment>Clothing that is intended to be worn around the
Neck and knotted at the front.</rdfs:comment>
</owl:Class>

<owl:Class rdf:ID= "Tilling">
<rdfs:subClassOf rdf:resource ="#Digging"/>
<rdfs:comment>Any Process of Digging, e.g. breaking and
turning over the earth that facilitates Agriculture.</rdfs:comment>
</owl:Class>

<owl:Class rdf:ID= "Tin">
<rdfs:subClassOf rdf:resource 
="http://127.0.0.1:8000/ontology/SUMO.owl#ElementalSubstance"/>
<atomicNumber>50</atomicNumber>
<rdfs:comment>Silvery malleable metallic element belonging to group
14 of the periodic table.  Twenty-six isotopes are known, five of which
are radioactive.  Chemically reactive.  Combines directly with chlorine
and oxygen and displaces hydrogen from dilute acids.  </rdfs:comment>
</owl:Class>

<owl:Class rdf:ID= "Toad">
<rdfs:subClassOf rdf:resource 
="http://127.0.0.1:8000/ontology/SUMO.owl#Amphibian"/>
<rdfs:comment>An Amphibian that lacks a Tail and lives at least
partially outside of water.</rdfs:comment>
</owl:Class>

<owl:Class rdf:ID= "Tobacco">
<rdfs:subClassOf rdf:resource 
="http://127.0.0.1:8000/ontology/SUMO.owl#FloweringPlant"/>
<rdfs:comment>A FloweringPlant containing nicotine whose leaves
are dried and then smoked or ingested.</rdfs:comment>
</owl:Class>

<owl:Class rdf:ID= "Toe">
<rdfs:subClassOf rdf:resource ="#DigitAppendage"/>
<rdfs:comment>The five extremities of a Foot.</rdfs:comment>
</owl:Class>

<owl:Class rdf:ID= "Toilet">
<rdfs:subClassOf rdf:resource ="http://127.0.0.1:8000/ontology/SUMO.owl#Device"/>
<rdfs:comment>A Device for urination and defecation.</rdfs:comment>
</owl:Class>

<owl:Class rdf:ID= "Tomb">
<rdfs:subClassOf rdf:resource 
="http://127.0.0.1:8000/ontology/SUMO.owl#StationaryArtifact"/>
<rdfs:comment>A StationaryArtifact which is meant to contain someone
who is Dead.</rdfs:comment>
</owl:Class>

<owl:Class rdf:ID= "TonMass">
<rdfs:subClassOf rdf:resource 
="http://127.0.0.1:8000/ontology/SUMO.owl#MassMeasure"/>
<rdf:type rdf:resource = 
"http://127.0.0.1:8000/ontology/SUMO.owl#UnitOfMeasure"/>
<rdfs:comment>English mass unit that is equal to 2000 pounds.</rdfs:comment>
</owl:Class>

<owl:Class rdf:ID= "TonalLanguage">
<rdfs:subClassOf rdf:resource 
="http://127.0.0.1:8000/ontology/SUMO.owl#SpokenHumanLanguage"/>
<rdfs:comment>Any SpokenHumanLanguage that uses pitch to
differentiate otherwise identical words, e.g. Chinese.</rdfs:comment>
</owl:Class>

<owl:Class rdf:ID= "Tongue">
<rdfs:subClassOf rdf:resource 
="http://127.0.0.1:8000/ontology/SUMO.owl#AnimalAnatomicalStructure"/>
<rdfs:subClassOf rdf:resource 
="http://127.0.0.1:8000/ontology/SUMO.owl#BodyPart"/>
<rdfs:comment>Part of the Mouth, used for Tasting Food,
Vocalizing, and the initial stage of Digesting.</rdfs:comment>
</owl:Class>

<owl:Class rdf:ID= "Tooth">
<rdfs:subClassOf rdf:resource ="http://127.0.0.1:8000/ontology/SUMO.owl#Bone"/>
<rdfs:comment>Part of the Mouth, used for biting and chewing.</rdfs:comment>
</owl:Class>

<owl:Class rdf:ID= "Torso">
<rdfs:subClassOf rdf:resource 
="http://127.0.0.1:8000/ontology/SUMO.owl#AnimalAnatomicalStructure"/>
<rdfs:subClassOf rdf:resource 
="http://127.0.0.1:8000/ontology/SUMO.owl#BodyPart"/>
<rdfs:comment>The body of a Primate excluding its Limbs.</rdfs:comment>
</owl:Class>

<owl:Class rdf:ID= "Towel">
<rdfs:subClassOf rdf:resource ="#FabricArtifact"/>
<rdfs:comment>A piece of Fabric which is used for Drying.</rdfs:comment>
</owl:Class>

<owl:Class rdf:ID= "Tracing">
<rdfs:subClassOf rdf:resource 
="http://127.0.0.1:8000/ontology/SUMO.owl#ContentDevelopment"/>
<rdfs:subClassOf rdf:resource 
="http://127.0.0.1:8000/ontology/SUMO.owl#SurfaceChange"/>
<rdfs:comment>Any ContentDevelopment that results in a 
Blueprint.</rdfs:comment>
</owl:Class>

<owl:Class rdf:ID= "TractorTrailer">
<rdfs:subClassOf rdf:resource ="#RoadVehicle"/>
<rdfs:comment>TractorTrailer is the subclass of
RoadVehicles that are truck tractor- truck trailer 
combinations.</rdfs:comment>
</owl:Class>

<owl:Class rdf:ID= "Trailer">
<rdfs:subClassOf rdf:resource ="#RoadVehicle"/>
<sumo:disjoint rdf:resource = "#SelfPoweredVehicle" />
<sumo:disjoint rdf:resource = "#UserPoweredVehicle" />
<rdfs:comment>Trailer is the class of RoadVehicles that
are designed for towing with another RoadVehicle.</rdfs:comment>
</owl:Class>

<owl:Class rdf:ID= "Train">
<rdfs:subClassOf rdf:resource ="#RailwayVehicle"/>
<rdfs:subClassOf rdf:resource ="#SelfPoweredVehicle"/>
<rdfs:subClassOf rdf:resource 
="http://127.0.0.1:8000/ontology/SUMO.owl#Collection"/>
<rdfs:comment>Train is the subclass of TransportationDevice
whose instances are linked sequences of RollingStock whose motion is
driven by one or more Locomotives or MotorizedRailwayCars.</rdfs:comment>
</owl:Class>

<owl:Class rdf:ID= "TrainStation">
<rdfs:subClassOf rdf:resource ="#TerminalBuilding"/>
<rdfs:comment>TrainStation is the subclass of
Buildings that are located at a RailwayTerminal and used in support
of its functions, especially for the handling of passengers and 
freight.</rdfs:comment>
</owl:Class>

<owl:Class rdf:ID= "Transducer">
<rdfs:subClassOf rdf:resource 
="http://127.0.0.1:8000/ontology/SUMO.owl#Machine"/>
<rdfs:comment>A Device which is capable of converting one form of
energy into another.</rdfs:comment>
</owl:Class>

<owl:Class rdf:ID= "TransferringPosition">
<rdfs:subClassOf rdf:resource 
="http://127.0.0.1:8000/ontology/SUMO.owl#OrganizationalProcess"/>
<rdfs:comment>Any process within an Organization
where a person is moved from one Position to another, e.g. the promotion
or demotion of an employee.</rdfs:comment>
</owl:Class>

<owl:Class rdf:ID= "TransitTerminal">
<rdfs:subClassOf rdf:resource 
="http://127.0.0.1:8000/ontology/SUMO.owl#StationaryArtifact"/>
<rdfs:comment>A TransitTerminal is a place where
travellers or transportation devices begin or end their journeys, or
where passengers and/or goods may be transferred.  At a terminal,
Vehicles may be received, assigned, sent out, or
stored.</rdfs:comment>
</owl:Class>

<owl:Class rdf:about= "Transitway">
<rdfs:subClassOf rdf:resource ="http://127.0.0.1:8000/ontology/SUMO.owl#Region"/>
<rdfs:subClassOf rdf:resource 
="http://127.0.0.1:8000/ontology/SUMO.owl#SelfConnectedObject"/>
<rdfs:comment>Transitway is the broadest class
of regions which may be passed through as a path in instances
of Translocation.  Transitway includes land, air, and sea
regions, and it includes both natural and artificial 
transitways.</rdfs:comment>
</owl:Class>

<owl:Class rdf:ID= "TransitwayJunction">
<rdfs:subClassOf rdf:resource 
="http://127.0.0.1:8000/ontology/SUMO.owl#Transitway"/>
<rdfs:comment>TransitwayJunction is the class of
regions where two or more Transitways meet and traffic may transfer
from one transitway to another.</rdfs:comment>
</owl:Class>

<owl:Class rdf:ID= "TransportationCompany">
<rdfs:subClassOf rdf:resource 
="http://127.0.0.1:8000/ontology/SUMO.owl#CommercialAgent"/>
<rdfs:comment>A CommercialAgent whose services
include Transportation, e.g. a RailroadCompany, an airline, a cruise
ship line, etc.</rdfs:comment>
</owl:Class>

<owl:Class rdf:ID= "TransportationSystem">
<rdfs:subClassOf rdf:resource ="http://127.0.0.1:8000/ontology/SUMO.owl#Object"/>
<rdfs:comment>TransportationSystem is the
subclass of complex Objects consisting of networks of Transitways
and TransitJunctions that link together a number of GeographicRegions
or TransitTerminals.  TransportationSystem covers worldwide
networks, such as internationally recognized shipping lanes or air
corridors, also route systems such as those flown by a single airline,
as well as LocalTransitSystems such as BART (Bay Area Rapid 
Transit).</rdfs:comment>
</owl:Class>

<owl:Class rdf:ID= "TrapOrCage">
<rdfs:subClassOf rdf:resource ="#Holder"/>
<rdfs:comment>A Device whose purpose is to trap or cage Animals,
i.e. to be in instrument in an act of Confining.</rdfs:comment>
</owl:Class>

<owl:Class rdf:ID= "TravelContainer">
<rdfs:subClassOf rdf:resource ="#Container"/>
<rdfs:comment>Any Container which is intended to be
used for carrying personal effects from one point to another.  This class
covers suitcases, briefcases, backpacks, etc.</rdfs:comment>
</owl:Class>

<owl:Class rdf:ID= "Tray">
<rdfs:subClassOf rdf:resource ="#Holder"/>
<rdfs:comment>A Holder that is designed for Food, dishes, and
flatware.</rdfs:comment>
</owl:Class>

<owl:Class rdf:ID= "Treasurer">
<rdfs:subClassOf rdf:resource ="#SkilledOccupation"/>
<rdfs:comment>Any SkilledOccupation which involves receiving
and disbursing money.</rdfs:comment>
</owl:Class>

<owl:Class rdf:ID= "TreeBranch">
<rdfs:subClassOf rdf:resource ="#PlantBranch"/>
<rdfs:comment>Any PlantBranch which is part of a
BotanicalTree.</rdfs:comment>
</owl:Class>

<owl:Class rdf:ID= "TreeGraph">
<rdfs:subClassOf rdf:resource ="#Graph"/>
<rdfs:comment>A TreeGraph is a DirectedGraph that has no
GraphLoops.</rdfs:comment>
</owl:Class>

<owl:Class rdf:ID= "Trembling">
<rdfs:subClassOf rdf:resource 
="http://127.0.0.1:8000/ontology/SUMO.owl#BodyMotion"/>
<rdfs:subClassOf rdf:resource ="#Tremor"/>
<sumo:disjoint rdf:resource = 
"http://127.0.0.1:8000/ontology/SUMO.owl#IntentionalProcess" />
<rdfs:comment>Any BodyMotion which is involuntary and which is
repeated many times over a short time frame, e.g. a spasm in the 
hands.</rdfs:comment>
</owl:Class>

<owl:Class rdf:ID= "Tremor">
<rdfs:subClassOf rdf:resource ="#Rotating"/>
<rdfs:comment>Motion that involves rapidly Rotating between
two positions.</rdfs:comment>
</owl:Class>

<owl:Class rdf:ID= "Trespassing">
<rdfs:subClassOf rdf:resource ="#CriminalAction"/>
<rdfs:subClassOf rdf:resource 
="http://127.0.0.1:8000/ontology/SUMO.owl#Translocation"/>
<rdfs:comment>Entering property that does not belong to one and without
the permission of the owner of the property.</rdfs:comment>
</owl:Class>

<owl:Class rdf:ID= "Triangle">
<rdfs:subClassOf rdf:resource ="#Polygon"/>
<rdfs:comment>Any three-sided Polygon.</rdfs:comment>
</owl:Class>

<owl:Class rdf:ID= "TropicalClimateZone">
<rdfs:subClassOf rdf:resource ="#ClimateZone"/>
<rdfs:comment>TropicalClimateZone is a
subclass of ClimateZone in which the average temperature of the
coldest month is greater than 18 degrees Celsius.  This is Class
'A' in the Koeppen climate classification system.</rdfs:comment>
</owl:Class>

<owl:Class rdf:ID= "Trousers">
<rdfs:subClassOf rdf:resource 
="http://127.0.0.1:8000/ontology/SUMO.owl#Clothing"/>
<rdfs:comment>A piece of Clothing that covers each Leg
of a person separately.</rdfs:comment>
</owl:Class>

<owl:Class rdf:ID= "Truck">
<rdfs:subClassOf rdf:resource ="#SelfPoweredRoadVehicle"/>
<rdfs:comment>Truck is the subclass of RoadVehicles that
are designed primarily for transporting various kinds of non-passenger
loads.  Truck is the class of single-bodied trucks or TruckTractors.
Note: TractorTrailer combinations are a distinct class.</rdfs:comment>
</owl:Class>

<owl:Class rdf:ID= "TruckTractor">
<rdfs:subClassOf rdf:resource ="#Truck"/>
<rdfs:comment>TruckTractor is the subclass of Trucks
that are used to tow truck trailers.  Truck tractors are the cab portions
of tractor-trailers.  See also TruckTrailer.</rdfs:comment>
</owl:Class>

<owl:Class rdf:ID= "TruckTrailer">
<rdfs:subClassOf rdf:resource ="#Trailer"/>
<rdfs:comment>TruckTrailer is the subclass of Trailers
that are towed by TruckTractors.  These are the trailers used in
tractor-trailer (semi-trailer) rigs.</rdfs:comment>
</owl:Class>

<owl:Class rdf:ID= "Tube">
<rdfs:subClassOf rdf:resource 
="http://127.0.0.1:8000/ontology/SUMO.owl#Artifact"/>
<rdfs:comment>A long, narrow, and hollow Artifact that is designed for
moving Fluids from place to another.</rdfs:comment>
</owl:Class>

<owl:Class rdf:ID= "Tumor">
<rdfs:subClassOf rdf:resource 
="http://127.0.0.1:8000/ontology/SUMO.owl#AbnormalAnatomicalStructure"/>
<rdfs:comment>Any AbnormalAnatomicalStructure which consists of a
mass of Tissue.  Note that this class covers both malignant (i.e. cancerous)
and benign tumors.</rdfs:comment>
</owl:Class>

<owl:Class rdf:ID= "TundraClimateZone">
<rdfs:subClassOf rdf:resource ="#PolarClimateZone"/>
<rdfs:comment>TundraClimateZone is a subclass of
PolarClimateZone characterized by having an average temperature
above zero degrees Celsius (but below 10 degrees) in the warmest month.
Koeppen subtype 'ET'.</rdfs:comment>
</owl:Class>

<owl:Class rdf:ID= "Tunnel">
<rdfs:subClassOf rdf:resource 
="http://127.0.0.1:8000/ontology/SUMO.owl#LandTransitway"/>
<rdfs:subClassOf rdf:resource 
="http://127.0.0.1:8000/ontology/SUMO.owl#StationaryArtifact"/>
<rdfs:comment>Tunnel is a subclass of Transitways that
consist of a lengthwise enclosed Hole that allows for transit
underground, as through mountains, below a body of water, or beneath a
city.</rdfs:comment>
</owl:Class>

<owl:Class rdf:ID= "Turbine">
<rdfs:subClassOf rdf:resource ="#Engine"/>
<rdfs:comment>An Engine which converts the kinetic energy of a moving
Liquid (typically Water) into mechanical energy.</rdfs:comment>
</owl:Class>

<owl:Class rdf:ID= "TurningOffDevice">
<rdfs:subClassOf rdf:resource 
="http://127.0.0.1:8000/ontology/SUMO.owl#InternalChange"/>
<rdfs:comment>Any Process whose result is that the patient
of the process is in the state of DeviceOff.  In other words, this class 
covers
any process of turning off a device, e.g. turning off the lights, switching 
off a
television set, etc.</rdfs:comment>
</owl:Class>

<owl:Class rdf:ID= "TurningOnDevice">
<rdfs:subClassOf rdf:resource 
="http://127.0.0.1:8000/ontology/SUMO.owl#InternalChange"/>
<rdfs:comment>Any Process whose result is that the patient
of the process is in the state of DeviceOn.  In other words, this class 
covers
any process of turning on a device, e.g. turning on the lights, switching on 
a
television set, etc.</rdfs:comment>
</owl:Class>

<owl:Class rdf:ID= "Tying">
<rdfs:subClassOf rdf:resource 
="http://127.0.0.1:8000/ontology/SUMO.owl#Attaching"/>
<rdfs:comment>The Process of tying two things, or two strands of
the same thing, together.</rdfs:comment>
</owl:Class>

<owl:Class rdf:ID= "UnionOrganization">
<rdfs:subClassOf rdf:resource 
="http://127.0.0.1:8000/ontology/SUMO.owl#Organization"/>
<rdfs:comment>An Organization comprised of workers from
the same Corporation or Industry.  The purpose of the UnionOrganization
is to strengthen its representation in bargaining with the Corporation or
Industry.</rdfs:comment>
</owl:Class>

<owl:Class rdf:ID= "UnionSoldier">
<rdfs:subClassOf rdf:resource ="#Soldier"/>
<rdfs:comment>Any Soldier that served on the union side during
the American Civil War.</rdfs:comment>
</owl:Class>

<owl:Class rdf:ID= "UnitedKingdomGallon">
<rdfs:subClassOf rdf:resource 
="http://127.0.0.1:8000/ontology/SUMO.owl#VolumeMeasure"/>
<rdf:type rdf:resource = 
"http://127.0.0.1:8000/ontology/SUMO.owl#UnitOfMeasure"/>
<sumo:relatedInternalConcept rdf:resource = 
"http://127.0.0.1:8000/ontology/SUMO.owl#UnitedStatesGallon" />
<rdfs:comment>Unit of volume commonly used in the
United Kingdom.</rdfs:comment>
</owl:Class>

<owl:Class rdf:ID= "University">
<rdfs:subClassOf rdf:resource ="#PostSecondarySchool"/>
<rdfs:comment>A School which admits students that
have graduated from high school (known as undergraduate students) and
students who have received a bachelor's degree (known as graduate
students).  A University confers both bachelor's and graduate
degrees.</rdfs:comment>
</owl:Class>

<owl:Class rdf:ID= "UnskilledOccupation">
<rdfs:subClassOf rdf:resource ="#ManualLabor"/>
<sumo:disjoint rdf:resource = "#SkilledOccupation" />
<rdfs:comment>Any Position which does not
require learning a set of skills.</rdfs:comment>
</owl:Class>

<owl:Class rdf:ID= "UnsurfacedRoadway">
<rdfs:subClassOf rdf:resource 
="http://127.0.0.1:8000/ontology/SUMO.owl#Roadway"/>
<rdfs:comment>UnsurfacedRoadway is the subclass
of Roadways that have natural, unimproved surfaces of dirt or 
sand.</rdfs:comment>
</owl:Class>

<owl:Class rdf:ID= "Untying">
<rdfs:subClassOf rdf:resource 
="http://127.0.0.1:8000/ontology/SUMO.owl#Detaching"/>
<sumo:disjoint rdf:resource = "#Tying" />
<rdfs:comment>The Process of untying two things, or two strands
of the same thing.</rdfs:comment>
</owl:Class>

<owl:Class rdf:ID= "UplandArea">
<rdfs:subClassOf rdf:resource ="#LandForm"/>
<rdfs:comment>An UplandArea is a LandArea elevated above the surrounding 
terrain.</rdfs:comment>
</owl:Class>

<owl:Class rdf:ID= "Urea">
<rdfs:subClassOf rdf:resource ="#OrganicCompound"/>
<rdfs:comment>Urea is a dry, soluble, nitrogenous substance
that is the major solid component of the urine of mammals, and which
may be synthesized from ammonia and carbon dioxide; it is useful in the
production of Plastic and in Fertilizers.</rdfs:comment>
</owl:Class>

<owl:Class rdf:ID= "UserPoweredDevice">
<rdfs:subClassOf rdf:resource ="#Engine"/>
<rdfs:comment>UserPoweredDevice is a subclass of
Engine that perform work when a power input is supplied by the 
user.</rdfs:comment>
</owl:Class>

<owl:Class rdf:ID= "UserPoweredVehicle">
<rdfs:subClassOf rdf:resource 
="http://127.0.0.1:8000/ontology/SUMO.owl#Vehicle"/>
<rdfs:subClassOf rdf:resource ="#UserPoweredDevice"/>
<rdfs:comment>UserPoweredVehicle is the subclass of
Vehicles whose power source is the rider or user.  Examples: Bicycles,
Canoes, grocery carts.</rdfs:comment>
</owl:Class>

<owl:Class rdf:ID= "UsingAnAccount">
<rdfs:subClassOf rdf:resource 
="http://127.0.0.1:8000/ontology/SUMO.owl#FinancialTransaction"/>
<rdfs:comment>An activity of using a financial account</rdfs:comment>
</owl:Class>

<owl:Class rdf:ID= "Vacationing">
<rdfs:subClassOf rdf:resource 
="http://127.0.0.1:8000/ontology/SUMO.owl#RecreationOrExercise"/>
<rdfs:comment>Taking time off from one's occupation.</rdfs:comment>
</owl:Class>

<owl:Class rdf:ID= "VehicleBrake">
<rdfs:subClassOf rdf:resource ="#VehicleController"/>
<rdfs:comment>A VehicleController which is capable of stopping
the motion of a Vehicle.</rdfs:comment>
</owl:Class>

<owl:Class rdf:ID= "VehicleController">
<rdfs:subClassOf rdf:resource ="http://127.0.0.1:8000/ontology/SUMO.owl#Device"/>
<rdfs:comment>Any Device which is used to start, stop or
control the movements of a Vehicle.  This class covers steering wheels, 
brakes,
acceleration pedals, airplane sticks, etc.</rdfs:comment>
</owl:Class>

<owl:Class rdf:ID= "VehicleLight">
<rdfs:subClassOf rdf:resource ="#IlluminationDevice"/>
<rdfs:comment>Any IlluminationDevice which is attached to the
surface of a Vehicle and whose purpose is to illuminate that area around
the Vehicle so that potential obstacles can be detected or 
alerted.</rdfs:comment>
</owl:Class>

<owl:Class rdf:ID= "VehicleThrottle">
<rdfs:subClassOf rdf:resource ="#VehicleController"/>
<rdfs:comment>A VehicleController which controls the amount
of Fuel which is supplied to the Engine.</rdfs:comment>
</owl:Class>

<owl:Class rdf:ID= "VehicleTire">
<rdfs:subClassOf rdf:resource 
="http://127.0.0.1:8000/ontology/SUMO.owl#Artifact"/>
<rdfs:comment>A covering, usually made of rubber, for a 
Wheel.</rdfs:comment>
</owl:Class>

<owl:Class rdf:ID= "VehicleWheel">
<rdfs:subClassOf rdf:resource ="#Wheel"/>
<rdfs:comment>VehicleWheel is a class of cylindrical
Devices used to move a RoadVehicle along a road, running either
directly on the wheel rims or on tires attached to the wheel 
rims.</rdfs:comment>
</owl:Class>

<owl:Class rdf:ID= "VehicleWindow">
<rdfs:subClassOf rdf:resource ="#Window"/>
<rdfs:comment>Any Window which is part of a Vehicle,
e.g. the Windshield and RearWindow of an Automobile.</rdfs:comment>
</owl:Class>

<owl:Class rdf:ID= "Vein">
<rdfs:subClassOf rdf:resource ="#BloodVessel"/>
<sumo:relatedInternalConcept rdf:resource = "#Artery" />
<rdfs:comment>Any BloodVessel which transfers Blood from
the extremities of the body to the Heart.</rdfs:comment>
</owl:Class>

<owl:Class rdf:ID= "VendingDevice">
<rdfs:subClassOf rdf:resource ="http://127.0.0.1:8000/ontology/SUMO.owl#Device"/>
<rdfs:comment>A Device which is capable of Selling a Product
to a customer automatically when the customer inserts the appropriate amount 
of
Currency.</rdfs:comment>
</owl:Class>

<owl:Class rdf:ID= "Violin">
<rdfs:subClassOf rdf:resource ="#StringInstrument"/>
<rdfs:comment>A StringInstrument that has four strings, a hollow
body, and is played on the shoulder with a bow.</rdfs:comment>
</owl:Class>

<owl:Class rdf:ID= "ViralDisease">
<rdfs:subClassOf rdf:resource ="#InfectiousDisease"/>
<rdfs:comment>A disease that is caused by instances of
Virus.</rdfs:comment>
</owl:Class>

<owl:Class rdf:ID= "VocalMusic">
<rdfs:subClassOf rdf:resource ="http://127.0.0.1:8000/ontology/SUMO.owl#Music"/>
<rdfs:comment>Music which is produced (at least in part)
by Singing.</rdfs:comment>
</owl:Class>

<owl:Class rdf:ID= "VocationalSchool">
<rdfs:subClassOf rdf:resource ="#School"/>
<rdfs:comment>Any School whose aim is to teach
students an OccupationalTrade.</rdfs:comment>
</owl:Class>

<owl:Class rdf:ID= "Volt">
<rdfs:subClassOf rdf:resource 
="http://127.0.0.1:8000/ontology/SUMO.owl#FunctionQuantity"/>
<rdf:type rdf:resource = 
"http://127.0.0.1:8000/ontology/SUMO.owl#SystemeInternationalUnit"/>
<rdfs:comment>SI electric potential measure.  Symbol: V.  It is
the difference of electric potential between two points of a conducting
wire carrying a constant current of 1 Ampere, when the power dissipated
between these points is equal to 1 Watt.  Volt = W/A =
m^2*kg*s^(-3)*A^(-1).</rdfs:comment>
</owl:Class>

<owl:Class rdf:ID= "VotingPoll">
<rdfs:subClassOf rdf:resource 
="http://127.0.0.1:8000/ontology/SUMO.owl#StationaryArtifact"/>
<rdfs:comment>A structure where Voting for an Election
takes place.</rdfs:comment>
</owl:Class>

<owl:Class rdf:ID= "Vowel">
<rdfs:subClassOf rdf:resource ="#AlphabeticCharacter"/>
<rdfs:comment>An AlphabeticCharacter that denotes a speech sound that
does not result in audible friction when it is pronounced.</rdfs:comment>
</owl:Class>

<owl:Class rdf:ID= "Vulture">
<rdfs:subClassOf rdf:resource ="http://127.0.0.1:8000/ontology/SUMO.owl#Bird"/>
<rdfs:comment>A diurnal bird of prey with a bald head that
feeds on carrion.</rdfs:comment>
</owl:Class>

<owl:Class rdf:ID= "Wading">
<rdfs:subClassOf rdf:resource 
="http://127.0.0.1:8000/ontology/SUMO.owl#Walking"/>
<rdfs:comment>Any instance of Walking which occurs through a
BodyOfWater.</rdfs:comment>
</owl:Class>

<owl:Class rdf:ID= "Wagon">
<rdfs:subClassOf rdf:resource ="#LandVehicle"/>
<rdfs:comment>A Landcraft that is not self-propelled, but must be
pulled by either an Animal or a self-propelled Vehicle to move along the
ground.</rdfs:comment>
</owl:Class>

<owl:Class rdf:ID= "WakingUp">
<rdfs:subClassOf rdf:resource 
="http://127.0.0.1:8000/ontology/SUMO.owl#PsychologicalProcess"/>
<rdfs:comment>The process of transitioning from a state of being
Asleep to a state of being Awake.</rdfs:comment>
</owl:Class>

<owl:Class rdf:ID= "WalkingCane">
<rdfs:subClassOf rdf:resource ="http://127.0.0.1:8000/ontology/SUMO.owl#Device"/>
<rdfs:comment>A Device which has the form of a staff with
a handle and which enables some people to walk with greater 
assurance.</rdfs:comment>
</owl:Class>

<owl:Class rdf:ID= "Wall">
<rdfs:subClassOf rdf:resource 
="http://127.0.0.1:8000/ontology/SUMO.owl#StationaryArtifact"/>
<rdfs:comment>A StationaryArtifact that supports a Building or
partitions it into Rooms.</rdfs:comment>
</owl:Class>

<owl:Class rdf:ID= "Wallpaper">
<rdfs:subClassOf rdf:resource 
="http://127.0.0.1:8000/ontology/SUMO.owl#ArtWork"/>
<rdfs:comment>Any decorative paper that is used to cover the
Walls of Rooms.</rdfs:comment>
</owl:Class>

<owl:Class rdf:ID= "Warehouse">
<rdfs:subClassOf rdf:resource ="#CommercialBuilding"/>
<rdfs:comment>A very large CommercialBuilding whose purpose is
to store commodities.</rdfs:comment>
</owl:Class>

<owl:Class rdf:ID= "WashBasin">
<rdfs:subClassOf rdf:resource ="#WashingDevice"/>
<rdfs:comment>A WashingDevice which is intended to be used by
Humans for washing their Hands.</rdfs:comment>
</owl:Class>

<owl:Class rdf:ID= "Washing">
<rdfs:subClassOf rdf:resource 
="http://127.0.0.1:8000/ontology/SUMO.owl#Removing"/>
<rdfs:comment>Removing small particles from something by means of
a Detergent and Water.</rdfs:comment>
</owl:Class>

<owl:Class rdf:ID= "WashingDevice">
<rdfs:subClassOf rdf:resource ="http://127.0.0.1:8000/ontology/SUMO.owl#Device"/>
<rdfs:comment>Any Device whose purpose is Washing
something, e.g. washing machines, dishwashers, bathtubs, etc.</rdfs:comment>
</owl:Class>

<owl:Class rdf:ID= "Wastebasket">
<rdfs:subClassOf rdf:resource ="#Container"/>
<rdfs:comment>A Container which is used for trash.</rdfs:comment>
</owl:Class>

<owl:Class rdf:ID= "WatchClock">
<rdfs:subClassOf rdf:resource ="#Clock"/>
<rdfs:comment>A Clock that can be worn on the Wrist.</rdfs:comment>
</owl:Class>

<owl:Class rdf:ID= "WaterMotion">
<rdfs:subClassOf rdf:resource 
="http://127.0.0.1:8000/ontology/SUMO.owl#LiquidMotion"/>
<rdfs:comment>Any LiquidMotion where the Liquid is Water.</rdfs:comment>
</owl:Class>

<owl:Class rdf:ID= "WaterTransportation">
<rdfs:subClassOf rdf:resource 
="http://127.0.0.1:8000/ontology/SUMO.owl#Transportation"/>
<rdfs:comment>Any instance of Transportation where
the instrument is a Watercraft.</rdfs:comment>
</owl:Class>

<owl:Class rdf:ID= "WaterWave">
<rdfs:subClassOf rdf:resource ="#WaterMotion"/>
<rdfs:comment>A WaterWave is a raised ridge of water
moving along the surface of a body of water.  The WaterWave moves
in a direction approximately transverse to the crest line of the wave.
The patient of the WaterWave is successive regions of water, which
do not travel in the direction of the wave or with it.</rdfs:comment>
</owl:Class>

<owl:Class rdf:ID= "WatercolorPaint">
<rdfs:subClassOf rdf:resource ="#Paint"/>
<rdfs:comment>Any Paint which is a water-based Solution.</rdfs:comment>
</owl:Class>

<owl:Class rdf:ID= "WatercolorPicture">
<rdfs:subClassOf rdf:resource ="#PaintedPicture"/>
<rdfs:comment>Any PaintedPicture which is created
with water-based paints.</rdfs:comment>
</owl:Class>

<owl:Class rdf:ID= "Watercraft">
<rdfs:subClassOf rdf:resource 
="http://127.0.0.1:8000/ontology/SUMO.owl#Vehicle"/>
<rdfs:comment>Watercraft is the class of all Vehicles
used to travel on or in water.</rdfs:comment>
</owl:Class>

<owl:Class rdf:ID= "Waterfall">
<rdfs:subClassOf rdf:resource 
="http://127.0.0.1:8000/ontology/SUMO.owl#StreamWaterArea"/>
<rdfs:comment>Waterfall is the subclass of StreamWaterAreas
where running water falls steeply downhill.</rdfs:comment>
</owl:Class>

<owl:Class rdf:ID= "Waterway">
<rdfs:subClassOf rdf:resource 
="http://127.0.0.1:8000/ontology/SUMO.owl#Transitway"/>
<rdfs:subClassOf rdf:resource 
="http://127.0.0.1:8000/ontology/SUMO.owl#WaterArea"/>
<rdfs:comment>Waterway is the class of navigable waters,
including oceans, seaLanes, rivers, canals, lakes, and inland bodies
of water.</rdfs:comment>
</owl:Class>

<owl:Class rdf:ID= "Watt">
<rdfs:subClassOf rdf:resource 
="http://127.0.0.1:8000/ontology/SUMO.owl#FunctionQuantity"/>
<rdf:type rdf:resource = 
"http://127.0.0.1:8000/ontology/SUMO.owl#SystemeInternationalUnit"/>
<rdfs:comment>SI power measure.  Symbol: W.  A UnitOfMeasure
that measures power, i.e. energy produced or expended divided by
TimeDuration. It is the power which gives rise to the production
of energy (or work) at the rate of one Joule per SecondDuration.
Watt = J/s = m^2*kg*s^(-3).</rdfs:comment>
</owl:Class>

<owl:Class rdf:ID= "Waving">
<rdfs:subClassOf rdf:resource ="#HandGesture"/>
<rdfs:comment>Moving a Hand to indicate a greeting, farewell,
recognition, goodwill, etc.</rdfs:comment>
</owl:Class>

<owl:Class rdf:ID= "Wax">
<rdfs:subClassOf rdf:resource 
="http://127.0.0.1:8000/ontology/SUMO.owl#Substance"/>
<rdfs:comment>Any Substance of high molecular weight that resembles
beeswax.</rdfs:comment>
</owl:Class>

<owl:Class rdf:ID= "WeaponOfMassDestruction">
<rdfs:subClassOf rdf:resource ="http://127.0.0.1:8000/ontology/SUMO.owl#Weapon"/>
<rdfs:comment>Nuclear, chemical and biological weapons.
What these weapons have in common is that they are designed to kill large 
numbers
of people indiscriminately.</rdfs:comment>
</owl:Class>

<owl:Class rdf:ID= "WeatherFront">
<rdfs:subClassOf rdf:resource 
="http://127.0.0.1:8000/ontology/SUMO.owl#WeatherProcess"/>
<rdfs:comment>WeatherFront is the class of weather
processes that are involve relationships between two air masses, such
as a high pressure weather system or a low pressure system.</rdfs:comment>
</owl:Class>

<owl:Class rdf:ID= "Weber">
<rdfs:subClassOf rdf:resource 
="http://127.0.0.1:8000/ontology/SUMO.owl#FunctionQuantity"/>
<rdf:type rdf:resource = 
"http://127.0.0.1:8000/ontology/SUMO.owl#SystemeInternationalUnit"/>
<rdfs:comment>SI magnetic flux measure.  Symbol: Wb. It is the
magnetic flux which, linking a circuit of one turn, produces in it an
electromotive force of 1 Volt as it is reduced to zero at a uniform
rate in 1 SecondDuration.  Weber = V*s = 
m^2*kg*s^(-2)*A^(-1).</rdfs:comment>
</owl:Class>

<owl:Class rdf:ID= "Weekend">
<rdfs:subClassOf rdf:resource 
="http://127.0.0.1:8000/ontology/SUMO.owl#TimeInterval"/>
<rdfs:comment>Any Saturday and Sunday which are contiguous.</rdfs:comment>
</owl:Class>

<owl:Class rdf:ID= "Weeping">
<rdfs:subClassOf rdf:resource ="#FacialExpression"/>
<rdfs:comment>Expressing unhappiness by shedding tears.</rdfs:comment>
</owl:Class>

<owl:Class rdf:ID= "Welfare">
<rdfs:subClassOf rdf:resource 
="http://127.0.0.1:8000/ontology/SUMO.owl#Funding"/>
<rdfs:comment>Any Funding which is provided by a ServiceOrganization
to people in need.</rdfs:comment>
</owl:Class>

<owl:Class rdf:ID= "WetTropicalClimateZone">
<rdfs:subClassOf rdf:resource ="#TropicalClimateZone"/>
<rdfs:comment>WetTropicalClimateZone is
the subclass of TropicalClimateZone that is characterized by having
no dry months.  At least 60 mm of rainfall occur in the driest month.
This is subtype 'Af' in the Koeppen climate system.</rdfs:comment>
</owl:Class>

<owl:Class rdf:ID= "Wheat">
<rdfs:subClassOf rdf:resource ="#CerealGrain"/>
<rdfs:comment>A long CerealGrain which is produced by certain grasses and
which is used to make BreadOrBiscuits.</rdfs:comment>
</owl:Class>

<owl:Class rdf:ID= "Wheel">
<rdfs:subClassOf rdf:resource 
="http://127.0.0.1:8000/ontology/SUMO.owl#Artifact"/>
<rdfs:comment>A circular Artifact which is a component of
LandVehicles and of some Devices.</rdfs:comment>
</owl:Class>

<owl:Class rdf:ID= "Whip">
<rdfs:subClassOf rdf:resource ="http://127.0.0.1:8000/ontology/SUMO.owl#Weapon"/>
<rdfs:comment>A Weapon that consists of a thin strand of
Fabric, usually Leather, and a handle by which the strand is
impelled at a high rate of speed.</rdfs:comment>
</owl:Class>

<owl:Class rdf:ID= "Whiskey">
<rdfs:subClassOf rdf:resource ="#DistilledAlcoholicBeverage"/>
<rdfs:comment>A DistilledAlcoholicBeverage that is prepared by
distilling fermented grain mash.</rdfs:comment>
</owl:Class>

<owl:Class rdf:ID= "WhiteBloodCell">
<rdfs:subClassOf rdf:resource ="#BloodCell"/>
<rdfs:comment>BloodCells that lack hemoglobin, contain a
CellNucleus, and have no color.</rdfs:comment>
</owl:Class>

<owl:Class rdf:ID= "WholesaleStore">
<rdfs:subClassOf rdf:resource 
="http://127.0.0.1:8000/ontology/SUMO.owl#MercantileOrganization"/>
<rdfs:subClassOf rdf:resource ="#Agency"/>
<rdfs:comment>A MercantileOrganization that sells its
goods exclusively to Corporations.</rdfs:comment>
</owl:Class>

<owl:Class rdf:ID= "WillowTree">
<rdfs:subClassOf rdf:resource ="#BotanicalTree"/>
<rdfs:comment>A BotanicalTree of the genus Salix.</rdfs:comment>
</owl:Class>

<owl:Class rdf:ID= "WindInstrument">
<rdfs:subClassOf rdf:resource 
="http://127.0.0.1:8000/ontology/SUMO.owl#MusicalInstrument"/>
<rdfs:comment>A MusicalInstrument which is played by
blowing it and which uses a reed.</rdfs:comment>
</owl:Class>

<owl:Class rdf:ID= "Windmill">
<rdfs:subClassOf rdf:resource ="#Engine"/>
<rdfs:comment>Windmill is the subclass of Engines that
produce mechanical power from Wind energy.</rdfs:comment>
</owl:Class>

<owl:Class rdf:ID= "Window">
<rdfs:subClassOf rdf:resource 
="http://127.0.0.1:8000/ontology/SUMO.owl#Artifact"/>
<rdfs:comment>An Artifact composed of transparent glass or
plastic that admits light (and possibly air) into a Room, Building
or Vehicle.</rdfs:comment>
</owl:Class>

<owl:Class rdf:ID= "WindowCovering">
<rdfs:subClassOf rdf:resource 
="http://127.0.0.1:8000/ontology/SUMO.owl#Artifact"/>
<rdfs:comment>An Artifact that is used to cover
Windows.  Note that this class includes blinds, drapes, shutters,
etc.</rdfs:comment>
</owl:Class>

<owl:Class rdf:ID= "Windshield">
<rdfs:subClassOf rdf:resource ="#VehicleWindow"/>
<sumo:disjoint rdf:resource = "#RearWindow" />
<rdfs:comment>Any VehicleWindow which located at the front
of an Automobile.</rdfs:comment>
</owl:Class>

<owl:Class rdf:ID= "Wine">
<rdfs:subClassOf rdf:resource ="#AlcoholicBeverage"/>
<rdfs:comment>An AlcoholicBeverage that is prepared by fermenting
the juice of grapes.</rdfs:comment>
</owl:Class>

<owl:Class rdf:ID= "Wing">
<rdfs:subClassOf rdf:resource ="#Limb"/>
<rdfs:comment>Any Limb which is capable of being an
instrument in Flying.</rdfs:comment>
</owl:Class>

<owl:Class rdf:ID= "WingDevice">
<rdfs:subClassOf rdf:resource 
="http://127.0.0.1:8000/ontology/SUMO.owl#EngineeringComponent"/>
<rdfs:comment>The wings of Aircraft, i.e. the parts of Aircraft
that allow them to become and remain airborne.</rdfs:comment>
</owl:Class>

<owl:Class rdf:ID= "Winking">
<rdfs:subClassOf rdf:resource ="#ClosingEyes"/>
<rdfs:subClassOf rdf:resource 
="http://127.0.0.1:8000/ontology/SUMO.owl#Gesture"/>
<rdfs:comment>Any instance of ClosingEyes which is intended to
express something to someone else.</rdfs:comment>
</owl:Class>

<owl:Class rdf:ID= "WinterSeason">
<rdfs:subClassOf rdf:resource ="#SeasonOfYear"/>
<rdfs:comment>The SeasonOfYear that begins at the winter
solstice and ends at the spring equinox.</rdfs:comment>
</owl:Class>

<owl:Class rdf:ID= "Wire">
<rdfs:subClassOf rdf:resource 
="http://127.0.0.1:8000/ontology/SUMO.owl#Artifact"/>
<rdfs:comment>A long, thin strand of Metal that is used in a wide
range of applications, including the wiring of electrical systems, creating
bundles and the construction of cages.</rdfs:comment>
</owl:Class>

<owl:Class rdf:ID= "WireLine">
<rdfs:subClassOf rdf:resource ="#Wire"/>
<rdfs:subClassOf rdf:resource 
="http://127.0.0.1:8000/ontology/SUMO.owl#EngineeringComponent"/>
<rdfs:comment>A Wire that is designed for conducting 
electricity.</rdfs:comment>
</owl:Class>

<owl:Class rdf:ID= "WireSpring">
<rdfs:subClassOf rdf:resource ="#Wire"/>
<rdfs:subClassOf rdf:resource 
="http://127.0.0.1:8000/ontology/SUMO.owl#EngineeringComponent"/>
<rdfs:comment>An EngineeringComponent consisting of a coil of
Wire that returns to its original shape when pulled apart or pressed 
together.</rdfs:comment>
</owl:Class>

<owl:Class rdf:ID= "Withdrawal">
<rdfs:subClassOf rdf:resource 
="http://127.0.0.1:8000/ontology/SUMO.owl#FinancialTransaction"/>
<rdfs:comment>An activity of money being transferred from a customer's
account at a financial institution.</rdfs:comment>
</owl:Class>

<owl:Class rdf:ID= "Wood">
<rdfs:subClassOf rdf:resource ="http://127.0.0.1:8000/ontology/SUMO.owl#Tissue"/>
<rdfs:subClassOf rdf:resource 
="http://127.0.0.1:8000/ontology/SUMO.owl#PlantSubstance"/>
<sumo:relatedInternalConcept rdf:resource = "#WoodArtifact" />
<rdfs:comment>Tissue that comprises the inner trunk of Trees.
It is often used in constructing Buildings and other 
Artifacts.</rdfs:comment>
</owl:Class>

<owl:Class rdf:ID= "WoodArtifact">
<rdfs:subClassOf rdf:resource 
="http://127.0.0.1:8000/ontology/SUMO.owl#Artifact"/>
<rdfs:comment>Wood that has been cut (and perhaps treated) for
some purpose, e.g. Constructing or Combustion.  Note that this class covers
both lumber and firewood.</rdfs:comment>
</owl:Class>

<owl:Class rdf:ID= "Wool">
<rdfs:subClassOf rdf:resource ="http://127.0.0.1:8000/ontology/SUMO.owl#Fabric"/>
<rdfs:comment>Fabric that is made from the Hair of Sheep.</rdfs:comment>
</owl:Class>

<owl:Class rdf:ID= "WorkerInsect">
<rdfs:subClassOf rdf:resource ="http://127.0.0.1:8000/ontology/SUMO.owl#Insect"/>
<rdfs:comment>Sterile members of an Insect colony which
are responsible for locating food and caring for eggs, larvae, 
etc.</rdfs:comment>
</owl:Class>

<owl:Class rdf:ID= "Workshop">
<rdfs:subClassOf rdf:resource 
="http://127.0.0.1:8000/ontology/SUMO.owl#StationaryArtifact"/>
<rdfs:comment>A Room, suite of Rooms or Building which is
devoted to hand-crafting Artifacts.</rdfs:comment>
</owl:Class>

<owl:Class rdf:ID= "Wrist">
<rdfs:subClassOf rdf:resource ="#BodyJoint"/>
<rdfs:comment>The joint in the Arm connecting the radius and carpal
bones.</rdfs:comment>
</owl:Class>

<owl:Class rdf:ID= "WritingDevice">
<rdfs:subClassOf rdf:resource ="http://127.0.0.1:8000/ontology/SUMO.owl#Device"/>
<rdfs:comment>A Device whose purpose is to be an instrument
of Writing, e.g. pens, pencils, crayons, etc.</rdfs:comment>
</owl:Class>

<owl:Class rdf:ID= "WrittenCommunication">
<rdfs:subClassOf rdf:resource 
="http://127.0.0.1:8000/ontology/SUMO.owl#LinguisticCommunication"/>
<rdfs:comment>Any LinguisticCommunication where the
instrument is a Text, e.g. a letter, an email, a memo, etc.</rdfs:comment>
</owl:Class>

<owl:Class rdf:ID= "XRayRadiation">
<rdfs:subClassOf rdf:resource 
="http://127.0.0.1:8000/ontology/SUMO.owl#Radiating"/>
<rdfs:comment>Electro-magnetic radiation of short wavelength,
often made use of by devices that scan the inside of objects.</rdfs:comment>
</owl:Class>

<owl:Class rdf:ID= "YardLength">
<rdfs:subClassOf rdf:resource 
="http://127.0.0.1:8000/ontology/SUMO.owl#LengthMeasure"/>
<rdf:type rdf:resource = 
"http://127.0.0.1:8000/ontology/SUMO.owl#UnitOfMeasure"/>
<rdfs:comment>English unit of length, equal to 3 FeetLength.</rdfs:comment>
</owl:Class>

<owl:Class rdf:ID= "Zinc">
<rdfs:subClassOf rdf:resource 
="http://127.0.0.1:8000/ontology/SUMO.owl#ElementalSubstance"/>
<atomicNumber>30</atomicNumber>
<rdfs:comment>Blue-white metallic element.  Occurs in multiple
compounds naturally.  Five stable isotopes are six radioactive isotopes
have been found.  Chemically a reactive metal, combines with oxygen and
other non-metals, reacts with dilute acids to release 
hydrogen.</rdfs:comment>
</owl:Class>

<owl:ObjectProperty   rdf:ID= "BeginNodeFn">
<rdfs:comment>A UnaryFunction that maps a GraphPath
to the GraphNode that is the beginning of the GraphPath.  Note that,
unlike InitialNodeFn (which relates a GraphArc to a GraphNode),
BeginNodeFn is a total function - every GraphPath has a 
beginning.</rdfs:comment>
<rdf:type rdf:resource = 
"http://127.0.0.1:8000/ontology/SUMO.owl#UnaryFunction"/>
<rdf:type rdf:resource = 
"http://127.0.0.1:8000/ontology/SUMO.owl#TotalValuedRelation"/>
<rdfs:domain rdf:resource="#GraphPath"/>
<rdfs:range rdf:resource = "#GraphNode"/>
<sumo:relatedInternalConcept rdf:resource = "#InitialNodeFn" />
</owl:ObjectProperty>

<owl:ObjectProperty   rdf:ID= "CenterOfCircleFn">
<rdfs:comment>(CenterOfCircleFn ?CIRCLE) denotes the
GeometricPoint that is the center of the Circle ?CIRCLE.</rdfs:comment>
<rdf:type rdf:resource = 
"http://127.0.0.1:8000/ontology/SUMO.owl#UnaryFunction"/>
<rdf:type rdf:resource = 
"http://127.0.0.1:8000/ontology/SUMO.owl#TotalValuedRelation"/>
<rdfs:domain rdf:resource="#Circle"/>
<rdfs:range rdf:resource = 
"http://127.0.0.1:8000/ontology/SUMO.owl#GeometricPoint"/>
</owl:ObjectProperty>

<owl:ObjectProperty   rdf:ID= "CitizenryFn">
<rdfs:comment>(CitizenryFn ?AREA) denotes the
GroupOfPeople who are legal and permanent residents of the
GeopoliticalArea ?AREA.</rdfs:comment>
<rdfs:domain 
rdf:resource="http://127.0.0.1:8000/ontology/SUMO.owl#GeopoliticalArea"/>
<rdfs:range rdf:resource = 
"http://127.0.0.1:8000/ontology/SUMO.owl#GroupOfPeople"/>
<rdfs:subPropertyOf rdf:resource="#ResidentFn"/>
</owl:ObjectProperty>

<owl:ObjectProperty   rdf:ID= "CutSetFn">
<rdfs:comment>A UnaryFunction that assigns a Graph the
Class of GraphPaths that partition the graph into two separate
graphs if cut.  There may be more than one cutset for a given 
graph.</rdfs:comment>
<rdf:type rdf:resource = 
"http://127.0.0.1:8000/ontology/SUMO.owl#UnaryFunction"/>
<rdfs:domain rdf:resource="#Graph"/>
<sumo:rangeSubclass rdf:resource = "#GraphPath" />
</owl:ObjectProperty>

<owl:ObjectProperty   rdf:ID= "DescendantsFn">
<rdfs:comment>(DescendantsFn ?PERSON) denotes all and only
the descendants of ?PERSON, i.e. the Group consisting of ?OFFSPRING who
satisfy the following formula:  (ancestor ?OFFSPRING 
?PERSON).</rdfs:comment>
<rdf:type rdf:resource = 
"http://127.0.0.1:8000/ontology/SUMO.owl#UnaryFunction"/>
<rdfs:domain rdf:resource="http://127.0.0.1:8000/ontology/SUMO.owl#Human"/>
<rdfs:range rdf:resource = 
"http://127.0.0.1:8000/ontology/SUMO.owl#FamilyGroup"/>
</owl:ObjectProperty>

<owl:ObjectProperty   rdf:ID= "DiameterFn">
<rdfs:comment>(DiameterFn ?CIRCLE) denotes the length of the
diameter of the Circle ?CIRCLE.</rdfs:comment>
<rdf:type rdf:resource = 
"http://127.0.0.1:8000/ontology/SUMO.owl#UnaryFunction"/>
<rdf:type rdf:resource = 
"http://127.0.0.1:8000/ontology/SUMO.owl#TotalValuedRelation"/>
<rdfs:domain rdf:resource="#Circle"/>
<rdfs:range rdf:resource = 
"http://127.0.0.1:8000/ontology/SUMO.owl#LengthMeasure"/>
</owl:ObjectProperty>

<owl:ObjectProperty   rdf:ID= "DocumentFn">
<rdfs:comment>(DocumentFn ?PROP) denotes the class
of ContentBearingObjects that contain the information ?PROP.</rdfs:comment>
<rdf:type rdf:resource = 
"http://127.0.0.1:8000/ontology/SUMO.owl#UnaryFunction"/>
<rdfs:domain rdf:resource="http://127.0.0.1:8000/ontology/SUMO.owl#Proposition"/>
<sumo:rangeSubclass rdf:resource = "http://127.0.0.1:8000/ontology/SUMO.owl#Text"
/>
</owl:ObjectProperty>

<owl:ObjectProperty   rdf:ID= "EndNodeFn">
<rdfs:comment>A UnaryFunction that maps a GraphPath
to the GraphNode that is the end of the GraphPath.  Note that, unlike
TerminalNodeFn (which relates a GraphArc to a GraphNode),
EndNodeFn is a total function - every GraphPath has a end.</rdfs:comment>
<rdf:type rdf:resource = 
"http://127.0.0.1:8000/ontology/SUMO.owl#UnaryFunction"/>
<rdf:type rdf:resource = 
"http://127.0.0.1:8000/ontology/SUMO.owl#TotalValuedRelation"/>
<rdfs:domain rdf:resource="#GraphPath"/>
<rdfs:range rdf:resource = "#GraphNode"/>
<sumo:relatedInternalConcept rdf:resource = "#TerminalNodeFn" />
</owl:ObjectProperty>

<owl:ObjectProperty   rdf:ID= "ExecutiveBranchFn">
<rdfs:comment>(ExecutiveBranchFn ?ORG) denotes the
executive branch of ?ORG, with all its officials and agencies, considered
as a whole.</rdfs:comment>
<rdf:type rdf:resource = 
"http://127.0.0.1:8000/ontology/SUMO.owl#UnaryFunction"/>
<rdfs:domain rdf:resource="http://127.0.0.1:8000/ontology/SUMO.owl#Agent"/>
<rdfs:range rdf:resource = 
"http://127.0.0.1:8000/ontology/SUMO.owl#Organization"/>
</owl:ObjectProperty>

<owl:ObjectProperty   rdf:ID= "FirstFn">
<rdfs:comment>(FirstFn ?LIST) returns the first item in
the List ?LIST.  For example, (FirstFn (ListFn Monday Tuesday
Wednesday)) would return the value of Monday.</rdfs:comment>
<rdf:type rdf:resource = 
"http://127.0.0.1:8000/ontology/SUMO.owl#UnaryFunction"/>
<rdfs:domain rdf:resource="http://127.0.0.1:8000/ontology/SUMO.owl#List"/>
<rdfs:range rdf:resource = "http://127.0.0.1:8000/ontology/SUMO.owl#Entity"/>
</owl:ObjectProperty>

<owl:ObjectProperty   rdf:ID= "InitialNodeFn">
<rdfs:comment>A UnaryFunction that maps a
GraphArc to the initial node of the GraphArc.  Note
that this is a partial function.  In particular, the function is
undefined for GraphArcs that are not part of a DirectedGraph.</rdfs:comment>
<rdf:type rdf:resource = 
"http://127.0.0.1:8000/ontology/SUMO.owl#UnaryFunction"/>
<rdf:type rdf:resource = 
"http://127.0.0.1:8000/ontology/SUMO.owl#PartialValuedRelation"/>
<rdfs:domain rdf:resource="#GraphArc"/>
<rdfs:range rdf:resource = "#GraphNode"/>
</owl:ObjectProperty>

<owl:ObjectProperty   rdf:ID= "JudiciaryFn">
<rdfs:comment>(JudiciaryFn ?AREA) denotes the judicial
branch of the GeopoliticalArea ?AREA, that is, the
JudicialOrganization(s) associated with the government of ?AREA,
considered as a whole.</rdfs:comment>
<rdf:type rdf:resource = 
"http://127.0.0.1:8000/ontology/SUMO.owl#UnaryFunction"/>
<rdfs:domain 
rdf:resource="http://127.0.0.1:8000/ontology/SUMO.owl#GeopoliticalArea"/>
<rdfs:range rdf:resource = 
"http://127.0.0.1:8000/ontology/SUMO.owl#GovernmentOrganization"/>
<rdfs:range rdf:resource = 
"http://127.0.0.1:8000/ontology/SUMO.owl#JudicialOrganization"/>
</owl:ObjectProperty>

<owl:ObjectProperty   rdf:ID= "LastFn">
<rdfs:comment>(LastFn ?LIST) returns the last item in the
List ?LIST.  For example, (LastFn (ListFn Monday Tuesday
Wednesday)) would return the value of Wednesday.</rdfs:comment>
<rdf:type rdf:resource = 
"http://127.0.0.1:8000/ontology/SUMO.owl#UnaryFunction"/>
<rdfs:domain rdf:resource="http://127.0.0.1:8000/ontology/SUMO.owl#List"/>
<rdfs:range rdf:resource = "http://127.0.0.1:8000/ontology/SUMO.owl#Entity"/>
</owl:ObjectProperty>

<owl:ObjectProperty   rdf:ID= "LegislatureFn">
<rdfs:comment>(LegislatureFn ?AREA) denotes the
legislative branch of the GeopoliticalArea ?AREA.</rdfs:comment>
<rdf:type rdf:resource = 
"http://127.0.0.1:8000/ontology/SUMO.owl#UnaryFunction"/>
<rdfs:domain 
rdf:resource="http://127.0.0.1:8000/ontology/SUMO.owl#GeopoliticalArea"/>
<rdfs:range rdf:resource = "#LegislativeOrganization"/>
</owl:ObjectProperty>

<owl:ObjectProperty   rdf:ID= "MinimalCutSetFn">
<rdfs:comment>A UnaryFunction that assigns a Graph
the Class of GraphPaths which comprise cutsets for the Graph and
which have the least number of GraphArcs.</rdfs:comment>
<rdf:type rdf:resource = 
"http://127.0.0.1:8000/ontology/SUMO.owl#UnaryFunction"/>
<rdfs:domain rdf:resource="#Graph"/>
<sumo:rangeSubclass rdf:resource = "#GraphPath" />
<sumo:relatedInternalConcept rdf:resource = "#CutSetFn" />
</owl:ObjectProperty>

<owl:ObjectProperty   rdf:ID= "OccupationFn">
<rdfs:comment>(OccupationFn ?PROCESS) denotes the
subclass of ?PROCESS where instances of ?PROCESS are performed as
one's occupation, i.e. as part of a FinancialTransaction where one
earns money for the performance of ?PROCESS.</rdfs:comment>
<rdf:type rdf:resource = 
"http://127.0.0.1:8000/ontology/SUMO.owl#UnaryFunction"/>
<rdfs:domain 
rdf:resource="http://127.0.0.1:8000/ontology/SUMO.owl#IntentionalProcess"/>
<sumo:rangeSubclass rdf:resource = 
"http://127.0.0.1:8000/ontology/SUMO.owl#FinancialTransaction" />
</owl:ObjectProperty>

<owl:ObjectProperty   rdf:ID= "OperatingFn">
<rdfs:comment>(OperatingFn ?TYPE) denotes the class
of events in which a Device of ?TYPE is being operated.</rdfs:comment>
<rdf:type rdf:resource = 
"http://127.0.0.1:8000/ontology/SUMO.owl#UnaryFunction"/>
<rdfs:domain rdf:resource="http://127.0.0.1:8000/ontology/SUMO.owl#Device"/>
<sumo:rangeSubclass rdf:resource = 
"http://127.0.0.1:8000/ontology/SUMO.owl#Process" />
</owl:ObjectProperty>

<owl:DatatypeProperty  rdf:ID= "PathWeightFn">
<rdfs:comment>A UnaryFunction that maps a
GraphPath to the sum of the arcWeights on the GraphArcs in
the GraphPath.</rdfs:comment>
<rdf:type rdf:resource = 
"http://127.0.0.1:8000/ontology/SUMO.owl#UnaryFunction"/>
<rdfs:domain rdf:resource="#GraphPath"/>
<rdfs:range rdf:resource = "http://127.0.0.1:8000/ontology/SUMO.owl#RealNumber"/>
</owl:DatatypeProperty>

<owl:DatatypeProperty  rdf:ID= "PopulationFn">
<rdfs:comment>(PopulationFn ?AREA) denotes the Integer
that represents the count of the number of people inhabiting the
GeopoliticalArea ?AREA.  The total population presents one overall
measure of the potential impact of the country on the world and within its
region.</rdfs:comment>
<rdf:type rdf:resource = 
"http://127.0.0.1:8000/ontology/SUMO.owl#UnaryFunction"/>
<rdfs:range rdf:resource = "http://127.0.0.1:8000/ontology/SUMO.owl#Integer"/>
<sumo:domain rdf:resource = 
"http://127.0.0.1:8000/ontology/SUMO.owl#GeopoliticalArea" />
</owl:DatatypeProperty>

<owl:ObjectProperty   rdf:ID= "RadiusFn">
<rdfs:comment>(RadiusFn ?CIRCLE) denotes the length of the radius
of the Circle ?CIRCLE.</rdfs:comment>
<rdf:type rdf:resource = 
"http://127.0.0.1:8000/ontology/SUMO.owl#UnaryFunction"/>
<rdf:type rdf:resource = 
"http://127.0.0.1:8000/ontology/SUMO.owl#TotalValuedRelation"/>
<rdfs:domain rdf:resource="#Circle"/>
<rdfs:range rdf:resource = 
"http://127.0.0.1:8000/ontology/SUMO.owl#LengthMeasure"/>
</owl:ObjectProperty>

<owl:ObjectProperty   rdf:ID= "ResidentFn">
<rdfs:comment>(ResidentFn ?AREA) denotes the
GroupOfPeople who have their home in ?AREA.</rdfs:comment>
<rdf:type rdf:resource = 
"http://127.0.0.1:8000/ontology/SUMO.owl#UnaryFunction"/>
<rdfs:domain 
rdf:resource="http://127.0.0.1:8000/ontology/SUMO.owl#GeopoliticalArea"/>
<rdfs:range rdf:resource = 
"http://127.0.0.1:8000/ontology/SUMO.owl#GroupOfPeople"/>
</owl:ObjectProperty>

<owl:ObjectProperty   rdf:ID= "StartFn">
<rdfs:comment>(StartFn ?PROCESS) denotes IntentionalProcesses
of bringing it about that Processes of type ?PROCESS begin, e.g. start
working, begin running, etc.</rdfs:comment>
<rdf:type rdf:resource = 
"http://127.0.0.1:8000/ontology/SUMO.owl#UnaryFunction"/>
<rdfs:domain rdf:resource="http://127.0.0.1:8000/ontology/SUMO.owl#Process"/>
<sumo:rangeSubclass rdf:resource = 
"http://127.0.0.1:8000/ontology/SUMO.owl#IntentionalProcess" />
</owl:ObjectProperty>

<owl:ObjectProperty   rdf:ID= "StopFn">
<rdfs:comment>(StopFn ?PROCESS) denotes IntentionalProcesses
of bringing it about that Processes of type ?PROCESS end, e.g. stop
walking, quit working, etc.</rdfs:comment>
<rdf:type rdf:resource = 
"http://127.0.0.1:8000/ontology/SUMO.owl#UnaryFunction"/>
<rdfs:domain rdf:resource="http://127.0.0.1:8000/ontology/SUMO.owl#Process"/>
<sumo:rangeSubclass rdf:resource = 
"http://127.0.0.1:8000/ontology/SUMO.owl#IntentionalProcess" />
</owl:ObjectProperty>

<owl:ObjectProperty   rdf:ID= "TerminalNodeFn">
<rdfs:comment>A UnaryFunction that maps a
GraphArc to the terminal node of the GraphArc.  Note that this
is a partial function.  In particular, the function is undefined
for GraphArcs that are not part of a DirectedGraph.</rdfs:comment>
<rdf:type rdf:resource = 
"http://127.0.0.1:8000/ontology/SUMO.owl#UnaryFunction"/>
<rdf:type rdf:resource = 
"http://127.0.0.1:8000/ontology/SUMO.owl#PartialValuedRelation"/>
<rdfs:domain rdf:resource="#GraphArc"/>
<rdfs:range rdf:resource = "#GraphNode"/>
</owl:ObjectProperty>

<owl:ObjectProperty   rdf:ID= "abbreviation">
<rdfs:comment>(abbreviation ?STRING ?THING) means that
?STRING is an abbreviation used to refer to ?THING.  Abbreviations include
acronyms and other abbreviated forms.</rdfs:comment>
<rdfs:subPropertyOf rdf:resource="#conventionalShortName"/>
</owl:ObjectProperty>

<owl:ObjectProperty   rdf:ID= "accountHolder">
<rdfs:comment>(accountHolder ?Account ?Agent) means that
?Agent is the account holder of the FinancialAccount 
?Account.</rdfs:comment>
<rdfs:domain rdf:resource="#FinancialAccount"/>
<rdfs:range rdf:resource = 
"http://127.0.0.1:8000/ontology/SUMO.owl#CognitiveAgent"/>
<rdfs:subPropertyOf rdf:resource="#agreementMember"/>
</owl:ObjectProperty>

<owl:ObjectProperty   rdf:ID= "address">
<rdfs:comment>(address ?AGENT ?ADDRESS) means that ?ADDRESS
is an address or part of an address for the Agent ?AGENT.</rdfs:comment>
<rdf:type rdf:resource = 
"http://127.0.0.1:8000/ontology/SUMO.owl#BinaryPredicate"/>
<rdfs:domain rdf:resource="http://127.0.0.1:8000/ontology/SUMO.owl#Agent"/>
<rdfs:range rdf:resource = "#Address"/>
</owl:ObjectProperty>

<owl:ObjectProperty   rdf:ID= "administrativeCenter">
<rdfs:comment>(administrativeCenter ?CENTER
?REGION) means that ?CENTER is the City (or other area) from which
the larger GeopoliticalArea ?REGION is administered.</rdfs:comment>
<rdf:type rdf:resource = 
"http://127.0.0.1:8000/ontology/SUMO.owl#BinaryPredicate"/>
<rdfs:domain 
rdf:resource="http://127.0.0.1:8000/ontology/SUMO.owl#GeopoliticalArea"/>
<rdfs:range rdf:resource = 
"http://127.0.0.1:8000/ontology/SUMO.owl#GeopoliticalArea"/>
<rdfs:subPropertyOf 
rdf:resource="http://127.0.0.1:8000/ontology/SUMO.owl#geopoliticalSubdivision"/>
</owl:ObjectProperty>

<owl:ObjectProperty   rdf:ID= "affiliatedOrganization">
<rdf:type rdf:resource = 
"http://127.0.0.1:8000/ontology/SUMO.owl#BinaryPredicate"/>
<rdfs:domain 
rdf:resource="http://127.0.0.1:8000/ontology/SUMO.owl#CognitiveAgent"/>
<rdfs:range rdf:resource = 
"http://127.0.0.1:8000/ontology/SUMO.owl#CognitiveAgent"/>
</owl:ObjectProperty>

<owl:ObjectProperty  rdf:about= "http://127.0.0.1:8000/ontology/SUMO.owl#agent">
<rdfs:subPropertyOf rdf:resource="#involvedInEvent"/>
</owl:ObjectProperty>

<owl:ObjectProperty   rdf:ID= "agentOperatesInArea">
<rdfs:comment>(agentOperatesInArea ?ORG ?AREA) means that the Organization
?ORG conducts operations (i.e. instances of IntentionalProcess) in 
?AREA.</rdfs:comment>
<rdfs:domain 
rdf:resource="http://127.0.0.1:8000/ontology/SUMO.owl#Organization"/>
<rdfs:range rdf:resource = 
"http://127.0.0.1:8000/ontology/SUMO.owl#GeopoliticalArea"/>
<rdfs:subPropertyOf 
rdf:resource="http://127.0.0.1:8000/ontology/SUMO.owl#located"/>
</owl:ObjectProperty>

<owl:ObjectProperty   rdf:ID= "agreementMember">
<rdfs:comment>(agreementMember ?Agreement ?Agent)
means that ?Agent is one of the participants of the DeonticAttribute
?Agreement.</rdfs:comment>
<rdf:type rdf:resource = 
"http://127.0.0.1:8000/ontology/SUMO.owl#BinaryPredicate"/>
<rdf:type rdf:resource = 
"http://127.0.0.1:8000/ontology/SUMO.owl#TotalValuedRelation"/>
<rdfs:domain 
rdf:resource="http://127.0.0.1:8000/ontology/SUMO.owl#DeonticAttribute"/>
<rdfs:range rdf:resource = "http://127.0.0.1:8000/ontology/SUMO.owl#Agent"/>
</owl:ObjectProperty>

<owl:ObjectProperty   rdf:ID= "agreementPeriod">
<rdfs:comment>(agreementPeriod ?Agreement ?Period) holds if
?Period specifies a Time interval during which ?Agreement is in 
force.</rdfs:comment>
<rdf:type rdf:resource = 
"http://127.0.0.1:8000/ontology/SUMO.owl#BinaryPredicate"/>
<rdfs:domain rdf:resource="http://127.0.0.1:8000/ontology/SUMO.owl#Contract"/>
<rdfs:range rdf:resource = 
"http://127.0.0.1:8000/ontology/SUMO.owl#TimeInterval"/>
</owl:ObjectProperty>

<owl:ObjectProperty   rdf:ID= "airTemperature">
<rdfs:comment>(airTemperature ?AREA ?TEMP) means that
the temperature of the air at ?AREA is ?TEMP.  Temperature is expressed
in units of TemperatureMeasure, including CelsiusDegree and
FahrenheitDegree, among others.</rdfs:comment>
<rdf:type rdf:resource = 
"http://127.0.0.1:8000/ontology/SUMO.owl#AsymmetricRelation"/>
<rdfs:domain rdf:resource="http://127.0.0.1:8000/ontology/SUMO.owl#Object"/>
<rdfs:range rdf:resource = 
"http://127.0.0.1:8000/ontology/SUMO.owl#TemperatureMeasure"/>
<rdfs:subPropertyOf 
rdf:resource="http://127.0.0.1:8000/ontology/SUMO.owl#measure"/>
</owl:ObjectProperty>

<owl:ObjectProperty   rdf:ID= "allegiance">
<rdfs:comment>(allegiance ?AGENT ?ENTITY) means that the CognitiveAgent
?AGENT owes its allegiance to the political entity ?ENTITY.</rdfs:comment>
<rdf:type rdf:resource = 
"http://127.0.0.1:8000/ontology/SUMO.owl#BinaryPredicate"/>
<rdfs:domain 
rdf:resource="http://127.0.0.1:8000/ontology/SUMO.owl#CognitiveAgent"/>
<rdfs:range rdf:resource = 
"http://127.0.0.1:8000/ontology/SUMO.owl#CognitiveAgent"/>
</owl:ObjectProperty>

<owl:ObjectProperty   rdf:ID= "ancestorOrganization">
<rdfs:comment>(ancestorOrganization ?ORG1 ?ORG2) means that
the Organization ?ORG1 descended from the Organization ?ORG2.</rdfs:comment>
<rdf:type rdf:resource = 
"http://127.0.0.1:8000/ontology/SUMO.owl#BinaryPredicate"/>
<rdf:type rdf:resource = 
"http://127.0.0.1:8000/ontology/SUMO.owl#TransitiveRelation"/>
<rdf:type rdf:resource = 
"http://127.0.0.1:8000/ontology/SUMO.owl#IrreflexiveRelation"/>
<rdfs:domain 
rdf:resource="http://127.0.0.1:8000/ontology/SUMO.owl#Organization"/>
<rdfs:range rdf:resource = 
"http://127.0.0.1:8000/ontology/SUMO.owl#Organization"/>
<sumo:disjointRelation rdf:resource = 
"http://127.0.0.1:8000/ontology/SUMO.owl#subOrganization" />
</owl:ObjectProperty>

<owl:ObjectProperty   rdf:ID= "anniversary">
<rdfs:comment>(anniversary ?PHYSICAL ?TIME) means that
?TIME is the class of TimeIntervals which mark the anniversary of
?PHYSICAL.  For example, (anniversary Christmas (DayFn 35 December))
means that Christmas is celebrated each year on the 25th of 
December.</rdfs:comment>
<rdf:type rdf:resource = 
"http://127.0.0.1:8000/ontology/SUMO.owl#BinaryPredicate"/>
<rdf:type rdf:resource = 
"http://127.0.0.1:8000/ontology/SUMO.owl#TemporalRelation"/>
<rdfs:domain rdf:resource="http://127.0.0.1:8000/ontology/SUMO.owl#Physical"/>
<rdfs:range rdf:resource = 
"http://127.0.0.1:8000/ontology/SUMO.owl#TimeInterval"/>
</owl:ObjectProperty>

<owl:DatatypeProperty  rdf:ID= "arcWeight">
<rdfs:comment>This predicate indicates the value of a
GraphArc in a Graph.  This could map to the length of a road in
a road network or the flow rate of a pipe in a plumbing 
system.</rdfs:comment>
<rdf:type rdf:resource = 
"http://127.0.0.1:8000/ontology/SUMO.owl#BinaryPredicate"/>
<rdf:type rdf:resource = 
"http://127.0.0.1:8000/ontology/SUMO.owl#SingleValuedRelation"/>
<rdfs:domain rdf:resource="#GraphArc"/>
<rdfs:range rdf:resource = "http://127.0.0.1:8000/ontology/SUMO.owl#RealNumber"/>
</owl:DatatypeProperty>

<owl:DatatypeProperty  rdf:ID= "atomicNumber">
<rdfs:comment>(atomicNumber ?ELEMENT ?NUMBER) means that the
ElementalSubstance ?ELEMENT has the atomic number ?NUMBER. The atomic number
is the number of Protons in the nucleus of an Atom.</rdfs:comment>
<rdfs:domain 
rdf:resource="http://127.0.0.1:8000/ontology/SUMO.owl#ElementalSubstance"/>
<rdfs:range rdf:resource = 
"http://127.0.0.1:8000/ontology/SUMO.owl#PositiveInteger"/>
<rdfs:subPropertyOf rdf:resource="#protonNumber"/>
</owl:DatatypeProperty>

<owl:ObjectProperty   rdf:ID= "aunt">
<rdfs:comment>(aunt ?AUNT ?PERSON) means that ?AUNT is
the sister of a parent of ?PERSON.</rdfs:comment>
<rdfs:domain rdf:resource="http://127.0.0.1:8000/ontology/SUMO.owl#Woman"/>
<rdfs:range rdf:resource = "http://127.0.0.1:8000/ontology/SUMO.owl#Human"/>
<rdfs:subPropertyOf 
rdf:resource="http://127.0.0.1:8000/ontology/SUMO.owl#familyRelation"/>
</owl:ObjectProperty>

<owl:DatatypeProperty  rdf:ID= "average">
<rdfs:comment>A partial function that relates a List to a
RealNumber, provided that the List only has list elements that are
RealNumbers. The RealNumber associated with the List is equal to the
mathematical average of the RealNumbers in the List divided by the total
number of list elements.</rdfs:comment>
<rdf:type rdf:resource = 
"http://127.0.0.1:8000/ontology/SUMO.owl#BinaryPredicate"/>
<rdf:type rdf:resource = 
"http://127.0.0.1:8000/ontology/SUMO.owl#PartialValuedRelation"/>
<rdf:type rdf:resource = 
"http://127.0.0.1:8000/ontology/SUMO.owl#SingleValuedRelation"/>
<rdfs:domain rdf:resource="http://127.0.0.1:8000/ontology/SUMO.owl#List"/>
<rdfs:range rdf:resource = "http://127.0.0.1:8000/ontology/SUMO.owl#RealNumber"/>
</owl:DatatypeProperty>

<owl:ObjectProperty   rdf:ID= "barometricPressure">
<rdfs:comment>(barometricPressure ?AREA ?PRESSURE)
means that the atmospheric pressure measured at ?AREA is ?PRESSURE.
Barometric pressure is typically expressed in units of InchMercury or
MmMercury.  For example, standard sea level pressure is 29.92 inches
(760 mm) of mercury: (barometricPressure SeaLevel (MeasureFn 29.92
InchMercury)).</rdfs:comment>
<rdf:type rdf:resource = 
"http://127.0.0.1:8000/ontology/SUMO.owl#BinaryPredicate"/>
<rdf:type rdf:resource = 
"http://127.0.0.1:8000/ontology/SUMO.owl#AsymmetricRelation"/>
<rdfs:domain rdf:resource="http://127.0.0.1:8000/ontology/SUMO.owl#Object"/>
<rdfs:range rdf:resource = "#AtmosphericPressureMeasure"/>
<rdfs:subPropertyOf 
rdf:resource="http://127.0.0.1:8000/ontology/SUMO.owl#measure"/>
</owl:ObjectProperty>

<owl:ObjectProperty   rdf:ID= "birthday">
<rdfs:comment>(birthday ?PERSON ?DAY) means that ?DAY is the
anniversary each year of the birth of ?PERSON.  For example, (birthday
WilliamJeffersonClinton (DayFn 19 August)) means that Bill Clinton's
birthday is August 19th.</rdfs:comment>
<rdfs:domain rdf:resource="http://127.0.0.1:8000/ontology/SUMO.owl#Human"/>
<rdfs:range rdf:resource = "http://127.0.0.1:8000/ontology/SUMO.owl#Day"/>
<rdfs:subPropertyOf rdf:resource="#anniversary"/>
</owl:ObjectProperty>

<owl:ObjectProperty   rdf:ID= "birthplace">
<rdfs:comment>(birthplace ?INDIV ?PLACE) means that the Animal ?INDIV was 
born
at the location ?PLACE.  The location may be a geographic area or a 
building, such as a hospital.</rdfs:comment>
<rdf:type rdf:resource = 
"http://127.0.0.1:8000/ontology/SUMO.owl#BinaryPredicate"/>
<rdfs:domain rdf:resource="http://127.0.0.1:8000/ontology/SUMO.owl#Animal"/>
<rdfs:range rdf:resource = "http://127.0.0.1:8000/ontology/SUMO.owl#Object"/>
</owl:ObjectProperty>

<owl:ObjectProperty   rdf:ID= "borrower">
<rdfs:comment>(borrower ?Loan ?Agent) means that ?Agent is a borrower of the 
?Loan</rdfs:comment>
<rdfs:domain rdf:resource="#Loan"/>
<rdfs:range rdf:resource = 
"http://127.0.0.1:8000/ontology/SUMO.owl#CognitiveAgent"/>
<rdfs:subPropertyOf rdf:resource="#agreementMember"/>
</owl:ObjectProperty>

<owl:ObjectProperty   rdf:ID= "brandName">
<rdfs:comment>(brandName ?NAME ?PRODUCT) means that ?NAME
is the brand name for the product class ?PRODUCT, e.g. Cheerios is the
brand name for a certain class of breakfast cereal.</rdfs:comment>
<rdfs:range rdf:resource = "http://127.0.0.1:8000/ontology/SUMO.owl#Product"/>
<rdfs:subPropertyOf 
rdf:resource="http://127.0.0.1:8000/ontology/SUMO.owl#names"/>
<sumo:domain rdf:resource = 
"http://127.0.0.1:8000/ontology/SUMO.owl#SymbolicString" />
</owl:ObjectProperty>

<owl:ObjectProperty   rdf:ID= "capacity">
<rdfs:comment>(capacity ?OBJ ?QUANTITY) means that ?OBJ can contain
something that has the measure of ?QUANTITY.  This predicate denotes maximal
capacity, i.e. ?OBJ can hold no more than ?QUANTITY.  Note, however, that 
this
does not mean that capacity is a SingleValuedRelation, since an object may
have various maximal capacities across different dimensions, e.g. a 
particular
box may have a capacity of 3 pounds and a capacity of 1 
liter.</rdfs:comment>
<rdf:type rdf:resource = 
"http://127.0.0.1:8000/ontology/SUMO.owl#BinaryPredicate"/>
<rdfs:domain 
rdf:resource="http://127.0.0.1:8000/ontology/SUMO.owl#SelfConnectedObject"/>
<rdfs:range rdf:resource = 
"http://127.0.0.1:8000/ontology/SUMO.owl#ConstantQuantity"/>
<sumo:relatedInternalConcept rdf:resource = "#humanCapacity" />
</owl:ObjectProperty>

<owl:ObjectProperty   rdf:ID= "capitalCity">
<rdfs:comment>(capitalCity ?CITY ?REGION) means that the
City ?CITY is the capital of the GeopoliticalArea ?REGION.</rdfs:comment>
<rdf:type rdf:resource = 
"http://127.0.0.1:8000/ontology/SUMO.owl#BinaryPredicate"/>
<rdfs:domain rdf:resource="http://127.0.0.1:8000/ontology/SUMO.owl#City"/>
<rdfs:range rdf:resource = 
"http://127.0.0.1:8000/ontology/SUMO.owl#GeopoliticalArea"/>
<rdfs:subPropertyOf rdf:resource="#administrativeCenter"/>
</owl:ObjectProperty>

<owl:ObjectProperty   rdf:ID= "cargoType">
<rdfs:comment>(cargoType ?DEVICE ?TYPE) means that the
TransportationDevice ?DEVICE can, and typically does, carry cargo of
the kind ?TYPE.</rdfs:comment>
<rdf:type rdf:resource = 
"http://127.0.0.1:8000/ontology/SUMO.owl#BinaryPredicate"/>
<rdfs:domain 
rdf:resource="http://127.0.0.1:8000/ontology/SUMO.owl#TransportationDevice"/>
<rdfs:range rdf:resource = "http://127.0.0.1:8000/ontology/SUMO.owl#Object"/>
</owl:ObjectProperty>

<owl:ObjectProperty  rdf:about= "http://127.0.0.1:8000/ontology/SUMO.owl#causes">
<rdfs:subPropertyOf rdf:resource="#relatedEvent"/>
</owl:ObjectProperty>

<owl:ObjectProperty   rdf:ID= "checkAccount">
<rdfs:comment>(checkAccount ?Check ?Account) means that ?Account
is the FinancialAccount from which the amount specifed on the check is 
paid.</rdfs:comment>
<rdf:type rdf:resource = 
"http://127.0.0.1:8000/ontology/SUMO.owl#BinaryPredicate"/>
<rdfs:domain rdf:resource="#Check"/>
<rdfs:range rdf:resource = "#FinancialAccount"/>
</owl:ObjectProperty>

<owl:ObjectProperty   rdf:ID= "cityAddress">
<rdfs:comment>(cityAddress ?CITY ?ADDRESS) means that the
City ?CITY is part of the address ?ADDRESS.</rdfs:comment>
<rdfs:domain rdf:resource="http://127.0.0.1:8000/ontology/SUMO.owl#City"/>
<rdfs:range rdf:resource = "#Address"/>
<rdfs:subPropertyOf rdf:resource="#address"/>
</owl:ObjectProperty>

<owl:ObjectProperty   rdf:ID= "climateTypeInArea">
<rdfs:comment>(climateTypeInArea ?TYPE ?REGION)
means that all or part of the GeographicArea ?REGION is of the
ClimateZone ?TYPE.</rdfs:comment>
<rdf:type rdf:resource = 
"http://127.0.0.1:8000/ontology/SUMO.owl#BinaryPredicate"/>
<rdfs:domain 
rdf:resource="http://127.0.0.1:8000/ontology/SUMO.owl#GeographicArea"/>
<rdfs:range rdf:resource = "#ClimateZone"/>
</owl:ObjectProperty>

<owl:ObjectProperty   rdf:ID= "conjugate">
<rdfs:comment>(conjugate ?COMPOUND1 ?COMPOUND2) means that
?COMPOUND1 and ?COMPOUND2 are identical CompoundSubstances except that
one has one more Proton than the other.</rdfs:comment>
<rdf:type rdf:resource = 
"http://127.0.0.1:8000/ontology/SUMO.owl#BinaryPredicate"/>
<rdf:type rdf:resource = 
"http://127.0.0.1:8000/ontology/SUMO.owl#IrreflexiveRelation"/>
<rdf:type rdf:resource = 
"http://127.0.0.1:8000/ontology/SUMO.owl#SymmetricRelation"/>
<rdf:type rdf:resource = 
"http://127.0.0.1:8000/ontology/SUMO.owl#TransitiveRelation"/>
<rdfs:domain 
rdf:resource="http://127.0.0.1:8000/ontology/SUMO.owl#CompoundSubstance"/>
<rdfs:range rdf:resource = 
"http://127.0.0.1:8000/ontology/SUMO.owl#CompoundSubstance"/>
</owl:ObjectProperty>

<owl:ObjectProperty   rdf:ID= "contestParticipant">
<rdfs:comment>(contestParticipant ?CONTEST ?AGENT)
means that ?AGENT is one of the sides in the Contest ?CONTEST.  For
example, if the ?CONTEST is a football game, then ?AGENT would be one of
the opposing teams.  For another example, if ?CONTEST is a Battle, then
?AGENT would be one of the sides fighting each other.</rdfs:comment>
<rdf:type rdf:resource = 
"http://127.0.0.1:8000/ontology/SUMO.owl#TotalValuedRelation"/>
<rdfs:domain rdf:resource="http://127.0.0.1:8000/ontology/SUMO.owl#Contest"/>
<rdfs:range rdf:resource = "http://127.0.0.1:8000/ontology/SUMO.owl#Agent"/>
<rdfs:subPropertyOf 
rdf:resource="http://127.0.0.1:8000/ontology/SUMO.owl#agent"/>
<rdfs:subPropertyOf rdf:resource="#involvedInEvent"/>
</owl:ObjectProperty>

<owl:ObjectProperty   rdf:ID= "conventionalLongName">
<rdfs:comment>(conventionalLongName ?NAME ?THING)
means that the string ?NAME is the long form of the name conventionally
used for ?THING.</rdfs:comment>
<rdfs:subPropertyOf 
rdf:resource="http://127.0.0.1:8000/ontology/SUMO.owl#names"/>
</owl:ObjectProperty>

<owl:ObjectProperty   rdf:ID= "conventionalShortName">
<rdfs:comment>(conventionalShortName ?NAME
?THING) means that the string ?NAME is the short form of the name
conventionally used for ?THING.  For a more specialized subset of short
names, see abbreviation.</rdfs:comment>
<rdfs:subPropertyOf 
rdf:resource="http://127.0.0.1:8000/ontology/SUMO.owl#names"/>
</owl:ObjectProperty>

<owl:ObjectProperty   rdf:ID= "couponInterest">
<rdfs:comment>(couponInterest ?BOND ?INTEREST) means that ?INTEREST is
the periodic interest payment made to bondholders during the life of the 
?BOND.</rdfs:comment>
<rdf:type rdf:resource = 
"http://127.0.0.1:8000/ontology/SUMO.owl#BinaryPredicate"/>
<rdfs:domain rdf:resource="#Bond"/>
<rdfs:range rdf:resource = 
"http://127.0.0.1:8000/ontology/SUMO.owl#CurrencyMeasure"/>
</owl:ObjectProperty>

<owl:ObjectProperty   rdf:ID= "cousin">
<rdfs:comment>(cousin ?PERSON1 ?PERSON2) means that ?PERSON1
and ?PERSON2 are cousins, i.e. ?PERSON1 and ?PERSON2 have grandparents
(but not parents) in common.</rdfs:comment>
<rdfs:domain rdf:resource="http://127.0.0.1:8000/ontology/SUMO.owl#Human"/>
<rdfs:range rdf:resource = "http://127.0.0.1:8000/ontology/SUMO.owl#Human"/>
<rdfs:subPropertyOf 
rdf:resource="http://127.0.0.1:8000/ontology/SUMO.owl#familyRelation"/>
</owl:ObjectProperty>

<owl:ObjectProperty   rdf:ID= "currencyType">
<rdfs:comment>(currencyType ?AREA ?UNIT) means
that the official currency used in the GeopoliticalArea ?AREA
is the UnitOfMeasure ?UNIT.</rdfs:comment>
<rdf:type rdf:resource = 
"http://127.0.0.1:8000/ontology/SUMO.owl#BinaryPredicate"/>
<rdfs:domain 
rdf:resource="http://127.0.0.1:8000/ontology/SUMO.owl#GeopoliticalArea"/>
<rdfs:range rdf:resource = 
"http://127.0.0.1:8000/ontology/SUMO.owl#UnitOfMeasure"/>
<rdfs:range rdf:resource = 
"http://127.0.0.1:8000/ontology/SUMO.owl#CurrencyMeasure"/>
</owl:ObjectProperty>

<owl:ObjectProperty   rdf:ID= "customer">
<rdfs:comment>A very general relation that exists whenever there
is a CommercialService between an Agent and an Organization.
(customer ?AGENT ?ORG) means that ?AGENT is a customer of the Corporation
?ORG.</rdfs:comment>
<rdf:type rdf:resource = 
"http://127.0.0.1:8000/ontology/SUMO.owl#IrreflexiveRelation"/>
<rdf:type rdf:resource = 
"http://127.0.0.1:8000/ontology/SUMO.owl#AsymmetricRelation"/>
<rdf:type rdf:resource = 
"http://127.0.0.1:8000/ontology/SUMO.owl#BinaryPredicate"/>
<rdfs:domain rdf:resource="http://127.0.0.1:8000/ontology/SUMO.owl#Agent"/>
<rdfs:range rdf:resource = 
"http://127.0.0.1:8000/ontology/SUMO.owl#Corporation"/>
</owl:ObjectProperty>

<owl:ObjectProperty   rdf:ID= "defendant">
<rdfs:comment>(defendant ?AGENT ?ACTION) means the LegalAction
?ACTION makes a legal claim against ?AGENT.</rdfs:comment>
<rdfs:domain 
rdf:resource="http://127.0.0.1:8000/ontology/SUMO.owl#CognitiveAgent"/>
<rdfs:range rdf:resource = 
"http://127.0.0.1:8000/ontology/SUMO.owl#LegalAction"/>
<rdfs:subPropertyOf 
rdf:resource="http://127.0.0.1:8000/ontology/SUMO.owl#patient"/>
<rdfs:subPropertyOf rdf:resource="#involvedInEvent"/>
</owl:ObjectProperty>

<owl:ObjectProperty   rdf:ID= "dependentGeopoliticalArea">
<rdfs:comment>(dependentGeopoliticalArea
?AREA1 ?AREA2) means that ?AREA1 is a geopolitical possession of the
GeopoliticalArea ?AREA2 and is not a geopoliticalSubdivision of
?AREA2.  For example, (dependentGeopoliticalArea Guam UnitedStates),
because Guam is a territory of the UnitedStates, not one of the fifty
U.S. states.  Contrast primaryGeopoliticalSubdivision.</rdfs:comment>
<rdf:type rdf:resource = 
"http://127.0.0.1:8000/ontology/SUMO.owl#AsymmetricRelation"/>
<rdf:type rdf:resource = 
"http://127.0.0.1:8000/ontology/SUMO.owl#TransitiveRelation"/>
<rdfs:domain 
rdf:resource="http://127.0.0.1:8000/ontology/SUMO.owl#GeopoliticalArea"/>
<rdfs:range rdf:resource = 
"http://127.0.0.1:8000/ontology/SUMO.owl#GeopoliticalArea"/>
<sumo:relatedInternalConcept rdf:resource = 
"#primaryGeopoliticalSubdivision" />
</owl:ObjectProperty>

<owl:ObjectProperty  rdf:about= 
"http://127.0.0.1:8000/ontology/SUMO.owl#destination">
<rdfs:subPropertyOf rdf:resource="#involvedInEvent"/>
</owl:ObjectProperty>

<owl:ObjectProperty   rdf:ID= "detainee">
<rdfs:comment>(detainee ?EVENT ?OBJECT) means that in the
Confining ?EVENT, the Object ?OBJECT is restrained by force, threat, or
other form of intimidation.</rdfs:comment>
<rdf:type rdf:resource = "http://127.0.0.1:8000/ontology/SUMO.owl#CaseRole"/>
<rdfs:domain rdf:resource="http://127.0.0.1:8000/ontology/SUMO.owl#Confining"/>
<rdfs:range rdf:resource = "http://127.0.0.1:8000/ontology/SUMO.owl#Animal"/>
<rdfs:subPropertyOf 
rdf:resource="http://127.0.0.1:8000/ontology/SUMO.owl#patient"/>
<rdfs:subPropertyOf rdf:resource="#involvedInEvent"/>
</owl:ObjectProperty>

<owl:ObjectProperty   rdf:ID= "deviceState">
<rdfs:comment>(deviceState ?DEVICE ?STATE) means that
the Object ?DEVICE is in the DeviceStateAttribute ?STATE.</rdfs:comment>
<rdf:type rdf:resource = 
"http://127.0.0.1:8000/ontology/SUMO.owl#BinaryPredicate"/>
<rdfs:domain rdf:resource="http://127.0.0.1:8000/ontology/SUMO.owl#Object"/>
<rdfs:range rdf:resource = "#DeviceStateAttribute"/>
</owl:ObjectProperty>

<owl:ObjectProperty  rdf:about= 
"http://127.0.0.1:8000/ontology/SUMO.owl#direction">
<rdfs:subPropertyOf rdf:resource="#involvedInEvent"/>
</owl:ObjectProperty>

<owl:ObjectProperty   rdf:ID= "disapproves">
<rdfs:comment>(disapproves ?AGENT ?FORMULA) means that
?AGENT has a feeling of antipathy to the state of affairs represented by
?FORMULA, i.e. ?AGENT believes that the realization of ?FORMULA will
thwart one of his/her goals.  Note that there is no implication that what
is disapproved of by an agent is not already true.</rdfs:comment>
<rdf:type rdf:resource = 
"http://127.0.0.1:8000/ontology/SUMO.owl#PropositionalAttitude"/>
<rdfs:domain 
rdf:resource="http://127.0.0.1:8000/ontology/SUMO.owl#CognitiveAgent"/>
<rdfs:range rdf:resource = "http://127.0.0.1:8000/ontology/SUMO.owl#Formula"/>
<rdfs:subPropertyOf 
rdf:resource="http://127.0.0.1:8000/ontology/SUMO.owl#inScopeOfInterest"/>
<sumo:disjointRelation rdf:resource = 
"http://127.0.0.1:8000/ontology/SUMO.owl#desires" />
</owl:ObjectProperty>

<owl:ObjectProperty   rdf:ID= "dislikes">
<rdfs:comment>(dislikes ?AGENT ?OBJECT) means that ?AGENT has a
feeling of antipathy to ?OBJECT, i.e. ?AGENT believes that ?OBJECT will
thwart one of his/her goals.  Note that there is no implication that what
is hated by an agent is not already possessed by the agent.</rdfs:comment>
<rdf:type rdf:resource = 
"http://127.0.0.1:8000/ontology/SUMO.owl#ObjectAttitude"/>
<rdfs:domain 
rdf:resource="http://127.0.0.1:8000/ontology/SUMO.owl#CognitiveAgent"/>
<rdfs:range rdf:resource = "http://127.0.0.1:8000/ontology/SUMO.owl#Object"/>
<rdfs:subPropertyOf 
rdf:resource="http://127.0.0.1:8000/ontology/SUMO.owl#inScopeOfInterest"/>
<sumo:disjointRelation rdf:resource = 
"http://127.0.0.1:8000/ontology/SUMO.owl#wants" />
<sumo:relatedInternalConcept rdf:resource = "#disapproves" />
</owl:ObjectProperty>

<owl:ObjectProperty   rdf:ID= "doubts">
<rdfs:comment>(doubts ?AGENT ?FORMULA) means that ?AGENT is unsure
about the truth of ?FORMULA, in particular ?AGENT does not believe that
?FORMULA is true.</rdfs:comment>
<rdf:type rdf:resource = 
"http://127.0.0.1:8000/ontology/SUMO.owl#PropositionalAttitude"/>
<rdfs:domain 
rdf:resource="http://127.0.0.1:8000/ontology/SUMO.owl#CognitiveAgent"/>
<rdfs:range rdf:resource = "http://127.0.0.1:8000/ontology/SUMO.owl#Formula"/>
</owl:ObjectProperty>

<owl:ObjectProperty   rdf:ID= "economyType">
<rdfs:comment>(economyType ?POLITY ?TYPE) means that the
GeopoliticalArea ?POLITY has an economic system of TYPE.</rdfs:comment>
<rdf:type rdf:resource = 
"http://127.0.0.1:8000/ontology/SUMO.owl#BinaryPredicate"/>
<rdfs:domain rdf:resource="http://127.0.0.1:8000/ontology/SUMO.owl#Agent"/>
<rdfs:range rdf:resource = "#EconomicAttribute"/>
<rdfs:subPropertyOf 
rdf:resource="http://127.0.0.1:8000/ontology/SUMO.owl#attribute"/>
</owl:ObjectProperty>

<owl:ObjectProperty   rdf:ID= "electionForPosition">
<rdfs:comment>(electionForPosition ?ELECTION
?POSITION) means that in the Election ?ELECTION, candidates run for
election to the role(s) ?POSITION.</rdfs:comment>
<rdf:type rdf:resource = 
"http://127.0.0.1:8000/ontology/SUMO.owl#BinaryPredicate"/>
<rdfs:domain rdf:resource="http://127.0.0.1:8000/ontology/SUMO.owl#Election"/>
<rdfs:range rdf:resource = "http://127.0.0.1:8000/ontology/SUMO.owl#SocialRole"/>
</owl:ObjectProperty>

<owl:DatatypeProperty  rdf:ID= "electronNumber">
<rdfs:comment>(electronNumber ?SUBSTANCE ?NUMBER) means that
the PureSubstance ?SUBSTANCE has the number of Electrons 
?NUMBER.</rdfs:comment>
<rdf:type rdf:resource = 
"http://127.0.0.1:8000/ontology/SUMO.owl#BinaryPredicate"/>
<rdf:type rdf:resource = 
"http://127.0.0.1:8000/ontology/SUMO.owl#SingleValuedRelation"/>
<rdf:type rdf:resource = 
"http://127.0.0.1:8000/ontology/SUMO.owl#TotalValuedRelation"/>
<rdfs:domain 
rdf:resource="http://127.0.0.1:8000/ontology/SUMO.owl#PureSubstance"/>
<rdfs:range rdf:resource = 
"http://127.0.0.1:8000/ontology/SUMO.owl#PositiveInteger"/>
</owl:DatatypeProperty>

<owl:ObjectProperty   rdf:ID= "enjoys">
<rdfs:comment>(enjoys ?AGENT ?PROCESS) means that the
CognitiveAgent ?AGENT tends to enjoy actions of type ?PROCESS,
i.e. tends to enjoy being the agent or experiencer of such
actions.</rdfs:comment>
<rdfs:domain 
rdf:resource="http://127.0.0.1:8000/ontology/SUMO.owl#CognitiveAgent"/>
<rdfs:range rdf:resource = 
"http://127.0.0.1:8000/ontology/SUMO.owl#IntentionalProcess"/>
<rdfs:subPropertyOf 
rdf:resource="http://127.0.0.1:8000/ontology/SUMO.owl#inScopeOfInterest"/>
</owl:ObjectProperty>

<owl:ObjectProperty   rdf:ID= "equipmentType">
<rdfs:comment>(equipmentType ?THING ?TYPE) means that
the Artifact ?THING has a component or attachment of Device ?TYPE.
See also equipmentTypeCount.</rdfs:comment>
<rdf:type rdf:resource = 
"http://127.0.0.1:8000/ontology/SUMO.owl#BinaryPredicate"/>
<rdfs:domain rdf:resource="http://127.0.0.1:8000/ontology/SUMO.owl#Artifact"/>
<rdfs:range rdf:resource = "http://127.0.0.1:8000/ontology/SUMO.owl#Device"/>
</owl:ObjectProperty>

<owl:ObjectProperty   rdf:ID= "expects">
<rdfs:comment>Any belief about the future.  (expects
?AGENT ?BELIEF) means that (believes ?AGENT ?BELIEF) and, if
?BELIEF happens, it will happen in the future, i.e. after the
expectation.</rdfs:comment>
<rdfs:subPropertyOf 
rdf:resource="http://127.0.0.1:8000/ontology/SUMO.owl#believes"/>
</owl:ObjectProperty>

<owl:ObjectProperty  rdf:about= 
"http://127.0.0.1:8000/ontology/SUMO.owl#experiencer">
<rdfs:subPropertyOf rdf:resource="#involvedInEvent"/>
</owl:ObjectProperty>

<owl:ObjectProperty   rdf:ID= "experimentalControl">
<rdfs:comment>(experimentalControl ?EXPERIMENT ?OBJ)
means that the Object ?OBJ serves as a control in the instance of
Experimenting ?EXPERIMENT, i.e. ?OBJ is the standard against which something
else in the experiment can be compared.</rdfs:comment>
<rdf:type rdf:resource = "http://127.0.0.1:8000/ontology/SUMO.owl#CaseRole"/>
<rdfs:domain 
rdf:resource="http://127.0.0.1:8000/ontology/SUMO.owl#Experimenting"/>
<rdfs:range rdf:resource = "http://127.0.0.1:8000/ontology/SUMO.owl#Object"/>
<rdfs:subPropertyOf rdf:resource="#involvedInEvent"/>
</owl:ObjectProperty>

<owl:ObjectProperty   rdf:ID= "expirationDate">
<rdfs:comment>(expirationDate ?CERTIFICATE ?DAY) means that
?DAY is the date on which ?CERTIFICATE expires.</rdfs:comment>
<rdf:type rdf:resource = 
"http://127.0.0.1:8000/ontology/SUMO.owl#BinaryPredicate"/>
<rdfs:domain rdf:resource="http://127.0.0.1:8000/ontology/SUMO.owl#Certificate"/>
<rdfs:range rdf:resource = "http://127.0.0.1:8000/ontology/SUMO.owl#Day"/>
</owl:ObjectProperty>

<owl:ObjectProperty   rdf:ID= "fears">
<rdfs:comment>(fears ?AGENT ?FORMULA) means that ?AGENT fears that
the proposition ?FORMULA will be true, i.e. he/she believes that it will
come to pass in the future and that it will be undesirable for 
?AGENT.</rdfs:comment>
<rdfs:subPropertyOf rdf:resource="#expects"/>
</owl:ObjectProperty>

<owl:ObjectProperty   rdf:ID= "financialAccount">
<rdfs:comment>A formal banking, brokerage, or business
relationship established to provide for regular services, dealings, and
other financial transactions.  (accountAt ?ACCOUNT ?ORG) means that
?ACCOUNT is a financial account opened at the FinancialCompany
?ORG.</rdfs:comment>
<rdfs:domain rdf:resource="#FinancialAccount"/>
<rdfs:range rdf:resource = "#FinancialCompany"/>
<rdfs:subPropertyOf rdf:resource="#agreementMember"/>
</owl:ObjectProperty>

<owl:ObjectProperty   rdf:ID= "financialAsset">
<rdfs:comment>A predicate that relates an Agent to any
item of economic value owned by the Agent.  Examples of financial assets
are cash, securities, accounts receivable, inventory, office equipment, a
house, a car, and other property.</rdfs:comment>
<rdfs:domain rdf:resource="http://127.0.0.1:8000/ontology/SUMO.owl#Agent"/>
<rdfs:range rdf:resource = "http://127.0.0.1:8000/ontology/SUMO.owl#Object"/>
<rdfs:subPropertyOf 
rdf:resource="http://127.0.0.1:8000/ontology/SUMO.owl#possesses"/>
</owl:ObjectProperty>

<owl:ObjectProperty   rdf:ID= "firstName">
<rdfs:comment>(firstName ?CHAR ?INDIV) means that the
SymbolicString ?CHAR contains the first (or given) name of the
Human ?INDIV.</rdfs:comment><rdfs:comment>(firstName ?CHAR ?INDIV) means 
that the
SymbolicString ?CHAR contains the first (or given) name of the
Human ?INDIV.</rdfs:comment>
<rdf:type rdf:resource = 
"http://127.0.0.1:8000/ontology/SUMO.owl#BinaryPredicate"/>
<rdf:type rdf:resource = 
"http://127.0.0.1:8000/ontology/SUMO.owl#AsymmetricRelation"/>
<rdf:type rdf:resource = 
"http://127.0.0.1:8000/ontology/SUMO.owl#BinaryPredicate"/>
<rdf:type rdf:resource = 
"http://127.0.0.1:8000/ontology/SUMO.owl#AsymmetricRelation"/>
<rdfs:domain 
rdf:resource="http://127.0.0.1:8000/ontology/SUMO.owl#SymbolicString"/>
<rdfs:range rdf:resource = "http://127.0.0.1:8000/ontology/SUMO.owl#Human"/>
<rdfs:subPropertyOf 
rdf:resource="http://127.0.0.1:8000/ontology/SUMO.owl#names"/>
<rdfs:subPropertyOf 
rdf:resource="http://127.0.0.1:8000/ontology/SUMO.owl#names"/>
</owl:ObjectProperty>

<owl:ObjectProperty   rdf:ID= "fiscalYearPeriod">
<rdfs:comment>The predicate fiscalYearPeriod
indicates the period that an Agent or Organization uses as its
12-month accounting period.  (fiscalYearPeriod ?AGENT Year) means
that ?AGENT observes its 12-month accounting period during the
regular calendar year (CY), from January to December.  For
fiscal years with other beginning and ending months (FYs), use
(fiscalYearPeriod ?AGENT (RecurrentTimeIntervalFn ?STARTMONTH ?ENDMONTH)).
For example, (fiscalYearPeriod (GovernmentFn UnitedStates)
(RecurrentTimeIntervalFn October September)).  For FYs that begin
or end mid-month, days may be specified within 
RecurrentTimeIntervalFn.</rdfs:comment>
<rdf:type rdf:resource = 
"http://127.0.0.1:8000/ontology/SUMO.owl#BinaryPredicate"/>
<rdfs:domain rdf:resource="http://127.0.0.1:8000/ontology/SUMO.owl#Agent"/>
<rdfs:range rdf:resource = 
"http://127.0.0.1:8000/ontology/SUMO.owl#TimeInterval"/>
</owl:ObjectProperty>

<owl:ObjectProperty   rdf:ID= "formerName">
<rdfs:comment>(formerName ?NAME ?THING) means that the
string ?NAME is a name formerly used for ?THING.</rdfs:comment>
<rdfs:subPropertyOf 
rdf:resource="http://127.0.0.1:8000/ontology/SUMO.owl#names"/>
</owl:ObjectProperty>

<owl:ObjectProperty   rdf:ID= "governmentType">
<rdfs:comment>(governmentType ?BODY ?FORM) means that
the GeopoliticalArea or Organization ?BODY has a government with
characteristic(s) of the type ?FORM.</rdfs:comment>
<rdf:type rdf:resource = 
"http://127.0.0.1:8000/ontology/SUMO.owl#BinaryPredicate"/>
<rdfs:domain rdf:resource="http://127.0.0.1:8000/ontology/SUMO.owl#Agent"/>
<rdfs:range rdf:resource = "#FormOfGovernment"/>
<rdfs:subPropertyOf 
rdf:resource="http://127.0.0.1:8000/ontology/SUMO.owl#attribute"/>
</owl:ObjectProperty>

<owl:ObjectProperty   rdf:ID= "grammaticalRelation">
<rdfs:comment>(grammaticalRelation ?PHRASE ?SENTENCE)
means that the Phrase ?PHRASE has a grammatical relation to the Sentence
?SENTENCE, i.e. it is a subject, object, main verb, etc. of the 
?SENTENCE.</rdfs:comment>
<rdf:type rdf:resource = 
"http://127.0.0.1:8000/ontology/SUMO.owl#BinaryPredicate"/>
<rdfs:domain rdf:resource="http://127.0.0.1:8000/ontology/SUMO.owl#Phrase"/>
<rdfs:range rdf:resource = "http://127.0.0.1:8000/ontology/SUMO.owl#Sentence"/>
</owl:ObjectProperty>

<owl:ObjectProperty   rdf:ID= "grandfather">
<rdfs:comment>(grandfather ?PERSON ?PARENT) means that
?PARENT is the grandfather of ?PERSON.</rdfs:comment>
<rdfs:domain rdf:resource="http://127.0.0.1:8000/ontology/SUMO.owl#Human"/>
<rdfs:range rdf:resource = "http://127.0.0.1:8000/ontology/SUMO.owl#Man"/>
<rdfs:subPropertyOf 
rdf:resource="http://127.0.0.1:8000/ontology/SUMO.owl#familyRelation"/>
</owl:ObjectProperty>

<owl:ObjectProperty   rdf:ID= "grandmother">
<rdfs:comment>(grandmother ?PERSON ?PARENT) means that
?PARENT is the grandmother of ?PERSON.</rdfs:comment>
<rdfs:domain rdf:resource="http://127.0.0.1:8000/ontology/SUMO.owl#Human"/>
<rdfs:range rdf:resource = "http://127.0.0.1:8000/ontology/SUMO.owl#Man"/>
<rdfs:subPropertyOf 
rdf:resource="http://127.0.0.1:8000/ontology/SUMO.owl#familyRelation"/>
</owl:ObjectProperty>

<owl:ObjectProperty   rdf:ID= "graphPart">
<rdfs:comment>A basic relation for Graphs and their
parts.  (graphPart ?PART ?GRAPH) means that ?PART is a GraphArc
or GraphNode of the Graph ?GRAPH.</rdfs:comment>
<rdf:type rdf:resource = 
"http://127.0.0.1:8000/ontology/SUMO.owl#BinaryPredicate"/>
<rdf:type rdf:resource = 
"http://127.0.0.1:8000/ontology/SUMO.owl#AsymmetricRelation"/>
<rdf:type rdf:resource = 
"http://127.0.0.1:8000/ontology/SUMO.owl#IrreflexiveRelation"/>
<rdfs:domain rdf:resource="#GraphElement"/>
<rdfs:range rdf:resource = "#Graph"/>
</owl:ObjectProperty>

<owl:ObjectProperty   rdf:ID= "groupMember">
<rdfs:comment>A subrelation of member, groupMember
is used to relate a Human to a GroupOfPeople of which he/she is a
member.</rdfs:comment>
<rdfs:domain rdf:resource="http://127.0.0.1:8000/ontology/SUMO.owl#Human"/>
<rdfs:range rdf:resource = 
"http://127.0.0.1:8000/ontology/SUMO.owl#GroupOfPeople"/>
<rdfs:subPropertyOf 
rdf:resource="http://127.0.0.1:8000/ontology/SUMO.owl#member"/>
</owl:ObjectProperty>

<owl:ObjectProperty   rdf:ID= "half">
<rdfs:comment>(half ?HALF ?WHOLE) means that ?HALF is one half
of ?WHOLE.</rdfs:comment>
<rdfs:subPropertyOf rdf:resource="http://127.0.0.1:8000/ontology/SUMO.owl#part"/>
</owl:ObjectProperty>

<owl:ObjectProperty   rdf:ID= "hasExpertise">
<rdfs:comment>(hasExpertise ?AGENT ?FIELD) means that ?AGENT has
studied the FieldOfStudy ?FIELD and is regarded as an expert.</rdfs:comment>
<rdf:type rdf:resource = 
"http://127.0.0.1:8000/ontology/SUMO.owl#BinaryPredicate"/>
<rdfs:domain 
rdf:resource="http://127.0.0.1:8000/ontology/SUMO.owl#CognitiveAgent"/>
<rdfs:range rdf:resource = 
"http://127.0.0.1:8000/ontology/SUMO.owl#FieldOfStudy"/>
</owl:ObjectProperty>

<owl:ObjectProperty   rdf:ID= "headquartersOfOrganization">
<rdfs:comment>(headquartersOfOrganization ?ORG ?AREA)
means that the Organization ?ORG is headquartered in ?AREA.</rdfs:comment>
<rdfs:domain 
rdf:resource="http://127.0.0.1:8000/ontology/SUMO.owl#Organization"/>
<rdfs:range rdf:resource = 
"http://127.0.0.1:8000/ontology/SUMO.owl#GeopoliticalArea"/>
<rdfs:subPropertyOf 
rdf:resource="http://127.0.0.1:8000/ontology/SUMO.owl#located"/>
</owl:ObjectProperty>

<owl:ObjectProperty   rdf:ID= "hopes">
<rdfs:comment>(hopes ?AGENT ?FORMULA) means that ?AGENT hopes that
the proposition ?FORMULA will be true, i.e. he/she believes that it will
come to pass in the future and that it will be desirable for 
?AGENT.</rdfs:comment>
<rdfs:subPropertyOf rdf:resource="#expects"/>
</owl:ObjectProperty>

<owl:ObjectProperty   rdf:ID= "hostileForces">
<rdfs:comment>(hostileForces ?UNIT1 ?UNIT2) means that
the MilitaryUnits ?UNIT1 and ?UNIT2 are, respectively, allied with
GeopoliticalAreas that are at war with one another.</rdfs:comment>
<rdf:type rdf:resource = 
"http://127.0.0.1:8000/ontology/SUMO.owl#BinaryPredicate"/>
<rdf:type rdf:resource = 
"http://127.0.0.1:8000/ontology/SUMO.owl#IrreflexiveRelation"/>
<rdfs:domain rdf:resource="#MilitaryUnit"/>
<rdfs:range rdf:resource = "#MilitaryUnit"/>
</owl:ObjectProperty>

<owl:DatatypeProperty  rdf:ID= "humanCapacity">
<rdfs:comment>(humanCapacity ?CONSTRUCT ?NUMBER) means that the
StationaryArtifact ?CONSTRUCT, e.g. a Building or a Room, can hold a maximum
of ?NUMBER Humans without crowding.</rdfs:comment>
<rdf:type rdf:resource = 
"http://127.0.0.1:8000/ontology/SUMO.owl#BinaryPredicate"/>
<rdf:type rdf:resource = 
"http://127.0.0.1:8000/ontology/SUMO.owl#SingleValuedRelation"/>
<rdfs:domain 
rdf:resource="http://127.0.0.1:8000/ontology/SUMO.owl#StationaryArtifact"/>
<rdfs:range rdf:resource = 
"http://127.0.0.1:8000/ontology/SUMO.owl#PositiveInteger"/>
</owl:DatatypeProperty>

<owl:ObjectProperty   rdf:ID= "ideologicalAffiliationOfOrganization">
<rdfs:comment>(ideologicalAffiliationOfOrganization
?ORG ?GOV) means that one of the goals of ?ORG is to realize the 
FormOfGovernment ?GOV.</rdfs:comment>
<rdf:type rdf:resource = 
"http://127.0.0.1:8000/ontology/SUMO.owl#BinaryPredicate"/>
<rdfs:domain 
rdf:resource="http://127.0.0.1:8000/ontology/SUMO.owl#Organization"/>
<rdfs:range rdf:resource = "#FormOfGovernment"/>
</owl:ObjectProperty>

<owl:ObjectProperty   rdf:ID= "industryOfArea">
<rdfs:comment>(industryOfArea ?AREA ?SECTOR)
means that the GeopoliticalArea ?AREA produces goods or services
in the economic area ?SECTOR.</rdfs:comment>
<rdf:type rdf:resource = 
"http://127.0.0.1:8000/ontology/SUMO.owl#BinaryPredicate"/>
<rdfs:domain 
rdf:resource="http://127.0.0.1:8000/ontology/SUMO.owl#GeopoliticalArea"/>
<rdfs:range rdf:resource = "http://127.0.0.1:8000/ontology/SUMO.owl#Physical"/>
</owl:ObjectProperty>

<owl:ObjectProperty   rdf:ID= "industryProductType">
<rdfs:comment>(industryProductType ?INDUSTRY ?TYPE) means that the Industry 
?INDUSTRY
produces products of the kind ?TYPE.</rdfs:comment>
<rdf:type rdf:resource = 
"http://127.0.0.1:8000/ontology/SUMO.owl#BinaryPredicate"/>
<rdfs:domain rdf:resource="#Industry"/>
<rdfs:range rdf:resource = "http://127.0.0.1:8000/ontology/SUMO.owl#Product"/>
</owl:ObjectProperty>

<owl:ObjectProperty  rdf:about= 
"http://127.0.0.1:8000/ontology/SUMO.owl#instrument">
<rdfs:subPropertyOf rdf:resource="#involvedInEvent"/>
</owl:ObjectProperty>

<owl:ObjectProperty   rdf:ID= "insured">
<rdfs:comment>(insured ?Contract ?Org) means that ?Contract is insured
by the ?Organization.</rdfs:comment>
<rdf:type rdf:resource = 
"http://127.0.0.1:8000/ontology/SUMO.owl#BinaryPredicate"/>
<rdfs:domain rdf:resource="http://127.0.0.1:8000/ontology/SUMO.owl#Contract"/>
<rdfs:range rdf:resource = 
"http://127.0.0.1:8000/ontology/SUMO.owl#Organization"/>
</owl:ObjectProperty>

<owl:DatatypeProperty  rdf:ID= "intelligenceQuotient">
<rdfs:comment>(intelligenceQuotient ?PERSON ?NUMBER)
means that ?NUMBER is the I.Q. of ?PERSON.  The I.Q. of a person is the 
ratio
of their mental age (determined by a standardized test) divided by their
chronological age, multiplied by 100.</rdfs:comment>
<rdf:type rdf:resource = 
"http://127.0.0.1:8000/ontology/SUMO.owl#BinaryPredicate"/>
<rdf:type rdf:resource = 
"http://127.0.0.1:8000/ontology/SUMO.owl#SingleValuedRelation"/>
<rdfs:domain rdf:resource="http://127.0.0.1:8000/ontology/SUMO.owl#Human"/>
<rdfs:range rdf:resource = 
"http://127.0.0.1:8000/ontology/SUMO.owl#RationalNumber"/>
</owl:DatatypeProperty>

<owl:ObjectProperty   rdf:ID= "inventory">
<rdfs:comment>(inventory ?CBO ?COLLECTION) means that
the ContentBearingObject ?CBO contains a list or enumeration of the
members of the Collection ?COLLECTION.</rdfs:comment>
<rdf:type rdf:resource = 
"http://127.0.0.1:8000/ontology/SUMO.owl#BinaryPredicate"/>
<rdfs:domain 
rdf:resource="http://127.0.0.1:8000/ontology/SUMO.owl#ContentBearingObject"/>
<rdfs:range rdf:resource = "http://127.0.0.1:8000/ontology/SUMO.owl#Collection"/>
</owl:ObjectProperty>

<owl:ObjectProperty   rdf:ID= "involvedInEvent">
<rdfs:comment>(involvedInEvent ?EVENT ?THING) means
that in the Process ?EVENT, the Entity ?THING plays some 
CaseRole.</rdfs:comment>
<rdf:type rdf:resource = 
"http://127.0.0.1:8000/ontology/SUMO.owl#BinaryPredicate"/>
<rdf:type rdf:resource = 
"http://127.0.0.1:8000/ontology/SUMO.owl#AsymmetricRelation"/>
<rdfs:domain rdf:resource="http://127.0.0.1:8000/ontology/SUMO.owl#Process"/>
<rdfs:range rdf:resource = "http://127.0.0.1:8000/ontology/SUMO.owl#Entity"/>
</owl:ObjectProperty>

<owl:ObjectProperty   rdf:ID= "issuedBy">
<rdfs:comment>(issuedBy ?Certificate ?Agent) means that the
Certificate ?Certificate is produced and offered by ?Agent.</rdfs:comment>
<rdf:type rdf:resource = 
"http://127.0.0.1:8000/ontology/SUMO.owl#BinaryPredicate"/>
<rdfs:domain rdf:resource="http://127.0.0.1:8000/ontology/SUMO.owl#Certificate"/>
<rdfs:range rdf:resource = 
"http://127.0.0.1:8000/ontology/SUMO.owl#CognitiveAgent"/>
</owl:ObjectProperty>

<owl:ObjectProperty   rdf:ID= "lacks">
<rdfs:comment>(lacks ?AGENT ?OBJECT) means that ?AGENT needs
?OBJECT and it is not the case that ?AGENT possesses ?OBJECT.</rdfs:comment>
<rdfs:subPropertyOf 
rdf:resource="http://127.0.0.1:8000/ontology/SUMO.owl#needs"/>
</owl:ObjectProperty>

<owl:ObjectProperty   rdf:ID= "landlord">
<rdfs:comment>(landlord ?PERSON ?UNIT) means that ?PERSON is a
landlord of the Residence ?UNIT, i.e. he or she owns ?UNIT and is renting
the unit to someone else.</rdfs:comment>
<rdf:type rdf:resource = 
"http://127.0.0.1:8000/ontology/SUMO.owl#BinaryPredicate"/>
<rdfs:domain rdf:resource="http://127.0.0.1:8000/ontology/SUMO.owl#Human"/>
<sumo:domain rdf:resource = 
"http://127.0.0.1:8000/ontology/SUMO.owl#PermanentResidence" />
</owl:ObjectProperty>

<owl:ObjectProperty   rdf:ID= "lastName">
<rdfs:comment>(lastName ?CHAR ?INDIV) means that the
SymbolicString ?CHAR contains the last (surname or family) name of the
Human ?INDIV.</rdfs:comment><rdfs:comment>(lastName ?CHAR ?INDIV) means that 
the
SymbolicString ?CHAR contains the last (surname or family) name of the
Human ?INDIV.</rdfs:comment>
<rdf:type rdf:resource = 
"http://127.0.0.1:8000/ontology/SUMO.owl#BinaryPredicate"/>
<rdf:type rdf:resource = 
"http://127.0.0.1:8000/ontology/SUMO.owl#AsymmetricRelation"/>
<rdf:type rdf:resource = 
"http://127.0.0.1:8000/ontology/SUMO.owl#BinaryPredicate"/>
<rdf:type rdf:resource = 
"http://127.0.0.1:8000/ontology/SUMO.owl#AsymmetricRelation"/>
<rdfs:domain 
rdf:resource="http://127.0.0.1:8000/ontology/SUMO.owl#SymbolicString"/>
<rdfs:range rdf:resource = "http://127.0.0.1:8000/ontology/SUMO.owl#Human"/>
<rdfs:subPropertyOf 
rdf:resource="http://127.0.0.1:8000/ontology/SUMO.owl#names"/>
<rdfs:subPropertyOf 
rdf:resource="http://127.0.0.1:8000/ontology/SUMO.owl#names"/>
</owl:ObjectProperty>

<owl:ObjectProperty   rdf:ID= "leaderPosition">
<rdfs:comment>(leaderPosition ?ORG ?ROLE)
means that in the organization ?ORG, the leader is the person
who holds the Position ?ROLE in the organization.</rdfs:comment>
<rdf:type rdf:resource = 
"http://127.0.0.1:8000/ontology/SUMO.owl#BinaryPredicate"/>
<rdf:type rdf:resource = 
"http://127.0.0.1:8000/ontology/SUMO.owl#AsymmetricRelation"/>
<rdfs:domain rdf:resource="http://127.0.0.1:8000/ontology/SUMO.owl#Agent"/>
<rdfs:range rdf:resource = "http://127.0.0.1:8000/ontology/SUMO.owl#Position"/>
</owl:ObjectProperty>

<owl:ObjectProperty   rdf:ID= "legalSystemType">
<rdfs:comment>(legalSystemType ?AREA ?TYPE) means
that the GeopoliticalArea ?AREA has a legal system characterized by
the LegalSystemAttribute ?TYPE.  For example, (legalSystemType
UnitedStates EnglishCommonLaw).  A legal system may have multiple
characteristics.</rdfs:comment>
<rdf:type rdf:resource = 
"http://127.0.0.1:8000/ontology/SUMO.owl#BinaryPredicate"/>
<rdfs:domain 
rdf:resource="http://127.0.0.1:8000/ontology/SUMO.owl#GeopoliticalArea"/>
<rdfs:range rdf:resource = "#LegalSystemAttribute"/>
</owl:ObjectProperty>

<owl:ObjectProperty   rdf:ID= "lender">
<rdfs:comment>(lender ?Loan ?Agent) means that ?Agent is a private, public 
or
institutional entity that put up the funds for the ?Loan.</rdfs:comment>
<rdfs:domain rdf:resource="#Loan"/>
<rdfs:range rdf:resource = 
"http://127.0.0.1:8000/ontology/SUMO.owl#CognitiveAgent"/>
<rdfs:subPropertyOf rdf:resource="#agreementMember"/>
</owl:ObjectProperty>

<owl:ObjectProperty   rdf:ID= "loanForPurchase">
<rdfs:comment>(loanForPurchase ?ACCOUNT ?PRODUCT) means that ?ACCOUNT is a
loan to finance the purchase of ?PRODUCT.</rdfs:comment>
<rdf:type rdf:resource = 
"http://127.0.0.1:8000/ontology/SUMO.owl#BinaryPredicate"/>
<rdfs:domain rdf:resource="#Loan"/>
<rdfs:range rdf:resource = "http://127.0.0.1:8000/ontology/SUMO.owl#Object"/>
</owl:ObjectProperty>

<owl:ObjectProperty   rdf:ID= "localLongName">
<rdfs:comment>(localLongName ?NAME ?THING) means that
the string ?NAME is the long form of the name used for ?THING in its local
area or language.</rdfs:comment>
<rdfs:subPropertyOf 
rdf:resource="http://127.0.0.1:8000/ontology/SUMO.owl#names"/>
</owl:ObjectProperty>

<owl:ObjectProperty   rdf:ID= "localShortName">
<rdfs:comment>(localShortName ?NAME ?THING) means that
the string ?NAME is the short form of the name used for ?THING in its
local area or language.</rdfs:comment>
<rdfs:subPropertyOf 
rdf:resource="http://127.0.0.1:8000/ontology/SUMO.owl#names"/>
</owl:ObjectProperty>

<owl:ObjectProperty   rdf:ID= "loss">
<rdfs:comment>The amount by which the cost of an investment or
business operation exceeds its return, i.e. the negative quantity left
after subtracting for all expenses.</rdfs:comment>
<rdf:type rdf:resource = 
"http://127.0.0.1:8000/ontology/SUMO.owl#AsymmetricRelation"/>
<rdfs:domain 
rdf:resource="http://127.0.0.1:8000/ontology/SUMO.owl#FinancialTransaction"/>
<rdfs:range rdf:resource = 
"http://127.0.0.1:8000/ontology/SUMO.owl#CurrencyMeasure"/>
</owl:ObjectProperty>

<owl:ObjectProperty   rdf:ID= "maturityDate">
<rdfs:comment>The date on which the principal amount of the account
becomes due and payable.</rdfs:comment>
<rdf:type rdf:resource = 
"http://127.0.0.1:8000/ontology/SUMO.owl#BinaryPredicate"/>
<rdfs:domain rdf:resource="#FinancialAccount"/>
<rdfs:range rdf:resource = "http://127.0.0.1:8000/ontology/SUMO.owl#Day"/>
</owl:ObjectProperty>

<owl:ObjectProperty   rdf:ID= "measurementReading">
<rdfs:comment>(measurementReading ?DEVICE ?QUANTITY)
means that ?QUANTITY is a reading of the MeasuringDevice ?DEVICE, e.g. if
?THERMOMETER is a Thermometer, (measurementReading ?THERMOMETER
(MeasureFn 42 CelsiusDegree)) would mean that ?THERMOMETER registers 42
degrees Celsius.</rdfs:comment>
<rdf:type rdf:resource = 
"http://127.0.0.1:8000/ontology/SUMO.owl#BinaryPredicate"/>
<rdfs:domain 
rdf:resource="http://127.0.0.1:8000/ontology/SUMO.owl#MeasuringDevice"/>
<rdfs:range rdf:resource = 
"http://127.0.0.1:8000/ontology/SUMO.owl#ConstantQuantity"/>
</owl:ObjectProperty>

<owl:ObjectProperty   rdf:ID= "memberType">
<rdfs:comment>(memberType ?GROUP ?TYPE) means that all
the members of the Collection ?GROUP belong to the SetOrClass
?TYPE.</rdfs:comment>
<rdf:type rdf:resource = 
"http://127.0.0.1:8000/ontology/SUMO.owl#BinaryPredicate"/>
<rdfs:domain rdf:resource="http://127.0.0.1:8000/ontology/SUMO.owl#Collection"/>
<rdfs:range rdf:resource = "http://127.0.0.1:8000/ontology/SUMO.owl#SetOrClass"/>
</owl:ObjectProperty>

<owl:ObjectProperty   rdf:ID= "middleName">
<rdfs:comment>(middleName ?CHAR ?INDIV) means that the
SymbolicString ?CHAR contains the middle name of the Human 
?INDIV.</rdfs:comment><rdfs:comment>(middleName ?CHAR ?INDIV) means that the
SymbolicString ?CHAR contains the middle name of the Human 
?INDIV.</rdfs:comment>
<rdf:type rdf:resource = 
"http://127.0.0.1:8000/ontology/SUMO.owl#BinaryPredicate"/>
<rdf:type rdf:resource = 
"http://127.0.0.1:8000/ontology/SUMO.owl#AsymmetricRelation"/>
<rdf:type rdf:resource = 
"http://127.0.0.1:8000/ontology/SUMO.owl#BinaryPredicate"/>
<rdf:type rdf:resource = 
"http://127.0.0.1:8000/ontology/SUMO.owl#AsymmetricRelation"/>
<rdfs:domain 
rdf:resource="http://127.0.0.1:8000/ontology/SUMO.owl#SymbolicString"/>
<rdfs:range rdf:resource = "http://127.0.0.1:8000/ontology/SUMO.owl#Human"/>
<rdfs:subPropertyOf 
rdf:resource="http://127.0.0.1:8000/ontology/SUMO.owl#names"/>
<rdfs:subPropertyOf 
rdf:resource="http://127.0.0.1:8000/ontology/SUMO.owl#names"/>
</owl:ObjectProperty>

<owl:ObjectProperty   rdf:ID= "most">
<rdfs:comment>(most ?MOST ?WHOLE) means that ?MOST is a part
of ?WHOLE that is greater than half of ?WHOLE.</rdfs:comment>
<rdfs:subPropertyOf rdf:resource="http://127.0.0.1:8000/ontology/SUMO.owl#part"/>
</owl:ObjectProperty>

<owl:DatatypeProperty  rdf:ID= "multiplicativeFactor">
<rdfs:comment>(multiplicativeFactor ?NUMBER1 ?NUMBER2)
means that ?NUMBER1 is a factor of ?NUMBER2, i.e. ?NUMBER1 can be multiplied 
by
some Integer to give ?NUMBER2 as a result.</rdfs:comment>
<rdf:type rdf:resource = 
"http://127.0.0.1:8000/ontology/SUMO.owl#BinaryPredicate"/>
<rdf:type rdf:resource = 
"http://127.0.0.1:8000/ontology/SUMO.owl#TransitiveRelation"/>
<rdfs:domain rdf:resource="http://127.0.0.1:8000/ontology/SUMO.owl#Integer"/>
<rdfs:range rdf:resource = "http://127.0.0.1:8000/ontology/SUMO.owl#Integer"/>
</owl:DatatypeProperty>

<owl:ObjectProperty   rdf:ID= "neighbor">
<rdfs:comment>(neighbor ?PERSON1 ?PERSON2) means that ?PERSON1 is
a neighbor of ?PERSON2, i.e. ?PERSON1 and ?PERSON2 have their homes Near
one another.</rdfs:comment>
<rdf:type rdf:resource = 
"http://127.0.0.1:8000/ontology/SUMO.owl#BinaryPredicate"/>
<rdf:type rdf:resource = 
"http://127.0.0.1:8000/ontology/SUMO.owl#SymmetricRelation"/>
<rdf:type rdf:resource = 
"http://127.0.0.1:8000/ontology/SUMO.owl#IrreflexiveRelation"/>
<rdfs:domain rdf:resource="http://127.0.0.1:8000/ontology/SUMO.owl#Human"/>
<rdfs:range rdf:resource = "http://127.0.0.1:8000/ontology/SUMO.owl#Human"/>
</owl:ObjectProperty>

<owl:ObjectProperty   rdf:ID= "nephew">
<rdfs:comment>(nephew ?NEPHEW ?PERSON) means that ?NEPHEW is
the son of a sibling of ?PERSON.</rdfs:comment>
<rdfs:domain rdf:resource="http://127.0.0.1:8000/ontology/SUMO.owl#Man"/>
<rdfs:range rdf:resource = "http://127.0.0.1:8000/ontology/SUMO.owl#Human"/>
<rdfs:subPropertyOf 
rdf:resource="http://127.0.0.1:8000/ontology/SUMO.owl#familyRelation"/>
</owl:ObjectProperty>

<owl:ObjectProperty   rdf:ID= "niece">
<rdfs:comment>(niece ?NIECE ?PERSON) means that ?NIECE is
the daughter of a sibling of ?PERSON.</rdfs:comment>
<rdfs:domain rdf:resource="http://127.0.0.1:8000/ontology/SUMO.owl#Woman"/>
<rdfs:range rdf:resource = "http://127.0.0.1:8000/ontology/SUMO.owl#Human"/>
<rdfs:subPropertyOf 
rdf:resource="http://127.0.0.1:8000/ontology/SUMO.owl#familyRelation"/>
</owl:ObjectProperty>

<owl:ObjectProperty   rdf:ID= "occupation">
<rdfs:comment>(occupation ?PERSON ?TYPE) means that the occupation
of ?PERSON is ?TYPE.  This predicate is most often used in combination with 
the
function OccupationFn, e.g. (occupation PoliceOfficerWilkins (OccupationFn
LawEnforcement)).</rdfs:comment>
<rdf:type rdf:resource = 
"http://127.0.0.1:8000/ontology/SUMO.owl#BinaryPredicate"/>
<rdfs:domain rdf:resource="http://127.0.0.1:8000/ontology/SUMO.owl#Human"/>
<rdfs:range rdf:resource = 
"http://127.0.0.1:8000/ontology/SUMO.owl#FinancialTransaction"/>
</owl:ObjectProperty>

<owl:ObjectProperty   rdf:ID= "older">
<rdfs:comment>(older ?OBJ1 ?OBJ2) means that ?OBJ1 is older than
?OBJ2, i.e. the age of ?OBJ1 is greaterThan the age of ?OBJ2.</rdfs:comment>
<rdf:type rdf:resource = 
"http://127.0.0.1:8000/ontology/SUMO.owl#BinaryPredicate"/>
<rdfs:domain rdf:resource="http://127.0.0.1:8000/ontology/SUMO.owl#Object"/>
<rdfs:range rdf:resource = "http://127.0.0.1:8000/ontology/SUMO.owl#Object"/>
</owl:ObjectProperty>

<owl:ObjectProperty   rdf:ID= "onboard">
<rdfs:comment>(onboard ?OBJ ?VEHICLE) means that the
SelfConnectedObject ?OBJ is inside the Vehicle ?VEHICLE.</rdfs:comment>
<rdfs:domain 
rdf:resource="http://127.0.0.1:8000/ontology/SUMO.owl#SelfConnectedObject"/>
<rdfs:range rdf:resource = "http://127.0.0.1:8000/ontology/SUMO.owl#Vehicle"/>
<rdfs:subPropertyOf 
rdf:resource="http://127.0.0.1:8000/ontology/SUMO.owl#located"/>
</owl:ObjectProperty>

<owl:ObjectProperty   rdf:ID= "orbits">
<rdfs:comment>(orbits ?SATELLITE ?FOCUS) means that the Object
?SATELLITE revolves around the AstronomicalBody ?FOCUS.</rdfs:comment>
<rdf:type rdf:resource = 
"http://127.0.0.1:8000/ontology/SUMO.owl#BinaryPredicate"/>
<rdf:type rdf:resource = 
"http://127.0.0.1:8000/ontology/SUMO.owl#AsymmetricRelation"/>
<rdfs:domain rdf:resource="http://127.0.0.1:8000/ontology/SUMO.owl#Object"/>
<rdfs:range rdf:resource = 
"http://127.0.0.1:8000/ontology/SUMO.owl#AstronomicalBody"/>
</owl:ObjectProperty>

<owl:ObjectProperty  rdf:about= "http://127.0.0.1:8000/ontology/SUMO.owl#origin">
<rdfs:subPropertyOf rdf:resource="#involvedInEvent"/>
</owl:ObjectProperty>

<owl:ObjectProperty   rdf:ID= "parasite">
<rdfs:comment>(parasite ?ORGANISM1 ?ORGANISM2) means that there
is a parasitic relationship between ?ORGANISM1 and ?ORGANISM2, i.e. 
?ORGANISM1
inhabits and obtains nourishment from ?ORGANISM2 in such a way that
?ORGANISM2 is injured.</rdfs:comment>
<rdf:type rdf:resource = 
"http://127.0.0.1:8000/ontology/SUMO.owl#BinaryPredicate"/>
<rdfs:domain rdf:resource="http://127.0.0.1:8000/ontology/SUMO.owl#Organism"/>
<rdfs:range rdf:resource = "http://127.0.0.1:8000/ontology/SUMO.owl#Organism"/>
</owl:ObjectProperty>

<owl:ObjectProperty  rdf:about= "http://127.0.0.1:8000/ontology/SUMO.owl#path">
<rdfs:subPropertyOf rdf:resource="#involvedInEvent"/>
</owl:ObjectProperty>

<owl:ObjectProperty   rdf:ID= "pathInSystem">
<rdfs:comment>(pathInSystem ?PATH ?SYSTEM) means that
the Physical thing ?PATH consists of one or more connected routes in
the PhysicalSystem ?SYSTEM.</rdfs:comment>
<rdf:type rdf:resource = 
"http://127.0.0.1:8000/ontology/SUMO.owl#BinaryPredicate"/>
<rdfs:domain rdf:resource="http://127.0.0.1:8000/ontology/SUMO.owl#Transitway"/>
<rdfs:range rdf:resource = "#TransportationSystem"/>
<rdfs:subPropertyOf rdf:resource="http://127.0.0.1:8000/ontology/SUMO.owl#part"/>
</owl:ObjectProperty>

<owl:DatatypeProperty  rdf:ID= "pathLength">
<rdfs:comment>A BinaryPredicate that specifies the
length (in number of GraphNodes) of a GraphPath.
(pathLength ?PATH ?NUMBER) means that there are ?NUMBER nodes in
the GraphPath ?PATH.</rdfs:comment>
<rdf:type rdf:resource = 
"http://127.0.0.1:8000/ontology/SUMO.owl#BinaryPredicate"/>
<rdf:type rdf:resource = 
"http://127.0.0.1:8000/ontology/SUMO.owl#AsymmetricRelation"/>
<rdf:type rdf:resource = 
"http://127.0.0.1:8000/ontology/SUMO.owl#IrreflexiveRelation"/>
<rdfs:domain rdf:resource="#GraphPath"/>
<rdfs:range rdf:resource = 
"http://127.0.0.1:8000/ontology/SUMO.owl#PositiveInteger"/>
</owl:DatatypeProperty>

<owl:ObjectProperty  rdf:about= 
"http://127.0.0.1:8000/ontology/SUMO.owl#patient">
<rdfs:subPropertyOf rdf:resource="#involvedInEvent"/>
</owl:ObjectProperty>

<owl:ObjectProperty   rdf:ID= "patientMedical">
<rdfs:comment>The relation of receiving medical care
from a recognized medical practitioner.  (patientMedical ?PATIENT
?DOCTOR) means that ?PATIENT is the patient of ?DOCTOR.  Note that
argument type restriction on the second argument is CognitiveAgent
to allow for cases where someone is the patient of an Organization,
viz. a CareOrganization.</rdfs:comment>
<rdf:type rdf:resource = 
"http://127.0.0.1:8000/ontology/SUMO.owl#BinaryPredicate"/>
<rdfs:domain rdf:resource="http://127.0.0.1:8000/ontology/SUMO.owl#Human"/>
<rdfs:range rdf:resource = 
"http://127.0.0.1:8000/ontology/SUMO.owl#CognitiveAgent"/>
</owl:ObjectProperty>

<owl:ObjectProperty   rdf:ID= "placeOfDeath">
<rdfs:comment>(placeOfDeath ?INDIV ?PLACE) means that the Animal ?INDIV died
at the location ?PLACE.  The location may be a geographic area or a 
building, such as a hospital.</rdfs:comment>
<rdf:type rdf:resource = 
"http://127.0.0.1:8000/ontology/SUMO.owl#BinaryPredicate"/>
<rdfs:domain rdf:resource="http://127.0.0.1:8000/ontology/SUMO.owl#Animal"/>
<rdfs:range rdf:resource = "http://127.0.0.1:8000/ontology/SUMO.owl#Object"/>
</owl:ObjectProperty>

<owl:ObjectProperty   rdf:ID= "plaintiff">
<rdfs:comment>(plaintiff ?AGENT ?ACTION) means that ?AGENT
is responsible for initiating the LegalAction ?ACTION.</rdfs:comment>
<rdfs:domain 
rdf:resource="http://127.0.0.1:8000/ontology/SUMO.owl#CognitiveAgent"/>
<rdfs:range rdf:resource = 
"http://127.0.0.1:8000/ontology/SUMO.owl#LegalAction"/>
<rdfs:subPropertyOf 
rdf:resource="http://127.0.0.1:8000/ontology/SUMO.owl#agent"/>
<rdfs:subPropertyOf rdf:resource="#involvedInEvent"/>
</owl:ObjectProperty>

<owl:ObjectProperty   rdf:ID= "postalBoxNumber">
<rdfs:comment>(postalBoxNumber ?NUMBER ?ADDRESS) means
that the post office box ?NUMBER is part of the address 
?ADDRESS.</rdfs:comment>
<rdfs:domain 
rdf:resource="http://127.0.0.1:8000/ontology/SUMO.owl#PositiveInteger"/>
<rdfs:range rdf:resource = "#Address"/>
<rdfs:subPropertyOf 
rdf:resource="http://127.0.0.1:8000/ontology/SUMO.owl#uniqueIdentifier"/>
</owl:ObjectProperty>

<owl:ObjectProperty   rdf:ID= "postalCode">
<rdfs:comment>(postalCode ?NUMBER ?ADDRESS) means that the
the postal code, e.g. zip code, ?NUMBER is part of the address 
?ADDRESS.</rdfs:comment>
<rdfs:domain 
rdf:resource="http://127.0.0.1:8000/ontology/SUMO.owl#PositiveInteger"/>
<rdfs:range rdf:resource = "#Address"/>
<rdfs:subPropertyOf 
rdf:resource="http://127.0.0.1:8000/ontology/SUMO.owl#uniqueIdentifier"/>
</owl:ObjectProperty>

<owl:DatatypeProperty  rdf:ID= "potentialOfHydrogen">
<rdfs:comment>(potentialOfHydrogen ?SOLUTION ?NUMBER)
means that the Solution ?SOLUTION has a pH value of ?NUMBER.  The ph varies
between 0 and 14, and it is a measure of the acidity or alkalinity of 
?SOLUTION.
More precisely,  and it is the logarithm of the reciprocal of the quantity 
of
AtomGrams of Hydrogen ions.</rdfs:comment>
<rdf:type rdf:resource = 
"http://127.0.0.1:8000/ontology/SUMO.owl#BinaryPredicate"/>
<rdfs:domain rdf:resource="http://127.0.0.1:8000/ontology/SUMO.owl#Solution"/>
<rdfs:range rdf:resource = "http://127.0.0.1:8000/ontology/SUMO.owl#RealNumber"/>
</owl:DatatypeProperty>

<owl:ObjectProperty   rdf:ID= "powerPlant">
<rdfs:comment>(powerPlant ?GENERATOR ?THING) means that
the Device ?GENERATOR is the power-producing component of the Artifact
?THING which provides the energy for its operation.</rdfs:comment>
<rdf:type rdf:resource = 
"http://127.0.0.1:8000/ontology/SUMO.owl#BinaryPredicate"/>
<rdf:type rdf:resource = 
"http://127.0.0.1:8000/ontology/SUMO.owl#AsymmetricRelation"/>
<rdf:type rdf:resource = 
"http://127.0.0.1:8000/ontology/SUMO.owl#IrreflexiveRelation"/>
<rdfs:domain rdf:resource="http://127.0.0.1:8000/ontology/SUMO.owl#Device"/>
<rdfs:range rdf:resource = "http://127.0.0.1:8000/ontology/SUMO.owl#Artifact"/>
<rdfs:subPropertyOf 
rdf:resource="http://127.0.0.1:8000/ontology/SUMO.owl#component"/>
</owl:ObjectProperty>

<owl:ObjectProperty   rdf:ID= "primaryGeopoliticalSubdivision">
<rdfs:comment>(primaryGeopoliticalSubdivision ?AREA ?COUNTRY) means that the
GeopoliticalArea ?AREA is one of the first-order administrative
divisions of the Nation ?COUNTRY.  For example, in the United States,
any of the fifty states.  This does not include subordinate regions that
have a lesser status, such as British Crown colonies, U.S. territories,
or protectorates.  See geopoliticalSubdivision.</rdfs:comment>
<rdf:type rdf:resource = 
"http://127.0.0.1:8000/ontology/SUMO.owl#BinaryPredicate"/>
<rdf:type rdf:resource = 
"http://127.0.0.1:8000/ontology/SUMO.owl#AsymmetricRelation"/>
<rdfs:domain 
rdf:resource="http://127.0.0.1:8000/ontology/SUMO.owl#GeopoliticalArea"/>
<rdfs:range rdf:resource = 
"http://127.0.0.1:8000/ontology/SUMO.owl#GeopoliticalArea"/>
<rdfs:subPropertyOf 
rdf:resource="http://127.0.0.1:8000/ontology/SUMO.owl#geopoliticalSubdivision"/>
</owl:ObjectProperty>

<owl:ObjectProperty   rdf:ID= "principalAmount">
<rdfs:comment>(principalAmount ?ACCOUNT ?BALANCE) means
that ?BALANCE is the amount originally borrowed (excluding 
interest).</rdfs:comment>
<rdf:type rdf:resource = 
"http://127.0.0.1:8000/ontology/SUMO.owl#BinaryPredicate"/>
<rdfs:domain rdf:resource="#FinancialAccount"/>
<rdfs:range rdf:resource = 
"http://127.0.0.1:8000/ontology/SUMO.owl#CurrencyMeasure"/>
</owl:ObjectProperty>

<owl:ObjectProperty   rdf:ID= "profit">
<rdfs:comment>The positive gain from an investment or business
operation after subtracting for all expenses.</rdfs:comment>
<rdf:type rdf:resource = 
"http://127.0.0.1:8000/ontology/SUMO.owl#AsymmetricRelation"/>
<rdfs:domain 
rdf:resource="http://127.0.0.1:8000/ontology/SUMO.owl#FinancialTransaction"/>
<rdfs:range rdf:resource = 
"http://127.0.0.1:8000/ontology/SUMO.owl#CurrencyMeasure"/>
</owl:ObjectProperty>

<owl:DatatypeProperty  rdf:ID= "protonNumber">
<rdfs:comment>(protonNumber ?SUBSTANCE ?NUMBER) means that
the PureSubstance ?SUBSTANCE has the number of Protons 
?NUMBER.</rdfs:comment>
<rdf:type rdf:resource = 
"http://127.0.0.1:8000/ontology/SUMO.owl#BinaryPredicate"/>
<rdf:type rdf:resource = 
"http://127.0.0.1:8000/ontology/SUMO.owl#SingleValuedRelation"/>
<rdf:type rdf:resource = 
"http://127.0.0.1:8000/ontology/SUMO.owl#TotalValuedRelation"/>
<rdfs:domain 
rdf:resource="http://127.0.0.1:8000/ontology/SUMO.owl#PureSubstance"/>
<rdfs:range rdf:resource = 
"http://127.0.0.1:8000/ontology/SUMO.owl#PositiveInteger"/>
</owl:DatatypeProperty>

<owl:ObjectProperty   rdf:ID= "quarter">
<rdfs:comment>(quarter ?QUART ?WHOLE) means that ?QUART is a
quarter of ?WHOLE.</rdfs:comment>
<rdfs:subPropertyOf rdf:resource="http://127.0.0.1:8000/ontology/SUMO.owl#part"/>
</owl:ObjectProperty>

<owl:ObjectProperty   rdf:ID= "reactant">
<rdfs:comment>(reactant ?PROCESS ?SUBSTANCE) means that ?SUBSTANCE
is a chemical reactant in the chemical reaction ?PROCESS, i.e. ?SUBSTANCE is
present at the beginning of the chemical reaction ?PROCESS.</rdfs:comment>
<rdfs:domain 
rdf:resource="http://127.0.0.1:8000/ontology/SUMO.owl#ChemicalProcess"/>
<rdfs:range rdf:resource = "http://127.0.0.1:8000/ontology/SUMO.owl#Substance"/>
<rdfs:subPropertyOf 
rdf:resource="http://127.0.0.1:8000/ontology/SUMO.owl#resource"/>
</owl:ObjectProperty>

<owl:ObjectProperty   rdf:ID= "reagent">
<rdfs:comment>(reagent ?PROCESS ?SUBSTANCE) means that ?SUBSTANCE
is a chemical agent in the chemical reaction ?PROCESS.</rdfs:comment>
<rdfs:domain 
rdf:resource="http://127.0.0.1:8000/ontology/SUMO.owl#ChemicalProcess"/>
<rdfs:range rdf:resource = "http://127.0.0.1:8000/ontology/SUMO.owl#Substance"/>
<rdfs:subPropertyOf 
rdf:resource="http://127.0.0.1:8000/ontology/SUMO.owl#instrument"/>
</owl:ObjectProperty>

<owl:ObjectProperty   rdf:ID= "registeredItem">
<rdfs:comment>(registeredItem ?DOCUMENT ?ITEM) means
that the Text ?DOCUMENT contains an official record of the Physical
thing ?ITEM.  The registered item could be an object or an event, e.g.,
an automobile, a ship, a marriage, an adoption.</rdfs:comment>
<rdf:type rdf:resource = 
"http://127.0.0.1:8000/ontology/SUMO.owl#BinaryPredicate"/>
<rdfs:domain rdf:resource="http://127.0.0.1:8000/ontology/SUMO.owl#Text"/>
<rdfs:range rdf:resource = "http://127.0.0.1:8000/ontology/SUMO.owl#Physical"/>
<rdfs:subPropertyOf 
rdf:resource="http://127.0.0.1:8000/ontology/SUMO.owl#refers"/>
</owl:ObjectProperty>

<owl:ObjectProperty   rdf:ID= "relatedEvent">
<rdfs:comment>(relatedEvent ?EVENT1 ?EVENT2) means
that the Process ?EVENT1 is related to the Process ?EVENT2.  The
relationship is between separate individual events, not events and
their subprocesses.  On the other hand, two subProcesses of the same
overarching event may be relatedEvents.  The argument order does not
imply temporal ordering.</rdfs:comment>
<rdf:type rdf:resource = 
"http://127.0.0.1:8000/ontology/SUMO.owl#BinaryPredicate"/>
<rdf:type rdf:resource = 
"http://127.0.0.1:8000/ontology/SUMO.owl#SymmetricRelation"/>
<rdfs:domain rdf:resource="http://127.0.0.1:8000/ontology/SUMO.owl#Process"/>
</owl:ObjectProperty>

<owl:ObjectProperty   rdf:ID= "religiousAffiliationOfOrganization">
<rdfs:comment>(religiousAffiliationOfOrganization
?ORG ?BELIEF) means that one of the goals of ?ORG is to advance the 
religious teachings
of the BeliefGroup ?BELIEF.</rdfs:comment>
<rdf:type rdf:resource = 
"http://127.0.0.1:8000/ontology/SUMO.owl#BinaryPredicate"/>
<rdfs:domain 
rdf:resource="http://127.0.0.1:8000/ontology/SUMO.owl#Organization"/>
<rdfs:range rdf:resource = 
"http://127.0.0.1:8000/ontology/SUMO.owl#BeliefGroup"/>
</owl:ObjectProperty>

<owl:ObjectProperty  rdf:about= 
"http://127.0.0.1:8000/ontology/SUMO.owl#resource">
<rdfs:subPropertyOf rdf:resource="#involvedInEvent"/>
</owl:ObjectProperty>

<owl:ObjectProperty  rdf:about= "http://127.0.0.1:8000/ontology/SUMO.owl#result">
<rdfs:subPropertyOf rdf:resource="#involvedInEvent"/>
</owl:ObjectProperty>

<owl:ObjectProperty   rdf:ID= "routeInSystem">
<rdfs:comment>(routeInSystem ?PART ?SYSTEM) means that
the Transitway ?PART is an established route of the
TransportationSystem ?SYSTEM.</rdfs:comment>
<rdf:type rdf:resource = 
"http://127.0.0.1:8000/ontology/SUMO.owl#BinaryPredicate"/>
<rdfs:domain rdf:resource="http://127.0.0.1:8000/ontology/SUMO.owl#Transitway"/>
<rdfs:range rdf:resource = "#TransportationSystem"/>
<rdfs:subPropertyOf rdf:resource="#pathInSystem"/>
</owl:ObjectProperty>

<owl:ObjectProperty   rdf:ID= "secretesSubstance">
<rdfs:comment>(secretesSubstance ?OBJ ?STUFF) means
that the subclass of OrganicObject (either Organism or BodyPart)
?OBJ produces the subclass of Substance ?STUFF.</rdfs:comment>
<rdf:type rdf:resource = 
"http://127.0.0.1:8000/ontology/SUMO.owl#BinaryPredicate"/>
<rdfs:domain 
rdf:resource="http://127.0.0.1:8000/ontology/SUMO.owl#OrganicObject"/>
<rdfs:range rdf:resource = 
"http://127.0.0.1:8000/ontology/SUMO.owl#NaturalSubstance"/>
</owl:ObjectProperty>

<owl:ObjectProperty   rdf:ID= "securedBy">
<rdfs:comment>Assets pledged by a borrower to secure a loan
or other credit, and subject to seizure in the event of 
FinancialDefault.</rdfs:comment>
<rdf:type rdf:resource = 
"http://127.0.0.1:8000/ontology/SUMO.owl#BinaryPredicate"/>
<rdfs:domain rdf:resource="#FinancialAccount"/>
<rdfs:range rdf:resource = "http://127.0.0.1:8000/ontology/SUMO.owl#Object"/>
</owl:ObjectProperty>

<owl:ObjectProperty   rdf:ID= "sententialObject">
<rdfs:comment>(sententialObject ?OBJECT ?SENTENCE)
means that the NounPhrase ?OBJECT is the object of the Sentence
?SENTENCE.</rdfs:comment>
<rdfs:domain rdf:resource="http://127.0.0.1:8000/ontology/SUMO.owl#NounPhrase"/>
<rdfs:range rdf:resource = "http://127.0.0.1:8000/ontology/SUMO.owl#Sentence"/>
<rdfs:subPropertyOf rdf:resource="#grammaticalRelation"/>
</owl:ObjectProperty>

<owl:ObjectProperty   rdf:ID= "sententialSubject">
<rdfs:comment>(sententialSubject ?SUBJECT ?SENTENCE)
means that the NounPhrase ?SUBJECT is the subject of the Sentence
?SENTENCE.</rdfs:comment>
<rdfs:domain rdf:resource="http://127.0.0.1:8000/ontology/SUMO.owl#NounPhrase"/>
<rdfs:range rdf:resource = "http://127.0.0.1:8000/ontology/SUMO.owl#Sentence"/>
<rdfs:subPropertyOf rdf:resource="#grammaticalRelation"/>
</owl:ObjectProperty>

<owl:ObjectProperty   rdf:ID= "sideOfFigure">
<rdfs:comment>(sideOfFigure ?SIDE ?FIGURE) means that the
OneDimensionalFigure ?SIDE is a side of the Polygon ?FIGURE.</rdfs:comment>
<rdfs:domain 
rdf:resource="http://127.0.0.1:8000/ontology/SUMO.owl#OneDimensionalFigure"/>
<rdfs:range rdf:resource = "#Polygon"/>
<rdfs:subPropertyOf 
rdf:resource="http://127.0.0.1:8000/ontology/SUMO.owl#geometricPart"/>
</owl:ObjectProperty>

<owl:ObjectProperty   rdf:ID= "signedBy">
<rdfs:comment>(signedBy ?Certificate ?Agent) means that ?Certificate
has been signed by ?Agent.</rdfs:comment>
<rdf:type rdf:resource = 
"http://127.0.0.1:8000/ontology/SUMO.owl#BinaryPredicate"/>
<rdfs:domain rdf:resource="http://127.0.0.1:8000/ontology/SUMO.owl#Certificate"/>
<rdfs:range rdf:resource = 
"http://127.0.0.1:8000/ontology/SUMO.owl#CognitiveAgent"/>
</owl:ObjectProperty>

<owl:ObjectProperty   rdf:ID= "speaksLanguage">
<rdfs:comment>(speaksLanguage ?AGENT ?LANGUAGE) means that the
SentientAgent ?AGENT is capable of understanding and/or generating the 
Language
?LANGUAGE.</rdfs:comment>
<rdf:type rdf:resource = 
"http://127.0.0.1:8000/ontology/SUMO.owl#BinaryPredicate"/>
<rdfs:domain 
rdf:resource="http://127.0.0.1:8000/ontology/SUMO.owl#SentientAgent"/>
<rdfs:range rdf:resource = "http://127.0.0.1:8000/ontology/SUMO.owl#Language"/>
</owl:ObjectProperty>

<owl:ObjectProperty   rdf:ID= "stepfather">
<rdfs:comment>(stepfather ?PERSON ?FATHER) means that ?FATHER
is the stepfather of ?PERSON, i.e. ?FATHER is the spouse of the mother
of ?PERSON, without also being the father of ?PERSON.</rdfs:comment>
<rdfs:domain rdf:resource="http://127.0.0.1:8000/ontology/SUMO.owl#Human"/>
<rdfs:range rdf:resource = "http://127.0.0.1:8000/ontology/SUMO.owl#Man"/>
<rdfs:subPropertyOf 
rdf:resource="http://127.0.0.1:8000/ontology/SUMO.owl#legalRelation"/>
</owl:ObjectProperty>

<owl:ObjectProperty   rdf:ID= "stepmother">
<rdfs:comment>(stepmother ?PERSON ?MOTHER) means that ?MOTHER
is the stepmother of ?PERSON, i.e. ?MOTHER is the spouse of the father
of ?PERSON, without also being the mother of ?PERSON.</rdfs:comment>
<rdfs:domain rdf:resource="http://127.0.0.1:8000/ontology/SUMO.owl#Human"/>
<rdfs:range rdf:resource = "http://127.0.0.1:8000/ontology/SUMO.owl#Woman"/>
<rdfs:subPropertyOf 
rdf:resource="http://127.0.0.1:8000/ontology/SUMO.owl#legalRelation"/>
</owl:ObjectProperty>

<owl:ObjectProperty   rdf:ID= "stockHolder">
<rdfs:comment>(stockHolder ?Stock ?Agent) means that
?Agent possesses the Stock ?Stock.</rdfs:comment>
<rdf:type rdf:resource = 
"http://127.0.0.1:8000/ontology/SUMO.owl#BinaryPredicate"/>
<rdfs:domain rdf:resource="#Stock"/>
<rdfs:range rdf:resource = 
"http://127.0.0.1:8000/ontology/SUMO.owl#CognitiveAgent"/>
</owl:ObjectProperty>

<owl:ObjectProperty   rdf:ID= "streetAddress">
<rdfs:comment>(streetAddress ?STREET ?ADDRESS) means
that the Roadway ?STREET is part of the address ?ADDRESS.</rdfs:comment>
<rdfs:domain rdf:resource="http://127.0.0.1:8000/ontology/SUMO.owl#Roadway"/>
<rdfs:range rdf:resource = "#Address"/>
<rdfs:subPropertyOf rdf:resource="#address"/>
</owl:ObjectProperty>

<owl:ObjectProperty   rdf:ID= "streetNumber">
<rdfs:comment>(streetNumber ?BUILDING ?ADDRESS) means
that the Building ?BUILDING is part of the address ?ADDRESS.</rdfs:comment>
<rdfs:domain rdf:resource="http://127.0.0.1:8000/ontology/SUMO.owl#Building"/>
<rdfs:range rdf:resource = "#Address"/>
<rdfs:subPropertyOf rdf:resource="#address"/>
</owl:ObjectProperty>

<owl:ObjectProperty   rdf:ID= "student">
<rdfs:comment>(student ?AGENT ?ORG) means that ?AGENT is enrolled
in the EducationalOrganization ?ORG.</rdfs:comment>
<rdfs:domain 
rdf:resource="http://127.0.0.1:8000/ontology/SUMO.owl#CognitiveAgent"/>
<rdfs:range rdf:resource = 
"http://127.0.0.1:8000/ontology/SUMO.owl#EducationalOrganization"/>
<rdfs:subPropertyOf 
rdf:resource="http://127.0.0.1:8000/ontology/SUMO.owl#member"/>
</owl:ObjectProperty>

<owl:ObjectProperty   rdf:ID= "subField">
<rdfs:comment>(subField ?FIELD1 ?FIELD2) means that ?FIELD1 is a proper
part of the FieldOfStudy ?FIELD2.  For example, Physiology is a subField of
Biology.</rdfs:comment>
<rdf:type rdf:resource = 
"http://127.0.0.1:8000/ontology/SUMO.owl#TransitiveRelation"/>
<rdf:type rdf:resource = 
"http://127.0.0.1:8000/ontology/SUMO.owl#IrreflexiveRelation"/>
<rdfs:domain 
rdf:resource="http://127.0.0.1:8000/ontology/SUMO.owl#FieldOfStudy"/>
<rdfs:range rdf:resource = 
"http://127.0.0.1:8000/ontology/SUMO.owl#FieldOfStudy"/>
<rdfs:subPropertyOf 
rdf:resource="http://127.0.0.1:8000/ontology/SUMO.owl#subProposition"/>
</owl:ObjectProperty>

<owl:ObjectProperty   rdf:ID= "subGraph">
<rdfs:comment>The relation between two Graphs when one
Graph is a part of the other.  (subGraph ?GRAPH1 ?GRAPH2) means
that ?GRAPH1 is a part of ?GRAPH2.</rdfs:comment>
<rdf:type rdf:resource = 
"http://127.0.0.1:8000/ontology/SUMO.owl#BinaryPredicate"/>
<rdf:type rdf:resource = 
"http://127.0.0.1:8000/ontology/SUMO.owl#ReflexiveRelation"/>
<rdf:type rdf:resource = 
"http://127.0.0.1:8000/ontology/SUMO.owl#TransitiveRelation"/>
<rdfs:domain rdf:resource="#Graph"/>
<rdfs:range rdf:resource = "#Graph"/>
</owl:ObjectProperty>

<owl:ObjectProperty   rdf:ID= "subRegion">
<rdfs:comment>(subRegion ?PART ?WHOLE) means that the Region
?PART is a part of the Region ?WHOLE.</rdfs:comment>
<rdfs:domain rdf:resource="http://127.0.0.1:8000/ontology/SUMO.owl#Region"/>
<rdfs:range rdf:resource = "http://127.0.0.1:8000/ontology/SUMO.owl#Region"/>
<rdfs:subPropertyOf rdf:resource="http://127.0.0.1:8000/ontology/SUMO.owl#part"/>
</owl:ObjectProperty>

<owl:ObjectProperty   rdf:ID= "tangent">
<rdfs:comment>(tangent ?LINE ?CIRCLE) means that the straight line
?LINE is tangent to the Circle ?CIRCLE, i.e. ?LINE touches ?CIRCLE without
intersecting it.</rdfs:comment>
<rdf:type rdf:resource = 
"http://127.0.0.1:8000/ontology/SUMO.owl#BinaryPredicate"/>
<rdfs:domain 
rdf:resource="http://127.0.0.1:8000/ontology/SUMO.owl#OneDimensionalFigure"/>
<rdfs:range rdf:resource = "#Circle"/>
</owl:ObjectProperty>

<owl:ObjectProperty   rdf:ID= "targetInAttack">
<rdf:type rdf:resource = 
"http://127.0.0.1:8000/ontology/SUMO.owl#BinaryPredicate"/>
<rdfs:domain rdf:resource="http://127.0.0.1:8000/ontology/SUMO.owl#Process"/>
<rdfs:range rdf:resource = "http://127.0.0.1:8000/ontology/SUMO.owl#Object"/>
</owl:ObjectProperty>

<owl:ObjectProperty   rdf:ID= "teacher">
<rdfs:comment>(teacher ?AGENT ?ORG) means that ?AGENT is a
teacher at the EducationalOrganization ?ORG.</rdfs:comment>
<rdfs:domain 
rdf:resource="http://127.0.0.1:8000/ontology/SUMO.owl#CognitiveAgent"/>
<rdfs:range rdf:resource = 
"http://127.0.0.1:8000/ontology/SUMO.owl#EducationalOrganization"/>
<rdfs:subPropertyOf 
rdf:resource="http://127.0.0.1:8000/ontology/SUMO.owl#member"/>
</owl:ObjectProperty>

<owl:ObjectProperty   rdf:ID= "telephoneNumber">
<rdfs:comment>(telephoneNumber ?NUMBER ?AGENT) means
that ?NUMBER is a telephone number at which ?AGENT can be regularly 
contacted.</rdfs:comment>
<rdfs:domain 
rdf:resource="http://127.0.0.1:8000/ontology/SUMO.owl#SymbolicString"/>
<rdfs:range rdf:resource = "http://127.0.0.1:8000/ontology/SUMO.owl#Agent"/>
<rdfs:subPropertyOf 
rdf:resource="http://127.0.0.1:8000/ontology/SUMO.owl#uniqueIdentifier"/>
<sumo:relatedInternalConcept rdf:resource = "#address" />
</owl:ObjectProperty>

<owl:ObjectProperty   rdf:ID= "tenant">
<rdfs:comment>(tenant ?PERSON ?UNIT) means that ?PERSON is a tenant
of the Residence ?UNIT, i.e. he or she is renting the unit.</rdfs:comment>
<rdf:type rdf:resource = 
"http://127.0.0.1:8000/ontology/SUMO.owl#BinaryPredicate"/>
<rdfs:domain rdf:resource="http://127.0.0.1:8000/ontology/SUMO.owl#Human"/>
<rdfs:range rdf:resource = "http://127.0.0.1:8000/ontology/SUMO.owl#Residence"/>
</owl:ObjectProperty>

<owl:ObjectProperty   rdf:ID= "third">
<rdfs:comment>(third ?THIRD ?WHOLE) means that ?THIRD is one
third of ?WHOLE.</rdfs:comment>
<rdfs:subPropertyOf rdf:resource="http://127.0.0.1:8000/ontology/SUMO.owl#part"/>
</owl:ObjectProperty>

<owl:ObjectProperty   rdf:ID= "titles">
<rdfs:comment>A predicate used to indicate the title of a Text.
Note that the second argument type restriction is a subclass, rather than
an instance, of Text.  Thus, the title Murder_on_the_Orient_Express
corresponds to a large class of Books, and not just to a single copy of
the book.</rdfs:comment>
<rdfs:domain 
rdf:resource="http://127.0.0.1:8000/ontology/SUMO.owl#SymbolicString"/>
<rdfs:subPropertyOf 
rdf:resource="http://127.0.0.1:8000/ontology/SUMO.owl#names"/>
</owl:ObjectProperty>

<owl:ObjectProperty   rdf:ID= "totalGDP">
<rdfs:comment>(totalGDP ?AREA ?AMOUNT) means that the value
of all final goods and services produced within the GeopoliticalArea
?AREA is ?AMOUNT, in U.S. dollars, calculated on a purchasing power parity
basis.  This represents Gross Domestic Product (GDP).</rdfs:comment>
<rdf:type rdf:resource = 
"http://127.0.0.1:8000/ontology/SUMO.owl#BinaryPredicate"/>
<rdfs:domain 
rdf:resource="http://127.0.0.1:8000/ontology/SUMO.owl#GeopoliticalArea"/>
<rdfs:range rdf:resource = 
"http://127.0.0.1:8000/ontology/SUMO.owl#CurrencyMeasure"/>
</owl:ObjectProperty>

<owl:ObjectProperty   rdf:ID= "uncle">
<rdfs:comment>(uncle ?UNCLE ?PERSON) means that ?UNCLE is
the brother of a parent of ?PERSON.</rdfs:comment>
<rdfs:domain rdf:resource="http://127.0.0.1:8000/ontology/SUMO.owl#Man"/>
<rdfs:range rdf:resource = "http://127.0.0.1:8000/ontology/SUMO.owl#Human"/>
<rdfs:subPropertyOf 
rdf:resource="http://127.0.0.1:8000/ontology/SUMO.owl#familyRelation"/>
</owl:ObjectProperty>

<owl:ObjectProperty   rdf:ID= "unitNumber">
<rdfs:comment>(unitNumber ?UNIT ?ADDRESS) means that the
StationaryArtifact ?UNIT is part of the address ?ADDRESS.</rdfs:comment>
<rdfs:domain 
rdf:resource="http://127.0.0.1:8000/ontology/SUMO.owl#StationaryArtifact"/>
<rdfs:range rdf:resource = "#Address"/>
<rdfs:subPropertyOf rdf:resource="#address"/>
</owl:ObjectProperty>

<owl:ObjectProperty   rdf:ID= "waterDepth">
<rdfs:comment>(waterDepth ?AREA ?LENGTH) means that the
depth of water at the Region ?AREA is ?LENGTH.</rdfs:comment>
<rdfs:domain rdf:resource="http://127.0.0.1:8000/ontology/SUMO.owl#WaterArea"/>
<rdfs:range rdf:resource = 
"http://127.0.0.1:8000/ontology/SUMO.owl#LengthMeasure"/>
<rdfs:subPropertyOf 
rdf:resource="http://127.0.0.1:8000/ontology/SUMO.owl#length"/>
</owl:ObjectProperty>

<owl:ObjectProperty   rdf:ID= "wavelength">
<rdfs:comment>(wavelength ?RADIATION ?MEASURE) means that the
instance of radiation, ?RADIATION, has an average wavelength of 
?MEASURE.</rdfs:comment>
<rdf:type rdf:resource = 
"http://127.0.0.1:8000/ontology/SUMO.owl#SingleValuedRelation"/>
<rdfs:domain rdf:resource="http://127.0.0.1:8000/ontology/SUMO.owl#Radiating"/>
<rdfs:range rdf:resource = 
"http://127.0.0.1:8000/ontology/SUMO.owl#LengthMeasure"/>
<rdfs:subPropertyOf 
rdf:resource="http://127.0.0.1:8000/ontology/SUMO.owl#measure"/>
</owl:ObjectProperty>

<owl:DatatypeProperty  rdf:ID= "yearOfFounding">
<rdfs:comment>(yearOfFounding ?ORG ?NUMBER) means that the Organization
?ORG was founded in the year expressed in ?NUMBER.</rdfs:comment>
<rdf:type rdf:resource = 
"http://127.0.0.1:8000/ontology/SUMO.owl#BinaryPredicate"/>
<rdf:type rdf:resource = 
"http://127.0.0.1:8000/ontology/SUMO.owl#AsymmetricRelation"/>
<rdfs:domain 
rdf:resource="http://127.0.0.1:8000/ontology/SUMO.owl#Organization"/>
<rdfs:range rdf:resource = "http://127.0.0.1:8000/ontology/SUMO.owl#Integer"/>
</owl:DatatypeProperty>

</rdf:RDF>
