<rdf:RDF
xmlns = "http://127.0.0.1:8000/ontology/simplified_sumo.owl#"
xml:base = "http://127.0.0.1:8000/ontology/simplified_sumo.owl"
xmlns:rdf = "http://www.w3.org/1999/02/22-rdf-syntax-ns#"
xmlns:rdfs="http://www.w3.org/2000/01/rdf-schema#"
xmlns:owl="http://www.w3.org/2002/07/owl#"
>

<owl:Class rdf:ID= "AgriculturalProduct">
<rdfs:subClassOf rdf:resource ="#Product"/>
<rdfs:subClassOf rdf:resource ="#OrganicObject"/>
<rdfs:comment>AgriculturalProduct is the
subclass of Product that comprises the products of agricultural
activity.</rdfs:comment>
</owl:Class>


<owl:Class rdf:ID= "Product">
<rdfs:subClassOf rdf:resource ="#Artifact"/>
<rdfs:comment>An Artifact that is produced by Manufacture and
that is intended to be sold.</rdfs:comment>
</owl:Class>

<owl:Class rdf:ID= "Artifact">
<rdfs:subClassOf rdf:resource ="#CorpuscularObject"/>
<rdfs:comment>A CorpuscularObject that is the product of a
Making.</rdfs:comment>
</owl:Class>

<owl:Class rdf:ID= "CorpuscularObject">
<rdfs:subClassOf rdf:resource ="#SelfConnectedObject"/>
<rdfs:comment>A SelfConnectedObject whose parts have
properties that are not shared by the whole.</rdfs:comment>
</owl:Class>

<owl:Class rdf:ID= "SelfConnectedObject">
<rdfs:subClassOf rdf:resource ="#Object"/>
<rdfs:comment>A SelfConnectedObject is any
Object that does not consist of two or more disconnected parts.</rdfs:comment>
</owl:Class>

<owl:Class rdf:ID= "Object">
<rdfs:subClassOf rdf:resource ="#Physical"/>
<rdfs:comment>Corresponds roughly to the class of ordinary
objects.  Examples include normal physical objects, geographical regions,
and locations of Processes, the complement of Objects in the Physical
class.  In a 4D ontology, an Object is something whose spatiotemporal
extent is thought of as dividing into spatial parts roughly parallel to the
time-axis.</rdfs:comment>
</owl:Class>

<owl:Class rdf:ID= "Physical">
<rdfs:subClassOf rdf:resource ="#Entity"/>
<rdfs:comment>An entity that has a location in space-time.
Note that locations are themselves understood to have a location in
space-time.</rdfs:comment>
</owl:Class>

<owl:Class rdf:ID= "Entity">
<rdfs:comment>The universal class of individuals.  This is the root
node of the ontology.</rdfs:comment>
</owl:Class>

<owl:Class rdf:ID= "OrganicObject">
<rdfs:subClassOf rdf:resource ="#CorpuscularObject"/>
<rdfs:comment>This class encompasses Organisms,
CorpuscularObjects that are parts of Organisms, i.e. BodyParts,
and CorpuscularObjects that are nonintentionally produced by
Organisms, e.g. ReproductiveBodies.</rdfs:comment>
</owl:Class>

<owl:Class rdf:ID= "ManufacturedProduct">
<rdfs:subClassOf rdf:resource ="#Product"/>
<rdfs:comment>ManufacturedProduct is
the subclass of Product that includes goods that are produced
or assembled in factories or other manufacturing processes,
in contrast to AgriculturalProducts.</rdfs:comment>
</owl:Class>

<owl:Class rdf:ID= "CanadianDollar">
<rdfs:subClassOf rdf:resource ="#CurrencyMeasure"/>
<rdfs:subClassOf rdf:resource = "#UnitOfMeasure"/>
<rdfs:comment>CanadianDollar represents the basic unit of
currency of Canada.</rdfs:comment>
</owl:Class>

<owl:Class rdf:about= "#EuroDollar">
<rdfs:subClassOf rdf:resource ="#CurrencyMeasure"/>
<rdfs:subClassOf rdf:resource = "#UnitOfMeasure"/>
<rdfs:comment>EuroDollar represents the basic unit of
currency of the EuropeanUnion.</rdfs:comment>
</owl:Class>


<owl:Class rdf:ID= "FrenchFranc">
<rdfs:subClassOf rdf:resource ="#CurrencyMeasure"/>
<rdfs:subClassOf rdf:resource = "#UnitOfMeasure"/>
<rdfs:comment>FrenchFranc represents the basic unit of
currency of France.</rdfs:comment>
</owl:Class>

<owl:Class rdf:ID= "GermanMark">
<rdfs:subClassOf rdf:resource ="#CurrencyMeasure"/>
<rdfs:subClassOf rdf:resource = "#UnitOfMeasure"/>
<rdfs:comment>GermanMark represents the basic unit of
currency of Germany.</rdfs:comment>
</owl:Class>

<owl:Class rdf:ID= "ItalianLire">
<rdfs:subClassOf rdf:resource ="#CurrencyMeasure"/>
<rdfs:subClassOf rdf:resource = "#UnitOfMeasure"/>
<rdfs:comment>ItalianLire represents the basic unit of
currency of Italy.</rdfs:comment>
</owl:Class>

<owl:Class rdf:ID= "JapaneseYen">
<rdfs:subClassOf rdf:resource ="#CurrencyMeasure"/>
<rdfs:subClassOf rdf:resource = "#UnitOfMeasure"/>
<rdfs:comment>JapaneseYen represents the basic unit of
currency of Japan.</rdfs:comment>
</owl:Class>

<owl:Class rdf:ID= "OldTajikSomoni">
<rdfs:subClassOf rdf:resource ="#CurrencyMeasure"/>
<rdfs:subClassOf rdf:resource = "#UnitOfMeasure"/>
<rdfs:comment>OldTajikSomoni represents a former unit of
currency of Tajikistan.</rdfs:comment>
</owl:Class>

<owl:Class rdf:ID= "TajikSomoni">
<rdfs:subClassOf rdf:resource ="#CurrencyMeasure"/>
<rdfs:subClassOf rdf:resource = "#UnitOfMeasure"/>
<rdfs:comment>TajikSomoni represents the basic unit of
currency of Tajikistan.</rdfs:comment>
</owl:Class>

<owl:Class rdf:ID= "AfghanAfghani">
<rdfs:subClassOf rdf:resource ="#CurrencyMeasure"/>
<rdfs:subClassOf rdf:resource = "#UnitOfMeasure"/>
<rdfs:comment>AfghanAfghani represents the basic unit of
currency of Afghanistan.</rdfs:comment>
</owl:Class>

<owl:Class rdf:ID= "BritishPound">
<rdfs:subClassOf rdf:resource ="#CurrencyMeasure"/>
<rdfs:subClassOf rdf:resource = "#UnitOfMeasure"/>
<rdfs:comment>BritishPound represents the basic unit of
currency of the UnitedKingdomOfGreatBritainAndNorthernIreland.</rdfs:comment>
</owl:Class>

<owl:Class rdf:ID= "CurrencyMeasure">
<rdfs:subClassOf rdf:resource ="#ConstantQuantity"/>
<rdfs:comment>Includes all standard measures of monetary
value, including UnitedStatesDollar, UnitedStatesCent, Lire, Yen, etc.</rdfs:comment>
</owl:Class>

<owl:Class rdf:ID= "ConstantQuantity">
<rdfs:subClassOf rdf:resource ="#PhysicalQuantity"/>
<rdfs:comment>A ConstantQuantity is a
PhysicalQuantity which has a constant value, e.g. 3 meters and 5 hours.
The magnitude (see MagnitudeFn) of every ConstantQuantity is a
RealNumber.  ConstantQuantities are distinguished from
FunctionQuantities, which map ConstantQuantities to other
ConstantQuantities.  All ConstantQuantites are expressed with the
BinaryFunction MeasureFn, which takes a Number and a UnitOfMeasure
as arguments.  For example, 3 Meters can be expressed as (MeasureFn 3
Meter).  ConstantQuantities form a partial order (see
PartialOrderingRelation) with the lessThan relation, since lessThan
is a RelationExtendedToQuantities and lessThan is defined over the
RealNumbers.  The lessThan relation is not a total order (see
TotalOrderingRelation) over the class ConstantQuantity since elements
of some subclasses of ConstantQuantity (such as length quantities)
are incomparable to elements of other subclasses of ConstantQuantity
(such as mass quantities).</rdfs:comment>
</owl:Class>

<owl:Class rdf:ID= "PhysicalQuantity">
<rdfs:subClassOf rdf:resource ="#Quantity"/>
<rdfs:comment>A PhysicalQuantity is a measure of
some quantifiable aspect of the modeled world, such as 'the earth's
diameter' (a constant length) and 'the stress in a loaded deformable
solid' (a measure of stress, which is a function of three spatial
coordinates).  All PhysicalQuantities are either ConstantQuantities
or FunctionQuantities.  Instances of ConstantQuantity are dependent
on a UnitOfMeasure, while instances of FunctionQuantity are
Functions that map instances of ConstantQuantity to other instances
of ConstantQuantity (e.g., TimeDependentQuantities are
FunctionQuantities).  Although the name and definition of
PhysicalQuantity is borrowed from physics, PhysicalQuantities need
not be material.  Aside from the dimensions of length, time, velocity,
etc., nonphysical dimensions such as currency are also possible.
Accordingly, amounts of money would be instances of PhysicalQuantity.
PhysicalQuantities are distinguished from Numbers by the fact that
the former are associated with a dimension of measurement.</rdfs:comment>
</owl:Class>

<owl:Class rdf:ID= "Quantity">
<rdfs:subClassOf rdf:resource ="#Abstract"/>
<rdfs:comment>Any specification of how many or how much of
something there is.  Accordingly, there are two subclasses of Quantity:
Number (how many) and PhysicalQuantity (how much).</rdfs:comment>
</owl:Class>

<owl:Class rdf:ID= "Abstract">
<rdfs:subClassOf rdf:resource ="#Entity"/>
<rdfs:comment>Properties or qualities as distinguished from any
particular embodiment of the properties/qualities in a physical medium.
Instances of Abstract can be said to exist in the same sense as mathematical
objects such as sets and relations, but they cannot exist at a particular
place and time without some physical encoding or embodiment.</rdfs:comment>
</owl:Class>


<owl:Class rdf:ID= "ClothesDrier">
<rdfs:subClassOf rdf:resource ="#MajorAppliance"/>
<rdfs:comment>ClothesDrier is the class of automatic clothes
driers.</rdfs:comment>
</owl:Class>

<owl:Class rdf:ID= "ClothesWashingMachine">
<rdfs:subClassOf rdf:resource ="#MajorAppliance"/>
<rdfs:comment>ClothesWashingMachine is the class of
washing machines.</rdfs:comment>
</owl:Class>


<owl:Class rdf:ID= "CookingOven">
<rdfs:subClassOf rdf:resource ="#MajorAppliance"/>
<rdfs:comment>CookingOven is the class of ovens for cooking.</rdfs:comment>
</owl:Class>

<owl:Class rdf:ID= "CookingRange">
<rdfs:subClassOf rdf:resource ="#MajorAppliance"/>
<rdfs:comment>CookingRange is the class of cooktops or
ranges.</rdfs:comment>
</owl:Class>

<owl:Class rdf:ID= "Dishwasher">
<rdfs:subClassOf rdf:resource ="#MajorAppliance"/>
<rdfs:comment>Dishwasher is the class of automatic dishwashers.</rdfs:comment>
</owl:Class>

<owl:Class rdf:ID= "Freezer">
<rdfs:subClassOf rdf:resource ="#MajorAppliance"/>
<rdfs:comment>Freezer is the class of household freezers.</rdfs:comment>
</owl:Class>

<owl:Class rdf:ID= "HotWaterHeater">
<rdfs:subClassOf rdf:resource ="#MajorAppliance"/>
<rdfs:comment>HotWaterHeater is the class of hot water
heaters.</rdfs:comment>
</owl:Class>

<owl:Class rdf:ID= "Refrigerator">
<rdfs:subClassOf rdf:resource ="#MajorAppliance"/>
<rdfs:comment>Refrigerator is the class of refrigerators.</rdfs:comment>
</owl:Class>

<owl:Class rdf:ID= "MajorAppliance">
<rdfs:subClassOf rdf:resource ="#ElectricDevice"/>
<rdfs:comment>MajorAppliance is the subclass of
ElectricDevices that are large s manufactured for use
in household tasks.</rdfs:comment>
</owl:Class>


<owl:Class rdf:ID= "ElectricDevice">
<rdfs:subClassOf rdf:resource ="#Device"/>
<rdfs:comment>Any Device that is powered by electricity.</rdfs:comment>
</owl:Class>

<owl:Class rdf:ID= "Device">
<rdfs:subClassOf rdf:resource ="#Artifact"/>
<rdfs:comment>A Device is an Artifact whose purpose is to
serve as an instrument in a specific subclass of Process.</rdfs:comment>
</owl:Class>

<owl:Class rdf:ID= "KilowattHour">
<rdfs:subClassOf rdf:resource = "#UnitOfMeasure"/>
<rdfs:subClassOf rdf:resource ="#FunctionQuantity"/>
<rdfs:comment>KilowattHour is a UnitOfMeasure for
energy that represents 1000 Watts (1 kW) of power expended over one
hour (1 h) of time.  This is the unit commonly used in commercial
power contexts.  It is equivalent to 3,600,000 Joules.</rdfs:comment>
</owl:Class>

<owl:Class rdf:ID= "UnitOfMeasure">
<rdfs:subClassOf rdf:resource ="#PhysicalQuantity"/>
<rdfs:comment>A standard of measurement for some dimension.
For example, the Meter is a UnitOfMeasure for the dimension of length,
as is the Inch.  There is no intrinsic property of a UnitOfMeasure that
makes it primitive or fundamental; rather, a system of units (e.g.
SystemeInternationalUnit) defines a set of orthogonal dimensions and
assigns units for each.</rdfs:comment>
</owl:Class>

<owl:Class rdf:ID= "FunctionQuantity">
<rdfs:subClassOf rdf:resource ="#PhysicalQuantity"/>
<rdfs:comment>A FunctionQuantity is a PhysicalQuantity
that is returned by a Function that maps from one or more instances of
ConstantQuantity to another instance of ConstantQuantity.  For example,
the velocity of a particle would be represented by a FunctionQuantity
relating values of time (which are ConstantQuantities) to values of distance
(also ConstantQuantities).  Note that all elements of the range of the
Function corresponding to a FunctionQuantity have the same physical
dimension as the FunctionQuantity itself.</rdfs:comment>
</owl:Class>

<owl:Class rdf:ID= "CompoundSubstance">
<rdfs:subClassOf rdf:resource ="#PureSubstance"/>
<rdfs:comment>The Class of Substances that contain
two or more elements (ElementalSubstances), in definite proportion by weight.
The composition of a pure compound will be invariant, regardless of the method
of preparation. Compounds are composed of more than one kind of atom (element).
The term molecule is often used for the smallest unit of a compound that still
retains all of the properties of the compound.  Examples: Table salt (sodium
chloride, NaCl), sugar (sucrose, C_{12}H_{22}O_{11}), and water (H_2O). </rdfs:comment>
</owl:Class>


<owl:Class rdf:ID= "PureSubstance">
<rdfs:subClassOf rdf:resource ="#Substance"/>
<rdfs:comment>The Class of Substances with constant
composition.  A PureSubstance can be either an element (ElementalSubstance)
or a compound of elements (CompoundSubstance).  Examples: Table salt
(sodium chloride, NaCl), sugar (sucrose, C_{12}H_{22}O_{11}), water (H_2O),
iron (Fe), copper (Cu), and oxygen (O_2).</rdfs:comment>
</owl:Class>

<owl:Class rdf:ID= "Substance">
<rdfs:subClassOf rdf:resource ="#SelfConnectedObject"/>
<rdfs:comment>An Object in which every part is similar to
every other in every relevant respect.  More precisely, something is a
Substance when it has only arbitrary pieces as parts - any parts have
properties which are similar to those of the whole.  Note that a Substance
may nonetheless have physical properties that vary.  For example, the
temperature, chemical constitution, density, etc. may change from one part
to another.  An example would be a body of water.</rdfs:comment>
</owl:Class>

<owl:Class rdf:ID= "CropProduction">
<rdfs:subClassOf rdf:resource = "#IndustryAttribute"/>
<subAttribute rdf:resource = "#AgriculturalSector" />
<industryProductType rdf:resource = "#Plant" />
<rdfs:comment>CropProduction is the IndustryAttribute
that describes crop farming operations.</rdfs:comment>
</owl:Class>

<owl:Property   rdf:ID= "subAttribute">
<rdfs:comment>Means that the second argument can be
ascribed to everything which has the first argument ascribed to it.</rdfs:comment>
<rdfs:domain rdf:resource="#Attribute"/>
<rdfs:range rdf:resource = "#Attribute"/>
</owl:Property>


<owl:Class rdf:ID= "Attribute">
<rdfs:subClassOf rdf:resource ="#Abstract"/>
<rdfs:comment>Qualities which we cannot or choose not to
reify into subclasses of Object.</rdfs:comment>
</owl:Class>

<owl:Property   rdf:ID= "industryProductType">
<rdfs:comment>(industryProductType ?INDUSTRY ?TYPE) means that the Industry ?INDUSTRY
produces products of the kind ?TYPE.</rdfs:comment>
<rdfs:domain rdf:resource="#Industry"/>
<rdfs:range rdf:resource = "#Product"/>
</owl:Property>

<owl:Class rdf:ID= "Industry">
<rdfs:subClassOf rdf:resource ="#Collection"/>
<rdfs:comment>The class of Collections of Corporations
which are in the same line of business.</rdfs:comment>
</owl:Class>

<owl:Class rdf:ID= "Collection">
<rdfs:subClassOf rdf:resource ="#Object"/>
<rdfs:comment>Collections have members like Classes, but,
unlike Classes, they have a position in space-time and members can be
added and subtracted without thereby changing the identity of the
Collection.  Some examples are toolkits, football teams, and flocks
of sheep.</rdfs:comment>
</owl:Class>

<owl:Class rdf:ID= "IndustryAttribute">
<rdfs:subClassOf rdf:resource ="#RelationalAttribute"/>
<rdfs:comment>IndustryAttribute is a class of
Attributes which identify an Organization as belonging to a particular
industry type.  For example, the company Hallmark has the attribute
of GreetingCardPublishers.</rdfs:comment>
</owl:Class>

<owl:Class rdf:ID= "RelationalAttribute">
<rdfs:subClassOf rdf:resource ="#Attribute"/>
<rdfs:comment>Any Attribute that an Entity has by
virtue of a relationship that it bears to another Entity or set of Entities,
e.g. SocialRoles and PositionalAttributes.</rdfs:comment>
</owl:Class>

<owl:Class rdf:ID= "AgriculturalSector">
<rdfs:subClassOf rdf:resource = "#EconomicSector"/>
<rdfs:comment>AgriculturalSector is an attribute
that describes commercial organizations or agents whose business is in
the agricultural sector of the economy.</rdfs:comment>
</owl:Class>

<owl:Class rdf:ID= "EconomicSector">
<rdfs:subClassOf rdf:resource ="#IndustryAttribute"/>
<rdfs:comment>EconomicSector is the subclass of
IndustryAttributes that describe broad characterizations of different
kinds of business activities; e.g., manufacturing; services; retail trade;
wholesale trade; finance, insurance, and real estate; transportation and
utilities; construction; mining; agriculture, forestry, and fishing.</rdfs:comment>
</owl:Class>

<owl:Class rdf:ID= "Plant">
<rdfs:subClassOf rdf:resource ="#Organism"/>
<rdfs:comment>An Organism having cellulose cell walls, growing
by synthesis of Substances, generally distinguished by the presence of
chlorophyll, and lacking the power of locomotion.</rdfs:comment>
</owl:Class>

<owl:Class rdf:ID= "Organism">
<rdfs:subClassOf rdf:resource ="#OrganicObject"/>
<rdfs:subClassOf rdf:resource ="#Agent"/>
<rdfs:comment>Generally, a living individual, including all
Plants and Animals.</rdfs:comment>
</owl:Class>

<owl:Class rdf:ID= "Agent">
<rdfs:subClassOf rdf:resource ="#Object"/>
<rdfs:comment>Something or someone that can act on its own and
produce changes in the world.</rdfs:comment>
</owl:Class>

<owl:Class rdf:ID= "Vegetable">
<rdfs:subClassOf rdf:resource ="#FruitOrVegetable"/>
</owl:Class>

<owl:Class rdf:ID= "FruitOrVegetable">
<rdfs:subClassOf rdf:resource ="#PlantAnatomicalStructure"/>
<rdfs:subClassOf rdf:resource ="#ReproductiveBody"/>
<rdfs:comment>Any fruit or vegetable, i.e. a
ripened ReproductiveBody of a Plant.  Note that FruitOrVegetable
is not a subclass of Food, because some fruits, e.g. poisonous
berries, are not edible.</rdfs:comment>
</owl:Class>

<owl:Class rdf:ID= "PlantAnatomicalStructure">
<rdfs:subClassOf rdf:resource ="#AnatomicalStructure"/>
<rdfs:comment>AnatomicalStructures that
are possessed exclusively by Plants.</rdfs:comment>
</owl:Class>

<owl:Class rdf:ID= "AnatomicalStructure">
<rdfs:subClassOf rdf:resource ="#OrganicObject"/>
<rdfs:comment>A normal or pathological part
of the anatomy or structural organization of an Organism.  This
class covers BodyParts, as well as structures that are given off
by Organisms, e.g. ReproductiveBodies.</rdfs:comment>
</owl:Class>

<owl:Class rdf:ID= "ReproductiveBody">
<rdfs:subClassOf rdf:resource ="#BodyPart"/>
<rdfs:comment>Reproductive structure of Organisms.
Consists of an Embryonic Object and a nutritive/protective envelope.
Note that this class includes seeds, spores, and FruitOrVegetables, as
well as the eggs produced by Animals.</rdfs:comment>
</owl:Class>


<owl:Class rdf:ID= "BodyPart">
<rdfs:subClassOf rdf:resource ="#AnatomicalStructure"/>
<rdfs:comment>A collection of Cells and Tissues which
are localized to a specific area of an Organism and which are not
pathological. The instances of this Class range from gross structures
to small components of complex Organs.</rdfs:comment>
</owl:Class>

<owl:Class rdf:ID= "FinancialTransaction">
<rdfs:subClassOf rdf:resource ="#Transaction"/>
<rdfs:comment>A Transaction where an instance
of Currency is exchanged for something else.</rdfs:comment>
</owl:Class>

<owl:Class rdf:ID= "Transaction">
<rdfs:subClassOf rdf:resource ="#ChangeOfPossession"/>
<rdfs:subClassOf rdf:resource ="#DualObjectProcess"/>
<rdfs:comment>The subclass of ChangeOfPossession where
something is exchanged for something else.</rdfs:comment>
</owl:Class>

<owl:Class rdf:ID= "DualObjectProcess"/>

<owl:Class rdf:ID= "ChangeOfPossession">
<rdfs:subClassOf rdf:resource ="#SocialInteraction"/>
<relatedInternalConcept rdf:resource = "#possesses" />
<rdfs:comment>The Class of Processes where
ownership of something is transferred from one Agent to another.</rdfs:comment>
</owl:Class>


<owl:Class rdf:ID= "SocialInteraction">
<rdfs:subClassOf rdf:resource ="#IntentionalProcess"/>
<rdfs:comment>The subclass of
IntentionalProcess that involves interactions between
CognitiveAgents.</rdfs:comment>
</owl:Class>


<owl:Class rdf:ID= "IntentionalProcess">
<rdfs:subClassOf rdf:resource ="#Process"/>
<rdfs:comment>A Process that has a specific
purpose for the CognitiveAgent who performs it.</rdfs:comment>
</owl:Class>


<owl:Class rdf:ID= "Process">
<rdfs:subClassOf rdf:resource ="#Physical"/>
<rdfs:comment>Intuitively, the class of things that happen
and have temporal parts or stages.  Examples include extended events
like a football match or a race, actions like Pursuing and Reading,
and biological processes. The formal definition is: anything that lasts
for a time but is not an Object.  Note that a Process may have
participants 'inside' it which are Objects, such as the players
in a football match.  In a 4D ontology, a Process is something whose
spatiotemporal extent is thought of as dividing into temporal stages
roughly perpendicular to the time-axis.</rdfs:comment>
</owl:Class>

<owl:Property   rdf:ID= "relatedInternalConcept">
<rdfs:comment>Means that the two arguments are
related concepts within the SUMO, i.e. there is a significant similarity
of meaning between them.  To indicate a meaning relation between a SUMO
concept and a concept from another source, use the Predicate
relatedExternalConcept.</rdfs:comment>
<rdfs:domain rdf:resource="#Entity"/>
<rdfs:range rdf:resource = "#Entity"/>
</owl:Property>

<owl:Property   rdf:ID= "possesses">
<rdfs:comment>Relation that holds between an Agent and
an Object when the Agent has ownership of the Object.</rdfs:comment>
<rdfs:domain rdf:resource="#Agent"/>
<rdfs:range rdf:resource = "#Object"/>
</owl:Property>


<owl:Class rdf:ID= "Gemstone">
<rdfs:subClassOf rdf:resource ="#Object"/>
<rdfs:comment>Gemstone is the subclass of Minerals or
petrified organic substances that are especially valued for use in
jewelry and other decorative items; some Gemstones are also valuable
for mechanical or industrial applications.</rdfs:comment>
</owl:Class>


<owl:Class rdf:ID= "ProductPackage">
<rdfs:subClassOf rdf:resource ="#Object"/>
<rdfs:comment>ProductPackage is the class of objects
designed to contain Products for shipping and sale.</rdfs:comment>
</owl:Class>


<owl:Class rdf:ID= "IndependentState">
<rdfs:subClassOf rdf:resource ="#GeopoliticalArea"/>
<rdfs:subClassOf rdf:resource ="#Nation"/>
<rdfs:comment>IndependentState is a subclass of
GeopoliticalArea, representing the classification 'Independent State'
used by the CIA World Fact Book.  Cf.
DependencyOrSpecialSovereigntyArea.</rdfs:comment>
</owl:Class>

<owl:Class rdf:ID= "GeopoliticalArea">
<rdfs:subClassOf rdf:resource ="#GeographicArea"/>
<rdfs:subClassOf rdf:resource ="#Agent"/>
<rdfs:comment>Any GeographicArea which is associated
with some sort of political structure.  This class includes Lands,
Cities, districts of cities, counties, etc.  Note that the identity
of a GeopoliticalArea may remain constant after a change in borders.</rdfs:comment>
</owl:Class>

<owl:Class rdf:ID= "GeographicArea">
<rdfs:subClassOf rdf:resource ="#Region"/>
<rdfs:comment>A geographic location, generally having
definite boundaries.  Note that this differs from its immediate superclass
Region in that a GeographicArea is a three-dimensional Region of the
earth.  Accordingly, all astronomical objects other than earth and all
one-dimensional and two-dimensional Regions are not classed under
GeographicArea.</rdfs:comment>
</owl:Class>

<owl:Class rdf:ID= "Region">
<rdfs:subClassOf rdf:resource ="#Object"/>
<rdfs:comment>A topographic location.  Regions encompass
surfaces of Objects, imaginary places, and GeographicAreas.  Note
that a Region is the only kind of Object which can be located at
itself.  Note too that Region is not a subclass of SelfConnectedObject,
because some Regions, e.g. archipelagos, have parts which are not
connected with one another.</rdfs:comment>
</owl:Class>

<owl:Class rdf:ID= "Nation">
<rdfs:subClassOf rdf:resource ="#GeopoliticalArea"/>
<rdfs:subClassOf rdf:resource ="#LandArea"/>
<rdfs:comment>The broadest GeopoliticalArea, i.e. Nations are
GeopoliticalAreas that are not part of any other overarching and
comprehensive governance structure (excepting commonwealths and other sorts
of loose international organizations).</rdfs:comment>
</owl:Class>

<owl:Class rdf:ID= "LandArea">
<rdfs:subClassOf rdf:resource ="#GeographicArea"/>
<rdfs:comment>An area which is predominantly solid ground,
e.g. a Nation, a mountain, a desert, etc.  Note that a LandArea may
contain some relatively small WaterAreas.  For example, Australia is
a LandArea even though it contains various rivers and lakes.</rdfs:comment>
</owl:Class>


<owl:Class rdf:ID= "Petroleum">
<rdfs:subClassOf rdf:resource ="#PetroleumProduct"/>
<rdfs:comment>Also known as crude oil.  It can be converted into
RefinedPetroleumProducts.</rdfs:comment>
</owl:Class>

<owl:Class rdf:ID= "PetroleumProduct">
<rdfs:subClassOf rdf:resource ="#OrganicCompound"/>
<rdfs:comment>PetroleumProduct is a broad class that
includes both crude oil (Petroleum) and RefinedPetroleumProducts.</rdfs:comment>
</owl:Class>


<owl:Class rdf:ID= "OrganicCompound">
<rdfs:subClassOf rdf:resource ="#CompoundSubstance"/>
<rdfs:comment>Any CompoundSubstance that has a Carbon
base.</rdfs:comment>
</owl:Class>

<owl:Class rdf:ID= "RefinedPetroleumProduct">
<rdfs:subClassOf rdf:resource ="#PetroleumProduct"/>
<rdfs:comment>RefinedPetroleumProduct is the
subclass of PetroleumProducts that are refined from Petroleum (crude oil).</rdfs:comment>
</owl:Class>

<owl:Class rdf:ID= "Livestock">
<rdfs:subClassOf rdf:resource ="#AnimalAgriculturalProduct"/>
<rdfs:comment>Livestock is the class of live animals
raised as AgriculturalProducts.</rdfs:comment>
</owl:Class>

<owl:Class rdf:ID= "AnimalAgriculturalProduct">
<rdfs:subClassOf rdf:resource ="#AgriculturalProduct"/>
<rdfs:comment>AnimalAgriculturalProduct is the class of AgriculturalProducts
that are animal in nature, including meat, fish, dairy products,
hides, furs, animal fats and oils, etc.</rdfs:comment>
</owl:Class>

<owl:Class rdf:ID= "Beverage">
<rdfs:subClassOf rdf:resource ="#Food"/>
<rdfs:comment>Any Food that is ingested by Drinking.
Note that this class is disjoint with the other subclasses of Food,
i.e. Meat and FruitOrVegetable.</rdfs:comment>
</owl:Class>


<owl:Class rdf:ID= "Food">
<rdfs:subClassOf rdf:resource ="#SelfConnectedObject"/>
<rdfs:comment>Any SelfConnectedObject containing Nutrients,
such as carbohydrates, proteins, and fats, that can be ingested by a
living Animal and metabolized into energy and body tissue.</rdfs:comment>
</owl:Class>

<owl:Class rdf:ID= "GroceryProduce">
<rdfs:subClassOf rdf:resource ="#PlantAgriculturalProduct"/>
<rdfs:subClassOf rdf:resource ="#FruitOrVegetable"/>
</owl:Class>

<owl:Class rdf:ID= "PlantAgriculturalProduct">
<rdfs:subClassOf rdf:resource ="#AgriculturalProduct"/>
<rdfs:comment>PlantAgriculturalProduct
is the class of AgriculturalProducts that are vegetable in nature,
in the widest sense, e.g., fruits, grains, green vegetables, cotton,
linen, flowers, wine grapes, hops.</rdfs:comment>
</owl:Class>

<owl:Class rdf:ID= "TropicalFruit">
<rdfs:subClassOf rdf:resource ="#Fruit"/>
<rdfs:subClassOf rdf:resource ="#GroceryProduce"/>
</owl:Class>

<owl:Class rdf:ID= "Fruit">
<rdfs:subClassOf rdf:resource ="#FruitOrVegetable"/>
</owl:Class>

<owl:Class rdf:ID= "ChickenMeat">
<rdfs:subClassOf rdf:resource ="#Meat"/>
<rdfs:comment>Meat that was originally part of a Chicken.</rdfs:comment>
</owl:Class>


<owl:Class rdf:ID= "Meat">
<rdfs:subClassOf rdf:resource ="#Food"/>
<rdfs:comment>Any Food which was originally part of an
Animal and is not ingested by drinking, including eggs and animal
blood that is eaten as food.  Note that this class covers both raw
meat and meat that has been prepared in some way, e.g. by cooking.
Note too that preparations involving Meat and FruitOrVegetable
are classed directly under Food.</rdfs:comment>
</owl:Class>


<owl:Class rdf:ID= "CitrusFruit">
<rdfs:subClassOf rdf:resource ="#Fruit"/>
<rdfs:subClassOf rdf:resource ="#GroceryProduce"/>
</owl:Class>

<owl:Class rdf:ID= "BeverageProduct">
<rdfs:subClassOf rdf:resource ="#Product"/>
<rdfs:comment>BeverageProduct is the class of products
that are Beverages, packaged or unpackaged.</rdfs:comment>
</owl:Class>


<owl:Class rdf:ID= "Crayfish">
<rdfs:subClassOf rdf:resource ="#Shellfish"/>
</owl:Class>

<owl:Class rdf:ID= "Shellfish">
<rdfs:subClassOf rdf:resource ="#Seafood"/>
</owl:Class>

<owl:Class rdf:ID= "Shrimp">
<rdfs:subClassOf rdf:resource ="#Shellfish"/>
</owl:Class>

<owl:Class rdf:ID= "Seafood">
<rdfs:subClassOf rdf:resource ="#Meat"/>
</owl:Class>

<owl:Class rdf:ID= "FoodFish">
<rdfs:subClassOf rdf:resource ="#Seafood"/>
</owl:Class>

<owl:Class rdf:ID= "ControlledSubstance">
<rdfs:subClassOf rdf:resource ="#BiologicallyActiveSubstance"/>
<rdfs:comment>ControlledSubstance is
the subclass of BiologicallyActiveSubstances whose distribution
and use is controlled by government regulation.</rdfs:comment>
</owl:Class>

<owl:Class rdf:ID= "BiologicallyActiveSubstance">
<rdfs:subClassOf rdf:resource ="#Substance"/>
<rdfs:comment>A Substance that is
capable of inducing a change in the structure or functioning of an
Organism.  This Class includes Substances used in the treatment,
diagnosis, prevention or analysis of normal and abnormal body function.
This Class also includes Substances that occur naturally in the body
and are administered therapeutically.  Finally, BiologicallyActiveSubstance
includes Nutrients, most drugs of abuse, and agents that require special
handling because of their toxicity.</rdfs:comment>
</owl:Class>

<owl:Class rdf:ID= "LambMeat">
<rdfs:subClassOf rdf:resource ="#MeatOfLandAnimal"/>
</owl:Class>

<owl:Class rdf:ID= "MeatOfLandAnimal">
<rdfs:subClassOf rdf:resource ="#Meat"/>
</owl:Class>

<owl:Class rdf:ID= "HoofedMammal">
<rdfs:subClassOf rdf:resource ="#Mammal"/>
<rdfs:comment>The Class of quadruped Mammals with hooves.
Includes horses, cows, sheep, pigs, antelope, etc.</rdfs:comment>
</owl:Class>

<owl:Class rdf:ID= "Mammal">
<rdfs:subClassOf rdf:resource ="#WarmBloodedVertebrate"/>
<rdfs:comment>A Vertebrate having a constant body temperature
and characterized by the presence of hair, mammary glands, and sweat
glands.</rdfs:comment>
</owl:Class>

<owl:Class rdf:ID= "WarmBloodedVertebrate">
<rdfs:subClassOf rdf:resource ="#Vertebrate"/>
<disjoint rdf:resource = "#ColdBloodedVertebrate" />
<rdfs:comment>Vertebrates whose body temperature
is internally regulated.</rdfs:comment>
</owl:Class>

<owl:Class rdf:ID= "ColdBloodedVertebrate">
<rdfs:subClassOf rdf:resource ="#Vertebrate"/>
<rdfs:comment>Vertebrates whose body temperature
is not internally regulated.</rdfs:comment>
</owl:Class>

<owl:Class rdf:ID= "Vertebrate">
<rdfs:subClassOf rdf:resource ="#Animal"/>
<rdfs:comment>An Animal which has a spinal column.</rdfs:comment>
</owl:Class>

<owl:Class rdf:ID= "Animal">
<rdfs:subClassOf rdf:resource ="#Organism"/>
<rdfs:comment>An Organism with eukaryotic Cells, and lacking
stiff cell walls, plastids, and photosynthetic pigments.</rdfs:comment>
</owl:Class>

<owl:Class rdf:ID= "Milk">
<rdfs:subClassOf rdf:resource ="#LiquidBodySubstance"/>
<rdfs:subClassOf rdf:resource ="#Beverage"/>
<rdfs:comment>A nutritious BodySubstance produced by Mammals.</rdfs:comment>
</owl:Class>

<owl:Class rdf:ID= "LiquidBodySubstance">
<rdfs:subClassOf rdf:resource ="#BodySubstance"/>
<rdfs:comment>Any BodySubstance which is Liquid
under normal circumstances.</rdfs:comment>
</owl:Class>


<owl:Class rdf:ID= "BodySubstance">
<rdfs:subClassOf rdf:resource ="#Mixture"/>
<rdfs:comment>Extracellular material and mixtures of
cells and extracellular material that are produced, excreted or accreted
by an Organism.  Included here are Substances such as saliva, dental
enamel, sweat, and gastric acid.</rdfs:comment>
</owl:Class>

<owl:Class rdf:ID= "Mixture">
<rdfs:subClassOf rdf:resource ="#Substance"/>
<rdfs:comment>A Mixture is two or more PureSubstances,
combined in varying proportions - each retaining its own specific properties.
The components of a Mixture can be separated by physical means, i.e. without
the making and breaking of chemical bonds. Examples: Air, table salt thoroughly
dissolved in water, milk, wood, and concrete. </rdfs:comment>
</owl:Class>

<owl:Class rdf:ID= "Salmon">
<rdfs:subClassOf rdf:resource ="#FoodFish"/>
</owl:Class>

<owl:Class rdf:ID= "TurkeyMeat">
<rdfs:subClassOf rdf:resource ="#MeatOfLandAnimal"/>
</owl:Class>

<owl:Class rdf:ID= "WaterBuffaloMeat">
<rdfs:subClassOf rdf:resource ="#MeatOfLandAnimal"/>
</owl:Class>

<owl:Class rdf:ID= "Wine">
<rdfs:subClassOf rdf:resource ="#AlcoholicBeverage"/>
<rdfs:comment>An AlcoholicBeverage that is prepared by fermenting
the juice of grapes.</rdfs:comment>
</owl:Class>


<owl:Class rdf:ID= "AlcoholicBeverage">
<rdfs:subClassOf rdf:resource ="#Beverage"/>
<rdfs:subClassOf rdf:resource ="#Depressant"/>
<rdfs:comment>Any Beverage that contains Alcohol.</rdfs:comment>
</owl:Class>

<owl:Class rdf:ID= "Depressant">
<rdfs:subClassOf rdf:resource ="#BiologicallyActiveSubstance"/>
<rdfs:comment>Any BiologicallyActiveSubstance which has
the effect of depressing the central nervous system, i.e. decreasing
function or activity in the Brain or SpinalCord.</rdfs:comment>
</owl:Class>

<owl:Class rdf:ID= "Pork">
<rdfs:subClassOf rdf:resource ="#MeatOfLandAnimal"/>
</owl:Class>

<owl:Class rdf:ID= "Beef">
<rdfs:subClassOf rdf:resource ="#Meat"/>
<rdfs:comment>Meat that was originally part of a Cow.</rdfs:comment>
</owl:Class>

<owl:Class rdf:ID= "Cheese">
<rdfs:subClassOf rdf:resource ="#DairyProduct"/>
</owl:Class>

<owl:Class rdf:ID= "DairyProduct">
<rdfs:subClassOf rdf:resource ="#AnimalAgriculturalProduct"/>
</owl:Class>


<owl:Class rdf:ID= "ChemicalProduct">
<rdfs:subClassOf rdf:resource ="#ManufacturedProduct"/>
<rdfs:subClassOf rdf:resource ="#CompoundSubstance"/>
<rdfs:comment>ChemicalProduct is the subclass
of Product comprising all chemical compounds that are end products
or industrial products used in the manufacture of end products.</rdfs:comment>
</owl:Class>

</rdf:RDF>