<rdf:RDF
xmlns:rdf ="http://www.w3.org/1999/02/22-rdf-syntax-ns#"
xmlns:rdfs="http://www.w3.org/2000/01/rdf-schema#"
xmlns:owl="http://www.w3.org/2002/07/owl#"
xmlns     ="http://127.0.0.1:8000/ontology/SUMO.owl#"
xml:base     ="http://127.0.0.1:8000/ontology/SUMO.owl"
>

<!--  copyright 2003 (c) Teknowledge 						-->
<!--  This program is free software; you can redistribute it and/or		-->
<!--  modify it under the terms of the GNU Lesser General Public		-->
<!--  License as published by the Free Software Foundation; either		-->
<!--  version 2.1 of the License, or (at your option) any later version.	-->
<!--										-->
<!--  This program is distributed in the hope that it will be useful,		-->
<!--  but WITHOUT ANY WARRANTY; without even the implied warranty of		-->
<!--  MERCHANTABILITY or FITNESS FOR A PARTICULAR PURPOSE.  See the GNU		-->
<!--  Lesser General Public License for more details.				-->
<!--										-->
<!--  You should have received a copy of the GNU Lesser General Public		-->
<!--  License along with this program; if not, write to the Free Software	-->
<!--  Foundation, Inc., 59 Temple Place, Suite 330, Boston, MA 02111-1307 USA	-->

<owl:Class rdf:ID= "AbnormalAnatomicalStructure">
<rdfs:subClassOf rdf:resource ="#AnatomicalStructure"/>
<rdfs:comment>Any AnatomicalStructure which
is not normally found in the Organism of which it is a part, i.e. it is
the result of a PathologicProcess.  This class covers tumors, birth marks,
goiters, etc.</rdfs:comment>
</owl:Class>

<owl:Class rdf:ID= "InternalAttribute"/>
<owl:Class rdf:ID= "Abstract"/>

<owl:Class rdf:ID= "Adjective">
<rdfs:subClassOf rdf:resource ="#Word"/>
<rdfs:comment>One of the parts of speech.  The Class of
Words that conventionally denote Attributes of Objects.</rdfs:comment>
</owl:Class>

<owl:Class rdf:ID= "Adverb">
<rdfs:subClassOf rdf:resource ="#Word"/>
<rdfs:comment>One of the parts of speech.  The Class of Words
that conventionally denote Attributes of Processes.</rdfs:comment>
</owl:Class>

<owl:Class rdf:ID= "AgeGroup">
<rdfs:subClassOf rdf:resource ="#GroupOfPeople"/>
<rdfs:comment>A GroupOfPeople whose members all have the
same age.</rdfs:comment>
</owl:Class>

<owl:Class rdf:ID= "Agent">
<rdfs:subClassOf rdf:resource ="#Object"/>
<rdfs:comment>Something or someone that can act on its own and
produce changes in the world.</rdfs:comment>
</owl:Class>

<owl:Class rdf:ID= "Air">
<rdfs:subClassOf rdf:resource ="#GasMixture"/>
<rdfs:comment>Air is the gaseous stuff that makes up the
atmosphere surrounding Earth.</rdfs:comment>
</owl:Class>

<owl:Class rdf:ID= "AlethicAttribute">
<rdfs:subClassOf rdf:resource ="#ObjectiveNorm"/>
<rdfs:comment>A Class containing all of the Attributes
relating to the notions of possibility and necessity.</rdfs:comment>
</owl:Class>

<owl:Class rdf:ID= "Alga">
<rdfs:subClassOf rdf:resource ="#NonFloweringPlant"/>
<rdfs:comment>A chiefly aquatic plant that contains chlorophyll,
but does not form embryos during development and lacks vascular tissue.</rdfs:comment>
</owl:Class>

<owl:Class rdf:ID= "Ambulating">
<rdfs:subClassOf rdf:resource ="#BodyMotion"/>
<rdfs:subClassOf rdf:resource ="#Translocation"/>
<rdfs:comment>Any BodyMotion which is accomplished by
means of the legs of an Animal for the purpose of moving from one
point to another.</rdfs:comment>
</owl:Class>

<owl:Class rdf:ID= "Amphibian">
<rdfs:subClassOf rdf:resource ="#ColdBloodedVertebrate"/>
<rdfs:comment>A cold-blooded, smooth-skinned Vertebrate
which characteristically hatches as an aquatic larva, breathing by
gills.  When mature, the Amphibian breathes with Lungs.</rdfs:comment>
</owl:Class>

<owl:Class rdf:ID= "AnatomicalStructure">
<rdfs:subClassOf rdf:resource ="#OrganicObject"/>
<rdfs:comment>A normal or pathological part
of the anatomy or structural organization of an Organism.  This
class covers BodyParts, as well as structures that are given off
by Organisms, e.g. ReproductiveBodies.</rdfs:comment>
</owl:Class>

<owl:Class rdf:ID= "AngleMeasure">
<rdfs:subClassOf rdf:resource ="#ConstantQuantity"/>
<rdfs:comment>The value of an angle in a plane or in a
solid.</rdfs:comment>
</owl:Class>

<owl:Class rdf:ID= "AngularDegree">
<rdfs:subClassOf rdf:resource ="#PlaneAngleMeasure"/>
<rdf:type rdf:resource = "#UnitOfMeasure"/>
<rdfs:comment>A plane angle measure.</rdfs:comment>
</owl:Class>



<owl:Class rdf:ID= "Animal">
<rdfs:subClassOf rdf:resource ="#Organism"/>
<rdfs:comment>An Organism with eukaryotic Cells, and lacking
stiff cell walls, plastids, and photosynthetic pigments.</rdfs:comment>
</owl:Class>

<owl:Class rdf:ID= "AnimalAnatomicalStructure">
<rdfs:subClassOf rdf:resource ="#AnatomicalStructure"/>
<rdfs:comment>AnatomicalStructures that
are possessed exclusively by Animals.</rdfs:comment>
</owl:Class>

<owl:Class rdf:ID= "AnimalLanguage">
<rdfs:subClassOf rdf:resource ="#Language"/>
<rdfs:comment>The subclass of Languages used by
Animals other than Humans.</rdfs:comment>
</owl:Class>

<owl:Class rdf:ID= "AnimalSubstance">
<rdfs:subClassOf rdf:resource ="#BodySubstance"/>
<rdfs:comment>BodySubstances that are produced
exclusively by Animals.</rdfs:comment>
</owl:Class>

<owl:Class rdf:ID= "AntisymmetricRelation">
<rdfs:subClassOf rdf:resource ="#BinaryRelation"/>
<rdfs:comment>BinaryRelation ?REL is an
AntisymmetricRelation if for distinct ?INST1 and ?INST2, (?REL ?INST1
?INST2) implies not (?REL ?INST2 ?INST1).  In other words, for all ?INST1
and ?INST2, (?REL ?INST1 ?INST2) and (?REL ?INST2 ?INST1) imply that ?INST1
and ?INST2 are identical.  Note that it is possible for an
AntisymmetricRelation to be a ReflexiveRelation.</rdfs:comment>
</owl:Class>

<owl:Class rdf:ID= "Ape">
<rdfs:subClassOf rdf:resource ="#Primate"/>
<rdfs:comment>Various Primates with no tails or only short
tails.</rdfs:comment>
</owl:Class>

<owl:Class rdf:ID= "April">
<rdfs:subClassOf rdf:resource ="#Month"/>
<rdfs:comment>The Class of all Months which are April.</rdfs:comment>
</owl:Class>

<owl:Class rdf:ID= "AquaticMammal">
<rdfs:subClassOf rdf:resource ="#Mammal"/>
<rdfs:comment>The Class of Mammals that dwell chiefly
in the water.  Includes whales, dolphins, manatees, seals, and walruses.</rdfs:comment>
</owl:Class>

<owl:Class rdf:ID= "Arachnid">
<rdfs:subClassOf rdf:resource ="#Arthropod"/>
<rdfs:comment>A Class of Arthropods that includes
ticks and spiders.</rdfs:comment>
</owl:Class>

<owl:Class rdf:ID= "AreaMeasure">
<rdfs:subClassOf rdf:resource ="#ConstantQuantity"/>
<rdfs:comment>Measures of the amount of space in two
dimensions.</rdfs:comment>
</owl:Class>

<owl:Class rdf:ID= "Argument">
<rdfs:subClassOf rdf:resource ="#Proposition"/>
<rdfs:comment>Any proposition which has the form of a deductive
or inductive argument, i.e. a set of premises which, it is claimed, imply
a conclusion.</rdfs:comment>
</owl:Class>

<owl:Class rdf:ID= "ArtWork">
<rdfs:subClassOf rdf:resource ="#Artifact"/>
<rdfs:comment>Artifacts that are created primarily for
aesthetic appreciation.  Note that this Class does not include
most examples of architecture, which belong under StationaryArtifact.</rdfs:comment>
</owl:Class>

<owl:Class rdf:ID= "Arthropod">
<rdfs:subClassOf rdf:resource ="#Invertebrate"/>
<rdfs:comment>A Class of Invertebrate that includes
Arachnids and Insects.</rdfs:comment>
</owl:Class>

<owl:Class rdf:ID= "Article">
<rdfs:subClassOf rdf:resource ="#Text"/>
<disjoint rdf:resource = "#Book" />
<rdfs:comment>A relatively short Text that either is unbound or is
bound with other Articles in a Book.</rdfs:comment>
</owl:Class>

<owl:Class rdf:ID= "Artifact">
<rdfs:subClassOf rdf:resource ="#CorpuscularObject"/>
<rdfs:comment>A CorpuscularObject that is the product of a
Making.</rdfs:comment>
</owl:Class>

<owl:Class rdf:ID= "ArtificialLanguage">
<rdfs:subClassOf rdf:resource ="#Language"/>
<rdfs:comment>The subclass of Languages that are
designed by Humans.</rdfs:comment>
</owl:Class>

<owl:Class rdf:ID= "AsexualReproduction">
<rdfs:subClassOf rdf:resource ="#Replication"/>
<rdfs:comment>Asexual Processes of biological
reproduction.</rdfs:comment>
</owl:Class>

<owl:Class rdf:ID= "AssociativeFunction">
<rdfs:subClassOf rdf:resource ="#BinaryFunction"/>
<rdfs:comment>A BinaryFunction is associative if
bracketing has no effect on the value returned by the Function.  More
precisely, a Function ?FUNCTION is associative just in case
(?FUNCTION ?INST1 (?FUNCTION ?INST2 ?INST3)) is equal to
(?FUNCTION (?FUNCTION ?INST1 ?INST2) ?INST3), for all ?INST1, ?INST2,
and ?INST3.</rdfs:comment>
</owl:Class>

<owl:Class rdf:ID= "AstronomicalBody">
<rdfs:subClassOf rdf:resource ="#Region"/>
<disjoint rdf:resource = "#GeographicArea" />
<rdfs:comment>The Class of all astronomical
objects of significant size.  It includes SelfConnectedObjects
like planets, stars, and asteroids, as well as Collections like
nebulae, galaxies, and constellations.  Note that the planet Earth
is an AstronomicalBody, but every Region of Earth is a
GeographicArea.</rdfs:comment>
</owl:Class>

<owl:Class rdf:ID= "AsymmetricRelation">
<rdfs:subClassOf rdf:resource ="#IrreflexiveRelation"/>
<rdfs:subClassOf rdf:resource ="#AntisymmetricRelation"/>
<rdfs:comment>A BinaryRelation is asymmetric only
if it is both an AntisymmetricRelation and an IrreflexiveRelation.</rdfs:comment>
</owl:Class>

<owl:Class rdf:ID= "Atom">
<rdfs:subClassOf rdf:resource ="#ElementalSubstance"/>
<rdfs:comment>An extremely small unit of matter that retains its
identity in Chemical reactions.  It consists of an AtomicNucleus and
Electrons surrounding the AtomicNucleus.</rdfs:comment>
</owl:Class>

<owl:Class rdf:ID= "AtomicNucleus">
<rdfs:subClassOf rdf:resource ="#SubatomicParticle"/>
<rdfs:comment>The core of the Atom.  It is composed of
Protons and Neutrons.</rdfs:comment>
</owl:Class>

<owl:Class rdf:ID= "Attaching">
<rdfs:subClassOf rdf:resource ="#DualObjectProcess"/>
<disjoint rdf:resource = "#Detaching" />
<relatedInternalConcept rdf:resource = "#Putting" />
<rdfs:comment>A Process where one Object becomes attached
to another Object.  Note that this differs from Putting in that two
things which are attached may already be in the same location.  Note that
Combining is different from Attaching in that the former applies to
Substances, while the latter applies to CorpuscularObjects.  Note too
that Attaching is different from Putting in that one or both of the
two things which are attached may or may not be moved from the location
where they were combined.</rdfs:comment>
</owl:Class>

<owl:Class rdf:ID= "AttachingDevice">
<rdfs:subClassOf rdf:resource ="#Device"/>
<rdfs:comment>A Device whose purpose is to attach one thing
to something else, e.g. nails, screws, buttons, etc.</rdfs:comment>
</owl:Class>

<owl:Class rdf:ID= "Attack">
<rdfs:subClassOf rdf:resource ="#Maneuver"/>
<rdfs:comment>A Maneuver in a ViolentContest where the
agent attempts to inflict damage on the patient.</rdfs:comment>
</owl:Class>



<owl:Class rdf:ID= "August">
<rdfs:subClassOf rdf:resource ="#Month"/>
<rdfs:comment>The Class of all Months which are August.</rdfs:comment>
</owl:Class>

<owl:Class rdf:ID= "AutonomicProcess">
<rdfs:subClassOf rdf:resource ="#PhysiologicProcess"/>
<disjoint rdf:resource = "#IntentionalProcess" />
<rdfs:comment>The class of PhysiologicProcesses of
which there is not conscious awareness and control.</rdfs:comment>
</owl:Class>

<owl:Class rdf:ID= "Bacterium">
<rdfs:subClassOf rdf:resource ="#Microorganism"/>
<rdfs:comment>A small, typically one-celled, prokaryotic
Microorganism.</rdfs:comment>
</owl:Class>

<owl:Class rdf:ID= "Battle">
<rdfs:subClassOf rdf:resource ="#ViolentContest"/>
<rdfs:comment>A ViolentContest between two or more military
units within the context of a war.  Note that this does not cover the
metaphorical sense of 'battle', which simply means a struggle of some
sort.  This sense should be represented with the more general concept of
Contest.</rdfs:comment>
</owl:Class>

<owl:Class rdf:ID= "BeliefGroup">
<rdfs:subClassOf rdf:resource ="#GroupOfPeople"/>
<rdfs:comment>A GroupOfPeople whose members share a belief
or set of beliefs.</rdfs:comment>
</owl:Class>

<owl:Class rdf:ID= "Betting">
<rdfs:subClassOf rdf:resource ="#FinancialTransaction"/>
<rdfs:comment>A FinancialTransaction where an instance of
CurrencyMeasure is exchanged for the possibility of winning a larger
instance of CurrencyMeasure within the context of some sort of
Game.</rdfs:comment>
</owl:Class>

<owl:Class rdf:ID= "Beverage">
<rdfs:subClassOf rdf:resource ="#Food"/>
<rdfs:comment>Any Food that is ingested by Drinking.
Note that this class is disjoint with the other subclasses of Food,
i.e. Meat and FruitOrVegetable.</rdfs:comment>
</owl:Class>

<owl:Class rdf:ID= "BinaryFunction">
<rdfs:subClassOf rdf:resource ="#Function"/>
<rdfs:subClassOf rdf:resource ="#TernaryRelation"/>
<rdf:type rdf:resource = "#InheritableRelation"/>
<rdfs:comment>The Class of Functions that require
two arguments.</rdfs:comment>
</owl:Class>

<owl:Class rdf:ID= "BinaryNumber">
<rdfs:subClassOf rdf:resource ="#RealNumber"/>
<rdfs:comment>Elements from the number system with base 2.
Every BinaryNumber is expressed as a sequence of the digits 1 and 0.</rdfs:comment>
</owl:Class>

<owl:Class rdf:ID= "BinaryPredicate">
<rdfs:subClassOf rdf:resource ="#Predicate"/>
<rdfs:subClassOf rdf:resource ="#BinaryRelation"/>
<rdf:type rdf:resource = "#InheritableRelation"/>
<rdfs:comment>A Predicate relating two items - its
valence is two.</rdfs:comment>
</owl:Class>

<owl:Class rdf:ID= "BinaryRelation">
<rdfs:subClassOf rdf:resource ="#Relation"/>
<rdf:type rdf:resource = "#InheritableRelation"/>
<rdfs:comment>BinaryRelations are relations that are
true only of pairs of things.  BinaryRelations are represented as slots
in frame systems.</rdfs:comment>
</owl:Class>



<owl:Class rdf:ID= "BiologicalProcess">
<rdfs:subClassOf rdf:resource ="#InternalChange"/>
<rdfs:comment>A Process embodied in an Organism.</rdfs:comment>
</owl:Class>

<owl:Class rdf:ID= "BiologicallyActiveSubstance">
<rdfs:subClassOf rdf:resource ="#Substance"/>
<rdfs:comment>A Substance that is
capable of inducing a change in the structure or functioning of an
Organism.  This Class includes Substances used in the treatment,
diagnosis, prevention or analysis of normal and abnormal body function.
This Class also includes Substances that occur naturally in the body
and are administered therapeutically.  Finally, BiologicallyActiveSubstance
includes Nutrients, most drugs of abuse, and agents that require special
handling because of their toxicity.</rdfs:comment>
</owl:Class>

<owl:Class rdf:ID= "Bird">
<rdfs:subClassOf rdf:resource ="#WarmBloodedVertebrate"/>
<disjoint rdf:resource = "#Mammal" />
<rdfs:comment>A Vertebrate having a constant body temperature
and characterized by the presence of feathers.</rdfs:comment>
</owl:Class>

<owl:Class rdf:ID= "Birth">
<rdfs:subClassOf rdf:resource ="#OrganismProcess"/>
<rdfs:comment>The Process of being born.</rdfs:comment>
</owl:Class>

<owl:Class rdf:ID= "Bit">
<rdfs:subClassOf rdf:resource ="#InformationMeasure"/>
<rdf:type rdf:resource = "#UnitOfMeasure"/>
<rdfs:comment>One Bit of information.  A one or a zero.</rdfs:comment>
</owl:Class>

<owl:Class rdf:ID= "Blood">
<rdfs:subClassOf rdf:resource ="#BodySubstance"/>
<rdfs:comment>A fluid present in Animals that transports
Nutrients to and waste products away from various BodyParts.</rdfs:comment>
</owl:Class>

<owl:Class rdf:ID= "BodyCavity">
<rdfs:subClassOf rdf:resource ="#BodyPart"/>
<rdfs:comment>Any BodyPart which contains an unfilled space,
e.g. BodyVessels, the atria and ventricles of the heart, the lungs, etc.</rdfs:comment>
</owl:Class>

<owl:Class rdf:ID= "BodyCovering">
<rdfs:subClassOf rdf:resource ="#BodyPart"/>
<rdfs:comment>Any BodyPart which is a covering of another
BodyPart or of an entire Organism.  This would include the rinds of
FruitOrVegetables and the skins of Animals.</rdfs:comment>
</owl:Class>

<owl:Class rdf:ID= "BodyJunction">
<rdfs:subClassOf rdf:resource ="#BodyPart"/>
<rdfs:comment>The place where two BodyParts
meet or connect.</rdfs:comment>
</owl:Class>

<owl:Class rdf:ID= "BodyMotion">
<rdfs:subClassOf rdf:resource ="#Motion"/>
<rdfs:comment>Any Motion where the agent is an Organism
and the patient is a BodyPart.</rdfs:comment>
</owl:Class>

<owl:Class rdf:ID= "BodyPart">
<rdfs:subClassOf rdf:resource ="#AnatomicalStructure"/>
<rdfs:comment>A collection of Cells and Tissues which
are localized to a specific area of an Organism and which are not
pathological. The instances of this Class range from gross structures
to small components of complex Organs.</rdfs:comment>
</owl:Class>


<owl:Class rdf:ID= "BodySubstance">
<rdfs:subClassOf rdf:resource ="#Mixture"/>
<rdfs:comment>Extracellular material and mixtures of
cells and extracellular material that are produced, excreted or accreted
by an Organism.  Included here are Substances such as saliva, dental
enamel, sweat, and gastric acid.</rdfs:comment>
</owl:Class>

<owl:Class rdf:ID= "BodyVessel">
<rdfs:subClassOf rdf:resource ="#BodyCavity"/>
<rdfs:comment>Any tube-like structure which occurs naturally in
an Organism and through which a BodySubstance can circulate.</rdfs:comment>
</owl:Class>

<owl:Class rdf:ID= "Boiling">
<rdfs:subClassOf rdf:resource ="#StateChange"/>
<rdfs:comment>The Class of Processes where an Object is
heated and converted from a Liquid to a Gas.</rdfs:comment>
</owl:Class>

<owl:Class rdf:ID= "Bone">
<rdfs:subClassOf rdf:resource ="#Tissue"/>
<rdfs:subClassOf rdf:resource ="#AnimalSubstance"/>
<rdfs:comment>Rigid Tissue composed largely of calcium that makes up
the skeleton of Vertebrates.  Note that this Class also includes teeth.</rdfs:comment>
</owl:Class>

<owl:Class rdf:ID= "Book">
<rdfs:subClassOf rdf:resource ="#Text"/>
<rdfs:comment>A Text that has pages and is bound.</rdfs:comment>
</owl:Class>

<owl:Class rdf:ID= "Borrowing">
<rdfs:subClassOf rdf:resource ="#Getting"/>
<rdfs:comment>The subclass of Getting Processes where
the agent gets something for a limited period of time with the expectation
that it will be returned later (perhaps with interest).</rdfs:comment>
</owl:Class>

<owl:Class rdf:ID= "Breathing">
<rdfs:subClassOf rdf:resource ="#OrganismProcess"/>
<rdfs:subClassOf rdf:resource ="#AutonomicProcess"/>
<rdfs:comment>The Process of respiration, by which oxygen
is made available to an Animal.  This covers processes of inhalation,
exhalation, and alternations between the two.</rdfs:comment>
</owl:Class>

<owl:Class rdf:ID= "BritishThermalUnit">
<rdfs:subClassOf rdf:resource ="#FunctionQuantity"/>
<rdf:type rdf:resource = "#UnitOfMeasure"/>
<rdfs:comment>An energy measure.</rdfs:comment>
</owl:Class>

<owl:Class rdf:ID= "Building">
<rdfs:subClassOf rdf:resource ="#StationaryArtifact"/>
<rdfs:comment>The Class of StationaryArtifacts which are
intended to house Humans and their activities.</rdfs:comment>
</owl:Class>

<owl:Class rdf:ID= "Buying">
<rdfs:subClassOf rdf:resource ="#FinancialTransaction"/>
<relatedInternalConcept rdf:resource = "#Selling" />
<rdfs:comment>A FinancialTransaction in which an instance of
CurrencyMeasure is exchanged for an instance of Physical.</rdfs:comment>
</owl:Class>

<owl:Class rdf:ID= "Byte">
<rdfs:subClassOf rdf:resource ="#InformationMeasure"/>
<rdf:type rdf:resource = "#UnitOfMeasure"/>
<rdfs:comment>One Byte of information.  A Byte is eight
Bits.</rdfs:comment>
</owl:Class>

<owl:Class rdf:ID= "Calculating">
<rdfs:subClassOf rdf:resource ="#IntentionalPsychologicalProcess"/>
<rdfs:comment>IntentionalPsychologicalProcesses which involve
the consideration and/or manipulation of instances of Quantity.</rdfs:comment>
</owl:Class>

<owl:Class rdf:ID= "Calorie">
<rdfs:subClassOf rdf:resource ="#FunctionQuantity"/>
<rdf:type rdf:resource = "#UnitOfMeasure"/>
<rdfs:comment>A Calorie is an energy measure.</rdfs:comment>
</owl:Class>

<owl:Class rdf:ID= "Canine">
<rdfs:subClassOf rdf:resource ="#Carnivore"/>
<disjoint rdf:resource = "#Feline" />
<rdfs:comment>The Class of Carnivores with completely
separable toes, nonretractable claws, and long muzzles.</rdfs:comment>
</owl:Class>

<owl:Class rdf:ID= "Carbohydrate">
<rdfs:subClassOf rdf:resource ="#Nutrient"/>
<rdfs:comment>An element of living cells and a source of
energy for Animals.  This class includes both simple Carbohydrates,
i.e. sugars, and complex Carbohydrates, i.e. starches.</rdfs:comment>
</owl:Class>

<owl:Class rdf:ID= "Carnivore">
<rdfs:subClassOf rdf:resource ="#Mammal"/>
<rdfs:comment>The Class of flesh-eating Mammals.  Members
of this Class typically have four or five claws on each paw.  Includes
cats, dogs, bears, racoons, and skunks.</rdfs:comment>
</owl:Class>

<owl:Class rdf:ID= "Carrying">
<rdfs:subClassOf rdf:resource ="#Transfer"/>
<rdfs:comment>Transfer from one point to another by means of
an Animal or Human.</rdfs:comment>
</owl:Class>

<owl:Class rdf:ID= "CaseRole">
<rdfs:subClassOf rdf:resource ="#BinaryPredicate"/>
<rdf:type rdf:resource = "#InheritableRelation"/>
<rdfs:subClassOf rdf:resource ="#AsymmetricRelation"/>
<rdfs:comment>The Class of Predicates relating the
spatially distinguished parts of a Process. CaseRoles include, for
example, the agent, patient or destination of an action, the flammable
substance in a burning process, or the water that falls in rain.</rdfs:comment>
</owl:Class>

<owl:Class rdf:ID= "Cell">
<rdfs:subClassOf rdf:resource ="#BodyPart"/>
<rdfs:comment>The fundamental structural and functional unit of
living Organisms.</rdfs:comment>
</owl:Class>

<owl:Class rdf:ID= "CelsiusDegree">
<rdfs:subClassOf rdf:resource ="#TemperatureMeasure"/>
<rdf:type rdf:resource = "#SystemeInternationalUnit"/>
<rdfs:comment>A TemperatureMeasure.  The freezing point
and the boiling point of water are, respectively, 0 CelsiusDegrees and 100
CelsiusDegrees.</rdfs:comment>
</owl:Class>

<owl:Class rdf:ID= "Centimeter">
<rdfs:subClassOf rdf:resource ="#LengthMeasure"/>
<rdf:type rdf:resource = "#UnitOfMeasure"/>
<rdfs:comment>Submultiple of Meter.  Symbol: cm. It is
the 100th part of a Meter</rdfs:comment>
</owl:Class>

<owl:Class rdf:ID= "Certificate">
<rdfs:subClassOf rdf:resource ="#Text"/>
<rdfs:comment>A Text that confers a right or obligation
on the holder of the Certificate.  Note that the right or obligation
need not be a legal one, as in the case of an academic diploma that grants
certain privileges in the professional world.</rdfs:comment>
</owl:Class>

<owl:Class rdf:ID= "ChangeOfPossession">
<rdfs:subClassOf rdf:resource ="#SocialInteraction"/>
<relatedInternalConcept rdf:resource = "#possesses" />
<rdfs:comment>The Class of Processes where
ownership of something is transferred from one Agent to another.</rdfs:comment>
</owl:Class>

<owl:Class rdf:ID= "Character">
<rdfs:subClassOf rdf:resource ="#SymbolicString"/>
<rdfs:comment>An element of an alphabet, a set of numerals, etc.
Note that a Character may or may not be part of a Language.  Character
is a subclass of SymbolicString, because every instance of Character is
an alphanumeric sequence consisting of a single element.</rdfs:comment>
</owl:Class>

<owl:Class rdf:ID= "ChemicalDecomposition">
<rdfs:subClassOf rdf:resource ="#ChemicalProcess"/>
<rdfs:subClassOf rdf:resource ="#Separating"/>
<rdfs:comment>The Class of ChemicalProcesses
in which a CompoundSubstance breaks down into simpler products.</rdfs:comment>
</owl:Class>

<owl:Class rdf:ID= "ChemicalProcess">
<rdfs:subClassOf rdf:resource ="#InternalChange"/>
<rdfs:comment>A ChemicalProcess occurs whenever
chemical compounds (CompoundSubstances) are formed or decomposed.
For example, reactants disappear as chemical change occurs, and products
appear as chemical change occurs.  In a chemical change a chemical
reaction takes place.  Catalysts in a ChemicalProcess may speed up the
reaction, but aren't themselves produced or consumed.  Examples: rusting of
iron and the decomposition of water, induced by an electric current, to
gaseous hydrogen and gaseous oxygen.</rdfs:comment>
</owl:Class>

<owl:Class rdf:ID= "ChemicalSynthesis">
<rdfs:subClassOf rdf:resource ="#ChemicalProcess"/>
<rdfs:subClassOf rdf:resource ="#Combining"/>
<rdfs:comment>The Class of ChemicalProcesses in
which a CompoundSubstance is formed from simpler reactants.</rdfs:comment>
</owl:Class>

<owl:Class rdf:ID= "City">
<rdfs:subClassOf rdf:resource ="#GeopoliticalArea"/>
<rdfs:subClassOf rdf:resource ="#LandArea"/>
<rdfs:comment>A LandArea of relatively small size, inhabited
by a community of people, and having some sort of political structure.
Note that this class includes both large cities and small settlements
like towns, villages, hamlets, etc.</rdfs:comment>
</owl:Class>

<owl:Class rdf:ID= "Class">
<rdfs:subClassOf rdf:resource ="#SetOrClass"/>
<rdfs:comment>Classes differ from Sets in three important respects.
First, Classes are not assumed to be extensional.  That is, distinct
Classes might well have exactly the same instances.  Second, Classes typically
have an associated `condition' that determines the instances of the Class.  So,
for example, the condition `human' determines the Class of Humans.  Note that
some Classes might satisfy their own condition (e.g., the Class of Abstract
things is Abstract) and hence be instances of themselves.  Third, the instances
of a class may occur only once within the class, i.e. a class cannot contain
duplicate instances.</rdfs:comment>
</owl:Class>

<owl:Class rdf:ID= "Classifying">
<rdfs:subClassOf rdf:resource ="#IntentionalPsychologicalProcess"/>
<rdfs:comment>The Class of IntentionalPsychologicalProcesses
which involve attaching a name or category to a thing or set of things.
Note that Classifying is distinguished from Learning by the fact
that the latter covers the acquisition by a CognitiveAgent of any
Proposition, while the former involves the assignment of a label
or category.</rdfs:comment>
</owl:Class>

<owl:Class rdf:ID= "ClosedTwoDimensionalFigure">
<rdfs:subClassOf rdf:resource ="#TwoDimensionalFigure"/>
<rdfs:comment>Any TwoDimensionalFigure which
has a well defined interior and exterior.</rdfs:comment>
</owl:Class>

<owl:Class rdf:ID= "Clothing">
<rdfs:subClassOf rdf:resource ="#Artifact"/>
<disjoint rdf:resource = "#StationaryArtifact" />
<rdfs:comment>Artifact made out of fabrics and possibly other
materials that are used to cover the bodies of Humans.</rdfs:comment>
</owl:Class>

<owl:Class rdf:ID= "Cloud">
<rdfs:subClassOf rdf:resource ="#GasMixture"/>
<rdfs:comment>Any GasMixture that is visible, e.g. Smoke produced
by a fire or clouds of water vapor in the sky.</rdfs:comment>
</owl:Class>

<owl:Class rdf:ID= "CognitiveAgent">
<rdfs:subClassOf rdf:resource ="#SentientAgent"/>
<rdfs:comment>A SentientAgent with responsibilities
and the ability to reason, deliberate, make plans, etc.  This is
essentially the legal/ethical notion of a person.  Note that, although
Human is a subclass of CognitiveAgent, there may be instances of
CognitiveAgent which are not also instances of Human.  For example,
chimpanzees, gorillas, dolphins, whales, and some extraterrestrials
(if they exist) may be CognitiveAgents.</rdfs:comment>
</owl:Class>

<owl:Class rdf:ID= "ColdBloodedVertebrate">
<rdfs:subClassOf rdf:resource ="#Vertebrate"/>
<rdfs:comment>Vertebrates whose body temperature
is not internally regulated.</rdfs:comment>
</owl:Class>

<owl:Class rdf:ID= "Collection">
<rdfs:subClassOf rdf:resource ="#Object"/>
<disjoint rdf:resource = "#SelfConnectedObject" />
<rdfs:comment>Collections have members like Classes, but,
unlike Classes, they have a position in space-time and members can be
added and subtracted without thereby changing the identity of the
Collection.  Some examples are toolkits, football teams, and flocks
of sheep.</rdfs:comment>
</owl:Class>



<owl:Class rdf:ID= "Coloring">
<rdfs:subClassOf rdf:resource ="#SurfaceChange"/>
<rdfs:comment>The subclass of SurfaceChange where a
ColorAttribute of the patient is altered.</rdfs:comment>
</owl:Class>

<owl:Class rdf:ID= "Combining">
<rdfs:subClassOf rdf:resource ="#DualObjectProcess"/>
<rdfs:comment>A Process where two or more SelfConnectedObjects
are incorporated into a single SelfConnectedObject.  Note that Combining
is different from Attaching in that the former results in one of the objects
being part of the other, while Attaching only results in the two objects
being connected with one another.  Note too that Combining is different
from Putting in that one or both of the two things which are combined may or
may not be moved from the location where they were combined.</rdfs:comment>
</owl:Class>

<owl:Class rdf:ID= "Combustion">
<rdfs:subClassOf rdf:resource ="#ChemicalDecomposition"/>
<rdfs:comment>The Class of ChemicalProcesses in which an Object
reacts with oxygen and gives off heat.  This includes all Processes in which
something is burning.</rdfs:comment>
</owl:Class>

<owl:Class rdf:ID= "CommercialAgent">
<rdfs:subClassOf rdf:resource ="#Agent"/>
<rdfs:comment>An Agent that provides products and/or
services for a fee with the aim of making a profit.</rdfs:comment>
</owl:Class>

<owl:Class rdf:ID= "CommercialService">
<rdfs:subClassOf rdf:resource ="#FinancialTransaction"/>
<rdfs:comment>Any FinancialTransaction by a
CommercialAgent where the aim is to produce a profit.</rdfs:comment>
</owl:Class>

<owl:Class rdf:ID= "Committing">
<rdfs:subClassOf rdf:resource ="#LinguisticCommunication"/>
<rdfs:comment>Instances of this Class commit the agent to some
future course.  For example, Bob promised Susan that he would be home by 11pm.</rdfs:comment>
</owl:Class>

<owl:Class rdf:ID= "Communication">
<rdfs:subClassOf rdf:resource ="#SocialInteraction"/>
<relatedInternalConcept rdf:resource = "#ContentDevelopment" />
<rdfs:comment>A SocialInteraction that involves
the transfer of information between two or more CognitiveAgents.
Note that Communication is closely related to, but essentially
different from, ContentDevelopment.  The latter involves the creation
or modification of a ContentBearingObject, while Communication is
the transfer of information for the purpose of conveying a message.</rdfs:comment>
</owl:Class>

<owl:Class rdf:ID= "CommutativeFunction">
<rdfs:subClassOf rdf:resource ="#BinaryFunction"/>
<rdfs:comment>A BinaryFunction is commutative if
the ordering of the arguments of the function has no effect on the value
returned by the function.  More precisely, a function ?FUNCTION is
commutative just in case (?FUNCTION ?INST1 ?INST2) is equal to (?FUNCTION
?INST2 ?INST1), for all ?INST1 and ?INST2.</rdfs:comment>
</owl:Class>

<owl:Class rdf:ID= "Comparing">
<rdfs:subClassOf rdf:resource ="#IntentionalPsychologicalProcess"/>
<rdfs:subClassOf rdf:resource ="#DualObjectProcess"/>
<rdfs:comment>The Class of IntentionalPsychologicalProcesses
which involve comparing, relating, contrasting, etc. the properties of
two or more Entities.</rdfs:comment>
</owl:Class>

<owl:Class rdf:ID= "ComplexNumber">
<rdfs:subClassOf rdf:resource ="#Number"/>
<disjoint rdf:resource = "#RealNumber" />
<rdfs:comment>A Number that has the form: x + yi, where x
and y are RealNumbers and i is the square root of -1.</rdfs:comment>
</owl:Class>

<owl:Class rdf:ID= "CompoundSubstance">
<rdfs:subClassOf rdf:resource ="#PureSubstance"/>
<rdfs:comment>The Class of Substances that contain
two or more elements (ElementalSubstances), in definite proportion by weight.
The composition of a pure compound will be invariant, regardless of the method
of preparation. Compounds are composed of more than one kind of atom (element).
The term molecule is often used for the smallest unit of a compound that still
retains all of the properties of the compound.  Examples: Table salt (sodium
chloride, NaCl), sugar (sucrose, C_{12}H_{22}O_{11}), and water (H_2O). </rdfs:comment>
</owl:Class>

<owl:Class rdf:ID= "ComputerLanguage">
<rdfs:subClassOf rdf:resource ="#ArtificialLanguage"/>
<rdfs:comment>The class of Languages designed for
and interpreted by a computer.</rdfs:comment>
</owl:Class>

<owl:Class rdf:ID= "ComputerProgram">
<rdfs:subClassOf rdf:resource ="#Procedure"/>
<rdfs:comment>A set of instructions in a computer
programming language that can be executed by a computer.</rdfs:comment>
</owl:Class>

<owl:Class rdf:ID= "Condensing">
<rdfs:subClassOf rdf:resource ="#StateChange"/>
<rdfs:comment>The Class of Processes where an Object is
cooled and converted from a Gas to a Liquid.</rdfs:comment>
</owl:Class>

<owl:Class rdf:ID= "Confining">
<rdfs:subClassOf rdf:resource ="#Keeping"/>
<rdfs:comment>The Class of Keeping Processes where the
patient is a Human or an Animal and is kept involuntarily.  This covers
caging, imprisonment, jailing, etc.</rdfs:comment>
</owl:Class>



<owl:Class rdf:ID= "ConstantQuantity">
<rdfs:subClassOf rdf:resource ="#PhysicalQuantity"/>
<rdfs:comment>A ConstantQuantity is a
PhysicalQuantity which has a constant value, e.g. 3 meters and 5 hours.
The magnitude (see MagnitudeFn) of every ConstantQuantity is a
RealNumber.  ConstantQuantities are distinguished from
FunctionQuantities, which map ConstantQuantities to other
ConstantQuantities.  All ConstantQuantites are expressed with the
BinaryFunction MeasureFn, which takes a Number and a UnitOfMeasure
as arguments.  For example, 3 Meters can be expressed as (MeasureFn 3
Meter).  ConstantQuantities form a partial order (see
PartialOrderingRelation) with the lessThan relation, since lessThan
is a RelationExtendedToQuantities and lessThan is defined over the
RealNumbers.  The lessThan relation is not a total order (see
TotalOrderingRelation) over the class ConstantQuantity since elements
of some subclasses of ConstantQuantity (such as length quantities)
are incomparable to elements of other subclasses of ConstantQuantity
(such as mass quantities).</rdfs:comment>
</owl:Class>

<owl:Class rdf:ID= "ConstructedLanguage">
<rdfs:subClassOf rdf:resource ="#HumanLanguage"/>
<rdfs:subClassOf rdf:resource ="#ArtificialLanguage"/>
<rdfs:comment>An ConstructedLanguage is a
HumanLanguage that did not evolve spontaneously within a language
community, but rather had its core grammar and vocabulary invented by
one or more language experts, often with an aim to produce a more
grammatically regular language than any language that has evolved
naturally.  This Class includes languages like Esperanto that were
created to facilitate international communication</rdfs:comment>
</owl:Class>

<owl:Class rdf:ID= "Constructing">
<rdfs:subClassOf rdf:resource ="#Making"/>
<rdfs:comment>The subclass of Making in which a
StationaryArtifact is built.</rdfs:comment>
</owl:Class>

<owl:Class rdf:ID= "ContentBearingObject">
<rdfs:subClassOf rdf:resource ="#CorpuscularObject"/>
<relatedInternalConcept rdf:resource = "#containsInformation" />
<rdfs:comment>Any SelfConnectedObject that expresses
content.  This content may be a Proposition, e.g. when the ContentBearingObject
is a Sentence or Text, or it may be a representation of an abstract or
physical object, as with an Icon, a Word or a Phrase.</rdfs:comment>
</owl:Class>

<owl:Class rdf:ID= "ContentDevelopment">
<rdfs:subClassOf rdf:resource ="#IntentionalProcess"/>
<rdfs:comment>A subclass of IntentionalProcess in
which content is modified, its form is altered or it is created anew.</rdfs:comment>
</owl:Class>

<owl:Class rdf:ID= "Contest">
<rdfs:subClassOf rdf:resource ="#SocialInteraction"/>
<rdfs:comment>A SocialInteraction where the agent and
patient are CognitiveAgents who are trying to defeat one another.
Note that this concept is often applied in a metaphorical sense in natural
language, when we speak, e.g., of the struggle of plants for space or
sunlight, or of bacteria for food resources in some environment.</rdfs:comment>
</owl:Class>

<owl:Class rdf:ID= "ContestAttribute">
<rdfs:subClassOf rdf:resource ="#ObjectiveNorm"/>
<rdfs:comment>A Class containing Attributes that are
specific to participants in a Contest.  In particular, these Attributes
indicate the position of one of the agents in the Contest with respect
to other agent(s) in the Contest.   Some examples of these Attributes
are winning, losing, won, lost, etc.</rdfs:comment>
</owl:Class>

<owl:Class rdf:ID= "Continent">
<rdfs:subClassOf rdf:resource ="#LandArea"/>
<rdfs:comment>One of the seven largest land masses on earth,
viz. Africa, North America, South America, Antarctica, Europe, Asia, and
Oceania.  Note that this naming scheme is the one used in the CIA World
Factbook.</rdfs:comment>
</owl:Class>

<owl:Class rdf:ID= "ContinuousFunction">
<rdfs:subClassOf rdf:resource ="#Function"/>
<rdfs:comment>Functions which are continuous.
This concept is taken as primitive until representations for limits
are devised.</rdfs:comment>
</owl:Class>

<owl:Class rdf:ID= "Cooking">
<rdfs:subClassOf rdf:resource ="#Making"/>
<rdfs:comment>The Making of an instance of Food.  Note
that this can cover any preparation of Food, e.g. making a salad,
cutting up fruit, etc.  It does not necessarily involve the application
of heat.</rdfs:comment>
</owl:Class>

<owl:Class rdf:ID= "Cooling">
<rdfs:subClassOf rdf:resource ="#Decreasing"/>
<rdfs:comment>Any Decreasing Process where the PhysicalQuantity
decreased is a TemperatureMeasure.</rdfs:comment>
</owl:Class>

<owl:Class rdf:ID= "Cooperation">
<rdfs:subClassOf rdf:resource ="#SocialInteraction"/>
<rdfs:comment>The subclass of SocialInteraction where
the participants involved work together for the achievement of a common
goal.</rdfs:comment>
</owl:Class>

<owl:Class rdf:ID= "Corporation">
<rdfs:subClassOf rdf:resource ="#CommercialAgent"/>
<rdfs:subClassOf rdf:resource ="#Organization"/>
<rdfs:comment>An Organization that has a special legal status
that allows a group of persons to act as a CommercialAgent and that insulates
the owners (shareholders) from many liabilities that might result from the
corporation's operation.</rdfs:comment>
</owl:Class>

<owl:Class rdf:ID= "CorpuscularObject">
<rdfs:subClassOf rdf:resource ="#SelfConnectedObject"/>
<disjoint rdf:resource = "#Substance" />
<rdfs:comment>A SelfConnectedObject whose parts have
properties that are not shared by the whole.</rdfs:comment>
</owl:Class>

<owl:Class rdf:ID= "Counting">
<rdfs:subClassOf rdf:resource ="#Calculating"/>
<rdfs:comment>Enumerating something.  The Class of Calculating
Processes where the aim is to determine the Number corresponding to the
patient.</rdfs:comment>
</owl:Class>

<owl:Class rdf:ID= "Covering">
<rdfs:subClassOf rdf:resource ="#Putting"/>
<rdfs:comment>The Class of Putting processes where the agent
covers the patient, either completely or only partially, with something
else.</rdfs:comment>
</owl:Class>

<owl:Class rdf:ID= "Creation">
<rdfs:subClassOf rdf:resource ="#InternalChange"/>
<relatedInternalConcept rdf:resource = "#Destruction" />
<rdfs:comment>The subclass of Process in which
something is created.  Note that the thing created is specified
with the result CaseRole.</rdfs:comment>
</owl:Class>

<owl:Class rdf:ID= "Crustacean">
<rdfs:subClassOf rdf:resource ="#Arthropod"/>
<rdfs:comment>A Class of Arthropods that mainly dwells
in water and has a segmented body and a chitinous exoskeleton.  Includes
lobsters, crabs, shrimp, and barnacles.</rdfs:comment>
</owl:Class>

<owl:Class rdf:ID= "Cup">
<rdfs:subClassOf rdf:resource ="#VolumeMeasure"/>
<rdf:type rdf:resource = "#UnitOfMeasure"/>
<rdfs:comment>English unit of volume equal to 1/2 of a
Pint.</rdfs:comment>
</owl:Class>

<owl:Class rdf:ID= "Currency">
<rdfs:subClassOf rdf:resource ="#FinancialInstrument"/>
<rdfs:comment>Any element of the official currrency of some
Nation.  This covers both CurrencyBills and CurrencyCoins.</rdfs:comment>
</owl:Class>

<owl:Class rdf:ID= "CurrencyBill">
<rdfs:subClassOf rdf:resource ="#Currency"/>
<rdfs:comment>Any instance of Currency that is made
of paper.</rdfs:comment>
</owl:Class>

<owl:Class rdf:ID= "CurrencyCoin">
<rdfs:subClassOf rdf:resource ="#Currency"/>
<rdfs:comment>Any instance of Currency that is made
of Metal.</rdfs:comment>
</owl:Class>

<owl:Class rdf:ID= "CurrencyMeasure">
<rdfs:subClassOf rdf:resource ="#ConstantQuantity"/>
<rdfs:comment>Includes all standard measures of monetary
value, including UnitedStatesDollar, UnitedStatesCent, Lire, Yen, etc.</rdfs:comment>
</owl:Class>

<owl:Class rdf:ID= "Cutting">
<rdfs:subClassOf rdf:resource ="#Poking"/>
<rdfs:comment>The subclass of Poking Processes which
involve a sharp instrument.</rdfs:comment>
</owl:Class>

<owl:Class rdf:ID= "Damaging">
<rdfs:subClassOf rdf:resource ="#InternalChange"/>
<disjoint rdf:resource = "#Repairing" />
<rdfs:comment>The Class of Processes where the agent
brings about a situation where the patient no longer functions normally
or as intended.</rdfs:comment>
</owl:Class>

<owl:Class rdf:ID= "Day">
<rdfs:subClassOf rdf:resource ="#TimeInterval"/>
<relatedInternalConcept rdf:resource = "#DayFn" />
<relatedInternalConcept rdf:resource = "#DayDuration" />
<rdfs:comment>The Class of all calendar Days.</rdfs:comment>
</owl:Class>

<owl:Class rdf:ID= "DayDuration">
<rdfs:subClassOf rdf:resource ="#TimeDuration"/>
<rdf:type rdf:resource = "#UnitOfMeasure"/>
<rdfs:comment>Time unit. 1 day = 24 hours.</rdfs:comment>
</owl:Class>

<owl:Class rdf:ID= "Death">
<rdfs:subClassOf rdf:resource ="#OrganismProcess"/>
<rdfs:comment>The Process of dying.</rdfs:comment>
</owl:Class>

<owl:Class rdf:ID= "December">
<rdfs:subClassOf rdf:resource ="#Month"/>
<rdfs:comment>The Class of all Months which are December.</rdfs:comment>
</owl:Class>

<owl:Class rdf:ID= "Deciding">
<rdfs:subClassOf rdf:resource ="#Selecting"/>
<rdfs:comment>The subclass of Selecting where the agent
opts for one course of action out of a set of multiple possibilities
that are open to him/her.</rdfs:comment>
</owl:Class>

<owl:Class rdf:ID= "Declaring">
<rdfs:subClassOf rdf:resource ="#LinguisticCommunication"/>
<rdfs:comment>The Class of LinguisticCommunications that
effect an institutional alteration when performed by competent authority.
Some examples are nominating, marrying, and excommunicating.</rdfs:comment>
</owl:Class>

<owl:Class rdf:ID= "Decoding">
<rdfs:subClassOf rdf:resource ="#Writing"/>
<disjoint rdf:resource = "#Encoding" />
<rdfs:comment>Converting a document or message that has previously
been encoded (see Encoding) into a Language that can be understood by a
relatively large number of speakers.</rdfs:comment>
</owl:Class>

<owl:Class rdf:ID= "Decreasing">
<rdfs:subClassOf rdf:resource ="#QuantityChange"/>
<relatedInternalConcept rdf:resource = "#Removing" />
<rdfs:comment>Any QuantityChange where the PhysicalQuantity
is decreased.</rdfs:comment>
</owl:Class>

<owl:Class rdf:ID= "DeductiveArgument">
<rdfs:subClassOf rdf:resource ="#Argument"/>
<rdfs:comment>An Argument which has the form of a
deduction, i.e. it is claimed that the set of premises entails the
conclusion.</rdfs:comment>
</owl:Class>

<owl:Class rdf:ID= "DefensiveManeuver">
<rdfs:subClassOf rdf:resource ="#Maneuver"/>
<rdfs:comment>A Maneuver in a ViolentContest
where the agent attempts to avoid being damaged.</rdfs:comment>
</owl:Class>

<owl:Class rdf:ID= "Demonstrating">
<rdfs:subClassOf rdf:resource ="#Disseminating"/>
<rdfs:comment>Exhibiting something or a range of things
before the public in a particular location.  This would cover software
demos, theatrical plays, lectures, dance and music recitals, museum
exhibitions, etc.</rdfs:comment>
</owl:Class>

<owl:Class rdf:ID= "DeonticAttribute">
<rdfs:subClassOf rdf:resource ="#ObjectiveNorm"/>
<rdfs:comment>A Class containing all of the Attributes
relating to the notions of permission, obligation, and prohibition.</rdfs:comment>
</owl:Class>

<owl:Class rdf:ID= "Designing">
<rdfs:subClassOf rdf:resource ="#IntentionalPsychologicalProcess"/>
<rdfs:comment>The spatial analogue of Planning.  Designing a
Collection of Objects involves determining a placement of the Objects
with respect to one another and perhaps other Objects as well, in order to
satisfy a particular purpose.</rdfs:comment>
</owl:Class>

<owl:Class rdf:ID= "Destruction">
<rdfs:subClassOf rdf:resource ="#Damaging"/>
<rdfs:comment>The subclass of Damagings in which
the patient (or an essential element of the patient) is destroyed.
Note that the difference between this concept and its superclass is solely
one of extent.</rdfs:comment>
</owl:Class>

<owl:Class rdf:ID= "Detaching">
<rdfs:subClassOf rdf:resource ="#DualObjectProcess"/>
<rdfs:comment>A Process where the agent detaches one thing
from something else.  Note that Detaching is different from Separating
in that the latter applies to Substances, while the former applies to CorpuscularObjects.  Note too that Detaching is different from Removing
in that one or both of the two things which are detached may or may not be
moved from the location where they were attached.</rdfs:comment>
</owl:Class>



<owl:Class rdf:ID= "Device">
<rdfs:subClassOf rdf:resource ="#Artifact"/>
<rdfs:comment>A Device is an Artifact whose purpose is to
serve as an instrument in a specific subclass of Process.</rdfs:comment>
</owl:Class>

<owl:Class rdf:ID= "DiagnosticProcess">
<rdfs:subClassOf rdf:resource ="#Investigating"/>
<rdfs:comment>A Process that is carried out for
the purpose of determining the nature of a DiseaseOrSyndrome.</rdfs:comment>
</owl:Class>

<owl:Class rdf:ID= "Digesting">
<rdfs:subClassOf rdf:resource ="#OrganismProcess"/>
<rdfs:subClassOf rdf:resource ="#AutonomicProcess"/>
<rdfs:comment>The Process by which Food that has been
ingested is broken down into simpler chemical compounds and absorbed by
the Organism.</rdfs:comment>
</owl:Class>

<owl:Class rdf:ID= "Directing">
<rdfs:subClassOf rdf:resource ="#LinguisticCommunication"/>
<rdfs:comment>Instances of this Class urge some further action
among the receivers.  A Directing can be an Ordering, a Requesting or
a Questioning.</rdfs:comment>
</owl:Class>

<owl:Class rdf:ID= "DirectionChange">
<rdfs:subClassOf rdf:resource ="#Motion"/>
<rdfs:comment>The act of changing the direction in
which the patient of the act is oriented.</rdfs:comment>
</owl:Class>

<owl:Class rdf:ID= "DirectionalAttribute">
<rdfs:subClassOf rdf:resource ="#PositionalAttribute"/>
<rdfs:comment>The subclass of PositionalAttributes
that concern compass directions.</rdfs:comment>
</owl:Class>

<owl:Class rdf:ID= "Discovering">
<rdfs:subClassOf rdf:resource ="#IntentionalPsychologicalProcess"/>
<rdfs:comment>Finding something that was sought.  Note that
this class is restricted to cases of discovering something Physical.
For cases involving the acquisition of knowledge, the class Learning
should be used.</rdfs:comment>
</owl:Class>



<owl:Class rdf:ID= "Disseminating">
<rdfs:subClassOf rdf:resource ="#Communication"/>
<rdfs:comment>Any Communication that involves a
single agent and many destinations.  This covers the release
of a published book, broadcasting, a theatrical performance, giving
orders to assembled troops, delivering a public lecture, etc.</rdfs:comment>
</owl:Class>

<owl:Class rdf:ID= "Drinking">
<rdfs:subClassOf rdf:resource ="#Ingesting"/>
<rdfs:comment>The Process by which liquid Food, i.e.
Beverages, are incorporated into an Animal.</rdfs:comment>
</owl:Class>

<owl:Class rdf:ID= "Driving">
<rdfs:subClassOf rdf:resource ="#Guiding"/>
<rdfs:comment>Controlling the direction and/or speed of a
Vehicle.  This includes navigating a ship, driving a car or truck,
operating a train, etc.</rdfs:comment>
</owl:Class>

<owl:Class rdf:ID= "Drying">
<rdfs:subClassOf rdf:resource ="#Removing"/>
<rdfs:comment>The Class of Processes where a Liquid is removed
from an Object.</rdfs:comment>
</owl:Class>

<owl:Class rdf:ID= "DualObjectProcess">
<rdfs:subClassOf rdf:resource ="#Process"/>
<rdfs:comment>Any Process that requires two,
nonidentical patients.</rdfs:comment>
</owl:Class>

<owl:Class rdf:ID= "Eating">
<rdfs:subClassOf rdf:resource ="#Ingesting"/>
<rdfs:comment>The Process by which solid Food is
incorporated into an Animal.</rdfs:comment>
</owl:Class>

<owl:Class rdf:ID= "EducationalOrganization">
<rdfs:subClassOf rdf:resource ="#Organization"/>
<rdfs:comment>A EducationalOrganization is
an institution of learning. Some examples are public and private K-12
schools, and colleges and universities.</rdfs:comment>
</owl:Class>

<owl:Class rdf:ID= "EducationalProcess">
<rdfs:subClassOf rdf:resource ="#Guiding"/>
<rdfs:comment>Any Process which is intended to result
in Learning.</rdfs:comment>
</owl:Class>

<owl:Class rdf:ID= "Egg">
<rdfs:subClassOf rdf:resource ="#ReproductiveBody"/>
<rdfs:subClassOf rdf:resource ="#AnimalAnatomicalStructure"/>
<rdfs:comment>The fertilized or unfertilized female ReproductiveBody
of an Animal.  This includes Bird and Reptile eggs, as well as mammalian
ova.</rdfs:comment>
</owl:Class>

<owl:Class rdf:ID= "Election">
<rdfs:subClassOf rdf:resource ="#OrganizationalProcess"/>
<rdfs:comment>Election is the class of events conducted by an
organization, in which qualified participants vote for officers, adopt
resolutions, or settle other issues in that Organization.</rdfs:comment>
</owl:Class>

<owl:Class rdf:ID= "Electron">
<rdfs:subClassOf rdf:resource ="#SubatomicParticle"/>
<rdfs:comment>SubatomicParticles that surround the
AtomicNucleus.  They have a negative charge.</rdfs:comment>
</owl:Class>

<owl:Class rdf:ID= "ElementalSubstance">
<rdfs:subClassOf rdf:resource ="#PureSubstance"/>
<rdfs:comment>The Class of PureSubstances that
cannot be separated into two or more Substances by ordinary chemical
(or physical) means. This excludes nuclear reactions. ElementalSubstances
are composed of only one kind of atom. Examples: Iron (Fe), copper (Cu),
and oxygen (O_2).  ElementalSubstances are the simplest
PureSubstances.</rdfs:comment>
</owl:Class>


<owl:Class rdf:ID= "Encoding">
<rdfs:subClassOf rdf:resource ="#Writing"/>
<rdfs:comment>Converting a document or message into a formal
language or into a code that can be understood only by a relatively small
body of Agents.  Generally speaking, this hinders wide dissemination of
the content in the original document or message.</rdfs:comment>
</owl:Class>

<owl:Class rdf:ID= "EngineeringComponent">
<rdfs:subClassOf rdf:resource ="#Device"/>
<rdfs:comment>A fundamental concept that applies
in many engineering domains.  An EngineeringComponent is an element of
a Device that is a physically whole object, such as one might
see listed as standard parts in a catalog.  The main difference betweeen
EngineeringComponents and arbitrary globs of matter is that
EngineeringComponents are object-like in a modeling sense.  Thus, an
EngineeringComponent is not an arbtrary subregion, but a part of a
system with a stable identity.</rdfs:comment>
</owl:Class>

<owl:Class rdf:ID= "EngineeringConnection">
<rdfs:subClassOf rdf:resource ="#EngineeringComponent"/>
<rdfs:comment>An EngineeringConnection is an
EngineeringComponent that represents a connection relationship between
two other EngineeringComponents.  It is a reification of the
Predicate connectedEngineeringComponents.  That means that whenever
this Predicate holds between two EngineeringComponents, there exists an
EngineeringConnection.  The practical reason for reifying a relationship
is to be able to attach other information about it. For example, one
might want to say that a particular connection is associated with some
shared parameters, or that it is of a particular type.
EngineeringConnections are EngineeringComponents and can therefore be
an engineeringSubcomponent of other EngineeringComponents.  However,
to provide for modular regularity in component systems,
EngineeringConnections cannot be connected.  For each pair of
EngineeringComponents related by connectedEngineeringComponents, there
exists at least one EngineeringConnection.  However, that object may not
be unique, and the same EngineeringConnection may be associated with
several pairs of EngineeringComponents.</rdfs:comment>
</owl:Class>


<owl:Class rdf:ID= "EquivalenceRelation">
<rdfs:subClassOf rdf:resource ="#TransitiveRelation"/>
<rdfs:subClassOf rdf:resource ="#SymmetricRelation"/>
<rdfs:subClassOf rdf:resource ="#ReflexiveRelation"/>
<rdfs:comment>A BinaryRelation is an equivalence
relation if it is a ReflexiveRelation, a SymmetricRelation, and a
TransitiveRelation.</rdfs:comment>
</owl:Class>

<owl:Class rdf:ID= "EthnicGroup">
<rdfs:subClassOf rdf:resource ="#GroupOfPeople"/>
<rdfs:comment>A GroupOfPeople whose members originate
from the same GeographicArea or share the same Language and/or cultural
practices.</rdfs:comment>
</owl:Class>

<owl:Class rdf:ID= "EuroCent">
<rdfs:subClassOf rdf:resource ="#CurrencyMeasure"/>
<rdf:type rdf:resource = "#UnitOfMeasure"/>
<rdfs:comment>A currency measure.  1 EuroCent is equal to .01
EuroDollars.</rdfs:comment>
</owl:Class>

<owl:Class rdf:ID= "EuroDollar">
<rdfs:subClassOf rdf:resource ="#CurrencyMeasure"/>
<rdf:type rdf:resource = "#UnitOfMeasure"/>
<rdfs:comment>A currency measure of most European Union countries.
It is based on the UnitedStatesDollar.</rdfs:comment>
</owl:Class>

<owl:Class rdf:ID= "EvenInteger">
<rdfs:subClassOf rdf:resource ="#Integer"/>
<rdfs:comment>An Integer that is evenly divisible
by 2.</rdfs:comment>
</owl:Class>

<owl:Class rdf:ID= "Experimenting">
<rdfs:subClassOf rdf:resource ="#Investigating"/>
<rdfs:comment>Investigating the truth of a Proposition
by constructing and observing a trial.  Note that the trial may be either
controlled or uncontrolled, blind or not blind.</rdfs:comment>
</owl:Class>

<owl:Class rdf:ID= "Explanation">
<rdfs:subClassOf rdf:resource ="#DeductiveArgument"/>
<rdfs:comment>An Argument where the conclusion is an
observed fact and the premises are other facts which collectively imply
the conclusion.  Note that this is the they hypothetico-deductive model
of explanation.</rdfs:comment>
</owl:Class>

<owl:Class rdf:ID= "Expressing">
<rdfs:subClassOf rdf:resource ="#Communication"/>
<rdfs:comment>Instances of this Class express a state of the agent.
For example, Jane thanked Barbara for the present she had given her.  The thanking
in this case expresses the gratitude of Jane towards Barbara.  Note that Expressing,
unlike the other speech act types, is not a subclass of LinguisticCommunication.
This is because emotions, for example, can be expressed without language, e.g. by
smiling.</rdfs:comment>
</owl:Class>

<owl:Class rdf:ID= "Fabric">
<rdfs:subClassOf rdf:resource ="#Artifact"/>
<disjoint rdf:resource = "#StationaryArtifact" />
<rdfs:comment>Artifacts that are created by weaving together
natural or synthetic fibers or by treating the skins of certain sorts of
Animals.  Note that this Class includes articles that are created by
stitching together various types of fabrics, e.g. bedspreads.  On the other
hand, Clothing is not a subclass of Fabric, because many clothing items
contain elements that are not fabrics.</rdfs:comment>
</owl:Class>

<owl:Class rdf:ID= "FactualText">
<rdfs:subClassOf rdf:resource ="#Text"/>
<disjoint rdf:resource = "#FictionalText" />
<rdfs:comment>The class of Texts that purport to
reveal facts about the world.  Such texts are often known as information
or as non-fiction.  Note that something can be an instance of
FactualText, even if it is wholly inaccurate.  Whether something
is a FactualText is determined by the beliefs of the agent creating
the text.</rdfs:comment>
</owl:Class>

<owl:Class rdf:ID= "FahrenheitDegree">
<rdfs:subClassOf rdf:resource ="#TemperatureMeasure"/>
<rdf:type rdf:resource = "#UnitOfMeasure"/>
<rdfs:comment>A TemperatureMeasure that is commonly
used in the United States.  On the Fahrenheit scale, the freezing point
of water is 32 FahrenheitDegrees, and the boiling point of water is
212 FahrenheitDegrees.</rdfs:comment>
</owl:Class>

<owl:Class rdf:ID= "FamilyGroup">
<rdfs:subClassOf rdf:resource ="#GroupOfPeople"/>
<rdfs:comment>A GroupOfPeople whose members bear
familyRelations to one another.</rdfs:comment>
</owl:Class>

<owl:Class rdf:ID= "FatTissue">
<rdfs:subClassOf rdf:resource ="#Tissue"/>
<rdfs:comment>Nonrigid Tissue that is composed largely of
fat cells.</rdfs:comment>
</owl:Class>

<owl:Class rdf:ID= "February">
<rdfs:subClassOf rdf:resource ="#Month"/>
<rdfs:comment>The Class of all Months which are February.</rdfs:comment>
</owl:Class>

<owl:Class rdf:ID= "Feline">
<rdfs:subClassOf rdf:resource ="#Carnivore"/>
<rdfs:comment>The Class of Carnivores with completely
separable toes, nonretractable claws, slim bodies, and rounded heads.</rdfs:comment>
</owl:Class>

<owl:Class rdf:ID= "Fern">
<rdfs:subClassOf rdf:resource ="#NonFloweringPlant"/>
<rdfs:comment>A NonFloweringPlant that contains vascular tissue.
This class includes true ferns, as well as horsetails, club mosses, and
whisk ferns.</rdfs:comment>
</owl:Class>

<owl:Class rdf:ID= "FictionalText">
<rdfs:subClassOf rdf:resource ="#Text"/>
<rdfs:comment>The class of Texts that purport to
be largely a product of the author's imagination, i.e. the author
does not believe that most of the content conveyed by the text is
an accurate depiction of the real world.  Note that something can
be an instance of FictionalText, even if it is completely true.
Whether something is a FictionalText is determined by the beliefs
of the agent creating the text.</rdfs:comment>
</owl:Class>

<owl:Class rdf:ID= "FieldOfStudy">
<rdfs:subClassOf rdf:resource ="#Proposition"/>
<rdfs:comment>An academic or applied discipline with
recognized experts and with a core of accepted theory or practice.  Note
that FieldOfStudy is a subclass of Proposition, because a
FieldOfStudy is understood to be a body of abstract, informational
content, with varying degrees of certainty attached to each element of
this content.</rdfs:comment>
</owl:Class>

<owl:Class rdf:ID= "FinancialInstrument">
<rdfs:subClassOf rdf:resource ="#Certificate"/>
<rdfs:comment>A document having monetary value
or recording a monetary transaction</rdfs:comment>
</owl:Class>

<owl:Class rdf:ID= "FinancialTransaction">
<rdfs:subClassOf rdf:resource ="#Transaction"/>
<rdfs:comment>A Transaction where an instance
of Currency is exchanged for something else.</rdfs:comment>
</owl:Class>

<owl:Class rdf:ID= "FiniteSet">
<rdfs:subClassOf rdf:resource ="#Set"/>
<rdfs:comment>A Set containing a finite number of elements.</rdfs:comment>
</owl:Class>

<owl:Class rdf:ID= "Fish">
<rdfs:subClassOf rdf:resource ="#ColdBloodedVertebrate"/>
<rdfs:comment>A cold-blooded aquatic Vertebrate characterized by
fins and breathing by gills. Included here are Fish having either a bony
skeleton, such as a perch, or a cartilaginous skeleton, such as a shark.
Also included are those Fish lacking a jaw, such as a lamprey or
hagfish.</rdfs:comment>
</owl:Class>

<owl:Class rdf:ID= "FloweringPlant">
<rdfs:subClassOf rdf:resource ="#Plant"/>
<rdfs:comment>A Plant that produces seeds and flowers.
This class includes trees, shrubs, herbs, and flowers.</rdfs:comment>
</owl:Class>

<owl:Class rdf:ID= "Food">
<rdfs:subClassOf rdf:resource ="#SelfConnectedObject"/>
<rdfs:comment>Any SelfConnectedObject containing Nutrients,
such as carbohydrates, proteins, and fats, that can be ingested by a
living Animal and metabolized into energy and body tissue.</rdfs:comment>
</owl:Class>

<owl:Class rdf:ID= "FootLength">
<rdfs:subClassOf rdf:resource ="#LengthMeasure"/>
<rdf:type rdf:resource = "#UnitOfMeasure"/>
<rdfs:comment>English length unit of feet.</rdfs:comment>
</owl:Class>

<owl:Class rdf:ID= "Formula">
<rdfs:subClassOf rdf:resource ="#Sentence"/>
<rdfs:comment>A syntactically well-formed formula in the
SUO-KIF knowledge representation language.</rdfs:comment>
</owl:Class>

<owl:Class rdf:ID= "Freezing">
<rdfs:subClassOf rdf:resource ="#StateChange"/>
<rdfs:comment>The Class of Processes where an Object is
cooled and converted from a Liquid to a Solid.</rdfs:comment>
</owl:Class>

<owl:Class rdf:ID= "FreshWaterArea">
<rdfs:subClassOf rdf:resource ="#WaterArea"/>
<rdfs:comment>A WaterArea whose Water is not saline,
e.g. most rivers and lakes.</rdfs:comment>
</owl:Class>

<owl:Class rdf:ID= "Friday">
<rdfs:subClassOf rdf:resource ="#Day"/>
<rdfs:comment>The Class of all calendar Fridays.</rdfs:comment>
</owl:Class>

<owl:Class rdf:ID= "FruitOrVegetable">
<rdfs:subClassOf rdf:resource ="#PlantAnatomicalStructure"/>
<rdfs:subClassOf rdf:resource ="#ReproductiveBody"/>
<rdfs:comment>Any fruit or vegetable, i.e. a
ripened ReproductiveBody of a Plant.  Note that FruitOrVegetable
is not a subclass of Food, because some fruits, e.g. poisonous
berries, are not edible.</rdfs:comment>
</owl:Class>

<owl:Class rdf:ID= "Function">
<rdfs:subClassOf rdf:resource ="#SingleValuedRelation"/>
<rdf:type rdf:resource = "#InheritableRelation"/>
<rdfs:comment>A Function is a term-forming Relation that
maps from a n-tuple of arguments to a range and that associates this
n-tuple with at most one range element.  Note that the range is a SetOrClass,
and each element of the range is an instance of the SetOrClass.</rdfs:comment>
</owl:Class>

<owl:Class rdf:ID= "FunctionQuantity">
<rdfs:subClassOf rdf:resource ="#PhysicalQuantity"/>
<rdfs:comment>A FunctionQuantity is a PhysicalQuantity
that is returned by a Function that maps from one or more instances of
ConstantQuantity to another instance of ConstantQuantity.  For example,
the velocity of a particle would be represented by a FunctionQuantity
relating values of time (which are ConstantQuantities) to values of distance
(also ConstantQuantities).  Note that all elements of the range of the
Function corresponding to a FunctionQuantity have the same physical
dimension as the FunctionQuantity itself.</rdfs:comment>
</owl:Class>

<owl:Class rdf:ID= "Funding">
<rdfs:subClassOf rdf:resource ="#Giving"/>
<rdfs:comment>Any instance of Giving where the patient is an
instance of Currency.  Note that this class covers both financing, e.g.
where a firm funds a software company with venture capital with the agreement
that a certain percentage of the profits on the investment will be returned
to the firm, and instances of UnilateralGiving, e.g. providing a tuition
waiver and/or a stipend to a student as part of scholarship or fellowship.</rdfs:comment>
</owl:Class>

<owl:Class rdf:ID= "Fungus">
<rdfs:subClassOf rdf:resource ="#NonFloweringPlant"/>
<rdfs:comment>A eukaryotic Organism characterized by the
absence of chlorophyll and the presence of rigid cell walls. Included
here are both slime molds and true fungi such as yeasts, molds, mildews,
and mushrooms.</rdfs:comment>
</owl:Class>

<owl:Class rdf:ID= "Game">
<rdfs:subClassOf rdf:resource ="#Contest"/>
<rdfs:subClassOf rdf:resource ="#RecreationOrExercise"/>
<rdfs:comment>A Contest whose purpose is the
enjoyment/stimulation of the participants or spectators of the Game.</rdfs:comment>
</owl:Class>

<owl:Class rdf:ID= "GasMixture">
<rdfs:subClassOf rdf:resource ="#Mixture"/>
<disjoint rdf:resource = "#LiquidMixture" />
<rdfs:comment>Any Mixture that satisfies two conditions,
viz. it is made up predominantly of things which are a Gas and any
component other than Gas in the Mixture is in the form of fine particles
which are suspended in the Gas.</rdfs:comment>
</owl:Class>

<owl:Class rdf:ID= "GasMotion">
<rdfs:subClassOf rdf:resource ="#Motion"/>
<rdfs:comment>Any Motion where the patient is a
Gas.  This class would cover, in particular, the motion of
Air, e.g. a breeze or wind.</rdfs:comment>
</owl:Class>

<owl:Class rdf:ID= "GeographicArea">
<rdfs:subClassOf rdf:resource ="#Region"/>
<rdfs:comment>A geographic location, generally having
definite boundaries.  Note that this differs from its immediate superclass
Region in that a GeographicArea is a three-dimensional Region of the
earth.  Accordingly, all astronomical objects other than earth and all
one-dimensional and two-dimensional Regions are not classed under
GeographicArea.</rdfs:comment>
</owl:Class>

<owl:Class rdf:ID= "GeologicalProcess">
<rdfs:subClassOf rdf:resource ="#Motion"/>
<disjoint rdf:resource = "#IntentionalProcess" />
<rdfs:comment>The class of activities that
are caused by geological forces and affect geological features,
and which may affect the biosphere as well.</rdfs:comment>
</owl:Class>

<owl:Class rdf:ID= "GeometricFigure">
<rdfs:subClassOf rdf:resource ="#ShapeAttribute"/>
<rdfs:comment>The class of all geometric figures, i.e. the
class of all abstract, spatial representations.  The instances of this class
are GeometricPoints, TwoDimensionalFigures or ThreeDimensionalFigures.</rdfs:comment>
</owl:Class>

<owl:Class rdf:ID= "GeometricPoint">
<rdfs:subClassOf rdf:resource ="#GeometricFigure"/>
<rdfs:comment>The class of zero-dimensional
GeometricFigures, i.e. the class of GeometricFigures that have position
but lack extension in any dimension.</rdfs:comment>
</owl:Class>

<owl:Class rdf:ID= "GeopoliticalArea">
<rdfs:subClassOf rdf:resource ="#GeographicArea"/>
<rdfs:subClassOf rdf:resource ="#Agent"/>
<rdfs:comment>Any GeographicArea which is associated
with some sort of political structure.  This class includes Lands,
Cities, districts of cities, counties, etc.  Note that the identity
of a GeopoliticalArea may remain constant after a change in borders.</rdfs:comment>
</owl:Class>

<owl:Class rdf:ID= "Gesture">
<rdfs:subClassOf rdf:resource ="#Communication"/>
<rdfs:subClassOf rdf:resource ="#BodyMotion"/>
<rdfs:comment>Any BodyMotion, e.g. a hand wave, a nod of the
head, a smile, which is also an instance of Communication.</rdfs:comment>
</owl:Class>

<owl:Class rdf:ID= "Getting">
<rdfs:subClassOf rdf:resource ="#ChangeOfPossession"/>
<rdfs:comment>The subclass of ChangeOfPossession where the
agent gets something.  Note that the source from which something is
obtained is specified with the origin CaseRole.</rdfs:comment>
</owl:Class>

<owl:Class rdf:ID= "Giving">
<rdfs:subClassOf rdf:resource ="#ChangeOfPossession"/>
<rdfs:comment>The subclass of ChangeOfPossession where the
agent gives the destination something.</rdfs:comment>
</owl:Class>

<owl:Class rdf:ID= "GivingBack">
<rdfs:subClassOf rdf:resource ="#Giving"/>
<rdfs:comment>Any instance of Giving where the agent gives
something to the destination which was previously given to the agent by
the destination, e.g. returing a book that was borrowed from someone.</rdfs:comment>
</owl:Class>

<owl:Class rdf:ID= "Government">
<rdfs:subClassOf rdf:resource ="#GovernmentOrganization"/>
<rdfs:comment>The ruling body of a GeopoliticalArea.</rdfs:comment>
</owl:Class>

<owl:Class rdf:ID= "GovernmentOrganization">
<rdfs:subClassOf rdf:resource ="#Organization"/>
<rdfs:comment>GovernmentOrganization is the
class of official Organizations that are concerned with the government
of a GeopoliticalArea at some level.  They may be a subOrganization
of a government.</rdfs:comment>
</owl:Class>

<owl:Class rdf:ID= "Grabbing">
<rdfs:subClassOf rdf:resource ="#Touching"/>
<rdfs:subClassOf rdf:resource ="#Attaching"/>
<rdfs:comment>Any instance of Touching which results in
a situation where the agent grasps the patient of the Touching.</rdfs:comment>
</owl:Class>

<owl:Class rdf:ID= "Graduation">
<rdfs:subClassOf rdf:resource ="#LeavingAnOrganization"/>
<rdfs:comment>The OrganizationalProcess of graduating
from an EducationalOrganization.</rdfs:comment>
</owl:Class>

<owl:Class rdf:ID= "Gram">
<rdfs:subClassOf rdf:resource ="#MassMeasure"/>
<rdf:type rdf:resource = "#SystemeInternationalUnit"/>
<rdfs:comment>Submultiple of kilogram.  Symbol: g.
1 kilogram = 1000 Grams.</rdfs:comment>
</owl:Class>

<owl:Class rdf:ID= "Group">
<rdfs:subClassOf rdf:resource ="#Collection"/>
<rdfs:subClassOf rdf:resource ="#Agent"/>
<rdfs:comment>A Collection of Agents, e.g. a flock
of sheep, a herd of goats, or the local Boy Scout troop.</rdfs:comment>
</owl:Class>

<owl:Class rdf:ID= "GroupOfPeople">
<rdfs:subClassOf rdf:resource ="#Group"/>
<rdfs:comment>Any Group whose members are
exclusively Humans.</rdfs:comment>
</owl:Class>

<owl:Class rdf:ID= "Growth">
<rdfs:subClassOf rdf:resource ="#AutonomicProcess"/>
<rdfs:comment>The Process of biological development in which
an Organism or part of an Organism changes its form or its size.</rdfs:comment>
</owl:Class>

<owl:Class rdf:ID= "Guiding">
<rdfs:subClassOf rdf:resource ="#IntentionalProcess"/>
<rdfs:comment>Any IntentionalProcess where the agent tries to
direct the behavior of another Object, whether an Agent or not.</rdfs:comment>
</owl:Class>

<owl:Class rdf:ID= "Hearing">
<rdfs:subClassOf rdf:resource ="#Perception"/>
<rdfs:comment>The subclass of Perception in which the
sensing is done by an auditory Organ.</rdfs:comment>
</owl:Class>

<owl:Class rdf:ID= "Heating">
<rdfs:subClassOf rdf:resource ="#Increasing"/>
<disjoint rdf:resource = "#Cooling" />
<rdfs:comment>Any Increasing Process where the PhysicalQuantity
increased is a TemperatureMeasure.</rdfs:comment>
</owl:Class>

<owl:Class rdf:ID= "Hertz">
<rdfs:subClassOf rdf:resource ="#TimeDependentQuantity"/>
<rdf:type rdf:resource = "#SystemeInternationalUnit"/>
<rdfs:comment>SI frequency measure.  Symbol: Hz. It is the
number of cycles per second.  Hertz = s^(-1).  Note that Hertz
does not have a conversion function.</rdfs:comment>
</owl:Class>

<owl:Class rdf:ID= "Hiring">
<rdfs:subClassOf rdf:resource ="#JoiningAnOrganization"/>
<rdfs:comment>OrganizationalProcesses where someone is made an
employee of an Organization.</rdfs:comment>
</owl:Class>

<owl:Class rdf:ID= "Hole">
<rdfs:subClassOf rdf:resource ="#Region"/>
<rdfs:comment>A hole is an immaterial body located at the surface
of an Object.  Since every Hole is ontologically dependent on its host
(i.e., the object in which it is a hole), being a Hole is defined as
being a hole in something.  Note that two Holes may occupy the same
region, or part of the same region, without sharing any parts.</rdfs:comment>
</owl:Class>

<owl:Class rdf:ID= "Hominid">
<rdfs:subClassOf rdf:resource ="#Primate"/>
<rdfs:comment>Includes Humans and relatively recent
ancestors of Humans.</rdfs:comment>
</owl:Class>

<owl:Class rdf:ID= "HoofedMammal">
<rdfs:subClassOf rdf:resource ="#Mammal"/>
<rdfs:comment>The Class of quadruped Mammals with hooves.
Includes horses, cows, sheep, pigs, antelope, etc.</rdfs:comment>
</owl:Class>

<owl:Class rdf:ID= "Hotel">
<rdfs:subClassOf rdf:resource ="#ResidentialBuilding"/>
<rdfs:subClassOf rdf:resource ="#TemporaryResidence"/>
<rdfs:subClassOf rdf:resource ="#CommercialAgent"/>
<rdfs:comment>A ResidentialBuilding which provides temporary
accommodations to guests in exchange for money.</rdfs:comment>
</owl:Class>

<owl:Class rdf:ID= "Hour">
<rdfs:subClassOf rdf:resource ="#TimeInterval"/>
<relatedInternalConcept rdf:resource = "#HourFn" />
<relatedInternalConcept rdf:resource = "#HourDuration" />
<rdfs:comment>The Class of all clock Hours.</rdfs:comment>
</owl:Class>

<owl:Class rdf:ID= "HourDuration">
<rdfs:subClassOf rdf:resource ="#TimeDuration"/>
<rdf:type rdf:resource = "#UnitOfMeasure"/>
<rdfs:comment>Time unit. 1 hour = 60 minutes.</rdfs:comment>
</owl:Class>

<owl:Class rdf:ID= "Human">
<rdfs:subClassOf rdf:resource ="#Hominid"/>
<rdfs:subClassOf rdf:resource ="#CognitiveAgent"/>
<rdfs:comment>Modern man, the only remaining species of the Homo
genus.</rdfs:comment>
</owl:Class>

<owl:Class rdf:ID= "HumanLanguage">
<rdfs:subClassOf rdf:resource ="#Language"/>
<rdfs:comment>The subclass of Languages used by
Humans.</rdfs:comment>
</owl:Class>

<owl:Class rdf:ID= "Icon">
<rdfs:subClassOf rdf:resource ="#ContentBearingObject"/>
<rdfs:comment>This is the subclass of ContentBearingObjects
which are not part of a Language and which have some sort of similarity
with the Objects that they represent.  This Class would include symbolic
roadway signs, representational art works, photographs, etc.</rdfs:comment>
</owl:Class>

<owl:Class rdf:ID= "ImaginaryNumber">
<rdfs:subClassOf rdf:resource ="#Number"/>
<rdfs:comment>Any Number that is the result of
multiplying a RealNumber by the square root of -1.</rdfs:comment>
</owl:Class>

<owl:Class rdf:ID= "Impacting">
<rdfs:subClassOf rdf:resource ="#Touching"/>
<rdfs:comment>Any Touching where something comes into
sudden, forceful, physical contact with something else.  Some examples
would be striking, knocking, whipping etc.</rdfs:comment>
</owl:Class>

<owl:Class rdf:ID= "Impelling">
<rdfs:subClassOf rdf:resource ="#Transfer"/>
<rdfs:comment>The subclass of Transfer where the patient
travels through space by means of a sudden, forceful event.  Some examples
would be shooting, throwing, tossing, etc.</rdfs:comment>
</owl:Class>

<owl:Class rdf:ID= "Inch">
<rdfs:subClassOf rdf:resource ="#LengthMeasure"/>
<rdf:type rdf:resource = "#UnitOfMeasure"/>
<rdfs:comment>English length unit of inches.</rdfs:comment>
</owl:Class>

<owl:Class rdf:ID= "Increasing">
<rdfs:subClassOf rdf:resource ="#QuantityChange"/>
<relatedInternalConcept rdf:resource = "#Putting" />
<rdfs:comment>Any QuantityChange where the PhysicalQuantity
is increased.</rdfs:comment>
</owl:Class>

<owl:Class rdf:ID= "InductiveArgument">
<rdfs:subClassOf rdf:resource ="#Argument"/>
<rdfs:comment>An Argument which is inductive, i.e. it is
claimed that a set of specific cases makes the conclusion, which generalizes
these cases, more likely to be true.</rdfs:comment>
</owl:Class>

<owl:Class rdf:ID= "InformationMeasure">
<rdfs:subClassOf rdf:resource ="#ConstantQuantity"/>
<rdfs:comment>Measures of the amount of information.
Includes Bit, Byte, and multiples of these, e.g. KiloByte and
MegaByte.</rdfs:comment>
</owl:Class>

<owl:Class rdf:ID= "Ingesting">
<rdfs:subClassOf rdf:resource ="#OrganismProcess"/>
<rdfs:comment>The Process by which Food is
taken into an Animal.</rdfs:comment>
</owl:Class>

<owl:Class rdf:ID= "InheritableRelation">
<rdf:type rdf:resource = "#Class"/>
<rdfs:comment>This is a Class of Classes.  Each
instance of InheritableRelation is a subclass of Relation whose
properties can be inherited downward in the class hierarchy via the
subrelation Predicate.</rdfs:comment>
</owl:Class>

<owl:Class rdf:ID= "Injecting">
<rdfs:subClassOf rdf:resource ="#Inserting"/>
<rdfs:comment>Inserting a BiologicallyActiveSubstance into an
Animal or a Human with a syringe.</rdfs:comment>
</owl:Class>

<owl:Class rdf:ID= "Injuring">
<rdfs:subClassOf rdf:resource ="#PathologicProcess"/>
<rdfs:subClassOf rdf:resource ="#Damaging"/>
<rdfs:comment>The process of creating a traumatic wound or
injury.  Since Injuring is not possible without some biologic function
of the organism being injured, it is a subclass of BiologicalProcess.</rdfs:comment>
</owl:Class>

<owl:Class rdf:ID= "Insect">
<rdfs:subClassOf rdf:resource ="#Arthropod"/>
<rdfs:comment>A Class of small Arthropods that are
air-breathing and that are distinguished by appearance.</rdfs:comment>
</owl:Class>

<owl:Class rdf:ID= "Inserting">
<rdfs:subClassOf rdf:resource ="#Putting"/>
<rdfs:comment>Putting one thing inside of another thing.</rdfs:comment>
</owl:Class>

<owl:Class rdf:ID= "Integer">
<rdfs:subClassOf rdf:resource ="#RationalNumber"/>
<rdfs:comment>A negative or nonnegative whole number.</rdfs:comment>
</owl:Class>

<owl:Class rdf:ID= "IntentionalProcess">
<rdfs:subClassOf rdf:resource ="#Process"/>
<rdfs:comment>A Process that has a specific
purpose for the CognitiveAgent who performs it.</rdfs:comment>
</owl:Class>

<owl:Class rdf:ID= "IntentionalPsychologicalProcess">
<rdfs:subClassOf rdf:resource ="#IntentionalProcess"/>
<rdfs:subClassOf rdf:resource ="#PsychologicalProcess"/>
<rdfs:comment>An IntentionalProcess that
can be realized entirely within the mind or brain of an Organism.  Thus,
for example, Reasoning is a subclass of IntentionalPsychologicalProcess,
because one can reason simply by exercising one's mind/brain.  On the other
hand, RecreationOrExercise is not a subclass of IntentionalPsychologicalProcess,
because many instances of RecreationOrExercise necessarily have subProcesses
of BodyMotion.</rdfs:comment>
</owl:Class>

<owl:Class rdf:ID= "IntentionalRelation">
<rdf:type rdf:resource = "#InheritableRelation"/>
<rdfs:comment>The Class of Relations between
an Agent and one or more Entities, where the Relation requires that
the Agent have awareness of the Entity.</rdfs:comment>
</owl:Class>



<owl:Class rdf:ID= "InternalChange">
<rdfs:subClassOf rdf:resource ="#Process"/>
<rdfs:comment>Processes which involve altering an internal
property of an Object, e.g. the shape of the Object, its coloring, its
structure, etc.  Processes that are not instances of this class include
changes that only affect the relationship to other objects, e.g. changes in
spatial or temporal location.</rdfs:comment>
</owl:Class>

<owl:Class rdf:ID= "Interpreting">
<rdfs:subClassOf rdf:resource ="#IntentionalPsychologicalProcess"/>
<rdfs:comment>Any Process of assigning a Proposition to
a Text, i.e. understanding the Text.</rdfs:comment>
</owl:Class>

<owl:Class rdf:ID= "IntransitiveRelation">
<rdfs:subClassOf rdf:resource ="#BinaryRelation"/>
<rdfs:comment>A BinaryRelation ?REL is
intransitive only if (?REL ?INST1 ?INST2) and (?REL ?INST2 ?INST3) imply not
(?REL ?INST1 ?INST3), for all ?INST1, ?INST2, and ?INST3.</rdfs:comment>
</owl:Class>

<owl:Class rdf:ID= "InvalidDeductiveArgument">
<rdfs:subClassOf rdf:resource ="#DeductiveArgument"/>
<rdfs:comment>DeductiveArguments that are not
ValidDeductiveArguments, i.e. it is not the case that the set of premises
in fact entails the conclusion.</rdfs:comment>
</owl:Class>

<owl:Class rdf:ID= "Invertebrate">
<rdfs:subClassOf rdf:resource ="#Animal"/>
<rdfs:comment>An Animal which has no spinal column.</rdfs:comment>
</owl:Class>

<owl:Class rdf:ID= "Investigating">
<rdfs:subClassOf rdf:resource ="#IntentionalPsychologicalProcess"/>
<rdfs:comment>The class of IntentionalPsychologicalProcesses
where the agent attempts to obtaina information (i.e. a Proposition denoted
by a Formula).</rdfs:comment>
</owl:Class>

<owl:Class rdf:ID= "IrrationalNumber">
<rdfs:subClassOf rdf:resource ="#RealNumber"/>
<rdfs:comment>Any RealNumber that is not also a
RationalNumber.</rdfs:comment>
</owl:Class>

<owl:Class rdf:ID= "IrreflexiveRelation">
<rdfs:subClassOf rdf:resource ="#BinaryRelation"/>
<rdfs:comment>Relation ?REL is irreflexive
if (?REL ?INST ?INST) holds for no value of ?INST.</rdfs:comment>
</owl:Class>

<owl:Class rdf:ID= "Island">
<rdfs:subClassOf rdf:resource ="#LandArea"/>
<rdfs:comment>A LandArea that is completely surrounded by a WaterArea.</rdfs:comment>
</owl:Class>

<owl:Class rdf:ID= "January">
<rdfs:subClassOf rdf:resource ="#Month"/>
<rdfs:comment>The Class of all Months which are January.</rdfs:comment>
</owl:Class>

<owl:Class rdf:ID= "JoiningAnOrganization">
<rdfs:subClassOf rdf:resource ="#OrganizationalProcess"/>
<rdfs:comment>The OrganizationalProcess of
becoming a member of an Organization.</rdfs:comment>
</owl:Class>

<owl:Class rdf:ID= "Judging">
<rdfs:subClassOf rdf:resource ="#Selecting"/>
<rdfs:comment>The subclass of Selecting where the agent opts
for one belief out of a set of multiple possibilities that are available to
him/her.</rdfs:comment>
</owl:Class>

<owl:Class rdf:ID= "JudicialOrganization">
<rdfs:subClassOf rdf:resource ="#Organization"/>
<rdfs:comment>JudicialOrganization is the class
of Organizations whose primary purpose is to render judgments according
to the statutes or regulations of a government or other organization.
Judicial bodies are not necessarily government organizations, for example,
those associated with sporting associations.</rdfs:comment>
</owl:Class>

<owl:Class rdf:ID= "JudicialProcess">
<rdfs:subClassOf rdf:resource ="#PoliticalProcess"/>
<rdfs:comment>Any legal proceeding which is conducted
by a JudicialOrganization.  Note that there is an important difference
between the concepts LegalAction and JudicialProcess.  The former
refers to legal claims that are brought by a plaintiff, e.g. law suits,
while the second refers to trials and other sorts of judicial hearings
where the merits of a LegalAction are decided.</rdfs:comment>
</owl:Class>

<owl:Class rdf:ID= "July">
<rdfs:subClassOf rdf:resource ="#Month"/>
<rdfs:comment>The Class of all Months which are July.</rdfs:comment>
</owl:Class>

<owl:Class rdf:ID= "June">
<rdfs:subClassOf rdf:resource ="#Month"/>
<rdfs:comment>The Class of all Months which are June.</rdfs:comment>
</owl:Class>

<owl:Class rdf:ID= "Keeping">
<rdfs:subClassOf rdf:resource ="#IntentionalProcess"/>
<rdfs:comment>The Class of Processes where the agent
keeps something in a particular location for an extended period of time.</rdfs:comment>
</owl:Class>

<owl:Class rdf:ID= "KelvinDegree">
<rdfs:subClassOf rdf:resource ="#TemperatureMeasure"/>
<rdf:type rdf:resource = "#SystemeInternationalUnit"/>
<rdfs:comment>SI TemperatureMeasure.  Symbol: K.
It is one of the base units in SI (it is also a unit in the ITS system).
Kelvin differs from the Celsius scale in that the triple point of water
is defined to be 273.16 KelvinDegrees while it is 0 CelsiusDegrees.
The magnitudes of intervals in the two scales are the same.  By definition
the conversion constant is 273.15.</rdfs:comment>
</owl:Class>

<owl:Class rdf:ID= "Killing">
<rdfs:subClassOf rdf:resource ="#Destruction"/>
<rdfs:comment>The subclass of Destruction in which the
death of an Organism is caused by an Organism.  Note that in cases
of suicide the Organism would be the same in both cases.</rdfs:comment>
</owl:Class>

<owl:Class rdf:ID= "KiloByte">
<rdfs:subClassOf rdf:resource ="#InformationMeasure"/>
<rdf:type rdf:resource = "#UnitOfMeasure"/>
<rdfs:comment>One KiloByte (KB) of information.  One
KiloByte is 1024 Bytes.  Note that this sense of 'kilo' is
different from the one accepted in the SI system.</rdfs:comment>
</owl:Class>

<owl:Class rdf:ID= "LandArea">
<rdfs:subClassOf rdf:resource ="#GeographicArea"/>
<rdfs:comment>An area which is predominantly solid ground,
e.g. a Nation, a mountain, a desert, etc.  Note that a LandArea may
contain some relatively small WaterAreas.  For example, Australia is
a LandArea even though it contains various rivers and lakes.</rdfs:comment>
</owl:Class>

<owl:Class rdf:ID= "LandTransitway">
<rdfs:subClassOf rdf:resource ="#Transitway"/>
<rdfs:subClassOf rdf:resource ="#LandArea"/>
<rdfs:comment>LandTransitway is the subclass of
Transitway that represents areas intended for motion over the ground.</rdfs:comment>
</owl:Class>

<owl:Class rdf:ID= "Language">
<rdfs:subClassOf rdf:resource ="#LinguisticExpression"/>
<rdfs:comment>A system of signs for expressing thought.  The
system can be either natural or artificial, i.e. something that emerges
gradually as a cultural artifact or something that is intentionally created
by a person or group of people.</rdfs:comment>
</owl:Class>

<owl:Class rdf:ID= "LeapYear">
<rdfs:subClassOf rdf:resource ="#Year"/>
<rdfs:comment>The Class of all leap years.  These are years
which are either (i.) evenly divisible by 4 and not by 100 or (ii.) evenly
divisible by 400 (this latter case is known as a leap century).</rdfs:comment>
</owl:Class>

<owl:Class rdf:ID= "Learning">
<rdfs:subClassOf rdf:resource ="#IntentionalPsychologicalProcess"/>
<rdfs:comment>The Class of Processes which relate to the
acquisition of information.</rdfs:comment>
</owl:Class>

<owl:Class rdf:ID= "LeavingAnOrganization">
<rdfs:subClassOf rdf:resource ="#OrganizationalProcess"/>
<disjoint rdf:resource = "#JoiningAnOrganization" />
<rdfs:comment>The OrganizationalProcess of
leaving an Organization, whether voluntarily or involuntarily.</rdfs:comment>
</owl:Class>

<owl:Class rdf:ID= "LegalAction">
<rdfs:subClassOf rdf:resource ="#Contest"/>
<rdfs:comment>Any Process where a CognitiveAgent seeks
to obtain something through a court of law.</rdfs:comment>
</owl:Class>

<owl:Class rdf:ID= "LegalDecision">
<rdfs:subClassOf rdf:resource ="#JudicialProcess"/>
<rdfs:subClassOf rdf:resource ="#Declaring"/>
<rdfs:comment>A decision issued by a court with respect to
a LegalAction.  Note that a LegalDecision is the act of Declaring a
decision of a court; it is not the act of judge or jury Deciding the merits
of a particular LegalAction.</rdfs:comment>
</owl:Class>

<owl:Class rdf:ID= "Lending">
<rdfs:subClassOf rdf:resource ="#Giving"/>
<rdfs:comment>The subclass of Giving Processes where
the agent gives the destination something for a limited period of
time with the expectation that it will be returned later (perhaps with
interest).</rdfs:comment>
</owl:Class>

<owl:Class rdf:ID= "LengthMeasure">
<rdfs:subClassOf rdf:resource ="#ConstantQuantity"/>
<rdfs:comment>The Class of ConstantQuantities relating
to length.</rdfs:comment>
</owl:Class>

<owl:Class rdf:ID= "LinguisticCommunication">
<rdfs:subClassOf rdf:resource ="#Communication"/>
<rdfs:comment>A Communication that involves
the transfer of information via a LinguisticExpression.</rdfs:comment>
</owl:Class>

<owl:Class rdf:ID= "LinguisticExpression">
<rdfs:subClassOf rdf:resource ="#ContentBearingObject"/>
<disjoint rdf:resource = "#Icon" />
<rdfs:comment>This is the subclass of
ContentBearingObjects which are language-related.  Note that this Class
encompasses both Language and the the elements of Languages,
e.g. Words.</rdfs:comment>
</owl:Class>

<owl:Class rdf:ID= "LiquidMixture">
<rdfs:subClassOf rdf:resource ="#Mixture"/>
<rdfs:comment>Any Mixture that satisfies two conditions,
viz. it is made up predominantly of things which are a Liquid and any
component other than Liquid in the Mixture is in the form of fine particles
which are suspended in the Liquid.</rdfs:comment>
</owl:Class>

<owl:Class rdf:ID= "LiquidMotion">
<rdfs:subClassOf rdf:resource ="#Motion"/>
<rdfs:comment>Any Motion where the patient is a
Liquid.  This class would cover, in particular, the flow of
Water.</rdfs:comment>
</owl:Class>

<owl:Class rdf:ID= "List">
<rdfs:subClassOf rdf:resource ="#Relation"/>
<rdfs:comment>Every List is a particular ordered n-tuple of
items.  Generally speaking, Lists are created by means of the ListFn
Function, which takes any number of items as arguments and returns a
List with the items in the same order.  Anything, including other
Lists, may be an item in a List.  Note too that Lists are
extensional - two lists that have the same items in the same order are
identical.  Note too that a List may contain no items.  In that case,
the List is the NullList.</rdfs:comment>
</owl:Class>

<owl:Class rdf:ID= "Listening">
<rdfs:subClassOf rdf:resource ="#Hearing"/>
<rdfs:subClassOf rdf:resource ="#IntentionalProcess"/>
<rdfs:comment>Any instance of Hearing which is intentional.</rdfs:comment>
</owl:Class>

<owl:Class rdf:ID= "Liter">
<rdfs:subClassOf rdf:resource ="#VolumeMeasure"/>
<rdf:type rdf:resource = "#UnitOfMeasure"/>
<rdfs:comment>Unit of volume in the metric system.  It is currently
defined to be equal to one cubic decimeter (0.001 cubic meter).  Symbol: l.</rdfs:comment>
</owl:Class>

<owl:Class rdf:ID= "Looking">
<rdfs:subClassOf rdf:resource ="#Seeing"/>
<rdfs:subClassOf rdf:resource ="#IntentionalProcess"/>
<rdfs:comment>Any instance of Seeing which is intentional.</rdfs:comment>
</owl:Class>

<owl:Class rdf:ID= "Machine">
<rdfs:subClassOf rdf:resource ="#Device"/>
<rdfs:comment>Machines are Devices that that have a
well-defined resource and result and that automatically convert
the resource into the result.</rdfs:comment>
</owl:Class>

<owl:Class rdf:ID= "Maintaining">
<rdfs:subClassOf rdf:resource ="#IntentionalProcess"/>
<rdfs:comment>The Class of Processes where the agent
cares for or maintains the Object.</rdfs:comment>
</owl:Class>

<owl:Class rdf:ID= "Making">
<rdfs:subClassOf rdf:resource ="#Creation"/>
<rdfs:subClassOf rdf:resource ="#IntentionalProcess"/>
<rdfs:comment>The subclass of Creation in which an individual
Artifact or a type of Artifact is made.</rdfs:comment>
</owl:Class>

<owl:Class rdf:ID= "Mammal">
<rdfs:subClassOf rdf:resource ="#WarmBloodedVertebrate"/>
<rdfs:comment>A Vertebrate having a constant body temperature
and characterized by the presence of hair, mammary glands, and sweat
glands.</rdfs:comment>
</owl:Class>

<owl:Class rdf:ID= "Man">
<rdfs:subClassOf rdf:resource ="#Human"/>
<rdfs:comment>The class of Male Humans.</rdfs:comment>
</owl:Class>

<owl:Class rdf:ID= "Managing">
<rdfs:subClassOf rdf:resource ="#OrganizationalProcess"/>
<rdfs:subClassOf rdf:resource ="#Guiding"/>
<rdfs:comment>OrganizationalProcesses that involve overseeing
the activities of others.  Note the key differences between RegulatoryProcess
and its sibling Managing.  The latter implies a long-term relationship between
the manager and the managed, while the former implies a normative standard to which
the activities of the regulated are referred.</rdfs:comment>
</owl:Class>

<owl:Class rdf:ID= "Maneuver">
<rdfs:subClassOf rdf:resource ="#IntentionalProcess"/>
<rdfs:comment>An intentional move or play within a Contest.
In many cases, a Maneuver is a realization of part of a strategy for
winning the Contest, but it also may be just an arbitrary or semi-arbitrary
division of the overarching Contest, e.g. innings in a baseball game.</rdfs:comment>
</owl:Class>

<owl:Class rdf:ID= "ManualHumanLanguage">
<rdfs:subClassOf rdf:resource ="#HumanLanguage"/>
<rdfs:comment>A ManualHumanLanguage is a
HumanLanguage which has as its medium gestures and movement, such
as the shape, position, and movement of the hands.</rdfs:comment>
</owl:Class>

<owl:Class rdf:ID= "Manufacture">
<rdfs:subClassOf rdf:resource ="#Making"/>
<rdfs:comment>The Making of Artifacts on a mass
scale.</rdfs:comment>
</owl:Class>

<owl:Class rdf:ID= "Manufacturer">
<rdfs:subClassOf rdf:resource ="#Corporation"/>
<rdfs:comment>Any Corporation which manufactures Products.</rdfs:comment>
</owl:Class>

<owl:Class rdf:ID= "March">
<rdfs:subClassOf rdf:resource ="#Month"/>
<rdfs:comment>The Class of all Months which are March.</rdfs:comment>
</owl:Class>

<owl:Class rdf:ID= "Marsupial">
<rdfs:subClassOf rdf:resource ="#Mammal"/>
<rdfs:comment>The Class of Mammals which have a pouch for
their young.</rdfs:comment>
</owl:Class>

<owl:Class rdf:ID= "MassMeasure">
<rdfs:subClassOf rdf:resource ="#ConstantQuantity"/>
<rdfs:comment>The Class of ConstantQuantities relating
to the amount of matter in an Object.</rdfs:comment>
</owl:Class>

<owl:Class rdf:ID= "Matriculation">
<rdfs:subClassOf rdf:resource ="#JoiningAnOrganization"/>
<rdfs:comment>The OrganizationalProcess of joining an
EducationalOrganization as a student.</rdfs:comment>
</owl:Class>

<owl:Class rdf:ID= "May">
<rdfs:subClassOf rdf:resource ="#Month"/>
<rdfs:comment>The Class of all Months which are May.</rdfs:comment>
</owl:Class>

<owl:Class rdf:ID= "Measuring">
<rdfs:subClassOf rdf:resource ="#Calculating"/>
<rdfs:comment>The Class of Calculating Processes where
the aim is to determine the PhysicalQuantity of some aspect of the patient.</rdfs:comment>
</owl:Class>

<owl:Class rdf:ID= "MeasuringDevice">
<rdfs:subClassOf rdf:resource ="#Device"/>
<rdfs:comment>Any Device whose purpose is to measure a
PhysicalQuantity.</rdfs:comment>
</owl:Class>

<owl:Class rdf:ID= "Meat">
<rdfs:subClassOf rdf:resource ="#Food"/>
<rdfs:comment>Any Food which was originally part of an
Animal and is not ingested by drinking, including eggs and animal
blood that is eaten as food.  Note that this class covers both raw
meat and meat that has been prepared in some way, e.g. by cooking.
Note too that preparations involving Meat and FruitOrVegetable
are classed directly under Food.</rdfs:comment>
</owl:Class>

<owl:Class rdf:ID= "Meeting">
<rdfs:subClassOf rdf:resource ="#SocialInteraction"/>
<rdfs:comment>The coming together of two or more
CognitiveAgents for the purpose of Communication.  This covers informal
meetings, e.g. visits with family members, and formal meetings, e.g. a board
of directors meeting.</rdfs:comment>
</owl:Class>

<owl:Class rdf:ID= "MegaByte">
<rdfs:subClassOf rdf:resource ="#InformationMeasure"/>
<rdf:type rdf:resource = "#UnitOfMeasure"/>
<rdfs:comment>One MegaByte (MB) of information.  One
MegaByte is 1024 KiloBytes.  Note that this sense of 'mega' is
different from the one accepted in the SI system.</rdfs:comment>
</owl:Class>

<owl:Class rdf:ID= "Melting">
<rdfs:subClassOf rdf:resource ="#StateChange"/>
<rdfs:comment>The Class of Processes where an Object is
heated and converted from a Solid to a Liquid.</rdfs:comment>
</owl:Class>

<owl:Class rdf:ID= "MercantileOrganization">
<rdfs:subClassOf rdf:resource ="#Corporation"/>
<rdfs:comment>Any Corporation which sells
goods or services to customers for a profit.</rdfs:comment>
</owl:Class>

<owl:Class rdf:ID= "Metal">
<rdfs:subClassOf rdf:resource ="#ElementalSubstance"/>
<rdfs:comment>A Metal is an ElementalSubstance that conducts heat
and electricity, is shiny and reflects many colors of light, and can be hammered
into sheets or drawn into wire.  About 80% of the known chemical elements
(ElementalSubstances) are metals.</rdfs:comment>
</owl:Class>

<owl:Class rdf:ID= "Meter">
<rdfs:subClassOf rdf:resource ="#LengthMeasure"/>
<rdf:type rdf:resource = "#SystemeInternationalUnit"/>
<rdfs:comment>SI LengthMeasure.  Symbol:  m. It is one of the
base units in SI, and it is currently defined as follows: the Meter
is the length of the path traveled by light in a vacuum during a time
interval of 1/299792458 of a SecondDuration.</rdfs:comment>
</owl:Class>

<owl:Class rdf:ID= "Microorganism">
<rdfs:subClassOf rdf:resource ="#Organism"/>
<rdfs:comment>An Organism that can be seen only with
the aid of a microscope.</rdfs:comment>
</owl:Class>

<owl:Class rdf:ID= "Mile">
<rdfs:subClassOf rdf:resource ="#LengthMeasure"/>
<rdf:type rdf:resource = "#UnitOfMeasure"/>
<rdfs:comment>English length unit of miles.</rdfs:comment>
</owl:Class>

<owl:Class rdf:ID= "MilitaryForce">
<rdfs:subClassOf rdf:resource ="#PoliticalOrganization"/>
<rdfs:comment>MilitaryForce is the subclass of
Organizations that are organized along military lines and for the
purpose of either defensive or offensive combat, whether or not
the force is an official GovernmentOrganization.</rdfs:comment>
</owl:Class>

<owl:Class rdf:ID= "MilitaryOrganization">
<rdfs:subClassOf rdf:resource ="#MilitaryForce"/>
<rdfs:subClassOf rdf:resource ="#GovernmentOrganization"/>
<rdfs:comment>Any heavily armed Organization
that is part of a Government and that is charged with representing the
Government in international conflicts.</rdfs:comment>
</owl:Class>

<owl:Class rdf:ID= "MilitaryProcess">
<rdfs:subClassOf rdf:resource ="#PoliticalProcess"/>
<rdfs:comment>Any Process that is carried out by a
military organization.  Note that this class covers Processes, e.g.
military operations, that are the result of careful planning, as well as
those which are unscripted.</rdfs:comment>
</owl:Class>

<owl:Class rdf:ID= "Mineral">
<rdfs:subClassOf rdf:resource ="#Substance"/>
<rdfs:comment> Any of various naturally occurring homogeneous substances (such as stone, coal, salt, sulfur, sand, petroleum), or synthetic substances having the chemical composition and crystalline form and properties of a naturally occurring mineral.</rdfs:comment>
</owl:Class>

<owl:Class rdf:ID= "Minute">
<rdfs:subClassOf rdf:resource ="#TimeInterval"/>
<relatedInternalConcept rdf:resource = "#MinuteFn" />
<relatedInternalConcept rdf:resource = "#MinuteDuration" />
<rdfs:comment>The Class of all clock Minutes.</rdfs:comment>
</owl:Class>

<owl:Class rdf:ID= "MinuteDuration">
<rdfs:subClassOf rdf:resource ="#TimeDuration"/>
<rdf:type rdf:resource = "#UnitOfMeasure"/>
<rdfs:comment>Time unit. 1 minute = 60 seconds. </rdfs:comment>
</owl:Class>

<owl:Class rdf:ID= "Mixture">
<rdfs:subClassOf rdf:resource ="#Substance"/>
<rdfs:comment>A Mixture is two or more PureSubstances,
combined in varying proportions - each retaining its own specific properties.
The components of a Mixture can be separated by physical means, i.e. without
the making and breaking of chemical bonds. Examples: Air, table salt thoroughly
dissolved in water, milk, wood, and concrete. </rdfs:comment>
</owl:Class>

<owl:Class rdf:ID= "Molecule">
<rdfs:subClassOf rdf:resource ="#CompoundSubstance"/>
<rdfs:comment>A molecule is the smallest unit of matter of a
CompoundSubstance that retains all the physical and chemical properties
of that substance, e.g., Ne, H2, H2O.  A molecule is two or more Atoms
linked by a chemical bond.</rdfs:comment>
</owl:Class>

<owl:Class rdf:ID= "Mollusk">
<rdfs:subClassOf rdf:resource ="#Invertebrate"/>
<rdfs:comment>Soft-bodied Invertebrate that is usually
contained in a shell.  Includes oysters, clams, mussels, snails, slugs,
octopi, and squid.</rdfs:comment>
</owl:Class>

<owl:Class rdf:ID= "Monday">
<rdfs:subClassOf rdf:resource ="#Day"/>
<rdfs:comment>The Class of all calendar Mondays.</rdfs:comment>
</owl:Class>

<owl:Class rdf:ID= "Monkey">
<rdfs:subClassOf rdf:resource ="#Primate"/>
<rdfs:comment>Various Primates with relatively long
tails.</rdfs:comment>
</owl:Class>

<owl:Class rdf:ID= "Month">
<rdfs:subClassOf rdf:resource ="#TimeInterval"/>
<relatedInternalConcept rdf:resource = "#MonthFn" />
<rdfs:comment>The Class of all calendar Months.</rdfs:comment>
</owl:Class>

<owl:Class rdf:ID= "Morpheme">
<rdfs:subClassOf rdf:resource ="#LinguisticExpression"/>
<rdfs:comment>Part of a Word which cannot be subdivided
and which expresses a meaning.</rdfs:comment>
</owl:Class>

<owl:Class rdf:ID= "Moss">
<rdfs:subClassOf rdf:resource ="#NonFloweringPlant"/>
<rdfs:comment>A NonFloweringPlant without true roots and little
if any vascular tissue.</rdfs:comment>
</owl:Class>

<owl:Class rdf:ID= "Motion">
<rdfs:subClassOf rdf:resource ="#Process"/>
<rdfs:comment>Any Process of movement.</rdfs:comment>
</owl:Class>

<owl:Class rdf:ID= "Muscle">
<rdfs:subClassOf rdf:resource ="#Tissue"/>
<rdfs:subClassOf rdf:resource ="#AnimalSubstance"/>
<rdfs:comment>Nonrigid Tissue appearing only in Animals and
composed largely of contractile cells.</rdfs:comment>
</owl:Class>

<owl:Class rdf:ID= "Music">
<rdfs:subClassOf rdf:resource ="#RadiatingSound"/>
<rdfs:comment>The subclass of RadiatingSound where the
sound is intended to be melodic and is produced deliberately.</rdfs:comment>
</owl:Class>

<owl:Class rdf:ID= "MusicalInstrument">
<rdfs:subClassOf rdf:resource ="#Device"/>
<rdfs:comment>A Device which is manipulated by a Human
and whose purpose is to produce Music.</rdfs:comment>
</owl:Class>

<owl:Class rdf:ID= "MutuallyDisjointClass">
<rdfs:subClassOf rdf:resource ="#SetOrClass"/>
<rdfs:comment>A SetOrClass is a MutuallyDisjointClass
just in case there exists nothing which is an instance of all of the instances of
the original SetOrClass.</rdfs:comment>
</owl:Class>

<owl:Class rdf:ID= "Myriapod">
<rdfs:subClassOf rdf:resource ="#Arthropod"/>
<rdfs:comment>A Class of Arthropods that includes
centipedes and millipedes.</rdfs:comment>
</owl:Class>

<owl:Class rdf:ID= "Naming">
<rdfs:subClassOf rdf:resource ="#Declaring"/>
<rdfs:comment>The Process of assigning a name to someone or something.</rdfs:comment>
</owl:Class>

<owl:Class rdf:ID= "Nation">
<rdfs:subClassOf rdf:resource ="#GeopoliticalArea"/>
<rdfs:subClassOf rdf:resource ="#LandArea"/>
<rdfs:comment>The broadest GeopoliticalArea, i.e. Nations are
GeopoliticalAreas that are not part of any other overarching and
comprehensive governance structure (excepting commonwealths and other sorts
of loose international organizations).</rdfs:comment>
</owl:Class>

<owl:Class rdf:ID= "NaturalLanguage">
<rdfs:subClassOf rdf:resource ="#HumanLanguage"/>
<rdfs:comment>The subclass of HumanLanguages which
are not designed and which evolve from generation to generation.  This
Class includes all of the national languages, e.g. English, Spanish,
Japanese, etc.  Note that this class includes dialects of natural
languages.</rdfs:comment>
</owl:Class>

<owl:Class rdf:ID= "NaturalSubstance">
<rdfs:subClassOf rdf:resource ="#Substance"/>
<rdfs:comment>Any Substance that is not the result of
an IntentionalProcess, i.e. any substance that occurs naturally.</rdfs:comment>
</owl:Class>

<owl:Class rdf:ID= "NegativeInteger">
<rdfs:subClassOf rdf:resource ="#Integer"/>
<rdfs:subClassOf rdf:resource ="#NegativeRealNumber"/>
<rdfs:comment>An Integer that is less than zero.</rdfs:comment>
</owl:Class>

<owl:Class rdf:ID= "NegativeRealNumber">
<rdfs:subClassOf rdf:resource ="#RealNumber"/>
<rdfs:comment>A RealNumber that is less than
zero.</rdfs:comment>
</owl:Class>

<owl:Class rdf:ID= "Neutron">
<rdfs:subClassOf rdf:resource ="#SubatomicParticle"/>
<rdfs:comment>Components of the AtomicNucleus.  They have no
charge.</rdfs:comment>
</owl:Class>

<owl:Class rdf:ID= "NonFloweringPlant">
<rdfs:subClassOf rdf:resource ="#Plant"/>
<disjoint rdf:resource = "#FloweringPlant" />
<rdfs:comment>A Plant that reproduces with spores and
does not produce flowers.</rdfs:comment>
</owl:Class>

<owl:Class rdf:ID= "NonNullSet">
<rdfs:subClassOf rdf:resource ="#SetOrClass"/>
<rdfs:comment>Any SetOrClass that contains at least one
instance.</rdfs:comment>
</owl:Class>

<owl:Class rdf:ID= "NonnegativeInteger">
<rdfs:subClassOf rdf:resource ="#Integer"/>
<rdfs:subClassOf rdf:resource ="#NonnegativeRealNumber"/>
<rdfs:comment>An Integer that is greater than
or equal to zero.</rdfs:comment>
</owl:Class>

<owl:Class rdf:ID= "NonnegativeRealNumber">
<rdfs:subClassOf rdf:resource ="#RealNumber"/>
<rdfs:comment>A RealNumber that is greater than
or equal to zero.</rdfs:comment>
</owl:Class>

<owl:Class rdf:ID= "NormativeAttribute">
<rdfs:subClassOf rdf:resource ="#RelationalAttribute"/>
<rdfs:comment>A Class containing all of the
Attributes that are specific to morality, legality, aesthetics,
etiquette, etc.  Many of these attributes express a judgement that
something ought or ought not to be the case.</rdfs:comment>
</owl:Class>

<owl:Class rdf:ID= "Noun">
<rdfs:subClassOf rdf:resource ="#Word"/>
<rdfs:comment>One of the parts of speech.  The Class of Words
that conventionally denote Objects.</rdfs:comment>
</owl:Class>

<owl:Class rdf:ID= "NounPhrase">
<rdfs:subClassOf rdf:resource ="#Phrase"/>
<disjoint rdf:resource = "#VerbPhrase" />
<rdfs:comment>A Phrase that has the same function as a
Noun.</rdfs:comment>
</owl:Class>

<owl:Class rdf:ID= "November">
<rdfs:subClassOf rdf:resource ="#Month"/>
<rdfs:comment>The Class of all Months which are November.</rdfs:comment>
</owl:Class>

<owl:Class rdf:ID= "NullSet">
<rdfs:subClassOf rdf:resource ="#SetOrClass"/>
<rdfs:comment>Any SetOrClass that contains no instances.</rdfs:comment>
</owl:Class>

<owl:Class rdf:ID= "Number">
<rdfs:subClassOf rdf:resource ="#Quantity"/>
<rdfs:comment>A measure of how many things there are, or how
much there is, of a certain kind.  Numbers are subclassed into
RealNumber, ComplexNumber, and ImaginaryNumber.</rdfs:comment>
</owl:Class>

<owl:Class rdf:ID= "Nutrient">
<rdfs:subClassOf rdf:resource ="#BiologicallyActiveSubstance"/>
<rdfs:comment>A BiologicallyActiveSubstance required by an Organism.
It is generally ingested as Food, and it is of primary interest because of its role
in the biologic functioning of the Organism.</rdfs:comment>
</owl:Class>

<owl:Class rdf:ID= "Object">
<rdfs:subClassOf rdf:resource ="#Physical"/>
<rdfs:comment>Corresponds roughly to the class of ordinary
objects.  Examples include normal physical objects, geographical regions,
and locations of Processes, the complement of Objects in the Physical
class.  In a 4D ontology, an Object is something whose spatiotemporal
extent is thought of as dividing into spatial parts roughly parallel to the
time-axis.</rdfs:comment>
</owl:Class>

<owl:Class rdf:ID= "ObjectAttitude">
<rdfs:subClassOf rdf:resource ="#IntentionalRelation"/>
<rdf:type rdf:resource = "#InheritableRelation"/>
<disjoint rdf:resource = "#PropositionalAttitude" />
<rdfs:comment>The Class of IntentionalRelations
where the Agent has awareness of an instance of Physical.</rdfs:comment>
</owl:Class>

<owl:Class rdf:ID= "ObjectiveNorm">
<rdfs:subClassOf rdf:resource ="#NormativeAttribute"/>
<rdfs:comment>The Class of NormativeAttributes that are
associated with an objective criterion for their attribution, i.e. there is
broad consensus about the cases where these attributes are applicable.</rdfs:comment>
</owl:Class>

<owl:Class rdf:ID= "October">
<rdfs:subClassOf rdf:resource ="#Month"/>
<rdfs:comment>The Class of all Months which are October.</rdfs:comment>
</owl:Class>

<owl:Class rdf:ID= "OddInteger">
<rdfs:subClassOf rdf:resource ="#Integer"/>
<rdfs:comment>An Integer that is not evenly divisible
by 2.</rdfs:comment>
</owl:Class>

<owl:Class rdf:ID= "Offering">
<rdfs:subClassOf rdf:resource ="#Committing"/>
<rdfs:comment>The subclass of Committing in which a CognitiveAgent offers something Physical to another agent. Offerings may be unconditional (in which case they are a promise to effect a UnilateralGiving) or conditional (in which case they are a promise to effect a Transaction of some sort).</rdfs:comment>
</owl:Class>

<owl:Class rdf:ID= "OneDimensionalFigure">
<rdfs:subClassOf rdf:resource ="#GeometricFigure"/>
<rdfs:comment>The class of GeometricFigures that
have position and an extension along a single dimension, viz. straight lines.</rdfs:comment>
</owl:Class>

<owl:Class rdf:ID= "OneToOneFunction">
<rdfs:subClassOf rdf:resource ="#UnaryFunction"/>
<rdfs:comment>The Class of UnaryFunctions which
are one to one.  A function F is one to one just in case for all X, Y in the
domain of F, if X is not identical to Y, then F(X) is not identical to F(Y).</rdfs:comment>
</owl:Class>

<owl:Class rdf:ID= "OpenTwoDimensionalFigure">
<rdfs:subClassOf rdf:resource ="#TwoDimensionalFigure"/>
<rdfs:comment>The class of TwoDimensionalFigures that
are not ClosedTwoDimensionalFigures.</rdfs:comment>
</owl:Class>

<owl:Class rdf:ID= "Ordering">
<rdfs:subClassOf rdf:resource ="#Directing"/>
<rdfs:comment>A Directing in which the receiver is
commanded to realize the content of a ContentBearingObject.  Orders
are injunctions, the disobedience of which involves sanctions, or
which express an obligation upon the part of the orderee.</rdfs:comment>
</owl:Class>

<owl:Class rdf:ID= "Organ">
<rdfs:subClassOf rdf:resource ="#BodyPart"/>
<rdfs:comment>A somewhat independent BodyPart that performs a
specialized function.  Note that this functional definition covers bodily
systems, e.g. the digestive system or the central nervous system.</rdfs:comment>
</owl:Class>

<owl:Class rdf:ID= "OrganOrTissueProcess">
<rdfs:subClassOf rdf:resource ="#AutonomicProcess"/>
<disjoint rdf:resource = "#OrganismProcess" />
<rdfs:comment>A PhysiologicProcess of a
particular Organ or Tissue.</rdfs:comment>
</owl:Class>

<owl:Class rdf:ID= "OrganicObject">
<rdfs:subClassOf rdf:resource ="#CorpuscularObject"/>
<disjoint rdf:resource = "#Artifact" />
<rdfs:comment>This class encompasses Organisms,
CorpuscularObjects that are parts of Organisms, i.e. BodyParts,
and CorpuscularObjects that are nonintentionally produced by
Organisms, e.g. ReproductiveBodies.</rdfs:comment>
</owl:Class>

<owl:Class rdf:ID= "Organism">
<rdfs:subClassOf rdf:resource ="#OrganicObject"/>
<rdfs:subClassOf rdf:resource ="#Agent"/>
<rdfs:comment>Generally, a living individual, including all
Plants and Animals.</rdfs:comment>
</owl:Class>

<owl:Class rdf:ID= "OrganismProcess">
<rdfs:subClassOf rdf:resource ="#PhysiologicProcess"/>
<rdfs:comment>A physiologic function of the
Organism as a whole, of multiple organ systems or of multiple
Organs or Tissues.</rdfs:comment>
</owl:Class>

<owl:Class rdf:ID= "Organization">
<rdfs:subClassOf rdf:resource ="#Group"/>
<rdfs:subClassOf rdf:resource ="#CognitiveAgent"/>
<rdfs:comment>An Organization is a corporate or similar
institution. The members of an Organization typically have a common
purpose or function. Note that this class also covers divisions, departments,
etc. of organizations.  For example, both the Shell Corporation and the
accounting department at Shell would both be instances of Organization.
Note too that the existence of an Organization is dependent on the existence
of at least one member (since Organization is a subclass of Collection).
Accordingly, in cases of purely legal organizations, a fictitious member
should be assumed.</rdfs:comment>
</owl:Class>

<owl:Class rdf:ID= "OrganizationalProcess">
<rdfs:subClassOf rdf:resource ="#IntentionalProcess"/>
<rdfs:comment>An IntentionalProcess that
involves an Organization.</rdfs:comment>
</owl:Class>

<owl:Class rdf:ID= "Ounce">
<rdfs:subClassOf rdf:resource ="#VolumeMeasure"/>
<rdf:type rdf:resource = "#UnitOfMeasure"/>
<rdfs:comment>English unit of volume equal to 1/8 of a
Cup.</rdfs:comment>
</owl:Class>

<owl:Class rdf:ID= "PairwiseDisjointClass">
<rdfs:subClassOf rdf:resource ="#SetOrClass"/>
<rdfs:comment>A SetOrClass is a PairwiseDisjointClass
just in case every instance of the SetOrClass is either equal to or disjoint
from every other instance of the SetOrClass.</rdfs:comment>
</owl:Class>

<owl:Class rdf:ID= "ParamilitaryOrganization">
<rdfs:subClassOf rdf:resource ="#MilitaryForce"/>
<disjoint rdf:resource = "#GovernmentOrganization" />
<rdfs:comment>An Organization which is much like
a MilitaryOrganization, e.g. it is made up of armed fighters, except that it
is not associated with a Government.</rdfs:comment>
</owl:Class>

<owl:Class rdf:ID= "PartialOrderingRelation">
<rdfs:subClassOf rdf:resource ="#TransitiveRelation"/>
<rdfs:subClassOf rdf:resource ="#AntisymmetricRelation"/>
<rdfs:subClassOf rdf:resource ="#ReflexiveRelation"/>
<rdfs:comment>A BinaryRelation is a partial
ordering if it is a ReflexiveRelation, an AntisymmetricRelation, and
a TransitiveRelation.</rdfs:comment>
</owl:Class>

<owl:Class rdf:ID= "PartialValuedRelation">
<rdfs:subClassOf rdf:resource ="#Relation"/>
<rdfs:comment>A Relation is a PartialValuedRelation
just in case it is not a TotalValuedRelation, i.e. just in case assigning values
to every argument position except the last one does not necessarily mean that there
is a value assignment for the last argument position.  Note that, if a Relation
is both a PartialValuedRelation and a SingleValuedRelation, then it is a partial
function.</rdfs:comment>
</owl:Class>

<owl:Class rdf:ID= "ParticleWord">
<rdfs:subClassOf rdf:resource ="#Word"/>
<rdfs:comment>An umbrella Class for any Word that does not
fit into the other subclasses of Word.  A ParticleWord is generally a small
term that serves a grammatical or logical function, e.g. 'and', 'of',
'since', etc.  At some point, this class might be broken up into the
subclasses 'Connective', 'Preposition', etc.  Note that the class ParticleWord
includes both personal and possessive pronouns, e.g. 'she', 'hers', 'it', 'its',
etc.</rdfs:comment>
</owl:Class>

<owl:Class rdf:ID= "Patent">
<rdfs:subClassOf rdf:resource ="#Certificate"/>
<rdfs:comment>A Certificate that expresses the content of an
invention that has been accorded legal protection by a governemental
entity.</rdfs:comment>
</owl:Class>

<owl:Class rdf:ID= "PathologicProcess">
<rdfs:subClassOf rdf:resource ="#BiologicalProcess"/>
<disjoint rdf:resource = "#PhysiologicProcess" />
<rdfs:comment>A disordered process, activity, or
state of the Organism as a whole, of a body system or systems, or of
multiple Organs or Tissues. Included here are normal responses to a
negative stimulus as well as patholologic conditions or states that are
less specific than a disease. Pathologic functions frequently have
systemic effects.</rdfs:comment>
</owl:Class>

<owl:Class rdf:ID= "Perception">
<rdfs:subClassOf rdf:resource ="#PsychologicalProcess"/>
<rdfs:comment>Sensing some aspect of the material world.
Note that the agent of this sensing is assumed to be an Animal.</rdfs:comment>
</owl:Class>

<owl:Class rdf:ID= "Periodical">
<rdfs:subClassOf rdf:resource ="#Series"/>
<rdfs:comment>A Series whose elements are published separately
and on a periodic basis.</rdfs:comment>
</owl:Class>

<owl:Class rdf:ID= "PermanentResidence">
<rdfs:subClassOf rdf:resource ="#Residence"/>
<rdfs:comment>A Residence where people live, i.e.
where people have a home.</rdfs:comment>
</owl:Class>

<owl:Class rdf:ID= "Phrase">
<rdfs:subClassOf rdf:resource ="#LinguisticExpression"/>
<rdfs:comment>A set of Words in a Language which form a unit,
i.e. express a meaning in the Language.</rdfs:comment>
</owl:Class>

<owl:Class rdf:ID= "Physical">
<rdfs:subClassOf rdf:resource ="#Entity"/>
<rdfs:comment>An entity that has a location in space-time.
Note that locations are themselves understood to have a location in
space-time.</rdfs:comment>
</owl:Class>

<owl:Class rdf:ID= "PhysicalQuantity">
<rdfs:subClassOf rdf:resource ="#Quantity"/>
<rdfs:comment>A PhysicalQuantity is a measure of
some quantifiable aspect of the modeled world, such as 'the earth's
diameter' (a constant length) and 'the stress in a loaded deformable
solid' (a measure of stress, which is a function of three spatial
coordinates).  All PhysicalQuantities are either ConstantQuantities
or FunctionQuantities.  Instances of ConstantQuantity are dependent
on a UnitOfMeasure, while instances of FunctionQuantity are
Functions that map instances of ConstantQuantity to other instances
of ConstantQuantity (e.g., TimeDependentQuantities are
FunctionQuantities).  Although the name and definition of
PhysicalQuantity is borrowed from physics, PhysicalQuantities need
not be material.  Aside from the dimensions of length, time, velocity,
etc., nonphysical dimensions such as currency are also possible.
Accordingly, amounts of money would be instances of PhysicalQuantity.
PhysicalQuantities are distinguished from Numbers by the fact that
the former are associated with a dimension of measurement.</rdfs:comment>
</owl:Class>

<owl:Class rdf:ID= "PhysicalState">
<rdfs:subClassOf rdf:resource ="#InternalAttribute"/>
<rdfs:comment>The physical state of an Object.  There
are three reified instances of this Class:  Solid, Liquid, and Gas.
Physical changes are not characterized by the transformation of one
substance into another, but rather by the change of the form (physical
states) of a given substance.  For example, melting an iron nail yields a
substance still called iron.</rdfs:comment>
</owl:Class>

<owl:Class rdf:ID= "PhysiologicProcess">
<rdfs:subClassOf rdf:resource ="#BiologicalProcess"/>
<rdfs:comment>A normal process of an Organism
or part of an Organism.</rdfs:comment>
</owl:Class>

<owl:Class rdf:ID= "DiseaseOrSyndrome">
<rdfs:subClassOf rdf:resource="#PhysiologicProcess"/>
</owl:Class>

<owl:Class rdf:ID= "Pint">
<rdfs:subClassOf rdf:resource ="#VolumeMeasure"/>
<rdf:type rdf:resource = "#UnitOfMeasure"/>
<rdfs:comment>English unit of volume equal to 1/2 of a
Quart.</rdfs:comment>
</owl:Class>

<owl:Class rdf:ID= "Plan">
<rdfs:subClassOf rdf:resource ="#Procedure"/>
<rdfs:comment>A specification of a sequence of Processes which
is intended to satisfy a specified purpose at some future time.</rdfs:comment>
</owl:Class>

<owl:Class rdf:ID= "PlaneAngleMeasure">
<rdfs:subClassOf rdf:resource ="#AngleMeasure"/>
<rdfs:comment>The value of an angle in a plane.</rdfs:comment>
</owl:Class>

<owl:Class rdf:ID= "Planning">
<rdfs:subClassOf rdf:resource ="#IntentionalPsychologicalProcess"/>
<rdfs:comment>Specifying a set of actions in order to meet a
set of goals or objectives.</rdfs:comment>
</owl:Class>

<owl:Class rdf:ID= "Plant">
<rdfs:subClassOf rdf:resource ="#Organism"/>
<rdfs:comment>An Organism having cellulose cell walls, growing
by synthesis of Substances, generally distinguished by the presence of
chlorophyll, and lacking the power of locomotion.</rdfs:comment>
</owl:Class>

<owl:Class rdf:ID= "PlantAnatomicalStructure">
<rdfs:subClassOf rdf:resource ="#AnatomicalStructure"/>
<rdfs:comment>AnatomicalStructures that
are possessed exclusively by Plants.</rdfs:comment>
</owl:Class>

<owl:Class rdf:ID= "PlantSubstance">
<rdfs:subClassOf rdf:resource ="#BodySubstance"/>
<rdfs:comment>BodySubstances that are produced
exclusively by Plants.</rdfs:comment>
</owl:Class>

<owl:Class rdf:ID= "Poking">
<rdfs:subClassOf rdf:resource ="#IntentionalProcess"/>
<rdfs:comment>The Class of Processes where the agent
pierces the surface of the Object with an instrument.</rdfs:comment>
</owl:Class>

<owl:Class rdf:ID= "PoliceOrganization">
<rdfs:subClassOf rdf:resource ="#GovernmentOrganization"/>
<rdfs:comment>Any GovernmentOrganization
that is charged with domestic enforcement of the laws of the Government.</rdfs:comment>
</owl:Class>

<owl:Class rdf:ID= "PoliticalOrganization">
<rdfs:subClassOf rdf:resource ="#Organization"/>
<rdfs:comment>An Organization that is a subOrganization
of a Government, or an Organization that is attempting to bring about some sort
of political change.</rdfs:comment>
</owl:Class>

<owl:Class rdf:ID= "PoliticalProcess">
<rdfs:subClassOf rdf:resource ="#OrganizationalProcess"/>
<rdfs:comment>An OrganizationalProcess carried
out by, for or against officially constituted governments.  Some examples
would be voting on proposed legislation, electing a government representative,
or even overthrowing a government in a revolution.</rdfs:comment>
</owl:Class>

<owl:Class rdf:ID= "Pollen">
<rdfs:subClassOf rdf:resource ="#ReproductiveBody"/>
<rdfs:subClassOf rdf:resource ="#PlantAnatomicalStructure"/>
<rdfs:comment>A powder produced by FloweringPlants that contains male
gametes and is capable of fertilizing the seeds of FloweringPlants of the same
species.</rdfs:comment>
</owl:Class>

<owl:Class rdf:ID= "Position">
<rdfs:subClassOf rdf:resource ="#SocialRole"/>
<rdfs:comment>A formal position of reponsibility within an
Organization. Examples of Positions include president, laboratory
director, senior researcher, sales representative, etc.</rdfs:comment>
</owl:Class>

<owl:Class rdf:ID= "PositionalAttribute">
<rdfs:subClassOf rdf:resource ="#RelationalAttribute"/>
<rdfs:comment>Attributes characterizing the
orientation of an Object, e.g. Vertical versus Horizontal, Left
versus Right etc.</rdfs:comment>
</owl:Class>

<owl:Class rdf:ID= "PositiveInteger">
<rdfs:subClassOf rdf:resource ="#NonnegativeInteger"/>
<rdfs:subClassOf rdf:resource ="#PositiveRealNumber"/>
<rdfs:comment>An Integer that is greater than zero.</rdfs:comment>
</owl:Class>

<owl:Class rdf:ID= "PositiveRealNumber">
<rdfs:subClassOf rdf:resource ="#NonnegativeRealNumber"/>
<rdfs:comment>A RealNumber that is greater than
zero.</rdfs:comment>
</owl:Class>

<owl:Class rdf:ID= "PoundMass">
<rdfs:subClassOf rdf:resource ="#MassMeasure"/>
<rdf:type rdf:resource = "#UnitOfMeasure"/>
<rdfs:comment>English mass unit of pounds.</rdfs:comment>
</owl:Class>

<owl:Class rdf:ID= "Precipitation">
<rdfs:subClassOf rdf:resource ="#WeatherProcess"/>
<rdfs:comment>Precipitation is the process of
water molecules falling from the air to the ground, in either a
liquid or frozen state.</rdfs:comment>
</owl:Class>

<owl:Class rdf:ID= "Predicate">
<rdfs:subClassOf rdf:resource ="#Relation"/>
<rdf:type rdf:resource = "#InheritableRelation"/>
<rdfs:comment>A Predicate is a sentence-forming Relation.
Each tuple in the Relation is a finite, ordered sequence of objects.
The fact that a particular tuple is an element of a Predicate is denoted
by '(*predicate* arg_1 arg_2 .. arg_n)', where the arg_i are the
objects so related.  In the case of BinaryPredicates, the fact can
be read as `arg_1 is *predicate* arg_2' or `a *predicate* of
arg_1 is arg_2'.</rdfs:comment>
</owl:Class>

<owl:Class rdf:ID= "Predicting">
<rdfs:subClassOf rdf:resource ="#IntentionalPsychologicalProcess"/>
<rdfs:comment>The Class of IntentionalPsychologicalProcesses
which involve the formulation of a Proposition about a state of affairs
which might be realized in the future.</rdfs:comment>
</owl:Class>

<owl:Class rdf:ID= "PrepositionalPhrase">
<rdfs:subClassOf rdf:resource ="#Phrase"/>
<rdfs:comment>A Phrase that begins with a
preposition and that functions as an Adjective or an Adverb.</rdfs:comment>
</owl:Class>

<owl:Class rdf:ID= "Pretending">
<rdfs:subClassOf rdf:resource ="#SocialInteraction"/>
<rdfs:comment>Any SocialInteraction where a
CognitiveAgent or Group of CognitiveAgents attempts to make
another CognitiveAgent or Group of CognitiveAgents believe
something that is false.  This covers deceit, affectation,
impersonation, and entertainment productions, to give just a few
examples.</rdfs:comment>
</owl:Class>



<owl:Class rdf:ID= "Primate">
<rdfs:subClassOf rdf:resource ="#Mammal"/>
<rdfs:comment>The Class of Mammals which are
Primates.</rdfs:comment>
</owl:Class>

<owl:Class rdf:ID= "PrimeNumber">
<rdfs:subClassOf rdf:resource ="#Integer"/>
<rdfs:comment>An Integer that is evenly divisible only
by itself and 1.</rdfs:comment>
</owl:Class>

<owl:Class rdf:ID= "ProbabilityAttribute">
<rdfs:subClassOf rdf:resource ="#ObjectiveNorm"/>
<rdfs:comment>A class containing all of the Attributes
relating to objective, qualitative assessments of probability, e.g. Likely and
Unlikely.</rdfs:comment>
</owl:Class>

<owl:Class rdf:ID= "ProbabilityRelation">
<rdfs:subClassOf rdf:resource ="#Relation"/>
<rdf:type rdf:resource = "#InheritableRelation"/>
<rdfs:comment>The Class of Relations that
permit assessment of the probability of an event or situation.</rdfs:comment>
</owl:Class>

<owl:Class rdf:ID= "Procedure">
<rdfs:subClassOf rdf:resource ="#Proposition"/>
<rdfs:comment>A sequence-dependent specification.  Some
examples are ComputerPrograms, finite-state machines, cooking recipes,
musical scores, conference schedules, driving directions, and the scripts
of plays and movies.</rdfs:comment>
</owl:Class>

<owl:Class rdf:ID= "Process">
<rdfs:subClassOf rdf:resource ="#Physical"/>
<rdfs:comment>Intuitively, the class of things that happen
and have temporal parts or stages.  Examples include extended events
like a football match or a race, actions like Pursuing and Reading,
and biological processes. The formal definition is: anything that lasts
for a time but is not an Object.  Note that a Process may have
participants 'inside' it which are Objects, such as the players
in a football match.  In a 4D ontology, a Process is something whose
spatiotemporal extent is thought of as dividing into temporal stages
roughly perpendicular to the time-axis.</rdfs:comment>
</owl:Class>

<owl:Class rdf:ID= "Product">
<rdfs:subClassOf rdf:resource ="#Artifact"/>
<rdfs:comment>An Artifact that is produced by Manufacture and
that is intended to be sold.</rdfs:comment>
</owl:Class>

<owl:Class rdf:ID= "Proposition">
<rdfs:subClassOf rdf:resource ="#Abstract"/>
<rdfs:comment>Propositions are Abstract entities that
express a complete thought or a set of such thoughts.  As an example,
the formula '(instance Yojo Cat)' expresses the Proposition that the
entity named Yojo is an element of the Class of Cats.  Note that
propositions are not restricted to the content expressed by individual
sentences of a Language.  They may encompass the content expressed by
theories, books, and even whole libraries.  It is important to distinguish
Propositions from the ContentBearingObjects that express them.  A
Proposition is a piece of information, e.g. that the cat is on the mat,
but a ContentBearingObject is an Object that represents this information.
A Proposition is an abstraction that may have multiple representations:
strings, sounds, icons, etc.  For example, the Proposition that the cat is
on the mat is represented here as a string of graphical characters displayed
on a monitor and/or printed on paper, but it can be represented by a sequence
of sounds or by some non-latin alphabet or by some cryptographic form</rdfs:comment>
</owl:Class>

<owl:Class rdf:ID= "PropositionalAttitude">
<rdfs:subClassOf rdf:resource ="#IntentionalRelation"/>
<rdfs:subClassOf rdf:resource ="#AsymmetricRelation"/>
<rdf:type rdf:resource = "#InheritableRelation"/>
<rdfs:comment>The Class of
IntentionalRelations where the Agent has awareness of a
Proposition.</rdfs:comment>
</owl:Class>

<owl:Class rdf:ID= "Protein">
<rdfs:subClassOf rdf:resource ="#Nutrient"/>
<rdfs:comment>A Nutrient made up of amino acids joined by
peptide bonds.</rdfs:comment>
</owl:Class>

<owl:Class rdf:ID= "Proton">
<rdfs:subClassOf rdf:resource ="#SubatomicParticle"/>
<rdfs:comment>Components of the AtomicNucleus.  They have a
positive charge.</rdfs:comment>
</owl:Class>





<owl:Class rdf:ID= "PsychologicalProcess">
<rdfs:subClassOf rdf:resource ="#BiologicalProcess"/>
<rdfs:comment>A BiologicalProcess which takes place in
the mind or brain of an Organism and which may be manifested in the behavior
of the Organism.</rdfs:comment>
</owl:Class>

<owl:Class rdf:ID= "Publication">
<rdfs:subClassOf rdf:resource ="#Manufacture"/>
<rdfs:subClassOf rdf:resource ="#ContentDevelopment"/>
<rdfs:comment>The Manufacture of Texts.  Note that
there is no implication that the Texts are distributed.  Such
distribution, when it occurs, is an instance of Dissemination.</rdfs:comment>
</owl:Class>

<owl:Class rdf:ID= "PureSubstance">
<rdfs:subClassOf rdf:resource ="#Substance"/>
<rdfs:comment>The Class of Substances with constant
composition.  A PureSubstance can be either an element (ElementalSubstance)
or a compound of elements (CompoundSubstance).  Examples: Table salt
(sodium chloride, NaCl), sugar (sucrose, C_{12}H_{22}O_{11}), water (H_2O),
iron (Fe), copper (Cu), and oxygen (O_2).</rdfs:comment>
</owl:Class>

<owl:Class rdf:ID= "Pursuing">
<rdfs:subClassOf rdf:resource ="#IntentionalProcess"/>
<rdfs:comment>The class of IntentionalProcesses where something is
sought.  Some examples would be hunting, shopping, trawling, and stalking.</rdfs:comment>
</owl:Class>

<owl:Class rdf:ID= "Putting">
<rdfs:subClassOf rdf:resource ="#Transfer"/>
<rdfs:comment>The Class of Processes where something is put
in a location.  Note that the location is specified with the CaseRole
destination.</rdfs:comment>
</owl:Class>

<owl:Class rdf:ID= "Quantity">
<rdfs:subClassOf rdf:resource ="#Abstract"/>
<rdfs:comment>Any specification of how many or how much of
something there is.  Accordingly, there are two subclasses of Quantity:
Number (how many) and PhysicalQuantity (how much).</rdfs:comment>
</owl:Class>

<owl:Class rdf:ID= "QuantityChange">
<rdfs:subClassOf rdf:resource ="#InternalChange"/>
<rdfs:comment>Any InternalChange where a PhysicalQuantity
associated with the patient is altered.</rdfs:comment>
</owl:Class>

<owl:Class rdf:ID= "Quart">
<rdfs:subClassOf rdf:resource ="#VolumeMeasure"/>
<rdf:type rdf:resource = "#UnitOfMeasure"/>
<rdfs:comment>English unit of volume equal to 1/4 of a
UnitedStatesGallon.</rdfs:comment>
</owl:Class>

<owl:Class rdf:ID= "QuaternaryFunction">
<rdfs:subClassOf rdf:resource ="#Function"/>
<rdfs:subClassOf rdf:resource ="#QuintaryRelation"/>
<rdf:type rdf:resource = "#InheritableRelation"/>
<rdfs:comment>The Class of Functions that require
exactly four arguments.</rdfs:comment>
</owl:Class>

<owl:Class rdf:ID= "QuaternaryPredicate">
<rdfs:subClassOf rdf:resource ="#Predicate"/>
<rdfs:subClassOf rdf:resource ="#QuaternaryRelation"/>
<rdf:type rdf:resource = "#InheritableRelation"/>
<rdfs:comment>The Class of Predicates that
require four arguments.</rdfs:comment>
</owl:Class>

<owl:Class rdf:ID= "QuaternaryRelation">
<rdfs:subClassOf rdf:resource ="#Relation"/>
<rdf:type rdf:resource = "#InheritableRelation"/>
<rdfs:comment>QuaternaryRelations relate four
items.  The two subclasses of QuaternaryRelation are
QuaternaryPredicate and TernaryFunction.</rdfs:comment>
</owl:Class>

<owl:Class rdf:ID= "Questioning">
<rdfs:subClassOf rdf:resource ="#Directing"/>
<rdfs:comment>A request for information.  For example, John asked
Bill if the President had said anything about taxes in his State of the Union
address.</rdfs:comment>
</owl:Class>

<owl:Class rdf:ID= "QuintaryPredicate">
<rdfs:subClassOf rdf:resource ="#Predicate"/>
<rdfs:subClassOf rdf:resource ="#QuintaryRelation"/>
<rdf:type rdf:resource = "#InheritableRelation"/>
<rdfs:comment>The Class of Predicates that
require five arguments.</rdfs:comment>
</owl:Class>

<owl:Class rdf:ID= "QuintaryRelation">
<rdfs:subClassOf rdf:resource ="#Relation"/>
<rdf:type rdf:resource = "#InheritableRelation"/>
<rdfs:comment>QuintaryRelations relate five items.
The two subclasses of QuintaryRelation are QuintaryPredicate and
QuaternaryFunction.</rdfs:comment>
</owl:Class>

<owl:Class rdf:ID= "Radian">
<rdfs:subClassOf rdf:resource ="#PlaneAngleMeasure"/>
<rdf:type rdf:resource = "#SystemeInternationalUnit"/>
<rdfs:comment>SI plane angle measure.  Symbol: rad.  It is the
angle of a circle subtended by an arc equal in length to the circle's
radius. Another definition is:  the plane angle between two radii of a
circle which cut off on the circumference an arc equal in length to the
radius.  Radian = m/m = 1.</rdfs:comment>
</owl:Class>

<owl:Class rdf:ID= "Radiating">
<rdfs:subClassOf rdf:resource ="#Motion"/>
<rdfs:comment>Processes in which some form of electromagnetic
radiation, e.g. radio waves, light waves, electrical energy, etc., is given
off or absorbed by something else.</rdfs:comment>
</owl:Class>

<owl:Class rdf:ID= "RadiatingLight">
<rdfs:subClassOf rdf:resource ="#Radiating"/>
<rdfs:comment>The subclass of Radiating in which
light is given off or absorbed.  Some examples include blinking, flashing,
and glittering.</rdfs:comment>
</owl:Class>

<owl:Class rdf:ID= "RadiatingNuclear">
<rdfs:subClassOf rdf:resource ="#Radiating"/>
<rdfs:comment>Releasing atomic energy, i.e. energy from
a nuclear reaction.</rdfs:comment>
</owl:Class>

<owl:Class rdf:ID= "RadiatingSound">
<rdfs:subClassOf rdf:resource ="#Radiating"/>
<rdfs:comment>The subclass of Radiating in which
sound waves are given off or absorbed.  Some examples include creaking,
roaring, and whistling.</rdfs:comment>
</owl:Class>

<owl:Class rdf:ID= "RankineDegree">
<rdfs:subClassOf rdf:resource ="#TemperatureMeasure"/>
<rdf:type rdf:resource = "#UnitOfMeasure"/>
<rdfs:comment>A TemperatureMeasure.  Note
that 0 RankineDegrees is the same as the absolute zero (i.e. 0
KelvinDegrees).</rdfs:comment>
</owl:Class>

<owl:Class rdf:ID= "RationalNumber">
<rdfs:subClassOf rdf:resource ="#RealNumber"/>
<rdfs:comment>Any RealNumber that is the product of
dividing two Integers.</rdfs:comment>
</owl:Class>

<owl:Class rdf:ID= "Reading">
<rdfs:subClassOf rdf:resource ="#ContentDevelopment"/>
<relatedInternalConcept rdf:resource = "#Interpreting" />
<rdfs:comment>A subclass of ContentDevelopment in which
content is converted from a written form into a spoken representation.
Note that the class Interpreting should be used in cases where a
Text is read silently.</rdfs:comment>
</owl:Class>

<owl:Class rdf:ID= "RealNumber">
<rdfs:subClassOf rdf:resource ="#Number"/>
<rdfs:comment>Any Number that can be expressed as a
(possibly infinite) decimal, i.e. any Number that has a position
on the number line.</rdfs:comment>
</owl:Class>

<owl:Class rdf:ID= "Reasoning">
<rdfs:subClassOf rdf:resource ="#IntentionalPsychologicalProcess"/>
<rdfs:comment>The Class of IntentionalPsychologicalProcesses
which involve concluding, on the basis of either deductive or inductive
evidence, that a particular Proposition or Sentence is true.</rdfs:comment>
</owl:Class>

<owl:Class rdf:ID= "RecreationOrExercise">
<rdfs:subClassOf rdf:resource ="#IntentionalProcess"/>
<rdfs:comment>A Process that is carried out for
the purpose of recreation or exercise.  Since RecreationOrExercise is a
subclass of IntentionalProcess, the intent of a process determines whether
or not it is an instance of the class.  Hence, if John and Bill watch the same
program on television, and John watches it to relax while Bill watches it solely
to satisfy an educational requirement, then John's watching the movie is an
instance of RecreationOrExercise, while Bill's is not (both cases of
watching the television program would however be in the class of Seeing, since
being an instance of this latter class is not determined by intention).</rdfs:comment>
</owl:Class>

<owl:Class rdf:ID= "ReflexiveRelation">
<rdfs:subClassOf rdf:resource ="#BinaryRelation"/>
<rdfs:comment>Relation ?REL is reflexive if
(?REL ?INST ?INST) for all ?INST.</rdfs:comment>
</owl:Class>

<owl:Class rdf:ID= "Region">
<rdfs:subClassOf rdf:resource ="#Object"/>
<rdfs:comment>A topographic location.  Regions encompass
surfaces of Objects, imaginary places, and GeographicAreas.  Note
that a Region is the only kind of Object which can be located at
itself.  Note too that Region is not a subclass of SelfConnectedObject,
because some Regions, e.g. archipelagos, have parts which are not
connected with one another.</rdfs:comment>
</owl:Class>

<owl:Class rdf:ID= "RegulatoryProcess">
<rdfs:subClassOf rdf:resource ="#Guiding"/>
<rdfs:comment>an Guiding whose aim is the enforcement
of rules or regulations.  Note the key differences between RegulatoryProcess
and the related concept Managing.  The latter implies a long-term relationship
between a single manager and limited number of agents who are managed, while the
former implies a normative standard to which the activities of the regulated are
referred.</rdfs:comment>
</owl:Class>

<owl:Class rdf:ID= "Relation">
<rdfs:subClassOf rdf:resource ="#Abstract"/>
<rdfs:comment>The Class of relations.  There are three kinds
of Relation:  Predicate, Function, and List.  Predicates and
Functions both denote sets of ordered n-tuples.  The difference between
these two Classes is that Predicates cover formula-forming operators, while
Functions cover term-forming operators.  A List, on the other hand, is a
particular ordered n-tuple.</rdfs:comment>
</owl:Class>

<owl:Class rdf:ID= "RelationExtendedToQuantities">
<rdfs:subClassOf rdf:resource ="#Relation"/>
<rdf:type rdf:resource = "#InheritableRelation"/>
<rdfs:comment>A
RelationExtendedToQuantities is a Relation that, when it is true on
a sequence of arguments that are RealNumbers, it is also true on a
sequence of ConstantQuantites with those magnitudes in some unit of
measure.  For example, the lessThan relation is extended to quantities.
This means that for all pairs of quantities ?QUANTITY1 and ?QUANTITY2,
(lessThan ?QUANTITY1 ?QUANTITY2) if and only if, for some ?NUMBER1,
?NUMBER2, and ?UNIT, ?QUANTITY1 = (MeasureFn ?NUMBER1 ?UNIT),
?QUANTITY2 = (MeasureFn ?NUMBER2 ?UNIT), and (lessThan ?NUMBER1 ?NUMBER2),
for all units ?UNIT on which ?QUANTITY1 and ?QUANTITY2 can be measured.
Note that, when a RelationExtendedToQuantities is extended from
RealNumbers to ConstantQuantities, the ConstantQuantities must be
measured along the same physical dimension.</rdfs:comment>
</owl:Class>

<owl:Class rdf:ID= "RelationalAttribute">
<rdfs:subClassOf rdf:resource ="#Attribute"/>
<rdfs:comment>Any Attribute that an Entity has by
virtue of a relationship that it bears to another Entity or set of Entities,
e.g. SocialRoles and PositionalAttributes.</rdfs:comment>
</owl:Class>

<owl:Class rdf:ID= "ReligiousOrganization">
<rdfs:subClassOf rdf:resource ="#Organization"/>
<rdfs:subClassOf rdf:resource ="#BeliefGroup"/>
<rdfs:comment>An Organization whose members
share a set of religious beliefs.</rdfs:comment>
</owl:Class>

<owl:Class rdf:ID= "ReligiousProcess">
<rdfs:subClassOf rdf:resource ="#OrganizationalProcess"/>
<rdfs:comment>An OrganizationalProcess that is
carried out within or by a ReligiousOrganization.</rdfs:comment>
</owl:Class>

<owl:Class rdf:ID= "Remembering">
<rdfs:subClassOf rdf:resource ="#PsychologicalProcess"/>
<rdfs:comment>The Class of PsychologicalProcesses which
involve the recollection of prior experiences and/or of knowledge
which was previously acquired.</rdfs:comment>
</owl:Class>

<owl:Class rdf:ID= "Removing">
<rdfs:subClassOf rdf:resource ="#Transfer"/>
<rdfs:comment>The Class of Processes where something is
taken away from a location.  Note that the thing removed and the location
are specified with the CaseRoles patient and origin, respectively.</rdfs:comment>
</owl:Class>

<owl:Class rdf:ID= "Repairing">
<rdfs:subClassOf rdf:resource ="#IntentionalProcess"/>
<relatedInternalConcept rdf:resource = "#Maintaining" />
<rdfs:comment>The Class of Processes where the agent
makes a modification or series of modifications to an Object that is not
functioning as intended so that it works properly.</rdfs:comment>
</owl:Class>

<owl:Class rdf:ID= "Replication">
<rdfs:subClassOf rdf:resource ="#OrganismProcess"/>
<rdfs:comment>The Process of biological reproduction.
This can be either a sexual or an asexual process.</rdfs:comment>
</owl:Class>

<owl:Class rdf:ID= "RepresentationalArtWork">
<rdfs:subClassOf rdf:resource ="#ArtWork"/>
<rdfs:subClassOf rdf:resource ="#Icon"/>
<rdfs:comment>Any ArtWork that represents
something Physical.</rdfs:comment>
</owl:Class>

<owl:Class rdf:ID= "ReproductiveBody">
<rdfs:subClassOf rdf:resource ="#BodyPart"/>
<rdfs:comment>Reproductive structure of Organisms.
Consists of an Embryonic Object and a nutritive/protective envelope.
Note that this class includes seeds, spores, and FruitOrVegetables, as
well as the eggs produced by Animals.</rdfs:comment>
</owl:Class>

<owl:Class rdf:ID= "Reptile">
<rdfs:subClassOf rdf:resource ="#ColdBloodedVertebrate"/>
<rdfs:comment>A ColdBloodedVertebrate having an external
covering of scales or horny plates.  Reptiles breathe by means of
Lungs and generally lay eggs.</rdfs:comment>
</owl:Class>

<owl:Class rdf:ID= "Requesting">
<rdfs:subClassOf rdf:resource ="#Directing"/>
<rdfs:comment>A request expresses a desire that some future
action be performed.  For example, the 5th Battalion requested air support
from the 3rd Bomber Group.  Note that this class covers proposals,
recommendations, suggestions, etc.</rdfs:comment>
</owl:Class>

<owl:Class rdf:ID= "Residence">
<rdfs:subClassOf rdf:resource ="#StationaryArtifact"/>
<rdfs:comment>A Building or part of a Building which provides
some accomodation for sleeping.</rdfs:comment>
</owl:Class>

<owl:Class rdf:ID= "ResidentialBuilding">
<rdfs:subClassOf rdf:resource ="#Building"/>
<rdfs:subClassOf rdf:resource ="#Residence"/>
<rdfs:comment>A Building which provides some
accomodation for sleeping.  Note that this class does not cover just
permanent residences, e.g. Houses and condominium and apartment buildings,
but also temporary residences, e.g. hotels and dormitories.
ResidentialBuildings are also distinguished from CommercialBuildings,
which are intended to serve an organizational rather than a residential
function.</rdfs:comment>
</owl:Class>

<owl:Class rdf:ID= "Roadway">
<rdfs:subClassOf rdf:resource ="#LandTransitway"/>
<rdfs:comment>Roadway is the subclass of LandTransitways
that are areas intended for surface travel by self-powered, wheeled
vehicles, excluding those that travel on tracks.  Roadways have been
at least minimally improved to enable the passage of vehicles.
Roadways include dirt and gravelled roads, paved streets, and
expressways.</rdfs:comment>
</owl:Class>

<owl:Class rdf:ID= "Rodent">
<rdfs:subClassOf rdf:resource ="#Mammal"/>
<rdfs:comment>The Class of Mammals with one or two pairs
of incisors for gnawing.  Includes rats, mice, guinea pigs, and
rabbits.</rdfs:comment>
</owl:Class>

<owl:Class rdf:ID= "Room">
<rdfs:subClassOf rdf:resource ="#StationaryArtifact"/>
<disjoint rdf:resource = "#Building" />
<rdfs:comment>A properPart of a Building which is separated from
the exterior of the Building and/or other Rooms of the Building by walls.
Some Rooms may have a specific purpose, e.g. sleeping, bathing, cooking,
entertainment, etc.</rdfs:comment>
</owl:Class>

<owl:Class rdf:ID= "Running">
<rdfs:subClassOf rdf:resource ="#Ambulating"/>
<rdfs:comment>Ambulating relatively quickly, i.e. moving in such a
way that, with each step, neither foot is in contact with the ground for a
period of time.</rdfs:comment>
</owl:Class>

<owl:Class rdf:ID= "SaltWaterArea">
<rdfs:subClassOf rdf:resource ="#WaterArea"/>
<disjoint rdf:resource = "#FreshWaterArea" />
<rdfs:comment>A WaterArea whose Water is saline, e.g.
oceans and seas.</rdfs:comment>
</owl:Class>

<owl:Class rdf:ID= "SaturationAttribute">
<rdfs:subClassOf rdf:resource ="#InternalAttribute"/>
<rdfs:comment>A Class of Attributes that specify, in
a qualitative manner, the extent of the presence of one kind of Object in
another kind of Object.</rdfs:comment>
</owl:Class>

<owl:Class rdf:ID= "Saturday">
<rdfs:subClassOf rdf:resource ="#Day"/>
<rdfs:comment>The Class of all calendar Saturdays.</rdfs:comment>
</owl:Class>

<owl:Class rdf:ID= "Second">
<rdfs:subClassOf rdf:resource ="#TimeInterval"/>
<relatedInternalConcept rdf:resource = "#SecondDuration" />
<relatedInternalConcept rdf:resource = "#SecondFn" />
<rdfs:comment>The Class of all clock Seconds.</rdfs:comment>
</owl:Class>

<owl:Class rdf:ID= "SecondDuration">
<rdfs:subClassOf rdf:resource ="#TimeDuration"/>
<rdf:type rdf:resource = "#SystemeInternationalUnit"/>
<rdfs:comment>SI TimeDuration.  Symbol: s.
It is one of the base units in SI, and it is currently defined as
follows: the SecondDuration is the duration of 9192631770 periods of
the radiation corresponding to the transition between the two hyperfine
levels of the ground state of the cesium 133 atom.</rdfs:comment>
</owl:Class>

<owl:Class rdf:ID= "Seed">
<rdfs:subClassOf rdf:resource ="#ReproductiveBody"/>
<rdfs:subClassOf rdf:resource ="#PlantAnatomicalStructure"/>
<rdfs:comment>The fertilized or unfertilized female ReproductiveBody
of a FloweringPlant.</rdfs:comment>
</owl:Class>

<owl:Class rdf:ID= "Seeing">
<rdfs:subClassOf rdf:resource ="#Perception"/>
<rdfs:comment>The subclass of Perception in which the
sensing is done by an ocular Organ.</rdfs:comment>
</owl:Class>

<owl:Class rdf:ID= "Selecting">
<rdfs:subClassOf rdf:resource ="#IntentionalPsychologicalProcess"/>
<rdfs:comment>The Class of IntentionalPsychologicalProcesses
which involve opting for one or more Entity out of a larger set of Entities.
Note that this covers all cases of judging or evaluating.</rdfs:comment>
</owl:Class>

<owl:Class rdf:ID= "SelfConnectedObject">
<rdfs:subClassOf rdf:resource ="#Object"/>
<rdfs:comment>A SelfConnectedObject is any
Object that does not consist of two or more disconnected parts.</rdfs:comment>
</owl:Class>

<owl:Class rdf:ID= "Selling">
<rdfs:subClassOf rdf:resource ="#FinancialTransaction"/>
<rdfs:comment>A FinancialTransaction in which an instance of
Physical is exchanged for an instance of CurrencyMeasure.</rdfs:comment>
</owl:Class>

<owl:Class rdf:ID= "Sentence">
<rdfs:subClassOf rdf:resource ="#LinguisticExpression"/>
<rdfs:comment>A syntactically well-formed formula of a
Language.  It includes, at minimum, a predicate and a subject (which
may be explicit or implicit), and it expresses a Proposition.</rdfs:comment>
</owl:Class>

<owl:Class rdf:ID= "SentientAgent">
<rdfs:subClassOf rdf:resource ="#Agent"/>
<rdfs:comment>An Agent that has rights but may or may
not have responsibilities and the ability to reason.  If the latter are
present, then the Agent is also an instance of CognitiveAgent.
Domesticated animals are an example of SentientAgents that are not
also CognitiveAgents.</rdfs:comment>
</owl:Class>

<owl:Class rdf:ID= "Separating">
<rdfs:subClassOf rdf:resource ="#DualObjectProcess"/>
<disjoint rdf:resource = "#Combining" />
<rdfs:comment>A Process where a SelfConnectedObject is
separated into (some of) its parts.  Note that Separating is different
from Detaching in that the latter only results in the two objects not
being connected.  Note too that Separating is different from
Removing in that one or both of the two things which are separated
may or may not be moved from the location where they were separated.</rdfs:comment>
</owl:Class>

<owl:Class rdf:ID= "September">
<rdfs:subClassOf rdf:resource ="#Month"/>
<rdfs:comment>The Class of all Months which are September.</rdfs:comment>
</owl:Class>

<owl:Class rdf:ID= "SequenceFunction">
<rdfs:subClassOf rdf:resource ="#OneToOneFunction"/>
<rdfs:comment>The Class of OneToOneFunctions whose range
is a subclass of the PositiveIntegers.</rdfs:comment>
</owl:Class>

<owl:Class rdf:ID= "Series">
<rdfs:subClassOf rdf:resource ="#Text"/>
<rdfs:comment>A Text consisting of multiple self-contained units.
Some examples are an encyclopedia containing a couple dozen volumes, a television
series made up of many episodes, a film serial, etc.</rdfs:comment>
</owl:Class>

<owl:Class rdf:ID= "Set">
<rdfs:subClassOf rdf:resource ="#SetOrClass"/>
<rdfs:comment>A SetOrClass that satisfies extensionality as well as
other constraints specified by some choice of set theory.  Sets differ
from Classes in two important respects.  First, Sets are extensional -
two Sets with the same elements are identical.  Second, a Set can be
an arbitrary stock of objects.  That is, there is no requirement that Sets
have an associated condition that determines their membership.  Note that Sets
are not assumed to be unique sets, i.e. elements of a Set may occur more
than once in the Set.</rdfs:comment>
</owl:Class>

<owl:Class rdf:ID= "SetOrClass">
<rdfs:subClassOf rdf:resource ="#Abstract"/>
<rdfs:comment>The SetOrClass of Sets and Classes, i.e. any instance
of Abstract that has elements or instances.</rdfs:comment>
</owl:Class>

<owl:Class rdf:ID= "SexualReproduction">
<rdfs:subClassOf rdf:resource ="#Replication"/>
<disjoint rdf:resource = "#AsexualReproduction" />
<rdfs:comment>Sexual Processes of biological
reproduction.</rdfs:comment>
</owl:Class>

<owl:Class rdf:ID= "ShapeAttribute">
<rdfs:subClassOf rdf:resource ="#InternalAttribute"/>
<rdfs:comment>Any Attribute that relates to the
shape of an Object.</rdfs:comment>
</owl:Class>

<owl:Class rdf:ID= "ShapeChange">
<rdfs:subClassOf rdf:resource ="#InternalChange"/>
<rdfs:comment>The Process of changing the shape of an Object.</rdfs:comment>
</owl:Class>

<owl:Class rdf:ID= "Shooting">
<rdfs:subClassOf rdf:resource ="#Impelling"/>
<rdfs:comment>The subclass of Impelling where the patient
is a projectile that is fired through the air by means of some sort of
Device.</rdfs:comment>
</owl:Class>

<owl:Class rdf:ID= "ShoreArea">
<rdfs:subClassOf rdf:resource ="#LandArea"/>
<rdfs:comment>A ShoreArea is a LandArea approximately
1-3 km wide bordering a body of water, such as an ocean, bay, river,
or lake.  A ShoreArea may comprise a variety of LandForms, such as dunes,
sloughs, and marshes.</rdfs:comment>
</owl:Class>

<owl:Class rdf:ID= "Singing">
<rdfs:subClassOf rdf:resource ="#Speaking"/>
<rdfs:subClassOf rdf:resource ="#Music"/>
<rdfs:comment>Speaking that is also Music.</rdfs:comment>
</owl:Class>

<owl:Class rdf:ID= "SingleFamilyResidence">
<rdfs:subClassOf rdf:resource ="#PermanentResidence"/>
<rdfs:comment>A PermanentResidence which is
intended to be the home of a single SocialUnit.  This class covers
Houses, ApartmentUnits, and CondominiumUnits.</rdfs:comment>
</owl:Class>

<owl:Class rdf:ID= "SingleValuedRelation">
<rdfs:subClassOf rdf:resource ="#Relation"/>
<rdf:type rdf:resource = "#InheritableRelation"/>
<rdfs:comment>A Relation is a SingleValuedRelation
just in case an assignment of values to every argument position except the last
one determines at most one assignment for the last argument position.  Note
that not all SingleValuedRelations are TotalValuedRelations.</rdfs:comment>
</owl:Class>

<owl:Class rdf:ID= "Smelling">
<rdfs:subClassOf rdf:resource ="#Perception"/>
<rdfs:comment>The subclass of Perception in which the
sensing is done by an olefactory Organ.</rdfs:comment>
</owl:Class>

<owl:Class rdf:ID= "Smoke">
<rdfs:subClassOf rdf:resource ="#Cloud"/>
<rdfs:comment>A mixture of fine particles suspended in a gas that is
produced by Combustion.</rdfs:comment>
</owl:Class>

<owl:Class rdf:ID= "SocialInteraction">
<rdfs:subClassOf rdf:resource ="#IntentionalProcess"/>
<rdfs:comment>The subclass of
IntentionalProcess that involves interactions between
CognitiveAgents.</rdfs:comment>
</owl:Class>

<owl:Class rdf:ID= "SocialRole">
<rdfs:subClassOf rdf:resource ="#RelationalAttribute"/>
<rdfs:comment>The Class of all Attributes that
specify the position or status of a CognitiveAgent within an
Organization or other Group.</rdfs:comment>
</owl:Class>

<owl:Class rdf:ID= "SocialUnit">
<rdfs:subClassOf rdf:resource ="#GroupOfPeople"/>
<rdfs:comment>A GroupOfPeople who all have the same home.</rdfs:comment>
</owl:Class>

<owl:Class rdf:ID= "SolidAngleMeasure">
<rdfs:subClassOf rdf:resource ="#AngleMeasure"/>
<disjoint rdf:resource = "#PlaneAngleMeasure" />
<rdfs:comment>The value of an angle in a solid.</rdfs:comment>
</owl:Class>

<owl:Class rdf:ID= "Solution">
<rdfs:subClassOf rdf:resource ="#LiquidMixture"/>
<rdfs:comment>A liquid mixture. The most abundant component in
a solution is called the solvent. Other components are called solutes.
A solution, though homogeneous, may nonetheless have variable composition.
Any amount of salt, up to a maximum limit, can be dissolved in a given
amount of water.</rdfs:comment>
</owl:Class>

<owl:Class rdf:ID= "SpatialRelation">
<rdfs:subClassOf rdf:resource ="#Relation"/>
<rdf:type rdf:resource = "#InheritableRelation"/>
<rdfs:comment>The Class of Relations that are
spatial in a wide sense.  This Class includes mereological relations
and topological relations.</rdfs:comment>
</owl:Class>

<owl:Class rdf:ID= "Speaking">
<rdfs:subClassOf rdf:resource ="#LinguisticCommunication"/>
<rdfs:subClassOf rdf:resource ="#Vocalizing"/>
<rdfs:comment>Any LinguisticGeneration which is also a
Vocalizing, i.e. any LinguisticCommunication by a Human which
involves his/her vocal cords.</rdfs:comment>
</owl:Class>

<owl:Class rdf:ID= "SpokenHumanLanguage">
<rdfs:subClassOf rdf:resource ="#HumanLanguage"/>
<rdfs:comment>A SpokenHumanLanguage is a
HumanLanguage which has as its medium the human voice. It can also
berepresented visually through writing, although not all
SpokenHumanLanguages have a codified written form.</rdfs:comment>
</owl:Class>

<owl:Class rdf:ID= "Spore">
<rdfs:subClassOf rdf:resource ="#ReproductiveBody"/>
<rdfs:subClassOf rdf:resource ="#PlantAnatomicalStructure"/>
<rdfs:comment>Any ReproductiveBody of a NonFloweringPlant.</rdfs:comment>
</owl:Class>

<owl:Class rdf:ID= "Sport">
<rdfs:subClassOf rdf:resource ="#Game"/>
<rdfs:comment>A Game which requires some degree of physical
exercion from the participants of the game.</rdfs:comment>
</owl:Class>

<owl:Class rdf:ID= "StateChange">
<rdfs:subClassOf rdf:resource ="#InternalChange"/>
<rdfs:comment>Any Process where the PhysicalState
of part of the patient of the Process changes.</rdfs:comment>
</owl:Class>



<owl:Class rdf:ID= "StateOrProvince">
<rdfs:subClassOf rdf:resource ="#GeopoliticalArea"/>
<rdfs:subClassOf rdf:resource ="#LandArea"/>
<rdfs:comment>Administrative subdivisions of a
Nation that are broader than any other political subdivisions that
may exist.  This Class includes the states of the United States, as
well as the provinces of Canada and European countries.</rdfs:comment>
</owl:Class>

<owl:Class rdf:ID= "StaticWaterArea">
<rdfs:subClassOf rdf:resource ="#WaterArea"/>
<rdfs:comment>A WaterArea in which water does not flow
constantly or in the same direction, e.g. most lakes and ponds.</rdfs:comment>
</owl:Class>

<owl:Class rdf:ID= "Stating">
<rdfs:subClassOf rdf:resource ="#LinguisticCommunication"/>
<rdfs:comment>Instances of this Class commit the agent to some truth.
For example, John claimed that the moon is made of green cheese.</rdfs:comment>
</owl:Class>

<owl:Class rdf:ID= "StationaryArtifact">
<rdfs:subClassOf rdf:resource ="#Artifact"/>
<rdfs:comment>A StationaryArtifact is an Artifact
that has a fixed spatial location.  Most instances of this Class are
architectural works, e.g. the Eiffel Tower, the Great Pyramids, office towers,
single-family houses, etc.</rdfs:comment>
</owl:Class>

<owl:Class rdf:ID= "Steradian">
<rdfs:subClassOf rdf:resource ="#SolidAngleMeasure"/>
<rdf:type rdf:resource = "#SystemeInternationalUnit"/>
<rdfs:comment>SI solid angle measure.  Symbol: sr.  It is
the solid angle of a sphere subtended by a portion of the surface whose
area is equal to the square of the sphere's radius.  Another definition
is: the solid angle which, having its vertex in the center of the sphere,
cuts off an area of the surface of the sphere equal to that of a square
with sides of length equal to the radius of the sphere.  Steradian =
m^2/m^2 = 1.</rdfs:comment>
</owl:Class>

<owl:Class rdf:ID= "StreamWaterArea">
<rdfs:subClassOf rdf:resource ="#WaterArea"/>
<disjoint rdf:resource = "#StaticWaterArea" />
<rdfs:comment>A relatively narrow WaterArea where the
water flows constantly and in the same direction, e.g. a river, a stream,
etc.</rdfs:comment>
</owl:Class>

<owl:Class rdf:ID= "SubatomicParticle">
<rdfs:subClassOf rdf:resource ="#ElementalSubstance"/>
<rdfs:comment>The class of ElementalSubstances that
are smaller than Atoms and compose Atoms.</rdfs:comment>
</owl:Class>

<owl:Class rdf:ID= "SubjectiveAssessmentAttribute">
<rdfs:subClassOf rdf:resource ="#NormativeAttribute"/>
<disjoint rdf:resource = "#ObjectiveNorm" />
<rdfs:comment>The Class of NormativeAttributes
which lack an objective criterion for their attribution, i.e. the attribution of
these Attributes varies from subject to subject and even with respect to the
same subject over time.  This Class is, generally speaking, only used when
mapping external knowledge sources to the SUMO.  If a term from such a knowledge
source seems to lack objective criteria for its attribution, it is assigned to
this Class.</rdfs:comment>
</owl:Class>

<owl:Class rdf:ID= "Substance">
<rdfs:subClassOf rdf:resource ="#SelfConnectedObject"/>
<rdfs:comment>An Object in which every part is similar to
every other in every relevant respect.  More precisely, something is a
Substance when it has only arbitrary pieces as parts - any parts have
properties which are similar to those of the whole.  Note that a Substance
may nonetheless have physical properties that vary.  For example, the
temperature, chemical constitution, density, etc. may change from one part
to another.  An example would be a body of water.</rdfs:comment>
</owl:Class>

<owl:Class rdf:ID= "Substituting">
<rdfs:subClassOf rdf:resource ="#Transfer"/>
<rdfs:subClassOf rdf:resource ="#DualObjectProcess"/>
<rdfs:comment>The Class of Transfers where one thing is
replaced with something else.</rdfs:comment>
</owl:Class>

<owl:Class rdf:ID= "Summary">
<rdfs:subClassOf rdf:resource ="#Text"/>
<rdfs:comment>A short Text that is a summary of another,
longer Text.</rdfs:comment>
</owl:Class>

<owl:Class rdf:ID= "Sunday">
<rdfs:subClassOf rdf:resource ="#Day"/>
<rdfs:comment>The Class of all calendar Sundays.</rdfs:comment>
</owl:Class>

<owl:Class rdf:ID= "Supposing">
<rdfs:subClassOf rdf:resource ="#LinguisticCommunication"/>
<rdfs:comment>Instances of this Class suppose, for the sake of
argument, that a proposition is true.  For example, John considered what he
would do if he won the lottery.</rdfs:comment>
</owl:Class>

<owl:Class rdf:ID= "SurfaceChange">
<rdfs:subClassOf rdf:resource ="#InternalChange"/>
<rdfs:comment>Processes which involve altering
the properties that apply to the surface of an Object.</rdfs:comment>
</owl:Class>

<owl:Class rdf:ID= "Surgery">
<rdfs:subClassOf rdf:resource ="#TherapeuticProcess"/>
<rdfs:comment>Any TherapeuticProcess that involves making an
incision in the Animal that is the patient of the TherapeuticProcess.</rdfs:comment>
</owl:Class>

<owl:Class rdf:ID= "Suspension">
<rdfs:subClassOf rdf:resource ="#LiquidMixture"/>
<rdfs:comment>A LiquidMixture where at least one of the
components of the Mixture is equally distributed throughout the Mixture
but is not dissolved in it.</rdfs:comment>
</owl:Class>

<owl:Class rdf:ID= "SymbolicString">
<rdfs:subClassOf rdf:resource ="#ContentBearingObject"/>
<rdfs:comment>The Class of alphanumeric sequences.</rdfs:comment>
</owl:Class>

<owl:Class rdf:ID= "SymmetricRelation">
<rdfs:subClassOf rdf:resource ="#BinaryRelation"/>
<rdfs:comment>A BinaryRelation ?REL is
symmetric just in case (?REL ?INST1 ?INST2) imples (?REL
?INST2 ?INST1), for all ?INST1 and ?INST2.</rdfs:comment>
</owl:Class>

<owl:Class rdf:ID= "SyntheticSubstance">
<rdfs:subClassOf rdf:resource ="#Substance"/>
<rdfs:comment>Any Substance that is the result of an
IntentionalProcess, i.e. any substance that is created by Humans.</rdfs:comment>
</owl:Class>

<owl:Class rdf:ID= "SystemeInternationalUnit">
<rdfs:subClassOf rdf:resource ="#UnitOfMeasure"/>
<rdfs:comment>The Class of Systeme
International (SI) units.</rdfs:comment>
</owl:Class>

<owl:Class rdf:ID= "TactilePerception">
<rdfs:subClassOf rdf:resource ="#Perception"/>
<rdfs:comment>The subclass of Perception in which
the sensing is done by Touching.  Note that Touching need not involve
TactilePerception.  For example, a person who has lost all sensation in
both of his legs would have no TactilePerception of anything his legs
were Touching.</rdfs:comment>
</owl:Class>

<owl:Class rdf:ID= "Tasting">
<rdfs:subClassOf rdf:resource ="#Perception"/>
<rdfs:comment>The subclass of Perception in which the
sensing is done by of an Organ which can discriminate various tastes.</rdfs:comment>
</owl:Class>

<owl:Class rdf:ID= "TemperatureMeasure">
<rdfs:subClassOf rdf:resource ="#ConstantQuantity"/>
<rdfs:comment>Measures of temperature.
In scientific circles, the temperature of something is understood as the
average velocity of the atoms or molecules that make up the thing.</rdfs:comment>
</owl:Class>

<owl:Class rdf:ID= "TemporalRelation">
<rdfs:subClassOf rdf:resource ="#Relation"/>
<rdf:type rdf:resource = "#InheritableRelation"/>
<rdfs:comment>The Class of temporal Relations.
This Class includes notions of (temporal) topology of intervals,
(temporal) schemata, and (temporal) extension.</rdfs:comment>
</owl:Class>

<owl:Class rdf:ID= "TemporaryResidence">
<rdfs:subClassOf rdf:resource ="#Residence"/>
<rdfs:comment>A Residence which is strictly temporary,
i.e. where no one makes his/her home.</rdfs:comment>
</owl:Class>

<owl:Class rdf:ID= "TerminatingEmployment">
<rdfs:subClassOf rdf:resource ="#LeavingAnOrganization"/>
<rdfs:comment>OrganizationalProcesses where someone
ceases to be an employee of an Organization.  Note that this covers being
laid off, being fired, and voluntarily leaving a job.</rdfs:comment>
</owl:Class>

<owl:Class rdf:ID= "TernaryFunction">
<rdfs:subClassOf rdf:resource ="#Function"/>
<rdfs:subClassOf rdf:resource ="#QuaternaryRelation"/>
<rdf:type rdf:resource = "#InheritableRelation"/>
<rdfs:comment>The Class of Functions that require
exactly three arguments.</rdfs:comment>
</owl:Class>

<owl:Class rdf:ID= "TernaryPredicate">
<rdfs:subClassOf rdf:resource ="#Predicate"/>
<rdfs:subClassOf rdf:resource ="#TernaryRelation"/>
<rdf:type rdf:resource = "#InheritableRelation"/>
<rdfs:comment>The Class of Predicates that require
exactly three arguments.</rdfs:comment>
</owl:Class>

<owl:Class rdf:ID= "TernaryRelation">
<rdfs:subClassOf rdf:resource ="#Relation"/>
<rdf:type rdf:resource = "#InheritableRelation"/>
<rdfs:comment>TernaryRelations relate three items.
The two subclasses of TernaryRelation are TernaryPredicate and
BinaryFunction.</rdfs:comment>
</owl:Class>

<owl:Class rdf:ID= "Text">
<rdfs:subClassOf rdf:resource ="#LinguisticExpression"/>
<rdfs:subClassOf rdf:resource ="#Artifact"/>
<rdfs:comment>A LinguisticExpression or set of
LinguisticExpressions that perform a specific function related
to Communication, e.g. express a discourse about a particular
topic, and that are inscribed in a CorpuscularObject by Humans.</rdfs:comment>
</owl:Class>

<owl:Class rdf:ID= "TherapeuticProcess">
<rdfs:subClassOf rdf:resource ="#Repairing"/>
<rdfs:comment>A Process that is carried out
for the purpose of curing, improving or reducing the pain associated
with a DiseaseOrSyndrome.</rdfs:comment>
</owl:Class>

<owl:Class rdf:ID= "ThreeDimensionalFigure">
<rdfs:subClassOf rdf:resource ="#GeometricFigure"/>
<rdfs:comment>The class of GeometricFigures that
have position and an extension along three dimensions, viz. geometric solids
like polyhedrons and cylinders.</rdfs:comment>
</owl:Class>

<owl:Class rdf:ID= "Thursday">
<rdfs:subClassOf rdf:resource ="#Day"/>
<rdfs:comment>The Class of all calendar Thursdays.</rdfs:comment>
</owl:Class>

<owl:Class rdf:ID= "TimeDependentQuantity">
<rdfs:subClassOf rdf:resource ="#UnaryConstantFunctionQuantity"/>
<rdfs:comment>A UnaryConstantFunctionQuantity of
continuous time.  All instances of this Class are returned by Functions
that map a time quantity into another ConstantQuantity such as temperature.
For example, 'the temperature at the top of the Empire State Building' is a
TimeDependentQuantity since its value depends on the time.</rdfs:comment>
</owl:Class>

<owl:Class rdf:ID= "TimeDuration">
<rdfs:subClassOf rdf:resource ="#TimeMeasure"/>
<rdfs:comment>Any measure of length of time,
with or without respect to the universal timeline.</rdfs:comment>
</owl:Class>

<owl:Class rdf:ID= "TimeInterval">
<rdfs:subClassOf rdf:resource ="#TimePosition"/>
<rdfs:comment>An interval of time.  Note that a
TimeInterval has both an extent and a location on the universal
timeline.  Note too that a TimeInterval has no gaps, i.e. this
class contains only convex time intervals.</rdfs:comment>
</owl:Class>

<owl:Class rdf:ID= "TimeMeasure">
<rdfs:subClassOf rdf:resource ="#ConstantQuantity"/>
<rdfs:comment>The class of temporal durations (instances
of TimeDuration) and positions of TimePoints and TimeIntervals along
the universal timeline (instances of TimePosition).</rdfs:comment>
</owl:Class>

<owl:Class rdf:ID= "TimePoint">
<rdfs:subClassOf rdf:resource ="#TimePosition"/>
<rdfs:comment>An extensionless point on the universal timeline.
The TimePoints at which Processes occur can be known with various
degrees of precision and approximation, but conceptually TimePoints are
point-like and not interval-like.  That is, it doesn't make sense to talk
about how long a TimePoint lasts.</rdfs:comment>
</owl:Class>

<owl:Class rdf:ID= "TimePosition">
<rdfs:subClassOf rdf:resource ="#TimeMeasure"/>
<rdfs:comment>Any TimePoint or TimeInterval
along the universal timeline from NegativeInfinity to
PositiveInfinity.</rdfs:comment>
</owl:Class>

<owl:Class rdf:ID= "TimeZone">
<rdfs:subClassOf rdf:resource ="#RelationalAttribute"/>
<rdfs:comment>An Attribute which is used to specify coordinates
in which time measures are uniform, i.e. all time devices are synchronized to
the same TimePositions.</rdfs:comment>
</owl:Class>

<owl:Class rdf:ID= "Tissue">
<rdfs:subClassOf rdf:resource ="#BodySubstance"/>
<rdfs:comment>An aggregation of similarly specialized Cells
and the associated intercellular substance. Tissues are relatively
non-localized in comparison to BodyParts, Organs or Organ components.
The main features of Tissues are self-connectivity (see
SelfConnectedObject) and being a homogeneous mass (all parts in the
same granularity are instances of Tissue as well).</rdfs:comment>
</owl:Class>

<owl:Class rdf:ID= "TotalOrderingRelation">
<rdfs:subClassOf rdf:resource ="#PartialOrderingRelation"/>
<rdfs:subClassOf rdf:resource ="#TrichotomizingRelation"/>
<rdfs:comment>A BinaryRelation is a
TotalOrderingRelation if it is a PartialOrderingRelation
and a TrichotomizingRelation.</rdfs:comment>
</owl:Class>

<owl:Class rdf:ID= "TotalValuedRelation">
<rdfs:subClassOf rdf:resource ="#Relation"/>
<rdf:type rdf:resource = "#InheritableRelation"/>
<rdfs:comment>A Relation is a TotalValuedRelation
just in case there exists an assignment for the last argument position of the
Relation given any assignment of values to every argument position except
the last one.  Note that declaring a Relation to be both a TotalValuedRelation
and a SingleValuedRelation means that it is a total function.</rdfs:comment>
</owl:Class>

<owl:Class rdf:ID= "Touching">
<rdfs:subClassOf rdf:resource ="#Transfer"/>
<rdfs:comment>Any Transfer where two Objects are
brought into immediate physical contact with one another.</rdfs:comment>
</owl:Class>



<owl:Class rdf:ID= "Transaction">
<rdfs:subClassOf rdf:resource ="#ChangeOfPossession"/>
<rdfs:subClassOf rdf:resource ="#DualObjectProcess"/>
<rdfs:comment>The subclass of ChangeOfPossession where
something is exchanged for something else.</rdfs:comment>
</owl:Class>

<owl:Class rdf:ID= "Transfer">
<rdfs:subClassOf rdf:resource ="#Translocation"/>
<rdfs:comment>Any instance of Translocation where the agent
and the patient are not the same thing.</rdfs:comment>
</owl:Class>

<owl:Class rdf:ID= "TransitiveRelation">
<rdfs:subClassOf rdf:resource ="#BinaryRelation"/>
<rdfs:comment>A BinaryRelation ?REL is transitive
if (?REL ?INST1 ?INST2) and (?REL ?INST2 ?INST3) imply (?REL ?INST1 ?INST3),
for all ?INST1, ?INST2, and ?INST3.</rdfs:comment>
</owl:Class>

<owl:Class rdf:ID= "Transitway">
<rdfs:subClassOf rdf:resource ="#Region"/>
<rdfs:subClassOf rdf:resource ="#SelfConnectedObject"/>
<rdfs:comment>Transitway is the broadest class
of regions which may be passed through as a path in instances
of Translocation.  Transitway includes land, air, and sea
regions, and it includes both natural and artificial transitways.</rdfs:comment>
</owl:Class>

<owl:Class rdf:ID= "Translating">
<rdfs:subClassOf rdf:resource ="#ContentDevelopment"/>
<rdfs:subClassOf rdf:resource ="#DualObjectProcess"/>
<rdfs:comment>Converting content from one Language into another.
This covers oral translation (i.e. interpreting) as well as written translation.</rdfs:comment>
</owl:Class>

<owl:Class rdf:ID= "Translocation">
<rdfs:subClassOf rdf:resource ="#Motion"/>
<rdfs:comment>Translocation is that class of Motions
in which an object moves from one place to another.  In the case of round
trips, the origin and destination are the same, but the intervening
motion passes through other locations.  Translocation represents linear
motion, in contrast to rotation or other movement in place.  A vehicle is
not necessary; Ambulating is a kind of Translocation.</rdfs:comment>
</owl:Class>

<owl:Class rdf:ID= "Transportation">
<rdfs:subClassOf rdf:resource ="#Translocation"/>
<relatedInternalConcept rdf:resource = "#TransportationDevice" />
<rdfs:comment>Motion from one point to another by means
of a TransportationDevice.</rdfs:comment>
</owl:Class>

<owl:Class rdf:ID= "TransportationDevice">
<rdfs:subClassOf rdf:resource ="#Device"/>
<rdfs:comment>A TransportationDevice is a Device
which serves as the instrument in a Transportation Process which carries
the patient of the Process from one point to another.</rdfs:comment>
</owl:Class>

<owl:Class rdf:ID= "TrichotomizingRelation">
<rdfs:subClassOf rdf:resource ="#BinaryRelation"/>
<rdfs:comment>A BinaryRelation ?REL is a
TrichotomizingRelation just in case all ordered pairs consisting of
distinct individuals are elements of ?REL.</rdfs:comment>
</owl:Class>

<owl:Class rdf:ID= "TruthValue">
<rdfs:subClassOf rdf:resource ="#RelationalAttribute"/>
<rdfs:comment>The Class of truth values, e.g. True and
False.  These are Attributes of Sentences and Propositions.</rdfs:comment>
</owl:Class>

<owl:Class rdf:ID= "Tuesday">
<rdfs:subClassOf rdf:resource ="#Day"/>
<rdfs:comment>The Class of all calendar Tuesdays.</rdfs:comment>
</owl:Class>

<owl:Class rdf:ID= "TwoDimensionalAngle">
<rdfs:subClassOf rdf:resource ="#OpenTwoDimensionalFigure"/>
<rdfs:comment>Any two OneDimensionalFigures (i.e.
straight lines) meeting at a single GeometricPoint.</rdfs:comment>
</owl:Class>

<owl:Class rdf:ID= "TwoDimensionalFigure">
<rdfs:subClassOf rdf:resource ="#GeometricFigure"/>
<rdfs:comment>The class of GeometricFigures that
have position and an extension along two dimensions, viz. plane figures
like circles and polygons.</rdfs:comment>
</owl:Class>

<owl:Class rdf:ID= "UnaryConstantFunctionQuantity">
<rdfs:subClassOf rdf:resource ="#FunctionQuantity"/>
<rdfs:comment>The class of FunctionQuantities
that are returned by UnaryFunctions that map from the Class ConstantQuantity
to the Class ConstantQuantity.</rdfs:comment>
</owl:Class>

<owl:Class rdf:ID= "UnaryFunction">
<rdfs:subClassOf rdf:resource ="#Function"/>
<rdfs:subClassOf rdf:resource ="#BinaryRelation"/>
<rdf:type rdf:resource = "#InheritableRelation"/>
<rdfs:comment>The Class of Functions that require a
single argument.</rdfs:comment>
</owl:Class>

<owl:Class rdf:ID= "Uncovering">
<rdfs:subClassOf rdf:resource ="#Removing"/>
<disjoint rdf:resource = "#Covering" />
<rdfs:comment>The Class of Removing processes where the agent
uncovers the patient, either completely or only partially.</rdfs:comment>
</owl:Class>

<owl:Class rdf:ID= "Ungrasping">
<rdfs:subClassOf rdf:resource ="#Detaching"/>
<rdfs:comment>Any instance of Detaching which results in
a situation where it is not the case that the agent grasps something
which he/she grasps previously.</rdfs:comment>
</owl:Class>

<owl:Class rdf:ID= "UnilateralGetting">
<rdfs:subClassOf rdf:resource ="#Getting"/>
<relatedInternalConcept rdf:resource = "#UnilateralGiving" />
<rdfs:comment>Any instance of Getting that is not part
of a Transaction.  In other words, any instance of Getting where nothing
is given in return.  Some examples of UnilateralGetting are:  appropriating,
commandeering, stealing, etc.</rdfs:comment>
</owl:Class>

<owl:Class rdf:ID= "UnilateralGiving">
<rdfs:subClassOf rdf:resource ="#Giving"/>
<rdfs:comment>Any instance of Giving that is not part
of a Transaction.  In other words, any instance of Giving where nothing
is received in return.  Some examples of UnilateralGiving are:  honorary
awards, gifts, and financial grants.</rdfs:comment>
</owl:Class>

<owl:Class rdf:ID= "UniqueList">
<rdfs:subClassOf rdf:resource ="#List"/>
<rdfs:comment>A List in which no item appears more than once,
i.e. a List for which there are no distinct numbers ?NUMBER1 and ?NUMBER2
such that (ListOrderFn ?LIST ?NUMBER1) and (ListOrderFn ?LIST ?NUMBER2)
return the same value.</rdfs:comment>
</owl:Class>

<owl:Class rdf:ID= "UnitOfMeasure">
<rdfs:subClassOf rdf:resource ="#PhysicalQuantity"/>
<rdfs:comment>A standard of measurement for some dimension.
For example, the Meter is a UnitOfMeasure for the dimension of length,
as is the Inch.  There is no intrinsic property of a UnitOfMeasure that
makes it primitive or fundamental; rather, a system of units (e.g.
SystemeInternationalUnit) defines a set of orthogonal dimensions and
assigns units for each.</rdfs:comment>
</owl:Class>

<owl:Class rdf:ID= "UnitedStatesCent">
<rdfs:subClassOf rdf:resource ="#CurrencyMeasure"/>
<rdf:type rdf:resource = "#UnitOfMeasure"/>
<rdfs:comment>A currency measure.  1 UnitedStatesCent is
equal to .01 UnitedStatesDollars.</rdfs:comment>
</owl:Class>

<owl:Class rdf:ID= "UnitedStatesDollar">
<rdfs:subClassOf rdf:resource ="#CurrencyMeasure"/>
<rdf:type rdf:resource = "#UnitOfMeasure"/>
<rdfs:comment>A currency measure.</rdfs:comment>
</owl:Class>

<owl:Class rdf:ID= "UnitedStatesGallon">
<rdfs:subClassOf rdf:resource ="#VolumeMeasure"/>
<rdf:type rdf:resource = "#UnitOfMeasure"/>
<rdfs:comment>Unit of volume commonly used in the
United States.</rdfs:comment>
</owl:Class>

<owl:Class rdf:ID= "ValidDeductiveArgument">
<rdfs:subClassOf rdf:resource ="#DeductiveArgument"/>
<rdfs:comment>A DeductiveArgument which is
valid, i.e. the set of premises in fact entails the conclusion.</rdfs:comment>
</owl:Class>

<owl:Class rdf:ID= "VariableArityRelation">
<rdfs:subClassOf rdf:resource ="#Relation"/>
<rdfs:comment>The Class of Relations that
do not have a fixed number of arguments.</rdfs:comment>
</owl:Class>

<owl:Class rdf:ID= "Vehicle">
<rdfs:subClassOf rdf:resource ="#TransportationDevice"/>
<rdfs:comment>Vehicle is the subclass of
TransportationDevices that transport passengers or goods
from one place to another by moving from one place to the other
with them, e.g., cars, trucks, ferries, and airplanes.  Contrast
with devices such as pipelines, escalators, or supermarket
checkout belts, which carry items from one place to another by means
of a moving part, without the device removing from the origin to
the destination.</rdfs:comment>
</owl:Class>

<owl:Class rdf:ID= "Verb">
<rdfs:subClassOf rdf:resource ="#Word"/>
<rdfs:comment>One of the parts of speech.  The Class of Words
that conventionally denote Processes.</rdfs:comment>
</owl:Class>

<owl:Class rdf:ID= "VerbPhrase">
<rdfs:subClassOf rdf:resource ="#Phrase"/>
<rdfs:comment>A Phrase that has the same function as a
Verb.</rdfs:comment>
</owl:Class>

<owl:Class rdf:ID= "Vertebrate">
<rdfs:subClassOf rdf:resource ="#Animal"/>
<rdfs:comment>An Animal which has a spinal column.</rdfs:comment>
</owl:Class>

<owl:Class rdf:ID= "ViolentContest">
<rdfs:subClassOf rdf:resource ="#Contest"/>
<rdfs:comment>A Contest where one participant attempts to
physically injure another participant.</rdfs:comment>
</owl:Class>

<owl:Class rdf:ID= "Virus">
<rdfs:subClassOf rdf:resource ="#Microorganism"/>
<rdfs:comment>An Organism consisting of a core of a single
nucleic acid enclosed in a protective coat of protein. A virus may replicate
only inside a host living cell. A virus exhibits some but not all of the
usual characteristics of living things.</rdfs:comment>
</owl:Class>

<owl:Class rdf:ID= "Vitamin">
<rdfs:subClassOf rdf:resource ="#Nutrient"/>
<rdfs:comment>A Nutrient present in natural products or made
synthetically, which is essential in the diet of Humans and other higher
Animals.  Included here are Vitamin precursors and provitamins.</rdfs:comment>
</owl:Class>

<owl:Class rdf:ID= "Vocalizing">
<rdfs:subClassOf rdf:resource ="#RadiatingSound"/>
<rdfs:subClassOf rdf:resource ="#BodyMotion"/>
<rdfs:comment>Any instance of RadiatingSound where the
instrument is the Human vocal cords.  This covers grunts, screams,
roars, as well as Speaking.</rdfs:comment>
</owl:Class>

<owl:Class rdf:ID= "VolumeMeasure">
<rdfs:subClassOf rdf:resource ="#ConstantQuantity"/>
<rdfs:comment>Measures of the amount of space in three
dimensions.</rdfs:comment>
</owl:Class>

<owl:Class rdf:ID= "Voting">
<rdfs:subClassOf rdf:resource ="#Deciding"/>
<rdfs:comment>Voting is the activity of voting in an
Election.  Voting is typically done by individuals, while Elections
are conducted by Organizations.  The voting process by an individual
voter is part of an Election process.</rdfs:comment>
</owl:Class>

<owl:Class rdf:ID= "Walking">
<rdfs:subClassOf rdf:resource ="#Ambulating"/>
<rdfs:comment>Ambulating relatively slowly, i.e. moving in such a
way that at least one foot is always in contact with the ground.</rdfs:comment>
</owl:Class>

<owl:Class rdf:ID= "War">
<rdfs:subClassOf rdf:resource ="#ViolentContest"/>
<rdfs:comment>A military confrontation between two or more
GeopoliticalAreas or Organizations whose members are GeopoliticalAreas.
As the corresponding axiom specifies, a War is made up of Battles.</rdfs:comment>
</owl:Class>

<owl:Class rdf:ID= "WarmBloodedVertebrate">
<rdfs:subClassOf rdf:resource ="#Vertebrate"/>
<disjoint rdf:resource = "#ColdBloodedVertebrate" />
<rdfs:comment>Vertebrates whose body temperature
is internally regulated.</rdfs:comment>
</owl:Class>

<owl:Class rdf:ID= "Water">
<rdfs:subClassOf rdf:resource ="#CompoundSubstance"/>
<rdfs:comment>The Class of samples of the compound H20.  Note
that this Class covers both pure and impure Water.</rdfs:comment>
</owl:Class>

<owl:Class rdf:ID= "WaterArea">
<rdfs:subClassOf rdf:resource ="#GeographicArea"/>
<rdfs:comment>A body which is made up predominantly of water,
e.g. rivers, lakes, oceans, etc.</rdfs:comment>
</owl:Class>

<owl:Class rdf:ID= "WaterCloud">
<rdfs:subClassOf rdf:resource ="#Cloud"/>
<rdfs:comment>Any Cloud that is composed primarily of water vapor.</rdfs:comment>
</owl:Class>

<owl:Class rdf:ID= "Weapon">
<rdfs:subClassOf rdf:resource ="#Device"/>
<rdfs:comment>The Class of Devices that are designed
primarily to damage or destroy Humans/Animals, StationaryArtifacts or
the places inhabited by Humans/Animals.</rdfs:comment>
</owl:Class>

<owl:Class rdf:ID= "WeatherProcess">
<rdfs:subClassOf rdf:resource ="#Motion"/>
<disjoint rdf:resource = "#IntentionalProcess" />
<rdfs:comment>WeatherProcess is the broadest class of
processes that involve weather, including weather seasons (not to be confused
with instances of SeasonOfYear), weather systems, and short-term weather
events.</rdfs:comment>
</owl:Class>

<owl:Class rdf:ID= "Wedding">
<rdfs:subClassOf rdf:resource ="#Declaring"/>
<rdfs:comment>Any Declaring that leads to one person being
the spouse of another.</rdfs:comment>
</owl:Class>

<owl:Class rdf:ID= "Wednesday">
<rdfs:subClassOf rdf:resource ="#Day"/>
<rdfs:comment>The Class of all calendar Wednesdays.</rdfs:comment>
</owl:Class>

<owl:Class rdf:ID= "Week">
<rdfs:subClassOf rdf:resource ="#TimeInterval"/>
<rdfs:comment>The Class of all calendar weeks.</rdfs:comment>
</owl:Class>

<owl:Class rdf:ID= "WeekDuration">
<rdfs:subClassOf rdf:resource ="#TimeDuration"/>
<rdf:type rdf:resource = "#UnitOfMeasure"/>
<rdfs:comment>Time unit.  A week's duration is seven days.</rdfs:comment>
</owl:Class>

<owl:Class rdf:ID= "Wetting">
<rdfs:subClassOf rdf:resource ="#Putting"/>
<rdfs:comment>The Class of Processes where a Liquid is
added to an Object.</rdfs:comment>
</owl:Class>

<owl:Class rdf:ID= "Wind">
<rdfs:subClassOf rdf:resource ="#GasMotion"/>
<rdfs:comment>Any Motion of Air.</rdfs:comment>
</owl:Class>

<owl:Class rdf:ID= "Woman">
<rdfs:subClassOf rdf:resource ="#Human"/>
<rdfs:comment>The class of Female Humans.</rdfs:comment>
</owl:Class>

<owl:Class rdf:ID= "Word">
<rdfs:subClassOf rdf:resource ="#LinguisticExpression"/>
<rdfs:comment>A term of a Language that represents a concept.</rdfs:comment>
</owl:Class>

<owl:Class rdf:ID= "Worm">
<rdfs:subClassOf rdf:resource ="#Invertebrate"/>
<rdfs:comment>Long, narrow, soft-bodied Invertebrates.</rdfs:comment>
</owl:Class>

<owl:Class rdf:ID= "Writing">
<rdfs:subClassOf rdf:resource ="#ContentDevelopment"/>
<rdfs:comment>A subclass of ContentDevelopment in which
content is converted from one form (e.g. uttered, written or represented
mentally) into a written form.  Note that this class covers both
transcription and original creation of written Texts.</rdfs:comment>
</owl:Class>

<owl:Class rdf:ID= "Year">
<rdfs:subClassOf rdf:resource ="#TimeInterval"/>
<relatedInternalConcept rdf:resource = "#YearFn" />
<relatedInternalConcept rdf:resource = "#YearDuration" />
<rdfs:comment>The Class of all calendar Years.</rdfs:comment>
</owl:Class>

<owl:Class rdf:ID= "YearDuration">
<rdfs:subClassOf rdf:resource ="#TimeDuration"/>
<rdf:type rdf:resource = "#UnitOfMeasure"/>
<rdfs:comment>Time unit. one calendar year. 1 year =
365 days = 31536000 seconds.</rdfs:comment>
</owl:Class>

<owl:DatatypeProperty  rdf:ID= "AbsoluteValueFn">
<rdfs:comment>The value of (AbsoluteValueFn ?NUMBER)
is the absolute value of the RealNumber ?NUMBER.</rdfs:comment>
<rdf:type rdf:resource = "#UnaryFunction"/>
<rdf:type rdf:resource = "#TotalValuedRelation"/>
<rdfs:domain rdf:resource="#RealNumber"/>
<rdfs:range rdf:resource = "#NonnegativeRealNumber"/>
</owl:DatatypeProperty>

<owl:ObjectProperty   rdf:ID= "AbstractionFn">
<rdfs:comment>A UnaryFunction that maps a Class into
the instance of Attribute that specifies the condition(s) for membership
in the Class.</rdfs:comment>
<rdf:type rdf:resource = "#UnaryFunction"/>
<rdf:type rdf:resource = "#PartialValuedRelation"/>
<rdfs:domain rdf:resource="#Class"/>
<rdfs:range rdf:resource = "#Attribute"/>
</owl:ObjectProperty>

<owl:ObjectProperty   rdf:ID= "BackFn">
<rdfs:comment>A Function that maps an Object to the side
that is opposite the FrontFn of the Object.  Note that this is a
partial function, since some Objects do not have sides, e.g. apples
and spheres.  Note too that the range of this Function is indefinite in
much the way that ImmediateFutureFn and ImmediatePastFn are indefinite.
Although this indefiniteness is undesirable from a theoretical standpoint,
it does not have significant practical implications, since there is
widespread intersubjective agreement about the most common cases.</rdfs:comment>
<rdf:type rdf:resource = "#SpatialRelation"/>
<rdf:type rdf:resource = "#PartialValuedRelation"/>
<rdf:type rdf:resource = "#UnaryFunction"/>
<rdf:type rdf:resource = "#AsymmetricRelation"/>
<rdf:type rdf:resource = "#IrreflexiveRelation"/>
<rdfs:domain rdf:resource="#SelfConnectedObject"/>
<rdfs:range rdf:resource = "#SelfConnectedObject"/>
</owl:ObjectProperty>

<owl:ObjectProperty   rdf:ID= "BeginFn">
<rdfs:comment>A UnaryFunction that maps a TimeInterval to
the TimePoint at which the interval begins.</rdfs:comment>
<rdf:type rdf:resource = "#TemporalRelation"/>
<rdf:type rdf:resource = "#UnaryFunction"/>
<rdf:type rdf:resource = "#TotalValuedRelation"/>
<rdfs:domain rdf:resource="#TimeInterval"/>
<rdfs:range rdf:resource = "#TimePoint"/>
</owl:ObjectProperty>

<owl:DatatypeProperty  rdf:ID= "CardinalityFn">
<rdfs:comment>(CardinalityFn ?CLASS) returns the
number of instances in the SetOrClass ?CLASS or the number of
members in the ?CLASS Collection.</rdfs:comment>
<rdf:type rdf:resource = "#UnaryFunction"/>
<rdf:type rdf:resource = "#TotalValuedRelation"/>
<rdf:type rdf:resource = "#AsymmetricRelation"/>
<rdfs:range rdf:resource = "#Number"/>
</owl:DatatypeProperty>

<owl:DatatypeProperty  rdf:ID= "CeilingFn">
<rdfs:comment>(CeilingFn ?NUMBER) returns the smallest
Integer greater than or equal to the RealNumber ?NUMBER.</rdfs:comment>
<rdf:type rdf:resource = "#UnaryFunction"/>
<rdf:type rdf:resource = "#TotalValuedRelation"/>
<rdfs:domain rdf:resource="#RealNumber"/>
<rdfs:range rdf:resource = "#Integer"/>
</owl:DatatypeProperty>

<owl:ObjectProperty   rdf:ID= "ComplementFn">
<rdfs:comment>The complement of a given SetOrClass C is the
SetOrClass of all things that are not instances of C.  In other words, an
object is an instance of the complement of a SetOrClass C just in case it
is not an instance of C.</rdfs:comment>
<rdf:type rdf:resource = "#UnaryFunction"/>
<rdf:type rdf:resource = "#TotalValuedRelation"/>
<rdfs:domain rdf:resource="#SetOrClass"/>
<rdfs:range rdf:resource = "#SetOrClass"/>
</owl:ObjectProperty>

<owl:DatatypeProperty  rdf:ID= "CosineFn">
<rdfs:comment>(CosineFn ?DEGREE) returns the cosine of the
PlaneAngleMeasure ?DEGREE.  The cosine of ?DEGREE is the ratio of the
side next to ?DEGREE to the hypotenuse in a right-angled triangle.</rdfs:comment>
<rdf:type rdf:resource = "#UnaryFunction"/>
<rdf:type rdf:resource = "#TotalValuedRelation"/>
<rdfs:domain rdf:resource="#PlaneAngleMeasure"/>
<rdfs:range rdf:resource = "#RealNumber"/>
</owl:DatatypeProperty>

<owl:DatatypeProperty  rdf:ID= "DenominatorFn">
<rdfs:comment>(DenominatorFn ?NUMBER) returns the
denominator of the canonical reduced form of the RealNumber ?NUMBER.</rdfs:comment>
<rdf:type rdf:resource = "#UnaryFunction"/>
<rdf:type rdf:resource = "#TotalValuedRelation"/>
<rdfs:domain rdf:resource="#RealNumber"/>
<rdfs:range rdf:resource = "#Integer"/>
</owl:DatatypeProperty>

<owl:ObjectProperty   rdf:ID= "EndFn">
<rdfs:comment>A UnaryFunction that maps a TimeInterval to
the TimePoint at which the interval ends.</rdfs:comment>
<rdf:type rdf:resource = "#TemporalRelation"/>
<rdf:type rdf:resource = "#UnaryFunction"/>
<rdf:type rdf:resource = "#TotalValuedRelation"/>
<rdfs:domain rdf:resource="#TimeInterval"/>
<rdfs:range rdf:resource = "#TimePoint"/>
</owl:ObjectProperty>

<owl:ObjectProperty   rdf:ID= "ExtensionFn">
<rdfs:comment>A UnaryFunction that maps an Attribute
into the Class whose condition for membership is the Attribute.</rdfs:comment>
<rdf:type rdf:resource = "#UnaryFunction"/>
<rdf:type rdf:resource = "#PartialValuedRelation"/>
<rdfs:domain rdf:resource="#Attribute"/>
<rdfs:range rdf:resource = "#Class"/>
</owl:ObjectProperty>

<owl:DatatypeProperty  rdf:ID= "FloorFn">
<rdfs:comment>(FloorFn ?NUMBER) returns the largest Integer
less than or equal to the RealNumber ?NUMBER.</rdfs:comment>
<rdf:type rdf:resource = "#UnaryFunction"/>
<rdf:type rdf:resource = "#TotalValuedRelation"/>
<rdfs:domain rdf:resource="#RealNumber"/>
<rdfs:range rdf:resource = "#Integer"/>
</owl:DatatypeProperty>

<owl:ObjectProperty   rdf:ID= "FrontFn">
<rdfs:comment>A Function that maps an Object to the side
that generally receives the most attention or that typically faces the
direction in which the Object moves.  Note that this is a partial
function, since some Objects do not have sides, e.g. apples and
spheres.  Note too that the range of this Function is indefinite in
much the way that ImmediateFutureFn and ImmediatePastFn are indefinite.
Although this indefiniteness is undesirable from a theoretical standpoint,
it does not have significant practical implications, since there is
widespread intersubjective agreement about the most common cases.</rdfs:comment>
<rdf:type rdf:resource = "#SpatialRelation"/>
<rdf:type rdf:resource = "#PartialValuedRelation"/>
<rdf:type rdf:resource = "#UnaryFunction"/>
<rdf:type rdf:resource = "#AsymmetricRelation"/>
<rdf:type rdf:resource = "#IrreflexiveRelation"/>
<rdfs:domain rdf:resource="#SelfConnectedObject"/>
<rdfs:range rdf:resource = "#SelfConnectedObject"/>
</owl:ObjectProperty>

<owl:ObjectProperty   rdf:ID= "FutureFn">
<rdfs:comment>A UnaryFunction that maps a TimePosition
to the TimeInterval which it meets and which ends at
PositiveInfinity.</rdfs:comment>
<rdf:type rdf:resource = "#TemporalRelation"/>
<rdf:type rdf:resource = "#UnaryFunction"/>
<rdf:type rdf:resource = "#TotalValuedRelation"/>
<rdfs:domain rdf:resource="#TimePosition"/>
<rdfs:range rdf:resource = "#TimeInterval"/>
</owl:ObjectProperty>

<owl:ObjectProperty   rdf:ID= "GeneralizedIntersectionFn">
<rdfs:comment>A UnaryFunction that takes a
SetOrClass of Classes as its single argument and returns a SetOrClass which
is the intersection of all of the Classes in the original SetOrClass, i.e.
the SetOrClass containing just those instances which are instances of all
instances of the original SetOrClass.</rdfs:comment>
<rdf:type rdf:resource = "#UnaryFunction"/>
<rdf:type rdf:resource = "#TotalValuedRelation"/>
<rdfs:domain rdf:resource="#SetOrClass"/>
<rdfs:range rdf:resource = "#SetOrClass"/>
</owl:ObjectProperty>

<owl:ObjectProperty   rdf:ID= "GeneralizedUnionFn">
<rdfs:comment>A UnaryFunction that takes a SetOrClass
of Classes as its single argument and returns a SetOrClass which is the
merge of all of the Classes in the original SetOrClass, i.e. the SetOrClass
containing just those instances which are instances of an instance of the
original SetOrClass.</rdfs:comment>
<rdf:type rdf:resource = "#UnaryFunction"/>
<rdf:type rdf:resource = "#TotalValuedRelation"/>
<rdfs:domain rdf:resource="#SetOrClass"/>
<rdfs:range rdf:resource = "#SetOrClass"/>
</owl:ObjectProperty>

<owl:ObjectProperty   rdf:ID= "GigaFn">
<rdfs:comment>A UnaryFunction that maps a UnitOfMeasure into
a UnitOfMeasure that is equal to 1,000,000,000 units of the original
UnitOfMeasure.  For example, (GigaFn Hertz) is 1,000,000,000 Hertz.</rdfs:comment>
<rdf:type rdf:resource = "#UnaryFunction"/>
<rdf:type rdf:resource = "#TotalValuedRelation"/>
<rdfs:domain rdf:resource="#UnitOfMeasure"/>
<rdfs:range rdf:resource = "#UnitOfMeasure"/>
</owl:ObjectProperty>

<owl:ObjectProperty   rdf:ID= "GovernmentFn">
<rdfs:comment>(GovernmentFn ?AREA) denotes the
Government of the GeopoliticalArea ?AREA.  For example,
(GovernmentFn UnitedStates) denotes the Federal-level government of
the United States; (GovernmentFn PuertoRico) denotes the government of
the Commonwealth of Puerto Rico.</rdfs:comment>
<rdf:type rdf:resource = "#UnaryFunction"/>
<rdfs:domain rdf:resource="#GeopoliticalArea"/>
<rdfs:range rdf:resource = "#Government"/>
</owl:ObjectProperty>

<owl:ObjectProperty   rdf:ID= "HoleHostFn">
<rdfs:comment>A UnaryFunction that maps a Hole to
the Object which is its principal host.  The principle host of a Hole
is its maximally connected host (a notion taken here to be defined only
when the argument is a hole).</rdfs:comment>
<rdf:type rdf:resource = "#SpatialRelation"/>
<rdf:type rdf:resource = "#UnaryFunction"/>
<rdf:type rdf:resource = "#TotalValuedRelation"/>
<rdf:type rdf:resource = "#AsymmetricRelation"/>
<rdfs:domain rdf:resource="#Hole"/>
<rdfs:range rdf:resource = "#Object"/>
</owl:ObjectProperty>

<owl:ObjectProperty   rdf:ID= "HoleSkinFn">
<rdfs:comment>A UnaryFunction that maps a Hole to the skin
of the Hole.  The skin of a Hole is the fusion of those superficial
parts (see superficialPart) of the Hole's principal host (see
HoleHostFn) with which the Hole is externally connected.</rdfs:comment>
<rdf:type rdf:resource = "#SpatialRelation"/>
<rdf:type rdf:resource = "#UnaryFunction"/>
<rdf:type rdf:resource = "#TotalValuedRelation"/>
<rdf:type rdf:resource = "#AsymmetricRelation"/>
<rdfs:domain rdf:resource="#Hole"/>
<rdfs:range rdf:resource = "#Object"/>
</owl:ObjectProperty>

<owl:DatatypeProperty  rdf:ID= "ImaginaryPartFn">
<rdfs:comment>(ImaginaryPartFn ?NUMBER) returns
the part of ?NUMBER that has the square root of -1 as its factor.</rdfs:comment>
<rdf:type rdf:resource = "#UnaryFunction"/>
<rdf:type rdf:resource = "#TotalValuedRelation"/>
<rdfs:domain rdf:resource="#ComplexNumber"/>
<rdfs:range rdf:resource = "#ImaginaryNumber"/>
</owl:DatatypeProperty>

<owl:ObjectProperty   rdf:ID= "ImmediateFamilyFn">
<rdfs:comment>(ImmediateFamilyFn ?PERSON) denotes the
immediate family of ?PERSON, i.e. the Group consisting of the parents of
?PERSON and anyone of whom ?PERSON is a parent.</rdfs:comment>
<rdf:type rdf:resource = "#UnaryFunction"/>
<rdfs:domain rdf:resource="#Human"/>
<rdfs:range rdf:resource = "#FamilyGroup"/>
</owl:ObjectProperty>

<owl:ObjectProperty   rdf:ID= "ImmediateFutureFn">
<rdfs:comment>A UnaryFunction that maps a
TimePosition to a short, indeterminate TimeInterval that
immediately follows the TimePosition.</rdfs:comment>
<rdf:type rdf:resource = "#TemporalRelation"/>
<rdf:type rdf:resource = "#UnaryFunction"/>
<rdf:type rdf:resource = "#TotalValuedRelation"/>
<rdfs:domain rdf:resource="#TimePosition"/>
<rdfs:range rdf:resource = "#TimeInterval"/>
</owl:ObjectProperty>

<owl:ObjectProperty   rdf:ID= "ImmediatePastFn">
<rdfs:comment>A UnaryFunction that maps a
TimePosition to a short, indeterminate TimeInterval that
immediately precedes the TimePosition.</rdfs:comment>
<rdf:type rdf:resource = "#TemporalRelation"/>
<rdf:type rdf:resource = "#UnaryFunction"/>
<rdf:type rdf:resource = "#TotalValuedRelation"/>
<rdfs:domain rdf:resource="#TimePosition"/>
<rdfs:range rdf:resource = "#TimeInterval"/>
</owl:ObjectProperty>

<owl:DatatypeProperty  rdf:ID= "IntegerSquareRootFn">
<rdfs:comment>(IntegerSquareRootFn ?NUMBER)
returns the integer square root of ?NUMBER.</rdfs:comment>
<rdf:type rdf:resource = "#UnaryFunction"/>
<rdf:type rdf:resource = "#PartialValuedRelation"/>
<rdfs:domain rdf:resource="#RealNumber"/>
<rdfs:range rdf:resource = "#NonnegativeInteger"/>
</owl:DatatypeProperty>

<owl:ObjectProperty   rdf:ID= "KiloFn">
<rdfs:comment>A UnaryFunction that maps a UnitOfMeasure into
a UnitOfMeasure that is equal to 1,000 units of the original UnitOfMeasure.
For example, (KiloFn Gram) is 1,000 Grams.</rdfs:comment>
<rdf:type rdf:resource = "#UnaryFunction"/>
<rdf:type rdf:resource = "#TotalValuedRelation"/>
<rdfs:domain rdf:resource="#UnitOfMeasure"/>
<rdfs:range rdf:resource = "#UnitOfMeasure"/>
</owl:ObjectProperty>

<owl:DatatypeProperty  rdf:ID= "ListLengthFn">
<rdfs:comment>A Function that takes a List as its sole
argument and returns the number of items in the List.  For example,
(ListLengthFn (ListFn Monday Tuesday Wednesday)) would return the
value 3.</rdfs:comment>
<rdf:type rdf:resource = "#UnaryFunction"/>
<rdf:type rdf:resource = "#TotalValuedRelation"/>
<rdfs:domain rdf:resource="#List"/>
<rdfs:range rdf:resource = "#NonnegativeInteger"/>
</owl:DatatypeProperty>

<owl:DatatypeProperty  rdf:ID= "MagnitudeFn">
<rdfs:comment>The magnitude of a ConstantQuantity is the
numeric value for the quantity.  In other words, MagnitudeFn converts
a ConstantQuantity with an associated UnitOfMeasure into an ordinary
RealNumber.  For example, the magnitude of the ConstantQuantity 2
Kilometers is the RealNumber 2.   Note that the magnitude of a
quantity in a given unit times that unit is equal to the original
quantity.</rdfs:comment>
<rdf:type rdf:resource = "#UnaryFunction"/>
<rdfs:domain rdf:resource="#ConstantQuantity"/>
<rdfs:range rdf:resource = "#RealNumber"/>
</owl:DatatypeProperty>

<owl:ObjectProperty   rdf:ID= "MegaFn">
<rdfs:comment>A UnaryFunction that maps a UnitOfMeasure into
a UnitOfMeasure that is equal to 1,000,000 units of the original
UnitOfMeasure.  For example, (MegaFn Hertz) is 1,000,000 Hertz.</rdfs:comment>
<rdf:type rdf:resource = "#UnaryFunction"/>
<rdf:type rdf:resource = "#TotalValuedRelation"/>
<rdfs:domain rdf:resource="#UnitOfMeasure"/>
<rdfs:range rdf:resource = "#UnitOfMeasure"/>
</owl:ObjectProperty>

<owl:ObjectProperty   rdf:ID= "MicroFn">
<rdfs:comment>A UnaryFunction that maps a UnitOfMeasure into
a UnitOfMeasure that is equal to .000001 units of the original UnitOfMeasure.
For example, (MicroFn Meter) is .000001 Meters.</rdfs:comment>
<rdf:type rdf:resource = "#UnaryFunction"/>
<rdf:type rdf:resource = "#TotalValuedRelation"/>
<rdfs:domain rdf:resource="#UnitOfMeasure"/>
<rdfs:range rdf:resource = "#UnitOfMeasure"/>
</owl:ObjectProperty>

<owl:ObjectProperty   rdf:ID= "MilliFn">
<rdfs:comment>A UnaryFunction that maps a UnitOfMeasure into
a UnitOfMeasure that is equal to .001 units of the original UnitOfMeasure.
For example, (MilliFn Gram) is .001 Grams.</rdfs:comment>
<rdf:type rdf:resource = "#UnaryFunction"/>
<rdf:type rdf:resource = "#TotalValuedRelation"/>
<rdfs:domain rdf:resource="#UnitOfMeasure"/>
<rdfs:range rdf:resource = "#UnitOfMeasure"/>
</owl:ObjectProperty>

<owl:ObjectProperty   rdf:ID= "NanoFn">
<rdfs:comment>A UnaryFunction that maps a UnitOfMeasure into
a UnitOfMeasure that is equal to .000000001 units of the original
UnitOfMeasure.  For example, (MicroFn SecondDuration) is .000000001
SecondDurations.</rdfs:comment>
<rdf:type rdf:resource = "#UnaryFunction"/>
<rdf:type rdf:resource = "#TotalValuedRelation"/>
<rdfs:domain rdf:resource="#UnitOfMeasure"/>
<rdfs:range rdf:resource = "#UnitOfMeasure"/>
</owl:ObjectProperty>

<owl:DatatypeProperty  rdf:ID= "NumeratorFn">
<rdfs:comment>(NumeratorFn ?NUMBER) returns the numerator
of the canonical reduced form ?NUMBER.</rdfs:comment>
<rdf:type rdf:resource = "#UnaryFunction"/>
<rdf:type rdf:resource = "#TotalValuedRelation"/>
<rdfs:domain rdf:resource="#RealNumber"/>
<rdfs:range rdf:resource = "#Integer"/>
</owl:DatatypeProperty>

<owl:ObjectProperty   rdf:ID= "PastFn">
<rdfs:comment>A UnaryFunction that maps a TimePosition
to the TimeInterval that meets it and that begins at
NegativeInfinity.</rdfs:comment>
<rdf:type rdf:resource = "#TemporalRelation"/>
<rdf:type rdf:resource = "#UnaryFunction"/>
<rdf:type rdf:resource = "#TotalValuedRelation"/>
<rdfs:domain rdf:resource="#TimePosition"/>
<rdfs:range rdf:resource = "#TimeInterval"/>
</owl:ObjectProperty>

<owl:ObjectProperty   rdf:ID= "PicoFn">
<rdfs:comment>A UnaryFunction that maps a UnitOfMeasure into
a UnitOfMeasure that is equal to .000000000001 units of the original
UnitOfMeasure.  For example, (PicoFn SecondDuration) is .000000000001
SecondDurations.</rdfs:comment>
<rdf:type rdf:resource = "#UnaryFunction"/>
<rdf:type rdf:resource = "#TotalValuedRelation"/>
<rdfs:domain rdf:resource="#UnitOfMeasure"/>
<rdfs:range rdf:resource = "#UnitOfMeasure"/>
</owl:ObjectProperty>

<owl:ObjectProperty   rdf:ID= "PowerSetFn">
<rdfs:comment>(PowerSetFn ?CLASS) maps the SetOrClass
?CLASS to the SetOrClass of all subclasses of ?CLASS.</rdfs:comment>
<rdf:type rdf:resource = "#UnaryFunction"/>
<rdf:type rdf:resource = "#TotalValuedRelation"/>
<rdfs:domain rdf:resource="#SetOrClass"/>
<rangeSubclass rdf:resource = "#SetOrClass" />
</owl:ObjectProperty>

<owl:DatatypeProperty  rdf:ID= "PredecessorFn">
<rdfs:comment>A UnaryFunction that maps an Integer to
its predecessor, e.g. the predecessor of 5 is 4.</rdfs:comment>
<rdf:type rdf:resource = "#UnaryFunction"/>
<rdf:type rdf:resource = "#TotalValuedRelation"/>
<rdfs:domain rdf:resource="#Integer"/>
<rdfs:range rdf:resource = "#Integer"/>
</owl:DatatypeProperty>

<owl:ObjectProperty   rdf:ID= "PremisesFn">
<rdfs:comment>(PremisesFn ?ARGUMENT) returns the complete
set of premises of the Argument ?ARGUMENT.</rdfs:comment>
<rdf:type rdf:resource = "#UnaryFunction"/>
<rdfs:domain rdf:resource="#Argument"/>
<rdfs:range rdf:resource = "#Proposition"/>
</owl:ObjectProperty>

<owl:DatatypeProperty  rdf:ID= "ProbabilityFn">
<rdfs:comment>One of the basic ProbabilityRelations,
ProbabilityFn is used to state the a priori probability of a state of
affairs.  (ProbabilityFn ?FORMULA) denotes the a priori probability
of ?FORMULA.</rdfs:comment>
<rdf:type rdf:resource = "#ProbabilityRelation"/>
<rdf:type rdf:resource = "#TotalValuedRelation"/>
<rdf:type rdf:resource = "#UnaryFunction"/>
<rdf:type rdf:resource = "#AsymmetricRelation"/>
<rdfs:domain rdf:resource="#Formula"/>
<rdfs:range rdf:resource = "#RealNumber"/>
</owl:DatatypeProperty>

<owl:ObjectProperty   rdf:ID= "PropertyFn">
<rdfs:comment>A UnaryFunction that maps an Agent to the
Set of Objects owned by the Agent.</rdfs:comment>
<rdf:type rdf:resource = "#UnaryFunction"/>
<rdf:type rdf:resource = "#TotalValuedRelation"/>
<rdfs:domain rdf:resource="#Agent"/>
<rdfs:range rdf:resource = "#Set"/>
</owl:ObjectProperty>

<owl:DatatypeProperty  rdf:ID= "RationalNumberFn">
<rdfs:comment>(RationalNumberFn ?NUMBER) returns
the rational representation of ?NUMBER.</rdfs:comment>
<rdf:type rdf:resource = "#UnaryFunction"/>
<rdfs:domain rdf:resource="#Number"/>
<rdfs:range rdf:resource = "#RationalNumber"/>
</owl:DatatypeProperty>

<owl:DatatypeProperty  rdf:ID= "RealNumberFn">
<rdfs:comment>(RealNumberFn ?NUMBER) returns the part of
?NUMBER that is a RealNumber.</rdfs:comment>
<rdf:type rdf:resource = "#UnaryFunction"/>
<rdfs:domain rdf:resource="#Number"/>
<rdfs:range rdf:resource = "#RealNumber"/>
</owl:DatatypeProperty>

<owl:DatatypeProperty  rdf:ID= "ReciprocalFn">
<rdfs:comment>(ReciprocalFn ?NUMBER) is the reciprocal
element of ?NUMBER with respect to the multiplication operator
(MultiplicationFn), i.e. 1/?NUMBER.  Not all numbers have a reciprocal
element.  For example the number 0 does not.  If a number ?NUMBER has a
reciprocal ?RECIP, then the product of ?NUMBER and ?RECIP will be
1, e.g. 3*1/3 = 1.  The reciprocal of an element is equal to
applying the ExponentiationFn function to the element to the power
-1.</rdfs:comment>
<rdf:type rdf:resource = "#UnaryFunction"/>
<rdf:type rdf:resource = "#RelationExtendedToQuantities"/>
<rdf:type rdf:resource = "#TotalValuedRelation"/>
<rdfs:domain rdf:resource="#Quantity"/>
<rdfs:range rdf:resource = "#Quantity"/>
</owl:DatatypeProperty>

<owl:DatatypeProperty  rdf:ID= "RoundFn">
<rdfs:comment>(RoundFn ?NUMBER) is the Integer closest
to ?NUMBER on the number line.  If ?NUMBER is halfway between two
Integers (for example 3.5), it denotes the larger Integer.</rdfs:comment>
<rdf:type rdf:resource = "#UnaryFunction"/>
<rdf:type rdf:resource = "#RelationExtendedToQuantities"/>
<rdf:type rdf:resource = "#TotalValuedRelation"/>
<rdfs:domain rdf:resource="#Quantity"/>
<rdfs:range rdf:resource = "#Quantity"/>
</owl:DatatypeProperty>

<owl:DatatypeProperty  rdf:ID= "SignumFn">
<rdfs:comment>(SignumFn ?NUMBER) denotes the sign of ?NUMBER.
This is one of the following values:  -1, 1, or 0.</rdfs:comment>
<rdf:type rdf:resource = "#UnaryFunction"/>
<rdf:type rdf:resource = "#TotalValuedRelation"/>
<rdfs:domain rdf:resource="#RealNumber"/>
<rdfs:range rdf:resource = "#Integer"/>
</owl:DatatypeProperty>

<owl:DatatypeProperty  rdf:ID= "SineFn">
<rdfs:comment>(SineFn ?DEGREE) is the sine of the
PlaneAngleMeasure ?DEGREE.  The sine of ?DEGREE is the ratio of the side
opposite ?DEGREE to the hypotenuse in a right-angled triangle.</rdfs:comment>
<rdf:type rdf:resource = "#UnaryFunction"/>
<rdf:type rdf:resource = "#TotalValuedRelation"/>
<rdfs:domain rdf:resource="#PlaneAngleMeasure"/>
<rdfs:range rdf:resource = "#RealNumber"/>
</owl:DatatypeProperty>

<owl:DatatypeProperty  rdf:ID= "SquareRootFn">
<rdfs:comment>(SquareRootFn ?NUMBER) is the principal
square root of ?NUMBER.</rdfs:comment>
<rdf:type rdf:resource = "#UnaryFunction"/>
<rdfs:domain rdf:resource="#RealNumber"/>
<rdfs:range rdf:resource = "#Number"/>
</owl:DatatypeProperty>

<owl:DatatypeProperty  rdf:ID= "SuccessorFn">
<rdfs:comment>A UnaryFunction that maps an Integer to
its successor, e.g. the successor of 5 is 6.</rdfs:comment>
<rdf:type rdf:resource = "#UnaryFunction"/>
<rdf:type rdf:resource = "#TotalValuedRelation"/>
<rdfs:domain rdf:resource="#Integer"/>
<rdfs:range rdf:resource = "#Integer"/>
</owl:DatatypeProperty>

<owl:DatatypeProperty  rdf:ID= "TangentFn">
<rdfs:comment>(TangentFn ?DEGREE) is the tangent of the
PlaneAngleMeasure ?DEGREE.  The tangent of ?DEGREE is the ratio of
the side opposite ?DEGREE to the side next to ?DEGREE in a right-angled
triangle.</rdfs:comment>
<rdf:type rdf:resource = "#UnaryFunction"/>
<rdf:type rdf:resource = "#TotalValuedRelation"/>
<rdfs:domain rdf:resource="#PlaneAngleMeasure"/>
<rdfs:range rdf:resource = "#RealNumber"/>
</owl:DatatypeProperty>

<owl:ObjectProperty   rdf:ID= "TeraFn">
<rdfs:comment>A UnaryFunction that maps a UnitOfMeasure
into a UnitOfMeasure that is equal to 1,000,000,000,000 units of the original
UnitOfMeasure.  For example, (TeraFn Hertz) is 1,000,000,000,000 Hertz.</rdfs:comment>
<rdf:type rdf:resource = "#UnaryFunction"/>
<rdf:type rdf:resource = "#TotalValuedRelation"/>
<rdfs:domain rdf:resource="#UnitOfMeasure"/>
<rdfs:range rdf:resource = "#UnitOfMeasure"/>
</owl:ObjectProperty>

<owl:ObjectProperty   rdf:ID= "WealthFn">
<rdfs:comment>A UnaryFunction that maps an Agent to a
CurrencyMeasure specifying the value of the property owned by the Agent.
Note that this Function is generally used in conjunction with the
Function PropertyFn, e.g. (WealthFn (PropertyFn BillGates)) would
return the monetary value of the sum of Bill Gates' holdings.</rdfs:comment>
<rdf:type rdf:resource = "#UnaryFunction"/>
<rdfs:domain rdf:resource="#Agent"/>
<rdfs:range rdf:resource = "#CurrencyMeasure"/>
</owl:ObjectProperty>

<owl:ObjectProperty   rdf:ID= "WhenFn">
<rdfs:comment>A UnaryFunction that maps an Object or
Process to the exact TimeInterval during which it exists.  Note
that, for every TimePoint ?TIME outside of the TimeInterval
(WhenFn ?THING), (time ?THING ?TIME) does not hold.</rdfs:comment>
<rdf:type rdf:resource = "#TemporalRelation"/>
<rdf:type rdf:resource = "#UnaryFunction"/>
<rdf:type rdf:resource = "#TotalValuedRelation"/>
<rdfs:domain rdf:resource="#Physical"/>
<rdfs:range rdf:resource = "#TimeInterval"/>
</owl:ObjectProperty>

<owl:ObjectProperty   rdf:ID= "YearFn">
<rdfs:comment>A UnaryFunction that maps a number to the corresponding calendar
Year.  For example, (YearFn 1912) returns the Class containing just one instance,
the year of 1912.  As might be expected, positive integers return years in the Common Era,
while negative integers return years in B.C.E.  Note that this function returns a Class
as a value.  The reason for this is that the related functions, viz. MonthFn, DayFn,
HourFn, MinuteFn, and SecondFn, are used to generate both specific TimeIntervals
and recurrent intervals, and the only way to do this is to make the domains and ranges of
these functions classes rather than individuals.</rdfs:comment>
<rdf:type rdf:resource = "#TemporalRelation"/>
<rdf:type rdf:resource = "#UnaryFunction"/>
<rdfs:domain rdf:resource="#Integer"/>
<rangeSubclass rdf:resource = "#Year" />
</owl:ObjectProperty>

<owl:ObjectProperty   rdf:ID= "age">
<rdfs:comment>Simply relates an Object to a ConstantQuantity
specifying the age of the Object.</rdfs:comment>
<rdf:type rdf:resource = "#SingleValuedRelation"/>
<rdfs:range rdf:resource = "#TimeDuration"/>
<rdfs:subPropertyOf rdf:resource="#measure"/>
</owl:ObjectProperty>

<owl:ObjectProperty   rdf:ID= "agent">
<rdfs:comment>(agent ?PROCESS ?AGENT) means that ?AGENT is
an active determinant, either animate or inanimate, of the Process
?PROCESS, with or without voluntary intention.  For example, Eve is an
agent in the following proposition: Eve bit an apple.</rdfs:comment>
<rdf:type rdf:resource = "#CaseRole"/>
<rdfs:domain rdf:resource="#Process"/>
<rdfs:range rdf:resource = "#Agent"/>
</owl:ObjectProperty>

<owl:ObjectProperty   rdf:ID= "ancestor">
<rdfs:comment>The transitive closure of the parent predicate.
(ancestor ?DESCENDANT ?ANCESTOR) means that ?ANCESTOR is either the
parent of ?DESCENDANT or the parent of the parent of DESCENDANT or
etc.</rdfs:comment>
<rdf:type rdf:resource = "#TransitiveRelation"/>
<rdf:type rdf:resource = "#IrreflexiveRelation"/>
<rdfs:domain rdf:resource="#Organism"/>
<rdfs:range rdf:resource = "#Organism"/>
<rdfs:subPropertyOf rdf:resource="#familyRelation"/>
</owl:ObjectProperty>

<owl:ObjectProperty   rdf:ID= "angleOfFigure">
<rdfs:comment>(angleOfFigure ?ANGLE ?FIGURE) means that
the TwoDimensionalAngle ?ANGLE is part of the GeometricFigure ?FIGURE.</rdfs:comment>
<rdfs:domain rdf:resource="#TwoDimensionalAngle"/>
<rdfs:range rdf:resource = "#GeometricFigure"/>
<rdfs:subPropertyOf rdf:resource="#geometricPart"/>
</owl:ObjectProperty>

<owl:DatatypeProperty  rdf:ID= "angularMeasure">
<rdfs:comment>(angularMeasure ?ANGLE ?MEASURE) means that
the two-dimensional geometric angle ?ANGLE has the PlaneAngleMeasure of
?MEASURE.</rdfs:comment>
<rdf:type rdf:resource = "#BinaryPredicate"/>
<rdf:type rdf:resource = "#TotalValuedRelation"/>
<rdfs:domain rdf:resource="#TwoDimensionalAngle"/>
<rdfs:range rdf:resource = "#PlaneAngleMeasure"/>
</owl:DatatypeProperty>

<owl:ObjectProperty   rdf:ID= "attends">
<rdfs:comment>(attends ?DEMO ?PERSON) means that ?PERSON attends,
i.e. is a member of the audience, of the performance event ?DEMO.</rdfs:comment>
<rdfs:domain rdf:resource="#Demonstrating"/>
<rdfs:range rdf:resource = "#Human"/>
<rdfs:subPropertyOf rdf:resource="#experiencer"/>
</owl:ObjectProperty>

<owl:ObjectProperty   rdf:ID= "attribute">
<rdfs:comment>(attribute ?OBJECT ?PROPERTY) means that
?PROPERTY is a Attribute of ?OBJECT.  For example,
(attribute MyLittleRedWagon Red).</rdfs:comment>
<rdf:type rdf:resource = "#AsymmetricRelation"/>
<rdf:type rdf:resource = "#IrreflexiveRelation"/>
<rdfs:domain rdf:resource="#Object"/>
<rdfs:subPropertyOf rdf:resource="#property"/>
</owl:ObjectProperty>

<owl:ObjectProperty   rdf:ID= "authors">
<rdfs:comment>(authors ?AGENT ?TEXT) means that ?AGENT is
creatively responsible for ?TEXT.  For example, Agatha Christie is
author of Murder_on_the_Orient_Express.</rdfs:comment>
<rdf:type rdf:resource = "#BinaryPredicate"/>
<rdf:type rdf:resource = "#AsymmetricRelation"/>
<rdfs:domain rdf:resource="#Agent"/>
<rdfs:range rdf:resource = "#Text"/>
</owl:ObjectProperty>

<owl:ObjectProperty   rdf:ID= "before">
<rdfs:comment>(before ?POINT1 ?POINT2) means that ?POINT1
precedes ?POINT2 on the universal timeline.</rdfs:comment>
<rdf:type rdf:resource = "#TemporalRelation"/>
<rdf:type rdf:resource = "#IrreflexiveRelation"/>
<rdf:type rdf:resource = "#TransitiveRelation"/>
<rdfs:domain rdf:resource="#TimePoint"/>
<rdfs:range rdf:resource = "#TimePoint"/>
<rdfs:subPropertyOf rdf:resource="#beforeOrEqual"/>
<relatedInternalConcept rdf:resource = "#earlier" />
</owl:ObjectProperty>

<owl:ObjectProperty   rdf:ID= "beforeOrEqual">
<rdfs:comment>(beforeOrEqual ?POINT1 ?POINT2) means that ?POINT1
is identical with ?POINT2 or occurs before it on the universal timeline.</rdfs:comment>
<rdf:type rdf:resource = "#BinaryPredicate"/>
<rdf:type rdf:resource = "#TemporalRelation"/>
<rdf:type rdf:resource = "#PartialOrderingRelation"/>
<rdfs:domain rdf:resource="#TimePoint"/>
<rdfs:range rdf:resource = "#TimePoint"/>
</owl:ObjectProperty>

<owl:ObjectProperty   rdf:ID= "believes">
<rdfs:comment>The epistemic predicate of belief.
(believes ?AGENT ?FORMULA) means that ?AGENT believes the proposition
expressed by ?FORMULA.</rdfs:comment>
<rdf:type rdf:resource = "#PropositionalAttitude"/>
<rdfs:domain rdf:resource="#CognitiveAgent"/>
<rdfs:range rdf:resource = "#Formula"/>
<rdfs:subPropertyOf rdf:resource="#inScopeOfInterest"/>
</owl:ObjectProperty>

<owl:ObjectProperty   rdf:ID= "bottom">
<rdfs:comment>(bottom ?BOTTOM ?OBJECT) holds if ?BOTTOM is the
lowest or deepest maximal superficial part of ?OBJECT.</rdfs:comment>
<rdfs:domain rdf:resource="#SelfConnectedObject"/>
<rdfs:range rdf:resource = "#SelfConnectedObject"/>
<rdfs:subPropertyOf rdf:resource="#superficialPart"/>
</owl:ObjectProperty>

<owl:ObjectProperty   rdf:ID= "brother">
<rdfs:comment>The general relationship of being a brother.
(brother ?MAN ?PERSON) means that ?MAN is the brother of ?PERSON.</rdfs:comment>
<rdf:type rdf:resource = "#IrreflexiveRelation"/>
<rdf:type rdf:resource = "#TransitiveRelation"/>
<rdfs:domain rdf:resource="#Man"/>
<rdfs:range rdf:resource = "#Human"/>
<rdfs:subPropertyOf rdf:resource="#sibling"/>
</owl:ObjectProperty>

<owl:ObjectProperty   rdf:ID= "causes">
<rdfs:comment>The causation relation between instances of Process.
(causes ?PROCESS1 ?PROCESS2) means that the instance of Process ?PROCESS1
brings about the instance of Process ?PROCESS2.</rdfs:comment>
<rdf:type rdf:resource = "#BinaryPredicate"/>
<rdf:type rdf:resource = "#AsymmetricRelation"/>
<rdfs:domain rdf:resource="#Process"/>
<rdfs:range rdf:resource = "#Process"/>
<relatedInternalConcept rdf:resource = "#causesSubclass" />
</owl:ObjectProperty>

<owl:ObjectProperty   rdf:ID= "causesSubclass">
<rdfs:comment>The causation relation between subclasses of Process.
(causesSubclass ?PROCESS1 ?PROCESS2) means that the subclass of Process ?PROCESS1
brings about the subclass of Process ?PROCESS2, e.g. (causesSubclass Killing
Death).</rdfs:comment>
<rdf:type rdf:resource = "#BinaryPredicate"/>
<rdf:type rdf:resource = "#AsymmetricRelation"/>
<rdfs:domain rdf:resource="#Process"/>
<rdfs:range rdf:resource = "#Process"/>
</owl:ObjectProperty>

<owl:ObjectProperty   rdf:ID= "citizen">
<rdfs:comment>(citizen ?PERSON ?NATION) means that the
Human ?PERSON is a citizen of Nation ?NATION.</rdfs:comment>
<rdf:type rdf:resource = "#BinaryPredicate"/>
<rdf:type rdf:resource = "#AsymmetricRelation"/>
<rdfs:domain rdf:resource="#Human"/>
<rdfs:range rdf:resource = "#Nation"/>
</owl:ObjectProperty>

<owl:ObjectProperty   rdf:ID= "closedOn">
<rdfs:comment>A BinaryFunction is closed on a SetOrClass
if it is defined for all instances of the SetOrClass and its value is
always an instance of the SetOrClass.</rdfs:comment>
<rdf:type rdf:resource = "#BinaryPredicate"/>
<rdf:type rdf:resource = "#AsymmetricRelation"/>
<rdfs:domain rdf:resource="#Function"/>
<rdfs:range rdf:resource = "#SetOrClass"/>
</owl:ObjectProperty>

<owl:ObjectProperty   rdf:ID= "completelyFills">
<rdfs:comment>(completelyFills ?OBJ ?HOLE)
means that some part of the Object ?OBJ fills the Hole ?HOLE.
Note that if (completelyFills ?OBJ1 ?HOLE) and (part
?OBJ1 ?OBJ2), then (completelyFills ?OBJ2 ?HOLE).</rdfs:comment>
<rdf:type rdf:resource = "#AsymmetricRelation"/>
<rdfs:subPropertyOf rdf:resource="#partiallyFills"/>
</owl:ObjectProperty>

<owl:ObjectProperty   rdf:ID= "component">
<rdfs:comment>A specialized common sense notion of part
for heterogeneous parts of complexes. (component ?COMPONENT ?WHOLE)
means that ?COMPONENT is a component of ?WHOLE. Examples of component
include the doors and walls of a house, the states or provinces of a
country, or the limbs and organs of an animal.  Compare piece, which
is also a subrelation of part.</rdfs:comment>
<rdfs:domain rdf:resource="#CorpuscularObject"/>
<rdfs:range rdf:resource = "#CorpuscularObject"/>
<rdfs:subPropertyOf rdf:resource="#part"/>
</owl:ObjectProperty>

<owl:ObjectProperty   rdf:ID= "conclusion">
<rdfs:comment>(conclusion ?ARGUMENT ?PROPOSITION) means that
the Proposition ?PROPOSITION is the conclusion explicitly drawn from the
Argument ?ARGUMENT.  Note that it may or may not be the case that ?ARGUMENT
entails ?PROPOSITION.</rdfs:comment>
<rdf:type rdf:resource = "#BinaryPredicate"/>
<rdf:type rdf:resource = "#SingleValuedRelation"/>
<rdf:type rdf:resource = "#TotalValuedRelation"/>
<rdfs:domain rdf:resource="#Argument"/>
<rdfs:range rdf:resource = "#Proposition"/>
</owl:ObjectProperty>

<owl:ObjectProperty   rdf:ID= "connected">
<rdfs:comment>(connected ?OBJ1 ?OBJ2) means that ?OBJ1
meetsSpatially ?OBJ2 or that ?OBJ1 overlapsSpatially ?OBJ2.</rdfs:comment>
<rdf:type rdf:resource = "#BinaryPredicate"/>
<rdf:type rdf:resource = "#SpatialRelation"/>
<rdf:type rdf:resource = "#ReflexiveRelation"/>
<rdf:type rdf:resource = "#SymmetricRelation"/>
<rdfs:domain rdf:resource="#Object"/>
<rdfs:range rdf:resource = "#Object"/>
</owl:ObjectProperty>

<owl:ObjectProperty   rdf:ID= "linked">
<rdfs:comment>(linked ?OBJ1 ?OBJ2) means that between ?OBJ1
and ?OBJ2 extist some type of connection or link, e.g. hypermedia link etc.</rdfs:comment>
<rdf:type rdf:resource = "#BinaryPredicate"/>
<rdf:type rdf:resource = "#ReflexiveRelation"/>
<rdf:type rdf:resource = "#SymmetricRelation"/>
<rdfs:domain rdf:resource="#Object"/>
<rdfs:range rdf:resource = "#Object"/>
</owl:ObjectProperty>

<owl:ObjectProperty   rdf:ID= "connectedEngineeringComponents">
<rdfs:comment>This is the most general
connection relation between EngineeringComponents.  If
(connectedEngineeringComponents ?COMP1 ?COMP2), then neither ?COMP1 nor
?COMP2 can be an engineeringSubcomponent of the other.  The relation
connectedEngineeringComponents is a SymmetricRelation; there is no
information in the direction of connection between two components.  It is
also an IrreflexiveRelation; no EngineeringComponent bears this relation
to itself.  Note that this relation does not associate a name or type
with the connection.</rdfs:comment>
<rdf:type rdf:resource = "#SymmetricRelation"/>
<rdf:type rdf:resource = "#IrreflexiveRelation"/>
<rdfs:domain rdf:resource="#EngineeringComponent"/>
<rdfs:range rdf:resource = "#EngineeringComponent"/>
<rdfs:subPropertyOf rdf:resource="#connected"/>
</owl:ObjectProperty>

<owl:ObjectProperty   rdf:ID= "considers">
<rdfs:comment>(considers ?AGENT ?FORMULA) means that ?AGENT
considers or wonders about the truth of the proposition expressed by
?FORMULA.</rdfs:comment>
<rdf:type rdf:resource = "#PropositionalAttitude"/>
<rdfs:domain rdf:resource="#CognitiveAgent"/>
<rdfs:range rdf:resource = "#Formula"/>
<rdfs:subPropertyOf rdf:resource="#inScopeOfInterest"/>
</owl:ObjectProperty>

<owl:ObjectProperty   rdf:ID= "consistent">
<rdfs:comment>(consistent ?PROP1 ?PROP2) means that the two
Propositions ?PROP1 and ?PROP2 are consistent with one another, i.e. it
is possible for both of them to be true at the same time.</rdfs:comment>
<rdf:type rdf:resource = "#BinaryPredicate"/>
<rdf:type rdf:resource = "#SymmetricRelation"/>
<rdfs:domain rdf:resource="#Proposition"/>
<rdfs:range rdf:resource = "#Proposition"/>
</owl:ObjectProperty>

<owl:ObjectProperty   rdf:ID= "contains">
<rdfs:comment>The relation of spatial containment for two
separable objects.  When the two objects are not separable (e.g. an
automobile and one of its seats), the relation of part should be used.
(contains ?OBJ1 ?OBJ2) means that the SelfConnectedObject ?OBJ1 has
a space (i.e. a Hole) which is at least partially filled by ?OBJ2.</rdfs:comment>
<rdf:type rdf:resource = "#SpatialRelation"/>
<rdf:type rdf:resource = "#AsymmetricRelation"/>
<rdfs:domain rdf:resource="#SelfConnectedObject"/>
<rdfs:range rdf:resource = "#Object"/>
<rdfs:subPropertyOf rdf:resource="#partlyLocated"/>
<disjointRelation rdf:resource = "#part" />
</owl:ObjectProperty>

<owl:ObjectProperty   rdf:ID= "containsInformation">
<rdfs:comment>A subrelation of represents.  This
predicate relates a ContentBearingObject to the Proposition that is
expressed by the ContentBearingObject. Examples include the relationships
between a physical novel and its story and between a printed score and its
musical content.</rdfs:comment>
<rdf:type rdf:resource = "#BinaryPredicate"/>
<rdf:type rdf:resource = "#AsymmetricRelation"/>
<rdfs:domain rdf:resource="#ContentBearingObject"/>
<rdfs:range rdf:resource = "#Proposition"/>
<rdfs:subPropertyOf rdf:resource="#represents"/>
</owl:ObjectProperty>

<owl:ObjectProperty   rdf:ID= "cooccur">
<rdfs:comment>(cooccur ?THING1 ?THING2) means that the
Object or Process ?THING1 occurs at the same time as, together with,
or jointly with the Object or Process ?THING2.  This covers the
following temporal relations:  is co-incident with, is concurrent with,
is contemporaneous with, and is concomitant with.</rdfs:comment>
<rdf:type rdf:resource = "#BinaryPredicate"/>
<rdf:type rdf:resource = "#TemporalRelation"/>
<rdf:type rdf:resource = "#EquivalenceRelation"/>
<rdfs:domain rdf:resource="#Physical"/>
<rdfs:range rdf:resource = "#Physical"/>
</owl:ObjectProperty>

<owl:ObjectProperty   rdf:ID= "copy">
<rdfs:comment>relates an Object to an exact copy of the
Object, where an exact copy is indistinguishable from the original
with regard to every property except (possibly) spatial and/or temporal
location.</rdfs:comment>
<rdf:type rdf:resource = "#BinaryPredicate"/>
<rdf:type rdf:resource = "#EquivalenceRelation"/>
<rdfs:domain rdf:resource="#Object"/>
<rdfs:range rdf:resource = "#Object"/>
</owl:ObjectProperty>

<owl:ObjectProperty   rdf:ID= "crosses">
<rdfs:comment>(crosses ?OBJ1 ?OBJ2) means that
Object ?OBJ1 traverses Object ?OBJ2, without being connected
to it.</rdfs:comment>
<rdf:type rdf:resource = "#AsymmetricRelation"/>
<rdf:type rdf:resource = "#TransitiveRelation"/>
<rdfs:subPropertyOf rdf:resource="#traverses"/>
<disjointRelation rdf:resource = "#connected" />
</owl:ObjectProperty>

<owl:ObjectProperty   rdf:ID= "date">
<rdfs:comment>A BinaryPredicate that specifies a
TimePosition in absolute calendar time, at the resolution
of one day, for a particular Object or Process.</rdfs:comment>
<rdf:type rdf:resource = "#BinaryPredicate"/>
<rdf:type rdf:resource = "#SingleValuedRelation"/>
<rdf:type rdf:resource = "#AsymmetricRelation"/>
<rdfs:domain rdf:resource="#Physical"/>
<rdfs:range rdf:resource = "#Day"/>
<rdfs:subPropertyOf rdf:resource="#time"/>
</owl:ObjectProperty>

<owl:ObjectProperty   rdf:ID= "daughter">
<rdfs:comment>The general relationship of daughterhood.
(daughter ?CHILD ?PARENT) means that ?CHILD is the biological daughter
of ?PARENT.</rdfs:comment>
<rdfs:domain rdf:resource="#Woman"/>
<rdfs:range rdf:resource = "#Human"/>
<rdfs:subPropertyOf rdf:resource="#parent"/>
</owl:ObjectProperty>

<owl:ObjectProperty   rdf:ID= "decreasesLikelihood">
<rdfs:comment>One of the basic ProbabilityRelations.
(decreasesLikelihood ?FORMULA1 ?FORMULA2) means that ?FORMULA2 is less
likely to be true if ?FORMULA1 is true.</rdfs:comment>
<rdf:type rdf:resource = "#ProbabilityRelation"/>
<rdf:type rdf:resource = "#BinaryPredicate"/>
<rdf:type rdf:resource = "#IrreflexiveRelation"/>
<rdfs:domain rdf:resource="#Formula"/>
<rdfs:range rdf:resource = "#Formula"/>
</owl:ObjectProperty>

<owl:ObjectProperty   rdf:ID= "desires">
<rdfs:comment>(desires ?AGENT ?FORMULA) means that ?AGENT wants
to bring about the state of affairs expressed by ?FORMULA.  Note that there
is no implication that what is desired by the agent is not already true.
Note too that desires is distinguished from wants only in that the former
is a PropositionalAttitude, while wants is an ObjectAttitude.</rdfs:comment>
<rdf:type rdf:resource = "#PropositionalAttitude"/>
<rdfs:domain rdf:resource="#CognitiveAgent"/>
<rdfs:range rdf:resource = "#Formula"/>
<rdfs:subPropertyOf rdf:resource="#inScopeOfInterest"/>
<relatedInternalConcept rdf:resource = "#wants" />
</owl:ObjectProperty>

<owl:ObjectProperty   rdf:ID= "destination">
<rdfs:comment>(destination ?PROCESS ?GOAL) means that
?GOAL is the target or goal of the Process ?PROCESS.  For example,
Danbury would be the destination in the following proposition:  Bob went
to Danbury.  Note that this is a very general CaseRole and, in
particular, that it covers the concepts of 'recipient' and 'beneficiary'.
Thus, John would be the destination in the following proposition:
Tom gave a book to John.</rdfs:comment>
<rdf:type rdf:resource = "#CaseRole"/>
<rdfs:domain rdf:resource="#Process"/>
<rdfs:range rdf:resource = "#Entity"/>
</owl:ObjectProperty>

<owl:ObjectProperty   rdf:ID= "developmentalForm">
<rdfs:comment>(developmentalForm ?OBJECT ?FORM)
means that ?FORM is an earlier stage in the individual maturation of
?OBJECT.  For example, tadpole and caterpillar are developmentalForms
of frogs and butterflies, respectively.</rdfs:comment>
<rdf:type rdf:resource = "#BinaryPredicate"/>
<rdf:type rdf:resource = "#AsymmetricRelation"/>
<rdf:type rdf:resource = "#TransitiveRelation"/>
<rdfs:domain rdf:resource="#OrganicObject"/>
<rdfs:range rdf:resource = "#DevelopmentalAttribute"/>
<rdfs:subPropertyOf rdf:resource="#attribute"/>
</owl:ObjectProperty>

<owl:ObjectProperty   rdf:ID= "diameter">
<rdfs:comment>BinaryPredicate that is used to state the
measure of a circular Object from side to side.</rdfs:comment>
<rdfs:subPropertyOf rdf:resource="#width"/>
</owl:ObjectProperty>

<owl:ObjectProperty   rdf:ID= "direction">
<rdfs:comment>(direction ?PROC ?ATTR) means that the
Process ?PROC is moving in the direction ?ATTR.  For example, one
would use this Predicate to represent the fact that Max is moving
North.</rdfs:comment>
<rdf:type rdf:resource = "#CaseRole"/>
<rdfs:domain rdf:resource="#Process"/>
<rdfs:range rdf:resource = "#DirectionalAttribute"/>
</owl:ObjectProperty>

<owl:ObjectProperty   rdf:ID= "disjoint">
<rdfs:comment>Classes are disjoint only if they share no
instances, i.e. just in case the result of applying IntersectionFn to
them is empty.</rdfs:comment>
<rdf:type rdf:resource = "#BinaryPredicate"/>
<rdf:type rdf:resource = "#SymmetricRelation"/>
<rdfs:domain rdf:resource="#SetOrClass"/>
<rdfs:range rdf:resource = "#SetOrClass"/>
</owl:ObjectProperty>

<owl:ObjectProperty   rdf:ID= "distributes">
<rdfs:comment>A BinaryFunction ?FUNCTION1 is
distributive over another BinaryFunction ?FUNCTION2 just in case
(?FUNCTION1 ?INST1 (?FUNCTION2 ?INST2 ?INST3)) is equal to
(?FUNCTION2 (?FUNCTION1 ?INST1 ?INST2) (?FUNCTION1 ?INST1 ?INST3)),
for all ?INST1, ?INST2, and ?INST3.</rdfs:comment>
<rdf:type rdf:resource = "#BinaryPredicate"/>
<rdf:type rdf:resource = "#BinaryRelation"/>
<rdfs:domain rdf:resource="#BinaryFunction"/>
<rdfs:range rdf:resource = "#BinaryFunction"/>
</owl:ObjectProperty>

<owl:ObjectProperty   rdf:ID= "documentation">
<rdfs:comment>A relation between objects in the domain
of discourse and strings of natural language text.  The domain of
documentation is not constants (names), but the objects themselves.
This means that one does not quote the names when associating them with
their documentation.</rdfs:comment>
<rdf:type rdf:resource = "#BinaryPredicate"/>
<rdf:type rdf:resource = "#AsymmetricRelation"/>
<rdfs:domain rdf:resource="#Entity"/>
<rdfs:range rdf:resource = "#SymbolicString"/>
</owl:ObjectProperty>

<owl:ObjectProperty   rdf:ID= "duration">
<rdfs:comment>(duration ?POS ?TIME) means that the
duration of the TimePosition ?POS is ?TIME.  Note that this
Predicate can be used in conjunction with the Function WhenFn
to specify the duration of any instance of Physical.</rdfs:comment>
<rdf:type rdf:resource = "#BinaryPredicate"/>
<rdf:type rdf:resource = "#AsymmetricRelation"/>
<rdf:type rdf:resource = "#TotalValuedRelation"/>
<rdfs:domain rdf:resource="#TimeInterval"/>
<rdfs:range rdf:resource = "#TimeDuration"/>
</owl:ObjectProperty>

<owl:ObjectProperty   rdf:ID= "during">
<rdfs:comment>(during ?INTERVAL1 ?INTERVAL2) means that
?INTERVAL1 starts after and ends before ?INTERVAL2.</rdfs:comment>
<rdf:type rdf:resource = "#TransitiveRelation"/>
<rdf:type rdf:resource = "#IrreflexiveRelation"/>
<rdfs:domain rdf:resource="#TimeInterval"/>
<rdfs:range rdf:resource = "#TimeInterval"/>
<rdfs:subPropertyOf rdf:resource="#temporalPart"/>
<rdfs:subPropertyOf rdf:resource="#overlapsTemporally"/>
</owl:ObjectProperty>

<owl:ObjectProperty   rdf:ID= "earlier">
<rdfs:comment>(earlier ?INTERVAL1 ?INTERVAL2) means that
the TimeInterval ?INTERVAL1 ends before the TimeInterval ?INTERVAL2
begins.</rdfs:comment>
<rdf:type rdf:resource = "#BinaryPredicate"/>
<rdf:type rdf:resource = "#TemporalRelation"/>
<rdf:type rdf:resource = "#TransitiveRelation"/>
<rdf:type rdf:resource = "#IrreflexiveRelation"/>
<rdfs:domain rdf:resource="#TimeInterval"/>
<rdfs:range rdf:resource = "#TimeInterval"/>
</owl:ObjectProperty>

<owl:ObjectProperty   rdf:ID= "editor">
<rdfs:comment>(editor ?AGENT ?TEXT) means that ?AGENT is
an editor of ?TEXT.</rdfs:comment>
<rdf:type rdf:resource = "#BinaryPredicate"/>
<rdf:type rdf:resource = "#AsymmetricRelation"/>
<rdfs:domain rdf:resource="#Agent"/>
<rdfs:range rdf:resource = "#Text"/>
</owl:ObjectProperty>

<owl:ObjectProperty   rdf:ID= "element">
<rdfs:comment>(element ?ENTITY ?SET) is true just in case
?ENTITY is contained in the Set ?SET.  An Entity can be an element
of another Entity only if the latter is a Set.</rdfs:comment>
<rdf:type rdf:resource = "#BinaryPredicate"/>
<rdf:type rdf:resource = "#AsymmetricRelation"/>
<rdf:type rdf:resource = "#IntransitiveRelation"/>
<rdfs:domain rdf:resource="#Entity"/>
<rdfs:range rdf:resource = "#Set"/>
<rdfs:subPropertyOf rdf:resource="#instance"/>
</owl:ObjectProperty>

<owl:ObjectProperty   rdf:ID= "employs">
<rdfs:comment>(employs ?ORG ?PERSON) means that ?ORG has
hired ?PERSON and currently retains ?PERSON, on a salaried, hourly
or contractual basis, to provide services in exchange for monetary
compensation.</rdfs:comment>
<rdf:type rdf:resource = "#BinaryPredicate"/>
<rdfs:domain rdf:resource="#Organization"/>
<rdfs:range rdf:resource = "#CognitiveAgent"/>
</owl:ObjectProperty>

<owl:ObjectProperty   rdf:ID= "engineeringSubcomponent">
<rdfs:comment>(engineeringSubcomponent ?SUB
?SUPER) means that the EngineeringComponent ?SUB is structurally a
properPart of ?SUPER.  This relation is an AsymmetricRelation, since
two EngineeringComponents cannot be subcomponents of each other.</rdfs:comment>
<rdfs:domain rdf:resource="#EngineeringComponent"/>
<rdfs:range rdf:resource = "#EngineeringComponent"/>
<rdfs:subPropertyOf rdf:resource="#properPart"/>
</owl:ObjectProperty>

<owl:ObjectProperty   rdf:ID= "entails">
<rdfs:comment>The operator of logical entailment.  (entails
?FORMULA1 ?FORMULA2) means that ?FORMULA2 can be derived from ?FORMULA1
by means of the proof theory of SUO-KIF.</rdfs:comment>
<rdf:type rdf:resource = "#BinaryPredicate"/>
<rdfs:domain rdf:resource="#Formula"/>
<rdfs:range rdf:resource = "#Formula"/>
</owl:ObjectProperty>

<owl:ObjectProperty   rdf:ID= "equal">
<rdfs:comment>(equal ?ENTITY1 ?ENTITY2) is true just in case
?ENTITY1 is identical with ?ENTITY2.</rdfs:comment>
<rdf:type rdf:resource = "#BinaryPredicate"/>
<rdf:type rdf:resource = "#EquivalenceRelation"/>
<rdf:type rdf:resource = "#RelationExtendedToQuantities"/>
<rdfs:domain rdf:resource="#Entity"/>
<rdfs:range rdf:resource = "#Entity"/>
</owl:ObjectProperty>

<owl:ObjectProperty   rdf:ID= "equivalenceRelationOn">
<rdfs:comment>A BinaryRelation is an
equivalenceRelationOn a SetOrClass only if the relation is reflexiveOn
the SetOrClass and it is both a TransitiveRelation and a
SymmetricRelation.</rdfs:comment>
<rdf:type rdf:resource = "#BinaryPredicate"/>
<rdf:type rdf:resource = "#AsymmetricRelation"/>
<rdfs:domain rdf:resource="#BinaryRelation"/>
<rdfs:range rdf:resource = "#SetOrClass"/>
</owl:ObjectProperty>

<owl:ObjectProperty   rdf:ID= "equivalentContentClass">
<rdfs:comment>A BinaryPredicate that relates two
subclasses of ContentBearingObject.  (equivalentContentClass ?CLASS1
?CLASS2) means that the content expressed by each instance of ?CLASS1 is
also expressed by each instance of ?CLASS2, and vice versa.  An example
would be the relationship between English and Russian editions of Agatha
Christie's 'Murder on the Orient Express'.  Note that
(equivalentContentClass ?CLASS1 ?CLASS2) implies (subsumesContentClass
?CLASS1 ?CLASS2) and (subsumesContentClass ?CLASS2 ?CLASS1).</rdfs:comment>
<rdf:type rdf:resource = "#EquivalenceRelation"/>
<rdfs:domain rdf:resource="#ContentBearingObject"/>
<rdfs:range rdf:resource = "#ContentBearingObject"/>
<rdfs:subPropertyOf rdf:resource="#subsumesContentClass"/>
</owl:ObjectProperty>

<owl:ObjectProperty   rdf:ID= "equivalentContentInstance">
<rdfs:comment>A BinaryPredicate relating two
instances of ContentBearingObject.  (equivalentContentInstance
?OBJ1 ?OBJ2) means that the content expressed by ?OBJ1 is identical to
the content expressed by ?OBJ2.  An example would be the relationship
between a handwritten draft of a letter to one's lawyer and a typed
copy of the same letter.  Note that (equivalentContentInstance ?OBJ1
?OBJ2) implies (subsumesContentInstance ?OBJ1 ?OBJ2) and
(subsumesContentInstance ?OBJ2 ?OBJ2).</rdfs:comment>
<rdf:type rdf:resource = "#EquivalenceRelation"/>
<rdfs:domain rdf:resource="#ContentBearingObject"/>
<rdfs:range rdf:resource = "#ContentBearingObject"/>
<rdfs:subPropertyOf rdf:resource="#subsumesContentInstance"/>
<relatedInternalConcept rdf:resource = "#equivalentContentClass" />
</owl:ObjectProperty>

<owl:ObjectProperty   rdf:ID= "exactlyLocated">
<rdfs:comment>The actual, minimal location of an
Object.  This is a subrelation of the more general Predicate
located.</rdfs:comment>
<rdfs:subPropertyOf rdf:resource="#located"/>
</owl:ObjectProperty>

<owl:ObjectProperty   rdf:ID= "experiencer">
<rdfs:comment>(experiencer ?PROCESS ?AGENT) means
that ?AGENT experiences the Process ?PROCESS.  For example, Yojo
is the experiencer of seeing in the following proposition:  Yojo
sees the fish.  Note that experiencer, unlike agent, does
not entail a causal relation between its arguments.</rdfs:comment>
<rdf:type rdf:resource = "#CaseRole"/>
<rdfs:domain rdf:resource="#Process"/>
<rdfs:range rdf:resource = "#Agent"/>
</owl:ObjectProperty>

<owl:ObjectProperty   rdf:ID= "exploits">
<rdfs:comment>(exploits ?OBJ ?AGENT) means that ?OBJ is used
by ?AGENT as a resource in an unspecified instance of Process.  This
Predicate, as its corresponding axiom indicates, is a composition of the
relations agent and resource.</rdfs:comment>
<rdf:type rdf:resource = "#BinaryPredicate"/>
<rdf:type rdf:resource = "#AsymmetricRelation"/>
<rdfs:domain rdf:resource="#Object"/>
<rdfs:range rdf:resource = "#Agent"/>
</owl:ObjectProperty>

<owl:ObjectProperty   rdf:ID= "expressedInLanguage">
<rdfs:comment>(expressedInLanguage ?EXPRESS ?LANG)
means that the LinguisticExpression ?EXPRESS is part of the Language
?LANG.</rdfs:comment>
<rdf:type rdf:resource = "#BinaryPredicate"/>
<rdf:type rdf:resource = "#AsymmetricRelation"/>
<rdfs:domain rdf:resource="#LinguisticExpression"/>
<rdfs:range rdf:resource = "#Language"/>
</owl:ObjectProperty>

<owl:ObjectProperty   rdf:ID= "faces">
<rdfs:comment>(faces ?OBJ ?DIRECTION) means that the front of
?OBJ (see FrontFn) is positioned towards the compass direction ?DIRECTION.
More precisely, it means that if a line were extended from the center of
?DIRECTION, the line would intersect with the front of ?OBJ before it
intersected with its back (see BackFn).</rdfs:comment>
<rdf:type rdf:resource = "#BinaryPredicate"/>
<rdfs:domain rdf:resource="#Object"/>
<rdfs:range rdf:resource = "#DirectionalAttribute"/>
</owl:ObjectProperty>

<owl:ObjectProperty   rdf:ID= "familyRelation">
<rdfs:comment>A very general Predicate for biological
relationships. (familyRelation ?ORGANISM1 ?ORGANISM2) means that
?ORGANISM1 and ?ORGANISM2 are biologically derived from a common ancestor.</rdfs:comment>
<rdf:type rdf:resource = "#BinaryPredicate"/>
<rdf:type rdf:resource = "#EquivalenceRelation"/>
<rdfs:domain rdf:resource="#Organism"/>
<rdfs:range rdf:resource = "#Organism"/>
</owl:ObjectProperty>

<owl:ObjectProperty   rdf:ID= "father">
<rdfs:comment>The general relationship of fatherhood.
(father ?CHILD ?FATHER) means that ?FATHER is the biological father
of ?CHILD.</rdfs:comment>
<rdf:type rdf:resource = "#SingleValuedRelation"/>
<rdfs:domain rdf:resource="#Organism"/>
<rdfs:range rdf:resource = "#Organism"/>
<rdfs:subPropertyOf rdf:resource="#parent"/>
</owl:ObjectProperty>

<owl:ObjectProperty   rdf:ID= "fills">
<rdfs:comment>Holes can be filled.  (fills ?OBJ ?HOLE)
means that the Object ?OBJ fills the Hole ?HOLE.  Note that
fills here means perfectly filled.</rdfs:comment>
<rdf:type rdf:resource = "#AsymmetricRelation"/>
<rdfs:domain rdf:resource="#Object"/>
<rdfs:range rdf:resource = "#Hole"/>
<rdfs:subPropertyOf rdf:resource="#completelyFills"/>
<rdfs:subPropertyOf rdf:resource="#properlyFills"/>
<relatedInternalConcept rdf:resource = "#Fillable" />
</owl:ObjectProperty>

<owl:ObjectProperty   rdf:ID= "finishes">
<rdfs:comment>(finishes ?INTERVAL1 ?INTERVAL2) means that
?INTERVAL1 and ?INTERVAL2 are both TimeIntervals that have the same
ending TimePoint and that ?INTERVAL2 begins before ?INTERVAL1.</rdfs:comment>
<rdf:type rdf:resource = "#TemporalRelation"/>
<rdf:type rdf:resource = "#TransitiveRelation"/>
<rdf:type rdf:resource = "#IrreflexiveRelation"/>
<rdfs:domain rdf:resource="#TimeInterval"/>
<rdfs:range rdf:resource = "#TimeInterval"/>
<rdfs:subPropertyOf rdf:resource="#temporalPart"/>
</owl:ObjectProperty>

<owl:ObjectProperty   rdf:ID= "frequency">
<rdfs:comment>(frequency ?PROC ?TIME) means that the
Process type of ?PROC recurs after every interval of ?TIME.</rdfs:comment>
<rdf:type rdf:resource = "#BinaryPredicate"/>
<rdf:type rdf:resource = "#AsymmetricRelation"/>
<rdfs:domain rdf:resource="#Process"/>
<rdfs:range rdf:resource = "#TimeDuration"/>
</owl:ObjectProperty>

<owl:ObjectProperty   rdf:ID= "geographicSubregion">
<rdfs:comment>(geographicSubregion ?PART ?WHOLE)
means that the GeographicArea ?PART is part of the GeographicArea
?WHOLE.</rdfs:comment>
<rdf:type rdf:resource = "#BinaryPredicate"/>
<rdf:type rdf:resource = "#TransitiveRelation"/>
<rdf:type rdf:resource = "#AsymmetricRelation"/>
<rdfs:domain rdf:resource="#GeographicArea"/>
<rdfs:range rdf:resource = "#GeographicArea"/>
<rdfs:subPropertyOf rdf:resource="#properPart"/>
<rdfs:subPropertyOf rdf:resource="#located"/>
</owl:ObjectProperty>

<owl:ObjectProperty   rdf:ID= "geometricPart">
<rdfs:comment>(geometricPart ?PART ?WHOLE) means that the
GeometricFigure ?PART is part of the GeometricFigure ?WHOLE.</rdfs:comment>
<rdf:type rdf:resource = "#BinaryPredicate"/>
<rdf:type rdf:resource = "#PartialOrderingRelation"/>
<rdfs:domain rdf:resource="#GeometricFigure"/>
<rdfs:range rdf:resource = "#GeometricFigure"/>
</owl:ObjectProperty>

<owl:ObjectProperty   rdf:ID= "geopoliticalSubdivision">
<rdfs:comment>(geopoliticalSubdivision
?AREA1 ?AREA2) means that ?AREA1 is any geopolitical part of ?AREA2;
that is, ?AREA1 is an integral geographicSubregion of ?AREA2 (not a
DependencyOrSpecialSovereigntyArea), having its own associated
GovernmentOrganization which is subordinated to or constrained by
the government of ?AREA2.  Cf. dependentGeopoliticalArea.</rdfs:comment>
<rdf:type rdf:resource = "#AsymmetricRelation"/>
<rdf:type rdf:resource = "#TransitiveRelation"/>
<rdfs:domain rdf:resource="#GeopoliticalArea"/>
<rdfs:range rdf:resource = "#GeopoliticalArea"/>
<rdfs:subPropertyOf rdf:resource="#geographicSubregion"/>
</owl:ObjectProperty>

<owl:ObjectProperty   rdf:ID= "grasps">
<rdfs:comment>The state of grasping an Object.  (grasps
?ANIMAL ?OBJ) means that the Animal ?ANIMAL is intentionally holding
on to the Object ?OBJ.</rdfs:comment>
<rdfs:domain rdf:resource="#Animal"/>
<rdfs:range rdf:resource = "#Object"/>
<rdfs:subPropertyOf rdf:resource="#meetsSpatially"/>
</owl:ObjectProperty>

<owl:DatatypeProperty  rdf:ID= "greaterThan">
<rdfs:comment>(greaterThan ?NUMBER1 ?NUMBER2) is true
just in case the Quantity ?NUMBER1 is greater than the Quantity
?NUMBER2.</rdfs:comment>
<rdf:type rdf:resource = "#BinaryPredicate"/>
<rdf:type rdf:resource = "#TransitiveRelation"/>
<rdf:type rdf:resource = "#IrreflexiveRelation"/>
<rdf:type rdf:resource = "#RelationExtendedToQuantities"/>
<rdfs:domain rdf:resource="#Quantity"/>
<rdfs:range rdf:resource = "#Quantity"/>
<trichotomizingOn rdf:resource = "#RealNumber" />
<inverse rdf:resource = "#lessThan" />
</owl:DatatypeProperty>

<owl:DatatypeProperty  rdf:ID= "greaterThanOrEqualTo">
<rdfs:comment>(greaterThanOrEqualTo ?NUMBER1
?NUMBER2) is true just in case the Quantity ?NUMBER1 is greater
than the Quantity ?NUMBER2.</rdfs:comment>
<rdf:type rdf:resource = "#BinaryPredicate"/>
<rdf:type rdf:resource = "#PartialOrderingRelation"/>
<rdf:type rdf:resource = "#RelationExtendedToQuantities"/>
<rdfs:domain rdf:resource="#Quantity"/>
<rdfs:range rdf:resource = "#Quantity"/>
<trichotomizingOn rdf:resource = "#RealNumber" />
<inverse rdf:resource = "#lessThanOrEqualTo" />
</owl:DatatypeProperty>

<owl:ObjectProperty   rdf:ID= "hasPurpose">
<rdfs:comment>This Predicate expresses the concept of a
conventional goal, i.e. a goal with a neutralized agent's intention.
Accordingly, (hasPurpose ?THING ?FORMULA) means that the instance of
Physical ?THING has, as its purpose, the Proposition expressed by
?FORMULA.  Note that there is an important difference in meaning between
the Predicates hasPurpose and result.  Although the second argument
of the latter can satisfy the second argument of the former,
a conventional goal is an expected and desired outcome, while a result
may be neither expected nor desired.  For example, a machine process may
have outcomes but no goals, aimless wandering may have an outcome but no
goal; a learning process may have goals with no outcomes, and so on.</rdfs:comment>
<rdf:type rdf:resource = "#BinaryPredicate"/>
<rdf:type rdf:resource = "#AsymmetricRelation"/>
<rdfs:domain rdf:resource="#Physical"/>
<rdfs:range rdf:resource = "#Formula"/>
</owl:ObjectProperty>

<owl:ObjectProperty   rdf:ID= "hasSkill">
<rdfs:comment>Similar to the capability Predicate
with the additional restriction that the ability be practised/
demonstrated to some measurable degree.</rdfs:comment>
<rdf:type rdf:resource = "#BinaryPredicate"/>
<rdf:type rdf:resource = "#AsymmetricRelation"/>
<rdfs:domain rdf:resource="#Process"/>
<rdfs:range rdf:resource = "#Agent"/>
</owl:ObjectProperty>

<owl:ObjectProperty   rdf:ID= "height">
<rdfs:comment>The height of an Object is the distance between
its top and its bottom.</rdfs:comment>
<rdfs:domain rdf:resource="#SelfConnectedObject"/>
<rdfs:range rdf:resource = "#LengthMeasure"/>
<rdfs:subPropertyOf rdf:resource="#length"/>
</owl:ObjectProperty>

<owl:ObjectProperty   rdf:ID= "holdsDuring">
<rdfs:comment>(holdsDuring ?TIME ?FORMULA) means that the
proposition denoted by ?FORMULA is true in the time frame ?TIME.  Note
that this implies that ?FORMULA is true at every TimePoint which is a
temporalPart of ?TIME.</rdfs:comment>
<rdf:type rdf:resource = "#BinaryPredicate"/>
<rdf:type rdf:resource = "#AsymmetricRelation"/>
<rdfs:domain rdf:resource="#TimePosition"/>
<rdfs:range rdf:resource = "#Formula"/>
</owl:ObjectProperty>

<owl:ObjectProperty   rdf:ID= "hole">
<rdfs:comment>(hole ?HOLE ?OBJ) means that ?HOLE is a
Hole in ?OBJ.  A Hole is a fillable body located at the
surface an Object.</rdfs:comment>
<rdf:type rdf:resource = "#BinaryPredicate"/>
<rdf:type rdf:resource = "#SpatialRelation"/>
<rdf:type rdf:resource = "#AsymmetricRelation"/>
<rdfs:domain rdf:resource="#Hole"/>
<rdfs:range rdf:resource = "#SelfConnectedObject"/>
</owl:ObjectProperty>

<owl:ObjectProperty   rdf:ID= "home">
<rdfs:comment>The relation between a Human and a PermanentResidence
of the Human.</rdfs:comment>
<rdfs:domain rdf:resource="#Human"/>
<rdfs:range rdf:resource = "#PermanentResidence"/>
<rdfs:subPropertyOf rdf:resource="#inhabits"/>
</owl:ObjectProperty>

<owl:ObjectProperty   rdf:ID= "husband">
<rdfs:comment>(husband ?MAN ?WOMAN) means that ?MAN is the
husband of ?WOMAN.</rdfs:comment>
<rdf:type rdf:resource = "#AsymmetricRelation"/>
<rdf:type rdf:resource = "#IrreflexiveRelation"/>
<rdfs:domain rdf:resource="#Man"/>
<rdfs:range rdf:resource = "#Woman"/>
<rdfs:subPropertyOf rdf:resource="#spouse"/>
<inverse rdf:resource = "#wife" />
</owl:ObjectProperty>

<owl:ObjectProperty   rdf:ID= "identicalListItems">
<rdfs:comment>(identicalListItems ?LIST1 ?LIST2) means that ?LIST1 and ?LIST2 have exactly the same items in their respective lists.  Although ?LIST1 and ?LIST2 are required to share exactly the same items, they may order these items differently.</rdfs:comment>
<rdf:type rdf:resource = "#BinaryPredicate"/>
<rdf:type rdf:resource = "#EquivalenceRelation"/>
<rdfs:domain rdf:resource="#List"/>
<rdfs:range rdf:resource = "#List"/>
</owl:ObjectProperty>

<owl:ObjectProperty   rdf:ID= "identityElement">
<rdfs:comment>An object ?ID is the identity element
for BinaryFunction ?FUNCTION just in case, for every instance ?INST,
applying ?FUNCTION to ?INST and ?ID results in ?INST.</rdfs:comment>
<rdf:type rdf:resource = "#BinaryPredicate"/>
<rdf:type rdf:resource = "#AsymmetricRelation"/>
<rdfs:domain rdf:resource="#BinaryFunction"/>
<rdfs:range rdf:resource = "#Entity"/>
</owl:ObjectProperty>

<owl:ObjectProperty   rdf:ID= "immediateInstance">
<rdfs:comment>An object is an immediateInstance of
a SetOrClass if it is an instance of the SetOrClass and it is not an
instance of a proper subclass of SetOrClass.</rdfs:comment>
<rdf:type rdf:resource = "#AsymmetricRelation"/>
<rdf:type rdf:resource = "#IntransitiveRelation"/>
<rdfs:subPropertyOf rdf:resource="#instance"/>
</owl:ObjectProperty>

<owl:ObjectProperty   rdf:ID= "immediateSubclass">
<rdfs:comment>A SetOrClass ?CLASS1 is an immediateSubclass
of another SetOrClass ?CLASS2 just in case ?CLASS1 is a subclass of ?CLASS2 and
there is no other subclass of ?CLASS2 such that ?CLASS1 is also a subclass of it.</rdfs:comment>
<rdf:type rdf:resource = "#AsymmetricRelation"/>
<rdf:type rdf:resource = "#IntransitiveRelation"/>
<rdfs:subPropertyOf rdf:resource="#subclass"/>
</owl:ObjectProperty>

<owl:ObjectProperty   rdf:ID= "inList">
<rdfs:comment>The analog of element and instance for Lists.
(inList ?OBJ ?LIST) means that ?OBJ is in the List ?LIST.  For example,
(inList Tuesday (ListFn Monday Tuesday Wednesday)) would be true.</rdfs:comment>
<rdf:type rdf:resource = "#BinaryPredicate"/>
<rdf:type rdf:resource = "#IrreflexiveRelation"/>
<rdf:type rdf:resource = "#AsymmetricRelation"/>
<rdfs:domain rdf:resource="#Entity"/>
<rdfs:range rdf:resource = "#List"/>
</owl:ObjectProperty>

<owl:ObjectProperty   rdf:ID= "inScopeOfInterest">
<rdfs:comment>A very general Predicate.
(inScopeOfInterest ?AGENT ?ENTITY) means that ?ENTITY is within the
scope of interest of ?AGENT.  Note that the interest indicated can be
either positive or negative, i.e. the ?AGENT can have an interest in
avoiding or promoting ?ENTITY.</rdfs:comment>
<rdf:type rdf:resource = "#BinaryPredicate"/>
<rdf:type rdf:resource = "#IntentionalRelation"/>
<rdfs:domain rdf:resource="#CognitiveAgent"/>
<rdfs:range rdf:resource = "#Entity"/>
</owl:ObjectProperty>

<owl:ObjectProperty   rdf:ID= "increasesLikelihood">
<rdfs:comment>One of the basic ProbabilityRelations.
(increasesLikelihood ?FORMULA1 ?FORMULA2) means that ?FORMULA2 is more
likely to be true if ?FORMULA1 is true.</rdfs:comment>
<rdf:type rdf:resource = "#ProbabilityRelation"/>
<rdf:type rdf:resource = "#BinaryPredicate"/>
<rdf:type rdf:resource = "#IrreflexiveRelation"/>
<rdfs:domain rdf:resource="#Formula"/>
<rdfs:range rdf:resource = "#Formula"/>
</owl:ObjectProperty>

<owl:ObjectProperty   rdf:ID= "independentProbability">
<rdfs:comment>One of the basic ProbabilityRelations.
(independentProbability ?FORMULA1 ?FORMULA2) means that the probabilities of
?FORMULA1 and ?FORMULA2 being true are independent.</rdfs:comment>
<rdf:type rdf:resource = "#ProbabilityRelation"/>
<rdf:type rdf:resource = "#BinaryPredicate"/>
<rdf:type rdf:resource = "#SymmetricRelation"/>
<rdfs:domain rdf:resource="#Formula"/>
<rdfs:range rdf:resource = "#Formula"/>
</owl:ObjectProperty>

<owl:ObjectProperty   rdf:ID= "inhabits">
<rdfs:comment>A very basic notion of living within something
else.  (inhabits ?ORGANISM ?OBJECT) means that ?OBJECT is the residence
(either permanent or temporary), nest, etc. of ?ORGANISM.</rdfs:comment>
<rdf:type rdf:resource = "#BinaryPredicate"/>
<rdf:type rdf:resource = "#AsymmetricRelation"/>
<rdfs:domain rdf:resource="#Organism"/>
<rdfs:range rdf:resource = "#Object"/>
</owl:ObjectProperty>

<owl:ObjectProperty   rdf:ID= "inhibits">
<rdfs:comment>A very general Predicate.  (inhibits
?PROC1 ?PROC2) means that the Process ?PROC1 inhibits or hinders
the occurrence of the Process ?PROC2.  For example, obstructing an
object inhibits moving it.  Note that this is a relation between types
of Processes, not between instances.</rdfs:comment>
<rdf:type rdf:resource = "#BinaryPredicate"/>
<rdf:type rdf:resource = "#IrreflexiveRelation"/>
<rdfs:domain rdf:resource="#Process"/>
<rdfs:range rdf:resource = "#Process"/>
</owl:ObjectProperty>

<owl:ObjectProperty   rdf:ID= "initialList">
<rdfs:comment>(initialList ?LIST1 ?LIST2) means that ?LIST1
is a subList of ?LIST2 and (ListOrderFn ?LIST1 ?NUMBER) returns the same
value as (ListOrderFn ?LIST2 ?NUMBER) for all of the values of ?NUMBER over
which (ListOrderFn ?LIST1 ?NUMBER) is defined.</rdfs:comment>
<rdf:type rdf:resource = "#BinaryPredicate"/>
<rdf:type rdf:resource = "#PartialOrderingRelation"/>
<rdfs:subPropertyOf rdf:resource="#subList"/>
</owl:ObjectProperty>

<owl:ObjectProperty   rdf:ID= "instance">
<rdfs:comment>An object is an instance of a SetOrClass if
it is included in that SetOrClass.  An individual may be an instance of many
classes, some of which may be subclasses of others.  Thus, there is no
assumption in the meaning of instance about specificity or uniqueness.</rdfs:comment>
<rdf:type rdf:resource = "#BinaryPredicate"/>
<rdfs:domain rdf:resource="#Entity"/>
<rdfs:range rdf:resource = "#SetOrClass"/>
</owl:ObjectProperty>

<owl:ObjectProperty   rdf:ID= "instrument">
<rdfs:comment>(instrument ?EVENT ?TOOL) means that ?TOOL
is used by an agent in bringing about ?EVENT and that ?TOOL is not
changed by ?EVENT.  For example, the key is an instrument in the
following proposition: The key opened the door.  Note that instrument
and resource cannot be satisfied by the same ordered pair.</rdfs:comment>
<rdfs:domain rdf:resource="#Process"/>
<rdfs:range rdf:resource = "#Object"/>
<rdfs:subPropertyOf rdf:resource="#patient"/>
</owl:ObjectProperty>

<owl:ObjectProperty   rdf:ID= "interiorPart">
<rdfs:comment>(interiorPart ?OBJ1 ?OBJ2) means
that ?OBJ1 is part ?OBJ2 and there is no overlap between ?OBJ1 and
any superficialPart ?OBJ2.</rdfs:comment>
<rdf:type rdf:resource = "#AsymmetricRelation"/>
<rdf:type rdf:resource = "#TransitiveRelation"/>
<rdfs:subPropertyOf rdf:resource="#part"/>
</owl:ObjectProperty>

<owl:ObjectProperty   rdf:ID= "inverse">
<rdfs:comment>The inverse of a BinaryRelation is a relation
in which all the tuples of the original relation are reversed.  In
other words, one BinaryRelation is the inverse of another if they are
equivalent when their arguments are swapped.</rdfs:comment>
<rdf:type rdf:resource = "#BinaryPredicate"/>
<rdf:type rdf:resource = "#IrreflexiveRelation"/>
<rdf:type rdf:resource = "#IntransitiveRelation"/>
<rdf:type rdf:resource = "#SymmetricRelation"/>
<rdfs:domain rdf:resource="#BinaryRelation"/>
<rdfs:range rdf:resource = "#BinaryRelation"/>
</owl:ObjectProperty>

<owl:ObjectProperty   rdf:ID= "irreflexiveOn">
<rdfs:comment>A BinaryRelation is irreflexive on a
SetOrClass only if no instance of the SetOrClass bears the relation to
itself.</rdfs:comment>
<rdf:type rdf:resource = "#BinaryPredicate"/>
<rdf:type rdf:resource = "#AsymmetricRelation"/>
<rdfs:domain rdf:resource="#BinaryRelation"/>
<rdfs:range rdf:resource = "#SetOrClass"/>
</owl:ObjectProperty>

<owl:ObjectProperty   rdf:ID= "knows">
<rdfs:comment>The epistemic predicate of knowing.  (knows
?AGENT ?FORMULA) means that ?AGENT knows the proposition expressed by
?FORMULA.  Note that knows entails conscious awareness, so this
Predicate cannot be used to express tacit or subconscious or
unconscious knowledge.</rdfs:comment>
<rdf:type rdf:resource = "#PropositionalAttitude"/>
<rdfs:domain rdf:resource="#CognitiveAgent"/>
<rdfs:range rdf:resource = "#Formula"/>
<rdfs:subPropertyOf rdf:resource="#inScopeOfInterest"/>
</owl:ObjectProperty>

<owl:ObjectProperty   rdf:ID= "larger">
<rdfs:comment>(larger ?OBJ1 ?OBJ2) means that ?OBJ1 is
larger, with respect to all LengthMeasures, than ?OBJ2.</rdfs:comment>
<rdf:type rdf:resource = "#BinaryPredicate"/>
<rdf:type rdf:resource = "#SpatialRelation"/>
<rdf:type rdf:resource = "#TransitiveRelation"/>
<rdf:type rdf:resource = "#IrreflexiveRelation"/>
<rdfs:domain rdf:resource="#Object"/>
<rdfs:range rdf:resource = "#Object"/>
</owl:ObjectProperty>

<owl:ObjectProperty   rdf:ID= "leader">
<rdfs:comment>(leader ?INSTITUTION ?PERSON)
means that the leader of ?INSTITUTION is ?PERSON.</rdfs:comment>
<rdf:type rdf:resource = "#BinaryPredicate"/>
<rdf:type rdf:resource = "#AsymmetricRelation"/>
<rdf:type rdf:resource = "#SingleValuedRelation"/>
<rdfs:domain rdf:resource="#Agent"/>
<rdfs:range rdf:resource = "#Human"/>
</owl:ObjectProperty>

<owl:ObjectProperty   rdf:ID= "legalRelation">
<rdfs:comment>(legalRelation ?AGENT1 ?AGENT2) means
that ?AGENT1 and ?AGENT2 are relatives by virtue of a legal relationship.
Some examples include marriage, adoption, etc.</rdfs:comment>
<rdf:type rdf:resource = "#BinaryPredicate"/>
<rdf:type rdf:resource = "#SymmetricRelation"/>
<rdfs:domain rdf:resource="#CognitiveAgent"/>
<rdfs:range rdf:resource = "#CognitiveAgent"/>
</owl:ObjectProperty>

<owl:ObjectProperty   rdf:ID= "length">
<rdfs:comment>BinaryPredicate that is used to state the measure
of an Object from one point to another point along its surface.  Note
that the difference between the predicates length and distance is that
the length is used to state the LengthMeasure of one of the dimensions of
a single object, while distance is used to state the LengthMeasure that
separates two distinct objects</rdfs:comment>
<rdfs:range rdf:resource = "#LengthMeasure"/>
<rdfs:subPropertyOf rdf:resource="#measure"/>
</owl:ObjectProperty>

<owl:DatatypeProperty  rdf:ID= "lessThan">
<rdfs:comment>(lessThan ?NUMBER1 ?NUMBER2) is true just
in case the Quantity ?NUMBER1 is less than the Quantity ?NUMBER2.</rdfs:comment>
<rdf:type rdf:resource = "#BinaryPredicate"/>
<rdf:type rdf:resource = "#TransitiveRelation"/>
<rdf:type rdf:resource = "#IrreflexiveRelation"/>
<rdf:type rdf:resource = "#RelationExtendedToQuantities"/>
<rdfs:domain rdf:resource="#Quantity"/>
<rdfs:range rdf:resource = "#Quantity"/>
<trichotomizingOn rdf:resource = "#RealNumber" />
</owl:DatatypeProperty>

<owl:DatatypeProperty  rdf:ID= "lessThanOrEqualTo">
<rdfs:comment>(lessThanOrEqualTo ?NUMBER1 ?NUMBER2)
is true just in case the Quantity ?NUMBER1 is less than or equal to
the Quantity ?NUMBER2.</rdfs:comment>
<rdf:type rdf:resource = "#BinaryPredicate"/>
<rdf:type rdf:resource = "#PartialOrderingRelation"/>
<rdf:type rdf:resource = "#RelationExtendedToQuantities"/>
<rdfs:domain rdf:resource="#Quantity"/>
<rdfs:range rdf:resource = "#Quantity"/>
<trichotomizingOn rdf:resource = "#RealNumber" />
</owl:DatatypeProperty>

<owl:ObjectProperty   rdf:ID= "lineMeasure">
<rdfs:comment>(lineMeasure ?LINE ?MEASURE) means that the
straight line ?LINE has the LengthMeasure of ?MEASURE.</rdfs:comment>
<rdf:type rdf:resource = "#BinaryPredicate"/>
<rdf:type rdf:resource = "#TotalValuedRelation"/>
<rdfs:domain rdf:resource="#OneDimensionalFigure"/>
<rdfs:range rdf:resource = "#LengthMeasure"/>
</owl:ObjectProperty>

<owl:ObjectProperty   rdf:ID= "located">
<rdfs:comment>(located ?PHYS ?OBJ) means that ?PHYS is partlyLocated
at ?OBJ, and there is no part or subProcess of ?PHYS that is not located at
?OBJ.</rdfs:comment>
<rdf:type rdf:resource = "#AntisymmetricRelation"/>
<rdf:type rdf:resource = "#TransitiveRelation"/>
<rdfs:subPropertyOf rdf:resource="#partlyLocated"/>
</owl:ObjectProperty>

<owl:ObjectProperty   rdf:ID= "manner">
<rdfs:comment>(manner ?PROCESS ?MANNER) means that the
Process ?PROCESS is qualified by the Attribute ?MANNER.  The Attributes
of Processes are usually denoted by adverbs and include things like the
speed of the wind, the style of a dance, or the intensity of a sports
competition.</rdfs:comment>
<rdf:type rdf:resource = "#AsymmetricRelation"/>
<rdf:type rdf:resource = "#IrreflexiveRelation"/>
<rdfs:domain rdf:resource="#Process"/>
<rdfs:subPropertyOf rdf:resource="#property"/>
<disjointRelation rdf:resource = "#attribute" />
</owl:ObjectProperty>

<owl:ObjectProperty   rdf:ID= "material">
<rdfs:comment>(material ?SUBSTANCE ?OBJECT) means that
?OBJECT is structurally made up in part of ?SUBSTANCE. This relation
encompasses the concepts of 'composed of', 'made of', and 'formed of'.
For example, plastic is a material of my computer monitor.  Compare
part and its subrelations, viz component and piece.</rdfs:comment>
<rdf:type rdf:resource = "#BinaryPredicate"/>
<rdfs:domain rdf:resource="#Substance"/>
<rdfs:range rdf:resource = "#CorpuscularObject"/>
</owl:ObjectProperty>

<owl:ObjectProperty   rdf:ID= "measure">
<rdfs:comment>A very general Predicate for asserting that a
particular Object is measured by a particular ConstantQuantity.
In general, the second argument of this Predicate will be an instance
of the Function MeasureFn.</rdfs:comment>
<rdf:type rdf:resource = "#BinaryPredicate"/>
<rdf:type rdf:resource = "#AsymmetricRelation"/>
<rdfs:domain rdf:resource="#Object"/>
<rdfs:range rdf:resource = "#PhysicalQuantity"/>
</owl:ObjectProperty>

<owl:ObjectProperty   rdf:ID= "meetsSpatially">
<rdfs:comment>(meetsSpatially ?OBJ1 ?OBJ2) means that
?OBJ1 and ?OBJ2 are connected but that neither ?OBJ1 nor ?OBJ2
overlapsSpatially the other.</rdfs:comment>
<rdf:type rdf:resource = "#IrreflexiveRelation"/>
<rdf:type rdf:resource = "#SymmetricRelation"/>
<rdfs:subPropertyOf rdf:resource="#connected"/>
<disjointRelation rdf:resource = "#overlapsSpatially" />
</owl:ObjectProperty>

<owl:ObjectProperty   rdf:ID= "meetsTemporally">
<rdfs:comment>(meetsTemporally ?INTERVAL1 ?INTERVAL2)
means that the terminal point of the TimeInterval ?INTERVAL1 is the
initial point of the TimeInterval ?INTERVAL2.</rdfs:comment>
<rdf:type rdf:resource = "#BinaryPredicate"/>
<rdf:type rdf:resource = "#TemporalRelation"/>
<rdf:type rdf:resource = "#AsymmetricRelation"/>
<rdf:type rdf:resource = "#IntransitiveRelation"/>
<rdfs:domain rdf:resource="#TimeInterval"/>
<rdfs:range rdf:resource = "#TimeInterval"/>
</owl:ObjectProperty>

<owl:ObjectProperty   rdf:ID= "member">
<rdfs:comment>A specialized common sense notion of part for
uniform parts of Collections.  For example, each sheep in a flock of
sheep would have the relationship of member to the flock.</rdfs:comment>
<rdf:type rdf:resource = "#AsymmetricRelation"/>
<rdf:type rdf:resource = "#IntransitiveRelation"/>
<rdfs:domain rdf:resource="#SelfConnectedObject"/>
<rdfs:range rdf:resource = "#Collection"/>
<rdfs:subPropertyOf rdf:resource="#part"/>
<relatedInternalConcept rdf:resource = "#instance" />
<relatedInternalConcept rdf:resource = "#element" />
</owl:ObjectProperty>

<owl:ObjectProperty   rdf:ID= "modalAttribute">
<rdfs:comment>A BinaryRelation that is used to state the
normative force of a Proposition.  (modalAttribute ?FORMULA ?PROP) means
that the Proposition expressed by ?FORMULA has the NormativeAttribute
?PROP.  For example, (modalAttribute (exists (?ACT ?OBJ) (and
(instance ?ACT Giving) (agent ?ACT John) (patient ?ACT ?OBJ)
(destination ?ACT Tom))) Obligation) means that John is obligated to give
Tom something.</rdfs:comment>
<rdf:type rdf:resource = "#BinaryPredicate"/>
<rdf:type rdf:resource = "#AsymmetricRelation"/>
<rdf:type rdf:resource = "#IrreflexiveRelation"/>
<rdfs:domain rdf:resource="#Formula"/>
<rdfs:range rdf:resource = "#NormativeAttribute"/>
<rdfs:subPropertyOf rdf:resource="#property"/>
</owl:ObjectProperty>

<owl:ObjectProperty   rdf:ID= "monetaryValue">
<rdfs:comment>A BinaryPredicate that associates an
Object or Process with its value expressed as an instance of
CurrencyMeasure.</rdfs:comment>
<rdf:type rdf:resource = "#SingleValuedRelation"/>
<rdfs:domain rdf:resource="#Physical"/>
<rdfs:range rdf:resource = "#CurrencyMeasure"/>
<rdfs:subPropertyOf rdf:resource="#measure"/>
</owl:ObjectProperty>

<owl:ObjectProperty   rdf:ID= "mother">
<rdfs:comment>The general relationship of motherhood.
(mother ?CHILD ?MOTHER) means that ?MOTHER is the biological mother
of ?CHILD.</rdfs:comment>
<rdf:type rdf:resource = "#SingleValuedRelation"/>
<rdfs:domain rdf:resource="#Organism"/>
<rdfs:range rdf:resource = "#Organism"/>
<rdfs:subPropertyOf rdf:resource="#parent"/>
</owl:ObjectProperty>

<owl:ObjectProperty   rdf:ID= "names">
<rdfs:comment>(names ?STRING ?ENTITY) means that the thing ?ENTITY
has the SymbolicString ?STRING as its name.  Note that names and represents
are the two immediate subrelations of refers.  The predicate names is used
when the referring item is merely a tag without connotative content, while the
predicate represents is used for referring items that have such content.</rdfs:comment>
<rdfs:domain rdf:resource="#SymbolicString"/>
<rdfs:subPropertyOf rdf:resource="#refers"/>
</owl:ObjectProperty>

<owl:ObjectProperty   rdf:ID= "needs">
<rdfs:comment>(needs ?AGENT ?OBJECT) means that ?OBJECT is
physically required for the continued existence of ?AGENT.</rdfs:comment>
<rdf:type rdf:resource = "#ObjectAttitude"/>
<rdfs:domain rdf:resource="#CognitiveAgent"/>
<rdfs:range rdf:resource = "#Physical"/>
<rdfs:subPropertyOf rdf:resource="#inScopeOfInterest"/>
</owl:ObjectProperty>

<owl:ObjectProperty   rdf:ID= "origin">
<rdfs:comment>(origin ?PROCESS ?SOURCE) means that ?SOURCE
indicates where the ?Process began.  Note that this relation implies
that ?SOURCE is present at the beginning of the process, but need not
participate throughout the process.  For example, the submarine is the
origin in the following proposition: the missile was launched from a
submarine.</rdfs:comment>
<rdf:type rdf:resource = "#CaseRole"/>
<rdfs:domain rdf:resource="#Process"/>
<rdfs:range rdf:resource = "#Object"/>
</owl:ObjectProperty>

<owl:ObjectProperty   rdf:ID= "overlapsPartially">
<rdfs:comment>(overlapsPartially ?OBJ1 ?OBJ2) means
that ?OBJ1 and ?OBJ2 have part(s) in common, but neither ?OBJ1 nor ?OBJ2
is a part of the other.</rdfs:comment>
<rdf:type rdf:resource = "#SymmetricRelation"/>
<rdf:type rdf:resource = "#IrreflexiveRelation"/>
<rdfs:subPropertyOf rdf:resource="#overlapsSpatially"/>
</owl:ObjectProperty>

<owl:ObjectProperty   rdf:ID= "overlapsSpatially">
<rdfs:comment>(overlapsSpatially ?OBJ1 ?OBJ2) means
that the Objects ?OBJ1 and ?OBJ2 have some parts in common.  This is a
reflexive and symmetric (but not transitive) relation.</rdfs:comment>
<rdf:type rdf:resource = "#ReflexiveRelation"/>
<rdf:type rdf:resource = "#SymmetricRelation"/>
<rdfs:subPropertyOf rdf:resource="#connected"/>
</owl:ObjectProperty>

<owl:ObjectProperty   rdf:ID= "overlapsTemporally">
<rdfs:comment>(overlapsTemporally ?INTERVAL1
?INTERVAL2) means that the TimeIntervals ?INTERVAL1 and ?INTERVAL2
have a TimeInterval as a common part.</rdfs:comment>
<rdf:type rdf:resource = "#BinaryPredicate"/>
<rdf:type rdf:resource = "#TemporalRelation"/>
<rdf:type rdf:resource = "#ReflexiveRelation"/>
<rdf:type rdf:resource = "#SymmetricRelation"/>
<rdfs:domain rdf:resource="#TimeInterval"/>
<rdfs:range rdf:resource = "#TimeInterval"/>
</owl:ObjectProperty>

<owl:ObjectProperty   rdf:ID= "parallel">
<rdfs:comment>(parallel ?LINE1 ?LINE2) means that the
OneDimensionalFigures ?LINE1 and ?LINE2 are parallel to one another,
i.e. they are equidistant from one another at every point.</rdfs:comment>
<rdf:type rdf:resource = "#BinaryPredicate"/>
<rdfs:domain rdf:resource="#OneDimensionalFigure"/>
<rdfs:range rdf:resource = "#OneDimensionalFigure"/>
</owl:ObjectProperty>

<owl:ObjectProperty   rdf:ID= "parent">
<rdfs:comment>The general relationship of parenthood.
(parent ?CHILD ?PARENT) means that ?PARENT is a biological parent
of ?CHILD.</rdfs:comment>
<rdf:type rdf:resource = "#BinaryPredicate"/>
<rdf:type rdf:resource = "#AsymmetricRelation"/>
<rdf:type rdf:resource = "#IntransitiveRelation"/>
<rdfs:domain rdf:resource="#Organism"/>
<rdfs:range rdf:resource = "#Organism"/>
<rdfs:subPropertyOf rdf:resource="#familyRelation"/>
</owl:ObjectProperty>

<owl:ObjectProperty   rdf:ID= "part">
<rdfs:comment>The basic mereological relation.  All other
mereological relations are defined in terms of this one.
(part ?PART ?WHOLE) simply means that the Object ?PART is part
of the Object ?WHOLE.  Note that, since part is a
ReflexiveRelation, every Object is a part of itself.</rdfs:comment>
<rdf:type rdf:resource = "#SpatialRelation"/>
<rdf:type rdf:resource = "#PartialOrderingRelation"/>
<rdfs:domain rdf:resource="#Object"/>
<rdfs:range rdf:resource = "#Object"/>
</owl:ObjectProperty>

<owl:ObjectProperty   rdf:ID= "partialOrderingOn">
<rdfs:comment>A BinaryRelation is a partial
ordering on a SetOrClass only if the relation is reflexiveOn the
SetOrClass, and it is both an AntisymmetricRelation, and a
TransitiveRelation.</rdfs:comment>
<rdf:type rdf:resource = "#BinaryPredicate"/>
<rdf:type rdf:resource = "#AsymmetricRelation"/>
<rdfs:domain rdf:resource="#BinaryRelation"/>
<rdfs:range rdf:resource = "#SetOrClass"/>
</owl:ObjectProperty>

<owl:ObjectProperty   rdf:ID= "partiallyFills">
<rdfs:comment>(partiallyFills ?OBJ ?HOLE) means that
?OBJ completelyFills some part of ?HOLE. Note that if (partiallyFills
?OBJ1 ?HOLE) and (part ?OBJ1 ?OBJ2), then (partiallyFills ?OBJ2 ?HOLE).
Note too that a partial filler need not be wholly inside a hole (it may
stick out), which means that every complete filler also qualifies as
(is a limit case of) a partial one.</rdfs:comment>
<rdf:type rdf:resource = "#SpatialRelation"/>
<rdf:type rdf:resource = "#AsymmetricRelation"/>
<rdfs:domain rdf:resource="#Object"/>
<rdfs:range rdf:resource = "#Hole"/>
<rdfs:subPropertyOf rdf:resource="#located"/>
</owl:ObjectProperty>

<owl:ObjectProperty   rdf:ID= "partlyLocated">
<rdfs:comment>(partlyLocated ?THING ?OBJ) means that the
instance of Physical ?THING is at least partially located at ?OBJ.  For
example, Istanbul is partly located in Asia and partly located in Europe.
Note that partlyLocated is the most basic localization relation:  located
is an immediate subrelation of partlyLocated and exactlyLocated is
an immediate subrelation of located.</rdfs:comment>
<rdf:type rdf:resource = "#SpatialRelation"/>
<rdf:type rdf:resource = "#AntisymmetricRelation"/>
<rdf:type rdf:resource = "#BinaryPredicate"/>
<rdfs:domain rdf:resource="#Physical"/>
<rdfs:range rdf:resource = "#Object"/>
</owl:ObjectProperty>

<owl:ObjectProperty   rdf:ID= "path">
<rdfs:comment>(path ?MOTION ?PATH) means that ?PATH is a route
along which ?MOTION occurs.  For example, Highway 101 is the path in the
following proposition:  the car drove up Highway 101.</rdfs:comment>
<rdf:type rdf:resource = "#CaseRole"/>
<rdfs:domain rdf:resource="#Motion"/>
<rdfs:range rdf:resource = "#Object"/>
</owl:ObjectProperty>

<owl:ObjectProperty   rdf:ID= "patient">
<rdfs:comment>(patient ?PROCESS ?ENTITY) means that ?ENTITY
is a participant in ?PROCESS that may be moved, said, experienced, etc.
For example, the direct objects in the sentences 'The cat swallowed the
canary' and 'Billy likes the beer' would be examples of patients.  Note
that the patient of a Process may or may not undergo structural
change as a result of the Process.  The CaseRole of patient is used
when one wants to specify as broadly as possible the object of a
Process.</rdfs:comment>
<rdf:type rdf:resource = "#CaseRole"/>
<rdfs:domain rdf:resource="#Process"/>
<rdfs:range rdf:resource = "#Entity"/>
</owl:ObjectProperty>

<owl:ObjectProperty   rdf:ID= "penetrates">
<rdfs:comment>(penetrates ?OBJ1 ?OBJ2) means that
?OBJ1 is connected to ?OBJ2 along at least one whole dimension (length,
width or depth).</rdfs:comment>
<rdf:type rdf:resource = "#AsymmetricRelation"/>
<rdf:type rdf:resource = "#IntransitiveRelation"/>
<rdfs:subPropertyOf rdf:resource="#traverses"/>
<rdfs:subPropertyOf rdf:resource="#meetsSpatially"/>
</owl:ObjectProperty>

<owl:ObjectProperty   rdf:ID= "piece">
<rdfs:comment>A specialized common sense notion of part for
arbitrary parts of Substances.  Quasi-synonyms are: chunk, hunk, bit,
etc.  Compare component, another subrelation of part.</rdfs:comment>
<rdfs:domain rdf:resource="#Substance"/>
<rdfs:range rdf:resource = "#Substance"/>
<rdfs:subPropertyOf rdf:resource="#part"/>
</owl:ObjectProperty>

<owl:ObjectProperty   rdf:ID= "pointOfFigure">
<rdfs:comment>(pointOfFigure ?POINT ?FIGURE) means that
the GeometricPoint ?POINT is part of the GeometricFigure ?FIGURE.</rdfs:comment>
<rdfs:domain rdf:resource="#GeometricPoint"/>
<rdfs:range rdf:resource = "#GeometricFigure"/>
<rdfs:subPropertyOf rdf:resource="#geometricPart"/>
</owl:ObjectProperty>

<owl:ObjectProperty   rdf:ID= "possesses">
<rdfs:comment>Relation that holds between an Agent and
an Object when the Agent has ownership of the Object.</rdfs:comment>
<rdf:type rdf:resource = "#BinaryPredicate"/>
<rdf:type rdf:resource = "#AsymmetricRelation"/>
<rdfs:domain rdf:resource="#Agent"/>
<rdfs:range rdf:resource = "#Object"/>
</owl:ObjectProperty>

<owl:ObjectProperty   rdf:ID= "precondition">
<rdfs:comment>A very general Predicate.  (precondition
?PROC1 ?PROC2) means that an instance of ?PROC2 can exist only if an
instance of ?PROC1 also exists.</rdfs:comment>
<rdf:type rdf:resource = "#BinaryPredicate"/>
<rdf:type rdf:resource = "#AsymmetricRelation"/>
<rdf:type rdf:resource = "#TransitiveRelation"/>
<rdfs:domain rdf:resource="#Process"/>
<rdfs:range rdf:resource = "#Process"/>
</owl:ObjectProperty>

<owl:ObjectProperty   rdf:ID= "premise">
<rdfs:comment>(premise ?ARGUMENT ?PROPOSITION) means that the
Proposition ?PROPOSITION is an explicit assumption of the Argument
?ARGUMENT.</rdfs:comment>
<rdf:type rdf:resource = "#BinaryPredicate"/>
<rdf:type rdf:resource = "#TotalValuedRelation"/>
<rdfs:domain rdf:resource="#Argument"/>
<rdfs:range rdf:resource = "#Proposition"/>
</owl:ObjectProperty>

<owl:ObjectProperty   rdf:ID= "prevents">
<rdfs:comment>A very general Predicate.  (prevents ?PROC1
?PROC2) means that ?PROC1 prevents the occurrence of ?PROC2.  In other
words, if ?PROC1 is occurring in a particular time and place, ?PROC2
cannot occur at the same time and place.  For example, innoculating
prevents contracting disease.  Note that this is a relation between types
of Processes, not between instances.</rdfs:comment>
<rdf:type rdf:resource = "#BinaryPredicate"/>
<rdf:type rdf:resource = "#IrreflexiveRelation"/>
<rdfs:domain rdf:resource="#Process"/>
<rdfs:range rdf:resource = "#Process"/>
<relatedInternalConcept rdf:resource = "#inhibits" />
</owl:ObjectProperty>

<owl:ObjectProperty   rdf:ID= "properPart">
<rdfs:comment>(properPart ?OBJ1 ?OBJ2) means that
?OBJ1 is a part of ?OBJ2 other than ?OBJ2 itself. This is a
TransitiveRelation and AsymmetricRelation (hence an
IrreflexiveRelation).</rdfs:comment>
<rdf:type rdf:resource = "#AsymmetricRelation"/>
<rdf:type rdf:resource = "#TransitiveRelation"/>
<rdfs:subPropertyOf rdf:resource="#part"/>
</owl:ObjectProperty>

<owl:ObjectProperty   rdf:ID= "properlyFills">
<rdfs:comment>(properlyFills ?OBJ ?HOLE)
means that ?HOLE is properly (though perhaps incompletely) filled by
?OBJ, i.e. some part of ?HOLE is perfectly filled by ?OBJ.  Note that
properlyFills is the dual of completelyFills, and is so
related to partiallyFills that ?OBJ properlyFills ?HOLE just in
case ?OBJ partiallyFills every part of ?HOLE.  (Thus, every perfect
filler is both complete and proper in this sense).</rdfs:comment>
<rdf:type rdf:resource = "#AsymmetricRelation"/>
<rdfs:domain rdf:resource="#Object"/>
<rdfs:range rdf:resource = "#Hole"/>
<rdfs:subPropertyOf rdf:resource="#partiallyFills"/>
</owl:ObjectProperty>

<owl:ObjectProperty   rdf:ID= "property">
<rdfs:comment>This Predicate holds between an instance of
Entity and an instance of Attribute.  (property ?ENTITY ?ATTR)
means that ?ENTITY has the Attribute ?ATTR.</rdfs:comment>
<rdf:type rdf:resource = "#BinaryPredicate"/>
<rdfs:domain rdf:resource="#Entity"/>
<rdfs:range rdf:resource = "#Attribute"/>
</owl:ObjectProperty>

<owl:ObjectProperty   rdf:ID= "publishes">
<rdfs:comment>(publishes ?ORG ?TEXT) means that ?ORG
publishes ?TEXT.  For example, Bantam Books publishes Agatha Christie's
Murder_on_the_Orient_Express.</rdfs:comment>
<rdf:type rdf:resource = "#BinaryPredicate"/>
<rdf:type rdf:resource = "#AsymmetricRelation"/>
<rdfs:domain rdf:resource="#Organization"/>
<rdfs:range rdf:resource = "#Text"/>
</owl:ObjectProperty>

<owl:ObjectProperty   rdf:ID= "range">
<rdfs:comment>Gives the range of a function.  In other words,
(range ?FUNCTION ?CLASS) means that all of the values assigned by
?FUNCTION are instances of ?CLASS.</rdfs:comment>
<rdf:type rdf:resource = "#BinaryPredicate"/>
<rdf:type rdf:resource = "#AsymmetricRelation"/>
<rdfs:domain rdf:resource="#Function"/>
<rdfs:range rdf:resource = "#SetOrClass"/>
</owl:ObjectProperty>

<owl:ObjectProperty   rdf:ID= "rangeSubclass">
<rdfs:comment>(rangeSubclass ?FUNCTION ?CLASS) means that
all of the values assigned by ?FUNCTION are subclasses of ?CLASS.</rdfs:comment>
<rdf:type rdf:resource = "#BinaryPredicate"/>
<rdf:type rdf:resource = "#AsymmetricRelation"/>
<rdfs:domain rdf:resource="#Function"/>
<rdfs:range rdf:resource = "#SetOrClass"/>
</owl:ObjectProperty>

<owl:ObjectProperty   rdf:ID= "realization">
<rdfs:comment>A subrelation of represents.
(realization ?PROCESS ?PROP) means that ?PROCESS is a Process which
expresses the content of ?PROP. Examples include a particular musical
performance, which realizes the content of a musical score, or the
reading of a poem.</rdfs:comment>
<rdf:type rdf:resource = "#AsymmetricRelation"/>
<rdfs:domain rdf:resource="#Process"/>
<rdfs:range rdf:resource = "#Proposition"/>
<rdfs:subPropertyOf rdf:resource="#represents"/>
<relatedInternalConcept rdf:resource = "#equivalentContentInstance" />
<relatedInternalConcept rdf:resource = "#containsInformation" />
</owl:ObjectProperty>

<owl:ObjectProperty   rdf:ID= "refers">
<rdfs:comment>(refers ?OBJ1 ?OBJ2) means that ?OBJ1
mentions or includes a reference to ?OBJ2. Note that refers is
more general in meaning than represents, because presumably something
can represent something else only if it refers to this other thing.
For example, an article whose topic is a recent change in the price of
oil may refer to many other things, e.g. the general state of the economy,
the weather in California, the prospect of global warming, the options
for alternative energy sources, the stock prices of various oil companies,
etc.</rdfs:comment>
<rdf:type rdf:resource = "#BinaryPredicate"/>
<rdfs:domain rdf:resource="#Entity"/>
<rdfs:range rdf:resource = "#Entity"/>
</owl:ObjectProperty>

<owl:ObjectProperty   rdf:ID= "reflexiveOn">
<rdfs:comment>A BinaryRelation is reflexive on a
SetOrClass only if every instance of the SetOrClass bears the relation
to itself.</rdfs:comment>
<rdf:type rdf:resource = "#BinaryPredicate"/>
<rdf:type rdf:resource = "#AsymmetricRelation"/>
<rdfs:domain rdf:resource="#BinaryRelation"/>
<rdfs:range rdf:resource = "#SetOrClass"/>
</owl:ObjectProperty>

<owl:ObjectProperty   rdf:ID= "relatedInternalConcept">
<rdfs:comment>Means that the two arguments are
related concepts within the SUMO, i.e. there is a significant similarity
of meaning between them.  To indicate a meaning relation between a SUMO
concept and a concept from another source, use the Predicate
relatedExternalConcept.</rdfs:comment>
<rdf:type rdf:resource = "#BinaryPredicate"/>
<rdf:type rdf:resource = "#EquivalenceRelation"/>
<rdfs:domain rdf:resource="#Entity"/>
<rdfs:range rdf:resource = "#Entity"/>
</owl:ObjectProperty>

<owl:ObjectProperty   rdf:ID= "represents">
<rdfs:comment>A very general semiotics Predicate.
(represents ?THING ?ENTITY) means that ?THING in some way indicates,
expresses, connotes, pictures, describes, etc. ?ENTITY.  The Predicates
containsInformation and realization are subrelations of represents.
Note that represents is a subrelation of refers, since something can
represent something else only if it refers to this other thing.  See the
documentation string for names.</rdfs:comment>
<rdfs:subPropertyOf rdf:resource="#refers"/>
</owl:ObjectProperty>

<owl:ObjectProperty   rdf:ID= "resource">
<rdfs:comment>(resource ?PROCESS ?RESOURCE) means that
?RESOURCE is present at the beginning of ?PROCESS, is used by ?PROCESS,
and as a consequence is changed by ?PROCESS.  For example, soap is a
resource in the following proposition:  the gun was carved out of soap.
Note that resource differs from instrument, another subrelation of
patient, in that its internal or physical properties are altered in
some way by the Process.</rdfs:comment>
<rdfs:domain rdf:resource="#Process"/>
<rdfs:range rdf:resource = "#Object"/>
<rdfs:subPropertyOf rdf:resource="#patient"/>
</owl:ObjectProperty>

<owl:ObjectProperty   rdf:ID= "result">
<rdfs:comment>(result ?ACTION ?OUTPUT) means that ?OUTPUT is
a product of ?ACTION.  For example, house is a result in the
following proposition: Eric built a house.</rdfs:comment>
<rdfs:domain rdf:resource="#Process"/>
<rdfs:range rdf:resource = "#Entity"/>
<rdfs:subPropertyOf rdf:resource="#patient"/>
</owl:ObjectProperty>

<owl:ObjectProperty   rdf:ID= "sibling">
<rdfs:comment>The relationship between two Organisms that
have the same mother and father.  Note that this relationship does
not hold between half-brothers, half-sisters, etc.</rdfs:comment>
<rdf:type rdf:resource = "#BinaryPredicate"/>
<rdf:type rdf:resource = "#SymmetricRelation"/>
<rdf:type rdf:resource = "#IrreflexiveRelation"/>
<rdfs:domain rdf:resource="#Organism"/>
<rdfs:range rdf:resource = "#Organism"/>
<rdfs:subPropertyOf rdf:resource="#familyRelation"/>
</owl:ObjectProperty>

<owl:ObjectProperty   rdf:ID= "side">
<rdfs:comment>(side ?SIDE ?OBJECT) means that ?SIDE is a side of the object,
as opposed to the top or bottom.</rdfs:comment>
<rdfs:domain rdf:resource="#SelfConnectedObject"/>
<rdfs:range rdf:resource = "#SelfConnectedObject"/>
<rdfs:subPropertyOf rdf:resource="#superficialPart"/>
</owl:ObjectProperty>

<owl:ObjectProperty   rdf:ID= "sister">
<rdfs:comment>The general relationship of being a sister.
(sister ?WOMAN ?PERSON) means that ?WOMAN is the sister of ?PERSON.</rdfs:comment>
<rdf:type rdf:resource = "#IrreflexiveRelation"/>
<rdf:type rdf:resource = "#TransitiveRelation"/>
<rdfs:domain rdf:resource="#Woman"/>
<rdfs:range rdf:resource = "#Human"/>
<rdfs:subPropertyOf rdf:resource="#sibling"/>
</owl:ObjectProperty>

<owl:ObjectProperty   rdf:ID= "smaller">
<rdfs:comment>(smaller ?OBJ1 ?OBJ2) means that ?OBJ1
is smaller, with respect to all LengthMeasures, than ?OBJ2.</rdfs:comment>
<rdf:type rdf:resource = "#BinaryPredicate"/>
<rdf:type rdf:resource = "#SpatialRelation"/>
<rdf:type rdf:resource = "#TransitiveRelation"/>
<rdf:type rdf:resource = "#IrreflexiveRelation"/>
<rdfs:domain rdf:resource="#Object"/>
<rdfs:range rdf:resource = "#Object"/>
<inverse rdf:resource = "#larger" />
</owl:ObjectProperty>

<owl:ObjectProperty   rdf:ID= "son">
<rdfs:comment>The general relationship of being a son.
(son ?CHILD ?PARENT) means that ?CHILD is the biological
son of ?PARENT.</rdfs:comment>
<rdfs:domain rdf:resource="#Man"/>
<rdfs:range rdf:resource = "#Human"/>
<rdfs:subPropertyOf rdf:resource="#parent"/>
</owl:ObjectProperty>

<owl:ObjectProperty   rdf:ID= "spouse">
<rdfs:comment>The relationship of marriage between two Humans.</rdfs:comment>
<rdf:type rdf:resource = "#IrreflexiveRelation"/>
<rdf:type rdf:resource = "#SymmetricRelation"/>
<rdfs:domain rdf:resource="#Human"/>
<rdfs:range rdf:resource = "#Human"/>
<rdfs:subPropertyOf rdf:resource="#legalRelation"/>
</owl:ObjectProperty>

<owl:ObjectProperty   rdf:ID= "starts">
<rdfs:comment>(starts ?INTERVAL1 ?INTERVAL2) means that
?INTERVAL1 and ?INTERVAL2 are both TimeIntervals that have the same
initial TimePoint and that ?INTERVAL1 ends before ?INTERVAL2.</rdfs:comment>
<rdf:type rdf:resource = "#TemporalRelation"/>
<rdf:type rdf:resource = "#TransitiveRelation"/>
<rdf:type rdf:resource = "#IrreflexiveRelation"/>
<rdfs:domain rdf:resource="#TimeInterval"/>
<rdfs:range rdf:resource = "#TimeInterval"/>
<rdfs:subPropertyOf rdf:resource="#temporalPart"/>
</owl:ObjectProperty>

<owl:ObjectProperty   rdf:ID= "stays">
<rdfs:comment>The relation between a Human and a TemporaryResidence
of the Human.</rdfs:comment>
<rdfs:domain rdf:resource="#Human"/>
<rdfs:range rdf:resource = "#TemporaryResidence"/>
<rdfs:subPropertyOf rdf:resource="#inhabits"/>
<disjointRelation rdf:resource = "#home" />
</owl:ObjectProperty>

<owl:ObjectProperty   rdf:ID= "subAttribute">
<rdfs:comment>Means that the second argument can be
ascribed to everything which has the first argument ascribed to it.</rdfs:comment>
<rdf:type rdf:resource = "#BinaryPredicate"/>
<rdf:type rdf:resource = "#PartialOrderingRelation"/>
<rdfs:domain rdf:resource="#Attribute"/>
<rdfs:range rdf:resource = "#Attribute"/>
<disjointRelation rdf:resource = "#successorAttribute" />
</owl:ObjectProperty>

<owl:ObjectProperty   rdf:ID= "subCollection">
<rdfs:comment>(subCollection ?COLL1 ?COLL2) means that
the Collection ?COLL1 is a proper part of the Collection ?COLL2.</rdfs:comment>
<rdf:type rdf:resource = "#BinaryPredicate"/>
<rdf:type rdf:resource = "#PartialOrderingRelation"/>
<rdfs:domain rdf:resource="#Collection"/>
<rdfs:range rdf:resource = "#Collection"/>
</owl:ObjectProperty>

<owl:ObjectProperty   rdf:ID= "subList">
<rdfs:comment>(subList ?LIST1 ?LIST2) means that ?LIST1 is a
sublist of ?LIST2, i.e. every element of ?LIST1 is an element of ?LIST2 and
the elements that are common to both Lists have the same order in both
Lists.</rdfs:comment>
<rdf:type rdf:resource = "#BinaryPredicate"/>
<rdf:type rdf:resource = "#PartialOrderingRelation"/>
<rdfs:domain rdf:resource="#List"/>
<rdfs:range rdf:resource = "#List"/>
</owl:ObjectProperty>

<owl:ObjectProperty   rdf:ID= "subOrganization">
<rdfs:comment>(subOrganization ?ORG1 ?ORG2) means
that ?ORG1 is an Organization which is a part of the Organization
?ORG2.  Note that subOrganization is a ReflexiveRelation, so every
Organization is a subOrganization of itself.</rdfs:comment>
<rdf:type rdf:resource = "#PartialOrderingRelation"/>
<rdfs:domain rdf:resource="#Organization"/>
<rdfs:range rdf:resource = "#Organization"/>
<rdfs:subPropertyOf rdf:resource="#subCollection"/>
</owl:ObjectProperty>

<owl:ObjectProperty   rdf:ID= "subPlan">
<rdfs:comment>(subPlan ?PLAN1 ?PLAN2) means that ?PLAN1
is a Plan which is a proper part of ?PLAN2.  This relation is generally
used to relate a supporting Plan to the overall Plan in a particular
context.</rdfs:comment>
<rdf:type rdf:resource = "#TransitiveRelation"/>
<rdf:type rdf:resource = "#IrreflexiveRelation"/>
<rdfs:domain rdf:resource="#Plan"/>
<rdfs:range rdf:resource = "#Plan"/>
<rdfs:subPropertyOf rdf:resource="#subProposition"/>
</owl:ObjectProperty>

<owl:ObjectProperty   rdf:ID= "subProcess">
<rdfs:comment>(subProcess ?SUBPROC ?PROC) means that ?SUBPROC
is a subprocess of ?PROC.  A subprocess is here understood as a temporally
distinguished part (proper or not) of a Process.</rdfs:comment>
<rdf:type rdf:resource = "#BinaryPredicate"/>
<rdf:type rdf:resource = "#PartialOrderingRelation"/>
<rdfs:domain rdf:resource="#Process"/>
<rdfs:range rdf:resource = "#Process"/>
</owl:ObjectProperty>

<owl:ObjectProperty   rdf:ID= "subProposition">
<rdfs:comment>(subProposition ?PROP1 ?PROP2) means that
?PROP1 is a Proposition which is a proper part of the Proposition ?PROP2.
In other words, subProposition is the analogue of properPart for chunks
of abstract content.</rdfs:comment>
<rdf:type rdf:resource = "#BinaryPredicate"/>
<rdf:type rdf:resource = "#TransitiveRelation"/>
<rdf:type rdf:resource = "#IrreflexiveRelation"/>
<rdfs:domain rdf:resource="#Proposition"/>
<rdfs:range rdf:resource = "#Proposition"/>
</owl:ObjectProperty>

<owl:ObjectProperty   rdf:ID= "subclass">
<rdfs:comment>(subclass ?CLASS1 ?CLASS2) means that ?CLASS1 is
a subclass of ?CLASS2, i.e. every instance of ?CLASS1 is also an instance of
?CLASS2.  A class may have multiple superclasses and subclasses.</rdfs:comment>
<rdf:type rdf:resource = "#BinaryPredicate"/>
<rdf:type rdf:resource = "#PartialOrderingRelation"/>
<rdfs:domain rdf:resource="#SetOrClass"/>
<rdfs:range rdf:resource = "#SetOrClass"/>
</owl:ObjectProperty>

<owl:ObjectProperty   rdf:ID= "subrelation">
<rdfs:comment>(subrelation ?REL1 ?REL2) means that
every tuple of ?REL1 is also a tuple of ?REL2.  In other words, if
the Relation ?REL1 holds for some arguments arg_1, arg_2, ... arg_n,
then the Relation ?REL2 holds for the same arguments.  A consequence
of this is that a Relation and its subrelations must have the same
valence. In CycL, subrelation is called #$genlPreds.</rdfs:comment>
<rdf:type rdf:resource = "#BinaryPredicate"/>
<rdf:type rdf:resource = "#PartialOrderingRelation"/>
<rdfs:domain rdf:resource="#Relation"/>
<rdfs:range rdf:resource = "#Relation"/>
</owl:ObjectProperty>

<owl:ObjectProperty   rdf:ID= "subset">
<rdfs:comment>(subset ?SET1 ?SET2) is true just in case the
elements of the Set ?SET1 are also elements of the Set ?SET2.</rdfs:comment>
<rdfs:domain rdf:resource="#Set"/>
<rdfs:range rdf:resource = "#Set"/>
<rdfs:subPropertyOf rdf:resource="#subclass"/>
</owl:ObjectProperty>

<owl:ObjectProperty   rdf:ID= "subsumesContentClass">
<rdfs:comment>A BinaryPredicate that relates two
subclasses of ContentBearingObject.  (subsumesContentClass ?CLASS1
?CLASS2) means that the content expressed by each instance of ?CLASS2 is
also expressed by each instance of ?CLASS1.  Examples include the
relationship between a poem and one of its stanzas or between a book and
one of its chapters.  Note that this is a relation between subclasses of
ContentBearingObject, rather than instances.  If one wants to relate
instances, the Predicate subsumesContentInstance can be used.  Note
that subsumesContentClass is needed in many cases.  Consider, for
example, the relation between the King James edition of the Bible and its
Book of Genesis.  This relation holds for every copy of this edition and
not just for a single instance.</rdfs:comment>
<rdf:type rdf:resource = "#BinaryPredicate"/>
<rdf:type rdf:resource = "#PartialOrderingRelation"/>
<rdfs:domain rdf:resource="#ContentBearingObject"/>
<rdfs:range rdf:resource = "#ContentBearingObject"/>
</owl:ObjectProperty>

<owl:ObjectProperty   rdf:ID= "subsumesContentInstance">
<rdfs:comment>A BinaryPredicate relating two
instances of ContentBearingObject.  (subsumesContentInstance ?OBJ1 ?OBJ2)
means that the content expressed by ?OBJ2 is part of the content expressed
by ?OBJ1.  An example is the relationship between a handwritten poem and
one of its stanzas.  Note that this is a relation between instances,
rather than Classes.  If one wants to assert a content relationship
between Classes, e.g. between the version of an intellectual work and a
part of that work, the relation subsumesContentClass should be used.</rdfs:comment>
<rdf:type rdf:resource = "#BinaryPredicate"/>
<rdf:type rdf:resource = "#PartialOrderingRelation"/>
<rdfs:domain rdf:resource="#ContentBearingObject"/>
<rdfs:range rdf:resource = "#ContentBearingObject"/>
<relatedInternalConcept rdf:resource = "#subsumesContentClass" />
</owl:ObjectProperty>

<owl:ObjectProperty   rdf:ID= "successorAttribute">
<rdfs:comment>(successorAttribute ?ATTR1 ?ATTR2)
means that ?ATTR2 is the Attribute that comes immediately after ?ATTR1
on the scale that they share.</rdfs:comment>
<rdf:type rdf:resource = "#BinaryPredicate"/>
<rdf:type rdf:resource = "#AsymmetricRelation"/>
<rdfs:domain rdf:resource="#Attribute"/>
<rdfs:range rdf:resource = "#Attribute"/>
</owl:ObjectProperty>

<owl:ObjectProperty   rdf:ID= "successorAttributeClosure">
<rdfs:comment>The transitive closure of
successorAttribute.  (successorAttributeClosure ?ATTR1 ?ATTR2) means
that there is a chain of successorAttribute assertions connecting
?ATTR1 and ?ATTR2.</rdfs:comment>
<rdf:type rdf:resource = "#BinaryPredicate"/>
<rdf:type rdf:resource = "#TransitiveRelation"/>
<rdf:type rdf:resource = "#IrreflexiveRelation"/>
<rdfs:domain rdf:resource="#Attribute"/>
<rdfs:range rdf:resource = "#Attribute"/>
<relatedInternalConcept rdf:resource = "#successorAttribute" />
</owl:ObjectProperty>

<owl:ObjectProperty   rdf:ID= "superficialPart">
<rdfs:comment>(superficialPart ?OBJ1 ?OBJ2)
means that ?OBJ1 is a part of ?OBJ2 that has no interior parts of its own
(or, intuitively, that only overlaps those parts of ?OBJ2 that are
externally connected with the mereological complement of ?OBJ2). This too
is a transitive relation closed under MereologicalSumFn and
MereologicalProductFn.</rdfs:comment>
<rdf:type rdf:resource = "#IrreflexiveRelation"/>
<rdf:type rdf:resource = "#TransitiveRelation"/>
<rdfs:subPropertyOf rdf:resource="#part"/>
</owl:ObjectProperty>

<owl:ObjectProperty   rdf:ID= "surface">
<rdfs:comment>(surface ?OBJ1 ?OBJ2) means that ?OBJ1
is a maximally connected superficialPart of ?OBJ2.  Note that some
SelfConnectedObjects have more than one surface, e.g. a hollow
object like a tennis ball has both an inner and an outer surface.</rdfs:comment>
<rdf:type rdf:resource = "#AsymmetricRelation"/>
<rdfs:domain rdf:resource="#SelfConnectedObject"/>
<rdfs:range rdf:resource = "#SelfConnectedObject"/>
<rdfs:subPropertyOf rdf:resource="#superficialPart"/>
</owl:ObjectProperty>

<owl:ObjectProperty   rdf:ID= "temporalPart">
<rdfs:comment>The temporal analogue of the spatial part predicate.
(temporalPart ?POS1 ?POS2) means that TimePosition ?POS1 is part of TimePosition ?POS2.  Note that since temporalPart is a ReflexiveRelation every TimePostion is a
temporalPart of itself.</rdfs:comment>
<rdf:type rdf:resource = "#BinaryPredicate"/>
<rdf:type rdf:resource = "#TemporalRelation"/>
<rdf:type rdf:resource = "#PartialOrderingRelation"/>
<rdfs:domain rdf:resource="#TimePosition"/>
<rdfs:range rdf:resource = "#TimePosition"/>
</owl:ObjectProperty>

<owl:ObjectProperty   rdf:ID= "time">
<rdfs:comment>This relation holds between an instance of
Physical and an instance of TimePosition just in case the temporal
lifespan of the former includes the latter.  In other words, (time
?THING ?TIME) means that ?THING existed or occurred at ?TIME.  Note
that time does for instances of Physical what holdsDuring does
for instances of Formula.  The constants located and time are
the basic spatial and temporal predicates, respectively.</rdfs:comment>
<rdf:type rdf:resource = "#BinaryPredicate"/>
<rdf:type rdf:resource = "#TemporalRelation"/>
<rdf:type rdf:resource = "#AsymmetricRelation"/>
<rdfs:domain rdf:resource="#Physical"/>
<rdfs:range rdf:resource = "#TimePosition"/>
<relatedInternalConcept rdf:resource = "#located" />
<relatedInternalConcept rdf:resource = "#holdsDuring" />
</owl:ObjectProperty>

<owl:ObjectProperty   rdf:ID= "top">
<rdfs:comment>(top ?TOP ?OBJECT) means that ?TOP is the highest maximal
superficial part of ?OBJECT.</rdfs:comment>
<rdfs:domain rdf:resource="#SelfConnectedObject"/>
<rdfs:range rdf:resource = "#SelfConnectedObject"/>
<rdfs:subPropertyOf rdf:resource="#superficialPart"/>
</owl:ObjectProperty>

<owl:ObjectProperty   rdf:ID= "totalOrderingOn">
<rdfs:comment>A BinaryRelation ?REL is a total
ordering on a SetOrClass only if it is a partial ordering for which either
(?REL ?INST1 ?INST2) or (?REL ?INST2 ?INST1) for every ?INST1 and ?INST2
in the SetOrClass.</rdfs:comment>
<rdf:type rdf:resource = "#BinaryPredicate"/>
<rdf:type rdf:resource = "#AsymmetricRelation"/>
<rdfs:domain rdf:resource="#BinaryRelation"/>
<rdfs:range rdf:resource = "#SetOrClass"/>
</owl:ObjectProperty>

<owl:ObjectProperty   rdf:ID= "transactionAmount">
<rdfs:comment>(transactionAmount ?TRANSACTION
?AMOUNT) means that ?AMOUNT is an instance of CurrencyMeasure being
exhanged in the FinancialTransaction ?TRANSACTION.</rdfs:comment>
<rdf:type rdf:resource = "#BinaryPredicate"/>
<rdf:type rdf:resource = "#SingleValuedRelation"/>
<rdf:type rdf:resource = "#TotalValuedRelation"/>
<rdfs:domain rdf:resource="#FinancialTransaction"/>
<rdfs:range rdf:resource = "#CurrencyMeasure"/>
</owl:ObjectProperty>

<owl:ObjectProperty   rdf:ID= "traverses">
<rdfs:comment>(traverses ?OBJ1 ?OBJ2) means that ?OBJ1
crosses or extends across ?OBJ2.  Note that crosses and
penetrates are subrelations of traverses.</rdfs:comment>
<rdf:type rdf:resource = "#BinaryPredicate"/>
<rdf:type rdf:resource = "#SpatialRelation"/>
<rdfs:domain rdf:resource="#Object"/>
<rdfs:range rdf:resource = "#Object"/>
</owl:ObjectProperty>

<owl:ObjectProperty   rdf:ID= "trichotomizingOn">
<rdfs:comment>A BinaryRelation ?REL is
trichotomizing on a SetOrClass only if, for all instances ?INST1 and ?INST2
of the SetOrClass, at least one of the following holds:  (?REL ?INST1 ?INST2),
(?REL ?INST2 ?INST1) or (equal ?INST1 ?INST2).</rdfs:comment>
<rdf:type rdf:resource = "#BinaryPredicate"/>
<rdf:type rdf:resource = "#AsymmetricRelation"/>
<rdfs:domain rdf:resource="#BinaryRelation"/>
<rdfs:range rdf:resource = "#SetOrClass"/>
</owl:ObjectProperty>

<owl:ObjectProperty   rdf:ID= "true">
<rdfs:comment>The BinaryPredicate that relates a Sentence
to its TruthValue.</rdfs:comment>
<rdfs:domain rdf:resource="#Sentence"/>
<rdfs:range rdf:resource = "#TruthValue"/>
<rdfs:subPropertyOf rdf:resource="#property"/>
</owl:ObjectProperty>

<owl:ObjectProperty   rdf:ID= "uniqueIdentifier">
<rdfs:comment>The class of names that uniquely identify
an instance of Entity.  Some examples of uniqueIdentifiers are the keys
of tables in database applications and the ISBN (International Standard Book
Number).</rdfs:comment>
<rdf:type rdf:resource = "#SingleValuedRelation"/>
<rdfs:subPropertyOf rdf:resource="#names"/>
</owl:ObjectProperty>

<owl:ObjectProperty   rdf:ID= "uses">
<rdfs:comment>(uses ?OBJECT AGENT) means that ?OBJECT is used by
?AGENT as an instrument in an unspecified Process.  This Predicate,
as its corresponding axiom indicates, is a composition of the CaseRoles
agent and instrument.</rdfs:comment>
<rdf:type rdf:resource = "#BinaryPredicate"/>
<rdf:type rdf:resource = "#AsymmetricRelation"/>
<rdfs:domain rdf:resource="#Object"/>
<rdfs:range rdf:resource = "#Agent"/>
</owl:ObjectProperty>

<owl:DatatypeProperty  rdf:ID= "valence">
<rdfs:comment>Specifies the number of arguments that a
relation can take.  If a relation does not have a fixed number of
arguments, it does not have a valence and it is an instance of
VariableArityRelation.  For example, holds is a
VariableArityRelation.</rdfs:comment>
<rdf:type rdf:resource = "#BinaryPredicate"/>
<rdf:type rdf:resource = "#AsymmetricRelation"/>
<rdf:type rdf:resource = "#SingleValuedRelation"/>
<rdfs:domain rdf:resource="#Relation"/>
<rdfs:range rdf:resource = "#PositiveInteger"/>
</owl:DatatypeProperty>

<owl:ObjectProperty   rdf:ID= "version">
<rdfs:comment>Some Artifacts have a life cycle with discrete
stages or versions.  (version ARTIFACT1 ARTIFACT2) means that ARTIFACT1
is a version of ARTIFACT2.  Note that this Predicate relates subclasses of
Artifact and not instances.</rdfs:comment>
<rdf:type rdf:resource = "#BinaryPredicate"/>
<rdf:type rdf:resource = "#AsymmetricRelation"/>
<rdf:type rdf:resource = "#TransitiveRelation"/>
<rdfs:domain rdf:resource="#Artifact"/>
<rdfs:range rdf:resource = "#Artifact"/>
</owl:ObjectProperty>

<owl:ObjectProperty   rdf:ID= "wants">
<rdfs:comment>(wants ?AGENT ?OBJECT) means that ?OBJECT is desired by ?AGENT,
i.e. ?AGENT believes that ?OBJECT will satisfy one of its goals.  Note that there is
no implication that what is wanted by an agent is not already possessed by the agent.</rdfs:comment>
<rdf:type rdf:resource = "#ObjectAttitude"/>
<rdfs:domain rdf:resource="#CognitiveAgent"/>
<rdfs:range rdf:resource = "#Physical"/>
<rdfs:subPropertyOf rdf:resource="#inScopeOfInterest"/>
<relatedInternalConcept rdf:resource = "#desires" />
</owl:ObjectProperty>

<owl:ObjectProperty   rdf:ID= "wears">
<rdfs:comment>(wears ?AGENT ?CLOTHING) means that ?AGENT is wearing
the item of Clothing ?CLOTHING.</rdfs:comment>
<rdf:type rdf:resource = "#BinaryPredicate"/>
<rdfs:domain rdf:resource="#Animal"/>
<rdfs:range rdf:resource = "#Clothing"/>
</owl:ObjectProperty>

<owl:ObjectProperty   rdf:ID= "width">
<rdfs:comment>BinaryPredicate that is used to state the measure
of an Object from side to side at its widest span.</rdfs:comment>
<rdf:type rdf:resource = "#SingleValuedRelation"/>
<rdfs:subPropertyOf rdf:resource="#length"/>
</owl:ObjectProperty>

<owl:ObjectProperty   rdf:ID= "wife">
<rdfs:comment>(wife ?WOMAN ?MAN) means that ?WOMAN is the wife of
?MAN.</rdfs:comment>
<rdf:type rdf:resource = "#AsymmetricRelation"/>
<rdf:type rdf:resource = "#IrreflexiveRelation"/>
<rdfs:domain rdf:resource="#Woman"/>
<rdfs:range rdf:resource = "#Man"/>
<rdfs:subPropertyOf rdf:resource="#spouse"/>
</owl:ObjectProperty>

</rdf:RDF>
